<?xml version="1.0"?>
<rdf:RDF xmlns="http://bigg-project.eu/ontology#"
     xml:base="http://bigg-project.eu/ontology"
     xmlns:dc="http://purl.org/dc/elements/1.1/"
     xmlns:owl="http://www.w3.org/2002/07/owl#"
     xmlns:rdf="http://www.w3.org/1999/02/22-rdf-syntax-ns#"
     xmlns:xml="http://www.w3.org/XML/1998/namespace"
     xmlns:xsd="http://www.w3.org/2001/XMLSchema#"
     xmlns:foaf="http://xmlns.com/foaf/0.1/"
     xmlns:prov="http://www.w3.org/ns/prov#"
     xmlns:rdfs="http://www.w3.org/2000/01/rdf-schema#"
     xmlns:skos="http://www.w3.org/2004/02/skos/core#"
     xmlns:time="http://www.w3.org/2006/time#"
     xmlns:vann="http://purl.org/vocab/vann/"
     xmlns:terms="http://purl.org/dc/terms/"
     xmlns:schema="https://schema.org/"
     xmlns:wgs84_pos="http://www.w3.org/2003/01/geo/wgs84_pos#">
    <owl:Ontology rdf:about="http://bigg-project.eu/ontology#">
        <owl:imports rdf:resource="http://www.w3.org/2006/time#2016"/>
    </owl:Ontology>
    


    <!-- 
    ///////////////////////////////////////////////////////////////////////////////////////
    //
    // Annotation properties
    //
    ///////////////////////////////////////////////////////////////////////////////////////
     -->


    


    <!-- http://purl.org/dc/elements/1.1/date -->


    <owl:AnnotationProperty rdf:about="http://purl.org/dc/elements/1.1/date"/>
    


    <!-- http://purl.org/dc/elements/1.1/description -->


    <owl:AnnotationProperty rdf:about="http://purl.org/dc/elements/1.1/description"/>
    


    <!-- http://purl.org/dc/elements/1.1/title -->


    <owl:AnnotationProperty rdf:about="http://purl.org/dc/elements/1.1/title"/>
    


    <!-- http://purl.org/dc/terms/abstract -->


    <owl:AnnotationProperty rdf:about="http://purl.org/dc/terms/abstract"/>
    


    <!-- http://purl.org/dc/terms/contributor -->


    <owl:AnnotationProperty rdf:about="http://purl.org/dc/terms/contributor"/>
    


    <!-- http://purl.org/dc/terms/created -->


    <owl:AnnotationProperty rdf:about="http://purl.org/dc/terms/created"/>
    


    <!-- http://purl.org/dc/terms/creator -->


    <owl:AnnotationProperty rdf:about="http://purl.org/dc/terms/creator"/>
    


    <!-- http://purl.org/dc/terms/dateCopyrighted -->


    <owl:AnnotationProperty rdf:about="http://purl.org/dc/terms/dateCopyrighted"/>
    


    <!-- http://purl.org/dc/terms/description -->


    <owl:AnnotationProperty rdf:about="http://purl.org/dc/terms/description"/>
    


    <!-- http://purl.org/dc/terms/issued -->


    <owl:AnnotationProperty rdf:about="http://purl.org/dc/terms/issued"/>
    


    <!-- http://purl.org/dc/terms/license -->


    <owl:AnnotationProperty rdf:about="http://purl.org/dc/terms/license"/>
    


    <!-- http://purl.org/dc/terms/modified -->


    <owl:AnnotationProperty rdf:about="http://purl.org/dc/terms/modified"/>
    


    <!-- http://purl.org/dc/terms/publisher -->


    <owl:AnnotationProperty rdf:about="http://purl.org/dc/terms/publisher"/>
    


    <!-- http://purl.org/dc/terms/replaces -->


    <owl:AnnotationProperty rdf:about="http://purl.org/dc/terms/replaces"/>
    


    <!-- http://purl.org/dc/terms/rights -->


    <owl:AnnotationProperty rdf:about="http://purl.org/dc/terms/rights"/>
    


    <!-- http://purl.org/dc/terms/rightsHolder -->


    <owl:AnnotationProperty rdf:about="http://purl.org/dc/terms/rightsHolder"/>
    


    <!-- http://purl.org/dc/terms/source -->


    <owl:AnnotationProperty rdf:about="http://purl.org/dc/terms/source"/>
    


    <!-- http://purl.org/dc/terms/title -->


    <owl:AnnotationProperty rdf:about="http://purl.org/dc/terms/title"/>
    


    <!-- http://purl.org/vocab/vann/preferredNamespacePrefix -->


    <owl:AnnotationProperty rdf:about="http://purl.org/vocab/vann/preferredNamespacePrefix"/>
    


    <!-- http://purl.org/vocab/vann/preferredNamespaceUri -->


    <owl:AnnotationProperty rdf:about="http://purl.org/vocab/vann/preferredNamespaceUri"/>
    


    <!-- http://www.w3.org/2001/XMLSchema#pattern -->


    <owl:AnnotationProperty rdf:about="http://www.w3.org/2001/XMLSchema#pattern"/>
    


    <!-- http://www.w3.org/2003/01/geo/wgs84_pos#alt -->


    <owl:AnnotationProperty rdf:about="http://www.w3.org/2003/01/geo/wgs84_pos#alt"/>
    


    <!-- http://www.w3.org/2003/01/geo/wgs84_pos#lat -->


    <owl:AnnotationProperty rdf:about="http://www.w3.org/2003/01/geo/wgs84_pos#lat"/>
    


    <!-- http://www.w3.org/2003/01/geo/wgs84_pos#location -->


    <owl:AnnotationProperty rdf:about="http://www.w3.org/2003/01/geo/wgs84_pos#location">
        <rdfs:range rdf:resource="http://www.w3.org/2003/01/geo/wgs84_pos#SpatialThing"/>
    </owl:AnnotationProperty>
    


    <!-- http://www.w3.org/2003/01/geo/wgs84_pos#long -->


    <owl:AnnotationProperty rdf:about="http://www.w3.org/2003/01/geo/wgs84_pos#long"/>
    


    <!-- http://www.w3.org/2004/02/skos/core#changeNote -->


    <owl:AnnotationProperty rdf:about="http://www.w3.org/2004/02/skos/core#changeNote"/>
    


    <!-- http://www.w3.org/2004/02/skos/core#definition -->


    <owl:AnnotationProperty rdf:about="http://www.w3.org/2004/02/skos/core#definition"/>
    


    <!-- http://www.w3.org/2004/02/skos/core#editorialNote -->


    <owl:AnnotationProperty rdf:about="http://www.w3.org/2004/02/skos/core#editorialNote"/>
    


    <!-- http://www.w3.org/2004/02/skos/core#example -->


    <owl:AnnotationProperty rdf:about="http://www.w3.org/2004/02/skos/core#example"/>
    


    <!-- http://www.w3.org/2004/02/skos/core#historyNote -->


    <owl:AnnotationProperty rdf:about="http://www.w3.org/2004/02/skos/core#historyNote"/>
    


    <!-- http://www.w3.org/2004/02/skos/core#note -->


    <owl:AnnotationProperty rdf:about="http://www.w3.org/2004/02/skos/core#note"/>
    


    <!-- http://www.w3.org/2004/02/skos/core#prefLabel -->


    <owl:AnnotationProperty rdf:about="http://www.w3.org/2004/02/skos/core#prefLabel"/>
    


    <!-- http://www.w3.org/2004/02/skos/core#scopeNote -->


    <owl:AnnotationProperty rdf:about="http://www.w3.org/2004/02/skos/core#scopeNote"/>
    


    <!-- http://www.w3.org/ns/prov#hadPrimarySource -->


    <owl:AnnotationProperty rdf:about="http://www.w3.org/ns/prov#hadPrimarySource"/>
    


    <!-- http://xmlns.com/foaf/0.1/PersonalProfileDocument -->


    <owl:AnnotationProperty rdf:about="http://xmlns.com/foaf/0.1/PersonalProfileDocument"/>
    


    <!-- http://xmlns.com/foaf/0.1/homepage -->


    <owl:AnnotationProperty rdf:about="http://xmlns.com/foaf/0.1/homepage"/>
    


    <!-- http://xmlns.com/foaf/0.1/name -->


    <owl:AnnotationProperty rdf:about="http://xmlns.com/foaf/0.1/name"/>
    


    <!-- https://schema.org/affiliation -->


    <owl:AnnotationProperty rdf:about="https://schema.org/affiliation"/>
    


    <!-- https://schema.org/email -->


    <owl:AnnotationProperty rdf:about="https://schema.org/email"/>
    


    <!-- https://schema.org/name -->


    <owl:AnnotationProperty rdf:about="https://schema.org/name"/>
    


    <!-- https://schema.org/url -->


    <owl:AnnotationProperty rdf:about="https://schema.org/url"/>
    


    <!-- 
    ///////////////////////////////////////////////////////////////////////////////////////
    //
    // Datatypes
    //
    ///////////////////////////////////////////////////////////////////////////////////////
     -->


    


    <!-- http://www.opengis.net/ont/geosparql#dggsLiteral -->


    <rdfs:Datatype rdf:about="http://www.opengis.net/ont/geosparql#dggsLiteral">
        <rdfs:isDefinedBy rdf:resource="http://www.opengis.net/ont/geosparql#"/>
        <rdfs:isDefinedBy rdf:resource="http://www.opengis.net/spec/geosparql/1.1/req/geometry-extension/dggs-literal"/>
        <rdfs:seeAlso rdf:resource="http://www.opengis.net/doc/AS/dggs/2.0"/>
        <skos:definition xml:lang="en">A textual serialization of a Discrete Global Grid (DGGS) Geometry object.</skos:definition>
        <skos:example rdf:resource="http://www.opengis.net/spec/geosparql/1.1/specification.html#B.1.2.4"/>
        <skos:example> &quot;&lt;https://w3id.org/dggs/auspix&gt; OrdinateList (R3234)&quot;^^&lt;http://www.opengis.net/ont/geosparql#dggsLiteral&gt;</skos:example>
        <skos:prefLabel xml:lang="en">DGGS Literal</skos:prefLabel>
        <skos:scopeNote>This datatype is not expected to be used directly but to serve as an abstract datatype for a series of specific DGGS literal types, for specific DGGS implementations</skos:scopeNote>
    </rdfs:Datatype>
    


    <!-- http://www.opengis.net/ont/geosparql#geoJSONLiteral -->


    <rdfs:Datatype rdf:about="http://www.opengis.net/ont/geosparql#geoJSONLiteral">
        <rdfs:isDefinedBy rdf:resource="http://www.opengis.net/ont/geosparql#"/>
        <rdfs:isDefinedBy rdf:resource="http://www.opengis.net/spec/geosparql/1.1/req/geometry-extension/geojson-literal"/>
        <rdfs:seeAlso rdf:resource="https://tools.ietf.org/html/rfc7946"/>
        <skos:definition xml:lang="en">A GeoJSON serialization of a Geometry object.</skos:definition>
        <skos:example rdf:resource="http://www.opengis.net/spec/geosparql/1.1/specification.html#B.1.2.4"/>
        <skos:prefLabel xml:lang="en">GeoJSON Literal</skos:prefLabel>
    </rdfs:Datatype>
    


    <!-- http://www.opengis.net/ont/geosparql#gmlLiteral -->


    <rdfs:Datatype rdf:about="http://www.opengis.net/ont/geosparql#gmlLiteral">
        <rdfs:isDefinedBy rdf:resource="http://www.opengis.net/ont/geosparql#"/>
        <rdfs:isDefinedBy rdf:resource="http://www.opengis.net/spec/geosparql/1.0/req/geometry-extension/gml-literal"/>
        <rdfs:isDefinedBy rdf:resource="http://www.opengis.net/spec/geosparql/1.1/req/geometry-extension/gml-literal"/>
        <rdfs:seeAlso rdf:resource="https://portal.ogc.org/files/?artifact_id=20509"/>
        <skos:definition xml:lang="en">A GML serialization of a Geometry object.</skos:definition>
        <skos:example rdf:resource="http://www.opengis.net/spec/geosparql/1.1/specification.html#B.1.2.4"/>
        <skos:prefLabel xml:lang="en">GML Literal</skos:prefLabel>
    </rdfs:Datatype>
    


    <!-- http://www.opengis.net/ont/geosparql#kmlLiteral -->


    <rdfs:Datatype rdf:about="http://www.opengis.net/ont/geosparql#kmlLiteral">
        <rdfs:isDefinedBy rdf:resource="http://www.opengis.net/ont/geosparql#"/>
        <rdfs:isDefinedBy rdf:resource="http://www.opengis.net/spec/geosparql/1.1/req/geometry-extension/kml-literal"/>
        <rdfs:seeAlso rdf:resource="https://www.ogc.org/standards/kml/"/>
        <skos:definition xml:lang="en">A KML serialization of a Geometry object.</skos:definition>
        <skos:example rdf:resource="http://www.opengis.net/spec/geosparql/1.1/specification.html#B.1.2.4"/>
        <skos:prefLabel xml:lang="en">KML Literal</skos:prefLabel>
    </rdfs:Datatype>
    


    <!-- http://www.opengis.net/ont/geosparql#wktLiteral -->


    <rdfs:Datatype rdf:about="http://www.opengis.net/ont/geosparql#wktLiteral">
        <rdfs:isDefinedBy rdf:resource="http://www.opengis.net/ont/geosparql#"/>
        <rdfs:isDefinedBy rdf:resource="http://www.opengis.net/spec/geosparql/1.0/req/geometry-extension/wkt-literal"/>
        <rdfs:isDefinedBy rdf:resource="http://www.opengis.net/spec/geosparql/1.1/req/geometry-extension/wkt-literal"/>
        <rdfs:seeAlso rdf:resource="https://portal.ogc.org/files/?artifact_id=25355"/>
        <skos:definition xml:lang="en">A Well-known Text serialization of a Geometry object.</skos:definition>
        <skos:example rdf:resource="http://www.opengis.net/spec/geosparql/1.1/specification.html#B.2.2.2"/>
        <skos:prefLabel xml:lang="en">Well-known Text Literal</skos:prefLabel>
    </rdfs:Datatype>
    


    <!-- http://www.w3.org/2001/XMLSchema#date -->


    <rdfs:Datatype rdf:about="http://www.w3.org/2001/XMLSchema#date"/>
    


    <!-- http://www.w3.org/2001/XMLSchema#dateTimeStamp -->


    <rdf:Description rdf:about="http://www.w3.org/2001/XMLSchema#dateTimeStamp">
        <rdfs:label xml:lang="es">sello de tiempo</rdfs:label>
    </rdf:Description>
    


    <!-- http://www.w3.org/2001/XMLSchema#duration -->


    <rdfs:Datatype rdf:about="http://www.w3.org/2001/XMLSchema#duration"/>
    


    <!-- http://www.w3.org/2001/XMLSchema#gDay -->


    <rdfs:Datatype rdf:about="http://www.w3.org/2001/XMLSchema#gDay"/>
    


    <!-- http://www.w3.org/2001/XMLSchema#gMonth -->


    <rdfs:Datatype rdf:about="http://www.w3.org/2001/XMLSchema#gMonth"/>
    


    <!-- http://www.w3.org/2001/XMLSchema#gYear -->


    <rdfs:Datatype rdf:about="http://www.w3.org/2001/XMLSchema#gYear"/>
    


    <!-- http://www.w3.org/2001/XMLSchema#gYearMonth -->


    <rdfs:Datatype rdf:about="http://www.w3.org/2001/XMLSchema#gYearMonth"/>
    


    <!-- http://www.w3.org/2006/time#generalDay -->


    <rdfs:Datatype rdf:about="http://www.w3.org/2006/time#generalDay">
        <rdfs:comment xml:lang="en">Day of month - formulated as a text string with a pattern constraint to reproduce the same lexical form as gDay, except that values up to 99 are permitted, in order to support calendars with more than 31 days in a month. 
Note that the value-space is not defined, so a generic OWL2 processor cannot compute ordering relationships of values of this type.</rdfs:comment>
        <rdfs:comment xml:lang="es">Día del mes - formulado como una cadena de texto con una restricción patrón para reproducir la misma forma léxica que gDay, excepto que se permiten valores hasta el 99, con el propósito de proporcionar soporte a calendarios con meses con más de 31 días.
            Nótese que el espacio de valores no está definido, por tanto, un procesador genérico de OWL2 no puede computar relaciones de orden de valores de este tipo.</rdfs:comment>
        <rdfs:label xml:lang="es">Día generalizado</rdfs:label>
        <rdfs:label xml:lang="en">Generalized day</rdfs:label>
        <skos:definition xml:lang="en">Day of month - formulated as a text string with a pattern constraint to reproduce the same lexical form as gDay, except that values up to 99 are permitted, in order to support calendars with more than 31 days in a month. 
Note that the value-space is not defined, so a generic OWL2 processor cannot compute ordering relationships of values of this type.</skos:definition>
        <skos:definition xml:lang="es">Día del mes - formulado como una cadena de texto con una restricción patrón para reproducir la misma forma léxica que gDay, excepto que se permiten valores hasta el 99, con el propósito de proporcionar soporte a calendarios con meses con más de 31 días.
            Nótese que el espacio de valores no está definido, por tanto, un procesador genérico de OWL2 no puede computar relaciones de orden de valores de este tipo.</skos:definition>
    </rdfs:Datatype>
    


    <!-- http://www.w3.org/2006/time#generalMonth -->


    <rdfs:Datatype rdf:about="http://www.w3.org/2006/time#generalMonth">
        <rdfs:comment xml:lang="es">Mes del año - formulado como una cadena de texto con una restricción patrón para reproducir la misma forma léxica que gMonth, excepto que se permiten valores hasta el 20, con el propósito de proporcionar soporte a calendarios con años con más de 12 meses.
            Nótese que el espacio de valores no está definido, por tanto, un procesador genérico de OWL2 no puede computar relaciones de orden de valores de este tipo.</rdfs:comment>
        <rdfs:comment xml:lang="en">Month of year - formulated as a text string with a pattern constraint to reproduce the same lexical form as gMonth, except that values up to 20 are permitted, in order to support calendars with more than 12 months in the year. 
Note that the value-space is not defined, so a generic OWL2 processor cannot compute ordering relationships of values of this type.</rdfs:comment>
        <rdfs:label xml:lang="en">Generalized month</rdfs:label>
        <rdfs:label xml:lang="es">Mes generalizado</rdfs:label>
        <skos:definition xml:lang="es">Mes del año - formulado como una cadena de texto con una restricción patrón para reproducir la misma forma léxica que gMonth, excepto que se permiten valores hasta el 20, con el propósito de proporcionar soporte a calendarios con años con más de 12 meses.
            Nótese que el espacio de valores no está definido, por tanto, un procesador genérico de OWL2 no puede computar relaciones de orden de valores de este tipo.</skos:definition>
        <skos:definition xml:lang="en">Month of year - formulated as a text string with a pattern constraint to reproduce the same lexical form as gMonth, except that values up to 20 are permitted, in order to support calendars with more than 12 months in the year. 
Note that the value-space is not defined, so a generic OWL2 processor cannot compute ordering relationships of values of this type.</skos:definition>
    </rdfs:Datatype>
    


    <!-- http://www.w3.org/2006/time#generalYear -->


    <rdfs:Datatype rdf:about="http://www.w3.org/2006/time#generalYear">
        <rdfs:comment xml:lang="es">Número de año - formulado como una cadena de texto con una restricción patrón para reproducir la misma forma léxica que gYear, aunque no está restringido a valores del calendario gregoriano.
            Nótese que el espacio de valores no está definido, por tanto, un procesador genérico de OWL2 no puede computar relaciones de orden de valores de este tipo.</rdfs:comment>
        <rdfs:comment xml:lang="en">Year number - formulated as a text string with a pattern constraint to reproduce the same lexical form as gYear, but not restricted to values from the Gregorian calendar. 
Note that the value-space is not defined, so a generic OWL2 processor cannot compute ordering relationships of values of this type.</rdfs:comment>
        <rdfs:label xml:lang="es">Año generalizado</rdfs:label>
        <rdfs:label xml:lang="en">Generalized year</rdfs:label>
        <skos:definition xml:lang="es">Número de año - formulado como una cadena de texto con una restricción patrón para reproducir la misma forma léxica que gYear, aunque no está restringido a valores del calendario gregoriano.
            Nótese que el espacio de valores no está definido, por tanto, un procesador genérico de OWL2 no puede computar relaciones de orden de valores de este tipo.</skos:definition>
        <skos:definition xml:lang="en">Year number - formulated as a text string with a pattern constraint to reproduce the same lexical form as gYear, but not restricted to values from the Gregorian calendar. 
Note that the value-space is not defined, so a generic OWL2 processor cannot compute ordering relationships of values of this type.</skos:definition>
    </rdfs:Datatype>
    


    <!-- 
    ///////////////////////////////////////////////////////////////////////////////////////
    //
    // Object Properties
    //
    ///////////////////////////////////////////////////////////////////////////////////////
     -->


    


    <!-- http://bigg-project.eu/ontology#manages -->


    <owl:ObjectProperty rdf:about="http://bigg-project.eu/ontology#manages">
        <rdfs:comment xml:lang="en">manages</rdfs:comment>
        <rdfs:label xml:lang="en">manages</rdfs:label>
    </owl:ObjectProperty>
    


    <!-- http://purl.obolibrary.org/obo/TAXRANK_1000000 -->


    <owl:ObjectProperty rdf:about="http://purl.obolibrary.org/obo/TAXRANK_1000000">
        <rdfs:label xml:lang="en">has taxon rank</rdfs:label>
    </owl:ObjectProperty>
    


    <!-- http://schema.org/affiliation -->


    <owl:ObjectProperty rdf:about="http://schema.org/affiliation"/>
    


    <!-- http://www.opengis.net/ont/geosparql#defaultGeometry -->


    <owl:ObjectProperty rdf:about="http://www.opengis.net/ont/geosparql#defaultGeometry">
        <owl:equivalentProperty rdf:resource="http://www.opengis.net/ont/geosparql#hasDefaultGeometry"/>
        <rdfs:subPropertyOf rdf:resource="http://www.opengis.net/ont/geosparql#hasGeometry"/>
        <rdfs:domain rdf:resource="http://www.opengis.net/ont/geosparql#Feature"/>
        <rdfs:range rdf:resource="http://www.opengis.net/ont/geosparql#Geometry"/>
        <rdfs:isDefinedBy rdf:resource="http://www.opengis.net/ont/geosparql#"/>
        <rdfs:isDefinedBy rdf:resource="http://www.opengis.net/spec/geosparql/1.1/req/geometry-extension/feature-properties"/>
        <skos:definition xml:lang="en">The default Geometry to be used in spatial calculations. It is usually the most detailed Geometry.</skos:definition>
        <skos:example rdf:resource="http://www.opengis.net/spec/geosparql/1.1/specification.html#B.1.2.2"/>
        <skos:example rdf:resource="http://www.opengis.net/spec/geosparql/1.1/specification.html#B.2.1"/>
        <skos:note>Duplicate properties defaultGeometry and hasDefaultGeometry exist because of an inconsistency between ontology and documentation in GeoSPARQL 1.0. Only hasDefaultGeometry is described in the documention.</skos:note>
        <skos:prefLabel xml:lang="en">default geometry</skos:prefLabel>
    </owl:ObjectProperty>
    


    <!-- http://www.opengis.net/ont/geosparql#ehContains -->


    <owl:ObjectProperty rdf:about="http://www.opengis.net/ont/geosparql#ehContains">
        <rdfs:domain rdf:resource="http://www.opengis.net/ont/geosparql#SpatialObject"/>
        <rdfs:range rdf:resource="http://www.opengis.net/ont/geosparql#SpatialObject"/>
        <rdfs:isDefinedBy rdf:resource="http://www.opengis.net/ont/geosparql#"/>
        <rdfs:isDefinedBy rdf:resource="http://www.opengis.net/spec/geosparql/1.0/req/geometry-extension/eh-spatial-relations"/>
        <rdfs:isDefinedBy rdf:resource="http://www.opengis.net/spec/geosparql/1.1/req/geometry-extension/eh-spatial-relations"/>
        <rdfs:seeAlso rdf:resource="http://dbpedia.org/resource/DE-9IM"/>
        <skos:definition xml:lang="en">States that the subject SpatialObject spatially contains the object SpatialObject. DE-9IM: T*TFF*FF*</skos:definition>
        <skos:prefLabel xml:lang="en">contains</skos:prefLabel>
    </owl:ObjectProperty>
    


    <!-- http://www.opengis.net/ont/geosparql#ehCoveredBy -->


    <owl:ObjectProperty rdf:about="http://www.opengis.net/ont/geosparql#ehCoveredBy">
        <rdfs:domain rdf:resource="http://www.opengis.net/ont/geosparql#SpatialObject"/>
        <rdfs:range rdf:resource="http://www.opengis.net/ont/geosparql#SpatialObject"/>
        <rdfs:isDefinedBy rdf:resource="http://www.opengis.net/ont/geosparql#"/>
        <rdfs:isDefinedBy rdf:resource="http://www.opengis.net/spec/geosparql/1.0/req/geometry-extension/eh-spatial-relations"/>
        <rdfs:isDefinedBy rdf:resource="http://www.opengis.net/spec/geosparql/1.1/req/geometry-extension/eh-spatial-relations"/>
        <rdfs:seeAlso rdf:resource="http://dbpedia.org/resource/DE-9IM"/>
        <skos:definition xml:lang="en">States that the subject SpatialObject is spatially covered by the object SpatialObject. DE-9IM: TFF*TFT**</skos:definition>
        <skos:prefLabel xml:lang="en">covered by</skos:prefLabel>
    </owl:ObjectProperty>
    


    <!-- http://www.opengis.net/ont/geosparql#ehCovers -->


    <owl:ObjectProperty rdf:about="http://www.opengis.net/ont/geosparql#ehCovers">
        <rdfs:domain rdf:resource="http://www.opengis.net/ont/geosparql#SpatialObject"/>
        <rdfs:range rdf:resource="http://www.opengis.net/ont/geosparql#SpatialObject"/>
        <rdfs:isDefinedBy rdf:resource="http://www.opengis.net/ont/geosparql#"/>
        <rdfs:isDefinedBy rdf:resource="http://www.opengis.net/spec/geosparql/1.0/req/geometry-extension/eh-spatial-relations"/>
        <rdfs:isDefinedBy rdf:resource="http://www.opengis.net/spec/geosparql/1.1/req/geometry-extension/eh-spatial-relations"/>
        <rdfs:seeAlso rdf:resource="http://dbpedia.org/resource/DE-9IM"/>
        <skos:definition xml:lang="en">States that the subject SpatialObject spatially covers the object SpatialObject. DE-9IM: T*TFT*FF*</skos:definition>
        <skos:prefLabel xml:lang="en">covers</skos:prefLabel>
    </owl:ObjectProperty>
    


    <!-- http://www.opengis.net/ont/geosparql#ehDisjoint -->


    <owl:ObjectProperty rdf:about="http://www.opengis.net/ont/geosparql#ehDisjoint">
        <owl:equivalentProperty rdf:resource="http://www.opengis.net/ont/geosparql#sfDisjoint"/>
        <rdfs:domain rdf:resource="http://www.opengis.net/ont/geosparql#SpatialObject"/>
        <rdfs:range rdf:resource="http://www.opengis.net/ont/geosparql#SpatialObject"/>
        <rdfs:isDefinedBy rdf:resource="http://www.opengis.net/ont/geosparql#"/>
        <rdfs:isDefinedBy rdf:resource="http://www.opengis.net/spec/geosparql/1.0/req/geometry-extension/eh-spatial-relations"/>
        <rdfs:isDefinedBy rdf:resource="http://www.opengis.net/spec/geosparql/1.1/req/geometry-extension/eh-spatial-relations"/>
        <rdfs:seeAlso rdf:resource="http://dbpedia.org/resource/DE-9IM"/>
        <skos:definition xml:lang="en">States that the subject SpatialObject is spatially disjoint from the object SpatialObject. DE-9IM: FF*FF****</skos:definition>
        <skos:prefLabel xml:lang="en">disjoint</skos:prefLabel>
    </owl:ObjectProperty>
    


    <!-- http://www.opengis.net/ont/geosparql#ehEquals -->


    <owl:ObjectProperty rdf:about="http://www.opengis.net/ont/geosparql#ehEquals">
        <owl:equivalentProperty rdf:resource="http://www.opengis.net/ont/geosparql#sfEquals"/>
        <rdfs:domain rdf:resource="http://www.opengis.net/ont/geosparql#SpatialObject"/>
        <rdfs:range rdf:resource="http://www.opengis.net/ont/geosparql#SpatialObject"/>
        <rdfs:isDefinedBy rdf:resource="http://www.opengis.net/ont/geosparql#"/>
        <rdfs:isDefinedBy rdf:resource="http://www.opengis.net/spec/geosparql/1.0/req/geometry-extension/eh-spatial-relations"/>
        <rdfs:isDefinedBy rdf:resource="http://www.opengis.net/spec/geosparql/1.1/req/geometry-extension/eh-spatial-relations"/>
        <rdfs:seeAlso rdf:resource="http://dbpedia.org/resource/DE-9IM"/>
        <skos:definition xml:lang="en">States that the subject SpatialObject spatially equals the object SpatialObject. DE-9IM: TFFFTFFFT</skos:definition>
        <skos:prefLabel xml:lang="en">equals</skos:prefLabel>
    </owl:ObjectProperty>
    


    <!-- http://www.opengis.net/ont/geosparql#ehInside -->


    <owl:ObjectProperty rdf:about="http://www.opengis.net/ont/geosparql#ehInside">
        <rdfs:domain rdf:resource="http://www.opengis.net/ont/geosparql#SpatialObject"/>
        <rdfs:range rdf:resource="http://www.opengis.net/ont/geosparql#SpatialObject"/>
        <rdfs:isDefinedBy rdf:resource="http://www.opengis.net/ont/geosparql#"/>
        <rdfs:isDefinedBy rdf:resource="http://www.opengis.net/spec/geosparql/1.0/req/geometry-extension/eh-spatial-relations"/>
        <rdfs:isDefinedBy rdf:resource="http://www.opengis.net/spec/geosparql/1.1/req/geometry-extension/eh-spatial-relations"/>
        <rdfs:seeAlso rdf:resource="http://dbpedia.org/resource/DE-9IM"/>
        <skos:definition xml:lang="en">States that the subject SpatialObject is spatially inside the object SpatialObject. DE-9IM: TFF*FFT**</skos:definition>
        <skos:prefLabel xml:lang="en">inside</skos:prefLabel>
    </owl:ObjectProperty>
    


    <!-- http://www.opengis.net/ont/geosparql#ehMeet -->


    <owl:ObjectProperty rdf:about="http://www.opengis.net/ont/geosparql#ehMeet">
        <owl:equivalentProperty rdf:resource="http://www.opengis.net/ont/geosparql#sfTouches"/>
        <rdfs:domain rdf:resource="http://www.opengis.net/ont/geosparql#SpatialObject"/>
        <rdfs:range rdf:resource="http://www.opengis.net/ont/geosparql#SpatialObject"/>
        <rdfs:isDefinedBy rdf:resource="http://www.opengis.net/ont/geosparql#"/>
        <rdfs:isDefinedBy rdf:resource="http://www.opengis.net/spec/geosparql/1.0/req/geometry-extension/eh-spatial-relations"/>
        <rdfs:isDefinedBy rdf:resource="http://www.opengis.net/spec/geosparql/1.1/req/geometry-extension/eh-spatial-relations"/>
        <rdfs:seeAlso rdf:resource="http://dbpedia.org/resource/DE-9IM"/>
        <skos:definition xml:lang="en">States that the subject SpatialObject spatially meets the object SpatialObject. DE-9IM: FT******* ^ F**T***** ^ F***T****</skos:definition>
        <skos:prefLabel xml:lang="en">meet</skos:prefLabel>
    </owl:ObjectProperty>
    


    <!-- http://www.opengis.net/ont/geosparql#ehOverlap -->


    <owl:ObjectProperty rdf:about="http://www.opengis.net/ont/geosparql#ehOverlap">
        <rdfs:domain rdf:resource="http://www.opengis.net/ont/geosparql#SpatialObject"/>
        <rdfs:range rdf:resource="http://www.opengis.net/ont/geosparql#SpatialObject"/>
        <rdfs:isDefinedBy rdf:resource="http://www.opengis.net/ont/geosparql#"/>
        <rdfs:isDefinedBy rdf:resource="http://www.opengis.net/spec/geosparql/1.0/req/geometry-extension/eh-spatial-relations"/>
        <rdfs:isDefinedBy rdf:resource="http://www.opengis.net/spec/geosparql/1.1/req/geometry-extension/eh-spatial-relations"/>
        <rdfs:seeAlso rdf:resource="http://dbpedia.org/resource/DE-9IM"/>
        <skos:definition xml:lang="en">States that the subject SpatialObject spatially overlaps the object SpatialObject. DE-9IM: T*T***T**</skos:definition>
        <skos:prefLabel xml:lang="en">overlap</skos:prefLabel>
    </owl:ObjectProperty>
    


    <!-- http://www.opengis.net/ont/geosparql#hasArea -->


    <owl:ObjectProperty rdf:about="http://www.opengis.net/ont/geosparql#hasArea">
        <rdfs:subPropertyOf rdf:resource="http://www.opengis.net/ont/geosparql#hasSize"/>
        <rdfs:domain rdf:resource="http://www.opengis.net/ont/geosparql#SpatialObject"/>
        <rdfs:isDefinedBy rdf:resource="http://www.opengis.net/ont/geosparql#"/>
        <rdfs:isDefinedBy rdf:resource="http://www.opengis.net/spec/geosparql/1.1/req/geometry-extension/spatial-object-properties"/>
        <skos:definition xml:lang="en">The area of a Spatial Object.</skos:definition>
        <skos:example rdf:resource="http://www.opengis.net/spec/geosparql/1.1/specification.html#B.1.1.2.4"/>
        <skos:example rdf:resource="http://www.opengis.net/spec/geosparql/1.1/specification.html#B.1.2.2"/>
        <skos:prefLabel xml:lang="en">has area</skos:prefLabel>
    </owl:ObjectProperty>
    


    <!-- http://www.opengis.net/ont/geosparql#hasBoundingBox -->


    <owl:ObjectProperty rdf:about="http://www.opengis.net/ont/geosparql#hasBoundingBox">
        <rdfs:subPropertyOf rdf:resource="http://www.opengis.net/ont/geosparql#hasGeometry"/>
        <rdfs:domain rdf:resource="http://www.opengis.net/ont/geosparql#Feature"/>
        <rdfs:range rdf:resource="http://www.opengis.net/ont/geosparql#Geometry"/>
        <rdfs:isDefinedBy rdf:resource="http://www.opengis.net/ont/geosparql#"/>
        <rdfs:isDefinedBy rdf:resource="http://www.opengis.net/spec/geosparql/1.1/req/geometry-extension/feature-properties"/>
        <skos:definition xml:lang="en">The minimum or smallest bounding or enclosing box of a given Feature.</skos:definition>
        <skos:example rdf:resource="http://www.opengis.net/spec/geosparql/1.1/specification.html#B.1.2.2"/>
        <skos:prefLabel xml:lang="en">has bounding box</skos:prefLabel>
        <skos:scopeNote xml:lang="en">The target is a Geometry that defines a rectilinear region whose edges are aligned with the axes of the coordinate reference system, which exactly contains the Feature, for example an instance of http://www.opengis.net/ont/sf#envelope.</skos:scopeNote>
    </owl:ObjectProperty>
    


    <!-- http://www.opengis.net/ont/geosparql#hasCentroid -->


    <owl:ObjectProperty rdf:about="http://www.opengis.net/ont/geosparql#hasCentroid">
        <rdfs:subPropertyOf rdf:resource="http://www.opengis.net/ont/geosparql#hasGeometry"/>
        <rdfs:domain rdf:resource="http://www.opengis.net/ont/geosparql#Feature"/>
        <rdfs:range rdf:resource="http://www.opengis.net/ont/geosparql#Geometry"/>
        <rdfs:isDefinedBy rdf:resource="http://www.opengis.net/ont/geosparql#"/>
        <rdfs:isDefinedBy rdf:resource="http://www.opengis.net/spec/geosparql/1.1/req/geometry-extension/feature-properties"/>
        <skos:definition xml:lang="en">The arithmetic mean position of all the Geometry points of a given Feature.</skos:definition>
        <skos:example rdf:resource="http://www.opengis.net/spec/geosparql/1.1/specification.html#B.1.2.2"/>
        <skos:prefLabel xml:lang="en">has centroid</skos:prefLabel>
        <skos:scopeNote xml:lang="en">The target Geometry shall describe a point, for example an instance of http://www.opengis.net/ont/sf#Point.</skos:scopeNote>
    </owl:ObjectProperty>
    


    <!-- http://www.opengis.net/ont/geosparql#hasDefaultGeometry -->


    <owl:ObjectProperty rdf:about="http://www.opengis.net/ont/geosparql#hasDefaultGeometry">
        <rdfs:subPropertyOf rdf:resource="http://www.opengis.net/ont/geosparql#hasGeometry"/>
        <rdfs:domain rdf:resource="http://www.opengis.net/ont/geosparql#Feature"/>
        <rdfs:range rdf:resource="http://www.opengis.net/ont/geosparql#Geometry"/>
        <rdfs:isDefinedBy rdf:resource="http://www.opengis.net/ont/geosparql#"/>
        <rdfs:isDefinedBy rdf:resource="http://www.opengis.net/spec/geosparql/1.0/req/geometry-extension/feature-properties"/>
        <rdfs:isDefinedBy rdf:resource="http://www.opengis.net/spec/geosparql/1.1/req/geometry-extension/feature-properties"/>
        <skos:definition xml:lang="en">The default Geometry to be used in spatial calculations. It is usually the most detailed Geometry.</skos:definition>
        <skos:note>Duplicate properties defaultGeometry and hasDefaultGeometry exist because of an inconsistency between ontology and documentation in GeoSPARQL 1.0. Only hasDefaultGeometry is described in the documention.</skos:note>
        <skos:prefLabel xml:lang="en">has default geometry</skos:prefLabel>
    </owl:ObjectProperty>
    


    <!-- http://www.opengis.net/ont/geosparql#hasGeometry -->


    <owl:ObjectProperty rdf:about="http://www.opengis.net/ont/geosparql#hasGeometry">
        <rdfs:domain rdf:resource="http://www.opengis.net/ont/geosparql#Feature"/>
        <rdfs:range rdf:resource="http://www.opengis.net/ont/geosparql#Geometry"/>
        <rdfs:comment xml:lang="en">A spatial representation for a given feature.</rdfs:comment>
        <rdfs:isDefinedBy rdf:resource="http://www.opengis.net/ont/geosparql#"/>
        <rdfs:isDefinedBy rdf:resource="http://www.opengis.net/spec/geosparql/1.0/req/geometry-extension/feature-properties"/>
        <rdfs:isDefinedBy rdf:resource="http://www.opengis.net/spec/geosparql/1.1/req/geometry-extension/feature-properties"/>
        <rdfs:label xml:lang="en">has geometry</rdfs:label>
        <rdfs:label xml:lang="en">hasGeometry</rdfs:label>
        <skos:definition xml:lang="en">A spatial representation for a given Feature.</skos:definition>
        <skos:example rdf:resource="http://www.opengis.net/spec/geosparql/1.1/specification.html#B.1.1.2.2"/>
        <skos:example rdf:resource="http://www.opengis.net/spec/geosparql/1.1/specification.html#B.1.1.2.3"/>
        <skos:example rdf:resource="http://www.opengis.net/spec/geosparql/1.1/specification.html#B.1.1.2.4"/>
        <skos:example rdf:resource="http://www.opengis.net/spec/geosparql/1.1/specification.html#B.1.1.2.5"/>
        <skos:example rdf:resource="http://www.opengis.net/spec/geosparql/1.1/specification.html#B.1.1.2.6"/>
        <skos:example rdf:resource="http://www.opengis.net/spec/geosparql/1.1/specification.html#B.1.1.2.8"/>
        <skos:example rdf:resource="http://www.opengis.net/spec/geosparql/1.1/specification.html#B.1.1.3.2"/>
        <skos:example rdf:resource="http://www.opengis.net/spec/geosparql/1.1/specification.html#B.1.1.3.3"/>
        <skos:example rdf:resource="http://www.opengis.net/spec/geosparql/1.1/specification.html#B.1.2.2"/>
        <skos:example rdf:resource="http://www.opengis.net/spec/geosparql/1.1/specification.html#B.1.2.3"/>
        <skos:example rdf:resource="http://www.opengis.net/spec/geosparql/1.1/specification.html#B.1.2.4"/>
        <skos:example rdf:resource="http://www.opengis.net/spec/geosparql/1.1/specification.html#B.2"/>
        <skos:prefLabel xml:lang="en">has geometry</skos:prefLabel>
    </owl:ObjectProperty>
    


    <!-- http://www.opengis.net/ont/geosparql#hasLength -->


    <owl:ObjectProperty rdf:about="http://www.opengis.net/ont/geosparql#hasLength">
        <rdfs:subPropertyOf rdf:resource="http://www.opengis.net/ont/geosparql#hasSize"/>
        <rdfs:domain rdf:resource="http://www.opengis.net/ont/geosparql#SpatialObject"/>
        <rdfs:isDefinedBy rdf:resource="http://www.opengis.net/ont/geosparql#"/>
        <rdfs:isDefinedBy rdf:resource="http://www.opengis.net/spec/geosparql/1.1/req/geometry-extension/spatial-object-properties"/>
        <skos:definition xml:lang="en">The length of a Spatial Object.</skos:definition>
        <skos:example rdf:resource="http://www.opengis.net/spec/geosparql/1.1/specification.html#B.1.1.2.7"/>
        <skos:example rdf:resource="http://www.opengis.net/spec/geosparql/1.1/specification.html#B.1.2.2"/>
        <skos:prefLabel xml:lang="en">has length</skos:prefLabel>
    </owl:ObjectProperty>
    


    <!-- http://www.opengis.net/ont/geosparql#hasPerimeterLength -->


    <owl:ObjectProperty rdf:about="http://www.opengis.net/ont/geosparql#hasPerimeterLength">
        <rdfs:subPropertyOf rdf:resource="http://www.opengis.net/ont/geosparql#hasSize"/>
        <rdfs:domain rdf:resource="http://www.opengis.net/ont/geosparql#SpatialObject"/>
        <rdfs:isDefinedBy rdf:resource="http://www.opengis.net/ont/geosparql#"/>
        <rdfs:isDefinedBy rdf:resource="http://www.opengis.net/spec/geosparql/1.1/req/geometry-extension/spatial-object-properties"/>
        <skos:definition xml:lang="en">The length of the perimeter of a Spatial Object.</skos:definition>
        <skos:example rdf:resource="http://www.opengis.net/spec/geosparql/1.1/specification.html#B.1.1.1.2"/>
        <skos:prefLabel xml:lang="en">has perimeter length</skos:prefLabel>
    </owl:ObjectProperty>
    


    <!-- http://www.opengis.net/ont/geosparql#hasSize -->


    <owl:ObjectProperty rdf:about="http://www.opengis.net/ont/geosparql#hasSize">
        <rdfs:domain rdf:resource="http://www.opengis.net/ont/geosparql#SpatialObject"/>
        <rdfs:isDefinedBy rdf:resource="http://www.opengis.net/ont/geosparql#"/>
        <rdfs:isDefinedBy rdf:resource="http://www.opengis.net/spec/geosparql/1.0/req/topology-vocab-extension/spatial-object-properties"/>
        <rdfs:isDefinedBy rdf:resource="http://www.opengis.net/spec/geosparql/1.1/req/topology-vocab-extension/spatial-object-properties"/>
        <skos:definition xml:lang="en">Subproperties of this property are used to indicate the size of a Spatial Object as a measurement or estimate of one or more dimensions of the Spatial Object&apos;s spatial presence.</skos:definition>
        <skos:note xml:lang="en">The recommended way to specify size is by using a subproperty of hasMetricSize. Subproperties of hasSize can be used if more complex expressions are necessary, for example if the unit of length can not be converted to meter, or if additional data are needed to describe the measurement or estimate.</skos:note>
        <skos:prefLabel xml:lang="en">has size</skos:prefLabel>
    </owl:ObjectProperty>
    


    <!-- http://www.opengis.net/ont/geosparql#hasSpatialAccuracy -->


    <owl:ObjectProperty rdf:about="http://www.opengis.net/ont/geosparql#hasSpatialAccuracy">
        <rdfs:domain rdf:resource="http://www.opengis.net/ont/geosparql#Geometry"/>
        <rdfs:isDefinedBy rdf:resource="http://www.opengis.net/ont/geosparql#"/>
        <rdfs:isDefinedBy rdf:resource="http://www.opengis.net/spec/geosparql/1.1/req/geometry-extension/geometry-properties"/>
        <skos:definition xml:lang="en">The positional accuracy of the coordinates of a Geometry.</skos:definition>
        <skos:example rdf:resource="http://www.opengis.net/spec/geosparql/1.1/specification.html#B.1.2.3"/>
        <skos:note xml:lang="en">Spatial accuracy is applicable when a Geometry is used to represent a Feature. It is expressed as a distance that indicates the truthfullness of the positions (coordinates) that define the Geometry. In this case accuracy defines a zone surrounding each coordinate within wich the real positions are known to be. The accuracy value defines this zone as a distance from the coordinate(s) in all directions (e.g. a line, a circle or a sphere, depending on spatial dimension).</skos:note>
        <skos:prefLabel xml:lang="en">has spatial accuracy</skos:prefLabel>
    </owl:ObjectProperty>
    


    <!-- http://www.opengis.net/ont/geosparql#hasSpatialResolution -->


    <owl:ObjectProperty rdf:about="http://www.opengis.net/ont/geosparql#hasSpatialResolution">
        <rdfs:domain rdf:resource="http://www.opengis.net/ont/geosparql#Geometry"/>
        <rdfs:isDefinedBy rdf:resource="http://www.opengis.net/ont/geosparql#"/>
        <rdfs:isDefinedBy rdf:resource="http://www.opengis.net/spec/geosparql/1.1/req/geometry-extension/feature-properties"/>
        <skos:definition xml:lang="en">The spatial resolution of a Geometry.</skos:definition>
        <skos:example rdf:resource="http://www.opengis.net/spec/geosparql/1.1/specification.html#B.1.2.2"/>
        <skos:note xml:lang="en">Spatial resolution specifies the level of detail of a Geometry. It the smallest distinguishable distance between spatially adjacent coordinates.</skos:note>
        <skos:prefLabel xml:lang="en">has spatial resolution</skos:prefLabel>
    </owl:ObjectProperty>
    


    <!-- http://www.opengis.net/ont/geosparql#hasVolume -->


    <owl:ObjectProperty rdf:about="http://www.opengis.net/ont/geosparql#hasVolume">
        <rdfs:subPropertyOf rdf:resource="http://www.opengis.net/ont/geosparql#hasSize"/>
        <rdfs:domain rdf:resource="http://www.opengis.net/ont/geosparql#SpatialObject"/>
        <rdfs:isDefinedBy rdf:resource="http://www.opengis.net/ont/geosparql#"/>
        <rdfs:isDefinedBy rdf:resource="http://www.opengis.net/spec/geosparql/1.1/req/geometry-extension/spatial-object-properties"/>
        <skos:definition xml:lang="en">The volume of a three-dimensional Spatial Object.</skos:definition>
        <skos:example rdf:resource="http://www.opengis.net/spec/geosparql/1.1/specification.html#B.1.2.2"/>
        <skos:prefLabel xml:lang="en">has volume</skos:prefLabel>
    </owl:ObjectProperty>
    


    <!-- http://www.opengis.net/ont/geosparql#rcc8dc -->


    <owl:ObjectProperty rdf:about="http://www.opengis.net/ont/geosparql#rcc8dc">
        <rdfs:domain rdf:resource="http://www.opengis.net/ont/geosparql#SpatialObject"/>
        <rdfs:range rdf:resource="http://www.opengis.net/ont/geosparql#SpatialObject"/>
        <rdfs:isDefinedBy rdf:resource="http://www.opengis.net/ont/geosparql#"/>
        <rdfs:isDefinedBy rdf:resource="http://www.opengis.net/spec/geosparql/1.0/req/topology-vocab-extension/rcc8-spatial-relations"/>
        <rdfs:isDefinedBy rdf:resource="http://www.opengis.net/spec/geosparql/1.1/req/topology-vocab-extension/rcc8-spatial-relations"/>
        <rdfs:seeAlso rdf:resource="http://dbpedia.org/resource/DE-9IM"/>
        <skos:definition xml:lang="en">States that the subject SpatialObject is spatially disjoint from the object SpatialObject. DE-9IM: FFTFFTTTT</skos:definition>
        <skos:prefLabel xml:lang="en">disconnected</skos:prefLabel>
    </owl:ObjectProperty>
    


    <!-- http://www.opengis.net/ont/geosparql#rcc8ec -->


    <owl:ObjectProperty rdf:about="http://www.opengis.net/ont/geosparql#rcc8ec">
        <rdfs:domain rdf:resource="http://www.opengis.net/ont/geosparql#SpatialObject"/>
        <rdfs:range rdf:resource="http://www.opengis.net/ont/geosparql#SpatialObject"/>
        <rdfs:isDefinedBy rdf:resource="http://www.opengis.net/ont/geosparql#"/>
        <rdfs:isDefinedBy rdf:resource="http://www.opengis.net/spec/geosparql/1.0/req/topology-vocab-extension/rcc8-spatial-relations"/>
        <rdfs:isDefinedBy rdf:resource="http://www.opengis.net/spec/geosparql/1.1/req/topology-vocab-extension/rcc8-spatial-relations"/>
        <rdfs:seeAlso rdf:resource="http://dbpedia.org/resource/DE-9IM"/>
        <skos:definition xml:lang="en">States that the subject SpatialObject spatially meets the object SpatialObject. DE-9IM: FFTFTTTTT</skos:definition>
        <skos:prefLabel xml:lang="en">externally connected</skos:prefLabel>
    </owl:ObjectProperty>
    


    <!-- http://www.opengis.net/ont/geosparql#rcc8eq -->


    <owl:ObjectProperty rdf:about="http://www.opengis.net/ont/geosparql#rcc8eq">
        <rdfs:domain rdf:resource="http://www.opengis.net/ont/geosparql#SpatialObject"/>
        <rdfs:range rdf:resource="http://www.opengis.net/ont/geosparql#SpatialObject"/>
        <rdfs:isDefinedBy rdf:resource="http://www.opengis.net/ont/geosparql#"/>
        <rdfs:isDefinedBy rdf:resource="http://www.opengis.net/spec/geosparql/1.0/req/topology-vocab-extension/rcc8-spatial-relations"/>
        <rdfs:isDefinedBy rdf:resource="http://www.opengis.net/spec/geosparql/1.1/req/topology-vocab-extension/rcc8-spatial-relations"/>
        <rdfs:seeAlso rdf:resource="http://dbpedia.org/resource/DE-9IM"/>
        <skos:definition xml:lang="en">States that the subject SpatialObject spatially equals the object SpatialObject. DE-9IM: TFFFTFFFT</skos:definition>
        <skos:prefLabel xml:lang="en">equals</skos:prefLabel>
    </owl:ObjectProperty>
    


    <!-- http://www.opengis.net/ont/geosparql#rcc8ntpp -->


    <owl:ObjectProperty rdf:about="http://www.opengis.net/ont/geosparql#rcc8ntpp">
        <rdfs:domain rdf:resource="http://www.opengis.net/ont/geosparql#SpatialObject"/>
        <rdfs:range rdf:resource="http://www.opengis.net/ont/geosparql#SpatialObject"/>
        <rdfs:isDefinedBy rdf:resource="http://www.opengis.net/ont/geosparql#"/>
        <rdfs:isDefinedBy rdf:resource="http://www.opengis.net/spec/geosparql/1.0/req/topology-vocab-extension/rcc8-spatial-relations"/>
        <rdfs:isDefinedBy rdf:resource="http://www.opengis.net/spec/geosparql/1.1/req/topology-vocab-extension/rcc8-spatial-relations"/>
        <rdfs:seeAlso rdf:resource="http://dbpedia.org/resource/DE-9IM"/>
        <skos:definition xml:lang="en">States that the subject SpatialObject is spatially inside the object SpatialObject. DE-9IM: TFFTFFTTT</skos:definition>
        <skos:prefLabel xml:lang="en">non-tangential proper part</skos:prefLabel>
    </owl:ObjectProperty>
    


    <!-- http://www.opengis.net/ont/geosparql#rcc8ntppi -->


    <owl:ObjectProperty rdf:about="http://www.opengis.net/ont/geosparql#rcc8ntppi">
        <rdfs:domain rdf:resource="http://www.opengis.net/ont/geosparql#SpatialObject"/>
        <rdfs:range rdf:resource="http://www.opengis.net/ont/geosparql#SpatialObject"/>
        <rdfs:isDefinedBy rdf:resource="http://www.opengis.net/ont/geosparql#"/>
        <rdfs:isDefinedBy rdf:resource="http://www.opengis.net/spec/geosparql/1.0/req/topology-vocab-extension/rcc8-spatial-relations"/>
        <rdfs:isDefinedBy rdf:resource="http://www.opengis.net/spec/geosparql/1.1/req/topology-vocab-extension/rcc8-spatial-relations"/>
        <rdfs:seeAlso rdf:resource="http://dbpedia.org/resource/DE-9IM"/>
        <skos:definition xml:lang="en">States that the subject SpatialObject spatially contains the object SpatialObject. DE-9IM: TTTFFTFFT</skos:definition>
        <skos:prefLabel xml:lang="en">non-tangential proper part inverse</skos:prefLabel>
    </owl:ObjectProperty>
    


    <!-- http://www.opengis.net/ont/geosparql#rcc8po -->


    <owl:ObjectProperty rdf:about="http://www.opengis.net/ont/geosparql#rcc8po">
        <rdfs:domain rdf:resource="http://www.opengis.net/ont/geosparql#SpatialObject"/>
        <rdfs:range rdf:resource="http://www.opengis.net/ont/geosparql#SpatialObject"/>
        <rdfs:isDefinedBy rdf:resource="http://www.opengis.net/ont/geosparql#"/>
        <rdfs:isDefinedBy rdf:resource="http://www.opengis.net/spec/geosparql/1.0/req/topology-vocab-extension/rcc8-spatial-relations"/>
        <rdfs:isDefinedBy rdf:resource="http://www.opengis.net/spec/geosparql/1.1/req/topology-vocab-extension/rcc8-spatial-relations"/>
        <rdfs:seeAlso rdf:resource="http://dbpedia.org/resource/DE-9IM"/>
        <skos:definition xml:lang="en">States that the subject SpatialObject spatially overlaps the object SpatialObject. DE-9IM: TTTTTTTTT</skos:definition>
        <skos:prefLabel xml:lang="en">partially overlapping</skos:prefLabel>
    </owl:ObjectProperty>
    


    <!-- http://www.opengis.net/ont/geosparql#rcc8tpp -->


    <owl:ObjectProperty rdf:about="http://www.opengis.net/ont/geosparql#rcc8tpp">
        <rdfs:domain rdf:resource="http://www.opengis.net/ont/geosparql#SpatialObject"/>
        <rdfs:range rdf:resource="http://www.opengis.net/ont/geosparql#SpatialObject"/>
        <rdfs:isDefinedBy rdf:resource="http://www.opengis.net/ont/geosparql#"/>
        <rdfs:isDefinedBy rdf:resource="http://www.opengis.net/spec/geosparql/1.0/req/topology-vocab-extension/rcc8-spatial-relations"/>
        <rdfs:isDefinedBy rdf:resource="http://www.opengis.net/spec/geosparql/1.1/req/topology-vocab-extension/rcc8-spatial-relations"/>
        <rdfs:seeAlso rdf:resource="http://dbpedia.org/resource/DE-9IM"/>
        <skos:definition xml:lang="en">States that the subject SpatialObject is spatially covered by the object SpatialObject. DE-9IM: TFFTTFTTT</skos:definition>
        <skos:prefLabel xml:lang="en">tangential proper part</skos:prefLabel>
    </owl:ObjectProperty>
    


    <!-- http://www.opengis.net/ont/geosparql#rcc8tppi -->


    <owl:ObjectProperty rdf:about="http://www.opengis.net/ont/geosparql#rcc8tppi">
        <rdfs:domain rdf:resource="http://www.opengis.net/ont/geosparql#SpatialObject"/>
        <rdfs:range rdf:resource="http://www.opengis.net/ont/geosparql#SpatialObject"/>
        <rdfs:isDefinedBy rdf:resource="http://www.opengis.net/ont/geosparql#"/>
        <rdfs:isDefinedBy rdf:resource="http://www.opengis.net/spec/geosparql/1.0/req/topology-vocab-extension/rcc8-spatial-relations"/>
        <rdfs:isDefinedBy rdf:resource="http://www.opengis.net/spec/geosparql/1.1/req/topology-vocab-extension/rcc8-spatial-relations"/>
        <rdfs:seeAlso rdf:resource="http://dbpedia.org/resource/DE-9IM"/>
        <skos:definition xml:lang="en">States that the subject SpatialObject spatially covers the object SpatialObject. DE-9IM: TTTFTTFFT</skos:definition>
        <skos:prefLabel xml:lang="en">tangential proper part inverse</skos:prefLabel>
    </owl:ObjectProperty>
    


    <!-- http://www.opengis.net/ont/geosparql#sfContains -->


    <owl:ObjectProperty rdf:about="http://www.opengis.net/ont/geosparql#sfContains">
        <rdfs:domain rdf:resource="http://www.opengis.net/ont/geosparql#SpatialObject"/>
        <rdfs:range rdf:resource="http://www.opengis.net/ont/geosparql#SpatialObject"/>
        <rdfs:comment xml:lang="en">Exists if the subject SpatialObject spatially contains the object SpatialObject. DE-9IM: T*****FF*</rdfs:comment>
        <rdfs:isDefinedBy rdf:resource="http://www.opengis.net/ont/geosparql"/>
        <rdfs:isDefinedBy rdf:resource="http://www.opengis.net/ont/geosparql#"/>
        <rdfs:isDefinedBy rdf:resource="http://www.opengis.net/spec/geosparql/1.0"/>
        <rdfs:isDefinedBy rdf:resource="http://www.opengis.net/spec/geosparql/1.0/req/topology-vocab-extension/rcc8-spatial-relations"/>
        <rdfs:isDefinedBy rdf:resource="http://www.opengis.net/spec/geosparql/1.1/req/topology-vocab-extension/rcc8-spatial-relations"/>
        <rdfs:label xml:lang="en">contains</rdfs:label>
        <rdfs:label xml:lang="en">sfContains</rdfs:label>
        <rdfs:seeAlso rdf:resource="http://dbpedia.org/resource/DE-9IM"/>
        <skos:definition xml:lang="en">States that the subject SpatialObject spatially contains the object SpatialObject. DE-9IM: T*****FF*</skos:definition>
        <skos:prefLabel xml:lang="en">contains</skos:prefLabel>
    </owl:ObjectProperty>
    


    <!-- http://www.opengis.net/ont/geosparql#sfCrosses -->


    <owl:ObjectProperty rdf:about="http://www.opengis.net/ont/geosparql#sfCrosses">
        <rdfs:domain rdf:resource="http://www.opengis.net/ont/geosparql#SpatialObject"/>
        <rdfs:range rdf:resource="http://www.opengis.net/ont/geosparql#SpatialObject"/>
        <rdfs:isDefinedBy rdf:resource="http://www.opengis.net/ont/geosparql#"/>
        <rdfs:isDefinedBy rdf:resource="http://www.opengis.net/spec/geosparql/1.0/req/topology-vocab-extension/sf-spatial-relations"/>
        <rdfs:isDefinedBy rdf:resource="http://www.opengis.net/spec/geosparql/1.1/req/topology-vocab-extension/sf-spatial-relations"/>
        <rdfs:seeAlso rdf:resource="http://dbpedia.org/resource/DE-9IM"/>
        <skos:definition xml:lang="en">States that the subject SpatialObject spatially crosses the object SpatialObject. DE-9IM: T*T******</skos:definition>
        <skos:prefLabel xml:lang="en">crosses</skos:prefLabel>
    </owl:ObjectProperty>
    


    <!-- http://www.opengis.net/ont/geosparql#sfDisjoint -->


    <owl:ObjectProperty rdf:about="http://www.opengis.net/ont/geosparql#sfDisjoint">
        <rdfs:domain rdf:resource="http://www.opengis.net/ont/geosparql#SpatialObject"/>
        <rdfs:range rdf:resource="http://www.opengis.net/ont/geosparql#SpatialObject"/>
        <rdfs:isDefinedBy rdf:resource="http://www.opengis.net/ont/geosparql#"/>
        <rdfs:isDefinedBy rdf:resource="http://www.opengis.net/spec/geosparql/1.0/req/topology-vocab-extension/sf-spatial-relations"/>
        <rdfs:isDefinedBy rdf:resource="http://www.opengis.net/spec/geosparql/1.1/req/topology-vocab-extension/sf-spatial-relations"/>
        <rdfs:seeAlso rdf:resource="http://dbpedia.org/resource/DE-9IM"/>
        <skos:definition xml:lang="en">States that the subject SpatialObject is spatially disjoint from the object SpatialObject. DE-9IM: FF*FF****</skos:definition>
        <skos:prefLabel xml:lang="en">disjoint</skos:prefLabel>
    </owl:ObjectProperty>
    


    <!-- http://www.opengis.net/ont/geosparql#sfEquals -->


    <owl:ObjectProperty rdf:about="http://www.opengis.net/ont/geosparql#sfEquals">
        <rdfs:domain rdf:resource="http://www.opengis.net/ont/geosparql#SpatialObject"/>
        <rdfs:range rdf:resource="http://www.opengis.net/ont/geosparql#SpatialObject"/>
        <rdfs:isDefinedBy rdf:resource="http://www.opengis.net/ont/geosparql#"/>
        <rdfs:isDefinedBy rdf:resource="http://www.opengis.net/spec/geosparql/1.0/req/topology-vocab-extension/sf-spatial-relations"/>
        <rdfs:isDefinedBy rdf:resource="http://www.opengis.net/spec/geosparql/1.1/req/topology-vocab-extension/sf-spatial-relations"/>
        <rdfs:seeAlso rdf:resource="http://dbpedia.org/resource/DE-9IM"/>
        <skos:definition xml:lang="en">States that the subject SpatialObject spatially equals the object SpatialObject. DE-9IM: TFFFTFFFT</skos:definition>
        <skos:prefLabel xml:lang="en">equals</skos:prefLabel>
    </owl:ObjectProperty>
    


    <!-- http://www.opengis.net/ont/geosparql#sfIntersects -->


    <owl:ObjectProperty rdf:about="http://www.opengis.net/ont/geosparql#sfIntersects">
        <rdfs:domain rdf:resource="http://www.opengis.net/ont/geosparql#SpatialObject"/>
        <rdfs:range rdf:resource="http://www.opengis.net/ont/geosparql#SpatialObject"/>
        <rdfs:isDefinedBy rdf:resource="http://www.opengis.net/ont/geosparql#"/>
        <rdfs:isDefinedBy rdf:resource="http://www.opengis.net/spec/geosparql/1.0/req/topology-vocab-extension/sf-spatial-relations"/>
        <rdfs:isDefinedBy rdf:resource="http://www.opengis.net/spec/geosparql/1.1/req/topology-vocab-extension/sf-spatial-relations"/>
        <rdfs:seeAlso rdf:resource="http://dbpedia.org/resource/DE-9IM"/>
        <skos:definition xml:lang="en">States that the subject SpatialObject is not spatially disjoint from the object SpatialObject. DE-9IM: T******** ^ *T******* ^ ***T***** ^ ****T****</skos:definition>
        <skos:prefLabel xml:lang="en">intersects</skos:prefLabel>
    </owl:ObjectProperty>
    


    <!-- http://www.opengis.net/ont/geosparql#sfOverlaps -->


    <owl:ObjectProperty rdf:about="http://www.opengis.net/ont/geosparql#sfOverlaps">
        <rdfs:domain rdf:resource="http://www.opengis.net/ont/geosparql#SpatialObject"/>
        <rdfs:range rdf:resource="http://www.opengis.net/ont/geosparql#SpatialObject"/>
        <rdfs:isDefinedBy rdf:resource="http://www.opengis.net/ont/geosparql#"/>
        <rdfs:isDefinedBy rdf:resource="http://www.opengis.net/spec/geosparql/1.0/req/topology-vocab-extension/sf-spatial-relations"/>
        <rdfs:isDefinedBy rdf:resource="http://www.opengis.net/spec/geosparql/1.1/req/topology-vocab-extension/sf-spatial-relations"/>
        <rdfs:seeAlso rdf:resource="http://dbpedia.org/resource/DE-9IM"/>
        <skos:definition xml:lang="en">States that the subject SpatialObject spatially overlaps the object SpatialObject. DE-9IM: T*T***T**</skos:definition>
        <skos:prefLabel xml:lang="en">overlaps</skos:prefLabel>
    </owl:ObjectProperty>
    


    <!-- http://www.opengis.net/ont/geosparql#sfTouches -->


    <owl:ObjectProperty rdf:about="http://www.opengis.net/ont/geosparql#sfTouches">
        <rdfs:domain rdf:resource="http://www.opengis.net/ont/geosparql#SpatialObject"/>
        <rdfs:range rdf:resource="http://www.opengis.net/ont/geosparql#SpatialObject"/>
        <rdfs:isDefinedBy rdf:resource="http://www.opengis.net/ont/geosparql#"/>
        <rdfs:isDefinedBy rdf:resource="http://www.opengis.net/spec/geosparql/1.0/req/topology-vocab-extension/sf-spatial-relations"/>
        <rdfs:isDefinedBy rdf:resource="http://www.opengis.net/spec/geosparql/1.1/req/topology-vocab-extension/sf-spatial-relations"/>
        <rdfs:seeAlso rdf:resource="http://dbpedia.org/resource/DE-9IM"/>
        <skos:definition xml:lang="en">States that the subject SpatialObject spatially touches the object SpatialObject. DE-9IM: FT******* ^ F**T***** ^ F***T****</skos:definition>
        <skos:prefLabel xml:lang="en">touches</skos:prefLabel>
    </owl:ObjectProperty>
    


    <!-- http://www.opengis.net/ont/geosparql#sfWithin -->


    <owl:ObjectProperty rdf:about="http://www.opengis.net/ont/geosparql#sfWithin">
        <rdfs:domain rdf:resource="http://www.opengis.net/ont/geosparql#SpatialObject"/>
        <rdfs:range rdf:resource="http://www.opengis.net/ont/geosparql#SpatialObject"/>
        <rdfs:comment xml:lang="en">Exists if the subject SpatialObject is spatially within the object SpatialObject. DE-9IM: T*F**F***</rdfs:comment>
        <rdfs:isDefinedBy rdf:resource="http://www.opengis.net/ont/geosparql"/>
        <rdfs:isDefinedBy rdf:resource="http://www.opengis.net/ont/geosparql#"/>
        <rdfs:isDefinedBy rdf:resource="http://www.opengis.net/spec/geosparql/1.0"/>
        <rdfs:isDefinedBy rdf:resource="http://www.opengis.net/spec/geosparql/1.0/req/topology-vocab-extension/sf-spatial-relations"/>
        <rdfs:isDefinedBy rdf:resource="http://www.opengis.net/spec/geosparql/1.1/req/topology-vocab-extension/sf-spatial-relations"/>
        <rdfs:label xml:lang="en">sfWithin</rdfs:label>
        <rdfs:label xml:lang="en">within</rdfs:label>
        <rdfs:seeAlso rdf:resource="http://dbpedia.org/resource/DE-9IM"/>
        <skos:definition xml:lang="en">States that the subject SpatialObject is spatially within the object SpatialObject. DE-9IM: T*F**F***</skos:definition>
        <skos:prefLabel xml:lang="en">within</skos:prefLabel>
    </owl:ObjectProperty>
    


    <!-- http://www.w3.org/2000/01/rdf-schema#member -->


    <owl:ObjectProperty rdf:about="http://www.w3.org/2000/01/rdf-schema#member"/>
    


    <!-- http://www.w3.org/2003/01/geo/wgs84_pos#location -->


    <owl:ObjectProperty rdf:about="http://www.w3.org/2003/01/geo/wgs84_pos#location">
        <rdfs:subPropertyOf rdf:resource="http://xmlns.com/foaf/0.1/based_near"/>
    </owl:ObjectProperty>
    


    <!-- http://www.w3.org/2003/01/geo/wgs84_pos#long -->


    <owl:ObjectProperty rdf:about="http://www.w3.org/2003/01/geo/wgs84_pos#long">
        <rdfs:domain rdf:resource="http://www.w3.org/2003/01/geo/wgs84_pos#SpatialThing"/>
    </owl:ObjectProperty>
    


    <!-- http://www.w3.org/2006/time#after -->


    <owl:ObjectProperty rdf:about="http://www.w3.org/2006/time#after">
        <owl:inverseOf rdf:resource="http://www.w3.org/2006/time#before"/>
        <rdfs:domain rdf:resource="http://www.w3.org/2006/time#TemporalEntity"/>
        <rdfs:range rdf:resource="http://www.w3.org/2006/time#TemporalEntity"/>
        <rdfs:comment xml:lang="es">Asume una dirección en el tiempo. Si una entidad temporal T1 está después de otra entidad temporal T2, entonces el principio de T1 está después del final de T2.</rdfs:comment>
        <rdfs:comment xml:lang="en">Gives directionality to time. If a temporal entity T1 is after another temporal entity T2, then the beginning of T1 is after the end of T2.</rdfs:comment>
        <rdfs:label xml:lang="en">after</rdfs:label>
        <rdfs:label xml:lang="es">después</rdfs:label>
        <skos:definition xml:lang="es">Asume una dirección en el tiempo. Si una entidad temporal T1 está después de otra entidad temporal T2, entonces el principio de T1 está después del final de T2.</skos:definition>
        <skos:definition xml:lang="en">Gives directionality to time. If a temporal entity T1 is after another temporal entity T2, then the beginning of T1 is after the end of T2.</skos:definition>
    </owl:ObjectProperty>
    


    <!-- http://www.w3.org/2006/time#before -->


    <owl:ObjectProperty rdf:about="http://www.w3.org/2006/time#before">
        <rdf:type rdf:resource="http://www.w3.org/2002/07/owl#TransitiveProperty"/>
        <rdfs:domain rdf:resource="http://www.w3.org/2006/time#TemporalEntity"/>
        <rdfs:range rdf:resource="http://www.w3.org/2006/time#TemporalEntity"/>
        <rdfs:comment xml:lang="es">Asume una dirección en el tiempo. Si una entidad temporal T1 está antes que otra entidad temporal T2, entonces el final de T1 está antes que el principio de T2. Así, &quot;antes&quot; se puede considerar básica para instantes y derivada para intervalos.</rdfs:comment>
        <rdfs:comment xml:lang="en">Gives directionality to time. If a temporal entity T1 is before another temporal entity T2, then the end of T1 is before the beginning of T2. Thus, &quot;before&quot; can be considered to be basic to instants and derived for intervals.</rdfs:comment>
        <rdfs:label xml:lang="es">antes</rdfs:label>
        <rdfs:label xml:lang="en">before</rdfs:label>
        <skos:definition xml:lang="es">Asume una dirección en el tiempo. Si una entidad temporal T1 está antes que otra entidad temporal T2, entonces el final de T1 está antes que el principio de T2. Así, &quot;antes&quot; se puede considerar básica para instantes y derivada para intervalos.</skos:definition>
        <skos:definition xml:lang="en">Gives directionality to time. If a temporal entity T1 is before another temporal entity T2, then the end of T1 is before the beginning of T2. Thus, &quot;before&quot; can be considered to be basic to instants and derived for intervals.</skos:definition>
    </owl:ObjectProperty>
    


    <!-- http://www.w3.org/2006/time#dayOfWeek -->


    <owl:ObjectProperty rdf:about="http://www.w3.org/2006/time#dayOfWeek">
        <rdfs:domain rdf:resource="http://www.w3.org/2006/time#GeneralDateTimeDescription"/>
        <rdfs:range rdf:resource="http://www.w3.org/2006/time#DayOfWeek"/>
        <rdfs:comment xml:lang="en">The day of week, whose value is a member of the class time:DayOfWeek</rdfs:comment>
        <rdfs:comment>El día de la semana, cuyo valor es un miembro de la clase &apos;día de la semana&apos;.</rdfs:comment>
        <rdfs:label xml:lang="en">day of week</rdfs:label>
        <rdfs:label xml:lang="es">día de la semana</rdfs:label>
        <skos:definition xml:lang="es">El día de la semana, cuyo valor es un miembro de la clase &apos;día de la semana&apos;.</skos:definition>
        <skos:definition xml:lang="en">The day of week, whose value is a member of the class time:DayOfWeek</skos:definition>
    </owl:ObjectProperty>
    


    <!-- http://www.w3.org/2006/time#hasBeginning -->


    <owl:ObjectProperty rdf:about="http://www.w3.org/2006/time#hasBeginning">
        <rdfs:subPropertyOf rdf:resource="http://www.w3.org/2006/time#hasTime"/>
        <rdfs:domain rdf:resource="http://www.w3.org/2006/time#TemporalEntity"/>
        <rdfs:range rdf:resource="http://www.w3.org/2006/time#Instant"/>
        <rdfs:comment xml:lang="en">Beginning of a temporal entity</rdfs:comment>
        <rdfs:comment xml:lang="es">Comienzo de una entidad temporal.</rdfs:comment>
        <rdfs:label xml:lang="en">has beginning</rdfs:label>
        <rdfs:label xml:lang="es">tiene principio</rdfs:label>
        <skos:definition xml:lang="en">Beginning of a temporal entity.</skos:definition>
        <skos:definition xml:lang="es">Comienzo de una entidad temporal.</skos:definition>
    </owl:ObjectProperty>
    


    <!-- http://www.w3.org/2006/time#hasDateTimeDescription -->


    <owl:ObjectProperty rdf:about="http://www.w3.org/2006/time#hasDateTimeDescription">
        <rdfs:domain rdf:resource="http://www.w3.org/2006/time#DateTimeInterval"/>
        <rdfs:range rdf:resource="http://www.w3.org/2006/time#GeneralDateTimeDescription"/>
        <rdfs:comment xml:lang="es">Valor de intervalo de fecha-hora expresado como un valor estructurado. El principio y el final del intervalo coincide con los límites del elemento más corto en la descripción.</rdfs:comment>
        <rdfs:comment xml:lang="en">Value of DateTimeInterval expressed as a structured value. The beginning and end of the interval coincide with the limits of the shortest element in the description.</rdfs:comment>
        <rdfs:label xml:lang="en">has Date-Time description</rdfs:label>
        <rdfs:label xml:lang="es">tiene descripción fecha-hora</rdfs:label>
        <skos:definition xml:lang="es">Valor de intervalo de fecha-hora expresado como un valor estructurado. El principio y el final del intervalo coincide con los límites del elemento más corto en la descripción.</skos:definition>
        <skos:definition xml:lang="en">Value of DateTimeInterval expressed as a structured value. The beginning and end of the interval coincide with the limits of the shortest element in the description.</skos:definition>
    </owl:ObjectProperty>
    


    <!-- http://www.w3.org/2006/time#hasDuration -->


    <owl:ObjectProperty rdf:about="http://www.w3.org/2006/time#hasDuration">
        <rdfs:subPropertyOf rdf:resource="http://www.w3.org/2006/time#hasTemporalDuration"/>
        <rdfs:range rdf:resource="http://www.w3.org/2006/time#Duration"/>
        <rdfs:comment xml:lang="es">Duración de una entidad temporal, expresada como un valor escalado o un valor nominal.</rdfs:comment>
        <rdfs:comment xml:lang="en">Duration of a temporal entity, expressed as a scaled value or nominal value</rdfs:comment>
        <rdfs:label xml:lang="en">has duration</rdfs:label>
        <rdfs:label xml:lang="es">tiene duración</rdfs:label>
        <skos:definition xml:lang="es">Duración de una entidad temporal, evento o actividad, o cosa, expresada como un valor escalado.</skos:definition>
        <skos:definition xml:lang="en">Duration of a temporal entity, event or activity, or thing, expressed as a scaled value</skos:definition>
    </owl:ObjectProperty>
    


    <!-- http://www.w3.org/2006/time#hasDurationDescription -->


    <owl:ObjectProperty rdf:about="http://www.w3.org/2006/time#hasDurationDescription">
        <rdfs:subPropertyOf rdf:resource="http://www.w3.org/2006/time#hasTemporalDuration"/>
        <rdfs:range rdf:resource="http://www.w3.org/2006/time#GeneralDurationDescription"/>
        <rdfs:comment xml:lang="es">Duración de una entidad temporal, expresada utilizando una descripción estructurada.</rdfs:comment>
        <rdfs:comment xml:lang="en">Duration of a temporal entity, expressed using a structured description</rdfs:comment>
        <rdfs:label xml:lang="en">has duration description</rdfs:label>
        <rdfs:label xml:lang="es">tiene descripción de duración</rdfs:label>
        <skos:definition xml:lang="es">Duración de una entidad temporal, expresada utilizando una descripción estructurada.</skos:definition>
        <skos:definition xml:lang="en">Duration of a temporal entity, expressed using a structured description</skos:definition>
    </owl:ObjectProperty>
    


    <!-- http://www.w3.org/2006/time#hasEnd -->


    <owl:ObjectProperty rdf:about="http://www.w3.org/2006/time#hasEnd">
        <rdfs:subPropertyOf rdf:resource="http://www.w3.org/2006/time#hasTime"/>
        <rdfs:domain rdf:resource="http://www.w3.org/2006/time#TemporalEntity"/>
        <rdfs:range rdf:resource="http://www.w3.org/2006/time#Instant"/>
        <rdfs:comment xml:lang="en">End of a temporal entity.</rdfs:comment>
        <rdfs:comment xml:lang="es">Final de una entidad temporal.</rdfs:comment>
        <rdfs:label xml:lang="en">has end</rdfs:label>
        <rdfs:label xml:lang="es">tiene fin</rdfs:label>
        <skos:definition xml:lang="en">End of a temporal entity.</skos:definition>
        <skos:definition xml:lang="es">Final de una entidad temporal.</skos:definition>
    </owl:ObjectProperty>
    


    <!-- http://www.w3.org/2006/time#hasTRS -->


    <owl:ObjectProperty rdf:about="http://www.w3.org/2006/time#hasTRS">
        <rdf:type rdf:resource="http://www.w3.org/2002/07/owl#FunctionalProperty"/>
        <rdfs:domain>
            <owl:Class>
                <owl:unionOf rdf:parseType="Collection">
                    <rdf:Description rdf:about="http://www.w3.org/2006/time#GeneralDurationDescription"/>
                    <rdf:Description rdf:about="http://www.w3.org/2006/time#TemporalPosition"/>
                </owl:unionOf>
            </owl:Class>
        </rdfs:domain>
        <rdfs:range rdf:resource="http://www.w3.org/2006/time#TRS"/>
        <rdfs:comment xml:lang="es">El sistema de referencia temporal utilizado por una posición temporal o descripción de extensión.</rdfs:comment>
        <rdfs:comment xml:lang="en">The temporal reference system used by a temporal position or extent description. </rdfs:comment>
        <rdfs:label xml:lang="en">Temporal reference system used</rdfs:label>
        <rdfs:label xml:lang="es">sistema de referencia temporal utilizado</rdfs:label>
        <skos:definition xml:lang="es">El sistema de referencia temporal utilizado por una posición temporal o descripción de extensión.</skos:definition>
        <skos:definition xml:lang="en">The temporal reference system used by a temporal position or extent description. </skos:definition>
    </owl:ObjectProperty>
    


    <!-- http://www.w3.org/2006/time#hasTemporalDuration -->


    <owl:ObjectProperty rdf:about="http://www.w3.org/2006/time#hasTemporalDuration">
        <rdfs:domain rdf:resource="http://www.w3.org/2006/time#TemporalEntity"/>
        <rdfs:range rdf:resource="http://www.w3.org/2006/time#TemporalDuration"/>
        <rdfs:comment xml:lang="es">Duración de una entidad temporal.</rdfs:comment>
        <rdfs:comment xml:lang="en">Duration of a temporal entity.</rdfs:comment>
        <rdfs:label xml:lang="en">has temporal duration</rdfs:label>
        <rdfs:label xml:lang="es">tiene duración temporal</rdfs:label>
        <skos:definition xml:lang="es">Duración de una entidad temporal.</skos:definition>
        <skos:definition xml:lang="en">Duration of a temporal entity.</skos:definition>
    </owl:ObjectProperty>
    


    <!-- http://www.w3.org/2006/time#hasTime -->


    <owl:ObjectProperty rdf:about="http://www.w3.org/2006/time#hasTime">
        <rdfs:range rdf:resource="http://www.w3.org/2006/time#TemporalEntity"/>
        <rdfs:comment xml:lang="es">Proporciona soporte a la asociación de una entidad temporal (instante o intervalo) a cualquier cosa.</rdfs:comment>
        <rdfs:comment xml:lang="en">Supports the association of a temporal entity (instant or interval) to any thing</rdfs:comment>
        <rdfs:label xml:lang="en">has time</rdfs:label>
        <rdfs:label xml:lang="es">tiene tiempo</rdfs:label>
        <skos:definition xml:lang="es">Proporciona soporte a la asociación de una entidad temporal (instante o intervalo) a cualquier cosa.</skos:definition>
        <skos:definition xml:lang="en">Supports the association of a temporal entity (instant or interval) to any thing</skos:definition>
        <skos:editorialNote xml:lang="es">Característica arriesgada -añadida en la revisión del 2017 que no ha sido todavía utilizada de forma amplia.</skos:editorialNote>
        <skos:editorialNote xml:lang="en">Feature at risk - added in 2017 revision, and not yet widely used. </skos:editorialNote>
    </owl:ObjectProperty>
    


    <!-- http://www.w3.org/2006/time#inDateTime -->


    <owl:ObjectProperty rdf:about="http://www.w3.org/2006/time#inDateTime">
        <rdfs:subPropertyOf rdf:resource="http://www.w3.org/2006/time#inTemporalPosition"/>
        <rdfs:domain rdf:resource="http://www.w3.org/2006/time#Instant"/>
        <rdfs:range rdf:resource="http://www.w3.org/2006/time#GeneralDateTimeDescription"/>
        <rdfs:comment xml:lang="es">Posición de un instante, expresada utilizando una descripción estructurada.</rdfs:comment>
        <rdfs:comment xml:lang="en">Position of an instant, expressed using a structured description</rdfs:comment>
        <rdfs:label xml:lang="es">en descripción de fecha-hora</rdfs:label>
        <rdfs:label xml:lang="en">in date-time description</rdfs:label>
        <skos:definition xml:lang="es">Posición de un instante, expresada utilizando una descripción estructurada.</skos:definition>
        <skos:definition xml:lang="en">Position of an instant, expressed using a structured description</skos:definition>
    </owl:ObjectProperty>
    


    <!-- http://www.w3.org/2006/time#inTemporalPosition -->


    <owl:ObjectProperty rdf:about="http://www.w3.org/2006/time#inTemporalPosition">
        <rdfs:domain rdf:resource="http://www.w3.org/2006/time#Instant"/>
        <rdfs:range rdf:resource="http://www.w3.org/2006/time#TemporalPosition"/>
        <rdfs:comment xml:lang="es">Posición de un instante de tiempo.</rdfs:comment>
        <rdfs:comment xml:lang="en">Position of a time instant</rdfs:comment>
        <rdfs:label xml:lang="en">Temporal position</rdfs:label>
        <rdfs:label xml:lang="es">posición temporal</rdfs:label>
        <skos:definition xml:lang="es">Posición de un instante de tiempo.</skos:definition>
        <skos:definition xml:lang="en">Position of a time instant</skos:definition>
    </owl:ObjectProperty>
    


    <!-- http://www.w3.org/2006/time#inTimePosition -->


    <owl:ObjectProperty rdf:about="http://www.w3.org/2006/time#inTimePosition">
        <rdfs:subPropertyOf rdf:resource="http://www.w3.org/2006/time#inTemporalPosition"/>
        <rdfs:domain rdf:resource="http://www.w3.org/2006/time#Instant"/>
        <rdfs:range rdf:resource="http://www.w3.org/2006/time#TimePosition"/>
        <rdfs:comment xml:lang="es">Posición de un instante, expresada como una coordenada temporal o un valor nominal.</rdfs:comment>
        <rdfs:comment xml:lang="en">Position of an instant, expressed as a temporal coordinate or nominal value</rdfs:comment>
        <rdfs:label xml:lang="en">Time position</rdfs:label>
        <rdfs:label xml:lang="es">posición de tiempo</rdfs:label>
        <skos:definition xml:lang="es">Posición de un instante, expresada como una coordenada temporal o un valor nominal.</skos:definition>
        <skos:definition xml:lang="en">Position of a time instant expressed as a TimePosition</skos:definition>
    </owl:ObjectProperty>
    


    <!-- http://www.w3.org/2006/time#inside -->


    <owl:ObjectProperty rdf:about="http://www.w3.org/2006/time#inside">
        <rdfs:domain rdf:resource="http://www.w3.org/2006/time#Interval"/>
        <rdfs:range rdf:resource="http://www.w3.org/2006/time#Instant"/>
        <rdfs:comment xml:lang="en">An instant that falls inside the interval. It is not intended to include beginnings and ends of intervals.</rdfs:comment>
        <rdfs:comment xml:lang="es">Un instante que cae dentro del intervalo. Se asume que no es ni el principio ni el final de ningún intervalo.</rdfs:comment>
        <rdfs:label xml:lang="en">has time instant inside</rdfs:label>
        <rdfs:label xml:lang="es">tiene instante de tiempo dentro</rdfs:label>
        <skos:definition xml:lang="en">An instant that falls inside the interval. It is not intended to include beginnings and ends of intervals.</skos:definition>
        <skos:definition xml:lang="es">Un instante que cae dentro del intervalo. Se asume que no es ni el principio ni el final de ningún intervalo.</skos:definition>
    </owl:ObjectProperty>
    


    <!-- http://www.w3.org/2006/time#intervalAfter -->


    <owl:ObjectProperty rdf:about="http://www.w3.org/2006/time#intervalAfter">
        <rdfs:subPropertyOf rdf:resource="http://www.w3.org/2006/time#after"/>
        <rdfs:subPropertyOf rdf:resource="http://www.w3.org/2006/time#intervalDisjoint"/>
        <owl:inverseOf rdf:resource="http://www.w3.org/2006/time#intervalBefore"/>
        <rdfs:domain rdf:resource="http://www.w3.org/2006/time#ProperInterval"/>
        <rdfs:range rdf:resource="http://www.w3.org/2006/time#ProperInterval"/>
        <rdfs:comment xml:lang="en">If a proper interval T1 is intervalAfter another proper interval T2, then the beginning of T1 is after the end of T2.</rdfs:comment>
        <rdfs:comment>Si un intervalo propio T1 es posterior a otro intervalo propio T2, entonces el principio de T1 está después que el final de T2.</rdfs:comment>
        <rdfs:label xml:lang="en">interval after</rdfs:label>
        <rdfs:label xml:lang="es">intervalo posterior</rdfs:label>
        <skos:definition xml:lang="en">If a proper interval T1 is intervalAfter another proper interval T2, then the beginning of T1 is after the end of T2.</skos:definition>
        <skos:definition xml:lang="es">Si un intervalo propio T1 es posterior a otro intervalo propio T2, entonces el principio de T1 está después que el final de T2.</skos:definition>
    </owl:ObjectProperty>
    


    <!-- http://www.w3.org/2006/time#intervalBefore -->


    <owl:ObjectProperty rdf:about="http://www.w3.org/2006/time#intervalBefore">
        <rdfs:subPropertyOf rdf:resource="http://www.w3.org/2006/time#before"/>
        <rdfs:subPropertyOf rdf:resource="http://www.w3.org/2006/time#intervalDisjoint"/>
        <rdfs:domain rdf:resource="http://www.w3.org/2006/time#ProperInterval"/>
        <rdfs:range rdf:resource="http://www.w3.org/2006/time#ProperInterval"/>
        <rdfs:comment xml:lang="en">If a proper interval T1 is intervalBefore another proper interval T2, then the end of T1 is before the beginning of T2.</rdfs:comment>
        <rdfs:comment xml:lang="es">Si un intervalo propio T1 está antes que otro intervalo propio T2, entonces el final de T1 está antes que el principio de T2.</rdfs:comment>
        <rdfs:label xml:lang="en">interval before</rdfs:label>
        <rdfs:label xml:lang="es">intervalo anterior</rdfs:label>
        <skos:definition xml:lang="en">If a proper interval T1 is intervalBefore another proper interval T2, then the end of T1 is before the beginning of T2.</skos:definition>
        <skos:definition xml:lang="es">Si un intervalo propio T1 está antes que otro intervalo propio T2, entonces el final de T1 está antes que el principio de T2.</skos:definition>
    </owl:ObjectProperty>
    


    <!-- http://www.w3.org/2006/time#intervalContains -->


    <owl:ObjectProperty rdf:about="http://www.w3.org/2006/time#intervalContains">
        <owl:inverseOf rdf:resource="http://www.w3.org/2006/time#intervalDuring"/>
        <rdfs:domain rdf:resource="http://www.w3.org/2006/time#ProperInterval"/>
        <rdfs:range rdf:resource="http://www.w3.org/2006/time#ProperInterval"/>
        <rdfs:comment xml:lang="en">If a proper interval T1 is intervalContains another proper interval T2, then the beginning of T1 is before the beginning of T2, and the end of T1 is after the end of T2.</rdfs:comment>
        <rdfs:comment xml:lang="es">Si un intervalo propio T1 contiene otro intervalo propio T2, entonces el principio de T1 está antes que el principio de T2, y el final de T1 está después del final de T2.</rdfs:comment>
        <rdfs:label xml:lang="en">interval contains</rdfs:label>
        <rdfs:label xml:lang="es">intervalo contiene</rdfs:label>
        <skos:definition xml:lang="en">If a proper interval T1 is intervalContains another proper interval T2, then the beginning of T1 is before the beginning of T2, and the end of T1 is after the end of T2.</skos:definition>
        <skos:definition xml:lang="es">Si un intervalo propio T1 contiene otro intervalo propio T2, entonces el principio de T1 está antes que el principio de T2, y el final de T1 está después del final de T2.</skos:definition>
    </owl:ObjectProperty>
    


    <!-- http://www.w3.org/2006/time#intervalDisjoint -->


    <owl:ObjectProperty rdf:about="http://www.w3.org/2006/time#intervalDisjoint">
        <rdfs:domain rdf:resource="http://www.w3.org/2006/time#ProperInterval"/>
        <rdfs:range rdf:resource="http://www.w3.org/2006/time#ProperInterval"/>
        <rdfs:comment xml:lang="en">If a proper interval T1 is intervalDisjoint another proper interval T2, then the beginning of T1 is after the end of T2, or the end of T1 is before the beginning of T2, i.e. the intervals do not overlap in any way, but their ordering relationship is not known.</rdfs:comment>
        <rdfs:comment xml:lang="es">Si un intervalo propio T1 es disjunto con otro intervalo propio T2, entonces el principio de T1 está después del final de T2, o el final de T1 está antes que el principio de T2, es decir, los intervalos no se solapan de ninguna forma, aunque su relación de orden no se conozca.</rdfs:comment>
        <rdfs:label xml:lang="en">interval disjoint</rdfs:label>
        <rdfs:label xml:lang="es">intervalo disjunto</rdfs:label>
        <skos:definition xml:lang="en">If a proper interval T1 is intervalDisjoint another proper interval T2, then the beginning of T1 is after the end of T2, or the end of T1 is before the beginning of T2, i.e. the intervals do not overlap in any way, but their ordering relationship is not known.</skos:definition>
        <skos:definition xml:lang="es">Si un intervalo propio T1 es disjunto con otro intervalo propio T2, entonces el principio de T1 está después del final de T2, o el final de T1 está antes que el principio de T2, es decir, los intervalos no se solapan de ninguna forma, aunque su relación de orden no se conozca.</skos:definition>
        <skos:note xml:lang="es">Esta relación entre intervalos no estaba incluida en las 13 relaciones básicas definidas por Allen (1984), pero está definida en T.3 como la unión de &apos;intervalo anterior&apos; con &apos;intervalo posterior&apos;. Sin embargo, esto está fuera de la expresividad de OWL2, por tanto, está implementado como una propiedad explícita, con &apos;intervalo anterior&apos; e &apos;intervalo posterior&apos; como sub-propiedades.</skos:note>
        <skos:note xml:lang="en">This interval relation is not included in the 13 basic relationships defined in Allen (1984), but is defined in (T.3) as the union of :intervalBefore v :intervalAfter . However, that is outside OWL2 expressivity, so is implemented as an explicit property, with :intervalBefore , :intervalAfter as sub-properties</skos:note>
    </owl:ObjectProperty>
    


    <!-- http://www.w3.org/2006/time#intervalDuring -->


    <owl:ObjectProperty rdf:about="http://www.w3.org/2006/time#intervalDuring">
        <rdfs:subPropertyOf rdf:resource="http://www.w3.org/2006/time#intervalIn"/>
        <rdfs:domain rdf:resource="http://www.w3.org/2006/time#ProperInterval"/>
        <rdfs:range rdf:resource="http://www.w3.org/2006/time#ProperInterval"/>
        <rdfs:comment xml:lang="en">If a proper interval T1 is intervalDuring another proper interval T2, then the beginning of T1 is after the beginning of T2, and the end of T1 is before the end of T2.</rdfs:comment>
        <rdfs:comment xml:lang="es">Si un intervalo propio T1 está durante otro intervalo propio T2, entonces del principio de T1 está después del principio de T2, y el final de T1 está antes que el final de T2.</rdfs:comment>
        <rdfs:label xml:lang="en">interval during</rdfs:label>
        <rdfs:label xml:lang="es">intervalo durante</rdfs:label>
        <skos:definition xml:lang="en">If a proper interval T1 is intervalDuring another proper interval T2, then the beginning of T1 is after the beginning of T2, and the end of T1 is before the end of T2.</skos:definition>
        <skos:definition xml:lang="es">Si un intervalo propio T1 está durante otro intervalo propio T2, entonces del principio de T1 está después del principio de T2, y el final de T1 está antes que el final de T2.</skos:definition>
    </owl:ObjectProperty>
    


    <!-- http://www.w3.org/2006/time#intervalEquals -->


    <owl:ObjectProperty rdf:about="http://www.w3.org/2006/time#intervalEquals">
        <rdfs:domain rdf:resource="http://www.w3.org/2006/time#ProperInterval"/>
        <rdfs:range rdf:resource="http://www.w3.org/2006/time#ProperInterval"/>
        <owl:propertyDisjointWith rdf:resource="http://www.w3.org/2006/time#intervalIn"/>
        <rdfs:comment xml:lang="en">If a proper interval T1 is intervalEquals another proper interval T2, then the beginning of T1 is coincident with the beginning of T2, and the end of T1 is coincident with the end of T2.</rdfs:comment>
        <rdfs:comment xml:lang="es">Si un intervalo propio T1 es igual a otro intervalo propio T2, entonces el principio de T1 coincide con el principio de T2, y el final de T1 coincide con el final de T2.</rdfs:comment>
        <rdfs:label xml:lang="en">interval equals</rdfs:label>
        <rdfs:label xml:lang="es">intervalo igual</rdfs:label>
        <skos:definition xml:lang="en">If a proper interval T1 is intervalEquals another proper interval T2, then the beginning of T1 is coincident with the beginning of T2, and the end of T1 is coincident with the end of T2.</skos:definition>
        <skos:definition xml:lang="es">Si un intervalo propio T1 es igual a otro intervalo propio T2, entonces el principio de T1 coincide con el principio de T2, y el final de T1 coincide con el final de T2.</skos:definition>
    </owl:ObjectProperty>
    


    <!-- http://www.w3.org/2006/time#intervalFinishedBy -->


    <owl:ObjectProperty rdf:about="http://www.w3.org/2006/time#intervalFinishedBy">
        <owl:inverseOf rdf:resource="http://www.w3.org/2006/time#intervalFinishes"/>
        <rdfs:domain rdf:resource="http://www.w3.org/2006/time#ProperInterval"/>
        <rdfs:range rdf:resource="http://www.w3.org/2006/time#ProperInterval"/>
        <rdfs:comment xml:lang="en">If a proper interval T1 is intervalFinishedBy another proper interval T2, then the beginning of T1 is before the beginning of T2, and the end of T1 is coincident with the end of T2.</rdfs:comment>
        <rdfs:comment xml:lang="es">Si un intervalo propio T1 está terminado por otro intervalo propio T2, entonces el principio de T1 está antes que el principio de T2, y el final de T1 coincide con el final de T2.</rdfs:comment>
        <rdfs:label xml:lang="en">interval finished by</rdfs:label>
        <rdfs:label xml:lang="es">intervalo terminado por</rdfs:label>
        <skos:definition xml:lang="en">If a proper interval T1 is intervalFinishedBy another proper interval T2, then the beginning of T1 is before the beginning of T2, and the end of T1 is coincident with the end of T2.</skos:definition>
        <skos:definition xml:lang="es">Si un intervalo propio T1 está terminado por otro intervalo propio T2, entonces el principio de T1 está antes que el principio de T2, y el final de T1 coincide con el final de T2.</skos:definition>
    </owl:ObjectProperty>
    


    <!-- http://www.w3.org/2006/time#intervalFinishes -->


    <owl:ObjectProperty rdf:about="http://www.w3.org/2006/time#intervalFinishes">
        <rdfs:subPropertyOf rdf:resource="http://www.w3.org/2006/time#intervalIn"/>
        <rdfs:domain rdf:resource="http://www.w3.org/2006/time#ProperInterval"/>
        <rdfs:range rdf:resource="http://www.w3.org/2006/time#ProperInterval"/>
        <rdfs:comment xml:lang="en">If a proper interval T1 is intervalFinishes another proper interval T2, then the beginning of T1 is after the beginning of T2, and the end of T1 is coincident with the end of T2.</rdfs:comment>
        <rdfs:comment xml:lang="es">Si un intervalo propio T1 termina otro intervalo propio T2, entonces del principio de T1 está después del principio de T2, y el final de T1 coincide con el final de T2.</rdfs:comment>
        <rdfs:label xml:lang="en">interval finishes</rdfs:label>
        <rdfs:label xml:lang="es">intervalo termina</rdfs:label>
        <skos:definition xml:lang="en">If a proper interval T1 is intervalFinishes another proper interval T2, then the beginning of T1 is after the beginning of T2, and the end of T1 is coincident with the end of T2.</skos:definition>
        <skos:definition xml:lang="es">Si un intervalo propio T1 termina otro intervalo propio T2, entonces del principio de T1 está después del principio de T2, y el final de T1 coincide con el final de T2.</skos:definition>
    </owl:ObjectProperty>
    


    <!-- http://www.w3.org/2006/time#intervalIn -->


    <owl:ObjectProperty rdf:about="http://www.w3.org/2006/time#intervalIn">
        <rdfs:domain rdf:resource="http://www.w3.org/2006/time#ProperInterval"/>
        <rdfs:range rdf:resource="http://www.w3.org/2006/time#ProperInterval"/>
        <rdfs:comment xml:lang="en">If a proper interval T1 is intervalIn another proper interval T2, then the beginning of T1 is after the beginning of T2 or is coincident with the beginning of T2, and the end of T1 is before the end of T2, or is coincident with the end of T2, except that end of T1 may not be coincident with the end of T2 if the beginning of T1 is coincident with the beginning of T2.</rdfs:comment>
        <rdfs:comment xml:lang="es">Si un intervalo propio T1 es un intervalo interior a otro intervalo propio T2, entonces el principio de T1 está después del principio de T2 o coincide con el principio de T2, y el final de T1 está antes que el final de T2, o coincide con el final de T2, excepto que el final de T1 puede no coincidir con el final de T2 si el principio de T1 coincide con el principio de T2.</rdfs:comment>
        <rdfs:label xml:lang="en">interval in</rdfs:label>
        <rdfs:label xml:lang="es">intervalo interior</rdfs:label>
        <skos:definition xml:lang="en">If a proper interval T1 is intervalIn another proper interval T2, then the beginning of T1 is after the beginning of T2 or is coincident with the beginning of T2, and the end of T1 is before the end of T2, or is coincident with the end of T2, except that end of T1 may not be coincident with the end of T2 if the beginning of T1 is coincident with the beginning of T2.</skos:definition>
        <skos:definition xml:lang="es">Si un intervalo propio T1 es un intervalo interior a otro intervalo propio T2, entonces el principio de T1 está después del principio de T2 o coincide con el principio de T2, y el final de T1 está antes que el final de T2, o coincide con el final de T2, excepto que el final de T1 puede no coincidir con el final de T2 si el principio de T1 coincide con el principio de T2.</skos:definition>
        <skos:note xml:lang="es">Esta relación entre intervalos no estaba incluida en las 13 relaciones básicas definidas por Allen (1984), pero se hace referencia a ella como &quot;una relación importante&quot; en Allen y Ferguson (1997). Es la unión disjunta de &apos;intervalo empieza&apos;, &apos;intervalo durante&apos; y con &apos;intervalo termina&apos;. Sin embargo, esto está fuera de la expresividad de OWL2, por tanto, se implementa como una propiedad explícita, con &apos;intervalo empieza&apos;, &apos;intervalo durante&apos; e &apos;intervalo termina&apos; como sub-propiedades.</skos:note>
        <skos:note xml:lang="en">This interval relation is not included in the 13 basic relationships defined in Allen (1984), but is referred to as &apos;an important relationship&apos; in Allen and Ferguson (1997). It is the disjoint union of :intervalStarts v :intervalDuring v :intervalFinishes . However, that is outside OWL2 expressivity, so is implemented as an explicit property, with :intervalStarts , :intervalDuring , :intervalFinishes as sub-properties</skos:note>
    </owl:ObjectProperty>
    


    <!-- http://www.w3.org/2006/time#intervalMeets -->


    <owl:ObjectProperty rdf:about="http://www.w3.org/2006/time#intervalMeets">
        <owl:inverseOf rdf:resource="http://www.w3.org/2006/time#intervalMetBy"/>
        <rdfs:domain rdf:resource="http://www.w3.org/2006/time#ProperInterval"/>
        <rdfs:range rdf:resource="http://www.w3.org/2006/time#ProperInterval"/>
        <rdfs:comment xml:lang="en">If a proper interval T1 is intervalMeets another proper interval T2, then the end of T1 is coincident with the beginning of T2.</rdfs:comment>
        <rdfs:comment xml:lang="es">Si un intervalo propio T1 se encuentra con otro intervalo propio T2, entonces el final de T1 coincide con el principio de T2.</rdfs:comment>
        <rdfs:label xml:lang="en">interval meets</rdfs:label>
        <rdfs:label xml:lang="es">intervalo se encuentra</rdfs:label>
        <skos:definition xml:lang="en">If a proper interval T1 is intervalMeets another proper interval T2, then the end of T1 is coincident with the beginning of T2.</skos:definition>
        <skos:definition xml:lang="es">Si un intervalo propio T1 se encuentra con otro intervalo propio T2, entonces el final de T1 coincide con el principio de T2.</skos:definition>
    </owl:ObjectProperty>
    


    <!-- http://www.w3.org/2006/time#intervalMetBy -->


    <owl:ObjectProperty rdf:about="http://www.w3.org/2006/time#intervalMetBy">
        <rdfs:domain rdf:resource="http://www.w3.org/2006/time#ProperInterval"/>
        <rdfs:range rdf:resource="http://www.w3.org/2006/time#ProperInterval"/>
        <rdfs:comment xml:lang="en">If a proper interval T1 is intervalMetBy another proper interval T2, then the beginning of T1 is coincident with the end of T2.</rdfs:comment>
        <rdfs:comment xml:lang="es">Si un intervalo propio T1 es &apos;intervalo encontrado por&apos; otro intervalo propio T2, entonces el principio de T1 coincide con el final de T2.</rdfs:comment>
        <rdfs:label xml:lang="en">interval met by</rdfs:label>
        <rdfs:label xml:lang="es">intervalo encontrado por</rdfs:label>
        <skos:definition xml:lang="en">If a proper interval T1 is intervalMetBy another proper interval T2, then the beginning of T1 is coincident with the end of T2.</skos:definition>
        <skos:definition xml:lang="es">Si un intervalo propio T1 es &apos;intervalo encontrado por&apos; otro intervalo propio T2, entonces el principio de T1 coincide con el final de T2.</skos:definition>
    </owl:ObjectProperty>
    


    <!-- http://www.w3.org/2006/time#intervalOverlappedBy -->


    <owl:ObjectProperty rdf:about="http://www.w3.org/2006/time#intervalOverlappedBy">
        <owl:inverseOf rdf:resource="http://www.w3.org/2006/time#intervalOverlaps"/>
        <rdfs:domain rdf:resource="http://www.w3.org/2006/time#ProperInterval"/>
        <rdfs:range rdf:resource="http://www.w3.org/2006/time#ProperInterval"/>
        <rdfs:comment xml:lang="en">If a proper interval T1 is intervalOverlappedBy another proper interval T2, then the beginning of T1 is after the beginning of T2, the beginning of T1 is before the end of T2, and the end of T1 is after the end of T2.</rdfs:comment>
        <rdfs:comment xml:lang="es">Si un intervalo propio T1 es &apos;intervalo solapado por&apos; otro intervalo propio T2, entonces el principio de T1 es posterior al principio de T2, y el principio de T1 es anterior al final de T2, y el final de T1 es posterior al final de T2.</rdfs:comment>
        <rdfs:label xml:lang="en">interval overlapped by</rdfs:label>
        <rdfs:label xml:lang="es">intervalo solapado por</rdfs:label>
        <skos:definition xml:lang="en">If a proper interval T1 is intervalOverlappedBy another proper interval T2, then the beginning of T1 is after the beginning of T2, the beginning of T1 is before the end of T2, and the end of T1 is after the end of T2.</skos:definition>
        <skos:definition xml:lang="es">Si un intervalo propio T1 es &apos;intervalo solapado por&apos; otro intervalo propio T2, entonces el principio de T1 es posterior al principio de T2, y el principio de T1 es anterior al final de T2, y el final de T1 es posterior al final de T2.</skos:definition>
    </owl:ObjectProperty>
    


    <!-- http://www.w3.org/2006/time#intervalOverlaps -->


    <owl:ObjectProperty rdf:about="http://www.w3.org/2006/time#intervalOverlaps">
        <rdfs:domain rdf:resource="http://www.w3.org/2006/time#ProperInterval"/>
        <rdfs:range rdf:resource="http://www.w3.org/2006/time#ProperInterval"/>
        <rdfs:comment xml:lang="es">Asume una dirección en el tiempo. Si una entidad temporal T1 está después de otra entidad temporal T2, entonces el principio de T1 está después del final de T2.</rdfs:comment>
        <rdfs:comment xml:lang="en">If a proper interval T1 is intervalOverlaps another proper interval T2, then the beginning of T1 is before the beginning of T2, the end of T1 is after the beginning of T2, and the end of T1 is before the end of T2.</rdfs:comment>
        <rdfs:comment xml:lang="es">Si un intervalo propio T1 se solapa con otro intervalo propio T2, entonces el principio de T1 es anterior al principio de T2, el final de T1 es posterior al principio de T2, y el final de T1 es anterior al final de T2.</rdfs:comment>
        <rdfs:label xml:lang="en">interval overlaps</rdfs:label>
        <rdfs:label xml:lang="es">intervalo se solapa</rdfs:label>
        <skos:definition xml:lang="en">If a proper interval T1 is intervalOverlaps another proper interval T2, then the beginning of T1 is before the beginning of T2, the end of T1 is after the beginning of T2, and the end of T1 is before the end of T2.</skos:definition>
        <skos:definition xml:lang="es">Si un intervalo propio T1 se solapa con otro intervalo propio T2, entonces el principio de T1 es anterior al principio de T2, el final de T1 es posterior al principio de T2, y el final de T1 es anterior al final de T2.</skos:definition>
    </owl:ObjectProperty>
    


    <!-- http://www.w3.org/2006/time#intervalStartedBy -->


    <owl:ObjectProperty rdf:about="http://www.w3.org/2006/time#intervalStartedBy">
        <owl:inverseOf rdf:resource="http://www.w3.org/2006/time#intervalStarts"/>
        <rdfs:domain rdf:resource="http://www.w3.org/2006/time#ProperInterval"/>
        <rdfs:range rdf:resource="http://www.w3.org/2006/time#ProperInterval"/>
        <rdfs:comment xml:lang="en">If a proper interval T1 is intervalStarted another proper interval T2, then the beginning of T1 is coincident with the beginning of T2, and the end of T1 is after the end of T2.</rdfs:comment>
        <rdfs:comment xml:lang="es">Si un intervalo propio T1 es empezado por otro intervalo propio T2, entonces el principio de T1 coincide con el principio de T2, y el final de T1 es posterior al final de T2.</rdfs:comment>
        <rdfs:label xml:lang="en">interval started by</rdfs:label>
        <skos:definition xml:lang="en">If a proper interval T1 is intervalStarted another proper interval T2, then the beginning of T1 is coincident with the beginning of T2, and the end of T1 is after the end of T2.</skos:definition>
        <skos:definition xml:lang="es">Si un intervalo propio T1 es empezado por otro intervalo propio T2, entonces el principio de T1 coincide con el principio de T2, y el final de T1 es posterior al final de T2.</skos:definition>
    </owl:ObjectProperty>
    


    <!-- http://www.w3.org/2006/time#intervalStarts -->


    <owl:ObjectProperty rdf:about="http://www.w3.org/2006/time#intervalStarts">
        <rdfs:subPropertyOf rdf:resource="http://www.w3.org/2006/time#intervalIn"/>
        <rdfs:domain rdf:resource="http://www.w3.org/2006/time#ProperInterval"/>
        <rdfs:range rdf:resource="http://www.w3.org/2006/time#ProperInterval"/>
        <rdfs:comment xml:lang="en">If a proper interval T1 is intervalStarts another proper interval T2, then the beginning of T1 is coincident with the beginning of T2, and the end of T1 is before the end of T2.</rdfs:comment>
        <rdfs:comment xml:lang="es">Si un intervalo propio T1 empieza otro intervalo propio T2, entonces del principio de T1 con el principio de T2, y el final de T1 es anterior al final de T2.</rdfs:comment>
        <rdfs:label xml:lang="en">interval starts</rdfs:label>
        <rdfs:label xml:lang="es">intervalo empieza</rdfs:label>
        <skos:definition xml:lang="en">If a proper interval T1 is intervalStarts another proper interval T2, then the beginning of T1 is coincident with the beginning of T2, and the end of T1 is before the end of T2.</skos:definition>
        <skos:definition xml:lang="es">Si un intervalo propio T1 empieza otro intervalo propio T2, entonces del principio de T1 con el final de T2, y el final de T1 es anterior al final de T2.</skos:definition>
    </owl:ObjectProperty>
    


    <!-- http://www.w3.org/2006/time#monthOfYear -->


    <owl:ObjectProperty rdf:about="http://www.w3.org/2006/time#monthOfYear">
        <rdfs:domain rdf:resource="http://www.w3.org/2006/time#GeneralDateTimeDescription"/>
        <rdfs:range rdf:resource="http://www.w3.org/2006/time#MonthOfYear"/>
        <rdfs:comment xml:lang="es">El mes del año, cuyo valor es un miembro de la clase &apos;mes del año&apos;.</rdfs:comment>
        <rdfs:comment xml:lang="en">The month of the year, whose value is a member of the class time:MonthOfYear</rdfs:comment>
        <rdfs:label xml:lang="es">mes del año</rdfs:label>
        <rdfs:label xml:lang="en">month of year</rdfs:label>
        <skos:definition xml:lang="es">El mes del año, cuyo valor es un miembro de la clase &apos;mes del año&apos;.</skos:definition>
        <skos:definition xml:lang="en">The month of the year, whose value is a member of the class time:MonthOfYear</skos:definition>
        <skos:editorialNote xml:lang="es">Característica arriesgada - añadida en la revisión de 2017, y todavía no ampliamente utilizada.</skos:editorialNote>
        <skos:editorialNote xml:lang="en">Feature at risk - added in 2017 revision, and not yet widely used. </skos:editorialNote>
    </owl:ObjectProperty>
    


    <!-- http://www.w3.org/2006/time#timeZone -->


    <owl:ObjectProperty rdf:about="http://www.w3.org/2006/time#timeZone">
        <rdfs:domain rdf:resource="http://www.w3.org/2006/time#GeneralDateTimeDescription"/>
        <rdfs:range rdf:resource="http://www.w3.org/2006/time#TimeZone"/>
        <rdfs:comment xml:lang="en">The time zone for clock elements in the temporal position</rdfs:comment>
        <rdfs:label xml:lang="es">en huso horario</rdfs:label>
        <rdfs:label xml:lang="en">in time zone</rdfs:label>
        <skos:historyNote xml:lang="es">En la versión original de OWL-Time de 2006, el rango de &apos;en huso horario&apos; se definió en un espacio de nombres diferente &quot;http://www.w3.org/2006/timezone#&quot;.
            Un axioma de alineación permite que los datos codificados de acuerdo con la versión anterior sean consistentes con la ontología actualizada.</skos:historyNote>
        <skos:historyNote>In the original 2006 version of OWL-Time, the range of time:timeZone was a TimeZone class in a separate namespace &quot;http://www.w3.org/2006/timezone#&quot;. 
An alignment axiom 
	tzont:TimeZone rdfs:subClassOf time:TimeZone . 
allows data encoded according to the previous version to be consistent with the updated ontology. </skos:historyNote>
        <skos:note xml:lang="es">IANA mantiene una base de datos de husos horarios. Éstas están bien mantenidas y generalmente se consideran autorizadas, pero los ítems individuales no están disponibles en URIs individuales, por tanto, no se pueden utilizar directamente en datos expresados utilizando OWL-Time.
            La BDPedia proporciona un conjunto de recursos correspondientes a los husos horarios de IANA, con una URI para cada uno (por ejemplo, http://dbpedia.org/resource/Australia/Eucla). El Servicio de Reloj Mundial también proporciona una lista de husos horarios con la descripción de cada uno de los disponibles como una página Web individual con una URI adecuada individual (por ejemplo, https://www.timeanddate.com/time/zones/acwst). Éstos, y otros recursos similares, se puden usar como un valor de la propiedad &apos;huso horario&apos;.</skos:note>
        <skos:note>IANA maintains a database of timezones. These are well maintained and generally considered authoritative, but individual items are not available at individual URIs, so cannot be used directly in data expressed using OWL-Time.

DBPedia provides a set of resources corresponding to the IANA timezones, with a URI for each (e.g. http://dbpedia.org/resource/Australia/Eucla). The World Clock service also provides a list of time zones with the description of each available as an individual webpage with a convenient individual URI (e.g. https://www.timeanddate.com/time/zones/acwst). These or other, similar, resources might be used as a value of the time:timeZone property.</skos:note>
    </owl:ObjectProperty>
    


    <!-- http://www.w3.org/2006/time#unitType -->


    <owl:ObjectProperty rdf:about="http://www.w3.org/2006/time#unitType">
        <rdfs:domain>
            <owl:Class>
                <owl:unionOf rdf:parseType="Collection">
                    <rdf:Description rdf:about="http://www.w3.org/2006/time#Duration"/>
                    <rdf:Description rdf:about="http://www.w3.org/2006/time#GeneralDateTimeDescription"/>
                </owl:unionOf>
            </owl:Class>
        </rdfs:domain>
        <rdfs:range rdf:resource="http://www.w3.org/2006/time#TemporalUnit"/>
        <rdfs:comment xml:lang="es">La unidad de tiempo que proporciona la precisión de un valor fecha-hora o la escala de una extensión temporal.</rdfs:comment>
        <rdfs:comment xml:lang="en">The temporal unit which provides the precision of a date-time value or scale of a temporal extent</rdfs:comment>
        <rdfs:label xml:lang="en">temporal unit type</rdfs:label>
        <rdfs:label xml:lang="es">tipo de unidad temporal</rdfs:label>
    </owl:ObjectProperty>
    


    <!-- http://www.w3.org/ns/sosa/hosts -->


    <owl:ObjectProperty rdf:about="http://www.w3.org/ns/sosa/hosts">
        <owl:inverseOf rdf:resource="http://www.w3.org/ns/sosa/isHostedBy"/>
        <rdfs:comment xml:lang="en">Relation between a platform and the systems it hosts.</rdfs:comment>
        <rdfs:isDefinedBy rdf:resource="http://www.w3.org/ns/sosa/"/>
        <rdfs:label xml:lang="en">host</rdfs:label>
    </owl:ObjectProperty>
    


    <!-- http://www.w3.org/ns/sosa/isHostedBy -->


    <owl:ObjectProperty rdf:about="http://www.w3.org/ns/sosa/isHostedBy">
        <rdfs:comment xml:lang="en">Relation between a system and its hosting platform.</rdfs:comment>
        <rdfs:isDefinedBy rdf:resource="http://www.w3.org/ns/sosa/"/>
        <rdfs:label xml:lang="en">is hosted by</rdfs:label>
    </owl:ObjectProperty>
    


    <!-- http://www.w3.org/ns/ssn/deployedOnPlatform -->


    <owl:ObjectProperty rdf:about="http://www.w3.org/ns/ssn/deployedOnPlatform">
        <owl:inverseOf rdf:resource="http://www.w3.org/ns/ssn/inDeployment"/>
        <rdfs:comment xml:lang="en">Relation between a deployment and the platform(s) involved in the deployment.</rdfs:comment>
        <rdfs:isDefinedBy rdf:resource="http://www.w3.org/ns/ssn/"/>
        <rdfs:label xml:lang="en">deployed on platform</rdfs:label>
    </owl:ObjectProperty>
    


    <!-- http://www.w3.org/ns/ssn/deployedSystem -->


    <owl:ObjectProperty rdf:about="http://www.w3.org/ns/ssn/deployedSystem">
        <owl:inverseOf rdf:resource="http://www.w3.org/ns/ssn/hasDeployment"/>
        <rdfs:comment xml:lang="en">Relation between a deployment and the system deployed.</rdfs:comment>
        <rdfs:isDefinedBy rdf:resource="http://www.w3.org/ns/ssn/"/>
        <rdfs:label xml:lang="en">deployed system</rdfs:label>
    </owl:ObjectProperty>
    


    <!-- http://www.w3.org/ns/ssn/hasDeployment -->


    <owl:ObjectProperty rdf:about="http://www.w3.org/ns/ssn/hasDeployment">
        <rdfs:isDefinedBy rdf:resource="http://www.w3.org/ns/ssn/"/>
        <rdfs:label xml:lang="en">has deployment</rdfs:label>
    </owl:ObjectProperty>
    


    <!-- http://www.w3.org/ns/ssn/hasSubSystem -->


    <owl:ObjectProperty rdf:about="http://www.w3.org/ns/ssn/hasSubSystem">
        <rdfs:isDefinedBy rdf:resource="http://www.w3.org/ns/ssn/"/>
        <rdfs:label xml:lang="en">has subsystem</rdfs:label>
    </owl:ObjectProperty>
    


    <!-- http://www.w3.org/ns/ssn/inDeployment -->


    <owl:ObjectProperty rdf:about="http://www.w3.org/ns/ssn/inDeployment">
        <rdfs:comment xml:lang="en">Relation between a platform and the deployment(s) that takes place in the platform.</rdfs:comment>
        <rdfs:isDefinedBy rdf:resource="http://www.w3.org/ns/ssn/"/>
        <rdfs:label xml:lang="en">in deployment</rdfs:label>
    </owl:ObjectProperty>
    


    <!-- http://xmlns.com/foaf/0.1/based_near -->


    <owl:ObjectProperty rdf:about="http://xmlns.com/foaf/0.1/based_near"/>
    


    <!-- http://xmlns.com/foaf/0.1/member -->


    <owl:ObjectProperty rdf:about="http://xmlns.com/foaf/0.1/member">
        <rdfs:label xml:lang="en">member</rdfs:label>
    </owl:ObjectProperty>
    


    <!-- https://saref.etsi.org/core/accomplishes -->


    <owl:ObjectProperty rdf:about="https://saref.etsi.org/core/accomplishes">
        <owl:inverseOf rdf:resource="https://saref.etsi.org/core/isAccomplishedBy"/>
        <rdfs:range rdf:resource="https://saref.etsi.org/core/Task"/>
        <rdfs:comment xml:lang="en">A relationship between a certain entity (e.g., a device) and the task it accomplishes</rdfs:comment>
        <rdfs:isDefinedBy rdf:resource="https://saref.etsi.org/core/"/>
        <rdfs:label xml:lang="en">accomplishes</rdfs:label>
    </owl:ObjectProperty>
    


    <!-- https://saref.etsi.org/core/actsUpon -->


    <owl:ObjectProperty rdf:about="https://saref.etsi.org/core/actsUpon">
        <rdfs:domain rdf:resource="https://saref.etsi.org/core/Command"/>
        <rdfs:range rdf:resource="https://saref.etsi.org/core/State"/>
        <rdfs:comment xml:lang="en">A relationship between a command and a state</rdfs:comment>
        <rdfs:isDefinedBy rdf:resource="https://saref.etsi.org/core/"/>
        <rdfs:label xml:lang="en">acts upon</rdfs:label>
    </owl:ObjectProperty>
    


    <!-- https://saref.etsi.org/core/consistsOf -->


    <owl:ObjectProperty rdf:about="https://saref.etsi.org/core/consistsOf">
        <rdfs:comment xml:lang="en">A relationship indicating a composite entity that consists of other entities (e.g., a temperature/humidity sensor that consists of a temperature sensor and a humidity sensor)</rdfs:comment>
        <rdfs:label xml:lang="en">consists of</rdfs:label>
    </owl:ObjectProperty>
    


    <!-- https://saref.etsi.org/core/controlsProperty -->


    <owl:ObjectProperty rdf:about="https://saref.etsi.org/core/controlsProperty">
        <rdfs:domain rdf:resource="https://saref.etsi.org/core/Device"/>
        <rdfs:range rdf:resource="https://saref.etsi.org/core/Property"/>
        <rdfs:comment xml:lang="en">A relationship specifying the property that can be controlled by a certain device</rdfs:comment>
        <rdfs:isDefinedBy rdf:resource="https://saref.etsi.org/core/"/>
        <rdfs:label xml:lang="en">controls property</rdfs:label>
    </owl:ObjectProperty>
    


    <!-- https://saref.etsi.org/core/hasCommand -->


    <owl:ObjectProperty rdf:about="https://saref.etsi.org/core/hasCommand">
        <owl:inverseOf rdf:resource="https://saref.etsi.org/core/isCommandOf"/>
        <rdfs:domain rdf:resource="https://saref.etsi.org/core/Function"/>
        <rdfs:range rdf:resource="https://saref.etsi.org/core/Command"/>
        <rdfs:comment xml:lang="en">A relationship between a function and a command</rdfs:comment>
        <rdfs:comment xml:lang="en">A relationship between an entity (such as a function) and a command</rdfs:comment>
        <rdfs:isDefinedBy rdf:resource="https://saref.etsi.org/core/"/>
        <rdfs:label xml:lang="en">has command</rdfs:label>
    </owl:ObjectProperty>
    


    <!-- https://saref.etsi.org/core/hasFunction -->


    <owl:ObjectProperty rdf:about="https://saref.etsi.org/core/hasFunction">
        <rdfs:domain rdf:resource="https://saref.etsi.org/core/Device"/>
        <rdfs:range rdf:resource="https://saref.etsi.org/core/Function"/>
        <rdfs:comment xml:lang="en">A relationship identifying the function of a device</rdfs:comment>
        <rdfs:comment xml:lang="en">A relationship identifying the type of function of a device</rdfs:comment>
        <rdfs:isDefinedBy rdf:resource="https://saref.etsi.org/core/"/>
        <rdfs:label xml:lang="en">has function</rdfs:label>
    </owl:ObjectProperty>
    


    <!-- https://saref.etsi.org/core/hasMeasurement -->


    <owl:ObjectProperty rdf:about="https://saref.etsi.org/core/hasMeasurement">
        <owl:inverseOf rdf:resource="https://saref.etsi.org/core/isMeasurementOf"/>
        <rdfs:domain rdf:resource="https://saref.etsi.org/core/FeatureOfInterest"/>
        <rdfs:range rdf:resource="https://saref.etsi.org/core/Measurement"/>
        <rdfs:comment xml:lang="en">A relationship between a feature of interest and a measurement about it</rdfs:comment>
        <rdfs:comment xml:lang="en">Relation betwwen a feature of interest and the measurments that are about it.</rdfs:comment>
        <rdfs:isDefinedBy rdf:resource="https://saref.etsi.org/core/"/>
        <rdfs:label xml:lang="en">has measurement</rdfs:label>
        <rdfs:label xml:lang="en">is feature of interest of</rdfs:label>
    </owl:ObjectProperty>
    


    <!-- https://saref.etsi.org/core/hasMeterReading -->


    <owl:ObjectProperty rdf:about="https://saref.etsi.org/core/hasMeterReading">
        <rdfs:domain rdf:resource="https://saref.etsi.org/core/MeteringFunction"/>
        <rdfs:range rdf:resource="https://saref.etsi.org/core/Measurement"/>
        <rdfs:comment xml:lang="en">A relationship between a metering function and the measurement of the reading</rdfs:comment>
        <rdfs:label xml:lang="en">has meter reading</rdfs:label>
    </owl:ObjectProperty>
    


    <!-- https://saref.etsi.org/core/hasMeterReadingType -->


    <owl:ObjectProperty rdf:about="https://saref.etsi.org/core/hasMeterReadingType">
        <rdfs:domain rdf:resource="https://saref.etsi.org/core/MeteringFunction"/>
        <rdfs:range rdf:resource="https://saref.etsi.org/core/Property"/>
        <rdfs:comment xml:lang="en">A relationship identifying the reading type of a metering function (e.g., Water, Gas, Pressure , Energy , Power, etc.)</rdfs:comment>
        <rdfs:label xml:lang="en">has meter reading type</rdfs:label>
    </owl:ObjectProperty>
    


    <!-- https://saref.etsi.org/core/hasPrice -->


    <owl:ObjectProperty rdf:about="https://saref.etsi.org/core/hasPrice">
        <rdfs:range rdf:resource="https://saref.etsi.org/core/Price"/>
        <rdfs:comment xml:lang="en">A relationship indentifying the price associated to an entity</rdfs:comment>
        <rdfs:label xml:lang="en">has price</rdfs:label>
    </owl:ObjectProperty>
    


    <!-- https://saref.etsi.org/core/hasProfile -->


    <owl:ObjectProperty rdf:about="https://saref.etsi.org/core/hasProfile">
        <rdfs:domain rdf:resource="https://saref.etsi.org/core/Device"/>
        <rdfs:range rdf:resource="https://saref.etsi.org/core/Profile"/>
        <rdfs:comment xml:lang="en">A relationship associating a profile to a certain device</rdfs:comment>
        <rdfs:label xml:lang="en">has profile</rdfs:label>
    </owl:ObjectProperty>
    


    <!-- https://saref.etsi.org/core/hasProperty -->


    <owl:ObjectProperty rdf:about="https://saref.etsi.org/core/hasProperty">
        <owl:inverseOf rdf:resource="https://saref.etsi.org/core/isPropertyOf"/>
        <rdfs:domain rdf:resource="https://saref.etsi.org/core/FeatureOfInterest"/>
        <rdfs:range rdf:resource="https://saref.etsi.org/core/Property"/>
        <rdfs:comment xml:lang="en">A relationship between a feature of interest and a property of that feature</rdfs:comment>
        <rdfs:comment xml:lang="en">Relation between a feature of interest and its properties.</rdfs:comment>
        <rdfs:isDefinedBy rdf:resource="https://saref.etsi.org/core/"/>
        <rdfs:label xml:lang="en">has property</rdfs:label>
    </owl:ObjectProperty>
    


    <!-- https://saref.etsi.org/core/hasSensingRange -->


    <owl:ObjectProperty rdf:about="https://saref.etsi.org/core/hasSensingRange">
        <rdfs:domain rdf:resource="https://saref.etsi.org/core/SensingFunction"/>
        <rdfs:range rdf:resource="https://saref.etsi.org/core/Measurement"/>
        <rdfs:comment xml:lang="en">A relationship between a sensing function and a measurement identifying the range of a sensor detection</rdfs:comment>
        <rdfs:label xml:lang="en">has sensing range</rdfs:label>
    </owl:ObjectProperty>
    


    <!-- https://saref.etsi.org/core/hasSensorType -->


    <owl:ObjectProperty rdf:about="https://saref.etsi.org/core/hasSensorType">
        <rdfs:domain rdf:resource="https://saref.etsi.org/core/SensingFunction"/>
        <rdfs:range rdf:resource="https://saref.etsi.org/core/Property"/>
        <rdfs:comment xml:lang="en">A relationship identifying the sensing type of a sensor detection (i.e., Temperature, Occupancy, Humidity, Motion , Smoke, Pressure, etc.) </rdfs:comment>
        <rdfs:label xml:lang="en">has sensor type</rdfs:label>
    </owl:ObjectProperty>
    


    <!-- https://saref.etsi.org/core/hasState -->


    <owl:ObjectProperty rdf:about="https://saref.etsi.org/core/hasState">
        <rdfs:domain rdf:resource="https://saref.etsi.org/core/Device"/>
        <rdfs:range rdf:resource="https://saref.etsi.org/core/State"/>
        <rdfs:comment xml:lang="en">A relationship identifying the type of state of a device</rdfs:comment>
        <rdfs:isDefinedBy rdf:resource="https://saref.etsi.org/core/"/>
        <rdfs:label xml:lang="en">has state</rdfs:label>
    </owl:ObjectProperty>
    


    <!-- https://saref.etsi.org/core/hasThresholdMeasurement -->


    <owl:ObjectProperty rdf:about="https://saref.etsi.org/core/hasThresholdMeasurement">
        <rdfs:domain rdf:resource="https://saref.etsi.org/core/EventFunction"/>
        <rdfs:range rdf:resource="https://saref.etsi.org/core/Measurement"/>
        <rdfs:comment xml:lang="en">A relationship associated with an event function to notify that a certain threshold measurement has been exceeded</rdfs:comment>
        <rdfs:label xml:lang="en">has threshold measurement</rdfs:label>
    </owl:ObjectProperty>
    


    <!-- https://saref.etsi.org/core/hasTime -->


    <owl:ObjectProperty rdf:about="https://saref.etsi.org/core/hasTime">
        <rdfs:range rdf:resource="https://saref.etsi.org/core/Time"/>
        <rdfs:comment xml:lang="en">A relationship to associate time information to an entity</rdfs:comment>
        <rdfs:label xml:lang="en">has time</rdfs:label>
    </owl:ObjectProperty>
    


    <!-- https://saref.etsi.org/core/hasTypicalConsumption -->


    <owl:ObjectProperty rdf:about="https://saref.etsi.org/core/hasTypicalConsumption">
        <rdfs:comment xml:lang="en">A relationship identifying the typical (energy or power) consumption of a device</rdfs:comment>
        <rdfs:label xml:lang="en">has typical consumption</rdfs:label>
    </owl:ObjectProperty>
    


    <!-- https://saref.etsi.org/core/isAbout -->


    <owl:ObjectProperty rdf:about="https://saref.etsi.org/core/isAbout">
        <rdfs:comment xml:lang="en">A relationship identifying what an entity, such as a profile, is about</rdfs:comment>
        <rdfs:label xml:lang="en">isAbout</rdfs:label>
    </owl:ObjectProperty>
    


    <!-- https://saref.etsi.org/core/isAccomplishedBy -->


    <owl:ObjectProperty rdf:about="https://saref.etsi.org/core/isAccomplishedBy">
        <rdfs:domain rdf:resource="https://saref.etsi.org/core/Task"/>
        <rdfs:comment xml:lang="en">A relationship identifying an entity (e.g., a device) that can accomplish a task.</rdfs:comment>
        <rdfs:comment xml:lang="en">A relationship indentifying the task accomplished by a certain entity (e.g., a device)</rdfs:comment>
        <rdfs:isDefinedBy rdf:resource="https://saref.etsi.org/core/"/>
        <rdfs:label xml:lang="en">is accomplished by</rdfs:label>
    </owl:ObjectProperty>
    


    <!-- https://saref.etsi.org/core/isCommandOf -->


    <owl:ObjectProperty rdf:about="https://saref.etsi.org/core/isCommandOf">
        <rdfs:domain rdf:resource="https://saref.etsi.org/core/Command"/>
        <rdfs:range rdf:resource="https://saref.etsi.org/core/Function"/>
        <rdfs:comment xml:lang="en">A relationship between a command and a function.</rdfs:comment>
        <rdfs:isDefinedBy rdf:resource="https://saref.etsi.org/core/"/>
        <rdfs:label xml:lang="en">is command of</rdfs:label>
    </owl:ObjectProperty>
    


    <!-- https://saref.etsi.org/core/isControlledByDevice -->


    <owl:ObjectProperty rdf:about="https://saref.etsi.org/core/isControlledByDevice">
        <rdfs:domain rdf:resource="https://saref.etsi.org/core/Property"/>
        <rdfs:range rdf:resource="https://saref.etsi.org/core/Device"/>
        <rdfs:comment xml:lang="en">A relationship specifying the devices that can control a certain property</rdfs:comment>
        <rdfs:isDefinedBy rdf:resource="https://saref.etsi.org/core/"/>
        <rdfs:label xml:lang="en">is controlled by device</rdfs:label>
    </owl:ObjectProperty>
    


    <!-- https://saref.etsi.org/core/isMeasuredByDevice -->


    <owl:ObjectProperty rdf:about="https://saref.etsi.org/core/isMeasuredByDevice">
        <rdfs:domain rdf:resource="https://saref.etsi.org/core/Property"/>
        <rdfs:range rdf:resource="https://saref.etsi.org/core/Device"/>
        <rdfs:comment xml:lang="en">A relationship specifying the devices that can measure a certain property</rdfs:comment>
        <rdfs:isDefinedBy rdf:resource="https://saref.etsi.org/core/"/>
        <rdfs:label xml:lang="en">is measured by device</rdfs:label>
    </owl:ObjectProperty>
    


    <!-- https://saref.etsi.org/core/isMeasuredIn -->


    <owl:ObjectProperty rdf:about="https://saref.etsi.org/core/isMeasuredIn">
        <rdfs:domain rdf:resource="https://saref.etsi.org/core/Measurement"/>
        <rdfs:range rdf:resource="https://saref.etsi.org/core/UnitOfMeasure"/>
        <rdfs:comment xml:lang="en">A relation between a measurement and the unit of measure in which the measurement value is expressed.</rdfs:comment>
        <rdfs:comment xml:lang="en">A relationship identifying the unit of measure used for a certain entity.</rdfs:comment>
        <rdfs:isDefinedBy rdf:resource="https://saref.etsi.org/core/"/>
        <rdfs:isDefinedBy>https://saref.etsi.org/core/</rdfs:isDefinedBy>
        <rdfs:label xml:lang="en">is measured in</rdfs:label>
    </owl:ObjectProperty>
    


    <!-- https://saref.etsi.org/core/isMeasurementOf -->


    <owl:ObjectProperty rdf:about="https://saref.etsi.org/core/isMeasurementOf">
        <rdfs:domain rdf:resource="https://saref.etsi.org/core/Measurement"/>
        <rdfs:range rdf:resource="https://saref.etsi.org/core/FeatureOfInterest"/>
        <rdfs:comment xml:lang="en">A relationship between a measurement and the feature of interest whose quality was measured</rdfs:comment>
        <rdfs:comment xml:lang="en">Relation between a measurement and the feature of interest being measured.</rdfs:comment>
        <rdfs:isDefinedBy rdf:resource="https://saref.etsi.org/core/"/>
        <rdfs:label xml:lang="en">has feature of interest</rdfs:label>
        <rdfs:label xml:lang="en">is measurement of</rdfs:label>
        <rdfs:label xml:lang="en">isMeasurementOf</rdfs:label>
    </owl:ObjectProperty>
    


    <!-- https://saref.etsi.org/core/isOfferedBy -->


    <owl:ObjectProperty rdf:about="https://saref.etsi.org/core/isOfferedBy">
        <owl:inverseOf rdf:resource="https://saref.etsi.org/core/offers"/>
        <rdfs:domain rdf:resource="https://saref.etsi.org/core/Service"/>
        <rdfs:range rdf:resource="https://saref.etsi.org/core/Device"/>
        <rdfs:comment xml:lang="en">A relationship between a service and a device that offers the service</rdfs:comment>
        <rdfs:label xml:lang="en">is offered by</rdfs:label>
    </owl:ObjectProperty>
    


    <!-- https://saref.etsi.org/core/isPropertyOf -->


    <owl:ObjectProperty rdf:about="https://saref.etsi.org/core/isPropertyOf">
        <rdfs:domain rdf:resource="https://saref.etsi.org/core/Property"/>
        <rdfs:range rdf:resource="https://saref.etsi.org/core/FeatureOfInterest"/>
        <rdfs:comment xml:lang="en">A relationship between a property and the feature of interest it belongs to</rdfs:comment>
        <rdfs:comment xml:lang="en">Relation between a property and a feature of interest in which such property appears.</rdfs:comment>
        <rdfs:isDefinedBy rdf:resource="https://saref.etsi.org/core/"/>
        <rdfs:label xml:lang="en">is property of</rdfs:label>
    </owl:ObjectProperty>
    


    <!-- https://saref.etsi.org/core/isUsedFor -->


    <owl:ObjectProperty rdf:about="https://saref.etsi.org/core/isUsedFor">
        <rdfs:comment xml:lang="en">A relationship specifying the commodity for which a device is used for</rdfs:comment>
        <rdfs:label xml:lang="en">is used for</rdfs:label>
    </owl:ObjectProperty>
    


    <!-- https://saref.etsi.org/core/makesMeasurement -->


    <owl:ObjectProperty rdf:about="https://saref.etsi.org/core/makesMeasurement">
        <owl:inverseOf rdf:resource="https://saref.etsi.org/core/measurementMadeBy"/>
        <rdfs:domain rdf:resource="https://saref.etsi.org/core/Device"/>
        <rdfs:range rdf:resource="https://saref.etsi.org/core/Measurement"/>
        <rdfs:comment xml:lang="en">A relation between a device and the measurements it makes. Such measurement will link together the value of the measurement, its unit of measure and the property to which it relates.</rdfs:comment>
        <rdfs:isDefinedBy rdf:resource="https://saref.etsi.org/core/"/>
        <rdfs:label xml:lang="en">makes measurement</rdfs:label>
    </owl:ObjectProperty>
    


    <!-- https://saref.etsi.org/core/measurementMadeBy -->


    <owl:ObjectProperty rdf:about="https://saref.etsi.org/core/measurementMadeBy">
        <rdfs:domain rdf:resource="https://saref.etsi.org/core/Measurement"/>
        <rdfs:range rdf:resource="https://saref.etsi.org/core/Device"/>
        <rdfs:comment xml:lang="en">A relation between a measurement and the device that made it.</rdfs:comment>
        <rdfs:comment xml:lang="en">Relation between a measurement and the device that made it.</rdfs:comment>
        <rdfs:isDefinedBy rdf:resource="https://saref.etsi.org/core/"/>
        <rdfs:label xml:lang="en">measurement made by</rdfs:label>
    </owl:ObjectProperty>
    


    <!-- https://saref.etsi.org/core/measuresProperty -->


    <owl:ObjectProperty rdf:about="https://saref.etsi.org/core/measuresProperty">
        <rdfs:domain rdf:resource="https://saref.etsi.org/core/Device"/>
        <rdfs:range rdf:resource="https://saref.etsi.org/core/Property"/>
        <rdfs:comment xml:lang="en">A relationship specifying the property that can be measured by a certain device</rdfs:comment>
        <rdfs:isDefinedBy rdf:resource="https://saref.etsi.org/core/"/>
        <rdfs:label xml:lang="en">measures property</rdfs:label>
    </owl:ObjectProperty>
    


    <!-- https://saref.etsi.org/core/offers -->


    <owl:ObjectProperty rdf:about="https://saref.etsi.org/core/offers">
        <rdfs:domain rdf:resource="https://saref.etsi.org/core/Device"/>
        <rdfs:range rdf:resource="https://saref.etsi.org/core/Service"/>
        <rdfs:comment xml:lang="en">A relationship between a device and a service</rdfs:comment>
        <rdfs:label xml:lang="en">offers</rdfs:label>
    </owl:ObjectProperty>
    


    <!-- https://saref.etsi.org/core/relatesToMeasurement -->


    <owl:ObjectProperty rdf:about="https://saref.etsi.org/core/relatesToMeasurement">
        <owl:inverseOf rdf:resource="https://saref.etsi.org/core/relatesToProperty"/>
        <rdfs:domain rdf:resource="https://saref.etsi.org/core/Property"/>
        <rdfs:range rdf:resource="https://saref.etsi.org/core/Measurement"/>
        <rdfs:comment xml:lang="en">A relationship between a property and the measurements it relates to</rdfs:comment>
        <rdfs:isDefinedBy rdf:resource="https://saref.etsi.org/core/"/>
        <rdfs:label xml:lang="en">relates to measurement</rdfs:label>
    </owl:ObjectProperty>
    


    <!-- https://saref.etsi.org/core/relatesToProperty -->


    <owl:ObjectProperty rdf:about="https://saref.etsi.org/core/relatesToProperty">
        <rdfs:domain rdf:resource="https://saref.etsi.org/core/Measurement"/>
        <rdfs:range rdf:resource="https://saref.etsi.org/core/Property"/>
        <rdfs:comment xml:lang="en">A relation between a measurement and the property such measurement is about.</rdfs:comment>
        <rdfs:comment xml:lang="en">A relationship between a measurement and the property it relates to</rdfs:comment>
        <rdfs:isDefinedBy rdf:resource="https://saref.etsi.org/core/"/>
        <rdfs:isDefinedBy>https://saref.etsi.org/core/</rdfs:isDefinedBy>
        <rdfs:label xml:lang="en">relates to property</rdfs:label>
    </owl:ObjectProperty>
    


    <!-- https://saref.etsi.org/core/represents -->


    <owl:ObjectProperty rdf:about="https://saref.etsi.org/core/represents">
        <rdfs:domain rdf:resource="https://saref.etsi.org/core/Service"/>
        <rdfs:range rdf:resource="https://saref.etsi.org/core/Function"/>
        <rdfs:comment xml:lang="en">A relationship between a service and a function.</rdfs:comment>
        <rdfs:label xml:lang="en">represents</rdfs:label>
    </owl:ObjectProperty>
    


    <!-- https://saref.etsi.org/saref4agri/contains -->


    <owl:ObjectProperty rdf:about="https://saref.etsi.org/saref4agri/contains">
        <rdfs:subPropertyOf rdf:resource="http://www.opengis.net/ont/geosparql#sfContains"/>
        <owl:inverseOf rdf:resource="https://saref.etsi.org/saref4agri/isContainedIn"/>
        <rdfs:comment xml:lang="en">contains</rdfs:comment>
        <rdfs:label xml:lang="en">contains</rdfs:label>
    </owl:ObjectProperty>
    


    <!-- https://saref.etsi.org/saref4agri/generates -->


    <owl:ObjectProperty rdf:about="https://saref.etsi.org/saref4agri/generates">
        <rdfs:subPropertyOf rdf:resource="https://saref.etsi.org/core/hasProperty"/>
        <rdfs:comment xml:lang="en">A relation to represent the yield generated by a Crop.</rdfs:comment>
        <rdfs:label xml:lang="en">generates</rdfs:label>
    </owl:ObjectProperty>
    


    <!-- https://saref.etsi.org/saref4agri/hasDeploymentPeriod -->


    <owl:ObjectProperty rdf:about="https://saref.etsi.org/saref4agri/hasDeploymentPeriod">
        <rdfs:comment xml:lang="en">Relation to indicate the temporal duration or period of a deployment.</rdfs:comment>
        <rdfs:comment xml:lang="en">has deployment period</rdfs:comment>
        <rdfs:label xml:lang="en">has deployment period</rdfs:label>
    </owl:ObjectProperty>
    


    <!-- https://saref.etsi.org/saref4agri/hasID -->


    <owl:ObjectProperty rdf:about="https://saref.etsi.org/saref4agri/hasID">
        <rdfs:subPropertyOf rdf:resource="http://www.w3.org/2002/07/owl#topObjectProperty"/>
        <rdfs:range rdf:resource="https://saref.etsi.org/saref4agri/ID"/>
        <rdfs:comment xml:lang="en">A relation to express the unique identifier of an animal.</rdfs:comment>
        <rdfs:label xml:lang="en">has id</rdfs:label>
    </owl:ObjectProperty>
    


    <!-- https://saref.etsi.org/saref4agri/hasMember -->


    <owl:ObjectProperty rdf:about="https://saref.etsi.org/saref4agri/hasMember">
        <owl:inverseOf rdf:resource="https://saref.etsi.org/saref4agri/isMemberOf"/>
        <rdfs:comment xml:lang="en">A relation to represent  the members of an AnimalGroup.</rdfs:comment>
        <rdfs:label xml:lang="en">has member</rdfs:label>
    </owl:ObjectProperty>
    


    <!-- https://saref.etsi.org/saref4agri/hasReceived -->


    <owl:ObjectProperty rdf:about="https://saref.etsi.org/saref4agri/hasReceived">
        <owl:inverseOf rdf:resource="https://saref.etsi.org/saref4agri/receives"/>
        <rdfs:comment xml:lang="en">has received</rdfs:comment>
        <rdfs:label xml:lang="en">has received</rdfs:label>
    </owl:ObjectProperty>
    


    <!-- https://saref.etsi.org/saref4agri/isContainedIn -->


    <owl:ObjectProperty rdf:about="https://saref.etsi.org/saref4agri/isContainedIn">
        <rdfs:comment xml:lang="en">is contained in</rdfs:comment>
        <rdfs:label xml:lang="en">is contained in</rdfs:label>
    </owl:ObjectProperty>
    


    <!-- https://saref.etsi.org/saref4agri/isDeployedAtSpace -->


    <owl:ObjectProperty rdf:about="https://saref.etsi.org/saref4agri/isDeployedAtSpace">
        <rdfs:comment xml:lang="en">Relation to indicate the geographical componet of a deployment.</rdfs:comment>
        <rdfs:comment xml:lang="en">is deployed at space</rdfs:comment>
        <rdfs:label xml:lang="en">is deployed at space</rdfs:label>
    </owl:ObjectProperty>
    


    <!-- https://saref.etsi.org/saref4agri/isLocatedIn -->


    <owl:ObjectProperty rdf:about="https://saref.etsi.org/saref4agri/isLocatedIn">
        <owl:inverseOf rdf:resource="https://saref.etsi.org/saref4agri/isLocationOf"/>
        <rdfs:comment xml:lang="en">A relation to express the physical location of a saref4agri entity (e.g., an animal)</rdfs:comment>
        <rdfs:label xml:lang="en">is located in</rdfs:label>
    </owl:ObjectProperty>
    


    <!-- https://saref.etsi.org/saref4agri/isLocationOf -->


    <owl:ObjectProperty rdf:about="https://saref.etsi.org/saref4agri/isLocationOf">
        <rdfs:comment xml:lang="en">is location of</rdfs:comment>
        <rdfs:label xml:lang="en">is location of</rdfs:label>
    </owl:ObjectProperty>
    


    <!-- https://saref.etsi.org/saref4agri/isMemberOf -->


    <owl:ObjectProperty rdf:about="https://saref.etsi.org/saref4agri/isMemberOf">
        <rdfs:comment xml:lang="en">A relation to express that an animal can be part of groups.</rdfs:comment>
        <rdfs:label xml:lang="en">is member of</rdfs:label>
    </owl:ObjectProperty>
    


    <!-- https://saref.etsi.org/saref4agri/managesFarm -->


    <owl:ObjectProperty rdf:about="https://saref.etsi.org/saref4agri/managesFarm">
        <rdfs:comment xml:lang="en">manages farm</rdfs:comment>
        <rdfs:label xml:lang="en">manages farm</rdfs:label>
    </owl:ObjectProperty>
    


    <!-- https://saref.etsi.org/saref4agri/receives -->


    <owl:ObjectProperty rdf:about="https://saref.etsi.org/saref4agri/receives">
        <rdfs:subPropertyOf rdf:resource="https://saref.etsi.org/core/hasMeasurement"/>
        <rdfs:comment xml:lang="en">A relation to represent the intake/consumption of certain substances in a Crop.</rdfs:comment>
        <rdfs:label xml:lang="en">receives</rdfs:label>
    </owl:ObjectProperty>
    


    <!-- https://saref.etsi.org/saref4bldg/airFlowRateMax -->


    <owl:ObjectProperty rdf:about="https://saref.etsi.org/saref4bldg/airFlowRateMax">
        <rdfs:comment xml:lang="en">Maximum allowable air flow rate. Usually measured in m3/s.</rdfs:comment>
        <rdfs:label xml:lang="en">air flow rate range max</rdfs:label>
    </owl:ObjectProperty>
    


    <!-- https://saref.etsi.org/saref4bldg/airFlowRateMin -->


    <owl:ObjectProperty rdf:about="https://saref.etsi.org/saref4bldg/airFlowRateMin">
        <rdfs:comment xml:lang="en">Minimum allowable air flow rate. Usually measured in m3/s.</rdfs:comment>
        <rdfs:label xml:lang="en">air flow rate range min</rdfs:label>
    </owl:ObjectProperty>
    


    <!-- https://saref.etsi.org/saref4bldg/ambientDesignDryBulbTemperature -->


    <owl:ObjectProperty rdf:about="https://saref.etsi.org/saref4bldg/ambientDesignDryBulbTemperature">
        <rdfs:comment xml:lang="en">Ambient design dry bulb temperature used for selecting the cooling tower. Usually measured in degrees Kelvin (K).</rdfs:comment>
        <rdfs:label xml:lang="en">ambient design dry bulb temperature</rdfs:label>
    </owl:ObjectProperty>
    


    <!-- https://saref.etsi.org/saref4bldg/ambientDesignWetBulbTemperature -->


    <owl:ObjectProperty rdf:about="https://saref.etsi.org/saref4bldg/ambientDesignWetBulbTemperature">
        <rdfs:comment xml:lang="en">Ambient design wet bulb temperature used for selecting the cooling tower. Usually measured in degrees Kelvin (K).</rdfs:comment>
        <rdfs:label xml:lang="en">ambient design wet bulb temperature</rdfs:label>
    </owl:ObjectProperty>
    


    <!-- https://saref.etsi.org/saref4bldg/apparentPowerMax -->


    <owl:ObjectProperty rdf:about="https://saref.etsi.org/saref4bldg/apparentPowerMax">
        <rdfs:comment xml:lang="en">Maximum apparent power/capacity in VA (volt ampere). Usually measured in Watts (W, J/s).</rdfs:comment>
        <rdfs:label xml:lang="en">maximum apparent power</rdfs:label>
    </owl:ObjectProperty>
    


    <!-- https://saref.etsi.org/saref4bldg/audioVolume -->


    <owl:ObjectProperty rdf:about="https://saref.etsi.org/saref4bldg/audioVolume">
        <rdfs:comment xml:lang="en">Indicates discrete audio volume levels and corresponding sound power offsets, if applicable. Missing values may be interpolated. Measured in watts.</rdfs:comment>
        <rdfs:label xml:lang="en">audio volume</rdfs:label>
    </owl:ObjectProperty>
    


    <!-- https://saref.etsi.org/saref4bldg/basinReserveVolume -->


    <owl:ObjectProperty rdf:about="https://saref.etsi.org/saref4bldg/basinReserveVolume">
        <rdfs:comment xml:lang="en">Volume between operating and overflow levels in cooling tower basin. Usually measured in cubic metre (m3).</rdfs:comment>
        <rdfs:label xml:lang="en">basin reserve volume</rdfs:label>
    </owl:ObjectProperty>
    


    <!-- https://saref.etsi.org/saref4bldg/bladeThickness -->


    <owl:ObjectProperty rdf:about="https://saref.etsi.org/saref4bldg/bladeThickness">
        <rdfs:comment xml:lang="en">The thickness of the damper blade. Usually measured in millimeters (mm).</rdfs:comment>
        <rdfs:label xml:lang="en">blade thickness</rdfs:label>
    </owl:ObjectProperty>
    


    <!-- https://saref.etsi.org/saref4bldg/bodyMass -->


    <owl:ObjectProperty rdf:about="https://saref.etsi.org/saref4bldg/bodyMass">
        <rdfs:comment xml:lang="en">Overall body mass of the heater. Usually measured in kilograms (kg) or grams (g).</rdfs:comment>
        <rdfs:label xml:lang="en">body mass</rdfs:label>
    </owl:ObjectProperty>
    


    <!-- https://saref.etsi.org/saref4bldg/capacityWeight -->


    <owl:ObjectProperty rdf:about="https://saref.etsi.org/saref4bldg/capacityWeight">
        <rdfs:comment xml:lang="en">Capacity of the transport element measured by weight. Usually measured in kilograms (kg) or grams (g).</rdfs:comment>
        <rdfs:label xml:lang="en">capacity weight</rdfs:label>
    </owl:ObjectProperty>
    


    <!-- https://saref.etsi.org/saref4bldg/closeOffRating -->


    <owl:ObjectProperty rdf:about="https://saref.etsi.org/saref4bldg/closeOffRating">
        <rdfs:comment xml:lang="en">Close off rating. Usually measured in Pascals (Pa, N/m2).</rdfs:comment>
        <rdfs:label xml:lang="en">close off rating</rdfs:label>
    </owl:ObjectProperty>
    


    <!-- https://saref.etsi.org/saref4bldg/coilLength -->


    <owl:ObjectProperty rdf:about="https://saref.etsi.org/saref4bldg/coilLength">
        <rdfs:comment xml:lang="en">Length of coil. Usually measured in millimeters (mm).</rdfs:comment>
        <rdfs:label xml:lang="en">coil length</rdfs:label>
    </owl:ObjectProperty>
    


    <!-- https://saref.etsi.org/saref4bldg/coilWidth -->


    <owl:ObjectProperty rdf:about="https://saref.etsi.org/saref4bldg/coilWidth">
        <rdfs:comment xml:lang="en">Width of coil. Usually measured in millimeters (mm</rdfs:comment>
        <rdfs:label xml:lang="en">coil width</rdfs:label>
    </owl:ObjectProperty>
    


    <!-- https://saref.etsi.org/saref4bldg/colorTemperature -->


    <owl:ObjectProperty rdf:about="https://saref.etsi.org/saref4bldg/colorTemperature">
        <rdfs:comment xml:lang="en">The color temperature of any source of radiation is defined as the temperature (in Kelvin) of a black-body or Planckian radiator whose radiation has the same chromaticity as the source of radiation. Often the values are only approximate color temperatures as the black-body radiator cannot emit radiation of every chromaticity value. The color temperatures of the commonest artificial light sources range from less than 3000K (warm white) to 4000K (intermediate) and over 5000K (daylight). Usually measured in degrees Kelvin (K).</rdfs:comment>
        <rdfs:label xml:lang="en">color temperature</rdfs:label>
    </owl:ObjectProperty>
    


    <!-- https://saref.etsi.org/saref4bldg/compressorSpeed -->


    <owl:ObjectProperty rdf:about="https://saref.etsi.org/saref4bldg/compressorSpeed">
        <rdfs:comment xml:lang="en">Compressor speed. Usually measured in cycles/s.</rdfs:comment>
        <rdfs:label xml:lang="en">compressor speed</rdfs:label>
    </owl:ObjectProperty>
    


    <!-- https://saref.etsi.org/saref4bldg/connectionSize -->


    <owl:ObjectProperty rdf:about="https://saref.etsi.org/saref4bldg/connectionSize">
        <rdfs:comment xml:lang="en">The connection size of the to and from the pump. Usually measured in millimeters (mm).</rdfs:comment>
        <rdfs:label xml:lang="en">connection size</rdfs:label>
    </owl:ObjectProperty>
    


    <!-- https://saref.etsi.org/saref4bldg/contains -->


    <owl:ObjectProperty rdf:about="https://saref.etsi.org/saref4bldg/contains">
        <owl:inverseOf rdf:resource="https://saref.etsi.org/saref4bldg/isContainedIn"/>
        <rdf:type rdf:resource="http://www.w3.org/2002/07/owl#TransitiveProperty"/>
        <rdfs:comment xml:lang="en">A relation between a physical space and the objects located in such space.</rdfs:comment>
        <rdfs:label xml:lang="en">contains</rdfs:label>
    </owl:ObjectProperty>
    


    <!-- https://saref.etsi.org/saref4bldg/contributedLuminousFlux -->


    <owl:ObjectProperty rdf:about="https://saref.etsi.org/saref4bldg/contributedLuminousFlux">
        <rdfs:comment xml:lang="en">Luminous flux is a photometric measure of radiant flux, i.e. the volume of light emitted from a light source. Luminous flux is measured either for the interior as a whole or for a part of the interior (partial luminous flux for a solid angle). All other photometric parameters are derivatives of luminous flux. Luminous flux is measured in lumens (lm). The luminous flux is given as a nominal value for each lamp. Usually measured in Lumen (lm, Candela Steradian).</rdfs:comment>
        <rdfs:label xml:lang="en">contributed luminous flux</rdfs:label>
    </owl:ObjectProperty>
    


    <!-- https://saref.etsi.org/saref4bldg/coverLength -->


    <owl:ObjectProperty rdf:about="https://saref.etsi.org/saref4bldg/coverLength">
        <rdfs:comment xml:lang="en">The length measured along the x-axis in the local coordinate system or the radius (in the case of a circular shape in plan) of the cover of the oil interceptor. Usually measured in millimeters (mm).</rdfs:comment>
        <rdfs:label xml:lang="en">cover length</rdfs:label>
    </owl:ObjectProperty>
    


    <!-- https://saref.etsi.org/saref4bldg/coverWidth -->


    <owl:ObjectProperty rdf:about="https://saref.etsi.org/saref4bldg/coverWidth">
        <rdfs:comment xml:lang="en">The length measured along the x-axis in the local coordinate system of the cover of the oil interceptor. Usually measured in millimeters (mm).</rdfs:comment>
        <rdfs:label xml:lang="en">cover width</rdfs:label>
    </owl:ObjectProperty>
    


    <!-- https://saref.etsi.org/saref4bldg/effectiveCapacity -->


    <owl:ObjectProperty rdf:about="https://saref.etsi.org/saref4bldg/effectiveCapacity">
        <rdfs:comment xml:lang="en">The total effective or actual volumetric capacity of the tank. Usually measured in cubic metre (m3).B3</rdfs:comment>
        <rdfs:label xml:lang="en">effective capacity</rdfs:label>
    </owl:ObjectProperty>
    


    <!-- https://saref.etsi.org/saref4bldg/electricGeneratorEfficiency -->


    <owl:ObjectProperty rdf:about="https://saref.etsi.org/saref4bldg/electricGeneratorEfficiency">
        <rdfs:comment xml:lang="en">The ratio of output capacity to intake capacity.</rdfs:comment>
        <rdfs:label xml:lang="en">electric generator efficiency</rdfs:label>
    </owl:ObjectProperty>
    


    <!-- https://saref.etsi.org/saref4bldg/electricMotorEfficiency -->


    <owl:ObjectProperty rdf:about="https://saref.etsi.org/saref4bldg/electricMotorEfficiency">
        <rdfs:comment xml:lang="en">The ratio of output capacity to intake capacity.</rdfs:comment>
        <rdfs:label xml:lang="en">electric motor efficiency</rdfs:label>
    </owl:ObjectProperty>
    


    <!-- https://saref.etsi.org/saref4bldg/externalSurfaceArea -->


    <owl:ObjectProperty rdf:about="https://saref.etsi.org/saref4bldg/externalSurfaceArea">
        <rdfs:comment xml:lang="en">External surface area (both primary and secondary area). Usually measured in square metre (m2).</rdfs:comment>
        <rdfs:label xml:lang="en">external surface area</rdfs:label>
    </owl:ObjectProperty>
    


    <!-- https://saref.etsi.org/saref4bldg/faceArea -->


    <owl:ObjectProperty rdf:about="https://saref.etsi.org/saref4bldg/faceArea">
        <rdfs:comment xml:lang="en">Face area open to the airstream. Usually measured in square metre (m2).</rdfs:comment>
        <rdfs:label xml:lang="en">face area</rdfs:label>
    </owl:ObjectProperty>
    


    <!-- https://saref.etsi.org/saref4bldg/finalResistance -->


    <owl:ObjectProperty rdf:about="https://saref.etsi.org/saref4bldg/finalResistance">
        <rdfs:comment xml:lang="en">Filter fluid resistance when replacement is required (i.e., Pressure drop at the maximum air flowrate across the filter when the filter needs replacement per ASHRAE Standard 52.1). Usually measured in Pascals (Pa, N/m2).</rdfs:comment>
        <rdfs:label xml:lang="en">final resistance</rdfs:label>
    </owl:ObjectProperty>
    


    <!-- https://saref.etsi.org/saref4bldg/firstCurvatureRadius -->


    <owl:ObjectProperty rdf:about="https://saref.etsi.org/saref4bldg/firstCurvatureRadius">
        <rdfs:comment xml:lang="en">FirstCurvatureRadius should be defined as the base or left side radius of curvature value. Usually measured in millimeters (mm).</rdfs:comment>
        <rdfs:label xml:lang="en">first curvature radius</rdfs:label>
    </owl:ObjectProperty>
    


    <!-- https://saref.etsi.org/saref4bldg/flowCoefficient -->


    <owl:ObjectProperty rdf:about="https://saref.etsi.org/saref4bldg/flowCoefficient">
        <rdfs:comment xml:lang="en">Flow coefficient (the quantity of fluid that passes through a fully open valve at unit pressure drop), typically expressed as the Kv or Cv value for the valve.</rdfs:comment>
        <rdfs:label xml:lang="en">flow coefficient</rdfs:label>
    </owl:ObjectProperty>
    


    <!-- https://saref.etsi.org/saref4bldg/flowResistanceMax -->


    <owl:ObjectProperty rdf:about="https://saref.etsi.org/saref4bldg/flowResistanceMax">
        <rdfs:comment xml:lang="en">Allowable range of frictional resistance against which the fluid is being pumped. Usually measured in Pascals (Pa, N/m2).</rdfs:comment>
        <rdfs:label xml:lang="en">flow resistance range</rdfs:label>
    </owl:ObjectProperty>
    


    <!-- https://saref.etsi.org/saref4bldg/flowResistanceMin -->


    <owl:ObjectProperty rdf:about="https://saref.etsi.org/saref4bldg/flowResistanceMin">
        <rdfs:comment xml:lang="en">Allowable range of frictional resistance against which the fluid is being pumped. Usually measured in Pascals (Pa, N/m2).</rdfs:comment>
        <rdfs:label xml:lang="en">flow resistance range</rdfs:label>
    </owl:ObjectProperty>
    


    <!-- https://saref.etsi.org/saref4bldg/fluidFlowRateMax -->


    <owl:ObjectProperty rdf:about="https://saref.etsi.org/saref4bldg/fluidFlowRateMax">
        <rdfs:comment xml:lang="en">Possible range of fluid flowrate that can be delivered. Usually measured in m3/s.</rdfs:comment>
        <rdfs:label xml:lang="en">fluid flow rate range</rdfs:label>
    </owl:ObjectProperty>
    


    <!-- https://saref.etsi.org/saref4bldg/fluidFlowRateMin -->


    <owl:ObjectProperty rdf:about="https://saref.etsi.org/saref4bldg/fluidFlowRateMin">
        <rdfs:comment xml:lang="en">Possible range of fluid flowrate that can be delivered. Usually measured in m3/s.</rdfs:comment>
        <rdfs:label xml:lang="en">fluid flow rate range</rdfs:label>
    </owl:ObjectProperty>
    


    <!-- https://saref.etsi.org/saref4bldg/foulingFactor -->


    <owl:ObjectProperty rdf:about="https://saref.etsi.org/saref4bldg/foulingFactor">
        <rdfs:comment xml:lang="en">Fouling factor of the tubes in the tube bundle. Usually measured in m2 Kelvin/Watt.</rdfs:comment>
        <rdfs:label xml:lang="en">fouling factor</rdfs:label>
    </owl:ObjectProperty>
    


    <!-- https://saref.etsi.org/saref4bldg/frameDepth -->


    <owl:ObjectProperty rdf:about="https://saref.etsi.org/saref4bldg/frameDepth">
        <rdfs:comment xml:lang="en">The length (or depth) of the damper frame. Usually measured in millimeters (mm).</rdfs:comment>
        <rdfs:label xml:lang="en">frame depth</rdfs:label>
    </owl:ObjectProperty>
    


    <!-- https://saref.etsi.org/saref4bldg/frameThickness -->


    <owl:ObjectProperty rdf:about="https://saref.etsi.org/saref4bldg/frameThickness">
        <rdfs:comment xml:lang="en">The thickness of the damper frame material. Usually measured in millimeters (mm).</rdfs:comment>
        <rdfs:label xml:lang="en">frame thickness</rdfs:label>
    </owl:ObjectProperty>
    


    <!-- https://saref.etsi.org/saref4bldg/hasSpace -->


    <owl:ObjectProperty rdf:about="https://saref.etsi.org/saref4bldg/hasSpace">
        <owl:inverseOf rdf:resource="https://saref.etsi.org/saref4bldg/isSpaceOf"/>
        <rdf:type rdf:resource="http://www.w3.org/2002/07/owl#TransitiveProperty"/>
        <rdfs:comment xml:lang="en">Relation between a building or a building space and the spaces it can be divided into.</rdfs:comment>
        <rdfs:label xml:lang="en">has space</rdfs:label>
    </owl:ObjectProperty>
    


    <!-- https://saref.etsi.org/saref4bldg/heatExchangeArea -->


    <owl:ObjectProperty rdf:about="https://saref.etsi.org/saref4bldg/heatExchangeArea">
        <rdfs:comment xml:lang="en">Heat exchange area. Usually measured in square metre (m2).</rdfs:comment>
        <rdfs:label xml:lang="en">heat exchange area</rdfs:label>
    </owl:ObjectProperty>
    


    <!-- https://saref.etsi.org/saref4bldg/heatTransferSurfaceArea -->


    <owl:ObjectProperty rdf:about="https://saref.etsi.org/saref4bldg/heatTransferSurfaceArea">
        <rdfs:comment xml:lang="en">Total heat transfer area of the vessel. Usually measured in square metre (m2).</rdfs:comment>
        <rdfs:label xml:lang="en">heat transfer surface area</rdfs:label>
    </owl:ObjectProperty>
    


    <!-- https://saref.etsi.org/saref4bldg/height -->


    <owl:ObjectProperty rdf:about="https://saref.etsi.org/saref4bldg/height">
        <rdfs:comment xml:lang="en">Height of the vibration isolator before tha application of load. Usually measured in millimeters (mm).</rdfs:comment>
        <rdfs:label xml:lang="en">height</rdfs:label>
    </owl:ObjectProperty>
    


    <!-- https://saref.etsi.org/saref4bldg/horizontalSpacing -->


    <owl:ObjectProperty rdf:about="https://saref.etsi.org/saref4bldg/horizontalSpacing">
        <rdfs:comment xml:lang="en">Horizontal spacing between tubes in the tube bundle. Usually measured in millimeters (mm).</rdfs:comment>
        <rdfs:label xml:lang="en">horizontal spacing</rdfs:label>
    </owl:ObjectProperty>
    


    <!-- https://saref.etsi.org/saref4bldg/hydraulicDiameter -->


    <owl:ObjectProperty rdf:about="https://saref.etsi.org/saref4bldg/hydraulicDiameter">
        <rdfs:comment xml:lang="en">Hydraulic diameter. Usually measured in millimeters (mm).</rdfs:comment>
        <rdfs:label xml:lang="en">hydraulic diameter</rdfs:label>
    </owl:ObjectProperty>
    


    <!-- https://saref.etsi.org/saref4bldg/idealCapacity -->


    <owl:ObjectProperty rdf:about="https://saref.etsi.org/saref4bldg/idealCapacity">
        <rdfs:comment xml:lang="en">Compressor capacity under ideal conditions. Usually measured in Watts (W, J/s).</rdfs:comment>
        <rdfs:label xml:lang="en">ideal capacity</rdfs:label>
    </owl:ObjectProperty>
    


    <!-- https://saref.etsi.org/saref4bldg/idealShaftPower -->


    <owl:ObjectProperty rdf:about="https://saref.etsi.org/saref4bldg/idealShaftPower">
        <rdfs:comment xml:lang="en">Compressor shaft power under ideal conditions. Usually measured in Watts (W, J/s).</rdfs:comment>
        <rdfs:label xml:lang="en">ideal shaft power</rdfs:label>
    </owl:ObjectProperty>
    


    <!-- https://saref.etsi.org/saref4bldg/imaginaryImpedanceRatio -->


    <owl:ObjectProperty rdf:about="https://saref.etsi.org/saref4bldg/imaginaryImpedanceRatio">
        <rdfs:comment xml:lang="en">The ratio between the imaginary part of the zero sequence impedance and the imaginary part of the positive impedance (i.e. imaginary part of the short-circuit voltage) of the transformer. Used for three-phase transformer which includes a N-conductor.</rdfs:comment>
        <rdfs:label xml:lang="en">imaginary impedance ratio</rdfs:label>
    </owl:ObjectProperty>
    


    <!-- https://saref.etsi.org/saref4bldg/impellerDiameter -->


    <owl:ObjectProperty rdf:about="https://saref.etsi.org/saref4bldg/impellerDiameter">
        <rdfs:comment xml:lang="en">Diameter of compressor impeller - used to scale performance of geometrically similar compressors. Usually measured in millimeters (mm).</rdfs:comment>
        <rdfs:label xml:lang="en">impeller diameter</rdfs:label>
    </owl:ObjectProperty>
    


    <!-- https://saref.etsi.org/saref4bldg/inLineRowSpacing -->


    <owl:ObjectProperty rdf:about="https://saref.etsi.org/saref4bldg/inLineRowSpacing">
        <rdfs:comment xml:lang="en">In-line tube row spacing. Usually measured in millimeters (mm).</rdfs:comment>
        <rdfs:label xml:lang="en">in line row spacing</rdfs:label>
    </owl:ObjectProperty>
    


    <!-- https://saref.etsi.org/saref4bldg/initialResistance -->


    <owl:ObjectProperty rdf:about="https://saref.etsi.org/saref4bldg/initialResistance">
        <rdfs:comment xml:lang="en">Initial new filter fluid resistance (i.e., pressure drop at the maximum air flowrate across the filter when the filter is new per ASHRAE Standard 52.1). Usually measured in Pascals (Pa, N/m2).</rdfs:comment>
        <rdfs:label xml:lang="en">initial resistance</rdfs:label>
    </owl:ObjectProperty>
    


    <!-- https://saref.etsi.org/saref4bldg/inletConnectionSize -->


    <owl:ObjectProperty rdf:about="https://saref.etsi.org/saref4bldg/inletConnectionSize">
        <rdfs:comment xml:lang="en">Size of the inlet connection. Usually measured in millimeters (mm).</rdfs:comment>
        <rdfs:label xml:lang="en">inlet connection size</rdfs:label>
    </owl:ObjectProperty>
    


    <!-- https://saref.etsi.org/saref4bldg/insideDiameter -->


    <owl:ObjectProperty rdf:about="https://saref.etsi.org/saref4bldg/insideDiameter">
        <rdfs:comment xml:lang="en">Actual inner diameter of the tube in the tube bundle. Usually measured in millimeters (mm).</rdfs:comment>
        <rdfs:label xml:lang="en">inside diameter</rdfs:label>
    </owl:ObjectProperty>
    


    <!-- https://saref.etsi.org/saref4bldg/internalRefrigerantVolume -->


    <owl:ObjectProperty rdf:about="https://saref.etsi.org/saref4bldg/internalRefrigerantVolume">
        <rdfs:comment xml:lang="en">Internal volume of evaporator (refrigerant side). Usually measured in cubic metre (m3).</rdfs:comment>
        <rdfs:label xml:lang="en">internal refrigerant volume</rdfs:label>
    </owl:ObjectProperty>
    


    <!-- https://saref.etsi.org/saref4bldg/internalSurfaceArea -->


    <owl:ObjectProperty rdf:about="https://saref.etsi.org/saref4bldg/internalSurfaceArea">
        <rdfs:comment xml:lang="en">Internal surface area. Usually measured in square metre (m2).</rdfs:comment>
        <rdfs:label xml:lang="en">internal surface area</rdfs:label>
    </owl:ObjectProperty>
    


    <!-- https://saref.etsi.org/saref4bldg/internalWaterVolume -->


    <owl:ObjectProperty rdf:about="https://saref.etsi.org/saref4bldg/internalWaterVolume">
        <rdfs:comment xml:lang="en">Internal volume of evaporator (water side). Usually measured in cubic metre (m3).</rdfs:comment>
        <rdfs:label xml:lang="en">internal water volume</rdfs:label>
    </owl:ObjectProperty>
    


    <!-- https://saref.etsi.org/saref4bldg/isContainedIn -->


    <owl:ObjectProperty rdf:about="https://saref.etsi.org/saref4bldg/isContainedIn">
        <rdf:type rdf:resource="http://www.w3.org/2002/07/owl#TransitiveProperty"/>
        <rdfs:comment xml:lang="en">A relation between an object and the physical space in which it is located.</rdfs:comment>
        <rdfs:label xml:lang="en">is contained in</rdfs:label>
    </owl:ObjectProperty>
    


    <!-- https://saref.etsi.org/saref4bldg/isSpaceOf -->


    <owl:ObjectProperty rdf:about="https://saref.etsi.org/saref4bldg/isSpaceOf">
        <rdf:type rdf:resource="http://www.w3.org/2002/07/owl#TransitiveProperty"/>
        <rdfs:comment xml:lang="en">Relation between a building space and the building or building space it belongs to.</rdfs:comment>
        <rdfs:label xml:lang="en">isSpaceOf</rdfs:label>
    </owl:ObjectProperty>
    


    <!-- https://saref.etsi.org/saref4bldg/isolatorCompressibility -->


    <owl:ObjectProperty rdf:about="https://saref.etsi.org/saref4bldg/isolatorCompressibility">
        <rdfs:comment xml:lang="en">The compressibility of the vibration isolator.</rdfs:comment>
        <rdfs:label xml:lang="en">isolator compressibility</rdfs:label>
    </owl:ObjectProperty>
    


    <!-- https://saref.etsi.org/saref4bldg/isolatorStaticDeflection -->


    <owl:ObjectProperty rdf:about="https://saref.etsi.org/saref4bldg/isolatorStaticDeflection">
        <rdfs:comment xml:lang="en">Static deflection of the vibration isolator. Usually measured in millimeters (mm).</rdfs:comment>
        <rdfs:label xml:lang="en">isolator static deflection</rdfs:label>
    </owl:ObjectProperty>
    


    <!-- https://saref.etsi.org/saref4bldg/lampMaintenanceFactor -->


    <owl:ObjectProperty rdf:about="https://saref.etsi.org/saref4bldg/lampMaintenanceFactor">
        <rdfs:comment xml:lang="en">Non recoverable losses of luminous flux of a lamp due to lamp depreciation i.e. the decreasing of light output of a luminaire due to aging and dirt.</rdfs:comment>
        <rdfs:label xml:lang="en">lamp maintenance factor</rdfs:label>
    </owl:ObjectProperty>
    


    <!-- https://saref.etsi.org/saref4bldg/leakageFullyClosed -->


    <owl:ObjectProperty rdf:about="https://saref.etsi.org/saref4bldg/leakageFullyClosed">
        <rdfs:comment xml:lang="en">Leakage when fully closed. Usually measured in m3/s.</rdfs:comment>
        <rdfs:label xml:lang="en">leakage fully closed</rdfs:label>
    </owl:ObjectProperty>
    


    <!-- https://saref.etsi.org/saref4bldg/length -->


    <owl:ObjectProperty rdf:about="https://saref.etsi.org/saref4bldg/length">
        <rdfs:comment xml:lang="en">The finished length of the device. Usually measured in millimeters (mm).</rdfs:comment>
        <rdfs:label xml:lang="en">length</rdfs:label>
    </owl:ObjectProperty>
    


    <!-- https://saref.etsi.org/saref4bldg/liftElevationDifference -->


    <owl:ObjectProperty rdf:about="https://saref.etsi.org/saref4bldg/liftElevationDifference">
        <rdfs:comment xml:lang="en">Elevation difference between cooling tower sump and the top of the tower. Usually measured in millimeters (mm).</rdfs:comment>
        <rdfs:label xml:lang="en">lift elevation difference</rdfs:label>
    </owl:ObjectProperty>
    


    <!-- https://saref.etsi.org/saref4bldg/lightEmitterNominalPower -->


    <owl:ObjectProperty rdf:about="https://saref.etsi.org/saref4bldg/lightEmitterNominalPower">
        <rdfs:comment xml:lang="en">Light emitter nominal power. Usually measured in Watts (W, J/s).</rdfs:comment>
        <rdfs:label xml:lang="en">light emitter nominal power</rdfs:label>
    </owl:ObjectProperty>
    


    <!-- https://saref.etsi.org/saref4bldg/limitingTerminalSize -->


    <owl:ObjectProperty rdf:about="https://saref.etsi.org/saref4bldg/limitingTerminalSize">
        <rdfs:comment xml:lang="en">The maximum terminal size capacity of the device. Usually measured in square metre (m2).</rdfs:comment>
        <rdfs:label xml:lang="en">limiting terminal size</rdfs:label>
    </owl:ObjectProperty>
    


    <!-- https://saref.etsi.org/saref4bldg/lockedRotorCurrent -->


    <owl:ObjectProperty rdf:about="https://saref.etsi.org/saref4bldg/lockedRotorCurrent">
        <rdfs:comment xml:lang="en">Input current when a motor armature is energized but not rotating. Usually measured in Ampere (A).</rdfs:comment>
        <rdfs:label xml:lang="en">locked rotor current</rdfs:label>
    </owl:ObjectProperty>
    


    <!-- https://saref.etsi.org/saref4bldg/netPositiveSuctionHead -->


    <owl:ObjectProperty rdf:about="https://saref.etsi.org/saref4bldg/netPositiveSuctionHead">
        <rdfs:comment xml:lang="en">Minimum liquid pressure at the pump inlet to prevent cavitation. Usually measured in Pascals (Pa, N/m2).</rdfs:comment>
        <rdfs:label xml:lang="en">net positive suction head</rdfs:label>
    </owl:ObjectProperty>
    


    <!-- https://saref.etsi.org/saref4bldg/nominalAirFlowRate -->


    <owl:ObjectProperty rdf:about="https://saref.etsi.org/saref4bldg/nominalAirFlowRate">
        <rdfs:comment xml:lang="en">Nominal rate of air flow. Usually measured in m3/s.</rdfs:comment>
        <rdfs:label xml:lang="en">nominal air flow rate</rdfs:label>
    </owl:ObjectProperty>
    


    <!-- https://saref.etsi.org/saref4bldg/nominalBodyDepth -->


    <owl:ObjectProperty rdf:about="https://saref.etsi.org/saref4bldg/nominalBodyDepth">
        <rdfs:comment xml:lang="en">Nominal or quoted =length, measured along the z-axis of the local coordinate system of the object, of the body of the object. Usually measured in millimeters (mm).</rdfs:comment>
        <rdfs:label xml:lang="en">nominal body depth</rdfs:label>
    </owl:ObjectProperty>
    


    <!-- https://saref.etsi.org/saref4bldg/nominalBodyLength -->


    <owl:ObjectProperty rdf:about="https://saref.etsi.org/saref4bldg/nominalBodyLength">
        <rdfs:comment xml:lang="en">Nominal or quoted length, measured along the x-axis of the local coordinate system of the object, of the body of the object. Usually measured in millimeters (mm).</rdfs:comment>
        <rdfs:label xml:lang="en">nominal body length</rdfs:label>
    </owl:ObjectProperty>
    


    <!-- https://saref.etsi.org/saref4bldg/nominalBodyWidth -->


    <owl:ObjectProperty rdf:about="https://saref.etsi.org/saref4bldg/nominalBodyWidth">
        <rdfs:comment xml:lang="en">Nominal or quoted length, measured along the y-axis of the local coordinate system of the object, of the body of the object. Usually measured in millimeters (mm).</rdfs:comment>
        <rdfs:label xml:lang="en">nominal body width</rdfs:label>
    </owl:ObjectProperty>
    


    <!-- https://saref.etsi.org/saref4bldg/nominalCapacity -->


    <owl:ObjectProperty rdf:about="https://saref.etsi.org/saref4bldg/nominalCapacity">
        <rdfs:comment xml:lang="en">Nominal capacity. Usually measured in Watts (W, J/s).</rdfs:comment>
        <rdfs:label xml:lang="en">nominal capacity</rdfs:label>
    </owl:ObjectProperty>
    


    <!-- https://saref.etsi.org/saref4bldg/nominalCondensingTemperature -->


    <owl:ObjectProperty rdf:about="https://saref.etsi.org/saref4bldg/nominalCondensingTemperature">
        <rdfs:comment xml:lang="en">Chiller condensing temperature. Usually measured in degrees Kelvin (K).</rdfs:comment>
        <rdfs:label xml:lang="en">nominal condensing temperature</rdfs:label>
    </owl:ObjectProperty>
    


    <!-- https://saref.etsi.org/saref4bldg/nominalCoolingCapacity -->


    <owl:ObjectProperty rdf:about="https://saref.etsi.org/saref4bldg/nominalCoolingCapacity">
        <rdfs:comment xml:lang="en">Nominal cooling capacity. Usually measured in Watts (W, J/s).</rdfs:comment>
        <rdfs:label xml:lang="en">nominal cooling capacity</rdfs:label>
    </owl:ObjectProperty>
    


    <!-- https://saref.etsi.org/saref4bldg/nominalDepth -->


    <owl:ObjectProperty rdf:about="https://saref.etsi.org/saref4bldg/nominalDepth">
        <rdfs:comment xml:lang="en">The nominal depth of the tank. Note: Not required for a horizontal cylindrical tank. Usually measured in millimeters (mm).</rdfs:comment>
        <rdfs:label xml:lang="en">nominal depth</rdfs:label>
    </owl:ObjectProperty>
    


    <!-- https://saref.etsi.org/saref4bldg/nominalDiameter -->


    <owl:ObjectProperty rdf:about="https://saref.etsi.org/saref4bldg/nominalDiameter">
        <rdfs:comment xml:lang="en">Nominal diameter or width of the tubes in the tube bundle. Usually measured in millimeters (mm).</rdfs:comment>
        <rdfs:label xml:lang="en">nominal diameter</rdfs:label>
    </owl:ObjectProperty>
    


    <!-- https://saref.etsi.org/saref4bldg/nominalEfficiency -->


    <owl:ObjectProperty rdf:about="https://saref.etsi.org/saref4bldg/nominalEfficiency">
        <rdfs:comment xml:lang="en">Nominal chiller efficiency under nominal conditions. </rdfs:comment>
        <rdfs:label xml:lang="en">nominal efficiency</rdfs:label>
    </owl:ObjectProperty>
    


    <!-- https://saref.etsi.org/saref4bldg/nominalEnergyConsumption -->


    <owl:ObjectProperty rdf:about="https://saref.etsi.org/saref4bldg/nominalEnergyConsumption">
        <rdfs:comment xml:lang="en">Nominal fuel consumption rate required to produce the total boiler heat output. Usually measured in Watts (W, J/s).</rdfs:comment>
        <rdfs:label xml:lang="en">nominal energy consumption</rdfs:label>
    </owl:ObjectProperty>
    


    <!-- https://saref.etsi.org/saref4bldg/nominalEvaporatingTemmperature -->


    <owl:ObjectProperty rdf:about="https://saref.etsi.org/saref4bldg/nominalEvaporatingTemmperature">
        <rdfs:comment xml:lang="en">Chiller evaporating temperature.Usually measured in degrees Kelvin (K).</rdfs:comment>
        <rdfs:label xml:lang="en">nominal evaporating temmperature</rdfs:label>
    </owl:ObjectProperty>
    


    <!-- https://saref.etsi.org/saref4bldg/nominalFilterFaceVelocity -->


    <owl:ObjectProperty rdf:about="https://saref.etsi.org/saref4bldg/nominalFilterFaceVelocity">
        <rdfs:comment xml:lang="en">Filter face velocity. Usually measured in m/s.</rdfs:comment>
        <rdfs:label xml:lang="en">nominal filter face velocity</rdfs:label>
    </owl:ObjectProperty>
    


    <!-- https://saref.etsi.org/saref4bldg/nominalFlowRate -->


    <owl:ObjectProperty rdf:about="https://saref.etsi.org/saref4bldg/nominalFlowRate">
        <rdfs:comment xml:lang="en">Nominal fluid flow rate through the filter. Usually measured in m3/s.</rdfs:comment>
        <rdfs:label xml:lang="en">nominal flow rate</rdfs:label>
    </owl:ObjectProperty>
    


    <!-- https://saref.etsi.org/saref4bldg/nominalFrequency -->


    <owl:ObjectProperty rdf:about="https://saref.etsi.org/saref4bldg/nominalFrequency">
        <rdfs:comment xml:lang="en">The nominal frequency of the supply. Usually measured in cycles/s or Hertz (Hz).</rdfs:comment>
        <rdfs:label xml:lang="en">nominal frequency</rdfs:label>
    </owl:ObjectProperty>
    


    <!-- https://saref.etsi.org/saref4bldg/nominalHeatRejectionRate -->


    <owl:ObjectProperty rdf:about="https://saref.etsi.org/saref4bldg/nominalHeatRejectionRate">
        <rdfs:comment xml:lang="en">Sum of the refrigeration effect and the heat equivalent of the power input to the compressor. Usually measured in Watts (W, J/s).</rdfs:comment>
        <rdfs:label xml:lang="en">nominal heat rejection rate</rdfs:label>
    </owl:ObjectProperty>
    


    <!-- https://saref.etsi.org/saref4bldg/nominalHeatTransferArea -->


    <owl:ObjectProperty rdf:about="https://saref.etsi.org/saref4bldg/nominalHeatTransferArea">
        <rdfs:comment xml:lang="en">Nominal heat transfer surface area associated with nominal overall heat transfer coefficient. Usually measured in square metre (m2).</rdfs:comment>
        <rdfs:label xml:lang="en">nominal heat transfer area</rdfs:label>
    </owl:ObjectProperty>
    


    <!-- https://saref.etsi.org/saref4bldg/nominalHeatTransferCoefficient -->


    <owl:ObjectProperty rdf:about="https://saref.etsi.org/saref4bldg/nominalHeatTransferCoefficient">
        <rdfs:comment xml:lang="en">Nominal overall heat transfer coefficient associated with nominal heat transfer area. Usually measured in Watts/m2 Kelvin.</rdfs:comment>
        <rdfs:label xml:lang="en">nominal heat transfer coefficient</rdfs:label>
    </owl:ObjectProperty>
    


    <!-- https://saref.etsi.org/saref4bldg/nominalHeatingCapacity -->


    <owl:ObjectProperty rdf:about="https://saref.etsi.org/saref4bldg/nominalHeatingCapacity">
        <rdfs:comment xml:lang="en">Nominal heating capacity. Usually measured in Watts (W, J/s).</rdfs:comment>
        <rdfs:label xml:lang="en">nominal heating capacity</rdfs:label>
    </owl:ObjectProperty>
    


    <!-- https://saref.etsi.org/saref4bldg/nominalLatentCapacity -->


    <owl:ObjectProperty rdf:about="https://saref.etsi.org/saref4bldg/nominalLatentCapacity">
        <rdfs:comment xml:lang="en">Nominal latent capacity. Usually measured in Watts (W, J/s).</rdfs:comment>
        <rdfs:label xml:lang="en">nominal latent capacity</rdfs:label>
    </owl:ObjectProperty>
    


    <!-- https://saref.etsi.org/saref4bldg/nominalLengthOrDiameter -->


    <owl:ObjectProperty rdf:about="https://saref.etsi.org/saref4bldg/nominalLengthOrDiameter">
        <rdfs:comment xml:lang="en">The nominal length or, in the case of a vertical cylindrical tank, the nominal diameter of the tank. Usually measured in millimeters (mm).</rdfs:comment>
        <rdfs:label xml:lang="en">nominal length or diameter</rdfs:label>
    </owl:ObjectProperty>
    


    <!-- https://saref.etsi.org/saref4bldg/nominalMediaSurfaceVelocity -->


    <owl:ObjectProperty rdf:about="https://saref.etsi.org/saref4bldg/nominalMediaSurfaceVelocity">
        <rdfs:comment xml:lang="en">Average fluid velocity at the media surface. Usually measured in m/s.</rdfs:comment>
        <rdfs:label xml:lang="en">nominal media surface velocity</rdfs:label>
    </owl:ObjectProperty>
    


    <!-- https://saref.etsi.org/saref4bldg/nominalMoistureGain -->


    <owl:ObjectProperty rdf:about="https://saref.etsi.org/saref4bldg/nominalMoistureGain">
        <rdfs:comment xml:lang="en">Nominal rate of water vapor added into the airstream. Usually measured in kg/s.</rdfs:comment>
        <rdfs:label xml:lang="en">nominal moisture gain</rdfs:label>
    </owl:ObjectProperty>
    


    <!-- https://saref.etsi.org/saref4bldg/nominalPartLoadRatio -->


    <owl:ObjectProperty rdf:about="https://saref.etsi.org/saref4bldg/nominalPartLoadRatio">
        <rdfs:comment xml:lang="en">Allowable part load ratio range.</rdfs:comment>
        <rdfs:label xml:lang="en">nominal part load ratio</rdfs:label>
    </owl:ObjectProperty>
    


    <!-- https://saref.etsi.org/saref4bldg/nominalParticleGeometricMeanDiameter -->


    <owl:ObjectProperty rdf:about="https://saref.etsi.org/saref4bldg/nominalParticleGeometricMeanDiameter">
        <rdfs:comment xml:lang="en">Particle geometric mean diameter associated with nominal efficiency. Usually measured in millimeters (mm).</rdfs:comment>
        <rdfs:label xml:lang="en">nominal particle geometric mean diameter</rdfs:label>
    </owl:ObjectProperty>
    


    <!-- https://saref.etsi.org/saref4bldg/nominalParticleGeometricStandardDeviation -->


    <owl:ObjectProperty rdf:about="https://saref.etsi.org/saref4bldg/nominalParticleGeometricStandardDeviation">
        <rdfs:comment xml:lang="en">Particle geometric standard deviation associated with nominal efficiency. </rdfs:comment>
        <rdfs:label xml:lang="en">nominal particle geometric standard deviation</rdfs:label>
    </owl:ObjectProperty>
    


    <!-- https://saref.etsi.org/saref4bldg/nominalPowerConsumption -->


    <owl:ObjectProperty rdf:about="https://saref.etsi.org/saref4bldg/nominalPowerConsumption">
        <rdfs:comment xml:lang="en">Nominal total power consumption. Usually measured in Watts (W, J/s).</rdfs:comment>
        <rdfs:label xml:lang="en">nominal power consumption</rdfs:label>
    </owl:ObjectProperty>
    


    <!-- https://saref.etsi.org/saref4bldg/nominalPowerRate -->


    <owl:ObjectProperty rdf:about="https://saref.etsi.org/saref4bldg/nominalPowerRate">
        <rdfs:comment xml:lang="en">Nominal fan power rate.Usually measured in Watts (W, J/s).</rdfs:comment>
        <rdfs:label xml:lang="en">nominal power rate</rdfs:label>
    </owl:ObjectProperty>
    


    <!-- https://saref.etsi.org/saref4bldg/nominalPressureDrop -->


    <owl:ObjectProperty rdf:about="https://saref.etsi.org/saref4bldg/nominalPressureDrop">
        <rdfs:comment xml:lang="en">Total pressure drop across the filter. Usually measured in Pascals (Pa, N/m2).</rdfs:comment>
        <rdfs:label xml:lang="en">nominal pressure drop</rdfs:label>
    </owl:ObjectProperty>
    


    <!-- https://saref.etsi.org/saref4bldg/nominalReturnWaterTemperatureCooling -->


    <owl:ObjectProperty rdf:about="https://saref.etsi.org/saref4bldg/nominalReturnWaterTemperatureCooling">
        <rdfs:comment xml:lang="en">Nominal return water temperature (refers to nominal cooling capacity). Usually measured in degrees Kelvin (K).</rdfs:comment>
        <rdfs:label xml:lang="en">nominal return water temperature cooling</rdfs:label>
    </owl:ObjectProperty>
    


    <!-- https://saref.etsi.org/saref4bldg/nominalReturnWaterTemperatureHeating -->


    <owl:ObjectProperty rdf:about="https://saref.etsi.org/saref4bldg/nominalReturnWaterTemperatureHeating">
        <rdfs:comment xml:lang="en">Nominal return water temperature (refers to nominal heating capacity). Usually measured in degrees Kelvin (K).</rdfs:comment>
        <rdfs:label xml:lang="en">nominal return water temperature heating</rdfs:label>
    </owl:ObjectProperty>
    


    <!-- https://saref.etsi.org/saref4bldg/nominalRotationSpeed -->


    <owl:ObjectProperty rdf:about="https://saref.etsi.org/saref4bldg/nominalRotationSpeed">
        <rdfs:comment xml:lang="en">Nominal fan wheel speed. Usually measured in cycles/s.</rdfs:comment>
        <rdfs:label xml:lang="en">nominal rotation speed</rdfs:label>
    </owl:ObjectProperty>
    


    <!-- https://saref.etsi.org/saref4bldg/nominalSensibleCapacity -->


    <owl:ObjectProperty rdf:about="https://saref.etsi.org/saref4bldg/nominalSensibleCapacity">
        <rdfs:comment xml:lang="en">Nominal sensible capacity. Usually measured in Watts (W, J/s).</rdfs:comment>
        <rdfs:label xml:lang="en">nominal sensible capacity</rdfs:label>
    </owl:ObjectProperty>
    


    <!-- https://saref.etsi.org/saref4bldg/nominalSorroundingHumidityCooling -->


    <owl:ObjectProperty rdf:about="https://saref.etsi.org/saref4bldg/nominalSorroundingHumidityCooling">
        <rdfs:comment xml:lang="en">Nominal surrounding humidity (refers to nominal cooling capacity). Usually measured in degrees Kelvin (K).</rdfs:comment>
        <rdfs:label xml:lang="en">nominal sorrounding humidity cooling</rdfs:label>
    </owl:ObjectProperty>
    


    <!-- https://saref.etsi.org/saref4bldg/nominalSorroundingTemperatureCooling -->


    <owl:ObjectProperty rdf:about="https://saref.etsi.org/saref4bldg/nominalSorroundingTemperatureCooling">
        <rdfs:comment xml:lang="en">Nominal surrounding temperature (refers to nominal cooling capacity). Usually measured in degrees Kelvin (K).</rdfs:comment>
        <rdfs:label xml:lang="en">nominal sorrounding temperature cooling</rdfs:label>
    </owl:ObjectProperty>
    


    <!-- https://saref.etsi.org/saref4bldg/nominalSorroundingTemperatureHeating -->


    <owl:ObjectProperty rdf:about="https://saref.etsi.org/saref4bldg/nominalSorroundingTemperatureHeating">
        <rdfs:comment xml:lang="en">Nominal surrounding temperature (refers to nominal heating capacity). Usually measured in degrees Kelvin (K).</rdfs:comment>
        <rdfs:label xml:lang="en">nominal sorrounding temperature heating</rdfs:label>
    </owl:ObjectProperty>
    


    <!-- https://saref.etsi.org/saref4bldg/nominalStaticPressure -->


    <owl:ObjectProperty rdf:about="https://saref.etsi.org/saref4bldg/nominalStaticPressure">
        <rdfs:comment xml:lang="en">The static pressure within the air stream that the fan must overcome to insure designed circulation of air. Usually measured in Pascals (Pa, N/m2).</rdfs:comment>
        <rdfs:label xml:lang="en">nominal static pressure</rdfs:label>
    </owl:ObjectProperty>
    


    <!-- https://saref.etsi.org/saref4bldg/nominalSupplyVoltage -->


    <owl:ObjectProperty rdf:about="https://saref.etsi.org/saref4bldg/nominalSupplyVoltage">
        <rdfs:comment xml:lang="en">The nominal voltage of the supply. Usually measured in Volts (V, W/A).</rdfs:comment>
        <rdfs:label xml:lang="en">nominal supply voltage</rdfs:label>
    </owl:ObjectProperty>
    


    <!-- https://saref.etsi.org/saref4bldg/nominalSupplyVoltageMax -->


    <owl:ObjectProperty rdf:about="https://saref.etsi.org/saref4bldg/nominalSupplyVoltageMax">
        <rdfs:comment xml:lang="en">The maximum and minimum allowed voltage of the supply e.g. boundaries of 380V/440V may be applied for a nominal voltage of 400V.</rdfs:comment>
        <rdfs:label xml:lang="en">nominal supply voltage offset</rdfs:label>
    </owl:ObjectProperty>
    


    <!-- https://saref.etsi.org/saref4bldg/nominalSupplyVoltageMin -->


    <owl:ObjectProperty rdf:about="https://saref.etsi.org/saref4bldg/nominalSupplyVoltageMin">
        <rdfs:comment xml:lang="en">The maximum and minimum allowed voltage of the supply e.g. boundaries of 380V/440V may be applied for a nominal voltage of 400V.</rdfs:comment>
        <rdfs:label xml:lang="en">nominal supply voltage offset</rdfs:label>
    </owl:ObjectProperty>
    


    <!-- https://saref.etsi.org/saref4bldg/nominalSupplyWaterTemperatureCooling -->


    <owl:ObjectProperty rdf:about="https://saref.etsi.org/saref4bldg/nominalSupplyWaterTemperatureCooling">
        <rdfs:comment xml:lang="en">Nominal supply water temperature (refers to nominal cooling capacity). Usually measured in degrees Kelvin (K).</rdfs:comment>
        <rdfs:label xml:lang="en">nominal supply water temperature cooling</rdfs:label>
    </owl:ObjectProperty>
    


    <!-- https://saref.etsi.org/saref4bldg/nominalSupplyWaterTemperatureHeating -->


    <owl:ObjectProperty rdf:about="https://saref.etsi.org/saref4bldg/nominalSupplyWaterTemperatureHeating">
        <rdfs:comment xml:lang="en">Nominal supply water temperature (refers to nominal heating capacity). Usually measured in degrees Kelvin (K).</rdfs:comment>
        <rdfs:label xml:lang="en">nominal supply water temperature heating</rdfs:label>
    </owl:ObjectProperty>
    


    <!-- https://saref.etsi.org/saref4bldg/nominalTotalPressure -->


    <owl:ObjectProperty rdf:about="https://saref.etsi.org/saref4bldg/nominalTotalPressure">
        <rdfs:comment xml:lang="en">Nominal total pressure rise across the fan. Usually measured in Pascals (Pa, N/m2).</rdfs:comment>
        <rdfs:label xml:lang="en">nominal total pressure</rdfs:label>
    </owl:ObjectProperty>
    


    <!-- https://saref.etsi.org/saref4bldg/nominalUa -->


    <owl:ObjectProperty rdf:about="https://saref.etsi.org/saref4bldg/nominalUa">
        <rdfs:comment xml:lang="en">Nominal UA value.</rdfs:comment>
        <rdfs:label xml:lang="en">nominal ua</rdfs:label>
    </owl:ObjectProperty>
    


    <!-- https://saref.etsi.org/saref4bldg/nominalVolumetricCapacity -->


    <owl:ObjectProperty rdf:about="https://saref.etsi.org/saref4bldg/nominalVolumetricCapacity">
        <rdfs:comment xml:lang="en">The total nominal or design volumetric capacity of the tank. Usually measured in cubic metre (m3).</rdfs:comment>
        <rdfs:label xml:lang="en">nominal volumetric capacity</rdfs:label>
    </owl:ObjectProperty>
    


    <!-- https://saref.etsi.org/saref4bldg/nominalWaterFlowCooling -->


    <owl:ObjectProperty rdf:about="https://saref.etsi.org/saref4bldg/nominalWaterFlowCooling">
        <rdfs:comment xml:lang="en">Nominal water flow (refers to nominal cooling capacity). Usually measured in m3/s.</rdfs:comment>
        <rdfs:label xml:lang="en">nominal water flow cooling</rdfs:label>
    </owl:ObjectProperty>
    


    <!-- https://saref.etsi.org/saref4bldg/nominalWaterFlowHeating -->


    <owl:ObjectProperty rdf:about="https://saref.etsi.org/saref4bldg/nominalWaterFlowHeating">
        <rdfs:comment xml:lang="en">Nominal water flow (refers to nominal heating capacity). Usually measured in m3/s.</rdfs:comment>
        <rdfs:label xml:lang="en">nominal water flow heating</rdfs:label>
    </owl:ObjectProperty>
    


    <!-- https://saref.etsi.org/saref4bldg/nominalWidthOrDiameter -->


    <owl:ObjectProperty rdf:about="https://saref.etsi.org/saref4bldg/nominalWidthOrDiameter">
        <rdfs:comment xml:lang="en">The nominal width or, in the case of a horizontal cylindrical tank, the nominal diameter of the tank. Note: Not required for a vertical cylindrical tank. Usually measured in millimeters (mm).</rdfs:comment>
        <rdfs:label xml:lang="en">nominal width or diameter</rdfs:label>
    </owl:ObjectProperty>
    


    <!-- https://saref.etsi.org/saref4bldg/nomminalRotationSpeed -->


    <owl:ObjectProperty rdf:about="https://saref.etsi.org/saref4bldg/nomminalRotationSpeed">
        <rdfs:comment xml:lang="en">Pump rotational speed under nominal conditions. Usually measured in cycles/s.</rdfs:comment>
        <rdfs:label xml:lang="en">nomminal rotation speed</rdfs:label>
    </owl:ObjectProperty>
    


    <!-- https://saref.etsi.org/saref4bldg/openPressureDrop -->


    <owl:ObjectProperty rdf:about="https://saref.etsi.org/saref4bldg/openPressureDrop">
        <rdfs:comment xml:lang="en">Total pressure drop across damper. Usually measured in Pascals (Pa, N/m2).</rdfs:comment>
        <rdfs:label xml:lang="en">open pressure drop</rdfs:label>
    </owl:ObjectProperty>
    


    <!-- https://saref.etsi.org/saref4bldg/operatingWeight -->


    <owl:ObjectProperty rdf:about="https://saref.etsi.org/saref4bldg/operatingWeight">
        <rdfs:comment xml:lang="en">Operating weight of the tank including all of its contents. Usually measured in kilograms (kg) or grams (g).</rdfs:comment>
        <rdfs:label xml:lang="en">operating weight</rdfs:label>
    </owl:ObjectProperty>
    


    <!-- https://saref.etsi.org/saref4bldg/operationTemperatureMax -->


    <owl:ObjectProperty rdf:about="https://saref.etsi.org/saref4bldg/operationTemperatureMax">
        <rdfs:comment xml:lang="en">Allowable operation ambient (air, fluid) temperature range. Usually measured in degrees Kelvin (K).</rdfs:comment>
        <rdfs:label xml:lang="en">operation temperature range</rdfs:label>
    </owl:ObjectProperty>
    


    <!-- https://saref.etsi.org/saref4bldg/operationTemperatureMin -->


    <owl:ObjectProperty rdf:about="https://saref.etsi.org/saref4bldg/operationTemperatureMin">
        <rdfs:comment xml:lang="en">Allowable operation ambient (air, fluid) temperature range. Usually measured in degrees Kelvin (K).</rdfs:comment>
        <rdfs:label xml:lang="en">operation temperature range</rdfs:label>
    </owl:ObjectProperty>
    


    <!-- https://saref.etsi.org/saref4bldg/operationalRiterial -->


    <owl:ObjectProperty rdf:about="https://saref.etsi.org/saref4bldg/operationalRiterial">
        <rdfs:comment xml:lang="en">Time of operation at maximum operational ambient air temperature. Measured in seconds (s) or days (d) or other units of time.</rdfs:comment>
        <rdfs:label xml:lang="en">operational riterial</rdfs:label>
    </owl:ObjectProperty>
    


    <!-- https://saref.etsi.org/saref4bldg/outletConnectionSize -->


    <owl:ObjectProperty rdf:about="https://saref.etsi.org/saref4bldg/outletConnectionSize">
        <rdfs:comment xml:lang="en">Size of the outlet connection. Usually measured in millimeters (mm).</rdfs:comment>
        <rdfs:label xml:lang="en">outlet connection size</rdfs:label>
    </owl:ObjectProperty>
    


    <!-- https://saref.etsi.org/saref4bldg/outletTemperatureMax -->


    <owl:ObjectProperty rdf:about="https://saref.etsi.org/saref4bldg/outletTemperatureMax">
        <rdfs:comment xml:lang="en">Allowable outlet temperature of either the water or the steam. Usually measured in degrees Kelvin (K).</rdfs:comment>
        <rdfs:label xml:lang="en">outlet temperature range</rdfs:label>
    </owl:ObjectProperty>
    


    <!-- https://saref.etsi.org/saref4bldg/outletTemperatureMin -->


    <owl:ObjectProperty rdf:about="https://saref.etsi.org/saref4bldg/outletTemperatureMin">
        <rdfs:comment xml:lang="en">Allowable outlet temperature of either the water or the steam. Usually measured in degrees Kelvin (K).</rdfs:comment>
        <rdfs:label xml:lang="en">outlet temperature range</rdfs:label>
    </owl:ObjectProperty>
    


    <!-- https://saref.etsi.org/saref4bldg/outputCapacity -->


    <owl:ObjectProperty rdf:about="https://saref.etsi.org/saref4bldg/outputCapacity">
        <rdfs:comment xml:lang="en">Total nominal heat output as listed by the manufacturer. Usually measured in Watts (W, J/s).</rdfs:comment>
        <rdfs:label xml:lang="en">output capacity</rdfs:label>
    </owl:ObjectProperty>
    


    <!-- https://saref.etsi.org/saref4bldg/outsideDiameter -->


    <owl:ObjectProperty rdf:about="https://saref.etsi.org/saref4bldg/outsideDiameter">
        <rdfs:comment xml:lang="en">Actual outside diameter of the tube in the tube bundle. Usually measured in millimeters (mm).</rdfs:comment>
        <rdfs:label xml:lang="en">outside diameter</rdfs:label>
    </owl:ObjectProperty>
    


    <!-- https://saref.etsi.org/saref4bldg/partLoadRatioMax -->


    <owl:ObjectProperty rdf:about="https://saref.etsi.org/saref4bldg/partLoadRatioMax">
        <rdfs:comment xml:lang="en">Maximum part load ratio as a fraction of nominal capacity.</rdfs:comment>
        <rdfs:label xml:lang="en">maximum part load ratio</rdfs:label>
    </owl:ObjectProperty>
    


    <!-- https://saref.etsi.org/saref4bldg/partLoadRatioMin -->


    <owl:ObjectProperty rdf:about="https://saref.etsi.org/saref4bldg/partLoadRatioMin">
        <rdfs:comment xml:lang="en">Minimum part load ratio as a fraction of nominal capacity.</rdfs:comment>
        <rdfs:label xml:lang="en">minimum part load ratio</rdfs:label>
    </owl:ObjectProperty>
    


    <!-- https://saref.etsi.org/saref4bldg/powerOutputMax -->


    <owl:ObjectProperty rdf:about="https://saref.etsi.org/saref4bldg/powerOutputMax">
        <rdfs:comment xml:lang="en">The maximum output power rating of the engine. Usually measured in Watts (W, J/s).</rdfs:comment>
        <rdfs:label xml:lang="en">maximum power output</rdfs:label>
    </owl:ObjectProperty>
    


    <!-- https://saref.etsi.org/saref4bldg/pressureRating -->


    <owl:ObjectProperty rdf:about="https://saref.etsi.org/saref4bldg/pressureRating">
        <rdfs:comment xml:lang="en">Nominal pressure rating of the boiler as rated by the agency having jurisdiction. Usually measured in Pascals (Pa, N/m2).</rdfs:comment>
        <rdfs:label xml:lang="en">pressure rating</rdfs:label>
    </owl:ObjectProperty>
    


    <!-- https://saref.etsi.org/saref4bldg/primaryAirFlowRateMax -->


    <owl:ObjectProperty rdf:about="https://saref.etsi.org/saref4bldg/primaryAirFlowRateMax">
        <rdfs:comment xml:lang="en">Maximum primary airflow that can be delivered. Usually measured in m3/s.</rdfs:comment>
        <rdfs:label xml:lang="en">primary air flow rate range</rdfs:label>
    </owl:ObjectProperty>
    


    <!-- https://saref.etsi.org/saref4bldg/primaryAirFlowRateMin -->


    <owl:ObjectProperty rdf:about="https://saref.etsi.org/saref4bldg/primaryAirFlowRateMin">
        <rdfs:comment xml:lang="en">Minimum primary airflow that can be delivered. Usually measured in m3/s.</rdfs:comment>
        <rdfs:label xml:lang="en">primary air flow rate range</rdfs:label>
    </owl:ObjectProperty>
    


    <!-- https://saref.etsi.org/saref4bldg/primaryApparentPower -->


    <owl:ObjectProperty rdf:about="https://saref.etsi.org/saref4bldg/primaryApparentPower">
        <rdfs:comment xml:lang="en">The power in VA (volt ampere) that has been transformed and that runs into the transformer on the primary side. Usually measured in Watts (W, J/s).</rdfs:comment>
        <rdfs:label xml:lang="en">primary apparent power</rdfs:label>
    </owl:ObjectProperty>
    


    <!-- https://saref.etsi.org/saref4bldg/primaryCurrent -->


    <owl:ObjectProperty rdf:about="https://saref.etsi.org/saref4bldg/primaryCurrent">
        <rdfs:comment xml:lang="en">The current that is going to be transformed and that runs into the transformer on the primary side. Usually measured in Ampere (A).</rdfs:comment>
        <rdfs:label xml:lang="en">primary current</rdfs:label>
    </owl:ObjectProperty>
    


    <!-- https://saref.etsi.org/saref4bldg/primaryFrequency -->


    <owl:ObjectProperty rdf:about="https://saref.etsi.org/saref4bldg/primaryFrequency">
        <rdfs:comment xml:lang="en">The frequency that is going to be transformed and that runs into the transformer on the primary side. Usually measured in cycles/s or Hertz (Hz).</rdfs:comment>
        <rdfs:label xml:lang="en">primary frequency</rdfs:label>
    </owl:ObjectProperty>
    


    <!-- https://saref.etsi.org/saref4bldg/primaryVoltage -->


    <owl:ObjectProperty rdf:about="https://saref.etsi.org/saref4bldg/primaryVoltage">
        <rdfs:comment xml:lang="en">The voltage that is going to be transformed and that runs into the transformer on the primary side. Usually measured in Volts (V, W/A).</rdfs:comment>
        <rdfs:label xml:lang="en">primary voltage</rdfs:label>
    </owl:ObjectProperty>
    


    <!-- https://saref.etsi.org/saref4bldg/pumpFlowRateMax -->


    <owl:ObjectProperty rdf:about="https://saref.etsi.org/saref4bldg/pumpFlowRateMax">
        <rdfs:comment xml:lang="en">Allowable range of volume of fluid being pumped against the resistance specified. Usually measured in kg/s.</rdfs:comment>
        <rdfs:label xml:lang="en">pump flow rate range</rdfs:label>
    </owl:ObjectProperty>
    


    <!-- https://saref.etsi.org/saref4bldg/pumpFlowRateMin -->


    <owl:ObjectProperty rdf:about="https://saref.etsi.org/saref4bldg/pumpFlowRateMin">
        <rdfs:comment xml:lang="en">Allowable range of volume of fluid being pumped against the resistance specified. Usually measured in kg/s.</rdfs:comment>
        <rdfs:label xml:lang="en">pump flow rate range</rdfs:label>
    </owl:ObjectProperty>
    


    <!-- https://saref.etsi.org/saref4bldg/realImpedanceRatio -->


    <owl:ObjectProperty rdf:about="https://saref.etsi.org/saref4bldg/realImpedanceRatio">
        <rdfs:comment xml:lang="en">The ratio between the real part of the zero sequence impedance and the real part of the positive impedance (i.e. real part of the short-circuit voltage) of the transformer. Used for three-phase transformer which includes a N-conductor.</rdfs:comment>
        <rdfs:label xml:lang="en">real impedance ratio</rdfs:label>
    </owl:ObjectProperty>
    


    <!-- https://saref.etsi.org/saref4bldg/secondCurvatureRadius -->


    <owl:ObjectProperty rdf:about="https://saref.etsi.org/saref4bldg/secondCurvatureRadius">
        <rdfs:comment xml:lang="en">SecondCurvatureRadius should be defined as the top or right side radius of curvature value. Usually measured in millimeters (mm).</rdfs:comment>
        <rdfs:label xml:lang="en">second curvature radius</rdfs:label>
    </owl:ObjectProperty>
    


    <!-- https://saref.etsi.org/saref4bldg/secondaryAirFlowRateMax -->


    <owl:ObjectProperty rdf:about="https://saref.etsi.org/saref4bldg/secondaryAirFlowRateMax">
        <rdfs:comment xml:lang="en">Maximum secondary airflow that can be delivered. Usually measured in Pascals (Pa, N/m2).</rdfs:comment>
        <rdfs:label xml:lang="en">secondary air flow rate range</rdfs:label>
    </owl:ObjectProperty>
    


    <!-- https://saref.etsi.org/saref4bldg/secondaryAirFlowRateMin -->


    <owl:ObjectProperty rdf:about="https://saref.etsi.org/saref4bldg/secondaryAirFlowRateMin">
        <rdfs:comment xml:lang="en">Maximum secondary airflow that can be delivered. Usually measured in Pascals (Pa, N/m2).</rdfs:comment>
        <rdfs:label xml:lang="en">secondary air flow rate range</rdfs:label>
    </owl:ObjectProperty>
    


    <!-- https://saref.etsi.org/saref4bldg/secondaryApparentPower -->


    <owl:ObjectProperty rdf:about="https://saref.etsi.org/saref4bldg/secondaryApparentPower">
        <rdfs:comment xml:lang="en">The power in VA (volt ampere) that has been transformed and is running out of the transformer on the secondary side. Usually measured in Watts (W, J/s).</rdfs:comment>
        <rdfs:label xml:lang="en">secondary apparent power</rdfs:label>
    </owl:ObjectProperty>
    


    <!-- https://saref.etsi.org/saref4bldg/secondaryCurrent -->


    <owl:ObjectProperty rdf:about="https://saref.etsi.org/saref4bldg/secondaryCurrent">
        <rdfs:comment xml:lang="en">The current that has been transformed and is running out of the transformer on the secondary side. Usually measured in Ampere (A).</rdfs:comment>
        <rdfs:label xml:lang="en">secondary current</rdfs:label>
    </owl:ObjectProperty>
    


    <!-- https://saref.etsi.org/saref4bldg/secondaryFrequency -->


    <owl:ObjectProperty rdf:about="https://saref.etsi.org/saref4bldg/secondaryFrequency">
        <rdfs:comment xml:lang="en">The frequency that has been transformed and is running out of the transformer on the secondary side. Usually measured in cycles/s or Hertz (Hz).</rdfs:comment>
        <rdfs:label xml:lang="en">secondary frequency</rdfs:label>
    </owl:ObjectProperty>
    


    <!-- https://saref.etsi.org/saref4bldg/secondaryVoltage -->


    <owl:ObjectProperty rdf:about="https://saref.etsi.org/saref4bldg/secondaryVoltage">
        <rdfs:comment xml:lang="en">The voltage that has been transformed and is running out of the transformer on the secondary side. Usually measured in Volts (V, W/A).</rdfs:comment>
        <rdfs:label xml:lang="en">secondary voltage</rdfs:label>
    </owl:ObjectProperty>
    


    <!-- https://saref.etsi.org/saref4bldg/shortCircuitVoltage -->


    <owl:ObjectProperty rdf:about="https://saref.etsi.org/saref4bldg/shortCircuitVoltage">
        <rdfs:comment xml:lang="en">A complex number that specifies the real and imaginary parts of the short-circuit voltage at rated current of a transformer given in %.</rdfs:comment>
        <rdfs:label xml:lang="en">short circuit voltage</rdfs:label>
    </owl:ObjectProperty>
    


    <!-- https://saref.etsi.org/saref4bldg/size -->


    <owl:ObjectProperty rdf:about="https://saref.etsi.org/saref4bldg/size">
        <rdfs:comment xml:lang="en">The size of the connection to the valve (or to each connection for faucets, mixing valves, etc.). Usually measured in millimeters (mm).</rdfs:comment>
        <rdfs:label xml:lang="en">size</rdfs:label>
    </owl:ObjectProperty>
    


    <!-- https://saref.etsi.org/saref4bldg/solarReflectance -->


    <owl:ObjectProperty rdf:about="https://saref.etsi.org/saref4bldg/solarReflectance">
        <rdfs:comment xml:lang="en">(Rsol): The ratio of incident solar radiation that is reflected by a shading system (also named _e). Note the following equation Asol + Rsol + Tsol = 1</rdfs:comment>
        <rdfs:label xml:lang="en">solar reflectance</rdfs:label>
    </owl:ObjectProperty>
    


    <!-- https://saref.etsi.org/saref4bldg/solarTransmittance -->


    <owl:ObjectProperty rdf:about="https://saref.etsi.org/saref4bldg/solarTransmittance">
        <rdfs:comment xml:lang="en">(Tsol) The ratio of incident solar radiation that directly passes through a shading system (also named _e). Note the following equation Asol + Rsol + Tsol = 1</rdfs:comment>
        <rdfs:label xml:lang="en">solar transmittance</rdfs:label>
    </owl:ObjectProperty>
    


    <!-- https://saref.etsi.org/saref4bldg/spectrumMax -->


    <owl:ObjectProperty rdf:about="https://saref.etsi.org/saref4bldg/spectrumMax">
        <rdfs:comment xml:lang="en">The spectrum of radiation describes its composition with regard to wavelength. Light, for example, as the portion of electromagnetic radiation that is visible to the human eye, is radiation with wavelengths in the range of approx. 380 to 780 nm (1 nm = 10 m). The corresponding range of colours varies from violet to indigo, blue, green, yellow, orange, and red. These colours form a continuous spectrum, in which the various spectral sectors merge into each other.</rdfs:comment>
        <rdfs:label xml:lang="en">maximum spectrum</rdfs:label>
    </owl:ObjectProperty>
    


    <!-- https://saref.etsi.org/saref4bldg/spectrumMin -->


    <owl:ObjectProperty rdf:about="https://saref.etsi.org/saref4bldg/spectrumMin">
        <rdfs:comment xml:lang="en">The spectrum of radiation describes its composition with regard to wavelength. Light, for example, as the portion of electromagnetic radiation that is visible to the human eye, is radiation with wavelengths in the range of approx. 380 to 780 nm (1 nm = 10 m). The corresponding range of colours varies from violet to indigo, blue, green, yellow, orange, and red. These colours form a continuous spectrum, in which the various spectral sectors merge into each other.</rdfs:comment>
        <rdfs:label xml:lang="en">minimum spectrum</rdfs:label>
    </owl:ObjectProperty>
    


    <!-- https://saref.etsi.org/saref4bldg/staggeredRowSpacing -->


    <owl:ObjectProperty rdf:about="https://saref.etsi.org/saref4bldg/staggeredRowSpacing">
        <rdfs:comment xml:lang="en">Staggered tube row spacing. Usually measured in millimeters (mm).</rdfs:comment>
        <rdfs:label xml:lang="en">staggered row spacing</rdfs:label>
    </owl:ObjectProperty>
    


    <!-- https://saref.etsi.org/saref4bldg/startCurrentFactor -->


    <owl:ObjectProperty rdf:about="https://saref.etsi.org/saref4bldg/startCurrentFactor">
        <rdfs:comment xml:lang="en">IEC. Start current factor defines how large the peek starting current will become on the engine. StartCurrentFactor is multiplied to NominalCurrent and we get the start current.</rdfs:comment>
        <rdfs:label xml:lang="en">start current factor</rdfs:label>
    </owl:ObjectProperty>
    


    <!-- https://saref.etsi.org/saref4bldg/startingTime -->


    <owl:ObjectProperty rdf:about="https://saref.etsi.org/saref4bldg/startingTime">
        <rdfs:comment xml:lang="en">The time (in s) needed for the motor to reach its rated speed with its driven equipment attached, starting from standstill and at the nominal voltage applied at its terminals.</rdfs:comment>
        <rdfs:label xml:lang="en">starting time</rdfs:label>
    </owl:ObjectProperty>
    


    <!-- https://saref.etsi.org/saref4bldg/supportedWeightMax -->


    <owl:ObjectProperty rdf:about="https://saref.etsi.org/saref4bldg/supportedWeightMax">
        <rdfs:comment xml:lang="en">The maximum weight that can be carried by the vibration isolator. Usually measured in kilograms (kg) or grams (g).</rdfs:comment>
        <rdfs:label xml:lang="en">maximum supported weight</rdfs:label>
    </owl:ObjectProperty>
    


    <!-- https://saref.etsi.org/saref4bldg/teTime -->


    <owl:ObjectProperty rdf:about="https://saref.etsi.org/saref4bldg/teTime">
        <rdfs:comment xml:lang="en">The maximum time (in s) at which the motor could run with locked rotor when the motor is used in an EX-environment. The time indicates that a protective device should trip before this time when the starting current of the motor is slowing through the device.</rdfs:comment>
        <rdfs:label xml:lang="en">te time</rdfs:label>
    </owl:ObjectProperty>
    


    <!-- https://saref.etsi.org/saref4bldg/temperatureRating -->


    <owl:ObjectProperty rdf:about="https://saref.etsi.org/saref4bldg/temperatureRating">
        <rdfs:comment xml:lang="en">Temperature rating. Usually measured in degrees Kelvin (K).</rdfs:comment>
        <rdfs:label xml:lang="en">temperature rating</rdfs:label>
    </owl:ObjectProperty>
    


    <!-- https://saref.etsi.org/saref4bldg/testPressure -->


    <owl:ObjectProperty rdf:about="https://saref.etsi.org/saref4bldg/testPressure">
        <rdfs:comment xml:lang="en">The maximum pressure to which the valve has been subjected under test. Usually measured in Pascals (Pa, N/m2).</rdfs:comment>
        <rdfs:label xml:lang="en">test pressure</rdfs:label>
    </owl:ObjectProperty>
    


    <!-- https://saref.etsi.org/saref4bldg/thermalConductivity -->


    <owl:ObjectProperty rdf:about="https://saref.etsi.org/saref4bldg/thermalConductivity">
        <rdfs:comment xml:lang="en">Fouling factor of the tubes in the tube bundle. Usually measured in m2 Kelvin/Watt.</rdfs:comment>
        <rdfs:label xml:lang="en">thermal conductivity</rdfs:label>
    </owl:ObjectProperty>
    


    <!-- https://saref.etsi.org/saref4bldg/thermalEfficiency -->


    <owl:ObjectProperty rdf:about="https://saref.etsi.org/saref4bldg/thermalEfficiency">
        <rdfs:comment xml:lang="en">Overall Thermal Efficiency is defined as gross energy output of the heat transfer device divided by the energy input.</rdfs:comment>
        <rdfs:label xml:lang="en">thermal efficiency</rdfs:label>
    </owl:ObjectProperty>
    


    <!-- https://saref.etsi.org/saref4bldg/thermalMassHeatCapacity -->


    <owl:ObjectProperty rdf:about="https://saref.etsi.org/saref4bldg/thermalMassHeatCapacity">
        <rdfs:comment xml:lang="en">Product of component mass and specific heat.</rdfs:comment>
        <rdfs:label xml:lang="en">thermal mass heat capacity</rdfs:label>
    </owl:ObjectProperty>
    


    <!-- https://saref.etsi.org/saref4bldg/thermalTransmittance -->


    <owl:ObjectProperty rdf:about="https://saref.etsi.org/saref4bldg/thermalTransmittance">
        <rdfs:comment xml:lang="en">Rate at which energy is transmitted through a body. Usually measured in Watts/m2 Kelvin.</rdfs:comment>
        <rdfs:label xml:lang="en">thermal transmittance</rdfs:label>
    </owl:ObjectProperty>
    


    <!-- https://saref.etsi.org/saref4bldg/ventilatingPipeSize -->


    <owl:ObjectProperty rdf:about="https://saref.etsi.org/saref4bldg/ventilatingPipeSize">
        <rdfs:comment xml:lang="en">Size of the ventilating pipe(s). Usually measured in millimeters (mm).</rdfs:comment>
        <rdfs:label xml:lang="en">ventilating pipe size</rdfs:label>
    </owl:ObjectProperty>
    


    <!-- https://saref.etsi.org/saref4bldg/verticalSpacing -->


    <owl:ObjectProperty rdf:about="https://saref.etsi.org/saref4bldg/verticalSpacing">
        <rdfs:comment xml:lang="en">Vertical spacing between tubes in the tube bundle.Usually measured in millimeters (mm).</rdfs:comment>
        <rdfs:label xml:lang="en">vertical spacing</rdfs:label>
    </owl:ObjectProperty>
    


    <!-- https://saref.etsi.org/saref4bldg/vibrationTransmissibility -->


    <owl:ObjectProperty rdf:about="https://saref.etsi.org/saref4bldg/vibrationTransmissibility">
        <rdfs:comment xml:lang="en">The vibration transmissibility percentage.</rdfs:comment>
        <rdfs:label xml:lang="en">vibration transmissibility</rdfs:label>
    </owl:ObjectProperty>
    


    <!-- https://saref.etsi.org/saref4bldg/visibleLightReflectance -->


    <owl:ObjectProperty rdf:about="https://saref.etsi.org/saref4bldg/visibleLightReflectance">
        <rdfs:comment xml:lang="en">Fraction of the visible light that is reflected by the glazing at normal incidence. It is a value without unit.</rdfs:comment>
        <rdfs:label xml:lang="en">visible light reflectance</rdfs:label>
    </owl:ObjectProperty>
    


    <!-- https://saref.etsi.org/saref4bldg/visibleLightTransmittance -->


    <owl:ObjectProperty rdf:about="https://saref.etsi.org/saref4bldg/visibleLightTransmittance">
        <rdfs:comment xml:lang="en">Fraction of the visible light that passes the shading system at normal incidence. It is a value without unit.</rdfs:comment>
        <rdfs:label xml:lang="en">visible light transmittance</rdfs:label>
    </owl:ObjectProperty>
    


    <!-- https://saref.etsi.org/saref4bldg/volumen -->


    <owl:ObjectProperty rdf:about="https://saref.etsi.org/saref4bldg/volumen">
        <rdfs:comment xml:lang="en">Total volume of fluid in the tubes and their headers. Usually measured in cubic metre (m3).</rdfs:comment>
        <rdfs:label xml:lang="en">volumen</rdfs:label>
    </owl:ObjectProperty>
    


    <!-- https://saref.etsi.org/saref4bldg/waterInletTemperatureMax -->


    <owl:ObjectProperty rdf:about="https://saref.etsi.org/saref4bldg/waterInletTemperatureMax">
        <rdfs:comment xml:lang="en">Allowable water inlet temperature range. Usually measured in degrees Kelvin (K).</rdfs:comment>
        <rdfs:label xml:lang="en">water inlet temperature range</rdfs:label>
    </owl:ObjectProperty>
    


    <!-- https://saref.etsi.org/saref4bldg/waterInletTemperatureMin -->


    <owl:ObjectProperty rdf:about="https://saref.etsi.org/saref4bldg/waterInletTemperatureMin">
        <rdfs:comment xml:lang="en">Allowable water inlet temperature range. Usually measured in degrees Kelvin (K).</rdfs:comment>
        <rdfs:label xml:lang="en">water inlet temperature range</rdfs:label>
    </owl:ObjectProperty>
    


    <!-- https://saref.etsi.org/saref4bldg/waterPressureMax -->


    <owl:ObjectProperty rdf:about="https://saref.etsi.org/saref4bldg/waterPressureMax">
        <rdfs:comment xml:lang="en">Allowable water circuit working pressure range. Usually measured in Pascals (Pa, N/m2).</rdfs:comment>
        <rdfs:label xml:lang="en">water pressure range</rdfs:label>
    </owl:ObjectProperty>
    


    <!-- https://saref.etsi.org/saref4bldg/waterPressureMin -->


    <owl:ObjectProperty rdf:about="https://saref.etsi.org/saref4bldg/waterPressureMin">
        <rdfs:comment xml:lang="en">Allowable water circuit working pressure range. Usually measured in Pascals (Pa, N/m2).</rdfs:comment>
        <rdfs:label xml:lang="en">water pressure range</rdfs:label>
    </owl:ObjectProperty>
    


    <!-- https://saref.etsi.org/saref4bldg/waterRequirement -->


    <owl:ObjectProperty rdf:about="https://saref.etsi.org/saref4bldg/waterRequirement">
        <rdfs:comment xml:lang="en">Make-up water requirement. Usually measured in m3/s.</rdfs:comment>
        <rdfs:label xml:lang="en">water requirement</rdfs:label>
    </owl:ObjectProperty>
    


    <!-- https://saref.etsi.org/saref4bldg/waterStorageCapacity -->


    <owl:ObjectProperty rdf:about="https://saref.etsi.org/saref4bldg/waterStorageCapacity">
        <rdfs:comment xml:lang="en">Water storage capacity. Usually measured in cubic metre (m3).</rdfs:comment>
        <rdfs:label xml:lang="en">water storage capacity</rdfs:label>
    </owl:ObjectProperty>
    


    <!-- https://saref.etsi.org/saref4bldg/weight -->


    <owl:ObjectProperty rdf:about="https://saref.etsi.org/saref4bldg/weight">
        <rdfs:comment xml:lang="en">The weight of the device. Usually measured in kilograms (kg) or grams (g).</rdfs:comment>
        <rdfs:label xml:lang="en">weight</rdfs:label>
    </owl:ObjectProperty>
    


    <!-- https://saref.etsi.org/saref4bldg/workingPressure -->


    <owl:ObjectProperty rdf:about="https://saref.etsi.org/saref4bldg/workingPressure">
        <rdfs:comment xml:lang="en">The normally expected maximum working pressure of the valve. Usually measured in Pascals (Pa, N/m2).</rdfs:comment>
        <rdfs:label xml:lang="en">working pressure</rdfs:label>
    </owl:ObjectProperty>
    


    <!-- https://saref.etsi.org/saref4bldg/workingPressureMax -->


    <owl:ObjectProperty rdf:about="https://saref.etsi.org/saref4bldg/workingPressureMax">
        <rdfs:comment xml:lang="en">Maximum working pressure. Usually measured in Pascals (Pa, N/m2).</rdfs:comment>
        <rdfs:label xml:lang="en">maximum working pressure</rdfs:label>
    </owl:ObjectProperty>
    


    <!-- https://saref.etsi.org/saref4bldg/workingPressureMin -->


    <owl:ObjectProperty rdf:about="https://saref.etsi.org/saref4bldg/workingPressureMin">
        <rdfs:comment xml:lang="en">Allowable minimum working pressure (relative to ambient pressure). Usually measured in Pascals (Pa, N/m2).</rdfs:comment>
        <rdfs:label xml:lang="en">minimum working pressure</rdfs:label>
    </owl:ObjectProperty>
    


    <!-- https://saref.etsi.org/saref4city/assesses -->


    <owl:ObjectProperty rdf:about="https://saref.etsi.org/saref4city/assesses">
        <rdfs:isDefinedBy rdf:resource="https://saref.etsi.org/saref4city/"/>
        <rdfs:label xml:lang="en">assesses</rdfs:label>
    </owl:ObjectProperty>
    


    <!-- https://saref.etsi.org/saref4city/hasCalculationPeriod -->


    <owl:ObjectProperty rdf:about="https://saref.etsi.org/saref4city/hasCalculationPeriod">
        <rdfs:isDefinedBy rdf:resource="https://saref.etsi.org/saref4city/"/>
        <rdfs:label xml:lang="en">has calculation period</rdfs:label>
    </owl:ObjectProperty>
    


    <!-- https://saref.etsi.org/saref4city/hasKPI -->


    <owl:ObjectProperty rdf:about="https://saref.etsi.org/saref4city/hasKPI">
        <owl:inverseOf rdf:resource="https://saref.etsi.org/saref4city/isKPIOf"/>
        <rdfs:isDefinedBy rdf:resource="https://saref.etsi.org/saref4city/"/>
        <rdfs:label xml:lang="en">has key performance indicator</rdfs:label>
    </owl:ObjectProperty>
    


    <!-- https://saref.etsi.org/saref4city/isAssessedBy -->


    <owl:ObjectProperty rdf:about="https://saref.etsi.org/saref4city/isAssessedBy">
        <rdfs:isDefinedBy rdf:resource="https://saref.etsi.org/saref4city/"/>
        <rdfs:label xml:lang="en">is assessed by</rdfs:label>
    </owl:ObjectProperty>
    


    <!-- https://saref.etsi.org/saref4city/isDerivedFrom -->


    <owl:ObjectProperty rdf:about="https://saref.etsi.org/saref4city/isDerivedFrom">
        <rdfs:isDefinedBy rdf:resource="https://saref.etsi.org/saref4city/"/>
        <rdfs:label xml:lang="en">is derived from</rdfs:label>
    </owl:ObjectProperty>
    


    <!-- https://saref.etsi.org/saref4city/isKPIOf -->


    <owl:ObjectProperty rdf:about="https://saref.etsi.org/saref4city/isKPIOf">
        <rdfs:isDefinedBy rdf:resource="https://saref.etsi.org/saref4city/"/>
        <rdfs:label xml:lang="en">is key performance indicator of</rdfs:label>
    </owl:ObjectProperty>
    


    <!-- https://saref.etsi.org/saref4city/quantifiesKPI -->


    <owl:ObjectProperty rdf:about="https://saref.etsi.org/saref4city/quantifiesKPI">
        <rdfs:isDefinedBy rdf:resource="https://saref.etsi.org/saref4city/"/>
        <rdfs:label xml:lang="en">quantifies KPI</rdfs:label>
    </owl:ObjectProperty>
    


    <!-- https://saref.etsi.org/saref4city/refersToFeature -->


    <owl:ObjectProperty rdf:about="https://saref.etsi.org/saref4city/refersToFeature">
        <rdfs:comment xml:lang="en">Relation between a KPI assessment and the geographical feature it refers to</rdfs:comment>
        <rdfs:isDefinedBy rdf:resource="https://saref.etsi.org/saref4city/"/>
        <rdfs:label xml:lang="en">refers to feature</rdfs:label>
    </owl:ObjectProperty>
    


    <!-- https://saref.etsi.org/saref4city/refersToTime -->


    <owl:ObjectProperty rdf:about="https://saref.etsi.org/saref4city/refersToTime">
        <rdfs:isDefinedBy rdf:resource="https://saref.etsi.org/saref4city/"/>
        <rdfs:label xml:lang="en">refers to time</rdfs:label>
    </owl:ObjectProperty>
    


    <!-- https://saref.etsi.org/saref4syst/connectedThrough -->


    <owl:ObjectProperty rdf:about="https://saref.etsi.org/saref4syst/connectedThrough">
        <owl:inverseOf rdf:resource="https://saref.etsi.org/saref4syst/connectsSystem"/>
        <rdfs:domain rdf:resource="https://saref.etsi.org/saref4syst/System"/>
        <rdfs:range rdf:resource="https://saref.etsi.org/saref4syst/Connection"/>
        <owl:propertyChainAxiom rdf:parseType="Collection">
            <rdf:Description rdf:about="https://saref.etsi.org/saref4syst/connectsAt"/>
            <rdf:Description rdf:about="https://saref.etsi.org/saref4syst/connectsSystemThrough"/>
        </owl:propertyChainAxiom>
        <rdfs:comment xml:lang="en">Links a system to one of its connections to other systems.</rdfs:comment>
        <rdfs:label xml:lang="en">connected through</rdfs:label>
    </owl:ObjectProperty>
    


    <!-- https://saref.etsi.org/saref4syst/connectedTo -->


    <owl:ObjectProperty rdf:about="https://saref.etsi.org/saref4syst/connectedTo">
        <rdf:type rdf:resource="http://www.w3.org/2002/07/owl#SymmetricProperty"/>
        <rdfs:domain rdf:resource="https://saref.etsi.org/saref4syst/System"/>
        <rdfs:range rdf:resource="https://saref.etsi.org/saref4syst/System"/>
        <rdfs:comment xml:lang="en">Links a system to a system it is connected to. Connected systems interact in some way. The exact meaning of &quot;interact&quot; is defined by sub properties of s4syst:connectedTo. Property s4syst:connectedTo is symmetric. This property can be qualified using class s4syst:Connection, which connects the two systems. If there is a connection between several systems, then one may infer these systems are pairwise connected.</rdfs:comment>
        <rdfs:label xml:lang="en">connected to</rdfs:label>
    </owl:ObjectProperty>
    


    <!-- https://saref.etsi.org/saref4syst/connectionPointOf -->


    <owl:ObjectProperty rdf:about="https://saref.etsi.org/saref4syst/connectionPointOf">
        <owl:inverseOf rdf:resource="https://saref.etsi.org/saref4syst/connectsAt"/>
        <rdf:type rdf:resource="http://www.w3.org/2002/07/owl#FunctionalProperty"/>
        <rdfs:domain rdf:resource="https://saref.etsi.org/saref4syst/ConnectionPoint"/>
        <rdfs:range rdf:resource="https://saref.etsi.org/saref4syst/System"/>
        <rdfs:comment xml:lang="en">Links a connection point to the one and only one system it belongs to.</rdfs:comment>
        <rdfs:label xml:lang="en">connection point to</rdfs:label>
    </owl:ObjectProperty>
    


    <!-- https://saref.etsi.org/saref4syst/connectsAt -->


    <owl:ObjectProperty rdf:about="https://saref.etsi.org/saref4syst/connectsAt">
        <rdf:type rdf:resource="http://www.w3.org/2002/07/owl#InverseFunctionalProperty"/>
        <rdfs:domain rdf:resource="https://saref.etsi.org/saref4syst/System"/>
        <rdfs:range rdf:resource="https://saref.etsi.org/saref4syst/ConnectionPoint"/>
        <rdfs:comment xml:lang="en">Links a system to one of the connection points at which it connects.</rdfs:comment>
        <rdfs:label xml:lang="en">connects at</rdfs:label>
    </owl:ObjectProperty>
    


    <!-- https://saref.etsi.org/saref4syst/connectsSystem -->


    <owl:ObjectProperty rdf:about="https://saref.etsi.org/saref4syst/connectsSystem">
        <rdfs:domain rdf:resource="https://saref.etsi.org/saref4syst/Connection"/>
        <rdfs:range rdf:resource="https://saref.etsi.org/saref4syst/System"/>
        <owl:propertyChainAxiom rdf:parseType="Collection">
            <rdf:Description rdf:about="https://saref.etsi.org/saref4syst/connectsSystemAt"/>
            <rdf:Description rdf:about="https://saref.etsi.org/saref4syst/connectionPointOf"/>
        </owl:propertyChainAxiom>
        <rdfs:comment xml:lang="en">Links a connection to one of the systems it connects.</rdfs:comment>
        <rdfs:label xml:lang="en">connects system</rdfs:label>
    </owl:ObjectProperty>
    


    <!-- https://saref.etsi.org/saref4syst/connectsSystemAt -->


    <owl:ObjectProperty rdf:about="https://saref.etsi.org/saref4syst/connectsSystemAt">
        <owl:inverseOf rdf:resource="https://saref.etsi.org/saref4syst/connectsSystemThrough"/>
        <rdfs:domain rdf:resource="https://saref.etsi.org/saref4syst/Connection"/>
        <rdfs:range rdf:resource="https://saref.etsi.org/saref4syst/ConnectionPoint"/>
        <rdfs:comment xml:lang="en">Links a connection to one of the connection points at which it connects a system.</rdfs:comment>
        <rdfs:label xml:lang="en">connects system at</rdfs:label>
    </owl:ObjectProperty>
    


    <!-- https://saref.etsi.org/saref4syst/connectsSystemThrough -->


    <owl:ObjectProperty rdf:about="https://saref.etsi.org/saref4syst/connectsSystemThrough">
        <rdfs:domain rdf:resource="https://saref.etsi.org/saref4syst/ConnectionPoint"/>
        <rdfs:range rdf:resource="https://saref.etsi.org/saref4syst/Connection"/>
        <rdfs:comment xml:lang="en">Links a connection point to one of the connections through which it connects its system.</rdfs:comment>
        <rdfs:label xml:lang="en">connects system through</rdfs:label>
    </owl:ObjectProperty>
    


    <!-- https://saref.etsi.org/saref4syst/hasSubSystem -->


    <owl:ObjectProperty rdf:about="https://saref.etsi.org/saref4syst/hasSubSystem">
        <owl:inverseOf rdf:resource="https://saref.etsi.org/saref4syst/subSystemOf"/>
        <rdf:type rdf:resource="http://www.w3.org/2002/07/owl#TransitiveProperty"/>
        <rdfs:domain rdf:resource="https://saref.etsi.org/saref4syst/System"/>
        <rdfs:range rdf:resource="https://saref.etsi.org/saref4syst/System"/>
        <rdfs:comment xml:lang="en">Links a system to one of its sub systems.</rdfs:comment>
        <rdfs:isDefinedBy rdf:resource="https://saref.etsi.org/saref4syst/"/>
        <rdfs:label xml:lang="en">has sub system</rdfs:label>
        <rdfs:label xml:lang="en">has sub-system</rdfs:label>
    </owl:ObjectProperty>
    


    <!-- https://saref.etsi.org/saref4syst/subSystemOf -->


    <owl:ObjectProperty rdf:about="https://saref.etsi.org/saref4syst/subSystemOf">
        <rdf:type rdf:resource="http://www.w3.org/2002/07/owl#TransitiveProperty"/>
        <rdfs:domain rdf:resource="https://saref.etsi.org/saref4syst/System"/>
        <rdfs:range rdf:resource="https://saref.etsi.org/saref4syst/System"/>
        <rdfs:comment xml:lang="en">Links a system to its super system. Properties of subsystems somehow contribute to the properties of the super system. The exact meaning of &quot;contribute is defined by sub properties of s4syst:subSystemOf. Property s4syst:subSystemOf is transitive.</rdfs:comment>
        <rdfs:label xml:lang="en">sub system of</rdfs:label>
    </owl:ObjectProperty>
    


    <!-- https://saref.etsi.org/saref4watr/appliesTo -->


    <owl:ObjectProperty rdf:about="https://saref.etsi.org/saref4watr/appliesTo">
        <rdfs:domain rdf:resource="https://saref.etsi.org/saref4watr/Tariff"/>
        <rdfs:range rdf:resource="https://saref.etsi.org/saref4watr/WaterMeter"/>
        <rdfs:comment xml:lang="en">The water meter to which a tariff applies to.</rdfs:comment>
        <rdfs:label xml:lang="en">applies to</rdfs:label>
    </owl:ObjectProperty>
    


    <!-- https://saref.etsi.org/saref4watr/controlsFeature -->


    <owl:ObjectProperty rdf:about="https://saref.etsi.org/saref4watr/controlsFeature">
        <rdfs:domain rdf:resource="https://saref.etsi.org/core/Device"/>
        <rdfs:range rdf:resource="https://saref.etsi.org/core/FeatureOfInterest"/>
        <rdfs:comment xml:lang="en">A relationship specifying the features of interest that are controlled by a device.</rdfs:comment>
        <rdfs:label xml:lang="en">controls feature</rdfs:label>
    </owl:ObjectProperty>
    


    <!-- https://saref.etsi.org/saref4watr/featureIsControlledByDevice -->


    <owl:ObjectProperty rdf:about="https://saref.etsi.org/saref4watr/featureIsControlledByDevice">
        <rdfs:domain rdf:resource="https://saref.etsi.org/core/FeatureOfInterest"/>
        <rdfs:range rdf:resource="https://saref.etsi.org/core/Device"/>
        <rdfs:comment xml:lang="en">A relationship specifying the devices that control a feature of interest.</rdfs:comment>
        <rdfs:label xml:lang="en">feature is controlled by device</rdfs:label>
    </owl:ObjectProperty>
    


    <!-- https://saref.etsi.org/saref4watr/featureIsMeasuredByDevice -->


    <owl:ObjectProperty rdf:about="https://saref.etsi.org/saref4watr/featureIsMeasuredByDevice">
        <rdfs:domain rdf:resource="https://saref.etsi.org/core/FeatureOfInterest"/>
        <rdfs:range rdf:resource="https://saref.etsi.org/core/Device"/>
        <rdfs:comment xml:lang="en">A relationship specifying the devices that measure a feature of interest.</rdfs:comment>
        <rdfs:label xml:lang="en">feature is measured by device</rdfs:label>
    </owl:ObjectProperty>
    


    <!-- https://saref.etsi.org/saref4watr/forAbsoluteTimeAtDay -->


    <owl:ObjectProperty rdf:about="https://saref.etsi.org/saref4watr/forAbsoluteTimeAtDay">
        <rdfs:domain rdf:resource="https://saref.etsi.org/saref4watr/TimeBasedTariff"/>
        <rdfs:range rdf:resource="http://www.w3.org/2006/time#Interval"/>
        <rdfs:comment xml:lang="en">The time interval in each day for which a tariff is applied (e.g., 8:00 to 10:00).</rdfs:comment>
        <rdfs:label xml:lang="en">for absolute time at day</rdfs:label>
    </owl:ObjectProperty>
    


    <!-- https://saref.etsi.org/saref4watr/forWeekDay -->


    <owl:ObjectProperty rdf:about="https://saref.etsi.org/saref4watr/forWeekDay">
        <rdfs:domain rdf:resource="https://saref.etsi.org/saref4watr/TimeBasedTariff"/>
        <rdfs:range rdf:resource="http://www.w3.org/2006/time#DayOfWeek"/>
        <rdfs:comment xml:lang="en">The day of the week for which a tariff is applied (e.g., each Saturday and Sunday).</rdfs:comment>
        <rdfs:label xml:lang="en">for week day</rdfs:label>
    </owl:ObjectProperty>
    


    <!-- https://saref.etsi.org/saref4watr/hasBillingPeriod -->


    <owl:ObjectProperty rdf:about="https://saref.etsi.org/saref4watr/hasBillingPeriod">
        <rdfs:domain rdf:resource="https://saref.etsi.org/saref4watr/Tariff"/>
        <rdfs:range rdf:resource="http://www.w3.org/2006/time#TemporalDuration"/>
        <rdfs:comment xml:lang="en">The billing period of a tariff.</rdfs:comment>
        <rdfs:label xml:lang="en">has billing period</rdfs:label>
    </owl:ObjectProperty>
    


    <!-- https://saref.etsi.org/saref4watr/hasDuration -->


    <owl:ObjectProperty rdf:about="https://saref.etsi.org/saref4watr/hasDuration">
        <rdfs:domain rdf:resource="https://saref.etsi.org/saref4watr/Tariff"/>
        <rdfs:range rdf:resource="http://www.w3.org/2006/time#TemporalDuration"/>
        <rdfs:comment xml:lang="en">The duration of a tariff.</rdfs:comment>
        <rdfs:label xml:lang="en">has duration</rdfs:label>
    </owl:ObjectProperty>
    


    <!-- https://saref.etsi.org/saref4watr/hasPeriod -->


    <owl:ObjectProperty rdf:about="https://saref.etsi.org/saref4watr/hasPeriod">
        <rdfs:domain rdf:resource="https://saref.etsi.org/saref4watr/Tariff"/>
        <rdfs:range rdf:resource="http://www.w3.org/2006/time#TemporalDuration"/>
        <rdfs:comment xml:lang="en">The period of a tariff.</rdfs:comment>
        <rdfs:label xml:lang="en">has period</rdfs:label>
    </owl:ObjectProperty>
    


    <!-- https://saref.etsi.org/saref4watr/hasPhenomenonTime -->


    <owl:ObjectProperty rdf:about="https://saref.etsi.org/saref4watr/hasPhenomenonTime">
        <rdfs:domain rdf:resource="https://saref.etsi.org/core/Measurement"/>
        <rdfs:range rdf:resource="http://www.w3.org/2006/time#TemporalEntity"/>
        <rdfs:comment xml:lang="en">The time for which the value of a measurement applies to the feature of interest.</rdfs:comment>
        <rdfs:label xml:lang="en">has phenomenon time</rdfs:label>
    </owl:ObjectProperty>
    


    <!-- https://saref.etsi.org/saref4watr/isDesignedFor -->


    <owl:ObjectProperty rdf:about="https://saref.etsi.org/saref4watr/isDesignedFor">
        <rdfs:comment xml:lang="en">The type of water for which an infrastructure is designed for.</rdfs:comment>
        <rdfs:label xml:lang="en">is designed for</rdfs:label>
    </owl:ObjectProperty>
    


    <!-- https://saref.etsi.org/saref4watr/isIntendedFor -->


    <owl:ObjectProperty rdf:about="https://saref.etsi.org/saref4watr/isIntendedFor">
        <rdfs:comment xml:lang="en">The intended use of the infrastructure.</rdfs:comment>
        <rdfs:label xml:lang="en">is intended for</rdfs:label>
    </owl:ObjectProperty>
    


    <!-- https://saref.etsi.org/saref4watr/measuresFeature -->


    <owl:ObjectProperty rdf:about="https://saref.etsi.org/saref4watr/measuresFeature">
        <rdfs:domain rdf:resource="https://saref.etsi.org/core/Device"/>
        <rdfs:range rdf:resource="https://saref.etsi.org/core/FeatureOfInterest"/>
        <rdfs:comment xml:lang="en">A relationship specifying the features of interest that are measured by a device.</rdfs:comment>
        <rdfs:label xml:lang="en">measures feature</rdfs:label>
    </owl:ObjectProperty>
    


    <!-- https://www.geonames.org/ontology#parentADM2 -->


    <owl:ObjectProperty rdf:about="https://www.geonames.org/ontology#parentADM2"/>
    


    <!-- https://www.geonames.org/ontology#parentADM3 -->


    <owl:ObjectProperty rdf:about="https://www.geonames.org/ontology#parentADM3"/>
    


    <!-- 
    ///////////////////////////////////////////////////////////////////////////////////////
    //
    // Data properties
    //
    ///////////////////////////////////////////////////////////////////////////////////////
     -->


    


    <!-- http://schema.org/familyName -->


    <owl:DatatypeProperty rdf:about="http://schema.org/familyName"/>
    


    <!-- http://schema.org/givenName -->


    <owl:DatatypeProperty rdf:about="http://schema.org/givenName"/>
    


    <!-- http://schema.org/name -->


    <owl:DatatypeProperty rdf:about="http://schema.org/name"/>
    


    <!-- http://www.opengis.net/ont/geosparql#asDGGS -->


    <owl:DatatypeProperty rdf:about="http://www.opengis.net/ont/geosparql#asDGGS">
        <rdfs:subPropertyOf rdf:resource="http://www.opengis.net/ont/geosparql#hasSerialization"/>
        <rdfs:domain rdf:resource="http://www.opengis.net/ont/geosparql#Geometry"/>
        <rdfs:range rdf:resource="http://www.opengis.net/ont/geosparql#dggsLiteral"/>
        <rdfs:isDefinedBy rdf:resource="http://www.opengis.net/ont/geosparql#"/>
        <rdfs:isDefinedBy rdf:resource="http://www.opengis.net/spec/geosparql/1.1/req/geometry-extension/geometry-as-dggs-literal"/>
        <skos:definition xml:lang="en">The Discrete Global Grid System (DGGS) serialization of a Geometry</skos:definition>
        <skos:example rdf:resource="http://www.opengis.net/spec/geosparql/1.1/specification.html#B.1.2.4"/>
        <skos:prefLabel xml:lang="en">as DGGS</skos:prefLabel>
    </owl:DatatypeProperty>
    


    <!-- http://www.opengis.net/ont/geosparql#asGML -->


    <owl:DatatypeProperty rdf:about="http://www.opengis.net/ont/geosparql#asGML">
        <rdfs:subPropertyOf rdf:resource="http://www.opengis.net/ont/geosparql#hasSerialization"/>
        <rdfs:domain rdf:resource="http://www.opengis.net/ont/geosparql#Geometry"/>
        <rdfs:range rdf:resource="http://www.opengis.net/ont/geosparql#gmlLiteral"/>
        <rdfs:isDefinedBy rdf:resource="http://www.opengis.net/ont/geosparql#"/>
        <rdfs:isDefinedBy rdf:resource="http://www.opengis.net/spec/geosparql/1.0/req/geometry-extension/geometry-as-gml-literal"/>
        <rdfs:isDefinedBy rdf:resource="http://www.opengis.net/spec/geosparql/1.1/req/geometry-extension/geometry-as-gml-literal"/>
        <skos:definition xml:lang="en">The GML serialization of a Geometry</skos:definition>
        <skos:example rdf:resource="http://www.opengis.net/spec/geosparql/1.1/specification.html#B.1.2.4"/>
        <skos:prefLabel xml:lang="en">as GML</skos:prefLabel>
    </owl:DatatypeProperty>
    


    <!-- http://www.opengis.net/ont/geosparql#asGeoJSON -->


    <owl:DatatypeProperty rdf:about="http://www.opengis.net/ont/geosparql#asGeoJSON">
        <rdfs:subPropertyOf rdf:resource="http://www.opengis.net/ont/geosparql#hasSerialization"/>
        <rdfs:domain rdf:resource="http://www.opengis.net/ont/geosparql#Geometry"/>
        <rdfs:range rdf:resource="http://www.opengis.net/ont/geosparql#geoJSONLiteral"/>
        <rdfs:isDefinedBy rdf:resource="http://www.opengis.net/ont/geosparql#"/>
        <rdfs:isDefinedBy rdf:resource="http://www.opengis.net/spec/geosparql/1.1/req/geometry-extension/geometry-as-geojson-literal"/>
        <rdfs:seeAlso rdf:resource="https://tools.ietf.org/html/rfc7946"/>
        <skos:definition xml:lang="en">The GeoJSON serialization of a Geometry</skos:definition>
        <skos:example rdf:resource="http://www.opengis.net/spec/geosparql/1.1/specification.html#B.1.2.4"/>
        <skos:prefLabel xml:lang="en">as GeoJSON</skos:prefLabel>
    </owl:DatatypeProperty>
    


    <!-- http://www.opengis.net/ont/geosparql#asKML -->


    <owl:DatatypeProperty rdf:about="http://www.opengis.net/ont/geosparql#asKML">
        <rdfs:subPropertyOf rdf:resource="http://www.opengis.net/ont/geosparql#hasSerialization"/>
        <rdfs:domain rdf:resource="http://www.opengis.net/ont/geosparql#Geometry"/>
        <rdfs:range rdf:resource="http://www.opengis.net/ont/geosparql#kmlLiteral"/>
        <rdfs:isDefinedBy rdf:resource="http://www.opengis.net/ont/geosparql#"/>
        <rdfs:isDefinedBy rdf:resource="http://www.opengis.net/spec/geosparql/1.1/req/geometry-extension/geometry-as-kml-literal"/>
        <rdfs:seeAlso rdf:resource="https://www.ogc.org/standards/kml"/>
        <skos:definition xml:lang="en">The KML serialization of a Geometry</skos:definition>
        <skos:example rdf:resource="http://www.opengis.net/spec/geosparql/1.1/specification.html#B.1.2.4"/>
        <skos:prefLabel xml:lang="en">as KML</skos:prefLabel>
    </owl:DatatypeProperty>
    


    <!-- http://www.opengis.net/ont/geosparql#asWKT -->


    <owl:DatatypeProperty rdf:about="http://www.opengis.net/ont/geosparql#asWKT">
        <rdfs:subPropertyOf rdf:resource="http://www.opengis.net/ont/geosparql#hasSerialization"/>
        <rdfs:domain rdf:resource="http://www.opengis.net/ont/geosparql#Geometry"/>
        <rdfs:range rdf:resource="http://www.opengis.net/ont/geosparql#wktLiteral"/>
        <rdfs:isDefinedBy rdf:resource="http://www.opengis.net/ont/geosparql#"/>
        <rdfs:isDefinedBy rdf:resource="http://www.opengis.net/spec/geosparql/1.0/req/geometry-extension/geometry-as-wkt-literal"/>
        <rdfs:isDefinedBy rdf:resource="http://www.opengis.net/spec/geosparql/1.1/req/geometry-extension/geometry-as-wkt-literal"/>
        <skos:definition xml:lang="en">The WKT serialization of a Geometry</skos:definition>
        <skos:example rdf:resource="http://www.opengis.net/spec/geosparql/1.1/specification.html#B.1.1.2.2"/>
        <skos:example rdf:resource="http://www.opengis.net/spec/geosparql/1.1/specification.html#B.1.1.2.3"/>
        <skos:example rdf:resource="http://www.opengis.net/spec/geosparql/1.1/specification.html#B.1.1.2.4"/>
        <skos:example rdf:resource="http://www.opengis.net/spec/geosparql/1.1/specification.html#B.1.1.2.5"/>
        <skos:example rdf:resource="http://www.opengis.net/spec/geosparql/1.1/specification.html#B.1.1.2.6"/>
        <skos:example rdf:resource="http://www.opengis.net/spec/geosparql/1.1/specification.html#B.1.1.2.8"/>
        <skos:example rdf:resource="http://www.opengis.net/spec/geosparql/1.1/specification.html#B.1.1.3.1"/>
        <skos:example rdf:resource="http://www.opengis.net/spec/geosparql/1.1/specification.html#B.1.1.3.2"/>
        <skos:example rdf:resource="http://www.opengis.net/spec/geosparql/1.1/specification.html#B.1.1.3.3"/>
        <skos:example rdf:resource="http://www.opengis.net/spec/geosparql/1.1/specification.html#B.1.2.2"/>
        <skos:example rdf:resource="http://www.opengis.net/spec/geosparql/1.1/specification.html#B.2.1"/>
        <skos:example rdf:resource="http://www.opengis.net/spec/geosparql/1.1/specification.html#B.2.2.4"/>
        <skos:prefLabel xml:lang="en">as WKT</skos:prefLabel>
    </owl:DatatypeProperty>
    


    <!-- http://www.opengis.net/ont/geosparql#coordinateDimension -->


    <owl:DatatypeProperty rdf:about="http://www.opengis.net/ont/geosparql#coordinateDimension">
        <rdfs:domain rdf:resource="http://www.opengis.net/ont/geosparql#Geometry"/>
        <rdfs:range rdf:resource="http://www.w3.org/2001/XMLSchema#integer"/>
        <rdfs:isDefinedBy rdf:resource="http://www.opengis.net/ont/geosparql#"/>
        <rdfs:isDefinedBy rdf:resource="http://www.opengis.net/spec/geosparql/1.1/req/geometry-extension/geometry-properties"/>
        <skos:definition xml:lang="en">The number of measurements or axes needed to describe the position of this Geometry in a coordinate system.</skos:definition>
        <skos:example rdf:resource="http://www.opengis.net/spec/geosparql/1.1/specification.html#B.1.2.3"/>
        <skos:prefLabel xml:lang="en">coordinate dimension</skos:prefLabel>
    </owl:DatatypeProperty>
    


    <!-- http://www.opengis.net/ont/geosparql#dimension -->


    <owl:DatatypeProperty rdf:about="http://www.opengis.net/ont/geosparql#dimension">
        <rdfs:domain rdf:resource="http://www.opengis.net/ont/geosparql#Geometry"/>
        <rdfs:range rdf:resource="http://www.w3.org/2001/XMLSchema#integer"/>
        <rdfs:isDefinedBy rdf:resource="http://www.opengis.net/ont/geosparql#"/>
        <rdfs:isDefinedBy rdf:resource="http://www.opengis.net/spec/geosparql/1.1/req/geometry-extension/geometry-properties"/>
        <skos:definition xml:lang="en">The topological dimension of this geometric object, which must be less than or equal to the coordinate dimension. In non-homogeneous collections, this will return the largest topological dimension of the contained objects.</skos:definition>
        <skos:example rdf:resource="http://www.opengis.net/spec/geosparql/1.1/specification.html#B.1.2.3"/>
        <skos:prefLabel xml:lang="en">dimension</skos:prefLabel>
    </owl:DatatypeProperty>
    


    <!-- http://www.opengis.net/ont/geosparql#hasMetricArea -->


    <owl:DatatypeProperty rdf:about="http://www.opengis.net/ont/geosparql#hasMetricArea">
        <rdfs:subPropertyOf rdf:resource="http://www.opengis.net/ont/geosparql#hasMetricSize"/>
        <rdfs:domain rdf:resource="http://www.opengis.net/ont/geosparql#SpatialObject"/>
        <rdfs:range rdf:resource="http://www.w3.org/2001/XMLSchema#double"/>
        <rdfs:isDefinedBy rdf:resource="http://www.opengis.net/ont/geosparql#"/>
        <rdfs:isDefinedBy rdf:resource="http://www.opengis.net/spec/geosparql/1.1/req/geometry-extension/spatial-object-properties"/>
        <skos:definition xml:lang="en">The area of a Spatial Object in square meters.</skos:definition>
        <skos:example rdf:resource="http://www.opengis.net/spec/geosparql/1.1/specification.html#B.1.1.2.3"/>
        <skos:example rdf:resource="http://www.opengis.net/spec/geosparql/1.1/specification.html#B.1.1.2.9"/>
        <skos:example rdf:resource="http://www.opengis.net/spec/geosparql/1.1/specification.html#B.1.1.3.3"/>
        <skos:example rdf:resource="http://www.opengis.net/spec/geosparql/1.1/specification.html#B.1.2.2"/>
        <skos:prefLabel xml:lang="en">has area in square meters</skos:prefLabel>
    </owl:DatatypeProperty>
    


    <!-- http://www.opengis.net/ont/geosparql#hasMetricLength -->


    <owl:DatatypeProperty rdf:about="http://www.opengis.net/ont/geosparql#hasMetricLength">
        <rdfs:subPropertyOf rdf:resource="http://www.opengis.net/ont/geosparql#hasMetricSize"/>
        <rdfs:domain rdf:resource="http://www.opengis.net/ont/geosparql#SpatialObject"/>
        <rdfs:range rdf:resource="http://www.w3.org/2001/XMLSchema#double"/>
        <rdfs:isDefinedBy rdf:resource="http://www.opengis.net/ont/geosparql#"/>
        <rdfs:isDefinedBy rdf:resource="http://www.opengis.net/spec/geosparql/1.1/req/geometry-extension/spatial-object-properties"/>
        <skos:definition xml:lang="en">The length of a Spatial Object in meters.</skos:definition>
        <skos:example rdf:resource="http://www.opengis.net/spec/geosparql/1.1/specification.html#B.1.2.2"/>
        <skos:prefLabel xml:lang="en">has length in meters</skos:prefLabel>
    </owl:DatatypeProperty>
    


    <!-- http://www.opengis.net/ont/geosparql#hasMetricPerimeterLength -->


    <owl:DatatypeProperty rdf:about="http://www.opengis.net/ont/geosparql#hasMetricPerimeterLength">
        <rdfs:subPropertyOf rdf:resource="http://www.opengis.net/ont/geosparql#hasMetricSize"/>
        <rdfs:domain rdf:resource="http://www.opengis.net/ont/geosparql#SpatialObject"/>
        <rdfs:range rdf:resource="http://www.w3.org/2001/XMLSchema#double"/>
        <rdfs:isDefinedBy rdf:resource="http://www.opengis.net/ont/geosparql#"/>
        <rdfs:isDefinedBy rdf:resource="http://www.opengis.net/spec/geosparql/1.1/req/geometry-extension/spatial-object-properties"/>
        <skos:definition xml:lang="en">The length of the perimeter of a Spatial Object in meters.</skos:definition>
        <skos:example rdf:resource="http://www.opengis.net/spec/geosparql/1.1/specification.html#B.1.1.1.2"/>
        <skos:prefLabel xml:lang="en">has perimeter length in meters</skos:prefLabel>
    </owl:DatatypeProperty>
    


    <!-- http://www.opengis.net/ont/geosparql#hasMetricSize -->


    <owl:DatatypeProperty rdf:about="http://www.opengis.net/ont/geosparql#hasMetricSize">
        <rdfs:domain rdf:resource="http://www.opengis.net/ont/geosparql#SpatialObject"/>
        <rdfs:range rdf:resource="http://www.w3.org/2001/XMLSchema#double"/>
        <rdfs:isDefinedBy rdf:resource="http://www.opengis.net/ont/geosparql#"/>
        <rdfs:isDefinedBy rdf:resource="http://www.opengis.net/spec/geosparql/1.1/req/geometry-extension/spatial-object-properties"/>
        <skos:definition xml:lang="en">Subproperties of this property are used to indicate the size of a Spatial Object, as a measurement or estimate of one or more dimensions of the Spatial Object&apos;s spatial presence. Units are always metric (meter, square meter or cubic meter).</skos:definition>
        <skos:prefLabel xml:lang="en">has metric size</skos:prefLabel>
    </owl:DatatypeProperty>
    


    <!-- http://www.opengis.net/ont/geosparql#hasMetricSpatialAccuracy -->


    <owl:DatatypeProperty rdf:about="http://www.opengis.net/ont/geosparql#hasMetricSpatialAccuracy">
        <rdfs:domain rdf:resource="http://www.opengis.net/ont/geosparql#Geometry"/>
        <rdfs:range rdf:resource="http://www.w3.org/2001/XMLSchema#double"/>
        <rdfs:isDefinedBy rdf:resource="http://www.opengis.net/ont/geosparql#"/>
        <rdfs:isDefinedBy rdf:resource="http://www.opengis.net/spec/geosparql/1.1/req/geometry-extension/geometry-properties"/>
        <skos:definition xml:lang="en">The positional accuracy of the coordinates of a Geometry in meters.</skos:definition>
        <skos:example rdf:resource="http://www.opengis.net/spec/geosparql/1.1/specification.html#B.1.2.3"/>
        <skos:note xml:lang="en">Spatial accuracy is applicable when a Geometry is used to represent a Feature. It is expressed as a distance that indicates the truthfullness of the positions (coordinates) that define the Geometry. In this case accuracy defines a zone surrounding each coordinate within wich the real positions are known to be. The accuracy value defines this zone as a distance from the coordinate(s) in all directions (e.g. a line, a circle or a sphere, depending on spatial dimension).</skos:note>
        <skos:prefLabel xml:lang="en">has spatial accuracy in meters</skos:prefLabel>
    </owl:DatatypeProperty>
    


    <!-- http://www.opengis.net/ont/geosparql#hasMetricSpatialResolution -->


    <owl:DatatypeProperty rdf:about="http://www.opengis.net/ont/geosparql#hasMetricSpatialResolution">
        <rdfs:domain rdf:resource="http://www.opengis.net/ont/geosparql#Geometry"/>
        <rdfs:range rdf:resource="http://www.w3.org/2001/XMLSchema#double"/>
        <rdfs:isDefinedBy rdf:resource="http://www.opengis.net/ont/geosparql#"/>
        <rdfs:isDefinedBy rdf:resource="http://www.opengis.net/spec/geosparql/1.1/req/geometry-extension/geometry-properties"/>
        <skos:definition xml:lang="en">The spatial resolution of a Geometry in meters.</skos:definition>
        <skos:example rdf:resource="http://www.opengis.net/spec/geosparql/1.1/specification.html#B.1.1.2.6"/>
        <skos:example rdf:resource="http://www.opengis.net/spec/geosparql/1.1/specification.html#B.1.2.2"/>
        <skos:note xml:lang="en">Spatial resolution specifies the level of detail of a Geometry. It the smallest dinstinguishable distance between spatially adjacent coordinates.</skos:note>
        <skos:prefLabel xml:lang="en">has spatial resolution in meters</skos:prefLabel>
    </owl:DatatypeProperty>
    


    <!-- http://www.opengis.net/ont/geosparql#hasMetricVolume -->


    <owl:DatatypeProperty rdf:about="http://www.opengis.net/ont/geosparql#hasMetricVolume">
        <rdfs:subPropertyOf rdf:resource="http://www.opengis.net/ont/geosparql#hasMetricSize"/>
        <rdfs:domain rdf:resource="http://www.opengis.net/ont/geosparql#SpatialObject"/>
        <rdfs:range rdf:resource="http://www.w3.org/2001/XMLSchema#double"/>
        <rdfs:isDefinedBy rdf:resource="http://www.opengis.net/ont/geosparql#"/>
        <rdfs:isDefinedBy rdf:resource="http://www.opengis.net/spec/geosparql/1.1/req/geometry-extension/spatial-object-properties"/>
        <skos:definition xml:lang="en">The volume of a Spatial Object in cubic meters.</skos:definition>
        <skos:example rdf:resource="http://www.opengis.net/spec/geosparql/1.1/specification.html#B.1.1.2.9"/>
        <skos:example rdf:resource="http://www.opengis.net/spec/geosparql/1.1/specification.html#B.1.2.2"/>
        <skos:prefLabel xml:lang="en">has volume in cubic meters</skos:prefLabel>
    </owl:DatatypeProperty>
    


    <!-- http://www.opengis.net/ont/geosparql#hasSerialization -->


    <owl:DatatypeProperty rdf:about="http://www.opengis.net/ont/geosparql#hasSerialization">
        <rdfs:domain rdf:resource="http://www.opengis.net/ont/geosparql#Geometry"/>
        <rdfs:range rdf:resource="http://www.w3.org/2000/01/rdf-schema#Literal"/>
        <rdfs:isDefinedBy rdf:resource="http://www.opengis.net/ont/geosparql#"/>
        <rdfs:isDefinedBy rdf:resource="http://www.opengis.net/spec/geosparql/1.0/req/geometry-extension/geometry-properties"/>
        <rdfs:isDefinedBy rdf:resource="http://www.opengis.net/spec/geosparql/1.1/req/geometry-extension/geometry-properties"/>
        <skos:definition xml:lang="en">Connects a Geometry object with its text-based serialization.</skos:definition>
        <skos:example rdf:resource="http://www.opengis.net/spec/geosparql/1.1/specification.html#B.1.2.3"/>
        <skos:prefLabel xml:lang="en">has serialization</skos:prefLabel>
    </owl:DatatypeProperty>
    


    <!-- http://www.opengis.net/ont/geosparql#isEmpty -->


    <owl:DatatypeProperty rdf:about="http://www.opengis.net/ont/geosparql#isEmpty">
        <rdfs:domain rdf:resource="http://www.opengis.net/ont/geosparql#Geometry"/>
        <rdfs:range rdf:resource="http://www.w3.org/2001/XMLSchema#boolean"/>
        <rdfs:isDefinedBy rdf:resource="http://www.opengis.net/ont/geosparql#"/>
        <rdfs:isDefinedBy rdf:resource="http://www.opengis.net/spec/geosparql/1.0/req/geometry-extension/geometry-properties"/>
        <rdfs:isDefinedBy rdf:resource="http://www.opengis.net/spec/geosparql/1.1/req/geometry-extension/geometry-properties"/>
        <skos:definition xml:lang="en">(true) if this geometric object is the empty Geometry. If true, then this geometric object represents the empty point set for the coordinate space.</skos:definition>
        <skos:example rdf:resource="http://www.opengis.net/spec/geosparql/1.1/specification.html#B.1.2.3"/>
        <skos:prefLabel xml:lang="en">is empty</skos:prefLabel>
    </owl:DatatypeProperty>
    


    <!-- http://www.opengis.net/ont/geosparql#isSimple -->


    <owl:DatatypeProperty rdf:about="http://www.opengis.net/ont/geosparql#isSimple">
        <rdfs:domain rdf:resource="http://www.opengis.net/ont/geosparql#Geometry"/>
        <rdfs:range rdf:resource="http://www.w3.org/2001/XMLSchema#boolean"/>
        <rdfs:isDefinedBy rdf:resource="http://www.opengis.net/ont/geosparql#"/>
        <rdfs:isDefinedBy rdf:resource="http://www.opengis.net/spec/geosparql/1.0/req/geometry-extension/geometry-properties"/>
        <rdfs:isDefinedBy rdf:resource="http://www.opengis.net/spec/geosparql/1.1/req/geometry-extension/geometry-properties"/>
        <rdfs:seeAlso rdf:resource="https://portal.ogc.org/files/?artifact_id=25355"/>
        <skos:definition xml:lang="en">(true) if this geometric object has no anomalous geometric points, such as self intersection or self tangency.</skos:definition>
        <skos:example rdf:resource="http://www.opengis.net/spec/geosparql/1.1/specification.html#B.1.2.3"/>
        <skos:prefLabel xml:lang="en">is simple</skos:prefLabel>
    </owl:DatatypeProperty>
    


    <!-- http://www.opengis.net/ont/geosparql#spatialDimension -->


    <owl:DatatypeProperty rdf:about="http://www.opengis.net/ont/geosparql#spatialDimension">
        <rdfs:domain rdf:resource="http://www.opengis.net/ont/geosparql#Geometry"/>
        <rdfs:range rdf:resource="http://www.w3.org/2001/XMLSchema#integer"/>
        <rdfs:isDefinedBy rdf:resource="http://www.opengis.net/ont/geosparql#"/>
        <rdfs:isDefinedBy rdf:resource="http://www.opengis.net/spec/geosparql/1.0/req/geometry-extension/geometry-properties"/>
        <rdfs:isDefinedBy rdf:resource="http://www.opengis.net/spec/geosparql/1.1/req/geometry-extension/geometry-properties"/>
        <skos:definition xml:lang="en">The number of measurements or axes needed to describe the spatial position of this Geometry in a coordinate system.</skos:definition>
        <skos:example rdf:resource="http://www.opengis.net/spec/geosparql/1.1/specification.html#B.1.2.3"/>
        <skos:prefLabel xml:lang="en">spatial dimension</skos:prefLabel>
    </owl:DatatypeProperty>
    


    <!-- http://www.w3.org/2003/01/geo/wgs84_pos#alt -->


    <owl:DatatypeProperty rdf:about="http://www.w3.org/2003/01/geo/wgs84_pos#alt">
        <rdfs:domain rdf:resource="http://www.w3.org/2003/01/geo/wgs84_pos#SpatialThing"/>
    </owl:DatatypeProperty>
    


    <!-- http://www.w3.org/2003/01/geo/wgs84_pos#lat -->


    <owl:DatatypeProperty rdf:about="http://www.w3.org/2003/01/geo/wgs84_pos#lat">
        <rdfs:domain rdf:resource="http://www.w3.org/2003/01/geo/wgs84_pos#SpatialThing"/>
    </owl:DatatypeProperty>
    


    <!-- http://www.w3.org/2006/time#day -->


    <owl:DatatypeProperty rdf:about="http://www.w3.org/2006/time#day">
        <rdfs:domain rdf:resource="http://www.w3.org/2006/time#GeneralDateTimeDescription"/>
        <rdfs:comment xml:lang="en">Day position in a calendar-clock system.

The range of this property is not specified, so can be replaced by any specific representation of a calendar day from any calendar. </rdfs:comment>
        <rdfs:comment xml:lang="es">Posición de día en un sistema calendario-reloj.</rdfs:comment>
        <rdfs:label xml:lang="en">day</rdfs:label>
        <rdfs:label xml:lang="es">día</rdfs:label>
        <skos:definition xml:lang="en">Day position in a calendar-clock system.

The range of this property is not specified, so can be replaced by any specific representation of a calendar day from any calendar. </skos:definition>
        <skos:definition xml:lang="es">Posición de día en un sistema calendario-reloj.

El rango de esta propiedad no está especificado, por tanto, se puede reemplazar por una representación específica de un día de calendario de cualquier calendario.</skos:definition>
    </owl:DatatypeProperty>
    


    <!-- http://www.w3.org/2006/time#dayOfYear -->


    <owl:DatatypeProperty rdf:about="http://www.w3.org/2006/time#dayOfYear">
        <rdfs:domain rdf:resource="http://www.w3.org/2006/time#GeneralDateTimeDescription"/>
        <rdfs:range rdf:resource="http://www.w3.org/2001/XMLSchema#nonNegativeInteger"/>
        <rdfs:comment xml:lang="es">El número de día en el año.</rdfs:comment>
        <rdfs:comment xml:lang="en">The number of the day within the year</rdfs:comment>
        <rdfs:label xml:lang="en">day of year</rdfs:label>
        <rdfs:label xml:lang="es">día del año</rdfs:label>
        <skos:definition xml:lang="es">El número de día en el año.</skos:definition>
        <skos:definition xml:lang="en">The number of the day within the year</skos:definition>
    </owl:DatatypeProperty>
    


    <!-- http://www.w3.org/2006/time#days -->


    <owl:DatatypeProperty rdf:about="http://www.w3.org/2006/time#days">
        <rdfs:domain rdf:resource="http://www.w3.org/2006/time#GeneralDurationDescription"/>
        <rdfs:range rdf:resource="http://www.w3.org/2001/XMLSchema#decimal"/>
        <rdfs:comment xml:lang="es">Longitud de, o elemento de la longitud de, una extensión temporal expresada en días.</rdfs:comment>
        <rdfs:comment xml:lang="en">length of, or element of the length of, a temporal extent expressed in days</rdfs:comment>
        <rdfs:label xml:lang="en">days duration</rdfs:label>
        <rdfs:label xml:lang="es">duración en días</rdfs:label>
        <skos:definition xml:lang="es">Longitud de, o elemento de la longitud de, una extensión temporal expresada en días.</skos:definition>
        <skos:definition xml:lang="en">length of, or element of the length of, a temporal extent expressed in days</skos:definition>
    </owl:DatatypeProperty>
    


    <!-- http://www.w3.org/2006/time#hasXSDDuration -->


    <owl:DatatypeProperty rdf:about="http://www.w3.org/2006/time#hasXSDDuration">
        <rdfs:domain rdf:resource="http://www.w3.org/2006/time#TemporalEntity"/>
        <rdfs:range rdf:resource="http://www.w3.org/2001/XMLSchema#duration"/>
        <rdfs:comment xml:lang="es">Extensión de una entidad temporal, expresada utilizando xsd:duration.</rdfs:comment>
        <rdfs:comment xml:lang="en">Extent of a temporal entity, expressed using xsd:duration</rdfs:comment>
        <rdfs:label xml:lang="en">has XSD duration</rdfs:label>
        <rdfs:label xml:lang="es">tiene duración XSD</rdfs:label>
        <skos:definition xml:lang="es">Extensión de una entidad temporal, expresada utilizando xsd:duration.</skos:definition>
        <skos:definition xml:lang="en">Extent of a temporal entity, expressed using xsd:duration</skos:definition>
        <skos:editorialNote xml:lang="es">Característica arriesgada - añadida en la revisión de 2017, y todavía no ampliamente utilizada.</skos:editorialNote>
        <skos:editorialNote xml:lang="en">Feature at risk - added in 2017 revision, and not yet widely used. </skos:editorialNote>
    </owl:DatatypeProperty>
    


    <!-- http://www.w3.org/2006/time#hour -->


    <owl:DatatypeProperty rdf:about="http://www.w3.org/2006/time#hour">
        <rdfs:domain rdf:resource="http://www.w3.org/2006/time#GeneralDateTimeDescription"/>
        <rdfs:range rdf:resource="http://www.w3.org/2001/XMLSchema#nonNegativeInteger"/>
        <rdfs:comment xml:lang="en">Hour position in a calendar-clock system.</rdfs:comment>
        <rdfs:comment xml:lang="es">Posición de hora en un sistema calendario-reloj.</rdfs:comment>
        <rdfs:label xml:lang="es">hora</rdfs:label>
        <rdfs:label xml:lang="en">hour</rdfs:label>
        <skos:definition xml:lang="en">Hour position in a calendar-clock system.</skos:definition>
        <skos:definition xml:lang="es">Posición de hora en un sistema calendario-reloj.</skos:definition>
    </owl:DatatypeProperty>
    


    <!-- http://www.w3.org/2006/time#hours -->


    <owl:DatatypeProperty rdf:about="http://www.w3.org/2006/time#hours">
        <rdfs:domain rdf:resource="http://www.w3.org/2006/time#GeneralDurationDescription"/>
        <rdfs:range rdf:resource="http://www.w3.org/2001/XMLSchema#decimal"/>
        <rdfs:comment xml:lang="es">Longitud de, o elemento de la longitud de, una extensión temporal expresada en horas.</rdfs:comment>
        <rdfs:comment xml:lang="en">length of, or element of the length of, a temporal extent expressed in hours</rdfs:comment>
        <rdfs:label xml:lang="es">duración en horas</rdfs:label>
        <rdfs:label xml:lang="en">hours duration</rdfs:label>
        <skos:definition xml:lang="es">Longitud de, o elemento de la longitud de, una extensión temporal expresada en horas.</skos:definition>
        <skos:definition xml:lang="en">length of, or element of the length of, a temporal extent expressed in hours</skos:definition>
    </owl:DatatypeProperty>
    


    <!-- http://www.w3.org/2006/time#inXSDDate -->


    <owl:DatatypeProperty rdf:about="http://www.w3.org/2006/time#inXSDDate">
        <rdfs:domain rdf:resource="http://www.w3.org/2006/time#Instant"/>
        <rdfs:range rdf:resource="http://www.w3.org/2001/XMLSchema#date"/>
        <rdfs:comment xml:lang="es">Posición de un instante, expresado utilizando xsd:date.</rdfs:comment>
        <rdfs:comment xml:lang="en">Position of an instant, expressed using xsd:date</rdfs:comment>
        <rdfs:label xml:lang="es">en fecha XSD</rdfs:label>
        <rdfs:label xml:lang="en">in XSD date</rdfs:label>
        <skos:definition xml:lang="es">Posición de un instante, expresado utilizando xsd:date.</skos:definition>
        <skos:definition xml:lang="en">Position of an instant, expressed using xsd:date</skos:definition>
    </owl:DatatypeProperty>
    


    <!-- http://www.w3.org/2006/time#inXSDDateTime -->


    <owl:DatatypeProperty rdf:about="http://www.w3.org/2006/time#inXSDDateTime">
        <rdfs:domain rdf:resource="http://www.w3.org/2006/time#Instant"/>
        <rdfs:range rdf:resource="http://www.w3.org/2001/XMLSchema#dateTime"/>
        <rdfs:comment xml:lang="es">Posición de un instante, expresado utilizando xsd:dateTime.</rdfs:comment>
        <rdfs:comment xml:lang="en">Position of an instant, expressed using xsd:dateTime</rdfs:comment>
        <rdfs:label xml:lang="es">en fecha-tiempo XSD</rdfs:label>
        <rdfs:label xml:lang="en">in XSD Date-Time</rdfs:label>
        <owl:deprecated rdf:datatype="http://www.w3.org/2001/XMLSchema#boolean">true</owl:deprecated>
        <skos:definition xml:lang="es">Posición de un instante, expresado utilizando xsd:dateTime.</skos:definition>
        <skos:definition xml:lang="en">Position of an instant, expressed using xsd:dateTime</skos:definition>
        <skos:note xml:lang="es">La propiedad &apos;en fecha-hora XSD&apos; ha sido reemplazada por &apos;en fecha-sello de tiempo XSD&apos; que hace obligatorio el campo &apos;huso horario&apos;.</skos:note>
        <skos:note xml:lang="en">The property :inXSDDateTime is replaced by :inXSDDateTimeStamp which makes the time-zone field mandatory.</skos:note>
    </owl:DatatypeProperty>
    


    <!-- http://www.w3.org/2006/time#inXSDDateTimeStamp -->


    <owl:DatatypeProperty rdf:about="http://www.w3.org/2006/time#inXSDDateTimeStamp">
        <rdfs:domain rdf:resource="http://www.w3.org/2006/time#Instant"/>
        <rdfs:range rdf:resource="http://www.w3.org/2001/XMLSchema#dateTimeStamp"/>
        <rdfs:comment xml:lang="es">Posición de un instante, expresado utilizando xsd:dateTimeStamp.</rdfs:comment>
        <rdfs:comment xml:lang="en">Position of an instant, expressed using xsd:dateTimeStamp</rdfs:comment>
        <rdfs:label xml:lang="es">en fecha-sello de tiempo XSD</rdfs:label>
        <rdfs:label xml:lang="en">in XSD Date-Time-Stamp</rdfs:label>
        <skos:definition xml:lang="es">Posición de un instante, expresado utilizando xsd:dateTimeStamp.</skos:definition>
        <skos:definition xml:lang="en">Position of an instant, expressed using xsd:dateTimeStamp</skos:definition>
    </owl:DatatypeProperty>
    


    <!-- http://www.w3.org/2006/time#inXSDgYear -->


    <owl:DatatypeProperty rdf:about="http://www.w3.org/2006/time#inXSDgYear">
        <rdfs:domain rdf:resource="http://www.w3.org/2006/time#Instant"/>
        <rdfs:range rdf:resource="http://www.w3.org/2001/XMLSchema#gYear"/>
        <rdfs:comment xml:lang="es">Posición de un instante, expresado utilizando xsd:gYear.</rdfs:comment>
        <rdfs:comment xml:lang="en">Position of an instant, expressed using xsd:gYear</rdfs:comment>
        <rdfs:label xml:lang="es">en año gregoriano XSD</rdfs:label>
        <rdfs:label xml:lang="en">in XSD g-Year</rdfs:label>
        <skos:definition xml:lang="es">Posición de un instante, expresado utilizando xsd:gYear.</skos:definition>
        <skos:definition xml:lang="en">Position of an instant, expressed using xsd:gYear</skos:definition>
    </owl:DatatypeProperty>
    


    <!-- http://www.w3.org/2006/time#inXSDgYearMonth -->


    <owl:DatatypeProperty rdf:about="http://www.w3.org/2006/time#inXSDgYearMonth">
        <rdfs:domain rdf:resource="http://www.w3.org/2006/time#Instant"/>
        <rdfs:range rdf:resource="http://www.w3.org/2001/XMLSchema#gYearMonth"/>
        <rdfs:comment xml:lang="es">Posición de un instante, expresado utilizando xsd:gYearMonth.</rdfs:comment>
        <rdfs:comment xml:lang="en">Position of an instant, expressed using xsd:gYearMonth</rdfs:comment>
        <rdfs:label xml:lang="es">en año-mes gregoriano XSD</rdfs:label>
        <rdfs:label xml:lang="en">in XSD g-YearMonth</rdfs:label>
        <skos:definition xml:lang="es">Posición de un instante, expresado utilizando xsd:gYearMonth.</skos:definition>
        <skos:definition xml:lang="en">Position of an instant, expressed using xsd:gYearMonth</skos:definition>
    </owl:DatatypeProperty>
    


    <!-- http://www.w3.org/2006/time#minute -->


    <owl:DatatypeProperty rdf:about="http://www.w3.org/2006/time#minute">
        <rdfs:domain rdf:resource="http://www.w3.org/2006/time#GeneralDateTimeDescription"/>
        <rdfs:range rdf:resource="http://www.w3.org/2001/XMLSchema#nonNegativeInteger"/>
        <rdfs:comment xml:lang="en">Minute position in a calendar-clock system.</rdfs:comment>
        <rdfs:comment xml:lang="es">Posición de minuto en un sistema calendario-reloj.</rdfs:comment>
        <rdfs:label xml:lang="en">minute</rdfs:label>
        <rdfs:label xml:lang="es">minuto</rdfs:label>
        <skos:definition xml:lang="en">Minute position in a calendar-clock system.</skos:definition>
        <skos:definition xml:lang="es">Posición de minuto en un sistema calendario-reloj.</skos:definition>
    </owl:DatatypeProperty>
    


    <!-- http://www.w3.org/2006/time#minutes -->


    <owl:DatatypeProperty rdf:about="http://www.w3.org/2006/time#minutes">
        <rdfs:domain rdf:resource="http://www.w3.org/2006/time#GeneralDurationDescription"/>
        <rdfs:range rdf:resource="http://www.w3.org/2001/XMLSchema#decimal"/>
        <rdfs:comment xml:lang="es">Longitud de, o elemento de la longitud de, una extensión temporal expresada en minutos.</rdfs:comment>
        <rdfs:comment xml:lang="en">length, or element of, a temporal extent expressed in minutes</rdfs:comment>
        <rdfs:label xml:lang="en">minutes</rdfs:label>
        <rdfs:label xml:lang="es">minutos</rdfs:label>
        <skos:definition xml:lang="es">Longitud de, o elemento de la longitud de, una extensión temporal expresada en minutos.</skos:definition>
        <skos:definition xml:lang="en">length, or element of, a temporal extent expressed in minutes</skos:definition>
    </owl:DatatypeProperty>
    


    <!-- http://www.w3.org/2006/time#month -->


    <owl:DatatypeProperty rdf:about="http://www.w3.org/2006/time#month">
        <rdfs:domain rdf:resource="http://www.w3.org/2006/time#GeneralDateTimeDescription"/>
        <rdfs:comment xml:lang="en">Month position in a calendar-clock system.

The range of this property is not specified, so can be replaced by any specific representation of a calendar month from any calendar. </rdfs:comment>
        <rdfs:comment xml:lang="es">Posición de mes en un sistema calendario-reloj.
    El rango de esta propiedad no está especificado, por tanto, se puede reemplazar por cualquier representación específica de un mes de calendario de un calendario cualquiera.</rdfs:comment>
        <rdfs:label xml:lang="es">mes</rdfs:label>
        <rdfs:label xml:lang="en">month</rdfs:label>
        <skos:definition xml:lang="en">Month position in a calendar-clock system.

The range of this property is not specified, so can be replaced by any specific representation of a calendar month from any calendar. </skos:definition>
        <skos:definition xml:lang="es">Posición de mes en un sistema calendario-reloj.
            El rango de esta propiedad no está especificado, por tanto, se puede reemplazar por cualquier representación específica de un mes de calendario de un calendario cualquiera.</skos:definition>
    </owl:DatatypeProperty>
    


    <!-- http://www.w3.org/2006/time#months -->


    <owl:DatatypeProperty rdf:about="http://www.w3.org/2006/time#months">
        <rdfs:domain rdf:resource="http://www.w3.org/2006/time#GeneralDurationDescription"/>
        <rdfs:range rdf:resource="http://www.w3.org/2001/XMLSchema#decimal"/>
        <rdfs:comment xml:lang="es">Longitud de, o elemento de la longitud de, una extensión temporal expresada en meses.</rdfs:comment>
        <rdfs:comment xml:lang="en">length of, or element of the length of, a temporal extent expressed in months</rdfs:comment>
        <rdfs:label xml:lang="es">duración en meses</rdfs:label>
        <rdfs:label xml:lang="en">months duration</rdfs:label>
        <skos:definition xml:lang="es">Longitud de, o elemento de la longitud de, una extensión temporal expresada en meses.</skos:definition>
        <skos:definition xml:lang="en">length of, or element of the length of, a temporal extent expressed in months</skos:definition>
    </owl:DatatypeProperty>
    


    <!-- http://www.w3.org/2006/time#nominalPosition -->


    <owl:DatatypeProperty rdf:about="http://www.w3.org/2006/time#nominalPosition">
        <rdfs:domain rdf:resource="http://www.w3.org/2006/time#TimePosition"/>
        <rdfs:range rdf:resource="http://www.w3.org/2001/XMLSchema#string"/>
        <rdfs:comment xml:lang="es">El valor (nominal) que indica posición temporal en un sistema de referencia ordinal.</rdfs:comment>
        <rdfs:comment xml:lang="en">The (nominal) value indicating temporal position in an ordinal reference system </rdfs:comment>
        <rdfs:label xml:lang="en">Name of temporal position</rdfs:label>
        <rdfs:label xml:lang="es">nombre de posición temporal</rdfs:label>
        <skos:definition xml:lang="es">El valor (nominal) que indica posición temporal en un sistema de referencia ordinal.</skos:definition>
        <skos:definition xml:lang="en">The (nominal) value indicating temporal position in an ordinal reference system </skos:definition>
    </owl:DatatypeProperty>
    


    <!-- http://www.w3.org/2006/time#numericDuration -->


    <owl:DatatypeProperty rdf:about="http://www.w3.org/2006/time#numericDuration">
        <rdfs:domain rdf:resource="http://www.w3.org/2006/time#Duration"/>
        <rdfs:range rdf:resource="http://www.w3.org/2001/XMLSchema#decimal"/>
        <rdfs:comment xml:lang="es">Valor de una extensión temporal expresada como un número decimal escalado por una unidad de tiempo.</rdfs:comment>
        <rdfs:comment xml:lang="en">Value of a temporal extent expressed as a decimal number scaled by a temporal unit</rdfs:comment>
        <rdfs:label xml:lang="en">Numeric value of temporal duration</rdfs:label>
        <rdfs:label xml:lang="es">valor numérico de duración temporal</rdfs:label>
        <skos:definition xml:lang="es">Valor de una extensión temporal expresada como un número decimal escalado por una unidad de tiempo.</skos:definition>
        <skos:definition xml:lang="en">Value of a temporal extent expressed as a decimal number scaled by a temporal unit</skos:definition>
    </owl:DatatypeProperty>
    


    <!-- http://www.w3.org/2006/time#numericPosition -->


    <owl:DatatypeProperty rdf:about="http://www.w3.org/2006/time#numericPosition">
        <rdfs:domain rdf:resource="http://www.w3.org/2006/time#TimePosition"/>
        <rdfs:range rdf:resource="http://www.w3.org/2001/XMLSchema#decimal"/>
        <rdfs:comment xml:lang="es">El valor (numérico) que indica posición temporal en un sistema de referencia ordinal.</rdfs:comment>
        <rdfs:comment xml:lang="en">The (numeric) value indicating position within a temporal coordinate system </rdfs:comment>
        <rdfs:label xml:lang="en">Numeric value of temporal position</rdfs:label>
        <rdfs:label xml:lang="es">valor numérico de posición temporal</rdfs:label>
        <skos:definition xml:lang="es">El valor (numérico) que indica posición temporal en un sistema de referencia ordinal.</skos:definition>
        <skos:definition xml:lang="en">The (numeric) value indicating position within a temporal coordinate system </skos:definition>
    </owl:DatatypeProperty>
    


    <!-- http://www.w3.org/2006/time#second -->


    <owl:DatatypeProperty rdf:about="http://www.w3.org/2006/time#second">
        <rdfs:domain rdf:resource="http://www.w3.org/2006/time#GeneralDateTimeDescription"/>
        <rdfs:range rdf:resource="http://www.w3.org/2001/XMLSchema#decimal"/>
        <rdfs:comment xml:lang="es">Posición de segundo en un sistema calendario-reloj.</rdfs:comment>
        <rdfs:comment xml:lang="en">Second position in a calendar-clock system.</rdfs:comment>
        <rdfs:label xml:lang="en">second</rdfs:label>
        <rdfs:label xml:lang="es">segundo</rdfs:label>
    </owl:DatatypeProperty>
    


    <!-- http://www.w3.org/2006/time#seconds -->


    <owl:DatatypeProperty rdf:about="http://www.w3.org/2006/time#seconds">
        <rdfs:domain rdf:resource="http://www.w3.org/2006/time#GeneralDurationDescription"/>
        <rdfs:range rdf:resource="http://www.w3.org/2001/XMLSchema#decimal"/>
        <rdfs:comment xml:lang="es">Longitud de, o elemento de la longitud de, una extensión temporal expresada en segundos.</rdfs:comment>
        <rdfs:comment xml:lang="en">length of, or element of the length of, a temporal extent expressed in seconds</rdfs:comment>
        <rdfs:label xml:lang="es">duración en segundos</rdfs:label>
        <rdfs:label xml:lang="en">seconds duration</rdfs:label>
        <rdfs:seeAlso rdf:resource="http://www.bipm.org/en/publications/si-brochure/second.html"/>
    </owl:DatatypeProperty>
    


    <!-- http://www.w3.org/2006/time#week -->


    <owl:DatatypeProperty rdf:about="http://www.w3.org/2006/time#week">
        <rdfs:domain rdf:resource="http://www.w3.org/2006/time#GeneralDateTimeDescription"/>
        <rdfs:range rdf:resource="http://www.w3.org/2001/XMLSchema#nonNegativeInteger"/>
        <rdfs:comment xml:lang="es">Número de semana en el año.</rdfs:comment>
        <rdfs:comment xml:lang="en">Week number within the year.</rdfs:comment>
        <rdfs:label xml:lang="es">semana</rdfs:label>
        <rdfs:label xml:lang="en">week</rdfs:label>
        <skos:note xml:lang="en">Weeks are numbered differently depending on the calendar in use and the local language or cultural conventions (locale). ISO-8601 specifies that the first week of the year includes at least four days, and that Monday is the first day of the week. In that system, week 1 is the week that contains the first Thursday in the year.</skos:note>
        <skos:scopeNote xml:lang="es">Las semanas están numeradas de forma diferente dependiendo del calendario en uso y de las convenciones lingüísticas y culturales locales (locale en inglés). El ISO-8601 especifica que la primera semana del año incluye al menos cuatro días, y que el lunes es el primer día de la semana. En ese sistema, la semana 1 es la semana que contiene el primer jueves del año.</skos:scopeNote>
    </owl:DatatypeProperty>
    


    <!-- http://www.w3.org/2006/time#weeks -->


    <owl:DatatypeProperty rdf:about="http://www.w3.org/2006/time#weeks">
        <rdfs:domain rdf:resource="http://www.w3.org/2006/time#GeneralDurationDescription"/>
        <rdfs:range rdf:resource="http://www.w3.org/2001/XMLSchema#decimal"/>
        <rdfs:comment xml:lang="es">Longitud de, o elemento de la longitud de, una extensión temporal expresada en semanas.</rdfs:comment>
        <rdfs:comment xml:lang="en">length of, or element of the length of, a temporal extent expressed in weeks</rdfs:comment>
        <rdfs:label xml:lang="es">duración en semanas</rdfs:label>
        <rdfs:label xml:lang="en">weeks duration</rdfs:label>
    </owl:DatatypeProperty>
    


    <!-- http://www.w3.org/2006/time#xsdDateTime -->


    <owl:DatatypeProperty rdf:about="http://www.w3.org/2006/time#xsdDateTime">
        <rdfs:domain rdf:resource="http://www.w3.org/2006/time#DateTimeInterval"/>
        <rdfs:range rdf:resource="http://www.w3.org/2001/XMLSchema#dateTime"/>
        <rdfs:comment xml:lang="es">Valor de &apos;intervalo de fecha-hora&apos; expresado como un valor compacto.</rdfs:comment>
        <rdfs:comment xml:lang="en">Value of DateTimeInterval expressed as a compact value.</rdfs:comment>
        <rdfs:label xml:lang="en">has XSD date-time</rdfs:label>
        <rdfs:label xml:lang="es">tiene fecha-hora XSD</rdfs:label>
        <owl:deprecated rdf:datatype="http://www.w3.org/2001/XMLSchema#boolean">true</owl:deprecated>
        <skos:note xml:lang="en">Using xsd:dateTime in this place means that the duration of the interval is implicit: it corresponds to the length of the smallest non-zero element of the date-time literal. However, this rule cannot be used for intervals whose duration is more than one rank smaller than the starting time - e.g. the first minute or second of a day, the first hour of a month, or the first day of a year. In these cases the desired interval cannot be distinguished from the interval corresponding to the next rank up. Because of this essential ambiguity, use of this property is not recommended and it is deprecated.</skos:note>
        <skos:note>Utilizando xsd:dateTime en este lugar significa que la duración del intervalo está implícita: se corresponde con la longitud del elemento más pequeño distinto de cero del literal fecha-hora. Sin embargo, esta regla no se puede utilizar para intervalos cuya duración es mayor que un rango más pequeño que el tiempo de comienzo - p.ej. el primer minuto o segundo del día, la primera hora del mes, o el primer día del año. En estos casos el intervalo deseado no se puede distinguir del intervalo correspondiente al próximo rango más alto. Debido a esta ambigüedad esencial, no se recomienda el uso de esta propiedad y está desaprobada.</skos:note>
    </owl:DatatypeProperty>
    


    <!-- http://www.w3.org/2006/time#year -->


    <owl:DatatypeProperty rdf:about="http://www.w3.org/2006/time#year">
        <rdfs:domain rdf:resource="http://www.w3.org/2006/time#GeneralDateTimeDescription"/>
        <rdfs:comment xml:lang="es">Posición de año en un sistema calendario-reloj.

l rango de esta propiedad no está especificado, por tanto, se puede reemplazar por cualquier representación específica de un año de calendario de un calendario cualquiera.</rdfs:comment>
        <rdfs:comment xml:lang="en">Year position in a calendar-clock system.

The range of this property is not specified, so can be replaced by any specific representation of a calendar year from any calendar. </rdfs:comment>
        <rdfs:label xml:lang="en">year</rdfs:label>
    </owl:DatatypeProperty>
    


    <!-- http://www.w3.org/2006/time#years -->


    <owl:DatatypeProperty rdf:about="http://www.w3.org/2006/time#years">
        <rdfs:domain rdf:resource="http://www.w3.org/2006/time#GeneralDurationDescription"/>
        <rdfs:range rdf:resource="http://www.w3.org/2001/XMLSchema#decimal"/>
        <rdfs:comment xml:lang="es">Longitud de, o elemento de la longitud de, una extensión temporal expresada en años.</rdfs:comment>
        <rdfs:comment xml:lang="en">length of, or element of the length of, a temporal extent expressed in years</rdfs:comment>
        <rdfs:label xml:lang="es">duración en años</rdfs:label>
        <rdfs:label xml:lang="en">years duration</rdfs:label>
    </owl:DatatypeProperty>
    


    <!-- http://www.w3.org/2006/vcard/ns#street-address -->


    <owl:DatatypeProperty rdf:about="http://www.w3.org/2006/vcard/ns#street-address"/>
    


    <!-- http://www.w3.org/2008/05/skos#notation -->


    <owl:DatatypeProperty rdf:about="http://www.w3.org/2008/05/skos#notation"/>
    


    <!-- http://www.w3.org/2015/03/inspire/cp#nationalCadastralReference -->


    <owl:DatatypeProperty rdf:about="http://www.w3.org/2015/03/inspire/cp#nationalCadastralReference">
        <rdfs:subPropertyOf rdf:resource="http://www.w3.org/2008/05/skos#notation"/>
        <rdfs:domain rdf:resource="http://www.w3.org/2015/03/inspire/cp#CadastralParcel"/>
        <rdfs:range rdf:resource="http://www.w3.org/2001/XMLSchema#string"/>
        <rdfs:comment xml:lang="en">Thematic identifier at national level, generally the full national code of the basic property unit. Must ensure the link to the national cadastral register or equivalent.</rdfs:comment>
        <rdfs:isDefinedBy rdf:resource="http://www.w3.org/2015/03/inspire/cp"/>
        <rdfs:label xml:lang="en">national cadastral reference</rdfs:label>
    </owl:DatatypeProperty>
    


    <!-- https://saref.etsi.org/core/hasDescription -->


    <owl:DatatypeProperty rdf:about="https://saref.etsi.org/core/hasDescription">
        <rdfs:range rdf:resource="http://www.w3.org/2001/XMLSchema#string"/>
        <rdfs:comment xml:lang="en">A relationship providing a description of an entity (e.g., device)</rdfs:comment>
        <rdfs:comment xml:lang="en">A relationship providing a description of an entity (e.g., device). The value is expected to be a string or a string with language tag.</rdfs:comment>
        <rdfs:comment xml:lang="en">DEPRECATED: The use of rdfs:comment is recommended instead.</rdfs:comment>
        <rdfs:isDefinedBy rdf:resource="https://saref.etsi.org/core/"/>
        <rdfs:label xml:lang="en">has description</rdfs:label>
        <owl:deprecated rdf:datatype="http://www.w3.org/2001/XMLSchema#boolean">true</owl:deprecated>
    </owl:DatatypeProperty>
    


    <!-- https://saref.etsi.org/core/hasManufacturer -->


    <owl:DatatypeProperty rdf:about="https://saref.etsi.org/core/hasManufacturer">
        <rdfs:range rdf:resource="http://www.w3.org/2001/XMLSchema#string"/>
        <rdfs:comment xml:lang="en">A relationship identifying the manufacturer of an entity (e.g., device)</rdfs:comment>
        <rdfs:comment xml:lang="en">A relationship identifying the manufacturer of an entity (e.g., device). The value is expected to be a string or a string with language tag.</rdfs:comment>
        <rdfs:isDefinedBy rdf:resource="https://saref.etsi.org/core/"/>
        <rdfs:label xml:lang="en">has manufacturer</rdfs:label>
    </owl:DatatypeProperty>
    


    <!-- https://saref.etsi.org/core/hasModel -->


    <owl:DatatypeProperty rdf:about="https://saref.etsi.org/core/hasModel">
        <rdfs:range rdf:resource="http://www.w3.org/2001/XMLSchema#string"/>
        <rdfs:comment xml:lang="en">A relationship identifying the model of an entity (e.g., device)</rdfs:comment>
        <rdfs:comment xml:lang="en">A relationship identifying the model of an entity (e.g., device). The value is expected to be a string or a string with language tag.</rdfs:comment>
        <rdfs:isDefinedBy rdf:resource="https://saref.etsi.org/core/"/>
        <rdfs:label xml:lang="en">has model</rdfs:label>
    </owl:DatatypeProperty>
    


    <!-- https://saref.etsi.org/core/hasTimestamp -->


    <owl:DatatypeProperty rdf:about="https://saref.etsi.org/core/hasTimestamp">
        <rdf:type rdf:resource="http://www.w3.org/2002/07/owl#FunctionalProperty"/>
        <rdfs:range rdf:resource="http://www.w3.org/2001/XMLSchema#dateTime"/>
        <rdfs:comment xml:lang="en">A relationship stating the timestamp of an entity (e.g. a measurement).</rdfs:comment>
        <rdfs:isDefinedBy rdf:resource="https://saref.etsi.org/core/"/>
        <rdfs:isDefinedBy>https://saref.etsi.org/core/</rdfs:isDefinedBy>
        <rdfs:label xml:lang="en">has timestamp</rdfs:label>
    </owl:DatatypeProperty>
    


    <!-- https://saref.etsi.org/core/hasValue -->


    <owl:DatatypeProperty rdf:about="https://saref.etsi.org/core/hasValue">
        <rdfs:comment xml:lang="en">A relationship defining the value of a certain property, e.g., energy or power</rdfs:comment>
        <rdfs:comment xml:lang="en">A relationship defining the value of a certain property, e.g., energy or power. Note that, even if numeric values are expected to enable reasoning, measurement values could use other datatypes.</rdfs:comment>
        <rdfs:isDefinedBy rdf:resource="https://saref.etsi.org/core/"/>
        <rdfs:label xml:lang="en">has value</rdfs:label>
    </owl:DatatypeProperty>
    


    <!-- https://saref.etsi.org/saref4agri/hasBirthDate -->


    <owl:DatatypeProperty rdf:about="https://saref.etsi.org/saref4agri/hasBirthDate">
        <rdfs:range rdf:resource="http://www.w3.org/2001/XMLSchema#dateTime"/>
        <rdfs:comment xml:lang="en">A relation to express the birth date of an animal.</rdfs:comment>
        <rdfs:label xml:lang="en">has birth date</rdfs:label>
    </owl:DatatypeProperty>
    


    <!-- https://saref.etsi.org/saref4agri/hasDeathDate -->


    <owl:DatatypeProperty rdf:about="https://saref.etsi.org/saref4agri/hasDeathDate">
        <rdfs:range rdf:resource="http://www.w3.org/2001/XMLSchema#dateTime"/>
        <rdfs:comment xml:lang="en">A relation to express the death date of an animal.</rdfs:comment>
        <rdfs:label xml:lang="en">has death date</rdfs:label>
    </owl:DatatypeProperty>
    


    <!-- https://saref.etsi.org/saref4agri/hasHarvestDate -->


    <owl:DatatypeProperty rdf:about="https://saref.etsi.org/saref4agri/hasHarvestDate">
        <rdfs:subPropertyOf rdf:resource="http://www.w3.org/2002/07/owl#topDataProperty"/>
        <rdfs:range rdf:resource="http://www.w3.org/2001/XMLSchema#dateTime"/>
        <rdfs:comment xml:lang="en">A relation to express the day the crop is harvested.</rdfs:comment>
        <rdfs:label xml:lang="en">has harvest date</rdfs:label>
    </owl:DatatypeProperty>
    


    <!-- https://saref.etsi.org/saref4agri/hasName -->


    <owl:DatatypeProperty rdf:about="https://saref.etsi.org/saref4agri/hasName">
        <rdfs:range rdf:resource="http://www.w3.org/2001/XMLSchema#string"/>
        <rdfs:comment xml:lang="en">A relation to express the name of an entity (e.g.,animal).</rdfs:comment>
        <rdfs:label xml:lang="en">has name</rdfs:label>
    </owl:DatatypeProperty>
    


    <!-- https://saref.etsi.org/saref4agri/hasPlantDate -->


    <owl:DatatypeProperty rdf:about="https://saref.etsi.org/saref4agri/hasPlantDate">
        <rdfs:subPropertyOf rdf:resource="http://www.w3.org/2002/07/owl#topDataProperty"/>
        <rdfs:range rdf:resource="http://www.w3.org/2001/XMLSchema#dateTime"/>
        <rdfs:comment xml:lang="en">A relation to express the day the crop is planted.</rdfs:comment>
        <rdfs:label xml:lang="en">has plant date</rdfs:label>
    </owl:DatatypeProperty>
    


    <!-- https://saref.etsi.org/saref4bldg/accessType -->


    <owl:DatatypeProperty rdf:about="https://saref.etsi.org/saref4bldg/accessType">
        <rdfs:range rdf:resource="http://www.w3.org/2001/XMLSchema#string"/>
        <rdfs:comment xml:lang="en">Defines the types of access (or cover) to a tank that may be specified. Note that covers are generally specified for rectangular tanks. For cylindrical tanks, access will normally be via a manhole.</rdfs:comment>
        <rdfs:label xml:lang="en">access type</rdfs:label>
    </owl:DatatypeProperty>
    


    <!-- https://saref.etsi.org/saref4bldg/application -->


    <owl:DatatypeProperty rdf:about="https://saref.etsi.org/saref4bldg/application">
        <rdfs:range rdf:resource="http://www.w3.org/2001/XMLSchema#string"/>
        <rdfs:comment xml:lang="en">Humidifier application. Fixed: Humidifier installed in a ducted flow distribution system. Portable: Humidifier is not installed in a ducted flow distribution system.</rdfs:comment>
        <rdfs:label xml:lang="en">application</rdfs:label>
    </owl:DatatypeProperty>
    


    <!-- https://saref.etsi.org/saref4bldg/arrangement -->


    <owl:DatatypeProperty rdf:about="https://saref.etsi.org/saref4bldg/arrangement">
        <rdfs:range rdf:resource="http://www.w3.org/2001/XMLSchema#string"/>
        <rdfs:comment xml:lang="en">Defines the basic flow arrangements for the heat exchanger: COUNTERFLOW: Counterflow heat exchanger arrangement. CROSSFLOW: Crossflow heat exchanger arrangement. PARALLELFLOW: Parallel flow heat exchanger arrangement. MULTIPASS: Multipass flow heat exchanger arrangement. OTHER: Other type of heat exchanger flow arrangement not defined above.</rdfs:comment>
        <rdfs:label xml:lang="en">arrangement</rdfs:label>
    </owl:DatatypeProperty>
    


    <!-- https://saref.etsi.org/saref4bldg/bladeAction -->


    <owl:DatatypeProperty rdf:about="https://saref.etsi.org/saref4bldg/bladeAction">
        <rdfs:range rdf:resource="http://www.w3.org/2001/XMLSchema#string"/>
        <rdfs:comment xml:lang="en">Blade action.</rdfs:comment>
        <rdfs:label xml:lang="en">blade action</rdfs:label>
    </owl:DatatypeProperty>
    


    <!-- https://saref.etsi.org/saref4bldg/bladeEdge -->


    <owl:DatatypeProperty rdf:about="https://saref.etsi.org/saref4bldg/bladeEdge">
        <rdfs:range rdf:resource="http://www.w3.org/2001/XMLSchema#string"/>
        <rdfs:comment xml:lang="en">Blade edge.</rdfs:comment>
        <rdfs:label xml:lang="en">blade edge</rdfs:label>
    </owl:DatatypeProperty>
    


    <!-- https://saref.etsi.org/saref4bldg/bladeShape -->


    <owl:DatatypeProperty rdf:about="https://saref.etsi.org/saref4bldg/bladeShape">
        <rdfs:range rdf:resource="http://www.w3.org/2001/XMLSchema#string"/>
        <rdfs:comment xml:lang="en">Blade shape. Flat means triple V-groove.</rdfs:comment>
        <rdfs:label xml:lang="en">blade shape</rdfs:label>
    </owl:DatatypeProperty>
    


    <!-- https://saref.etsi.org/saref4bldg/capacityControl -->


    <owl:DatatypeProperty rdf:about="https://saref.etsi.org/saref4bldg/capacityControl">
        <rdfs:range rdf:resource="http://www.w3.org/2001/XMLSchema#string"/>
        <rdfs:comment xml:lang="en">FanCycling: Fan is cycled on and off to control duty. TwoSpeedFan: Fan is switched between low and high speed to control duty. VariableSpeedFan: Fan speed is varied to control duty. DampersControl: Dampers modulate the air flow to control duty. BypassValveControl: Bypass valve modulates the water flow to control duty. MultipleSeriesPumps: Turn on/off multiple series pump to control duty. TwoSpeedPump: Switch between high/low pump speed to control duty. VariableSpeedPump: vary pump speed to control duty.</rdfs:comment>
        <rdfs:label xml:lang="en">capacity control</rdfs:label>
    </owl:DatatypeProperty>
    


    <!-- https://saref.etsi.org/saref4bldg/capacityControlType -->


    <owl:DatatypeProperty rdf:about="https://saref.etsi.org/saref4bldg/capacityControlType">
        <rdfs:range rdf:resource="http://www.w3.org/2001/XMLSchema#string"/>
        <rdfs:comment xml:lang="en">InletVane: Control by adjusting inlet vane. VariableSpeedDrive: Control by variable speed drive. BladePitchAngle: Control by adjusting blade pitch angle. TwoSpeed: Control by switch between high and low speed. DischargeDamper: Control by modulating discharge damper.</rdfs:comment>
        <rdfs:label xml:lang="en">capacity control type</rdfs:label>
    </owl:DatatypeProperty>
    


    <!-- https://saref.etsi.org/saref4bldg/capacityPeople -->


    <owl:DatatypeProperty rdf:about="https://saref.etsi.org/saref4bldg/capacityPeople">
        <rdfs:range rdf:resource="http://www.w3.org/2001/XMLSchema#nonNegativeInteger"/>
        <rdfs:comment xml:lang="en">Capacity of the transportation element measured in numbers of person.</rdfs:comment>
        <rdfs:label xml:lang="en">capacity people</rdfs:label>
    </owl:DatatypeProperty>
    


    <!-- https://saref.etsi.org/saref4bldg/circuitType -->


    <owl:DatatypeProperty rdf:about="https://saref.etsi.org/saref4bldg/circuitType">
        <rdfs:range rdf:resource="http://www.w3.org/2001/XMLSchema#string"/>
        <rdfs:comment xml:lang="en">OpenCircuit: Exposes water directly to the cooling atmosphere. CloseCircuit: The fluid is separated from the atmosphere by a heat exchanger. Wet: The air stream or the heat exchange surface is evaporatively cooled. Dry: No evaporation into the air stream. DryWet: A combination of a dry tower and a wet tower.</rdfs:comment>
        <rdfs:label xml:lang="en">circuit type</rdfs:label>
    </owl:DatatypeProperty>
    


    <!-- https://saref.etsi.org/saref4bldg/colorAppearance -->


    <owl:DatatypeProperty rdf:about="https://saref.etsi.org/saref4bldg/colorAppearance">
        <rdfs:range rdf:resource="http://www.w3.org/2001/XMLSchema#string"/>
        <rdfs:comment xml:lang="en">In both the DIN and CIE standards, artificial light sources are classified in terms of their color appearance. To the human eye they all appear to be white the difference can only be detected by direct comparison. Visual performance is not directly affected by differences in color appearance.</rdfs:comment>
        <rdfs:label xml:lang="en">color appearance</rdfs:label>
    </owl:DatatypeProperty>
    


    <!-- https://saref.etsi.org/saref4bldg/colorRenderingIndex -->


    <owl:DatatypeProperty rdf:about="https://saref.etsi.org/saref4bldg/colorRenderingIndex">
        <rdfs:range rdf:resource="http://www.w3.org/2001/XMLSchema#integer"/>
        <rdfs:comment xml:lang="en">The CRI indicates how well a light source renders eight standard colors compared to perfect reference lamp with the same color temperature. The CRI scale ranges from 1 to 100, with 100 representing perfect rendering properties.</rdfs:comment>
        <rdfs:label xml:lang="en">color rendering index</rdfs:label>
    </owl:DatatypeProperty>
    


    <!-- https://saref.etsi.org/saref4bldg/controlStrategy -->


    <owl:DatatypeProperty rdf:about="https://saref.etsi.org/saref4bldg/controlStrategy">
        <rdfs:range rdf:resource="http://www.w3.org/2001/XMLSchema#string"/>
        <rdfs:comment xml:lang="en">FixedExitingWaterTemp: The capacity is controlled to maintain a fixed exiting water temperature. WetBulbTempReset: The set-point is reset based on the wet-bulb temperature.</rdfs:comment>
        <rdfs:label xml:lang="en">control strategy</rdfs:label>
    </owl:DatatypeProperty>
    


    <!-- https://saref.etsi.org/saref4bldg/endShapeType -->


    <owl:DatatypeProperty rdf:about="https://saref.etsi.org/saref4bldg/endShapeType">
        <rdfs:range rdf:resource="http://www.w3.org/2001/XMLSchema#string"/>
        <rdfs:comment xml:lang="en">Defines the types of end shapes that can be used for preformed tanks. The convention for reading these enumerated values is that for a vertical cylinder, the first value is the base and the second is the top for a horizontal cylinder, the order of reading should be left to right. For a speherical tank, the value UNSET should be used.B5</rdfs:comment>
        <rdfs:label xml:lang="en">end shape type</rdfs:label>
    </owl:DatatypeProperty>
    


    <!-- https://saref.etsi.org/saref4bldg/energySource -->


    <owl:DatatypeProperty rdf:about="https://saref.etsi.org/saref4bldg/energySource">
        <rdfs:range rdf:resource="http://www.w3.org/2001/XMLSchema#string"/>
        <rdfs:comment xml:lang="en">Enumeration defining the energy source or fuel cumbusted to generate heat.</rdfs:comment>
        <rdfs:comment xml:lang="en">The source of energy.</rdfs:comment>
        <rdfs:label xml:lang="en">energy source</rdfs:label>
    </owl:DatatypeProperty>
    


    <!-- https://saref.etsi.org/saref4bldg/evaporationCoolant -->


    <owl:DatatypeProperty rdf:about="https://saref.etsi.org/saref4bldg/evaporationCoolant">
        <rdfs:range rdf:resource="http://www.w3.org/2001/XMLSchema#string"/>
        <rdfs:comment xml:lang="en">The fluid used for the coolant in the evaporator.</rdfs:comment>
        <rdfs:label xml:lang="en">evaporation coolant</rdfs:label>
    </owl:DatatypeProperty>
    


    <!-- https://saref.etsi.org/saref4bldg/evaporationMediumType -->


    <owl:DatatypeProperty rdf:about="https://saref.etsi.org/saref4bldg/evaporationMediumType">
        <rdfs:range rdf:resource="http://www.w3.org/2001/XMLSchema#string"/>
        <rdfs:comment xml:lang="en">ColdLiquid: Evaporator is using liquid type of fluid to exchange heat with refrigerant. ColdAir: Evaporator is using air to exchange heat with refrigerant.</rdfs:comment>
        <rdfs:label xml:lang="en">evaporation medium type</rdfs:label>
    </owl:DatatypeProperty>
    


    <!-- https://saref.etsi.org/saref4bldg/failPosition -->


    <owl:DatatypeProperty rdf:about="https://saref.etsi.org/saref4bldg/failPosition">
        <rdfs:range rdf:resource="http://www.w3.org/2001/XMLSchema#string"/>
        <rdfs:comment xml:lang="en">Specifies the required fail-safe position of the actuator.</rdfs:comment>
        <rdfs:label xml:lang="en">fail position</rdfs:label>
    </owl:DatatypeProperty>
    


    <!-- https://saref.etsi.org/saref4bldg/finishColor -->


    <owl:DatatypeProperty rdf:about="https://saref.etsi.org/saref4bldg/finishColor">
        <rdfs:range rdf:resource="http://www.w3.org/2001/XMLSchema#string"/>
        <rdfs:comment xml:lang="en">Finish color for cooled beam.</rdfs:comment>
        <rdfs:label xml:lang="en">finish color</rdfs:label>
    </owl:DatatypeProperty>
    


    <!-- https://saref.etsi.org/saref4bldg/fireExit -->


    <owl:DatatypeProperty rdf:about="https://saref.etsi.org/saref4bldg/fireExit">
        <rdfs:range rdf:resource="http://www.w3.org/2001/XMLSchema#boolean"/>
        <rdfs:comment xml:lang="en">Indication whether this object is designed to serve as an exit in the case of fire (TRUE) or not (FALSE). Here whether the transport element (in case of e.g., a lift) is designed to serve as a fire exit, e.g., for fire escape purposes.</rdfs:comment>
        <rdfs:label xml:lang="en">fire exit</rdfs:label>
    </owl:DatatypeProperty>
    


    <!-- https://saref.etsi.org/saref4bldg/flowArrangement -->


    <owl:DatatypeProperty rdf:about="https://saref.etsi.org/saref4bldg/flowArrangement">
        <rdfs:range rdf:resource="http://www.w3.org/2001/XMLSchema#string"/>
        <rdfs:comment xml:lang="en">CounterFlow: Air and water flow enter in different directions. CrossFlow: Air and water flow are perpendicular. ParallelFlow: air and water flow enter in same directions.</rdfs:comment>
        <rdfs:label xml:lang="en">flow arrangement</rdfs:label>
    </owl:DatatypeProperty>
    


    <!-- https://saref.etsi.org/saref4bldg/frameSize -->


    <owl:DatatypeProperty rdf:about="https://saref.etsi.org/saref4bldg/frameSize">
        <rdfs:range rdf:resource="http://www.w3.org/2001/XMLSchema#string"/>
        <rdfs:comment xml:lang="en">Designation of the frame size according to the named range of frame sizes designated at the place of use or according to a given standard.</rdfs:comment>
        <rdfs:label xml:lang="en">frame size</rdfs:label>
    </owl:DatatypeProperty>
    


    <!-- https://saref.etsi.org/saref4bldg/frameType -->


    <owl:DatatypeProperty rdf:about="https://saref.etsi.org/saref4bldg/frameType">
        <rdfs:range rdf:resource="http://www.w3.org/2001/XMLSchema#string"/>
        <rdfs:comment xml:lang="en">The type of frame used by the damper (e.g., Standard, Single Flange, Single Reversed Flange, Double Flange, etc.).</rdfs:comment>
        <rdfs:label xml:lang="en">frame type</rdfs:label>
    </owl:DatatypeProperty>
    


    <!-- https://saref.etsi.org/saref4bldg/hasDefrost -->


    <owl:DatatypeProperty rdf:about="https://saref.etsi.org/saref4bldg/hasDefrost">
        <rdfs:range rdf:resource="http://www.w3.org/2001/XMLSchema#boolean"/>
        <rdfs:comment xml:lang="en">Whether the heat exchanger has defrost function or not.</rdfs:comment>
        <rdfs:label xml:lang="en">has defrost</rdfs:label>
    </owl:DatatypeProperty>
    


    <!-- https://saref.etsi.org/saref4bldg/hasExteriorInsulation -->


    <owl:DatatypeProperty rdf:about="https://saref.etsi.org/saref4bldg/hasExteriorInsulation">
        <rdfs:range rdf:resource="http://www.w3.org/2001/XMLSchema#boolean"/>
        <rdfs:comment xml:lang="en">TRUE if the silencer has exterior insulation. FALSE if it does not.</rdfs:comment>
        <rdfs:label xml:lang="en">has exterior insulation</rdfs:label>
    </owl:DatatypeProperty>
    


    <!-- https://saref.etsi.org/saref4bldg/hasHotGasBypass -->


    <owl:DatatypeProperty rdf:about="https://saref.etsi.org/saref4bldg/hasHotGasBypass">
        <rdfs:range rdf:resource="http://www.w3.org/2001/XMLSchema#boolean"/>
        <rdfs:comment xml:lang="en">Whether or not hot gas bypass is provided for the compressor. TRUE = Yes, FALSE = No.</rdfs:comment>
        <rdfs:label xml:lang="en">has hot gas bypass</rdfs:label>
    </owl:DatatypeProperty>
    


    <!-- https://saref.etsi.org/saref4bldg/hasLock -->


    <owl:DatatypeProperty rdf:about="https://saref.etsi.org/saref4bldg/hasLock">
        <rdfs:range rdf:resource="http://www.w3.org/2001/XMLSchema#boolean"/>
        <rdfs:comment xml:lang="en">Indication of whether a switching device has a key operated lock (=TRUE) or not (= FALSE).</rdfs:comment>
        <rdfs:label xml:lang="en">has lock</rdfs:label>
    </owl:DatatypeProperty>
    


    <!-- https://saref.etsi.org/saref4bldg/hasPartWinding -->


    <owl:DatatypeProperty rdf:about="https://saref.etsi.org/saref4bldg/hasPartWinding">
        <rdfs:range rdf:resource="http://www.w3.org/2001/XMLSchema#boolean"/>
        <rdfs:comment xml:lang="en">Indication of whether the motor is single speed, i.e. has a single winding (= FALSE) or multi-speed i.e.has part winding (= TRUE) .</rdfs:comment>
        <rdfs:label xml:lang="en">has part winding</rdfs:label>
    </owl:DatatypeProperty>
    


    <!-- https://saref.etsi.org/saref4bldg/hasTurbulator -->


    <owl:DatatypeProperty rdf:about="https://saref.etsi.org/saref4bldg/hasTurbulator">
        <rdfs:range rdf:resource="http://www.w3.org/2001/XMLSchema#boolean"/>
        <rdfs:comment xml:lang="en">TRUE if the tube has a turbulator, FALSE if it does not.</rdfs:comment>
        <rdfs:label xml:lang="en">has turbulator</rdfs:label>
    </owl:DatatypeProperty>
    


    <!-- https://saref.etsi.org/saref4bldg/heatTransferDimension -->


    <owl:DatatypeProperty rdf:about="https://saref.etsi.org/saref4bldg/heatTransferDimension">
        <rdfs:range rdf:resource="http://www.w3.org/2001/XMLSchema#string"/>
        <rdfs:comment xml:lang="en">Indicates how heat is transmitted according to the shape of the space heater.</rdfs:comment>
        <rdfs:label xml:lang="en">heat transfer dimension</rdfs:label>
    </owl:DatatypeProperty>
    


    <!-- https://saref.etsi.org/saref4bldg/heatTransferMedium -->


    <owl:DatatypeProperty rdf:about="https://saref.etsi.org/saref4bldg/heatTransferMedium">
        <rdfs:range rdf:resource="http://www.w3.org/2001/XMLSchema#string"/>
        <rdfs:comment xml:lang="en">Enumeration defining the heat transfer medium if applicable.</rdfs:comment>
        <rdfs:label xml:lang="en">heat transfer medium</rdfs:label>
    </owl:DatatypeProperty>
    


    <!-- https://saref.etsi.org/saref4bldg/heatTransferTypeEnum -->


    <owl:DatatypeProperty rdf:about="https://saref.etsi.org/saref4bldg/heatTransferTypeEnum">
        <rdfs:range rdf:resource="http://www.w3.org/2001/XMLSchema#string"/>
        <rdfs:comment xml:lang="en">Type of heat transfer between the two air streams.</rdfs:comment>
        <rdfs:label xml:lang="en">heat transfer type enum</rdfs:label>
    </owl:DatatypeProperty>
    


    <!-- https://saref.etsi.org/saref4bldg/integratedLightingType -->


    <owl:DatatypeProperty rdf:about="https://saref.etsi.org/saref4bldg/integratedLightingType">
        <rdfs:range rdf:resource="http://www.w3.org/2001/XMLSchema#string"/>
        <rdfs:comment xml:lang="en">Integrated lighting in cooled beam.</rdfs:comment>
        <rdfs:label xml:lang="en">integrated lighting type</rdfs:label>
    </owl:DatatypeProperty>
    


    <!-- https://saref.etsi.org/saref4bldg/internalControl -->


    <owl:DatatypeProperty rdf:about="https://saref.etsi.org/saref4bldg/internalControl">
        <rdfs:range rdf:resource="http://www.w3.org/2001/XMLSchema#string"/>
        <rdfs:comment xml:lang="en">Internal modulation control.</rdfs:comment>
        <rdfs:label xml:lang="en">internal control</rdfs:label>
    </owl:DatatypeProperty>
    


    <!-- https://saref.etsi.org/saref4bldg/isExternal -->


    <owl:DatatypeProperty rdf:about="https://saref.etsi.org/saref4bldg/isExternal">
        <rdfs:range rdf:resource="http://www.w3.org/2001/XMLSchema#boolean"/>
        <rdfs:comment xml:lang="en">Indication whether the element is designed for use in the exterior (TRUE) or not (FALSE). If (TRUE) it is an external element and faces the outside of the building.</rdfs:comment>
        <rdfs:label xml:lang="en">is external</rdfs:label>
    </owl:DatatypeProperty>
    


    <!-- https://saref.etsi.org/saref4bldg/isFreeHanging -->


    <owl:DatatypeProperty rdf:about="https://saref.etsi.org/saref4bldg/isFreeHanging">
        <rdfs:range rdf:resource="http://www.w3.org/2001/XMLSchema#boolean"/>
        <rdfs:comment xml:lang="en">Is it free hanging type (not mounted in a false ceiling)?</rdfs:comment>
        <rdfs:label xml:lang="en">is free hanging</rdfs:label>
    </owl:DatatypeProperty>
    


    <!-- https://saref.etsi.org/saref4bldg/isGuarded -->


    <owl:DatatypeProperty rdf:about="https://saref.etsi.org/saref4bldg/isGuarded">
        <rdfs:range rdf:resource="http://www.w3.org/2001/XMLSchema#boolean"/>
        <rdfs:comment xml:lang="en">Indication of whether the motor enclosure is guarded (= TRUE) or not (= FALSE).</rdfs:comment>
        <rdfs:label xml:lang="en">is guarded</rdfs:label>
    </owl:DatatypeProperty>
    


    <!-- https://saref.etsi.org/saref4bldg/isIlluminated -->


    <owl:DatatypeProperty rdf:about="https://saref.etsi.org/saref4bldg/isIlluminated">
        <rdfs:range rdf:resource="http://www.w3.org/2001/XMLSchema#boolean"/>
        <rdfs:comment xml:lang="en">An indication of whether there is an illuminated indicator to show that the switch is on (=TRUE) or not (= FALSE).</rdfs:comment>
        <rdfs:label xml:lang="en">is illuminated</rdfs:label>
    </owl:DatatypeProperty>
    


    <!-- https://saref.etsi.org/saref4bldg/isNeutralPrimaryTerminalAvailable -->


    <owl:DatatypeProperty rdf:about="https://saref.etsi.org/saref4bldg/isNeutralPrimaryTerminalAvailable">
        <rdfs:range rdf:resource="http://www.w3.org/2001/XMLSchema#boolean"/>
        <rdfs:comment xml:lang="en">An indication of whether the neutral point of the primary winding is available as a terminal (=TRUE) or not (= FALSE).</rdfs:comment>
        <rdfs:label xml:lang="en">is neutral primary terminal available</rdfs:label>
    </owl:DatatypeProperty>
    


    <!-- https://saref.etsi.org/saref4bldg/isNeutralSecondaryTerminalAvailable -->


    <owl:DatatypeProperty rdf:about="https://saref.etsi.org/saref4bldg/isNeutralSecondaryTerminalAvailable">
        <rdfs:range rdf:resource="http://www.w3.org/2001/XMLSchema#boolean"/>
        <rdfs:comment xml:lang="en">An indication of whether the neutral point of the secondary winding is available as a terminal (=TRUE) or not (= FALSE).</rdfs:comment>
        <rdfs:label xml:lang="en">is neutral secondary terminal available</rdfs:label>
    </owl:DatatypeProperty>
    


    <!-- https://saref.etsi.org/saref4bldg/isPluggableOutlet -->


    <owl:DatatypeProperty rdf:about="https://saref.etsi.org/saref4bldg/isPluggableOutlet">
        <rdfs:range rdf:resource="http://www.w3.org/2001/XMLSchema#boolean"/>
        <rdfs:comment xml:lang="en">Indication of whether the outlet accepts a loose plug connection (= TRUE) or whether it is directly connected (= FALSE) or whether the form of connection has not yet been determined (= UNKNOWN).</rdfs:comment>
        <rdfs:label xml:lang="en">is pluggable outlet</rdfs:label>
    </owl:DatatypeProperty>
    


    <!-- https://saref.etsi.org/saref4bldg/isWaterStorageHeater -->


    <owl:DatatypeProperty rdf:about="https://saref.etsi.org/saref4bldg/isWaterStorageHeater">
        <rdfs:range rdf:resource="http://www.w3.org/2001/XMLSchema#boolean"/>
        <rdfs:comment xml:lang="en">This is used to identify if the boiler has storage capacity (TRUE). If FALSE, then there is no storage capacity built into the boiler, such as an instantaneous hot water heater.</rdfs:comment>
        <rdfs:label xml:lang="en">is water storage heater</rdfs:label>
    </owl:DatatypeProperty>
    


    <!-- https://saref.etsi.org/saref4bldg/lampBallastType -->


    <owl:DatatypeProperty rdf:about="https://saref.etsi.org/saref4bldg/lampBallastType">
        <rdfs:range rdf:resource="http://www.w3.org/2001/XMLSchema#string"/>
        <rdfs:comment xml:lang="en">The type of ballast used to stabilise gas discharge by limiting the current during operation and to deliver the necessary striking voltage for starting. Ballasts are needed to operate Discharge Lamps such as Fluorescent, Compact Fluorescent, High-pressure Mercury, Metal Halide and High-pressure Sodium Lamps. Magnetic ballasts are chokes which limit the current passing through a lamp connected in series on the principle of self-induction. The resultant current and power are decisive for the efficient operation of the lamp. A specially designed ballast is required for every type of lamp to comply with lamp rating in terms of Luminous Flux, Color Appearance and service life. The two types of magnetic ballasts for fluorescent lamps are KVG Conventional (EC-A series) and VVG Low-loss ballasts (EC-B series). Low-loss ballasts have a higher efficiency, which means reduced ballast losses and a lower thermal load. Electronic ballasts are used to run fluorescent lamps at high frequencies (approx. 35 - 40 kHz).</rdfs:comment>
        <rdfs:label xml:lang="en">lamp ballast type</rdfs:label>
    </owl:DatatypeProperty>
    


    <!-- https://saref.etsi.org/saref4bldg/lampCompensationType -->


    <owl:DatatypeProperty rdf:about="https://saref.etsi.org/saref4bldg/lampCompensationType">
        <rdfs:range rdf:resource="http://www.w3.org/2001/XMLSchema#string"/>
        <rdfs:comment xml:lang="en">Identifies the form of compensation used for power factor correction and radio suppression.</rdfs:comment>
        <rdfs:label xml:lang="en">lamp compensation type</rdfs:label>
    </owl:DatatypeProperty>
    


    <!-- https://saref.etsi.org/saref4bldg/legend -->


    <owl:DatatypeProperty rdf:about="https://saref.etsi.org/saref4bldg/legend">
        <rdfs:range rdf:resource="http://www.w3.org/2001/XMLSchema#string"/>
        <rdfs:comment xml:lang="en">A text inscribed or applied to the switch as a legend to indicate purpose or function.</rdfs:comment>
        <rdfs:label xml:lang="en">legend</rdfs:label>
    </owl:DatatypeProperty>
    


    <!-- https://saref.etsi.org/saref4bldg/manualOverride -->


    <owl:DatatypeProperty rdf:about="https://saref.etsi.org/saref4bldg/manualOverride">
        <rdfs:range rdf:resource="http://www.w3.org/2001/XMLSchema#boolean"/>
        <rdfs:comment xml:lang="en">Identifies whether hand-operated operation is provided as an override (= TRUE) or not (= FALSE). Note that this value should be set to FALSE by default in the case of a Hand Operated Actuator.</rdfs:comment>
        <rdfs:label xml:lang="en">manual override</rdfs:label>
    </owl:DatatypeProperty>
    


    <!-- https://saref.etsi.org/saref4bldg/mechanicalOperated -->


    <owl:DatatypeProperty rdf:about="https://saref.etsi.org/saref4bldg/mechanicalOperated">
        <rdfs:range rdf:resource="http://www.w3.org/2001/XMLSchema#boolean"/>
        <rdfs:comment xml:lang="en">Indication whether the element is operated machanically (TRUE) or not, i.e. manually (FALSE).</rdfs:comment>
        <rdfs:label xml:lang="en">mechanical operated</rdfs:label>
    </owl:DatatypeProperty>
    


    <!-- https://saref.etsi.org/saref4bldg/mediaSource -->


    <owl:DatatypeProperty rdf:about="https://saref.etsi.org/saref4bldg/mediaSource">
        <rdfs:range rdf:resource="http://www.w3.org/2001/XMLSchema#string"/>
        <rdfs:comment xml:lang="en">Indicates media sources and corresponding names of ports (DistributionPort with FlowDirection=SINK and PredefinedType=AUDIOVISUAL) or aggregated audio/video components (AudioVisualAppliance).</rdfs:comment>
        <rdfs:label xml:lang="en">media source</rdfs:label>
    </owl:DatatypeProperty>
    


    <!-- https://saref.etsi.org/saref4bldg/motorDriveType -->


    <owl:DatatypeProperty rdf:about="https://saref.etsi.org/saref4bldg/motorDriveType">
        <rdfs:range rdf:resource="http://www.w3.org/2001/XMLSchema#string"/>
        <rdfs:comment xml:lang="en">Motor drive type: DIRECTDRIVE: Direct drive. BELTDRIVE: Belt drive. COUPLING: Coupling. OTHER: Other type of motor drive. UNKNOWN: Unknown motor drive type. </rdfs:comment>
        <rdfs:label xml:lang="en">motor drive type</rdfs:label>
    </owl:DatatypeProperty>
    


    <!-- https://saref.etsi.org/saref4bldg/motorEnclosureType -->


    <owl:DatatypeProperty rdf:about="https://saref.etsi.org/saref4bldg/motorEnclosureType">
        <rdfs:range rdf:resource="http://www.w3.org/2001/XMLSchema#string"/>
        <rdfs:comment xml:lang="en">A list of the available types of motor enclosure from which that required may be selected.</rdfs:comment>
        <rdfs:label xml:lang="en">motor enclosure type</rdfs:label>
    </owl:DatatypeProperty>
    


    <!-- https://saref.etsi.org/saref4bldg/numberOfBlades -->


    <owl:DatatypeProperty rdf:about="https://saref.etsi.org/saref4bldg/numberOfBlades">
        <rdfs:range rdf:resource="http://www.w3.org/2001/XMLSchema#integer"/>
        <rdfs:comment xml:lang="en">Number of blades.</rdfs:comment>
        <rdfs:label xml:lang="en">number of blades</rdfs:label>
    </owl:DatatypeProperty>
    


    <!-- https://saref.etsi.org/saref4bldg/numberOfCells -->


    <owl:DatatypeProperty rdf:about="https://saref.etsi.org/saref4bldg/numberOfCells">
        <rdfs:range rdf:resource="http://www.w3.org/2001/XMLSchema#integer"/>
        <rdfs:comment xml:lang="en">Number of cells in one cooling tower unit.</rdfs:comment>
        <rdfs:label xml:lang="en">number of cells</rdfs:label>
    </owl:DatatypeProperty>
    


    <!-- https://saref.etsi.org/saref4bldg/numberOfCircuits -->


    <owl:DatatypeProperty rdf:about="https://saref.etsi.org/saref4bldg/numberOfCircuits">
        <rdfs:range rdf:resource="http://www.w3.org/2001/XMLSchema#integer"/>
        <rdfs:comment xml:lang="en">Number of parallel fluid tube circuits.</rdfs:comment>
        <rdfs:label xml:lang="en">number of circuits</rdfs:label>
    </owl:DatatypeProperty>
    


    <!-- https://saref.etsi.org/saref4bldg/numberOfGangs -->


    <owl:DatatypeProperty rdf:about="https://saref.etsi.org/saref4bldg/numberOfGangs">
        <rdfs:range rdf:resource="http://www.w3.org/2001/XMLSchema#integer"/>
        <rdfs:comment xml:lang="en">Number of gangs/buttons on this switch.</rdfs:comment>
        <rdfs:label xml:lang="en">number of gangs</rdfs:label>
    </owl:DatatypeProperty>
    


    <!-- https://saref.etsi.org/saref4bldg/numberOfPanels -->


    <owl:DatatypeProperty rdf:about="https://saref.etsi.org/saref4bldg/numberOfPanels">
        <rdfs:range rdf:resource="http://www.w3.org/2001/XMLSchema#integer"/>
        <rdfs:comment xml:lang="en">Number of panels.</rdfs:comment>
        <rdfs:label xml:lang="en">number of panels</rdfs:label>
    </owl:DatatypeProperty>
    


    <!-- https://saref.etsi.org/saref4bldg/numberOfRows -->


    <owl:DatatypeProperty rdf:about="https://saref.etsi.org/saref4bldg/numberOfRows">
        <rdfs:range rdf:resource="http://www.w3.org/2001/XMLSchema#integer"/>
        <rdfs:comment xml:lang="en">Number of tube rows in the tube bundle assembly.</rdfs:comment>
        <rdfs:label xml:lang="en">number of rows</rdfs:label>
    </owl:DatatypeProperty>
    


    <!-- https://saref.etsi.org/saref4bldg/numberOfSections -->


    <owl:DatatypeProperty rdf:about="https://saref.etsi.org/saref4bldg/numberOfSections">
        <rdfs:range rdf:resource="http://www.w3.org/2001/XMLSchema#integer"/>
        <rdfs:comment xml:lang="en">Number of sections used.</rdfs:comment>
        <rdfs:label xml:lang="en">number of sections</rdfs:label>
    </owl:DatatypeProperty>
    


    <!-- https://saref.etsi.org/saref4bldg/numberOsSockets -->


    <owl:DatatypeProperty rdf:about="https://saref.etsi.org/saref4bldg/numberOsSockets">
        <rdfs:range rdf:resource="http://www.w3.org/2001/XMLSchema#integer"/>
        <rdfs:comment xml:lang="en">The number of sockets that may be connected. In case of inconsistency, sockets defined on ports take precedence.</rdfs:comment>
        <rdfs:label xml:lang="en">number os sockets</rdfs:label>
    </owl:DatatypeProperty>
    


    <!-- https://saref.etsi.org/saref4bldg/operatingMode -->


    <owl:DatatypeProperty rdf:about="https://saref.etsi.org/saref4bldg/operatingMode">
        <rdfs:range rdf:resource="http://www.w3.org/2001/XMLSchema#string"/>
        <rdfs:comment xml:lang="en">Identifies the operating mode of the boiler.</rdfs:comment>
        <rdfs:label xml:lang="en">operating mode</rdfs:label>
    </owl:DatatypeProperty>
    


    <!-- https://saref.etsi.org/saref4bldg/operation -->


    <owl:DatatypeProperty rdf:about="https://saref.etsi.org/saref4bldg/operation">
        <rdfs:range rdf:resource="http://www.w3.org/2001/XMLSchema#string"/>
        <rdfs:comment xml:lang="en">The operational mechanism for the damper operation.</rdfs:comment>
        <rdfs:label xml:lang="en">operation</rdfs:label>
    </owl:DatatypeProperty>
    


    <!-- https://saref.etsi.org/saref4bldg/orientation -->


    <owl:DatatypeProperty rdf:about="https://saref.etsi.org/saref4bldg/orientation">
        <rdfs:range rdf:resource="http://www.w3.org/2001/XMLSchema#string"/>
        <rdfs:comment xml:lang="en">The intended orientation for the damper as specified by the manufacturer.</rdfs:comment>
        <rdfs:label xml:lang="en">orientation</rdfs:label>
    </owl:DatatypeProperty>
    


    <!-- https://saref.etsi.org/saref4bldg/patternType -->


    <owl:DatatypeProperty rdf:about="https://saref.etsi.org/saref4bldg/patternType">
        <rdfs:range rdf:resource="http://www.w3.org/2001/XMLSchema#string"/>
        <rdfs:comment xml:lang="en">Defines the types of pattern (or shape of a tank that may be specified.</rdfs:comment>
        <rdfs:label xml:lang="en">pattern type</rdfs:label>
    </owl:DatatypeProperty>
    


    <!-- https://saref.etsi.org/saref4bldg/pipeConnectionEnum -->


    <owl:DatatypeProperty rdf:about="https://saref.etsi.org/saref4bldg/pipeConnectionEnum">
        <rdfs:range rdf:resource="http://www.w3.org/2001/XMLSchema#string"/>
        <rdfs:comment xml:lang="en">The manner in which the pipe connection is made to the cooled beam.</rdfs:comment>
        <rdfs:label xml:lang="en">pipe connection enum</rdfs:label>
    </owl:DatatypeProperty>
    


    <!-- https://saref.etsi.org/saref4bldg/placementType -->


    <owl:DatatypeProperty rdf:about="https://saref.etsi.org/saref4bldg/placementType">
        <rdfs:range rdf:resource="http://www.w3.org/2001/XMLSchema#string"/>
        <rdfs:comment xml:lang="en">Indicates how the device is designed to be placed.</rdfs:comment>
        <rdfs:label xml:lang="en">placement type</rdfs:label>
    </owl:DatatypeProperty>
    


    <!-- https://saref.etsi.org/saref4bldg/powerSource -->


    <owl:DatatypeProperty rdf:about="https://saref.etsi.org/saref4bldg/powerSource">
        <rdfs:range rdf:resource="http://www.w3.org/2001/XMLSchema#string"/>
        <rdfs:comment xml:lang="en">Type of power driving the compressor.</rdfs:comment>
        <rdfs:label xml:lang="en">power source</rdfs:label>
    </owl:DatatypeProperty>
    


    <!-- https://saref.etsi.org/saref4bldg/readOutType -->


    <owl:DatatypeProperty rdf:about="https://saref.etsi.org/saref4bldg/readOutType">
        <rdfs:range rdf:resource="http://www.w3.org/2001/XMLSchema#string"/>
        <rdfs:comment xml:lang="en">Indication of the form that readout from the meter takes. In the case of a dial read out, this may comprise multiple dials that give a cumulative reading and/or a mechanical odometer.</rdfs:comment>
        <rdfs:label xml:lang="en">read out type</rdfs:label>
    </owl:DatatypeProperty>
    


    <!-- https://saref.etsi.org/saref4bldg/refrigerantClass -->


    <owl:DatatypeProperty rdf:about="https://saref.etsi.org/saref4bldg/refrigerantClass">
        <rdfs:range rdf:resource="http://www.w3.org/2001/XMLSchema#string"/>
        <rdfs:comment xml:lang="en">Refrigerant class used by the compressor. CFC: Chlorofluorocarbons. HCFC: Hydrochlorofluorocarbons. HFC: Hydrofluorocarbons.</rdfs:comment>
        <rdfs:label xml:lang="en">refrigerant class</rdfs:label>
    </owl:DatatypeProperty>
    


    <!-- https://saref.etsi.org/saref4bldg/remoteReading -->


    <owl:DatatypeProperty rdf:about="https://saref.etsi.org/saref4bldg/remoteReading">
        <rdfs:range rdf:resource="http://www.w3.org/2001/XMLSchema#boolean"/>
        <rdfs:comment xml:lang="en">Indicates whether the meter has a connection for remote reading through connection of a communication device (set TRUE) or not (set FALSE).</rdfs:comment>
        <rdfs:label xml:lang="en">remote reading</rdfs:label>
    </owl:DatatypeProperty>
    


    <!-- https://saref.etsi.org/saref4bldg/roughness -->


    <owl:DatatypeProperty rdf:about="https://saref.etsi.org/saref4bldg/roughness">
        <rdfs:range rdf:resource="http://www.w3.org/2001/XMLSchema#string"/>
        <rdfs:comment xml:lang="en">A measure of the vertical deviations of the surface.</rdfs:comment>
        <rdfs:label xml:lang="en">roughness</rdfs:label>
    </owl:DatatypeProperty>
    


    <!-- https://saref.etsi.org/saref4bldg/secondaryCurrentType -->


    <owl:DatatypeProperty rdf:about="https://saref.etsi.org/saref4bldg/secondaryCurrentType">
        <rdfs:range rdf:resource="http://www.w3.org/2001/XMLSchema#string"/>
        <rdfs:comment xml:lang="en">A list of the secondary current types that can result from transformer output.</rdfs:comment>
        <rdfs:label xml:lang="en">secondary current type</rdfs:label>
    </owl:DatatypeProperty>
    


    <!-- https://saref.etsi.org/saref4bldg/shadingDeviceType -->


    <owl:DatatypeProperty rdf:about="https://saref.etsi.org/saref4bldg/shadingDeviceType">
        <rdfs:range rdf:resource="http://www.w3.org/2001/XMLSchema#string"/>
        <rdfs:comment xml:lang="en">Specifies the type of shading device.</rdfs:comment>
        <rdfs:label xml:lang="en">shading device type</rdfs:label>
    </owl:DatatypeProperty>
    


    <!-- https://saref.etsi.org/saref4bldg/sprayType -->


    <owl:DatatypeProperty rdf:about="https://saref.etsi.org/saref4bldg/sprayType">
        <rdfs:range rdf:resource="http://www.w3.org/2001/XMLSchema#string"/>
        <rdfs:comment xml:lang="en">SprayFilled: Water is sprayed into airflow. SplashTypeFill: water cascades over successive rows of splash bars. FilmTypeFill: water flows in a thin layer over closely spaced sheets.</rdfs:comment>
        <rdfs:label xml:lang="en">spray type</rdfs:label>
    </owl:DatatypeProperty>
    


    <!-- https://saref.etsi.org/saref4bldg/standard -->


    <owl:DatatypeProperty rdf:about="https://saref.etsi.org/saref4bldg/standard">
        <rdfs:range rdf:resource="http://www.w3.org/2001/XMLSchema#string"/>
        <rdfs:comment xml:lang="en">The designation of the standard applicable for the definition of the characteristics of the unit.</rdfs:comment>
        <rdfs:label xml:lang="en">standard</rdfs:label>
    </owl:DatatypeProperty>
    


    <!-- https://saref.etsi.org/saref4bldg/storageType -->


    <owl:DatatypeProperty rdf:about="https://saref.etsi.org/saref4bldg/storageType">
        <rdfs:range rdf:resource="http://www.w3.org/2001/XMLSchema#string"/>
        <rdfs:comment xml:lang="en">Defines the general material category intended to be stored.</rdfs:comment>
        <rdfs:label xml:lang="en">storage type</rdfs:label>
    </owl:DatatypeProperty>
    


    <!-- https://saref.etsi.org/saref4bldg/switchFunction -->


    <owl:DatatypeProperty rdf:about="https://saref.etsi.org/saref4bldg/switchFunction">
        <rdfs:range rdf:resource="http://www.w3.org/2001/XMLSchema#string"/>
        <rdfs:comment xml:lang="en">Indicates types of switches which differs in functionality.</rdfs:comment>
        <rdfs:label xml:lang="en">switch function</rdfs:label>
    </owl:DatatypeProperty>
    


    <!-- https://saref.etsi.org/saref4bldg/temperatureClassification -->


    <owl:DatatypeProperty rdf:about="https://saref.etsi.org/saref4bldg/temperatureClassification">
        <rdfs:range rdf:resource="http://www.w3.org/2001/XMLSchema#string"/>
        <rdfs:comment xml:lang="en">Enumeration defining the temperature classification of the space heater surface temperature. low temperature - surface temperature is relatively low, usually heated by hot water or electricity. high temperature - surface temperature is relatively high, usually heated by gas or steam.</rdfs:comment>
        <rdfs:label xml:lang="en">temperature classification</rdfs:label>
    </owl:DatatypeProperty>
    


    <!-- https://saref.etsi.org/saref4bldg/transformerVectorGroup -->


    <owl:DatatypeProperty rdf:about="https://saref.etsi.org/saref4bldg/transformerVectorGroup">
        <rdfs:range rdf:resource="http://www.w3.org/2001/XMLSchema#string"/>
        <rdfs:comment xml:lang="en">List of the possible vector groups for the transformer from which that required may be set. Values in the enumeration list follow a standard international code where the first letter describes how the primary windings are connected, the second letter describes how the secondary windings are connected, and the numbers describe the rotation of voltages and currents from the primary to the secondary side in multiples of 30 degrees. D: means that the windings are delta-connected. Y: means that the windings are star-connected. Z: means that the windings are zig-zag connected (a special start-connected providing low reactance of the transformer). The connectivity is only relevant for three-phase transformers.</rdfs:comment>
        <rdfs:label xml:lang="en">transformer vector group</rdfs:label>
    </owl:DatatypeProperty>
    


    <!-- https://saref.etsi.org/saref4bldg/valveMechanism -->


    <owl:DatatypeProperty rdf:about="https://saref.etsi.org/saref4bldg/valveMechanism">
        <rdfs:range rdf:resource="http://www.w3.org/2001/XMLSchema#string"/>
        <rdfs:comment xml:lang="en">The mechanism by which the valve function is achieved where: BALL: Valve that has a ported ball that can be turned relative to the body seat ports. BUTTERFLY: Valve in which a streamlined disc pivots about a diametric axis. CONFIGUREDGATE: Screwdown valve in which the closing gate is shaped in a configured manner to have a more precise control of pressure and flow change across the valve. GLAND: Valve with a tapered seating, in which a rotatable plug is retained by means of a gland and gland packing. GLOBE: Screwdown valve that has a spherical body. LUBRICATEDPLUG: Plug valve in which a lubricant is injected under pressure between the plug face and the body. NEEDLE: Valve for regulating the flow in or from a pipe, in which a slender cone moves along the axis of flow to close against a fixed conical seat. PARALLELSLIDE: Screwdown valve that has a machined plate that slides in formed grooves to form a seal. PLUG: Valve that has a ported plug that can be turned relative to the body seat ports. WEDGEGATE: Screwdown valve that has a wedge shaped plate fitting into tapered guides to form a seal.</rdfs:comment>
        <rdfs:label xml:lang="en">valve mechanism</rdfs:label>
    </owl:DatatypeProperty>
    


    <!-- https://saref.etsi.org/saref4bldg/valveOperation -->


    <owl:DatatypeProperty rdf:about="https://saref.etsi.org/saref4bldg/valveOperation">
        <rdfs:range rdf:resource="http://www.w3.org/2001/XMLSchema#string"/>
        <rdfs:comment xml:lang="en">The method of valve operation where: DROPWEIGHT: A valve that is closed by the action of a weighted lever being released, the weight normally being prevented from dropping by being held by a wire, the closure normally being made by the action of heat on a fusible link in the wire FLOAT: A valve that is opened and closed by the action of a float that rises and falls with water level. The float may be a ball attached to a lever or other mechanism HYDRAULIC: A valve that is opened and closed by hydraulic actuation LEVER: A valve that is opened and closed by the action of a lever rotating the gate within the valve. LOCKSHIELD: A valve that requires the use of a special lockshield key for opening and closing, the operating mechanism being protected by a shroud during normal operation. MOTORIZED: A valve that is opened and closed by the action of an electric motor on an actuator PNEUMATIC: A valve that is opened and closed by pneumatic actuation SOLENOID: A valve that is normally held open by a magnetic field in a coil acting on the gate but that is closed immediately if the electrical current generating the magnetic field is removed. SPRING: A valve that is normally held in position by the pressure of a spring on a plate but that may be caused to open if the pressure of the fluid is sufficient to overcome the spring pressure. THERMOSTATIC: A valve in which the ports are opened or closed to maintain a required predetermined temperature. WHEEL: A valve that is opened and closed by the action of a wheel moving the gate within the valve.</rdfs:comment>
        <rdfs:label xml:lang="en">valve operation</rdfs:label>
    </owl:DatatypeProperty>
    


    <!-- https://saref.etsi.org/saref4bldg/valvePattern -->


    <owl:DatatypeProperty rdf:about="https://saref.etsi.org/saref4bldg/valvePattern">
        <rdfs:range rdf:resource="http://www.w3.org/2001/XMLSchema#string"/>
        <rdfs:comment xml:lang="en">The configuration of the ports of a valve according to either the linear route taken by a fluid flowing through the valve or by the number of ports where: SINGLEPORT: Valve that has a single entry port from the system that it serves, the exit port being to the surrounding environment. ANGLED_2_PORT: Valve in which the direction of flow is changed through 90 degrees. STRAIGHT_2_PORT: Valve in which the flow is straight through. STRAIGHT_3_PORT: Valve with three separate ports. CROSSOVER_4_PORT: Valve with 4 separate ports.</rdfs:comment>
        <rdfs:label xml:lang="en">valve pattern</rdfs:label>
    </owl:DatatypeProperty>
    


    <!-- https://saref.etsi.org/saref4bldg/waterFlowControlSystemType -->


    <owl:DatatypeProperty rdf:about="https://saref.etsi.org/saref4bldg/waterFlowControlSystemType">
        <rdfs:range rdf:resource="http://www.w3.org/2001/XMLSchema#string"/>
        <rdfs:comment xml:lang="en">Factory fitted waterflow control system.</rdfs:comment>
        <rdfs:label xml:lang="en">water flow control system type</rdfs:label>
    </owl:DatatypeProperty>
    


    <!-- https://saref.etsi.org/saref4city/hasCreationDate -->


    <owl:DatatypeProperty rdf:about="https://saref.etsi.org/saref4city/hasCreationDate">
        <rdfs:range rdf:resource="http://www.w3.org/2001/XMLSchema#dateTime"/>
        <rdfs:isDefinedBy rdf:resource="https://saref.etsi.org/saref4city/"/>
        <rdfs:label xml:lang="en">has creation date</rdfs:label>
    </owl:DatatypeProperty>
    


    <!-- https://saref.etsi.org/saref4city/hasExpirationDate -->


    <owl:DatatypeProperty rdf:about="https://saref.etsi.org/saref4city/hasExpirationDate">
        <rdfs:range rdf:resource="http://www.w3.org/2001/XMLSchema#dateTime"/>
        <rdfs:isDefinedBy rdf:resource="https://saref.etsi.org/saref4city/"/>
        <rdfs:label xml:lang="en">has expiration date</rdfs:label>
    </owl:DatatypeProperty>
    


    <!-- https://saref.etsi.org/saref4city/hasLastUpdateDate -->


    <owl:DatatypeProperty rdf:about="https://saref.etsi.org/saref4city/hasLastUpdateDate">
        <rdfs:range rdf:resource="http://www.w3.org/2001/XMLSchema#dateTime"/>
        <rdfs:isDefinedBy rdf:resource="https://saref.etsi.org/saref4city/"/>
        <rdfs:label xml:lang="en">has last update date</rdfs:label>
    </owl:DatatypeProperty>
    


    <!-- https://saref.etsi.org/saref4watr/forDayInMonth -->


    <owl:DatatypeProperty rdf:about="https://saref.etsi.org/saref4watr/forDayInMonth">
        <rdfs:domain rdf:resource="https://saref.etsi.org/saref4watr/TimeBasedTariff"/>
        <rdfs:range rdf:resource="http://www.w3.org/2001/XMLSchema#gDay"/>
        <rdfs:comment xml:lang="en">The day of the month for which a tariff is applied (e.g., each 15).</rdfs:comment>
        <rdfs:label xml:lang="en">for day in month</rdfs:label>
    </owl:DatatypeProperty>
    


    <!-- https://saref.etsi.org/saref4watr/forFinancialConsumption -->


    <owl:DatatypeProperty rdf:about="https://saref.etsi.org/saref4watr/forFinancialConsumption">
        <rdfs:domain rdf:resource="https://saref.etsi.org/saref4watr/ConsumptionBasedTariff"/>
        <rdfs:comment xml:lang="en">The financial consumption related to a tariff (e.g., prepaid tariffs).</rdfs:comment>
        <rdfs:label xml:lang="en">for financial consumption</rdfs:label>
    </owl:DatatypeProperty>
    


    <!-- https://saref.etsi.org/saref4watr/forVolumeConsumption -->


    <owl:DatatypeProperty rdf:about="https://saref.etsi.org/saref4watr/forVolumeConsumption">
        <rdfs:domain rdf:resource="https://saref.etsi.org/saref4watr/ConsumptionBasedTariff"/>
        <rdfs:comment xml:lang="en">The volume consumption related to a tariff (e.g., after consumption of 900 litres).</rdfs:comment>
        <rdfs:label xml:lang="en">for volume consumption</rdfs:label>
    </owl:DatatypeProperty>
    


    <!-- https://saref.etsi.org/saref4watr/forVolumeFlow -->


    <owl:DatatypeProperty rdf:about="https://saref.etsi.org/saref4watr/forVolumeFlow">
        <rdfs:domain rdf:resource="https://saref.etsi.org/saref4watr/ThresholdBasedTariff"/>
        <rdfs:comment xml:lang="en">The volume flow related to a tariff.</rdfs:comment>
        <rdfs:label xml:lang="en">for volume flow</rdfs:label>
    </owl:DatatypeProperty>
    


    <!-- https://saref.etsi.org/saref4watr/hasBillingDate -->


    <owl:DatatypeProperty rdf:about="https://saref.etsi.org/saref4watr/hasBillingDate">
        <rdfs:domain rdf:resource="https://saref.etsi.org/saref4watr/Tariff"/>
        <rdfs:range rdf:resource="http://www.w3.org/2001/XMLSchema#dateTime"/>
        <rdfs:comment xml:lang="en">The billing date of a tariff.</rdfs:comment>
        <rdfs:label xml:lang="en">has billing date</rdfs:label>
    </owl:DatatypeProperty>
    


    <!-- https://saref.etsi.org/saref4watr/hasFabricationNumber -->


    <owl:DatatypeProperty rdf:about="https://saref.etsi.org/saref4watr/hasFabricationNumber">
        <rdfs:range rdf:resource="http://www.w3.org/2000/01/rdf-schema#Literal"/>
        <rdfs:comment xml:lang="en">The fabrication number of a device.</rdfs:comment>
        <rdfs:label xml:lang="en">has fabrication number</rdfs:label>
    </owl:DatatypeProperty>
    


    <!-- https://saref.etsi.org/saref4watr/hasFirmwareVersion -->


    <owl:DatatypeProperty rdf:about="https://saref.etsi.org/saref4watr/hasFirmwareVersion">
        <rdfs:range rdf:resource="http://www.w3.org/2000/01/rdf-schema#Literal"/>
        <rdfs:comment xml:lang="en">The firmware version of a device.</rdfs:comment>
        <rdfs:label xml:lang="en">has firmware version</rdfs:label>
    </owl:DatatypeProperty>
    


    <!-- https://saref.etsi.org/saref4watr/hasHardwareVersion -->


    <owl:DatatypeProperty rdf:about="https://saref.etsi.org/saref4watr/hasHardwareVersion">
        <rdfs:range rdf:resource="http://www.w3.org/2000/01/rdf-schema#Literal"/>
        <rdfs:comment xml:lang="en">The hardware version of a device.</rdfs:comment>
        <rdfs:label xml:lang="en">has hardware version</rdfs:label>
    </owl:DatatypeProperty>
    


    <!-- https://saref.etsi.org/saref4watr/hasStartTimestamp -->


    <owl:DatatypeProperty rdf:about="https://saref.etsi.org/saref4watr/hasStartTimestamp">
        <rdfs:domain rdf:resource="https://saref.etsi.org/saref4watr/Tariff"/>
        <rdfs:range rdf:resource="http://www.w3.org/2001/XMLSchema#dateTime"/>
        <rdfs:comment xml:lang="en">The start date and time of a tariff.</rdfs:comment>
        <rdfs:label xml:lang="en">has start timestamp</rdfs:label>
    </owl:DatatypeProperty>
    


    <!-- https://saref.etsi.org/saref4watr/hasVersion -->


    <owl:DatatypeProperty rdf:about="https://saref.etsi.org/saref4watr/hasVersion">
        <rdfs:range rdf:resource="http://www.w3.org/2000/01/rdf-schema#Literal"/>
        <rdfs:comment xml:lang="en">The version of a device.</rdfs:comment>
        <rdfs:label xml:lang="en">has version</rdfs:label>
    </owl:DatatypeProperty>
    


    <!-- https://saref.etsi.org/saref4watr/operatesAtRadioFrequency -->


    <owl:DatatypeProperty rdf:about="https://saref.etsi.org/saref4watr/operatesAtRadioFrequency">
        <rdfs:comment xml:lang="en">The radio frequency at which a device operates.</rdfs:comment>
        <rdfs:label xml:lang="en">operates at radio frequency</rdfs:label>
    </owl:DatatypeProperty>
    


    <!-- https://saref.etsi.org/saref4watr/requiresPower -->


    <owl:DatatypeProperty rdf:about="https://saref.etsi.org/saref4watr/requiresPower">
        <rdfs:comment xml:lang="en">The power required by a device.</rdfs:comment>
        <rdfs:label xml:lang="en">requires power</rdfs:label>
    </owl:DatatypeProperty>
    


    <!-- https://www.geonames.org/ontology#name -->


    <owl:DatatypeProperty rdf:about="https://www.geonames.org/ontology#name"/>
    


    <!-- https://www.geonames.org/ontology#postalCode -->


    <owl:DatatypeProperty rdf:about="https://www.geonames.org/ontology#postalCode"/>
    


    <!-- 
    ///////////////////////////////////////////////////////////////////////////////////////
    //
    // Classes
    //
    ///////////////////////////////////////////////////////////////////////////////////////
     -->


    


    <!-- http://bigg-project.eu/ontology#Area -->


    <owl:Class rdf:about="http://bigg-project.eu/ontology#Area">
        <rdfs:subClassOf rdf:resource="https://saref.etsi.org/core/Property"/>
        <rdfs:comment xml:lang="en">A saref:Property related to some measurements that are characterized by a certain value measured in an energy unit (such as Kilowatt_Hour or Watt_hour). Furter specializations of the saref:Energy class can be found in the SAREF4ENER extension, where classes such as EnergyMax, EnergyMin and EnergyExpected are defined. </rdfs:comment>
    </owl:Class>
    


    <!-- http://bigg-project.eu/ontology#EnergyAsset -->


    <owl:Class rdf:about="http://bigg-project.eu/ontology#EnergyAsset">
        <rdfs:subClassOf rdf:resource="http://www.opengis.net/ont/geosparql#Feature"/>
        <rdfs:subClassOf rdf:resource="https://saref.etsi.org/core/FeatureOfInterest"/>
        <rdfs:subClassOf rdf:resource="https://saref.etsi.org/saref4syst/System"/>
        <rdfs:comment xml:lang="en">A energy asset is a physical entity used in the process of transporting, treating, storing and distributing energy.</rdfs:comment>
        <rdfs:label xml:lang="en">Energy asset</rdfs:label>
    </owl:Class>
    


    <!-- http://bigg-project.eu/ontology#EnergyDevice -->


    <owl:Class rdf:about="http://bigg-project.eu/ontology#EnergyDevice">
        <rdfs:subClassOf rdf:resource="http://bigg-project.eu/ontology#EnergyAsset"/>
        <rdfs:subClassOf rdf:resource="https://saref.etsi.org/core/Device"/>
        <rdfs:comment xml:lang="en">An energy device is a device that is also an energy asset.</rdfs:comment>
        <rdfs:label xml:lang="en">Energy device</rdfs:label>
    </owl:Class>
    


    <!-- http://bigg-project.eu/ontology#EnergyMeter -->


    <owl:Class rdf:about="http://bigg-project.eu/ontology#EnergyMeter">
        <rdfs:subClassOf rdf:resource="http://bigg-project.eu/ontology#EnergyDevice"/>
        <rdfs:subClassOf rdf:resource="https://saref.etsi.org/core/Meter"/>
        <rdfs:subClassOf>
            <owl:Restriction>
                <owl:onProperty rdf:resource="https://saref.etsi.org/core/measuresProperty"/>
                <owl:someValuesFrom rdf:resource="https://saref.etsi.org/core/Energy"/>
            </owl:Restriction>
        </rdfs:subClassOf>
        <rdfs:subClassOf>
            <owl:Restriction>
                <owl:onProperty rdf:resource="https://saref.etsi.org/core/hasProperty"/>
                <owl:allValuesFrom rdf:resource="https://saref.etsi.org/saref4watr/WaterMeterProperty"/>
            </owl:Restriction>
        </rdfs:subClassOf>
        <rdfs:subClassOf>
            <owl:Restriction>
                <owl:onProperty rdf:resource="https://saref.etsi.org/saref4watr/hasFabricationNumber"/>
                <owl:maxCardinality rdf:datatype="http://www.w3.org/2001/XMLSchema#nonNegativeInteger">1</owl:maxCardinality>
            </owl:Restriction>
        </rdfs:subClassOf>
        <rdfs:subClassOf>
            <owl:Restriction>
                <owl:onProperty rdf:resource="https://saref.etsi.org/saref4watr/hasFirmwareVersion"/>
                <owl:maxCardinality rdf:datatype="http://www.w3.org/2001/XMLSchema#nonNegativeInteger">1</owl:maxCardinality>
            </owl:Restriction>
        </rdfs:subClassOf>
        <rdfs:subClassOf>
            <owl:Restriction>
                <owl:onProperty rdf:resource="https://saref.etsi.org/saref4watr/hasHardwareVersion"/>
                <owl:maxCardinality rdf:datatype="http://www.w3.org/2001/XMLSchema#nonNegativeInteger">1</owl:maxCardinality>
            </owl:Restriction>
        </rdfs:subClassOf>
        <rdfs:subClassOf>
            <owl:Restriction>
                <owl:onProperty rdf:resource="https://saref.etsi.org/saref4watr/hasVersion"/>
                <owl:maxCardinality rdf:datatype="http://www.w3.org/2001/XMLSchema#nonNegativeInteger">1</owl:maxCardinality>
            </owl:Restriction>
        </rdfs:subClassOf>
        <rdfs:comment xml:lang="en">A energy meter is an instrument intended to measure continuously, memorize, and display the amouint of energy passing through the meter.</rdfs:comment>
        <rdfs:label xml:lang="en">Energy meter</rdfs:label>
    </owl:Class>
    


    <!-- http://bigg-project.eu/ontology#Patrimony -->


    <owl:Class rdf:about="http://bigg-project.eu/ontology#Patrimony">
        <rdfs:subClassOf rdf:resource="http://www.opengis.net/ont/geosparql#Feature"/>
        <rdfs:subClassOf>
            <owl:Restriction>
                <owl:onProperty rdf:resource="https://saref.etsi.org/saref4agri/contains"/>
                <owl:someValuesFrom rdf:resource="https://saref.etsi.org/saref4agri/Building"/>
            </owl:Restriction>
        </rdfs:subClassOf>
        <rdfs:subClassOf>
            <owl:Restriction>
                <owl:onProperty rdf:resource="https://saref.etsi.org/saref4agri/contains"/>
                <owl:someValuesFrom rdf:resource="https://saref.etsi.org/saref4agri/Parcel"/>
            </owl:Restriction>
        </rdfs:subClassOf>
        <rdfs:subClassOf>
            <owl:Restriction>
                <owl:onProperty rdf:resource="https://saref.etsi.org/saref4agri/hasName"/>
                <owl:maxCardinality rdf:datatype="http://www.w3.org/2001/XMLSchema#nonNegativeInteger">1</owl:maxCardinality>
            </owl:Restriction>
        </rdfs:subClassOf>
        <rdfs:comment xml:lang="en">A set of real properties which can contain buildings and parcels.</rdfs:comment>
    </owl:Class>
    


    <!-- http://purl.obolibrary.org/obo/TAXRANK_0000000 -->


    <owl:Class rdf:about="http://purl.obolibrary.org/obo/TAXRANK_0000000">
        <rdfs:label xml:lang="en">Taxon rank</rdfs:label>
    </owl:Class>
    


    <!-- http://www.opengis.net/ont/geosparql#Feature -->


    <owl:Class rdf:about="http://www.opengis.net/ont/geosparql#Feature">
        <rdfs:subClassOf rdf:resource="http://www.opengis.net/ont/geosparql#SpatialObject"/>
        <rdfs:subClassOf>
            <owl:Restriction>
                <owl:onProperty rdf:resource="http://www.opengis.net/ont/geosparql#hasGeometry"/>
                <owl:allValuesFrom rdf:resource="http://www.opengis.net/ont/geosparql#Geometry"/>
            </owl:Restriction>
        </rdfs:subClassOf>
        <owl:disjointWith rdf:resource="http://www.opengis.net/ont/geosparql#Geometry"/>
        <rdfs:comment xml:lang="en">This class represents the top-level feature type. This class is equivalent to GFI_Feature defined in ISO 19156:2011, and it is superclass of all feature types.</rdfs:comment>
        <rdfs:isDefinedBy rdf:resource="http://www.opengis.net/ont/geosparql"/>
        <rdfs:isDefinedBy rdf:resource="http://www.opengis.net/ont/gml"/>
        <rdfs:isDefinedBy rdf:resource="http://www.opengis.net/ont/geosparql#"/>
        <rdfs:isDefinedBy rdf:resource="http://www.opengis.net/spec/geosparql/1.0/req/core/feature-class"/>
        <rdfs:isDefinedBy rdf:resource="http://www.opengis.net/spec/geosparql/1.1/req/core/feature-class"/>
        <rdfs:label xml:lang="en">Feature</rdfs:label>
        <skos:definition xml:lang="en">A discrete spatial phenomenon in a universe of discourse.</skos:definition>
        <skos:example rdf:resource="http://www.opengis.net/spec/geosparql/1.1/specification.html#B.1.1.2.1"/>
        <skos:example rdf:resource="http://www.opengis.net/spec/geosparql/1.1/specification.html#B.1.1.2.2"/>
        <skos:example rdf:resource="http://www.opengis.net/spec/geosparql/1.1/specification.html#B.1.1.2.3"/>
        <skos:example rdf:resource="http://www.opengis.net/spec/geosparql/1.1/specification.html#B.1.1.2.4"/>
        <skos:example rdf:resource="http://www.opengis.net/spec/geosparql/1.1/specification.html#B.1.1.2.5"/>
        <skos:example rdf:resource="http://www.opengis.net/spec/geosparql/1.1/specification.html#B.1.1.2.6"/>
        <skos:example rdf:resource="http://www.opengis.net/spec/geosparql/1.1/specification.html#B.1.1.2.7"/>
        <skos:example rdf:resource="http://www.opengis.net/spec/geosparql/1.1/specification.html#B.1.1.2.8"/>
        <skos:example rdf:resource="http://www.opengis.net/spec/geosparql/1.1/specification.html#B.1.1.2.9"/>
        <skos:example rdf:resource="http://www.opengis.net/spec/geosparql/1.1/specification.html#B.1.1.3.2"/>
        <skos:example rdf:resource="http://www.opengis.net/spec/geosparql/1.1/specification.html#B.1.1.3.3"/>
        <skos:example rdf:resource="http://www.opengis.net/spec/geosparql/1.1/specification.html#B.1.2.2"/>
        <skos:example rdf:resource="http://www.opengis.net/spec/geosparql/1.1/specification.html#B.1.2.3"/>
        <skos:example rdf:resource="http://www.opengis.net/spec/geosparql/1.1/specification.html#B.1.2.4"/>
        <skos:note xml:lang="en">A Feature represents a uniquely identifiable phenomenon, for example a river or an apple. While such phenomena (and therefore the Features used to represent them) are bounded, their boundaries may be crisp (e.g., the declared boundaries of a state), vague (e.g., the delineation of a valley versus its neighboring mountains), and change with time (e.g., a storm front). While discrete in nature, Features may be created from continuous observations, such as an isochrone that determines the region that can be reached by ambulance within 5 minutes.</skos:note>
        <skos:prefLabel xml:lang="en">Feature</skos:prefLabel>
    </owl:Class>
    


    <!-- http://www.opengis.net/ont/geosparql#FeatureCollection -->


    <owl:Class rdf:about="http://www.opengis.net/ont/geosparql#FeatureCollection">
        <rdfs:subClassOf rdf:resource="http://www.opengis.net/ont/geosparql#SpatialObjectCollection"/>
        <rdfs:subClassOf>
            <owl:Restriction>
                <owl:onProperty rdf:resource="http://www.w3.org/2000/01/rdf-schema#member"/>
                <owl:allValuesFrom rdf:resource="http://www.opengis.net/ont/geosparql#Feature"/>
            </owl:Restriction>
        </rdfs:subClassOf>
        <rdfs:isDefinedBy rdf:resource="http://www.opengis.net/ont/geosparql#"/>
        <rdfs:isDefinedBy rdf:resource="http://www.opengis.net/spec/geosparql/1.1/req/core/feature-collection-class"/>
        <skos:definition xml:lang="en">Any collection of individual Features.</skos:definition>
        <skos:example rdf:resource="http://www.opengis.net/spec/geosparql/1.1/specification.html#B.1.1.6"/>
        <skos:prefLabel xml:lang="en">Feature Collection</skos:prefLabel>
    </owl:Class>
    


    <!-- http://www.opengis.net/ont/geosparql#Geometry -->


    <owl:Class rdf:about="http://www.opengis.net/ont/geosparql#Geometry">
        <rdfs:subClassOf rdf:resource="http://www.opengis.net/ont/geosparql#SpatialObject"/>
        <rdfs:comment xml:lang="en">The class represents the top-level geometry type. This class is equivalent to the UML class GM_Object defined in ISO 19107, and it is superclass of all geometry types.</rdfs:comment>
        <rdfs:isDefinedBy rdf:resource="http://www.opengis.net/ont/geosparql"/>
        <rdfs:isDefinedBy rdf:resource="http://www.opengis.net/ont/geosparql#"/>
        <rdfs:isDefinedBy rdf:resource="http://www.opengis.net/spec/geosparql/1.0/req/geometry-extension/geometry-class"/>
        <rdfs:isDefinedBy rdf:resource="http://www.opengis.net/spec/geosparql/1.1/req/geometry-extension/geometry-class"/>
        <rdfs:label xml:lang="en">Geometry</rdfs:label>
        <skos:definition xml:lang="en">A coherent set of direct positions in Euclidian space. A direct position holds the coordinates for a position within a Coordinate Reference System (CRS).</skos:definition>
        <skos:example rdf:resource="http://www.opengis.net/spec/geosparql/1.1/specification.html#B.1.1.2.2"/>
        <skos:example rdf:resource="http://www.opengis.net/spec/geosparql/1.1/specification.html#B.1.1.2.3"/>
        <skos:example rdf:resource="http://www.opengis.net/spec/geosparql/1.1/specification.html#B.1.1.2.4"/>
        <skos:example rdf:resource="http://www.opengis.net/spec/geosparql/1.1/specification.html#B.1.1.2.5"/>
        <skos:example rdf:resource="http://www.opengis.net/spec/geosparql/1.1/specification.html#B.1.1.2.6"/>
        <skos:example rdf:resource="http://www.opengis.net/spec/geosparql/1.1/specification.html#B.1.1.2.8"/>
        <skos:example rdf:resource="http://www.opengis.net/spec/geosparql/1.1/specification.html#B.1.1.3.1"/>
        <skos:example rdf:resource="http://www.opengis.net/spec/geosparql/1.1/specification.html#B.1.1.3.2"/>
        <skos:example rdf:resource="http://www.opengis.net/spec/geosparql/1.1/specification.html#B.1.1.3.3"/>
        <skos:example rdf:resource="http://www.opengis.net/spec/geosparql/1.1/specification.html#B.1.2.2"/>
        <skos:example rdf:resource="http://www.opengis.net/spec/geosparql/1.1/specification.html#B.1.2.3"/>
        <skos:example rdf:resource="http://www.opengis.net/spec/geosparql/1.1/specification.html#B.1.2.4"/>
        <skos:note xml:lang="en">Geometry can be used as a representation of the shape, extent or location of a Feature, or can exist as a self-contained entity.</skos:note>
        <skos:prefLabel xml:lang="en">Geometry</skos:prefLabel>
    </owl:Class>
    


    <!-- http://www.opengis.net/ont/geosparql#GeometryCollection -->


    <owl:Class rdf:about="http://www.opengis.net/ont/geosparql#GeometryCollection">
        <rdfs:subClassOf rdf:resource="http://www.opengis.net/ont/geosparql#SpatialObjectCollection"/>
        <rdfs:subClassOf>
            <owl:Restriction>
                <owl:onProperty rdf:resource="http://www.w3.org/2000/01/rdf-schema#member"/>
                <owl:allValuesFrom rdf:resource="http://www.opengis.net/ont/geosparql#Geometry"/>
            </owl:Restriction>
        </rdfs:subClassOf>
        <rdfs:isDefinedBy rdf:resource="http://www.opengis.net/ont/geosparql#"/>
        <rdfs:isDefinedBy rdf:resource="http://www.opengis.net/spec/geosparql/1.1/req/core/geometry-collection-class"/>
        <skos:definition xml:lang="en">Any collection of individual Geometries.</skos:definition>
        <skos:example rdf:resource="http://www.opengis.net/spec/geosparql/1.1/specification.html#B.1.1.7"/>
        <skos:prefLabel xml:lang="en">Geometry Collection</skos:prefLabel>
    </owl:Class>
    


    <!-- http://www.opengis.net/ont/geosparql#SpatialObject -->


    <owl:Class rdf:about="http://www.opengis.net/ont/geosparql#SpatialObject">
        <rdfs:subClassOf>
            <owl:Restriction>
                <owl:onProperty rdf:resource="http://www.opengis.net/ont/geosparql#hasGeometry"/>
                <owl:allValuesFrom rdf:resource="http://www.opengis.net/ont/geosparql#Geometry"/>
            </owl:Restriction>
        </rdfs:subClassOf>
        <rdfs:subClassOf>
            <owl:Restriction>
                <owl:onProperty rdf:resource="http://www.opengis.net/ont/geosparql#sfContains"/>
                <owl:allValuesFrom rdf:resource="http://www.opengis.net/ont/geosparql#SpatialObject"/>
            </owl:Restriction>
        </rdfs:subClassOf>
        <rdfs:subClassOf>
            <owl:Restriction>
                <owl:onProperty rdf:resource="http://www.opengis.net/ont/geosparql#sfWithin"/>
                <owl:allValuesFrom rdf:resource="http://www.opengis.net/ont/geosparql#SpatialObject"/>
            </owl:Restriction>
        </rdfs:subClassOf>
        <rdfs:subClassOf>
            <owl:Restriction>
                <owl:onProperty rdf:resource="http://www.w3.org/2003/01/geo/wgs84_pos#location"/>
                <owl:allValuesFrom rdf:resource="http://www.w3.org/2003/01/geo/wgs84_pos#Point"/>
            </owl:Restriction>
        </rdfs:subClassOf>
        <rdfs:comment xml:lang="en">The class spatial-object represents everything that can have a spatial representation. It is superclass of feature and geometry.</rdfs:comment>
        <rdfs:isDefinedBy rdf:resource="http://www.opengis.net/ont/geosparql"/>
        <rdfs:isDefinedBy rdf:resource="http://www.opengis.net/ont/geosparql#"/>
        <rdfs:isDefinedBy rdf:resource="http://www.opengis.net/spec/geosparql/1.0/req/core/spatial-object-class"/>
        <rdfs:isDefinedBy rdf:resource="http://www.opengis.net/spec/geosparql/1.1/req/core/spatial-object-class"/>
        <rdfs:label xml:lang="en">Spatial object</rdfs:label>
        <rdfs:label xml:lang="en">SpatialObject</rdfs:label>
        <skos:definition xml:lang="en">Anything spatial (having or being a shape, position or an extent).</skos:definition>
        <skos:example rdf:resource="http://www.opengis.net/spec/geosparql/1.1/specification.html#B.1.1.1.1"/>
        <skos:example rdf:resource="http://www.opengis.net/spec/geosparql/1.1/specification.html#B.1.1.1.2"/>
        <skos:note xml:lang="en">Subclasses are expected to be used for instance data.</skos:note>
        <skos:prefLabel xml:lang="en">Spatial Object</skos:prefLabel>
    </owl:Class>
    


    <!-- http://www.opengis.net/ont/geosparql#SpatialObjectCollection -->


    <owl:Class rdf:about="http://www.opengis.net/ont/geosparql#SpatialObjectCollection">
        <rdfs:subClassOf rdf:resource="http://www.w3.org/2000/01/rdf-schema#Container"/>
        <rdfs:subClassOf>
            <owl:Restriction>
                <owl:onProperty rdf:resource="http://www.w3.org/2000/01/rdf-schema#member"/>
                <owl:allValuesFrom rdf:resource="http://www.opengis.net/ont/geosparql#SpatialObject"/>
            </owl:Restriction>
        </rdfs:subClassOf>
        <rdfs:isDefinedBy rdf:resource="http://www.opengis.net/ont/geosparql#"/>
        <rdfs:isDefinedBy rdf:resource="http://www.opengis.net/spec/geosparql/1.1/req/core/spatial-object-collection-class"/>
        <skos:definition xml:lang="en">Any collection of individual Spatial Objects. It is superclass of Feature Collection and Geometry Collection.</skos:definition>
        <skos:prefLabel xml:lang="en">Spatial Object Collection</skos:prefLabel>
    </owl:Class>
    


    <!-- http://www.opengis.net/ont/sf#Point -->


    <owl:Class rdf:about="http://www.opengis.net/ont/sf#Point">
        <rdfs:subClassOf rdf:resource="http://www.opengis.net/ont/geosparql#Geometry"/>
        <rdfs:isDefinedBy rdf:resource="http://www.opengis.net/ont/sf#"/>
        <rdfs:label xml:lang="en">Point</rdfs:label>
    </owl:Class>
    


    <!-- http://www.opengis.net/ont/sf#Polygon -->


    <owl:Class rdf:about="http://www.opengis.net/ont/sf#Polygon">
        <rdfs:subClassOf rdf:resource="http://www.opengis.net/ont/geosparql#Geometry"/>
        <rdfs:isDefinedBy rdf:resource="http://www.opengis.net/ont/sf#"/>
        <rdfs:label xml:lang="en">Polygon</rdfs:label>
    </owl:Class>
    


    <!-- http://www.w3.org/2000/01/rdf-schema#Container -->


    <owl:Class rdf:about="http://www.w3.org/2000/01/rdf-schema#Container"/>
    


    <!-- http://www.w3.org/2003/01/geo/wgs84_pos#Point -->


    <owl:Class rdf:about="http://www.w3.org/2003/01/geo/wgs84_pos#Point">
        <rdfs:subClassOf rdf:resource="http://www.opengis.net/ont/geosparql#Geometry"/>
        <rdfs:subClassOf rdf:resource="http://www.w3.org/2003/01/geo/wgs84_pos#SpatialThing"/>
        <rdfs:comment xml:lang="en">A point, typically described using a coordinate system relative to Earth, such as WGS84.</rdfs:comment>
        <rdfs:comment> 
Uniquely identified by lat/long/alt. i.e.

spaciallyIntersects(P1, P2) :- lat(P1, LAT), long(P1, LONG), alt(P1, ALT),
  lat(P2, LAT), long(P2, LONG), alt(P2, ALT).

sameThing(P1, P2) :- type(P1, Point), type(P2, Point), spaciallyIntersects(P1, P2).
  </rdfs:comment>
        <rdfs:comment>A point, typically described using a coordinate system relative to Earth, such as WGS84.
  </rdfs:comment>
        <rdfs:isDefinedBy rdf:resource="http://www.w3.org/2003/01/geo/wgs84_pos#"/>
        <rdfs:label xml:lang="en">Point</rdfs:label>
        <rdfs:label>point</rdfs:label>
    </owl:Class>
    


    <!-- http://www.w3.org/2003/01/geo/wgs84_pos#SpatialThing -->


    <owl:Class rdf:about="http://www.w3.org/2003/01/geo/wgs84_pos#SpatialThing">
        <rdfs:comment>Anything with spatial extent, i.e. size, shape, or position.
 e.g. people, places, bowling balls, as well as abstract areas like cubes.
</rdfs:comment>
        <rdfs:label>SpatialThing</rdfs:label>
    </owl:Class>
    


    <!-- http://www.w3.org/2006/time#DateTimeDescription -->


    <owl:Class rdf:about="http://www.w3.org/2006/time#DateTimeDescription">
        <rdfs:subClassOf rdf:resource="http://www.w3.org/2006/time#GeneralDateTimeDescription"/>
        <rdfs:subClassOf>
            <owl:Restriction>
                <owl:onProperty rdf:resource="http://www.w3.org/2006/time#hasTRS"/>
                <owl:hasValue rdf:resource="http://www.opengis.net/def/uom/ISO-8601/0/Gregorian"/>
            </owl:Restriction>
        </rdfs:subClassOf>
        <rdfs:subClassOf>
            <owl:Restriction>
                <owl:onProperty rdf:resource="http://www.w3.org/2006/time#day"/>
                <owl:allValuesFrom rdf:resource="http://www.w3.org/2001/XMLSchema#gDay"/>
            </owl:Restriction>
        </rdfs:subClassOf>
        <rdfs:subClassOf>
            <owl:Restriction>
                <owl:onProperty rdf:resource="http://www.w3.org/2006/time#month"/>
                <owl:allValuesFrom rdf:resource="http://www.w3.org/2001/XMLSchema#gMonth"/>
            </owl:Restriction>
        </rdfs:subClassOf>
        <rdfs:subClassOf>
            <owl:Restriction>
                <owl:onProperty rdf:resource="http://www.w3.org/2006/time#year"/>
                <owl:allValuesFrom rdf:resource="http://www.w3.org/2001/XMLSchema#gYear"/>
            </owl:Restriction>
        </rdfs:subClassOf>
        <rdfs:comment xml:lang="es">Descripción de fecha y tiempo estructurada con valores separados para los diferentes elementos de un sistema calendario-reloj. El sistema de referencia temporal está fijado al calendario gregoriano, y el rango de las propiedades año, mes, día restringidas a los correspondientes tipos del XML Schema xsd:gYear, xsd:gMonth y xsd:gDay respectivamente.</rdfs:comment>
        <rdfs:comment xml:lang="en">Description of date and time structured with separate values for the various elements of a calendar-clock system. The temporal reference system is fixed to Gregorian Calendar, and the range of year, month, day properties restricted to corresponding XML Schema types xsd:gYear, xsd:gMonth and xsd:gDay, respectively.</rdfs:comment>
        <rdfs:label xml:lang="en">Date-Time description</rdfs:label>
        <rdfs:label xml:lang="es">descripción de fecha-tiempo</rdfs:label>
        <skos:definition xml:lang="es">Descripción de fecha y tiempo estructurada con valores separados para los diferentes elementos de un sistema calendario-reloj. El sistema de referencia temporal está fijado al calendario gregoriano, y el rango de las propiedades año, mes, día restringidas a los correspondientes tipos del XML Schema xsd:gYear, xsd:gMonth y xsd:gDay respectivamente.</skos:definition>
        <skos:definition xml:lang="en">Description of date and time structured with separate values for the various elements of a calendar-clock system. The temporal reference system is fixed to Gregorian Calendar, and the range of year, month, day properties restricted to corresponding XML Schema types xsd:gYear, xsd:gMonth and xsd:gDay, respectively.</skos:definition>
    </owl:Class>
    


    <!-- http://www.w3.org/2006/time#DateTimeInterval -->


    <owl:Class rdf:about="http://www.w3.org/2006/time#DateTimeInterval">
        <rdfs:subClassOf rdf:resource="http://www.w3.org/2006/time#ProperInterval"/>
        <rdfs:comment xml:lang="es">&apos;intervalo de fecha-hora&apos; es una subclase de &apos;intervalo propio&apos;, definida utilizando el multi-elemento &apos;descripción de fecha-hora&apos;.</rdfs:comment>
        <rdfs:comment xml:lang="en">DateTimeInterval is a subclass of ProperInterval, defined using the multi-element DateTimeDescription.</rdfs:comment>
        <rdfs:label xml:lang="en">Date-time interval</rdfs:label>
        <rdfs:label xml:lang="es">intervalo de fecha-hora</rdfs:label>
        <skos:definition xml:lang="es">&apos;intervalo de fecha-hora&apos; es una subclase de &apos;intervalo propio&apos;, definida utilizando el multi-elemento &apos;descripción de fecha-hora&apos;.</skos:definition>
        <skos:definition xml:lang="en">DateTimeInterval is a subclass of ProperInterval, defined using the multi-element DateTimeDescription.</skos:definition>
        <skos:note xml:lang="es">&apos;intervalo de fecha-hora&apos; se puede utilizar sólo para un intervalo cuyos límites coinciden con un elemento de fecha-hora alineados con el calendario y la zona horaria indicados. Por ejemplo, aunque ambos tienen una duración de un día, el intervalo de 24 horas que empieza en la media noche del comienzo del 8 mayo en Europa Central se puede expresar como un &apos;intervalo de fecha-hora&apos;, el intervalo de 24 horas que empieza a las 1:30pm no.</skos:note>
        <skos:note xml:lang="en">:DateTimeInterval can only be used for an interval whose limits coincide with a date-time element aligned to the calendar and timezone indicated. For example, while both have a duration of one day, the 24-hour interval beginning at midnight at the beginning of 8 May in Central Europe can be expressed as a :DateTimeInterval, but the 24-hour interval starting at 1:30pm cannot.</skos:note>
    </owl:Class>
    


    <!-- http://www.w3.org/2006/time#DayOfWeek -->


    <owl:Class rdf:about="http://www.w3.org/2006/time#DayOfWeek">
        <rdfs:subClassOf rdf:resource="http://www.w3.org/2002/07/owl#Thing"/>
        <rdfs:comment xml:lang="es">El día de la semana</rdfs:comment>
        <rdfs:comment xml:lang="en">The day of week</rdfs:comment>
        <rdfs:comment xml:lang="en">The day of week.</rdfs:comment>
        <rdfs:isDefinedBy rdf:resource="http://www.w3.org/2006/time#"/>
        <rdfs:label xml:lang="en">Day of week</rdfs:label>
        <rdfs:label xml:lang="es">día de la semana</rdfs:label>
        <skos:changeNote xml:lang="en">Remove enumeration from definition, in order to allow other days to be used when required in other calendars. 
NOTE: existing days are still present as members of the class, but the class membership is now open. 

In the original OWL-Time the following constraint appeared: 
  owl:oneOf (
      time:Monday
      time:Tuesday
      time:Wednesday
      time:Thursday
      time:Friday
      time:Saturday
      time:Sunday
    ) ;</skos:changeNote>
        <skos:definition xml:lang="es">El día de la semana</skos:definition>
        <skos:definition xml:lang="en">The day of week</skos:definition>
        <skos:note xml:lang="es">La pertenencia a la clase &apos;día de la semana&apos; está abierta, para permitir longitudes de semana alternativas y diferentes nombres de días.</skos:note>
        <skos:note xml:lang="en">Membership of the class :DayOfWeek is open, to allow for alternative week lengths and different day names.</skos:note>
    </owl:Class>
    


    <!-- http://www.w3.org/2006/time#Duration -->


    <owl:Class rdf:about="http://www.w3.org/2006/time#Duration">
        <rdfs:subClassOf rdf:resource="http://www.w3.org/2006/time#TemporalDuration"/>
        <rdfs:subClassOf>
            <owl:Restriction>
                <owl:onProperty rdf:resource="http://www.w3.org/2006/time#unitType"/>
                <owl:cardinality rdf:datatype="http://www.w3.org/2001/XMLSchema#nonNegativeInteger">1</owl:cardinality>
            </owl:Restriction>
        </rdfs:subClassOf>
        <rdfs:subClassOf>
            <owl:Restriction>
                <owl:onProperty rdf:resource="http://www.w3.org/2006/time#numericDuration"/>
                <owl:cardinality rdf:datatype="http://www.w3.org/2001/XMLSchema#nonNegativeInteger">1</owl:cardinality>
            </owl:Restriction>
        </rdfs:subClassOf>
        <rdfs:comment xml:lang="es">Duración de una extensión temporal expresada como un número escalado por una unidad temporal.</rdfs:comment>
        <rdfs:comment xml:lang="en">Duration of a temporal extent expressed as a number scaled by a temporal unit</rdfs:comment>
        <rdfs:label xml:lang="en">Time duration</rdfs:label>
        <rdfs:label>duración de tiempo</rdfs:label>
        <skos:definition xml:lang="es">Duración de una extensión temporal expresada como un número escalado por una unidad temporal.</skos:definition>
        <skos:definition xml:lang="en">Duration of a temporal extent expressed as a number scaled by a temporal unit</skos:definition>
        <skos:note xml:lang="es">Alternativa a &apos;descripción de tiempo&apos; para proporcionar descripción soporte a una duración temporal diferente a utilizar un sistema de calendario/reloj.</skos:note>
        <skos:note xml:lang="en">Alternative to time:DurationDescription to support description of a temporal duration other than using a calendar/clock system.</skos:note>
    </owl:Class>
    


    <!-- http://www.w3.org/2006/time#DurationDescription -->


    <owl:Class rdf:about="http://www.w3.org/2006/time#DurationDescription">
        <rdfs:subClassOf rdf:resource="http://www.w3.org/2006/time#GeneralDurationDescription"/>
        <rdfs:subClassOf>
            <owl:Restriction>
                <owl:onProperty rdf:resource="http://www.w3.org/2006/time#hasTRS"/>
                <owl:hasValue rdf:resource="http://www.opengis.net/def/uom/ISO-8601/0/Gregorian"/>
            </owl:Restriction>
        </rdfs:subClassOf>
        <rdfs:subClassOf>
            <owl:Restriction>
                <owl:onProperty rdf:resource="http://www.w3.org/2006/time#days"/>
                <owl:allValuesFrom rdf:resource="http://www.w3.org/2001/XMLSchema#decimal"/>
            </owl:Restriction>
        </rdfs:subClassOf>
        <rdfs:subClassOf>
            <owl:Restriction>
                <owl:onProperty rdf:resource="http://www.w3.org/2006/time#hours"/>
                <owl:allValuesFrom rdf:resource="http://www.w3.org/2001/XMLSchema#decimal"/>
            </owl:Restriction>
        </rdfs:subClassOf>
        <rdfs:subClassOf>
            <owl:Restriction>
                <owl:onProperty rdf:resource="http://www.w3.org/2006/time#minutes"/>
                <owl:allValuesFrom rdf:resource="http://www.w3.org/2001/XMLSchema#decimal"/>
            </owl:Restriction>
        </rdfs:subClassOf>
        <rdfs:subClassOf>
            <owl:Restriction>
                <owl:onProperty rdf:resource="http://www.w3.org/2006/time#months"/>
                <owl:allValuesFrom rdf:resource="http://www.w3.org/2001/XMLSchema#decimal"/>
            </owl:Restriction>
        </rdfs:subClassOf>
        <rdfs:subClassOf>
            <owl:Restriction>
                <owl:onProperty rdf:resource="http://www.w3.org/2006/time#seconds"/>
                <owl:allValuesFrom rdf:resource="http://www.w3.org/2001/XMLSchema#decimal"/>
            </owl:Restriction>
        </rdfs:subClassOf>
        <rdfs:subClassOf>
            <owl:Restriction>
                <owl:onProperty rdf:resource="http://www.w3.org/2006/time#weeks"/>
                <owl:allValuesFrom rdf:resource="http://www.w3.org/2001/XMLSchema#decimal"/>
            </owl:Restriction>
        </rdfs:subClassOf>
        <rdfs:subClassOf>
            <owl:Restriction>
                <owl:onProperty rdf:resource="http://www.w3.org/2006/time#years"/>
                <owl:allValuesFrom rdf:resource="http://www.w3.org/2001/XMLSchema#decimal"/>
            </owl:Restriction>
        </rdfs:subClassOf>
        <rdfs:comment xml:lang="es">Descripción de extensión temporal estructurada con valores separados para los distintos elementos de un sistema de horario-calendario. El sistema de referencia temporal se fija al calendario gregoriano, y el intervalo de cada una de las propiedades numéricas se restringe a xsd:decimal.</rdfs:comment>
        <rdfs:comment xml:lang="en">Description of temporal extent structured with separate values for the various elements of a calendar-clock system. The temporal reference system is fixed to Gregorian Calendar, and the range of each of the numeric properties is restricted to xsd:decimal</rdfs:comment>
        <rdfs:label xml:lang="en">Duration description</rdfs:label>
        <rdfs:label xml:lang="es">descripción de duración</rdfs:label>
        <skos:definition xml:lang="es">Descripción de extensión temporal estructurada con valores separados para los distintos elementos de un sistema de horario-calendario. El sistema de referencia temporal se fija al calendario gregoriano, y el intervalo de cada una de las propiedades numéricas se restringe a xsd:decimal.</skos:definition>
        <skos:definition xml:lang="en">Description of temporal extent structured with separate values for the various elements of a calendar-clock system. The temporal reference system is fixed to Gregorian Calendar, and the range of each of the numeric properties is restricted to xsd:decimal</skos:definition>
        <skos:note xml:lang="es">En el calendario gregoriano la longitud de los meses no es fija. Por lo tanto, un valor como &quot;2,5 meses&quot; no se puede comparar exactamente con una duración similar expresada en términos de semanas o días.</skos:note>
        <skos:note xml:lang="en">In the Gregorian calendar the length of the month is not fixed. Therefore, a value like &quot;2.5 months&quot; cannot be exactly compared with a similar duration expressed in terms of weeks or days.</skos:note>
    </owl:Class>
    


    <!-- http://www.w3.org/2006/time#GeneralDateTimeDescription -->


    <owl:Class rdf:about="http://www.w3.org/2006/time#GeneralDateTimeDescription">
        <rdfs:subClassOf rdf:resource="http://www.w3.org/2006/time#TemporalPosition"/>
        <rdfs:subClassOf>
            <owl:Restriction>
                <owl:onProperty rdf:resource="http://www.w3.org/2006/time#unitType"/>
                <owl:cardinality rdf:datatype="http://www.w3.org/2001/XMLSchema#nonNegativeInteger">1</owl:cardinality>
            </owl:Restriction>
        </rdfs:subClassOf>
        <rdfs:subClassOf>
            <owl:Restriction>
                <owl:onProperty rdf:resource="http://www.w3.org/2006/time#dayOfWeek"/>
                <owl:maxCardinality rdf:datatype="http://www.w3.org/2001/XMLSchema#nonNegativeInteger">1</owl:maxCardinality>
            </owl:Restriction>
        </rdfs:subClassOf>
        <rdfs:subClassOf>
            <owl:Restriction>
                <owl:onProperty rdf:resource="http://www.w3.org/2006/time#monthOfYear"/>
                <owl:maxCardinality rdf:datatype="http://www.w3.org/2001/XMLSchema#nonNegativeInteger">1</owl:maxCardinality>
            </owl:Restriction>
        </rdfs:subClassOf>
        <rdfs:subClassOf>
            <owl:Restriction>
                <owl:onProperty rdf:resource="http://www.w3.org/2006/time#timeZone"/>
                <owl:maxCardinality rdf:datatype="http://www.w3.org/2001/XMLSchema#nonNegativeInteger">1</owl:maxCardinality>
            </owl:Restriction>
        </rdfs:subClassOf>
        <rdfs:subClassOf>
            <owl:Restriction>
                <owl:onProperty rdf:resource="http://www.w3.org/2006/time#day"/>
                <owl:maxCardinality rdf:datatype="http://www.w3.org/2001/XMLSchema#nonNegativeInteger">1</owl:maxCardinality>
            </owl:Restriction>
        </rdfs:subClassOf>
        <rdfs:subClassOf>
            <owl:Restriction>
                <owl:onProperty rdf:resource="http://www.w3.org/2006/time#dayOfYear"/>
                <owl:maxCardinality rdf:datatype="http://www.w3.org/2001/XMLSchema#nonNegativeInteger">1</owl:maxCardinality>
            </owl:Restriction>
        </rdfs:subClassOf>
        <rdfs:subClassOf>
            <owl:Restriction>
                <owl:onProperty rdf:resource="http://www.w3.org/2006/time#hour"/>
                <owl:maxCardinality rdf:datatype="http://www.w3.org/2001/XMLSchema#nonNegativeInteger">1</owl:maxCardinality>
            </owl:Restriction>
        </rdfs:subClassOf>
        <rdfs:subClassOf>
            <owl:Restriction>
                <owl:onProperty rdf:resource="http://www.w3.org/2006/time#minute"/>
                <owl:maxCardinality rdf:datatype="http://www.w3.org/2001/XMLSchema#nonNegativeInteger">1</owl:maxCardinality>
            </owl:Restriction>
        </rdfs:subClassOf>
        <rdfs:subClassOf>
            <owl:Restriction>
                <owl:onProperty rdf:resource="http://www.w3.org/2006/time#month"/>
                <owl:maxCardinality rdf:datatype="http://www.w3.org/2001/XMLSchema#nonNegativeInteger">1</owl:maxCardinality>
            </owl:Restriction>
        </rdfs:subClassOf>
        <rdfs:subClassOf>
            <owl:Restriction>
                <owl:onProperty rdf:resource="http://www.w3.org/2006/time#second"/>
                <owl:maxCardinality rdf:datatype="http://www.w3.org/2001/XMLSchema#nonNegativeInteger">1</owl:maxCardinality>
            </owl:Restriction>
        </rdfs:subClassOf>
        <rdfs:subClassOf>
            <owl:Restriction>
                <owl:onProperty rdf:resource="http://www.w3.org/2006/time#week"/>
                <owl:maxCardinality rdf:datatype="http://www.w3.org/2001/XMLSchema#nonNegativeInteger">1</owl:maxCardinality>
            </owl:Restriction>
        </rdfs:subClassOf>
        <rdfs:subClassOf>
            <owl:Restriction>
                <owl:onProperty rdf:resource="http://www.w3.org/2006/time#year"/>
                <owl:maxCardinality rdf:datatype="http://www.w3.org/2001/XMLSchema#nonNegativeInteger">1</owl:maxCardinality>
            </owl:Restriction>
        </rdfs:subClassOf>
        <rdfs:comment xml:lang="es">Descripción de fecha y hora estructurada con valores separados para los distintos elementos de un sistema calendario-reloj.</rdfs:comment>
        <rdfs:comment xml:lang="en">Description of date and time structured with separate values for the various elements of a calendar-clock system</rdfs:comment>
        <rdfs:label xml:lang="en">Generalized date-time description</rdfs:label>
        <rdfs:label xml:lang="es">descripción de fecha-hora generalizada</rdfs:label>
        <skos:definition xml:lang="en">Description of date and time structured with separate values for the various elements of a calendar-clock system</skos:definition>
        <skos:definition>Descripción de fecha y hora estructurada con valores separados para los distintos elementos de un sistema calendario-reloj.</skos:definition>
        <skos:note xml:lang="es">Algunas combinaciones de propiedades son redundantes - por ejemplo, dentro de un &apos;año&apos; especificado si se proporciona &apos;día del año&apos; entonces &apos;día&apos; y &apos;mes&apos; se pueden computar, y viceversa. Los valores individuales deberían ser consistentes entre ellos y con el calendario, indicado a través del valor de la propiedad &apos;tiene TRS&apos;.</skos:note>
        <skos:note>Some combinations of properties are redundant - for example, within a specified :year if :dayOfYear is provided then :day and :month can be computed, and vice versa. Individual values should be consistent with each other and the calendar, indicated through the value of the :hasTRS property.</skos:note>
    </owl:Class>
    


    <!-- http://www.w3.org/2006/time#GeneralDurationDescription -->


    <owl:Class rdf:about="http://www.w3.org/2006/time#GeneralDurationDescription">
        <rdfs:subClassOf rdf:resource="http://www.w3.org/2006/time#TemporalDuration"/>
        <rdfs:subClassOf>
            <owl:Restriction>
                <owl:onProperty rdf:resource="http://www.w3.org/2006/time#hasTRS"/>
                <owl:cardinality rdf:datatype="http://www.w3.org/2001/XMLSchema#nonNegativeInteger">1</owl:cardinality>
            </owl:Restriction>
        </rdfs:subClassOf>
        <rdfs:subClassOf>
            <owl:Restriction>
                <owl:onProperty rdf:resource="http://www.w3.org/2006/time#days"/>
                <owl:maxCardinality rdf:datatype="http://www.w3.org/2001/XMLSchema#nonNegativeInteger">1</owl:maxCardinality>
            </owl:Restriction>
        </rdfs:subClassOf>
        <rdfs:subClassOf>
            <owl:Restriction>
                <owl:onProperty rdf:resource="http://www.w3.org/2006/time#hours"/>
                <owl:maxCardinality rdf:datatype="http://www.w3.org/2001/XMLSchema#nonNegativeInteger">1</owl:maxCardinality>
            </owl:Restriction>
        </rdfs:subClassOf>
        <rdfs:subClassOf>
            <owl:Restriction>
                <owl:onProperty rdf:resource="http://www.w3.org/2006/time#minutes"/>
                <owl:maxCardinality rdf:datatype="http://www.w3.org/2001/XMLSchema#nonNegativeInteger">1</owl:maxCardinality>
            </owl:Restriction>
        </rdfs:subClassOf>
        <rdfs:subClassOf>
            <owl:Restriction>
                <owl:onProperty rdf:resource="http://www.w3.org/2006/time#months"/>
                <owl:maxCardinality rdf:datatype="http://www.w3.org/2001/XMLSchema#nonNegativeInteger">1</owl:maxCardinality>
            </owl:Restriction>
        </rdfs:subClassOf>
        <rdfs:subClassOf>
            <owl:Restriction>
                <owl:onProperty rdf:resource="http://www.w3.org/2006/time#seconds"/>
                <owl:maxCardinality rdf:datatype="http://www.w3.org/2001/XMLSchema#nonNegativeInteger">1</owl:maxCardinality>
            </owl:Restriction>
        </rdfs:subClassOf>
        <rdfs:subClassOf>
            <owl:Restriction>
                <owl:onProperty rdf:resource="http://www.w3.org/2006/time#weeks"/>
                <owl:maxCardinality rdf:datatype="http://www.w3.org/2001/XMLSchema#nonNegativeInteger">1</owl:maxCardinality>
            </owl:Restriction>
        </rdfs:subClassOf>
        <rdfs:subClassOf>
            <owl:Restriction>
                <owl:onProperty rdf:resource="http://www.w3.org/2006/time#years"/>
                <owl:maxCardinality rdf:datatype="http://www.w3.org/2001/XMLSchema#nonNegativeInteger">1</owl:maxCardinality>
            </owl:Restriction>
        </rdfs:subClassOf>
        <rdfs:comment xml:lang="es">Descripción de extensión temporal estructurada con valores separados para los distintos elementos de un sistema de horario-calendario.</rdfs:comment>
        <rdfs:comment xml:lang="en">Description of temporal extent structured with separate values for the various elements of a calendar-clock system.</rdfs:comment>
        <rdfs:label xml:lang="en">Generalized duration description</rdfs:label>
        <rdfs:label xml:lang="es">descripción de duración generalizada</rdfs:label>
        <skos:definition xml:lang="es">Descripción de extensión temporal estructurada con valores separados para los distintos elementos de un sistema de horario-calendario.</skos:definition>
        <skos:definition xml:lang="en">Description of temporal extent structured with separate values for the various elements of a calendar-clock system.</skos:definition>
        <skos:note xml:lang="es">La extensión de una duración de tiempo expresada como una &apos;descripción de duración general&apos; depende del Sistema de Referencia Temporal. En algunos calendarios la longitud de la semana o del mes no es constante a lo largo del año. Por tanto, un valor como &quot;25 meses&quot; puede no ser necesariamente ser comparado con un duración similar expresada en términos de semanas o días. Cuando se consideran calendarios que no están basados en el movimiento de la Tierra, se deben tomar incluso más precauciones en la comparación de duraciones.</skos:note>
        <skos:note xml:lang="en">The extent of a time duration expressed as a GeneralDurationDescription depends on the Temporal Reference System. In some calendars the length of the week or month is not constant within the year. Therefore, a value like &quot;2.5 months&quot; may not necessarily be exactly compared with a similar duration expressed in terms of weeks or days. When non-earth-based calendars are considered even more care must be taken in comparing durations.</skos:note>
    </owl:Class>
    


    <!-- http://www.w3.org/2006/time#Instant -->


    <owl:Class rdf:about="http://www.w3.org/2006/time#Instant">
        <rdfs:subClassOf rdf:resource="http://www.w3.org/2006/time#TemporalEntity"/>
        <owl:disjointWith rdf:resource="http://www.w3.org/2006/time#ProperInterval"/>
        <rdfs:comment xml:lang="en">A temporal entity with zero extent or duration</rdfs:comment>
        <rdfs:comment xml:lang="es">Una entidad temporal con una extensión o duración cero.</rdfs:comment>
        <rdfs:isDefinedBy rdf:resource="http://www.w3.org/2006/time#"/>
        <rdfs:label xml:lang="en">Instant</rdfs:label>
        <rdfs:label xml:lang="en">Time instant</rdfs:label>
        <rdfs:label xml:lang="es">instante de tiempo.</rdfs:label>
        <skos:definition xml:lang="en">A temporal entity with zero extent or duration</skos:definition>
        <skos:definition xml:lang="es">Una entidad temporal con una extensión o duración cero.</skos:definition>
    </owl:Class>
    


    <!-- http://www.w3.org/2006/time#Interval -->


    <owl:Class rdf:about="http://www.w3.org/2006/time#Interval">
        <rdfs:subClassOf rdf:resource="http://www.w3.org/2006/time#TemporalEntity"/>
        <rdfs:comment xml:lang="en">A temporal entity with an extent or duration</rdfs:comment>
        <rdfs:comment xml:lang="en">A temporal entity with an extent or duration.</rdfs:comment>
        <rdfs:comment xml:lang="es">Una entidad temporal con una extensión o duración.</rdfs:comment>
        <rdfs:isDefinedBy rdf:resource="http://www.w3.org/2006/time#"/>
        <rdfs:label xml:lang="en">Interval</rdfs:label>
        <rdfs:label xml:lang="en">Time interval</rdfs:label>
        <rdfs:label xml:lang="es">intervalo de tiempo</rdfs:label>
        <skos:definition xml:lang="en">A temporal entity with an extent or duration</skos:definition>
        <skos:definition xml:lang="es">Una entidad temporal con una extensión o duración.</skos:definition>
    </owl:Class>
    


    <!-- http://www.w3.org/2006/time#January -->


    <owl:Class rdf:about="http://www.w3.org/2006/time#January">
        <rdfs:subClassOf rdf:resource="http://www.w3.org/2006/time#DateTimeDescription"/>
        <rdfs:subClassOf>
            <owl:Restriction>
                <owl:onProperty rdf:resource="http://www.w3.org/2006/time#unitType"/>
                <owl:hasValue rdf:resource="http://www.w3.org/2006/time#unitMonth"/>
            </owl:Restriction>
        </rdfs:subClassOf>
        <rdfs:subClassOf>
            <owl:Restriction>
                <owl:onProperty rdf:resource="http://www.w3.org/2006/time#month"/>
                <owl:hasValue>--01</owl:hasValue>
            </owl:Restriction>
        </rdfs:subClassOf>
        <rdfs:label>January</rdfs:label>
        <owl:deprecated rdf:datatype="http://www.w3.org/2001/XMLSchema#boolean">true</owl:deprecated>
        <skos:historyNote>This class was present in the 2006 version of OWL-Time. It was presented as an example of how DateTimeDescription could be specialized, but does not belong in the revised ontology. </skos:historyNote>
    </owl:Class>
    


    <!-- http://www.w3.org/2006/time#MonthOfYear -->


    <owl:Class rdf:about="http://www.w3.org/2006/time#MonthOfYear">
        <rdfs:subClassOf rdf:resource="http://www.w3.org/2006/time#DateTimeDescription"/>
        <rdfs:subClassOf>
            <owl:Restriction>
                <owl:onProperty rdf:resource="http://www.w3.org/2006/time#unitType"/>
                <owl:hasValue rdf:resource="http://www.w3.org/2006/time#unitMonth"/>
            </owl:Restriction>
        </rdfs:subClassOf>
        <rdfs:subClassOf>
            <owl:Restriction>
                <owl:onProperty rdf:resource="http://www.w3.org/2006/time#day"/>
                <owl:cardinality rdf:datatype="http://www.w3.org/2001/XMLSchema#nonNegativeInteger">0</owl:cardinality>
            </owl:Restriction>
        </rdfs:subClassOf>
        <rdfs:subClassOf>
            <owl:Restriction>
                <owl:onProperty rdf:resource="http://www.w3.org/2006/time#hour"/>
                <owl:cardinality rdf:datatype="http://www.w3.org/2001/XMLSchema#nonNegativeInteger">0</owl:cardinality>
            </owl:Restriction>
        </rdfs:subClassOf>
        <rdfs:subClassOf>
            <owl:Restriction>
                <owl:onProperty rdf:resource="http://www.w3.org/2006/time#minute"/>
                <owl:cardinality rdf:datatype="http://www.w3.org/2001/XMLSchema#nonNegativeInteger">0</owl:cardinality>
            </owl:Restriction>
        </rdfs:subClassOf>
        <rdfs:subClassOf>
            <owl:Restriction>
                <owl:onProperty rdf:resource="http://www.w3.org/2006/time#month"/>
                <owl:cardinality rdf:datatype="http://www.w3.org/2001/XMLSchema#nonNegativeInteger">1</owl:cardinality>
            </owl:Restriction>
        </rdfs:subClassOf>
        <rdfs:subClassOf>
            <owl:Restriction>
                <owl:onProperty rdf:resource="http://www.w3.org/2006/time#second"/>
                <owl:cardinality rdf:datatype="http://www.w3.org/2001/XMLSchema#nonNegativeInteger">0</owl:cardinality>
            </owl:Restriction>
        </rdfs:subClassOf>
        <rdfs:subClassOf>
            <owl:Restriction>
                <owl:onProperty rdf:resource="http://www.w3.org/2006/time#week"/>
                <owl:cardinality rdf:datatype="http://www.w3.org/2001/XMLSchema#nonNegativeInteger">0</owl:cardinality>
            </owl:Restriction>
        </rdfs:subClassOf>
        <rdfs:subClassOf>
            <owl:Restriction>
                <owl:onProperty rdf:resource="http://www.w3.org/2006/time#year"/>
                <owl:cardinality rdf:datatype="http://www.w3.org/2001/XMLSchema#nonNegativeInteger">0</owl:cardinality>
            </owl:Restriction>
        </rdfs:subClassOf>
        <rdfs:comment xml:lang="es">El mes del año.</rdfs:comment>
        <rdfs:comment xml:lang="en">The month of the year</rdfs:comment>
        <rdfs:label xml:lang="en">Month of year</rdfs:label>
        <rdfs:label xml:lang="es">mes del año</rdfs:label>
        <skos:definition xml:lang="es">El mes del año.</skos:definition>
        <skos:definition xml:lang="en">The month of the year</skos:definition>
        <skos:editorialNote xml:lang="es">Característica en riesgo - añadida en la revisión de 2017, y no utilizada todavía de forma amplia.</skos:editorialNote>
        <skos:editorialNote xml:lang="en">Feature at risk - added in 2017 revision, and not yet widely used. </skos:editorialNote>
        <skos:note xml:lang="es">La pertenencia a la clase &apos;mes del año&apos; está abierta, a permitir calendarios anuales alternativos y diferentes nombres de meses.</skos:note>
        <skos:note xml:lang="en">Membership of the class :MonthOfYear is open, to allow for alternative annual calendars and different month names.</skos:note>
    </owl:Class>
    


    <!-- http://www.w3.org/2006/time#ProperInterval -->


    <owl:Class rdf:about="http://www.w3.org/2006/time#ProperInterval">
        <rdfs:subClassOf rdf:resource="http://www.w3.org/2006/time#Interval"/>
        <rdfs:comment xml:lang="en">A temporal entity with non-zero extent or duration, i.e. for which the value of the beginning and end are different</rdfs:comment>
        <rdfs:comment xml:lang="es">Una entidad temporal con extensión o duración distinta de cero, es decir, para la cual los valores de principio y fin del intervalo son diferentes.</rdfs:comment>
        <rdfs:label xml:lang="en">Proper interval</rdfs:label>
        <rdfs:label xml:lang="es">intervalo propio</rdfs:label>
        <skos:definition xml:lang="en">A temporal entity with non-zero extent or duration, i.e. for which the value of the beginning and end are different</skos:definition>
        <skos:definition xml:lang="es">Una entidad temporal con extensión o duración distinta de cero, es decir, para la cual los valores de principio y fin del intervalo son diferentes.</skos:definition>
    </owl:Class>
    


    <!-- http://www.w3.org/2006/time#TRS -->


    <owl:Class rdf:about="http://www.w3.org/2006/time#TRS">
        <rdfs:comment xml:lang="en">A temporal reference system, such as a temporal coordinate system (with an origin, direction, and scale), a calendar-clock combination, or a (possibly hierarchical) ordinal system. 

This is a stub class, representing the set of all temporal reference systems.</rdfs:comment>
        <rdfs:comment xml:lang="es">Un sistema de referencia temporal, tal como un sistema de coordenadas temporales (con un origen, una dirección y una escala), una combinación calendario-reloj, o un sistema ordinal (posiblemente jerárquico).
        Esta clase comodín representa el conjunto de todos los sistemas de referencia temporal.</rdfs:comment>
        <rdfs:label xml:lang="en">Temporal Reference System</rdfs:label>
        <rdfs:label xml:lang="es">sistema de referencia temporal</rdfs:label>
        <skos:definition xml:lang="en">A temporal reference system, such as a temporal coordinate system (with an origin, direction, and scale), a calendar-clock combination, or a (possibly hierarchical) ordinal system. 

This is a stub class, representing the set of all temporal reference systems.</skos:definition>
        <skos:definition xml:lang="es">Un sistema de referencia temporal, tal como un sistema de coordenadas temporales (con un origen, una dirección y una escala), una combinación calendario-reloj, o un sistema ordinal (posiblemente jerárquico).
    Esta clase comodín representa el conjunto de todos los sistemas de referencia temporal.</skos:definition>
        <skos:note xml:lang="en">A taxonomy of temporal reference systems is provided in ISO 19108:2002 [ISO19108], including (a) calendar + clock systems; (b) temporal coordinate systems (i.e. numeric offset from an epoch); (c) temporal ordinal reference systems (i.e. ordered sequence of named intervals, not necessarily of equal duration).</skos:note>
        <skos:note xml:lang="es">En el ISO 19108:2002 [ISO19108] se proporciona una taxonomía de sistemas de referencia temporal, incluyendo (a) sistemas de calendario + reloj; (b) sistemas de coordenadas temporales (es decir, desplazamiento numérico a partir de una época); (c) sistemas de referencia ordinales temporales (es decir, secuencia ordenada de intervalos nombrados, no necesariamente de igual duración).</skos:note>
    </owl:Class>
    


    <!-- http://www.w3.org/2006/time#TemporalDuration -->


    <owl:Class rdf:about="http://www.w3.org/2006/time#TemporalDuration">
        <rdfs:comment xml:lang="es">Extensión de tiempo; duración de un intervalo de tiempo independiente de su posición de inicio particular.</rdfs:comment>
        <rdfs:comment xml:lang="en">Time extent; duration of a time interval separate from its particular start position</rdfs:comment>
        <rdfs:isDefinedBy rdf:resource="http://www.w3.org/2006/time#"/>
        <rdfs:label xml:lang="en">Temporal duration</rdfs:label>
        <rdfs:label xml:lang="es">duración temporal</rdfs:label>
        <skos:definition xml:lang="es">Extensión de tiempo; duración de un intervalo de tiempo independiente de su posición de inicio particular.</skos:definition>
        <skos:definition xml:lang="en">Time extent; duration of a time interval separate from its particular start position</skos:definition>
    </owl:Class>
    


    <!-- http://www.w3.org/2006/time#TemporalEntity -->


    <owl:Class rdf:about="http://www.w3.org/2006/time#TemporalEntity">
        <owl:equivalentClass>
            <owl:Class>
                <owl:unionOf rdf:parseType="Collection">
                    <rdf:Description rdf:about="http://www.w3.org/2006/time#Instant"/>
                    <rdf:Description rdf:about="http://www.w3.org/2006/time#Interval"/>
                </owl:unionOf>
            </owl:Class>
        </owl:equivalentClass>
        <rdfs:subClassOf rdf:resource="http://www.w3.org/2002/07/owl#Thing"/>
        <rdfs:comment xml:lang="en">A temporal interval or instant.</rdfs:comment>
        <rdfs:comment xml:lang="es">Un intervalo temporal o un instante.</rdfs:comment>
        <rdfs:isDefinedBy rdf:resource="http://www.w3.org/2006/time#"/>
        <rdfs:label xml:lang="en">Temporal entity</rdfs:label>
        <rdfs:label xml:lang="es">entidad temporal</rdfs:label>
        <skos:definition xml:lang="en">A temporal interval or instant.</skos:definition>
        <skos:definition xml:lang="es">Un intervalo temporal o un instante.</skos:definition>
    </owl:Class>
    


    <!-- http://www.w3.org/2006/time#TemporalPosition -->


    <owl:Class rdf:about="http://www.w3.org/2006/time#TemporalPosition">
        <rdfs:subClassOf>
            <owl:Restriction>
                <owl:onProperty rdf:resource="http://www.w3.org/2006/time#hasTRS"/>
                <owl:cardinality rdf:datatype="http://www.w3.org/2001/XMLSchema#nonNegativeInteger">1</owl:cardinality>
            </owl:Restriction>
        </rdfs:subClassOf>
        <rdfs:comment xml:lang="en">A position on a time-line</rdfs:comment>
        <rdfs:comment xml:lang="es">Una posición sobre una línea de tiempo.</rdfs:comment>
        <rdfs:label xml:lang="en">Temporal position</rdfs:label>
        <rdfs:label xml:lang="es">posición temporal</rdfs:label>
        <skos:definition xml:lang="en">A position on a time-line</skos:definition>
        <skos:definition xml:lang="es">Una posición sobre una línea de tiempo.</skos:definition>
    </owl:Class>
    


    <!-- http://www.w3.org/2006/time#TemporalUnit -->


    <owl:Class rdf:about="http://www.w3.org/2006/time#TemporalUnit">
        <rdfs:subClassOf rdf:resource="http://www.w3.org/2006/time#TemporalDuration"/>
        <rdfs:comment xml:lang="en">A standard duration, which provides a scale factor for a time extent, or the granularity or precision for a time position.</rdfs:comment>
        <rdfs:comment xml:lang="es">Una duración estándar, que proporciona un factor de escala para una extensión de tiempo, o la granularidad o precisión para una posición de tiempo.</rdfs:comment>
        <rdfs:label xml:lang="en">Temporal unit</rdfs:label>
        <rdfs:label xml:lang="es">unidad de tiempo</rdfs:label>
        <skos:changeNote xml:lang="en">Remove enumeration from definition, in order to allow other units to be used when required in other coordinate systems. 
NOTE: existing units are still present as members of the class, but the class membership is now open. 

In the original OWL-Time the following constraint appeared: 
  owl:oneOf (
      time:unitSecond
      time:unitMinute
      time:unitHour
      time:unitDay
      time:unitWeek
      time:unitMonth
      time:unitYear
    ) ;</skos:changeNote>
        <skos:definition xml:lang="en">A standard duration, which provides a scale factor for a time extent, or the granularity or precision for a time position.</skos:definition>
        <skos:definition xml:lang="es">Una duración estándar, que proporciona un factor de escala para una extensión de tiempo, o la granularidad o precisión para una posición de tiempo.</skos:definition>
        <skos:note xml:lang="es">La pertenencia de la clase &apos;unidad de tiempo&apos; está abierta, para permitir otras unidades de tiempo utilizadas en algunas aplicaciones técnicas (por ejemplo, millones de años o el mes Baha&apos;i).</skos:note>
        <skos:note xml:lang="en">Membership of the class TemporalUnit is open, to allow for other temporal units used in some technical applications (e.g. millions of years, Baha&apos;i month).</skos:note>
    </owl:Class>
    


    <!-- http://www.w3.org/2006/time#TimePosition -->


    <owl:Class rdf:about="http://www.w3.org/2006/time#TimePosition">
        <rdfs:subClassOf rdf:resource="http://www.w3.org/2006/time#TemporalPosition"/>
        <rdfs:subClassOf>
            <owl:Class>
                <owl:unionOf rdf:parseType="Collection">
                    <owl:Restriction>
                        <owl:onProperty rdf:resource="http://www.w3.org/2006/time#nominalPosition"/>
                        <owl:cardinality rdf:datatype="http://www.w3.org/2001/XMLSchema#nonNegativeInteger">1</owl:cardinality>
                    </owl:Restriction>
                    <owl:Restriction>
                        <owl:onProperty rdf:resource="http://www.w3.org/2006/time#numericPosition"/>
                        <owl:cardinality rdf:datatype="http://www.w3.org/2001/XMLSchema#nonNegativeInteger">1</owl:cardinality>
                    </owl:Restriction>
                </owl:unionOf>
            </owl:Class>
        </rdfs:subClassOf>
        <rdfs:comment xml:lang="en">A temporal position described using either a (nominal) value from an ordinal reference system, or a (numeric) value in a temporal coordinate system. </rdfs:comment>
        <rdfs:comment xml:lang="es">Una posición temporal descrita utilizando bien un valor (nominal) de un sistema de referencia ordinal, o un valor (numérico) en un sistema de coordenadas temporales.</rdfs:comment>
        <rdfs:label xml:lang="en">Time position</rdfs:label>
        <rdfs:label xml:lang="es">posición de tiempo</rdfs:label>
        <skos:definition xml:lang="en">A temporal position described using either a (nominal) value from an ordinal reference system, or a (numeric) value in a temporal coordinate system. </skos:definition>
        <skos:definition xml:lang="es">Una posición temporal descrita utilizando bien un valor (nominal) de un sistema de referencia ordinal, o un valor (numérico) en un sistema de coordenadas temporales.</skos:definition>
    </owl:Class>
    


    <!-- http://www.w3.org/2006/time#TimeZone -->


    <owl:Class rdf:about="http://www.w3.org/2006/time#TimeZone">
        <rdfs:comment xml:lang="en">A Time Zone specifies the amount by which the local time is offset from UTC. 
	A time zone is usually denoted geographically (e.g. Australian Eastern Daylight Time), with a constant value in a given region. 
The region where it applies and the offset from UTC are specified by a locally recognised governing authority.</rdfs:comment>
        <rdfs:comment xml:lang="es">Un huso horario especifica la cantidad en que la hora local está desplazada con respecto a UTC.
        Un huso horario normalmente se denota geográficamente (p.ej. el horario de verano del este de Australia), con un valor constante en una región dada.
        La región donde aplica y el desplazamiento desde UTC las especifica una autoridad gubernamental localmente reconocida.</rdfs:comment>
        <rdfs:label xml:lang="en">Time Zone</rdfs:label>
        <rdfs:label xml:lang="es">huso horario</rdfs:label>
        <skos:definition xml:lang="en">A Time Zone specifies the amount by which the local time is offset from UTC. 
	A time zone is usually denoted geographically (e.g. Australian Eastern Daylight Time), with a constant value in a given region. 
The region where it applies and the offset from UTC are specified by a locally recognised governing authority.</skos:definition>
        <skos:definition xml:lang="es">Un huso horario especifica la cantidad en que la hora local está desplazada con respecto a UTC.
    Un huso horario normalmente se denota geográficamente (p.ej. el horario de verano del este de Australia), con un valor constante en una región dada.
    La región donde aplica y el desplazamiento desde UTC las especifica una autoridad gubernamental localmente reconocida.</skos:definition>
        <skos:historyNote xml:lang="es">En la versión original de OWL-Time de 2006, se definió, en un espacio de nombres diferente &quot;http://www.w3.org/2006/timezone#&quot;, la clase &apos;huso horario&apos;, con varias propiedades específicas correspondientes a un modelo específico de huso horario.
    En la versión actual hay una clase con el mismo nombre local en el espacio de nombres de OWL-Time, eliminando la dependencia del espacio de nombres externo.
    Un axioma de alineación permite que los datos codificados de acuerdo con la versión anterior sean consistentes con la ontología actualizada.</skos:historyNote>
        <skos:historyNote>In the original 2006 version of OWL-Time, the TimeZone class, with several properties corresponding to a specific model of time-zones, was defined in a separate namespace &quot;http://www.w3.org/2006/timezone#&quot;. 

In the current version a class with same local name is put into the main OWL-Time namespace, removing the dependency on the external namespace. 

An alignment axiom 
	tzont:TimeZone rdfs:subClassOf time:TimeZone . 
allows data encoded according to the previous version to be consistent with the updated ontology. </skos:historyNote>
        <skos:note xml:lang="en">A designated timezone is associated with a geographic region. However, for a particular region the offset from UTC often varies seasonally, and the dates of the changes may vary from year to year. The timezone designation usually changes for the different seasons (e.g. Australian Eastern Standard Time vs. Australian Eastern Daylight Time). Furthermore, the offset for a timezone may change over longer timescales, though its designation might not.  

Detailed guidance about working with time zones is given in http://www.w3.org/TR/timezone/ .</skos:note>
        <skos:note xml:lang="en">An ontology for time zone descriptions was described in [owl-time-20060927] and provided as RDF in a separate namespace tzont:. However, that ontology was incomplete in scope, and the example datasets were selective. Furthermore, since the use of a class from an external ontology as the range of an ObjectProperty in OWL-Time creates a dependency, reference to the time zone class has been replaced with the &apos;stub&apos; class in the normative part of this version of OWL-Time.</skos:note>
        <skos:note xml:lang="es">Un huso horario designado está asociado con una región geográfica. Sin embargo, para una región particular el desplazamiento desde UTC a menudo varía según las estaciones, y las fechas de los cambios pueden variar de un año a otro. La designación de huso horario  normalmente cambia de una estación a otra (por ejemplo, el horario estándar frente al horario de verano ambos del este de Australia). Además, del desplazamiento para un huso horario puede cambiar sobre escalas de tiempo mayores, aunque su designación no lo haga.
    Se puede encontrar una guía detallada sobre el funcionamiento de husos horarios en http://www.w3.org/TR/timezone/.&quot;@es , &quot;En [owl-time-20060927] se describió una ontología para descripciones de husos horarios, y se proporcionó en un espacio de nombres separado tzont:. Sin embargo, dicha ontología estaba incompleta en su alcance, y el ejemplo de conjuntos de datos (datasets) era selectivo. Además, puesto que el uso de una clase de una ontología externa como el rango de una propiedad de objeto en OWL-Time crea una dependencia, la referencia a la clase huso horario se ha reemplazado por una clase que viene a ser un &quot;cajón de sastre&quot; en la en la parte normativa de esta versión de OWL-Time.</skos:note>
        <skos:scopeNote xml:lang="es">En esta implementación &apos;huso horario&apos; no tiene definidas propiedades. Se debería pensar como una superclase &quot;abstracta&quot; de todas las implementaciones de huso horario específicas.</skos:scopeNote>
        <skos:scopeNote>In this implementation TimeZone has no properties defined. It should be thought of as an &apos;abstract&apos; superclass of all specific timezone implementations.</skos:scopeNote>
    </owl:Class>
    


    <!-- http://www.w3.org/2006/time#Year -->


    <owl:Class rdf:about="http://www.w3.org/2006/time#Year">
        <rdfs:subClassOf rdf:resource="http://www.w3.org/2006/time#DurationDescription"/>
        <rdfs:subClassOf>
            <owl:Restriction>
                <owl:onProperty rdf:resource="http://www.w3.org/2006/time#days"/>
                <owl:cardinality rdf:datatype="http://www.w3.org/2001/XMLSchema#nonNegativeInteger">0</owl:cardinality>
            </owl:Restriction>
        </rdfs:subClassOf>
        <rdfs:subClassOf>
            <owl:Restriction>
                <owl:onProperty rdf:resource="http://www.w3.org/2006/time#hours"/>
                <owl:cardinality rdf:datatype="http://www.w3.org/2001/XMLSchema#nonNegativeInteger">0</owl:cardinality>
            </owl:Restriction>
        </rdfs:subClassOf>
        <rdfs:subClassOf>
            <owl:Restriction>
                <owl:onProperty rdf:resource="http://www.w3.org/2006/time#minutes"/>
                <owl:cardinality rdf:datatype="http://www.w3.org/2001/XMLSchema#nonNegativeInteger">0</owl:cardinality>
            </owl:Restriction>
        </rdfs:subClassOf>
        <rdfs:subClassOf>
            <owl:Restriction>
                <owl:onProperty rdf:resource="http://www.w3.org/2006/time#months"/>
                <owl:cardinality rdf:datatype="http://www.w3.org/2001/XMLSchema#nonNegativeInteger">0</owl:cardinality>
            </owl:Restriction>
        </rdfs:subClassOf>
        <rdfs:subClassOf>
            <owl:Restriction>
                <owl:onProperty rdf:resource="http://www.w3.org/2006/time#seconds"/>
                <owl:cardinality rdf:datatype="http://www.w3.org/2001/XMLSchema#nonNegativeInteger">0</owl:cardinality>
            </owl:Restriction>
        </rdfs:subClassOf>
        <rdfs:subClassOf>
            <owl:Restriction>
                <owl:onProperty rdf:resource="http://www.w3.org/2006/time#weeks"/>
                <owl:cardinality rdf:datatype="http://www.w3.org/2001/XMLSchema#nonNegativeInteger">0</owl:cardinality>
            </owl:Restriction>
        </rdfs:subClassOf>
        <rdfs:subClassOf>
            <owl:Restriction>
                <owl:onProperty rdf:resource="http://www.w3.org/2006/time#years"/>
                <owl:cardinality rdf:datatype="http://www.w3.org/2001/XMLSchema#nonNegativeInteger">1</owl:cardinality>
            </owl:Restriction>
        </rdfs:subClassOf>
        <rdfs:comment>Year duration</rdfs:comment>
        <rdfs:label xml:lang="en">Year</rdfs:label>
        <owl:deprecated rdf:datatype="http://www.w3.org/2001/XMLSchema#boolean">true</owl:deprecated>
        <skos:definition>Year duration</skos:definition>
        <skos:historyNote>Year was proposed in the 2006 version of OWL-Time as an example of how DurationDescription could be specialized to allow for a duration to be restricted to a number of years. 

It is deprecated in this edition of OWL-Time. </skos:historyNote>
        <skos:prefLabel xml:lang="it">Anno</skos:prefLabel>
        <skos:prefLabel xml:lang="fr">Année (calendrier)</skos:prefLabel>
        <skos:prefLabel xml:lang="pt">Ano</skos:prefLabel>
        <skos:prefLabel xml:lang="es">Año</skos:prefLabel>
        <skos:prefLabel xml:lang="nl">Jaar</skos:prefLabel>
        <skos:prefLabel xml:lang="de">Jahr</skos:prefLabel>
        <skos:prefLabel xml:lang="pl">Rok</skos:prefLabel>
        <skos:prefLabel xml:lang="en">Year</skos:prefLabel>
        <skos:prefLabel xml:lang="ru">Год</skos:prefLabel>
        <skos:prefLabel xml:lang="ar">سنة</skos:prefLabel>
        <skos:prefLabel xml:lang="ja">年</skos:prefLabel>
        <skos:prefLabel xml:lang="zh">年</skos:prefLabel>
    </owl:Class>
    


    <!-- http://www.w3.org/2015/03/inspire/cp#CadastralParcel -->


    <owl:Class rdf:about="http://www.w3.org/2015/03/inspire/cp#CadastralParcel">
        <rdfs:subClassOf rdf:resource="http://www.opengis.net/ont/geosparql#SpatialObject"/>
        <rdfs:comment xml:lang="en">Areas defined by cadastral registers or equivalent.</rdfs:comment>
        <rdfs:isDefinedBy rdf:resource="http://www.w3.org/2015/03/inspire/cp"/>
        <rdfs:label xml:lang="en">Cadastral Parcel</rdfs:label>
    </owl:Class>
    


    <!-- http://www.w3.org/ns/sosa/Platform -->


    <owl:Class rdf:about="http://www.w3.org/ns/sosa/Platform">
        <rdfs:comment xml:lang="en">A Platform is an entity that hosts other entities, particularly Sensors, Actuators, Samplers, and other Platforms (definition taken from http://www.w3.org/ns/sosa/Platform)</rdfs:comment>
        <rdfs:isDefinedBy rdf:resource="http://www.w3.org/ns/sosa/"/>
        <rdfs:label xml:lang="en">Platform</rdfs:label>
    </owl:Class>
    


    <!-- http://www.w3.org/ns/ssn/Deployment -->


    <owl:Class rdf:about="http://www.w3.org/ns/ssn/Deployment">
        <rdfs:isDefinedBy rdf:resource="http://www.w3.org/ns/ssn/"/>
        <rdfs:label xml:lang="en">Deployment</rdfs:label>
    </owl:Class>
    


    <!-- http://www.w3.org/ns/ssn/System -->


    <owl:Class rdf:about="http://www.w3.org/ns/ssn/System">
        <rdfs:comment xml:lang="en">System is a unit of abstraction for pieces of infrastructure that implement Procedures. A System may have components, its subsystems, which are other Systems. (Definition taken from http://www.w3.org/ns/ssn/System)</rdfs:comment>
        <rdfs:isDefinedBy rdf:resource="http://www.w3.org/ns/ssn/"/>
        <rdfs:label xml:lang="en">System</rdfs:label>
    </owl:Class>
    


    <!-- http://xmlns.com/foaf/0.1/Agent -->


    <owl:Class rdf:about="http://xmlns.com/foaf/0.1/Agent">
        <rdfs:subClassOf>
            <owl:Restriction>
                <owl:onProperty rdf:resource="http://bigg-project.eu/ontology#manages"/>
                <owl:someValuesFrom rdf:resource="http://bigg-project.eu/ontology#Patrimony"/>
            </owl:Restriction>
        </rdfs:subClassOf>
        <rdfs:subClassOf>
            <owl:Restriction>
                <owl:onProperty rdf:resource="http://xmlns.com/foaf/0.1/member"/>
                <owl:someValuesFrom rdf:resource="http://xmlns.com/foaf/0.1/Agent"/>
            </owl:Restriction>
        </rdfs:subClassOf>
        <rdfs:label xml:lang="en">Agent</rdfs:label>
    </owl:Class>
    


    <!-- http://xmlns.com/foaf/0.1/Person -->


    <owl:Class rdf:about="http://xmlns.com/foaf/0.1/Person">
        <rdfs:subClassOf rdf:resource="http://xmlns.com/foaf/0.1/Agent"/>
        <rdfs:label xml:lang="en">Person</rdfs:label>
    </owl:Class>
    


    <!-- https://saref.etsi.org/core/ActuatingFunction -->


    <owl:Class rdf:about="https://saref.etsi.org/core/ActuatingFunction">
        <rdfs:subClassOf rdf:resource="https://saref.etsi.org/core/Function"/>
        <rdfs:comment xml:lang="en">A function that allows to transmit data to actuators, such as level settings (e.g., temperature) or binary switching (e.g., open/close, on/off)</rdfs:comment>
        <rdfs:label xml:lang="en">Actuating function</rdfs:label>
    </owl:Class>
    


    <!-- https://saref.etsi.org/core/Actuator -->


    <owl:Class rdf:about="https://saref.etsi.org/core/Actuator">
        <rdfs:subClassOf rdf:resource="https://saref.etsi.org/core/Device"/>
        <rdfs:subClassOf>
            <owl:Restriction>
                <owl:onProperty rdf:resource="https://saref.etsi.org/core/hasFunction"/>
                <owl:someValuesFrom rdf:resource="https://saref.etsi.org/core/ActuatingFunction"/>
            </owl:Restriction>
        </rdfs:subClassOf>
        <owl:disjointWith rdf:resource="https://saref.etsi.org/core/Sensor"/>
        <rdfs:comment xml:lang="en">A device responsible for moving or controlling a mechanism or system</rdfs:comment>
        <rdfs:comment xml:lang="en">A device responsible for moving or controlling a mechanism or system by performing an actuating function</rdfs:comment>
        <rdfs:comment xml:lang="en">A device responsible for moving or controlling a mechanism or system.</rdfs:comment>
        <rdfs:isDefinedBy rdf:resource="https://saref.etsi.org/core/"/>
        <rdfs:label xml:lang="en">Actuator</rdfs:label>
    </owl:Class>
    


    <!-- https://saref.etsi.org/core/Appliance -->


    <owl:Class rdf:about="https://saref.etsi.org/core/Appliance">
        <rdfs:subClassOf rdf:resource="https://saref.etsi.org/core/Device"/>
        <rdfs:comment xml:lang="en">An electrical/mechanical machine that accomplish some household functions, such as cleaning or cooking</rdfs:comment>
        <rdfs:label xml:lang="en">Appliance</rdfs:label>
    </owl:Class>
    


    <!-- https://saref.etsi.org/core/CloseCommand -->


    <owl:Class rdf:about="https://saref.etsi.org/core/CloseCommand">
        <rdfs:subClassOf rdf:resource="https://saref.etsi.org/core/Command"/>
        <rdfs:subClassOf>
            <owl:Restriction>
                <owl:onProperty rdf:resource="https://saref.etsi.org/core/actsUpon"/>
                <owl:someValuesFrom rdf:resource="https://saref.etsi.org/core/OpenCloseState"/>
            </owl:Restriction>
        </rdfs:subClassOf>
        <rdfs:subClassOf>
            <owl:Restriction>
                <owl:onProperty rdf:resource="https://saref.etsi.org/core/isCommandOf"/>
                <owl:allValuesFrom rdf:resource="https://saref.etsi.org/core/OpenCloseFunction"/>
            </owl:Restriction>
        </rdfs:subClassOf>
        <owl:disjointWith rdf:resource="https://saref.etsi.org/core/OpenCommand"/>
        <rdfs:comment xml:lang="en">A type of command</rdfs:comment>
        <rdfs:label xml:lang="en">Close command</rdfs:label>
    </owl:Class>
    


    <!-- https://saref.etsi.org/core/CloseState -->


    <owl:Class rdf:about="https://saref.etsi.org/core/CloseState">
        <rdfs:subClassOf rdf:resource="https://saref.etsi.org/core/OpenCloseState"/>
        <rdfs:comment xml:lang="en">The state of a device that is CLOSE</rdfs:comment>
        <rdfs:label xml:lang="en">Close state</rdfs:label>
    </owl:Class>
    


    <!-- https://saref.etsi.org/core/Coal -->


    <owl:Class rdf:about="https://saref.etsi.org/core/Coal">
        <rdfs:subClassOf rdf:resource="https://saref.etsi.org/core/Commodity"/>
        <rdfs:comment xml:lang="en">A type of commodity</rdfs:comment>
        <rdfs:label xml:lang="en">Coal</rdfs:label>
    </owl:Class>
    


    <!-- https://saref.etsi.org/core/Command -->


    <owl:Class rdf:about="https://saref.etsi.org/core/Command">
        <rdfs:subClassOf>
            <owl:Restriction>
                <owl:onProperty rdf:resource="https://saref.etsi.org/core/actsUpon"/>
                <owl:allValuesFrom rdf:resource="https://saref.etsi.org/core/State"/>
            </owl:Restriction>
        </rdfs:subClassOf>
        <rdfs:subClassOf>
            <owl:Restriction>
                <owl:onProperty rdf:resource="https://saref.etsi.org/core/isCommandOf"/>
                <owl:minQualifiedCardinality rdf:datatype="http://www.w3.org/2001/XMLSchema#nonNegativeInteger">1</owl:minQualifiedCardinality>
                <owl:onClass rdf:resource="https://saref.etsi.org/core/Function"/>
            </owl:Restriction>
        </rdfs:subClassOf>
        <rdfs:subClassOf>
            <owl:Restriction>
                <owl:onProperty rdf:resource="https://saref.etsi.org/core/hasDescription"/>
                <owl:maxCardinality rdf:datatype="http://www.w3.org/2001/XMLSchema#nonNegativeInteger">1</owl:maxCardinality>
            </owl:Restriction>
        </rdfs:subClassOf>
        <rdfs:comment xml:lang="en">A directive that a device must support to perform a certain function. A command may act upon a state, but does not necessarily act upon a state. For example, the ON command acts upon the ON/OFF state, but the GET command does not act upon any state, it simply gives a directive to retrieve a certain value. We propose here a list of commands that are relevant for the purpose of SAREF, but this list can be extended.</rdfs:comment>
        <rdfs:label xml:lang="en">Command</rdfs:label>
    </owl:Class>
    


    <!-- https://saref.etsi.org/core/Commodity -->


    <owl:Class rdf:about="https://saref.etsi.org/core/Commodity">
        <rdfs:comment xml:lang="en">A marketable item for which there is demand, but which is supplied without qualitative differentiation across a market. SAREF refers to energy commodities such as electricity, gas, coal and oil. </rdfs:comment>
        <rdfs:label xml:lang="en">Commodity</rdfs:label>
    </owl:Class>
    


    <!-- https://saref.etsi.org/core/Currency -->


    <owl:Class rdf:about="https://saref.etsi.org/core/Currency">
        <rdfs:subClassOf rdf:resource="https://saref.etsi.org/core/UnitOfMeasure"/>
        <rdfs:comment xml:lang="en">The class of units of measure for price</rdfs:comment>
        <rdfs:label xml:lang="en">Currency</rdfs:label>
    </owl:Class>
    


    <!-- https://saref.etsi.org/core/Device -->


    <owl:Class rdf:about="https://saref.etsi.org/core/Device">
        <rdfs:subClassOf rdf:resource="http://www.w3.org/ns/ssn/System"/>
        <rdfs:subClassOf rdf:resource="https://saref.etsi.org/saref4bldg/PhysicalObject"/>
        <rdfs:subClassOf>
            <owl:Restriction>
                <owl:onProperty rdf:resource="https://saref.etsi.org/core/consistsOf"/>
                <owl:allValuesFrom rdf:resource="https://saref.etsi.org/core/Device"/>
            </owl:Restriction>
        </rdfs:subClassOf>
        <rdfs:subClassOf>
            <owl:Restriction>
                <owl:onProperty rdf:resource="https://saref.etsi.org/core/controlsProperty"/>
                <owl:allValuesFrom rdf:resource="https://saref.etsi.org/core/Property"/>
            </owl:Restriction>
        </rdfs:subClassOf>
        <rdfs:subClassOf>
            <owl:Restriction>
                <owl:onProperty rdf:resource="https://saref.etsi.org/core/hasProfile"/>
                <owl:allValuesFrom rdf:resource="https://saref.etsi.org/core/Profile"/>
            </owl:Restriction>
        </rdfs:subClassOf>
        <rdfs:subClassOf>
            <owl:Restriction>
                <owl:onProperty rdf:resource="https://saref.etsi.org/core/hasState"/>
                <owl:allValuesFrom rdf:resource="https://saref.etsi.org/core/State"/>
            </owl:Restriction>
        </rdfs:subClassOf>
        <rdfs:subClassOf>
            <owl:Restriction>
                <owl:onProperty rdf:resource="https://saref.etsi.org/core/isUsedFor"/>
                <owl:allValuesFrom rdf:resource="https://saref.etsi.org/core/Commodity"/>
            </owl:Restriction>
        </rdfs:subClassOf>
        <rdfs:subClassOf>
            <owl:Restriction>
                <owl:onProperty rdf:resource="https://saref.etsi.org/core/makesMeasurement"/>
                <owl:allValuesFrom rdf:resource="https://saref.etsi.org/core/Measurement"/>
            </owl:Restriction>
        </rdfs:subClassOf>
        <rdfs:subClassOf>
            <owl:Restriction>
                <owl:onProperty rdf:resource="https://saref.etsi.org/core/measuresProperty"/>
                <owl:allValuesFrom rdf:resource="https://saref.etsi.org/core/Property"/>
            </owl:Restriction>
        </rdfs:subClassOf>
        <rdfs:subClassOf>
            <owl:Restriction>
                <owl:onProperty rdf:resource="https://saref.etsi.org/core/offers"/>
                <owl:allValuesFrom rdf:resource="https://saref.etsi.org/core/Service"/>
            </owl:Restriction>
        </rdfs:subClassOf>
        <rdfs:subClassOf>
            <owl:Restriction>
                <owl:onProperty rdf:resource="https://saref.etsi.org/core/accomplishes"/>
                <owl:minQualifiedCardinality rdf:datatype="http://www.w3.org/2001/XMLSchema#nonNegativeInteger">1</owl:minQualifiedCardinality>
                <owl:onClass rdf:resource="https://saref.etsi.org/core/Task"/>
            </owl:Restriction>
        </rdfs:subClassOf>
        <rdfs:subClassOf>
            <owl:Restriction>
                <owl:onProperty rdf:resource="https://saref.etsi.org/core/hasFunction"/>
                <owl:minQualifiedCardinality rdf:datatype="http://www.w3.org/2001/XMLSchema#nonNegativeInteger">1</owl:minQualifiedCardinality>
                <owl:onClass rdf:resource="https://saref.etsi.org/core/Function"/>
            </owl:Restriction>
        </rdfs:subClassOf>
        <rdfs:subClassOf>
            <owl:Restriction>
                <owl:onProperty rdf:resource="https://saref.etsi.org/core/hasManufacturer"/>
                <owl:maxCardinality rdf:datatype="http://www.w3.org/2001/XMLSchema#nonNegativeInteger">1</owl:maxCardinality>
            </owl:Restriction>
        </rdfs:subClassOf>
        <rdfs:subClassOf>
            <owl:Restriction>
                <owl:onProperty rdf:resource="https://saref.etsi.org/core/hasModel"/>
                <owl:maxCardinality rdf:datatype="http://www.w3.org/2001/XMLSchema#nonNegativeInteger">1</owl:maxCardinality>
            </owl:Restriction>
        </rdfs:subClassOf>
        <rdfs:comment xml:lang="en">A tangible object designed to accomplish a particular task in households, common public buildings or offices. In order to accomplish this task, the device performs one or more functions. For example, a washing machine is designed to wash (task) and to accomplish this task it performs a start and stop function. Devices can be structured in categories (subclasses) that reflect the different domain in which a device is used, e.g., smart appliances domain (subclass FunctionRelated) vs. building domain (subclass BuildingRelated) vs. smart grid domain (subclass EnergyRelated). New categories can be defined,if needed, to reflect other differences, for example different points of view, such as the point of view of the device&apos;s user vs. the point of view of the device&apos;s manufacturer. We propose a list of devices that are relevant for the purpose of SAREF, but this list can be extended.</rdfs:comment>
        <rdfs:comment xml:lang="en">A tangible object designed to accomplish a particular task in households, common public buildings or offices. In order to accomplish this task, the device performs one or more functions. For example, a washing machine is designed to wash (task) and to accomplish this task it performs the start and stop function.</rdfs:comment>
        <rdfs:comment xml:lang="en">A tangible object designed to accomplish a particular task. In order to accomplish this task, the device performs one or more functions. For example, a washing machine is designed to wash (task) and to accomplish this task it performs a start and stop function.</rdfs:comment>
        <rdfs:isDefinedBy rdf:resource="https://saref.etsi.org/core/"/>
        <rdfs:label xml:lang="en">Device</rdfs:label>
    </owl:Class>
    


    <!-- https://saref.etsi.org/core/DoorSwitch -->


    <owl:Class rdf:about="https://saref.etsi.org/core/DoorSwitch">
        <rdfs:subClassOf rdf:resource="https://saref.etsi.org/core/Switch"/>
        <rdfs:subClassOf>
            <owl:Restriction>
                <owl:onProperty rdf:resource="https://saref.etsi.org/core/hasFunction"/>
                <owl:someValuesFrom rdf:resource="https://saref.etsi.org/core/OpenCloseFunction"/>
            </owl:Restriction>
        </rdfs:subClassOf>
        <rdfs:subClassOf>
            <owl:Restriction>
                <owl:onProperty rdf:resource="https://saref.etsi.org/core/hasState"/>
                <owl:someValuesFrom rdf:resource="https://saref.etsi.org/core/OpenCloseState"/>
            </owl:Restriction>
        </rdfs:subClassOf>
        <rdfs:comment xml:lang="en">A switch that performs the saref:OpenCloseFunction, is used for controlling a door, and can be found in the state saref:OpenCloseState. A saref:DoorSwitch is typically used to accomplish saref:Safety.</rdfs:comment>
        <rdfs:label xml:lang="en">Door switch</rdfs:label>
    </owl:Class>
    


    <!-- https://saref.etsi.org/core/Electricity -->


    <owl:Class rdf:about="https://saref.etsi.org/core/Electricity">
        <rdfs:subClassOf rdf:resource="https://saref.etsi.org/core/Commodity"/>
        <rdfs:comment xml:lang="en">A type of commodity</rdfs:comment>
        <rdfs:label xml:lang="en">Electricity</rdfs:label>
    </owl:Class>
    


    <!-- https://saref.etsi.org/core/Energy -->


    <owl:Class rdf:about="https://saref.etsi.org/core/Energy">
        <rdfs:subClassOf rdf:resource="https://saref.etsi.org/core/Property"/>
        <rdfs:comment xml:lang="en">A saref:Property related to some measurements that are characterized by a certain value measured in an energy unit (such as Kilowatt_Hour or Watt_hour). Furter specializations of the saref:Energy class can be found in the SAREF4ENER extension, where classes such as EnergyMax, EnergyMin and EnergyExpected are defined. </rdfs:comment>
        <rdfs:label xml:lang="en">Energy</rdfs:label>
    </owl:Class>
    


    <!-- https://saref.etsi.org/core/EnergyUnit -->


    <owl:Class rdf:about="https://saref.etsi.org/core/EnergyUnit">
        <rdfs:subClassOf rdf:resource="https://saref.etsi.org/core/UnitOfMeasure"/>
        <rdfs:comment xml:lang="en">The unit of measure for energy</rdfs:comment>
        <rdfs:label xml:lang="en">Energy unit</rdfs:label>
    </owl:Class>
    


    <!-- https://saref.etsi.org/core/EventFunction -->


    <owl:Class rdf:about="https://saref.etsi.org/core/EventFunction">
        <rdfs:subClassOf rdf:resource="https://saref.etsi.org/core/Function"/>
        <rdfs:subClassOf>
            <owl:Restriction>
                <owl:onProperty rdf:resource="https://saref.etsi.org/core/hasThresholdMeasurement"/>
                <owl:minQualifiedCardinality rdf:datatype="http://www.w3.org/2001/XMLSchema#nonNegativeInteger">1</owl:minQualifiedCardinality>
                <owl:onClass rdf:resource="https://saref.etsi.org/core/Measurement"/>
            </owl:Restriction>
        </rdfs:subClassOf>
        <rdfs:comment xml:lang="en">A function that allows to notify about some relevant activity; e.g., that a certain threshold value has been exceeded or that some object has moved.</rdfs:comment>
        <rdfs:label xml:lang="en">Event function</rdfs:label>
    </owl:Class>
    


    <!-- https://saref.etsi.org/core/FeatureOfInterest -->


    <owl:Class rdf:about="https://saref.etsi.org/core/FeatureOfInterest">
        <rdfs:subClassOf>
            <owl:Restriction>
                <owl:onProperty rdf:resource="https://saref.etsi.org/core/hasMeasurement"/>
                <owl:allValuesFrom rdf:resource="https://saref.etsi.org/core/Measurement"/>
            </owl:Restriction>
        </rdfs:subClassOf>
        <rdfs:subClassOf>
            <owl:Restriction>
                <owl:onProperty rdf:resource="https://saref.etsi.org/core/hasProperty"/>
                <owl:allValuesFrom rdf:resource="https://saref.etsi.org/core/Property"/>
            </owl:Restriction>
        </rdfs:subClassOf>
        <rdfs:comment rdf:resource="https://saref.etsi.org/core/"/>
        <rdfs:comment xml:lang="en">A feature of interest represents any real world entity from which a property is measured.</rdfs:comment>
        <rdfs:isDefinedBy rdf:resource="https://saref.etsi.org/core/"/>
        <rdfs:label xml:lang="en">Feature of interest</rdfs:label>
    </owl:Class>
    


    <!-- https://saref.etsi.org/core/Function -->


    <owl:Class rdf:about="https://saref.etsi.org/core/Function">
        <rdfs:subClassOf>
            <owl:Restriction>
                <owl:onProperty rdf:resource="https://saref.etsi.org/core/hasCommand"/>
                <owl:minQualifiedCardinality rdf:datatype="http://www.w3.org/2001/XMLSchema#nonNegativeInteger">1</owl:minQualifiedCardinality>
                <owl:onClass rdf:resource="https://saref.etsi.org/core/Command"/>
            </owl:Restriction>
        </rdfs:subClassOf>
        <rdfs:comment xml:lang="en">The functionality necessary to accomplish the task for which a Device is designed. A device can be designed to perform more than one function. Functions can be structured in categories (subclasses) that reflect different points of view, for example, considering the specific application area for which a function can be used (e.g., light, temperature, motion, heat, power, etc.), or the capability that a function can support (e.g., receive, reply, notify, etc.), and so forth. </rdfs:comment>
        <rdfs:comment xml:lang="en">The functionality necessary to accomplish the task for which a device is designed. A device can be designed to perform more than one function. Functions can be structured in categories (subclasses) that reflect different points of view, for example, considering the specific application area for which a function can be used (e.g., light, temperature, motion, heat, power, etc.), or the capability that a function can support (e.g., receive, reply, notify, etc.), and so forth. </rdfs:comment>
        <rdfs:label xml:lang="en">Function</rdfs:label>
    </owl:Class>
    


    <!-- https://saref.etsi.org/core/Gas -->


    <owl:Class rdf:about="https://saref.etsi.org/core/Gas">
        <rdfs:subClassOf rdf:resource="https://saref.etsi.org/core/Commodity"/>
        <rdfs:comment xml:lang="en">A type of commodity</rdfs:comment>
        <rdfs:label xml:lang="en">Gas</rdfs:label>
    </owl:Class>
    


    <!-- https://saref.etsi.org/core/GetCommand -->


    <owl:Class rdf:about="https://saref.etsi.org/core/GetCommand">
        <rdfs:subClassOf rdf:resource="https://saref.etsi.org/core/Command"/>
        <rdfs:comment xml:lang="en">A type of command</rdfs:comment>
        <rdfs:label xml:lang="en">Get command</rdfs:label>
    </owl:Class>
    


    <!-- https://saref.etsi.org/core/GetCurrentMeterValueCommand -->


    <owl:Class rdf:about="https://saref.etsi.org/core/GetCurrentMeterValueCommand">
        <rdfs:subClassOf rdf:resource="https://saref.etsi.org/core/GetCommand"/>
        <rdfs:subClassOf>
            <owl:Restriction>
                <owl:onProperty rdf:resource="https://saref.etsi.org/core/isCommandOf"/>
                <owl:allValuesFrom rdf:resource="https://saref.etsi.org/core/MeteringFunction"/>
            </owl:Restriction>
        </rdfs:subClassOf>
        <rdfs:comment xml:lang="en">A type of get command</rdfs:comment>
        <rdfs:label xml:lang="en">Get current meter value command</rdfs:label>
    </owl:Class>
    


    <!-- https://saref.etsi.org/core/GetMeterDataCommand -->


    <owl:Class rdf:about="https://saref.etsi.org/core/GetMeterDataCommand">
        <rdfs:subClassOf rdf:resource="https://saref.etsi.org/core/GetCommand"/>
        <rdfs:subClassOf>
            <owl:Restriction>
                <owl:onProperty rdf:resource="https://saref.etsi.org/core/isCommandOf"/>
                <owl:allValuesFrom rdf:resource="https://saref.etsi.org/core/MeteringFunction"/>
            </owl:Restriction>
        </rdfs:subClassOf>
        <rdfs:comment xml:lang="en">A type of get command</rdfs:comment>
        <rdfs:label xml:lang="en">Get meter data command</rdfs:label>
    </owl:Class>
    


    <!-- https://saref.etsi.org/core/GetMeterHistoryCommand -->


    <owl:Class rdf:about="https://saref.etsi.org/core/GetMeterHistoryCommand">
        <rdfs:subClassOf rdf:resource="https://saref.etsi.org/core/GetCommand"/>
        <rdfs:subClassOf>
            <owl:Restriction>
                <owl:onProperty rdf:resource="https://saref.etsi.org/core/isCommandOf"/>
                <owl:allValuesFrom rdf:resource="https://saref.etsi.org/core/MeteringFunction"/>
            </owl:Restriction>
        </rdfs:subClassOf>
        <rdfs:comment xml:lang="en">A type of get command</rdfs:comment>
        <rdfs:label xml:lang="en">Get meter history command</rdfs:label>
    </owl:Class>
    


    <!-- https://saref.etsi.org/core/GetSensingDataCommand -->


    <owl:Class rdf:about="https://saref.etsi.org/core/GetSensingDataCommand">
        <rdfs:subClassOf rdf:resource="https://saref.etsi.org/core/GetCommand"/>
        <rdfs:subClassOf>
            <owl:Restriction>
                <owl:onProperty rdf:resource="https://saref.etsi.org/core/isCommandOf"/>
                <owl:allValuesFrom rdf:resource="https://saref.etsi.org/core/SensingFunction"/>
            </owl:Restriction>
        </rdfs:subClassOf>
        <rdfs:comment xml:lang="en">A type of get command</rdfs:comment>
        <rdfs:label xml:lang="en">Get sensing data command</rdfs:label>
    </owl:Class>
    


    <!-- https://saref.etsi.org/core/HVAC -->


    <owl:Class rdf:about="https://saref.etsi.org/core/HVAC">
        <rdfs:subClassOf rdf:resource="https://saref.etsi.org/core/Device"/>
        <rdfs:comment xml:lang="en">Heating, Ventilation and Air Conditioning (HVAC) device that provides indoor environmental comfort. A saref:HVAC is typically used to accomplish saref:Comfort.</rdfs:comment>
        <rdfs:label xml:lang="en">HVAC</rdfs:label>
    </owl:Class>
    


    <!-- https://saref.etsi.org/core/Humidity -->


    <owl:Class rdf:about="https://saref.etsi.org/core/Humidity">
        <rdfs:subClassOf rdf:resource="https://saref.etsi.org/core/Property"/>
        <rdfs:comment xml:lang="en">A saref:Property related to some measurements that are characterized by a certain value that is measured in a humidity unit</rdfs:comment>
        <rdfs:label xml:lang="en">Humidity</rdfs:label>
        <rdfs:label xml:lang="en">Humidiy</rdfs:label>
    </owl:Class>
    


    <!-- https://saref.etsi.org/core/IlluminanceUnit -->


    <owl:Class rdf:about="https://saref.etsi.org/core/IlluminanceUnit">
        <rdfs:subClassOf rdf:resource="https://saref.etsi.org/core/UnitOfMeasure"/>
        <rdfs:comment xml:lang="en">The unit of measure for light</rdfs:comment>
        <rdfs:label xml:lang="en">Illuminance unit</rdfs:label>
    </owl:Class>
    


    <!-- https://saref.etsi.org/core/LevelControlFunction -->


    <owl:Class rdf:about="https://saref.etsi.org/core/LevelControlFunction">
        <rdfs:subClassOf rdf:resource="https://saref.etsi.org/core/ActuatingFunction"/>
        <rdfs:comment xml:lang="en">An actuating function that allows to do level adjustments of a property in a certain range (e.g., 0%-100%), such as dimming a light in a room or setting the speed of an electric motor. </rdfs:comment>
        <rdfs:label xml:lang="en">Level control function</rdfs:label>
    </owl:Class>
    


    <!-- https://saref.etsi.org/core/Light -->


    <owl:Class rdf:about="https://saref.etsi.org/core/Light">
        <rdfs:subClassOf rdf:resource="https://saref.etsi.org/core/Property"/>
        <rdfs:comment xml:lang="en">A saref:Property related to some measurements that are characterized by a certain value that is measured in a illuminance unit (lux)</rdfs:comment>
        <rdfs:label xml:lang="en">Light</rdfs:label>
    </owl:Class>
    


    <!-- https://saref.etsi.org/core/LightSwitch -->


    <owl:Class rdf:about="https://saref.etsi.org/core/LightSwitch">
        <rdfs:subClassOf rdf:resource="https://saref.etsi.org/core/Switch"/>
        <rdfs:subClassOf>
            <owl:Restriction>
                <owl:onProperty rdf:resource="https://saref.etsi.org/core/controlsProperty"/>
                <owl:someValuesFrom rdf:resource="https://saref.etsi.org/core/Light"/>
            </owl:Restriction>
        </rdfs:subClassOf>
        <rdfs:subClassOf>
            <owl:Restriction>
                <owl:onProperty rdf:resource="https://saref.etsi.org/core/hasFunction"/>
                <owl:someValuesFrom rdf:resource="https://saref.etsi.org/core/OnOffFunction"/>
            </owl:Restriction>
        </rdfs:subClassOf>
        <rdfs:subClassOf>
            <owl:Restriction>
                <owl:onProperty rdf:resource="https://saref.etsi.org/core/hasState"/>
                <owl:someValuesFrom rdf:resource="https://saref.etsi.org/core/OnOffState"/>
            </owl:Restriction>
        </rdfs:subClassOf>
        <rdfs:subClassOf>
            <owl:Restriction>
                <owl:onProperty rdf:resource="https://saref.etsi.org/core/offers"/>
                <owl:someValuesFrom rdf:resource="https://saref.etsi.org/core/SwitchOnService"/>
            </owl:Restriction>
        </rdfs:subClassOf>
        <rdfs:comment xml:lang="en">A switch that performs the saref:OnOffFunction, controls the property saref:Light, and can be found in the state saref:OnOffState. It can offer a switch on service. A saref:LightSwitch is typically used to accomplish saref:Lighting.</rdfs:comment>
        <rdfs:label xml:lang="en">Light switch</rdfs:label>
    </owl:Class>
    


    <!-- https://saref.etsi.org/core/Measurement -->


    <owl:Class rdf:about="https://saref.etsi.org/core/Measurement">
        <rdfs:subClassOf>
            <owl:Restriction>
                <owl:onProperty rdf:resource="https://saref.etsi.org/core/isMeasuredIn"/>
                <owl:allValuesFrom rdf:resource="https://saref.etsi.org/core/UnitOfMeasure"/>
            </owl:Restriction>
        </rdfs:subClassOf>
        <rdfs:subClassOf>
            <owl:Restriction>
                <owl:onProperty rdf:resource="https://saref.etsi.org/core/isMeasurementOf"/>
                <owl:allValuesFrom rdf:resource="https://saref.etsi.org/core/FeatureOfInterest"/>
            </owl:Restriction>
        </rdfs:subClassOf>
        <rdfs:subClassOf>
            <owl:Restriction>
                <owl:onProperty rdf:resource="https://saref.etsi.org/core/relatesToProperty"/>
                <owl:allValuesFrom rdf:resource="https://saref.etsi.org/core/Property"/>
            </owl:Restriction>
        </rdfs:subClassOf>
        <rdfs:subClassOf>
            <owl:Restriction>
                <owl:onProperty rdf:resource="https://saref.etsi.org/core/isMeasuredIn"/>
                <owl:qualifiedCardinality rdf:datatype="http://www.w3.org/2001/XMLSchema#nonNegativeInteger">1</owl:qualifiedCardinality>
                <owl:onClass rdf:resource="https://saref.etsi.org/core/UnitOfMeasure"/>
            </owl:Restriction>
        </rdfs:subClassOf>
        <rdfs:subClassOf>
            <owl:Restriction>
                <owl:onProperty rdf:resource="https://saref.etsi.org/core/relatesToProperty"/>
                <owl:qualifiedCardinality rdf:datatype="http://www.w3.org/2001/XMLSchema#nonNegativeInteger">1</owl:qualifiedCardinality>
                <owl:onClass rdf:resource="https://saref.etsi.org/core/Property"/>
            </owl:Restriction>
        </rdfs:subClassOf>
        <rdfs:subClassOf>
            <owl:Restriction>
                <owl:onProperty rdf:resource="https://saref.etsi.org/core/hasTimestamp"/>
                <owl:allValuesFrom rdf:resource="http://www.w3.org/2001/XMLSchema#dateTime"/>
            </owl:Restriction>
        </rdfs:subClassOf>
        <rdfs:subClassOf>
            <owl:Restriction>
                <owl:onProperty rdf:resource="https://saref.etsi.org/core/hasValue"/>
                <owl:cardinality rdf:datatype="http://www.w3.org/2001/XMLSchema#nonNegativeInteger">1</owl:cardinality>
            </owl:Restriction>
        </rdfs:subClassOf>
        <rdfs:subClassOf>
            <owl:Restriction>
                <owl:onProperty rdf:resource="https://saref.etsi.org/core/hasValue"/>
                <owl:qualifiedCardinality rdf:datatype="http://www.w3.org/2001/XMLSchema#nonNegativeInteger">1</owl:qualifiedCardinality>
                <owl:onDataRange rdf:resource="http://www.w3.org/2001/XMLSchema#float"/>
            </owl:Restriction>
        </rdfs:subClassOf>
        <owl:disjointWith rdf:resource="https://saref.etsi.org/core/Property"/>
        <owl:disjointWith rdf:resource="https://saref.etsi.org/core/UnitOfMeasure"/>
        <rdfs:comment xml:lang="en">Represents the measured value made over a property. It is also linked to the unit of measure in which the value is expressed and the timestamp of the measurement.</rdfs:comment>
        <rdfs:isDefinedBy rdf:resource="https://saref.etsi.org/core/"/>
        <rdfs:isDefinedBy>https://saref.etsi.org/core/</rdfs:isDefinedBy>
        <rdfs:label xml:lang="en">Measurement</rdfs:label>
    </owl:Class>
    


    <!-- https://saref.etsi.org/core/Meter -->


    <owl:Class rdf:about="https://saref.etsi.org/core/Meter">
        <rdfs:subClassOf rdf:resource="https://saref.etsi.org/core/Device"/>
        <rdfs:subClassOf rdf:resource="https://saref.etsi.org/core/Sensor"/>
        <rdfs:subClassOf>
            <owl:Restriction>
                <owl:onProperty rdf:resource="https://saref.etsi.org/core/hasFunction"/>
                <owl:someValuesFrom rdf:resource="https://saref.etsi.org/core/MeteringFunction"/>
            </owl:Restriction>
        </rdfs:subClassOf>
        <rdfs:comment xml:lang="en">A device built to accurately detect and display a quantity in a form readable by a human being. Further, a device of category saref:Meter that performs a saref:MeteringFunction.</rdfs:comment>
        <rdfs:isDefinedBy rdf:resource="https://saref.etsi.org/core/"/>
        <rdfs:label xml:lang="en">Meter</rdfs:label>
    </owl:Class>
    


    <!-- https://saref.etsi.org/core/MeteringFunction -->


    <owl:Class rdf:about="https://saref.etsi.org/core/MeteringFunction">
        <rdfs:subClassOf rdf:resource="https://saref.etsi.org/core/Function"/>
        <rdfs:subClassOf>
            <owl:Restriction>
                <owl:onProperty rdf:resource="https://saref.etsi.org/core/hasMeterReading"/>
                <owl:allValuesFrom rdf:resource="https://saref.etsi.org/core/Measurement"/>
            </owl:Restriction>
        </rdfs:subClassOf>
        <rdfs:subClassOf>
            <owl:Restriction>
                <owl:onProperty rdf:resource="https://saref.etsi.org/core/hasMeterReadingType"/>
                <owl:allValuesFrom>
                    <owl:Class>
                        <owl:unionOf rdf:parseType="Collection">
                            <rdf:Description rdf:about="https://saref.etsi.org/core/Commodity"/>
                            <rdf:Description rdf:about="https://saref.etsi.org/core/Property"/>
                        </owl:unionOf>
                    </owl:Class>
                </owl:allValuesFrom>
            </owl:Restriction>
        </rdfs:subClassOf>
        <rdfs:comment xml:lang="en">A function that allows to get data from a meter, such as current meter reading or instantaneous demand</rdfs:comment>
        <rdfs:label xml:lang="en">Metering function</rdfs:label>
    </owl:Class>
    


    <!-- https://saref.etsi.org/core/Motion -->


    <owl:Class rdf:about="https://saref.etsi.org/core/Motion">
        <rdfs:subClassOf rdf:resource="https://saref.etsi.org/core/Property"/>
        <rdfs:comment xml:lang="en">A saref:Property related to some measurements that are characterized by a certain value that is measured in a unit of measure for motion</rdfs:comment>
        <rdfs:label xml:lang="en">Motion</rdfs:label>
    </owl:Class>
    


    <!-- https://saref.etsi.org/core/MultiLevelState -->


    <owl:Class rdf:about="https://saref.etsi.org/core/MultiLevelState">
        <rdfs:subClassOf rdf:resource="https://saref.etsi.org/core/State"/>
        <rdfs:comment xml:lang="en">A type of state</rdfs:comment>
        <rdfs:label xml:lang="en">Multi level state</rdfs:label>
    </owl:Class>
    


    <!-- https://saref.etsi.org/core/NotifyCommand -->


    <owl:Class rdf:about="https://saref.etsi.org/core/NotifyCommand">
        <rdfs:subClassOf rdf:resource="https://saref.etsi.org/core/Command"/>
        <rdfs:subClassOf>
            <owl:Restriction>
                <owl:onProperty rdf:resource="https://saref.etsi.org/core/isCommandOf"/>
                <owl:allValuesFrom rdf:resource="https://saref.etsi.org/core/EventFunction"/>
            </owl:Restriction>
        </rdfs:subClassOf>
        <rdfs:comment xml:lang="en">A type of command</rdfs:comment>
        <rdfs:label xml:lang="en">Notify command</rdfs:label>
    </owl:Class>
    


    <!-- https://saref.etsi.org/core/Occupancy -->


    <owl:Class rdf:about="https://saref.etsi.org/core/Occupancy">
        <rdfs:subClassOf rdf:resource="https://saref.etsi.org/core/Property"/>
        <rdfs:comment xml:lang="en">A saref:Property related to some measurements that are characterized by a certain value (saref:hasValue property) that is measured in a unit of measure for occupancy</rdfs:comment>
        <rdfs:label xml:lang="en">Occupancy</rdfs:label>
    </owl:Class>
    


    <!-- https://saref.etsi.org/core/OffCommand -->


    <owl:Class rdf:about="https://saref.etsi.org/core/OffCommand">
        <rdfs:subClassOf rdf:resource="https://saref.etsi.org/core/Command"/>
        <rdfs:subClassOf>
            <owl:Restriction>
                <owl:onProperty rdf:resource="https://saref.etsi.org/core/actsUpon"/>
                <owl:someValuesFrom rdf:resource="https://saref.etsi.org/core/OnOffState"/>
            </owl:Restriction>
        </rdfs:subClassOf>
        <rdfs:subClassOf>
            <owl:Restriction>
                <owl:onProperty rdf:resource="https://saref.etsi.org/core/isCommandOf"/>
                <owl:allValuesFrom rdf:resource="https://saref.etsi.org/core/OnOffFunction"/>
            </owl:Restriction>
        </rdfs:subClassOf>
        <owl:disjointWith rdf:resource="https://saref.etsi.org/core/OnCommand"/>
        <rdfs:comment xml:lang="en">A type of command</rdfs:comment>
        <rdfs:label xml:lang="en">Off command</rdfs:label>
    </owl:Class>
    


    <!-- https://saref.etsi.org/core/OffState -->


    <owl:Class rdf:about="https://saref.etsi.org/core/OffState">
        <rdfs:subClassOf rdf:resource="https://saref.etsi.org/core/OnOffState"/>
        <rdfs:comment xml:lang="en">The state of a device that is Off</rdfs:comment>
        <rdfs:label xml:lang="en">Off state</rdfs:label>
    </owl:Class>
    


    <!-- https://saref.etsi.org/core/OnCommand -->


    <owl:Class rdf:about="https://saref.etsi.org/core/OnCommand">
        <rdfs:subClassOf rdf:resource="https://saref.etsi.org/core/Command"/>
        <rdfs:subClassOf>
            <owl:Restriction>
                <owl:onProperty rdf:resource="https://saref.etsi.org/core/actsUpon"/>
                <owl:someValuesFrom rdf:resource="https://saref.etsi.org/core/OnOffState"/>
            </owl:Restriction>
        </rdfs:subClassOf>
        <rdfs:subClassOf>
            <owl:Restriction>
                <owl:onProperty rdf:resource="https://saref.etsi.org/core/isCommandOf"/>
                <owl:allValuesFrom rdf:resource="https://saref.etsi.org/core/OnOffFunction"/>
            </owl:Restriction>
        </rdfs:subClassOf>
        <rdfs:comment xml:lang="en">A type of command</rdfs:comment>
        <rdfs:label xml:lang="en">On command</rdfs:label>
    </owl:Class>
    


    <!-- https://saref.etsi.org/core/OnOffFunction -->


    <owl:Class rdf:about="https://saref.etsi.org/core/OnOffFunction">
        <rdfs:subClassOf rdf:resource="https://saref.etsi.org/core/ActuatingFunction"/>
        <rdfs:comment xml:lang="en">An actuating function that allows to switch on and off an actuator</rdfs:comment>
        <rdfs:label xml:lang="en">On off function</rdfs:label>
    </owl:Class>
    


    <!-- https://saref.etsi.org/core/OnOffState -->


    <owl:Class rdf:about="https://saref.etsi.org/core/OnOffState">
        <rdfs:subClassOf rdf:resource="https://saref.etsi.org/core/State"/>
        <rdfs:comment xml:lang="en">A type of state</rdfs:comment>
        <rdfs:label xml:lang="en">On off state</rdfs:label>
    </owl:Class>
    


    <!-- https://saref.etsi.org/core/OnState -->


    <owl:Class rdf:about="https://saref.etsi.org/core/OnState">
        <rdfs:subClassOf rdf:resource="https://saref.etsi.org/core/OnOffState"/>
        <rdfs:comment xml:lang="en">The state of a device that is On</rdfs:comment>
        <rdfs:label xml:lang="en">On state</rdfs:label>
    </owl:Class>
    


    <!-- https://saref.etsi.org/core/OpenCloseFunction -->


    <owl:Class rdf:about="https://saref.etsi.org/core/OpenCloseFunction">
        <rdfs:subClassOf rdf:resource="https://saref.etsi.org/core/ActuatingFunction"/>
        <rdfs:comment xml:lang="en">An actuating function that allows to open and close a device</rdfs:comment>
        <rdfs:label xml:lang="en">Open close function</rdfs:label>
    </owl:Class>
    


    <!-- https://saref.etsi.org/core/OpenCloseState -->


    <owl:Class rdf:about="https://saref.etsi.org/core/OpenCloseState">
        <rdfs:subClassOf rdf:resource="https://saref.etsi.org/core/State"/>
        <rdfs:comment xml:lang="en">A type of state</rdfs:comment>
        <rdfs:label xml:lang="en">Open close state</rdfs:label>
    </owl:Class>
    


    <!-- https://saref.etsi.org/core/OpenCommand -->


    <owl:Class rdf:about="https://saref.etsi.org/core/OpenCommand">
        <rdfs:subClassOf rdf:resource="https://saref.etsi.org/core/Command"/>
        <rdfs:subClassOf>
            <owl:Restriction>
                <owl:onProperty rdf:resource="https://saref.etsi.org/core/actsUpon"/>
                <owl:someValuesFrom rdf:resource="https://saref.etsi.org/core/OpenCloseState"/>
            </owl:Restriction>
        </rdfs:subClassOf>
        <rdfs:subClassOf>
            <owl:Restriction>
                <owl:onProperty rdf:resource="https://saref.etsi.org/core/isCommandOf"/>
                <owl:allValuesFrom rdf:resource="https://saref.etsi.org/core/OpenCloseFunction"/>
            </owl:Restriction>
        </rdfs:subClassOf>
        <rdfs:comment xml:lang="en">A type of command</rdfs:comment>
        <rdfs:label xml:lang="en">Open command</rdfs:label>
    </owl:Class>
    


    <!-- https://saref.etsi.org/core/OpenState -->


    <owl:Class rdf:about="https://saref.etsi.org/core/OpenState">
        <rdfs:subClassOf rdf:resource="https://saref.etsi.org/core/OpenCloseState"/>
        <rdfs:comment xml:lang="en">The state of a device that is OPEN </rdfs:comment>
        <rdfs:label xml:lang="en">Open state</rdfs:label>
    </owl:Class>
    


    <!-- https://saref.etsi.org/core/PauseCommand -->


    <owl:Class rdf:about="https://saref.etsi.org/core/PauseCommand">
        <rdfs:subClassOf rdf:resource="https://saref.etsi.org/core/Command"/>
        <rdfs:comment xml:lang="en">A type of command</rdfs:comment>
        <rdfs:label xml:lang="en">Pause command</rdfs:label>
    </owl:Class>
    


    <!-- https://saref.etsi.org/core/Power -->


    <owl:Class rdf:about="https://saref.etsi.org/core/Power">
        <rdfs:subClassOf rdf:resource="https://saref.etsi.org/core/Property"/>
        <rdfs:comment xml:lang="en">A saref:Property related to some measurements that are characterized by a certain value that is measured in a power unit (such as watt or kilowatt).  Further specializations of the saref:Power class can be found in the SAREF4ENER extension, where classes such as PowerMax, PowerMin and PowerExpected are defined.</rdfs:comment>
        <rdfs:label xml:lang="en">Power</rdfs:label>
    </owl:Class>
    


    <!-- https://saref.etsi.org/core/PowerUnit -->


    <owl:Class rdf:about="https://saref.etsi.org/core/PowerUnit">
        <rdfs:subClassOf rdf:resource="https://saref.etsi.org/core/UnitOfMeasure"/>
        <rdfs:comment xml:lang="en">The unit of measure for power</rdfs:comment>
        <rdfs:label xml:lang="en">Power unit</rdfs:label>
    </owl:Class>
    


    <!-- https://saref.etsi.org/core/Pressure -->


    <owl:Class rdf:about="https://saref.etsi.org/core/Pressure">
        <rdfs:subClassOf rdf:resource="https://saref.etsi.org/core/Property"/>
        <rdfs:comment xml:lang="en">A saref:Property related to some measurements that are characterized by a certain value that is measured in a pressure unit (bar or pascal)</rdfs:comment>
        <rdfs:label xml:lang="en">Pressure</rdfs:label>
    </owl:Class>
    


    <!-- https://saref.etsi.org/core/PressureUnit -->


    <owl:Class rdf:about="https://saref.etsi.org/core/PressureUnit">
        <rdfs:subClassOf rdf:resource="https://saref.etsi.org/core/UnitOfMeasure"/>
        <rdfs:comment xml:lang="en">The unit of measure for pressure</rdfs:comment>
        <rdfs:label xml:lang="en">Pressure unit</rdfs:label>
    </owl:Class>
    


    <!-- https://saref.etsi.org/core/Price -->


    <owl:Class rdf:about="https://saref.etsi.org/core/Price">
        <rdfs:subClassOf rdf:resource="https://saref.etsi.org/core/Property"/>
        <rdfs:comment xml:lang="en">A saref:Property crelated to some measurements that are characterized by a certain value that is measured using saref:Currency</rdfs:comment>
        <rdfs:label xml:lang="en">Price</rdfs:label>
    </owl:Class>
    


    <!-- https://saref.etsi.org/core/Profile -->


    <owl:Class rdf:about="https://saref.etsi.org/core/Profile">
        <rdfs:subClassOf>
            <owl:Restriction>
                <owl:onProperty rdf:resource="https://saref.etsi.org/core/consistsOf"/>
                <owl:allValuesFrom rdf:resource="https://saref.etsi.org/core/Profile"/>
            </owl:Restriction>
        </rdfs:subClassOf>
        <rdfs:subClassOf>
            <owl:Restriction>
                <owl:onProperty rdf:resource="https://saref.etsi.org/core/hasPrice"/>
                <owl:allValuesFrom rdf:resource="https://saref.etsi.org/core/Price"/>
            </owl:Restriction>
        </rdfs:subClassOf>
        <rdfs:subClassOf>
            <owl:Restriction>
                <owl:onProperty rdf:resource="https://saref.etsi.org/core/hasTime"/>
                <owl:allValuesFrom rdf:resource="https://saref.etsi.org/core/Time"/>
            </owl:Restriction>
        </rdfs:subClassOf>
        <rdfs:subClassOf>
            <owl:Restriction>
                <owl:onProperty rdf:resource="https://saref.etsi.org/core/isAbout"/>
                <owl:allValuesFrom>
                    <owl:Class>
                        <owl:unionOf rdf:parseType="Collection">
                            <rdf:Description rdf:about="https://saref.etsi.org/core/Commodity"/>
                            <rdf:Description rdf:about="https://saref.etsi.org/core/Property"/>
                        </owl:unionOf>
                    </owl:Class>
                </owl:allValuesFrom>
            </owl:Restriction>
        </rdfs:subClassOf>
        <rdfs:comment xml:lang="en">A specification associated to a device to collect information about a certain Property (e.g., Energy) for optimizing its usage in the home, office or building in which the device is located. This specification is about a certain Property (saref:isAbout), can be calculated over a time span (saref:hasTime) and can be associated to some costs (saref:hasPrice). An example is the Power Profile defined in the SAREF4ENER extension that can be associated to a device for optimizing the Energy efficiency in the home, office or building in which the device is located.</rdfs:comment>
        <rdfs:label xml:lang="en">Profile</rdfs:label>
    </owl:Class>
    


    <!-- https://saref.etsi.org/core/Property -->


    <owl:Class rdf:about="https://saref.etsi.org/core/Property">
        <rdfs:subClassOf>
            <owl:Restriction>
                <owl:onProperty rdf:resource="https://saref.etsi.org/core/isControlledByDevice"/>
                <owl:allValuesFrom rdf:resource="https://saref.etsi.org/core/Device"/>
            </owl:Restriction>
        </rdfs:subClassOf>
        <rdfs:subClassOf>
            <owl:Restriction>
                <owl:onProperty rdf:resource="https://saref.etsi.org/core/isMeasuredByDevice"/>
                <owl:allValuesFrom rdf:resource="https://saref.etsi.org/core/Device"/>
            </owl:Restriction>
        </rdfs:subClassOf>
        <rdfs:subClassOf>
            <owl:Restriction>
                <owl:onProperty rdf:resource="https://saref.etsi.org/core/isPropertyOf"/>
                <owl:allValuesFrom rdf:resource="https://saref.etsi.org/core/FeatureOfInterest"/>
            </owl:Restriction>
        </rdfs:subClassOf>
        <rdfs:subClassOf>
            <owl:Restriction>
                <owl:onProperty rdf:resource="https://saref.etsi.org/core/relatesToMeasurement"/>
                <owl:allValuesFrom rdf:resource="https://saref.etsi.org/core/Measurement"/>
            </owl:Restriction>
        </rdfs:subClassOf>
        <owl:disjointWith rdf:resource="https://saref.etsi.org/core/UnitOfMeasure"/>
        <rdfs:comment xml:lang="en">A quality of a feature of interest that can be measured; an aspect of a feature of interest that is intrinsic to and cannot exist without the feature</rdfs:comment>
        <rdfs:comment xml:lang="en">An aspect of an entity that can be observable by a sensor.</rdfs:comment>
        <rdfs:comment xml:lang="en">Anything that can be sensed, measured or controlled in households, common public buildings or offices. We propose here a list of properties that are relevant for the purpose of SAREF, but this list can be extended.</rdfs:comment>
        <rdfs:isDefinedBy rdf:resource="https://saref.etsi.org/core/"/>
        <rdfs:isDefinedBy>https://saref.etsi.org/core/</rdfs:isDefinedBy>
        <rdfs:label xml:lang="en">Property</rdfs:label>
    </owl:Class>
    


    <!-- https://saref.etsi.org/core/SensingFunction -->


    <owl:Class rdf:about="https://saref.etsi.org/core/SensingFunction">
        <rdfs:subClassOf rdf:resource="https://saref.etsi.org/core/Function"/>
        <rdfs:subClassOf>
            <owl:Restriction>
                <owl:onProperty rdf:resource="https://saref.etsi.org/core/hasSensingRange"/>
                <owl:someValuesFrom rdf:resource="https://saref.etsi.org/core/Measurement"/>
            </owl:Restriction>
        </rdfs:subClassOf>
        <rdfs:subClassOf>
            <owl:Restriction>
                <owl:onProperty rdf:resource="https://saref.etsi.org/core/hasSensorType"/>
                <owl:allValuesFrom rdf:resource="https://saref.etsi.org/core/Property"/>
            </owl:Restriction>
        </rdfs:subClassOf>
        <rdfs:comment xml:lang="en">A function that allows to transmit data from sensors, such as measurement values (e.g., temperature) or sensing data (e.g., occupancy)</rdfs:comment>
        <rdfs:label xml:lang="en">Sensing function</rdfs:label>
    </owl:Class>
    


    <!-- https://saref.etsi.org/core/Sensor -->


    <owl:Class rdf:about="https://saref.etsi.org/core/Sensor">
        <rdfs:subClassOf rdf:resource="https://saref.etsi.org/core/Device"/>
        <rdfs:subClassOf>
            <owl:Restriction>
                <owl:onProperty rdf:resource="https://saref.etsi.org/core/hasFunction"/>
                <owl:someValuesFrom rdf:resource="https://saref.etsi.org/core/SensingFunction"/>
            </owl:Restriction>
        </rdfs:subClassOf>
        <rdfs:comment xml:lang="en">A device that detects and responds to events or changes in the physical environment such as light, motion, or temperature changes.
A device that has category saref:Sensor and performs a saref:SensingFunction.</rdfs:comment>
        <rdfs:comment xml:lang="en">A device that detects and responds to events or changes in the physical environment such as light, motion, or temperature changes. A device that has category saref:Sensor and performs a saref:SensingFunction.</rdfs:comment>
        <rdfs:comment xml:lang="en">A device that detects and responds to events or changes in the physical environment such as light, motion, or temperature changes. Further, a device of category saref:Sensor that performs a saref:SensingFunction.</rdfs:comment>
        <rdfs:isDefinedBy rdf:resource="https://saref.etsi.org/core/"/>
        <rdfs:label xml:lang="en">Sensor</rdfs:label>
    </owl:Class>
    


    <!-- https://saref.etsi.org/core/Service -->


    <owl:Class rdf:about="https://saref.etsi.org/core/Service">
        <rdfs:subClassOf>
            <owl:Restriction>
                <owl:onProperty rdf:resource="https://saref.etsi.org/core/isOfferedBy"/>
                <owl:minQualifiedCardinality rdf:datatype="http://www.w3.org/2001/XMLSchema#nonNegativeInteger">1</owl:minQualifiedCardinality>
                <owl:onClass rdf:resource="https://saref.etsi.org/core/Device"/>
            </owl:Restriction>
        </rdfs:subClassOf>
        <rdfs:subClassOf>
            <owl:Restriction>
                <owl:onProperty rdf:resource="https://saref.etsi.org/core/represents"/>
                <owl:minQualifiedCardinality rdf:datatype="http://www.w3.org/2001/XMLSchema#nonNegativeInteger">1</owl:minQualifiedCardinality>
                <owl:onClass rdf:resource="https://saref.etsi.org/core/Function"/>
            </owl:Restriction>
        </rdfs:subClassOf>
        <rdfs:comment xml:lang="en">A service is a representation of a function to a network that makes the function discoverable, registerable, remotely controllable by other devices in the network. A service can represent one or more functions. A Service is offered by a device that wants (a certain set of) its function(s) to be discoverable, registerable, remotely controllable by other devices in the network. A Service must specify the device that is offering the service and the function(s) to be represented.</rdfs:comment>
        <rdfs:label xml:lang="en">Service</rdfs:label>
    </owl:Class>
    


    <!-- https://saref.etsi.org/core/SetAbsoluteLevelCommand -->


    <owl:Class rdf:about="https://saref.etsi.org/core/SetAbsoluteLevelCommand">
        <rdfs:subClassOf rdf:resource="https://saref.etsi.org/core/SetLevelCommand"/>
        <rdfs:comment xml:lang="en">A type of set level command</rdfs:comment>
        <rdfs:label xml:lang="en">Set absolute level command</rdfs:label>
    </owl:Class>
    


    <!-- https://saref.etsi.org/core/SetLevelCommand -->


    <owl:Class rdf:about="https://saref.etsi.org/core/SetLevelCommand">
        <rdfs:subClassOf rdf:resource="https://saref.etsi.org/core/Command"/>
        <rdfs:subClassOf>
            <owl:Restriction>
                <owl:onProperty rdf:resource="https://saref.etsi.org/core/actsUpon"/>
                <owl:someValuesFrom rdf:resource="https://saref.etsi.org/core/MultiLevelState"/>
            </owl:Restriction>
        </rdfs:subClassOf>
        <rdfs:subClassOf>
            <owl:Restriction>
                <owl:onProperty rdf:resource="https://saref.etsi.org/core/isCommandOf"/>
                <owl:allValuesFrom rdf:resource="https://saref.etsi.org/core/LevelControlFunction"/>
            </owl:Restriction>
        </rdfs:subClassOf>
        <rdfs:comment xml:lang="en">A type of command</rdfs:comment>
        <rdfs:label xml:lang="en">Set level command</rdfs:label>
    </owl:Class>
    


    <!-- https://saref.etsi.org/core/SetRelativeLevelCommand -->


    <owl:Class rdf:about="https://saref.etsi.org/core/SetRelativeLevelCommand">
        <rdfs:subClassOf rdf:resource="https://saref.etsi.org/core/SetLevelCommand"/>
        <rdfs:comment xml:lang="en">A type of set level command</rdfs:comment>
        <rdfs:label xml:lang="en">Set relative level command</rdfs:label>
    </owl:Class>
    


    <!-- https://saref.etsi.org/core/Smoke -->


    <owl:Class rdf:about="https://saref.etsi.org/core/Smoke">
        <rdfs:subClassOf rdf:resource="https://saref.etsi.org/core/Property"/>
        <rdfs:comment xml:lang="en">A saref:Property related to some measurements that are characterized by a certain value that is measured in a unit of measure for smoke</rdfs:comment>
        <rdfs:label xml:lang="en">Smoke</rdfs:label>
    </owl:Class>
    


    <!-- https://saref.etsi.org/core/SmokeSensor -->


    <owl:Class rdf:about="https://saref.etsi.org/core/SmokeSensor">
        <rdfs:subClassOf rdf:resource="https://saref.etsi.org/core/Sensor"/>
        <rdfs:subClassOf>
            <owl:Restriction>
                <owl:onProperty rdf:resource="https://saref.etsi.org/core/hasFunction"/>
                <owl:someValuesFrom rdf:resource="https://saref.etsi.org/core/EventFunction"/>
            </owl:Restriction>
        </rdfs:subClassOf>
        <rdfs:subClassOf>
            <owl:Restriction>
                <owl:onProperty rdf:resource="https://saref.etsi.org/core/hasFunction"/>
                <owl:someValuesFrom rdf:resource="https://saref.etsi.org/core/SensingFunction"/>
            </owl:Restriction>
        </rdfs:subClassOf>
        <rdfs:subClassOf>
            <owl:Restriction>
                <owl:onProperty rdf:resource="https://saref.etsi.org/core/measuresProperty"/>
                <owl:someValuesFrom rdf:resource="https://saref.etsi.org/core/Smoke"/>
            </owl:Restriction>
        </rdfs:subClassOf>
        <rdfs:comment xml:lang="en">A sensor that performs the saref:SensingFunction and the saref:EventFunction, and is used for the purpose of sensing a property of type saref:Smoke. A saref:SmokeSensor is typically used to saref:accomplish saref:Safety.</rdfs:comment>
        <rdfs:label xml:lang="en">Smoke sensor</rdfs:label>
    </owl:Class>
    


    <!-- https://saref.etsi.org/core/StartCommand -->


    <owl:Class rdf:about="https://saref.etsi.org/core/StartCommand">
        <rdfs:subClassOf rdf:resource="https://saref.etsi.org/core/Command"/>
        <rdfs:subClassOf>
            <owl:Restriction>
                <owl:onProperty rdf:resource="https://saref.etsi.org/core/actsUpon"/>
                <owl:someValuesFrom rdf:resource="https://saref.etsi.org/core/StartStopState"/>
            </owl:Restriction>
        </rdfs:subClassOf>
        <rdfs:subClassOf>
            <owl:Restriction>
                <owl:onProperty rdf:resource="https://saref.etsi.org/core/isCommandOf"/>
                <owl:allValuesFrom rdf:resource="https://saref.etsi.org/core/StartStopFunction"/>
            </owl:Restriction>
        </rdfs:subClassOf>
        <owl:disjointWith rdf:resource="https://saref.etsi.org/core/StopCommand"/>
        <rdfs:comment xml:lang="en">A type of command</rdfs:comment>
        <rdfs:label xml:lang="en">Start command</rdfs:label>
    </owl:Class>
    


    <!-- https://saref.etsi.org/core/StartState -->


    <owl:Class rdf:about="https://saref.etsi.org/core/StartState">
        <rdfs:subClassOf rdf:resource="https://saref.etsi.org/core/StartStopState"/>
        <rdfs:comment xml:lang="en">The state of a device that is STARTED</rdfs:comment>
        <rdfs:label xml:lang="en">Start state</rdfs:label>
    </owl:Class>
    


    <!-- https://saref.etsi.org/core/StartStopFunction -->


    <owl:Class rdf:about="https://saref.etsi.org/core/StartStopFunction">
        <rdfs:subClassOf rdf:resource="https://saref.etsi.org/core/ActuatingFunction"/>
        <rdfs:comment xml:lang="en">An actuating function that allows to start and stop a device</rdfs:comment>
        <rdfs:label xml:lang="en">Start stop function</rdfs:label>
    </owl:Class>
    


    <!-- https://saref.etsi.org/core/StartStopState -->


    <owl:Class rdf:about="https://saref.etsi.org/core/StartStopState">
        <rdfs:subClassOf rdf:resource="https://saref.etsi.org/core/State"/>
        <rdfs:comment xml:lang="en">A type of state</rdfs:comment>
        <rdfs:label xml:lang="en">Start stop state</rdfs:label>
    </owl:Class>
    


    <!-- https://saref.etsi.org/core/State -->


    <owl:Class rdf:about="https://saref.etsi.org/core/State">
        <rdfs:comment xml:lang="en">The state in which a device can be found, e.g, ON/OFF/STANDBY, or ONLINE/OFFLINE. We propose here a list of states that are relevant for the purpose of SAREF, but this list can be extended.</rdfs:comment>
        <rdfs:label xml:lang="en">State</rdfs:label>
    </owl:Class>
    


    <!-- https://saref.etsi.org/core/StepDownCommand -->


    <owl:Class rdf:about="https://saref.etsi.org/core/StepDownCommand">
        <rdfs:subClassOf rdf:resource="https://saref.etsi.org/core/Command"/>
        <rdfs:subClassOf>
            <owl:Restriction>
                <owl:onProperty rdf:resource="https://saref.etsi.org/core/actsUpon"/>
                <owl:someValuesFrom rdf:resource="https://saref.etsi.org/core/MultiLevelState"/>
            </owl:Restriction>
        </rdfs:subClassOf>
        <rdfs:subClassOf>
            <owl:Restriction>
                <owl:onProperty rdf:resource="https://saref.etsi.org/core/isCommandOf"/>
                <owl:allValuesFrom rdf:resource="https://saref.etsi.org/core/LevelControlFunction"/>
            </owl:Restriction>
        </rdfs:subClassOf>
        <owl:disjointWith rdf:resource="https://saref.etsi.org/core/StepUpCommand"/>
        <rdfs:comment xml:lang="en">A type of command</rdfs:comment>
        <rdfs:label xml:lang="en">Step down command</rdfs:label>
    </owl:Class>
    


    <!-- https://saref.etsi.org/core/StepUpCommand -->


    <owl:Class rdf:about="https://saref.etsi.org/core/StepUpCommand">
        <rdfs:subClassOf rdf:resource="https://saref.etsi.org/core/Command"/>
        <rdfs:subClassOf>
            <owl:Restriction>
                <owl:onProperty rdf:resource="https://saref.etsi.org/core/actsUpon"/>
                <owl:someValuesFrom rdf:resource="https://saref.etsi.org/core/MultiLevelState"/>
            </owl:Restriction>
        </rdfs:subClassOf>
        <rdfs:subClassOf>
            <owl:Restriction>
                <owl:onProperty rdf:resource="https://saref.etsi.org/core/isCommandOf"/>
                <owl:allValuesFrom rdf:resource="https://saref.etsi.org/core/LevelControlFunction"/>
            </owl:Restriction>
        </rdfs:subClassOf>
        <rdfs:comment xml:lang="en">A type of command</rdfs:comment>
        <rdfs:label xml:lang="en">Step up command</rdfs:label>
    </owl:Class>
    


    <!-- https://saref.etsi.org/core/StopCommand -->


    <owl:Class rdf:about="https://saref.etsi.org/core/StopCommand">
        <rdfs:subClassOf rdf:resource="https://saref.etsi.org/core/Command"/>
        <rdfs:subClassOf>
            <owl:Restriction>
                <owl:onProperty rdf:resource="https://saref.etsi.org/core/actsUpon"/>
                <owl:someValuesFrom rdf:resource="https://saref.etsi.org/core/StartStopState"/>
            </owl:Restriction>
        </rdfs:subClassOf>
        <rdfs:subClassOf>
            <owl:Restriction>
                <owl:onProperty rdf:resource="https://saref.etsi.org/core/isCommandOf"/>
                <owl:allValuesFrom rdf:resource="https://saref.etsi.org/core/StartStopFunction"/>
            </owl:Restriction>
        </rdfs:subClassOf>
        <rdfs:comment xml:lang="en">A type of command</rdfs:comment>
        <rdfs:label xml:lang="en">Stop command</rdfs:label>
    </owl:Class>
    


    <!-- https://saref.etsi.org/core/StopState -->


    <owl:Class rdf:about="https://saref.etsi.org/core/StopState">
        <rdfs:subClassOf rdf:resource="https://saref.etsi.org/core/StartStopState"/>
        <rdfs:comment xml:lang="en">The state of a device that is STOPPED</rdfs:comment>
        <rdfs:label xml:lang="en">Stop state</rdfs:label>
    </owl:Class>
    


    <!-- https://saref.etsi.org/core/Switch -->


    <owl:Class rdf:about="https://saref.etsi.org/core/Switch">
        <rdfs:subClassOf rdf:resource="https://saref.etsi.org/core/Actuator"/>
        <rdfs:comment xml:lang="en">A device of category saref:Actuator that performs an actuating function of type saref:OnOffFunction or saref:OpenCloseFunction</rdfs:comment>
        <rdfs:label xml:lang="en">Switch</rdfs:label>
    </owl:Class>
    


    <!-- https://saref.etsi.org/core/SwitchOnService -->


    <owl:Class rdf:about="https://saref.etsi.org/core/SwitchOnService">
        <rdfs:subClassOf rdf:resource="https://saref.etsi.org/core/Service"/>
        <rdfs:subClassOf>
            <owl:Restriction>
                <owl:onProperty rdf:resource="https://saref.etsi.org/core/isOfferedBy"/>
                <owl:someValuesFrom rdf:resource="https://saref.etsi.org/core/LightSwitch"/>
            </owl:Restriction>
        </rdfs:subClassOf>
        <rdfs:subClassOf>
            <owl:Restriction>
                <owl:onProperty rdf:resource="https://saref.etsi.org/core/represents"/>
                <owl:someValuesFrom rdf:resource="https://saref.etsi.org/core/OnOffFunction"/>
            </owl:Restriction>
        </rdfs:subClassOf>
        <rdfs:comment xml:lang="en">A type of service that represents an on/off function to the network</rdfs:comment>
        <rdfs:label xml:lang="en">Switch on service</rdfs:label>
    </owl:Class>
    


    <!-- https://saref.etsi.org/core/Task -->


    <owl:Class rdf:about="https://saref.etsi.org/core/Task">
        <rdfs:subClassOf>
            <owl:Restriction>
                <owl:onProperty rdf:resource="https://saref.etsi.org/core/isAccomplishedBy"/>
                <owl:minQualifiedCardinality rdf:datatype="http://www.w3.org/2001/XMLSchema#nonNegativeInteger">1</owl:minQualifiedCardinality>
                <owl:onClass rdf:resource="https://saref.etsi.org/core/Device"/>
            </owl:Restriction>
        </rdfs:subClassOf>
        <rdfs:comment xml:lang="en">The goal for which a device is designed (from a user perspective). For example, a washing machine is designed for the task of washing. We propose here a list of tasks that are relevant for the purpose of SAREF, but this list can be extended.</rdfs:comment>
        <rdfs:comment xml:lang="en">The goal for which a device is designed (from a user perspective). For example, a washing machine is designed for the task of washing. We propose here a list of tasks that are relevant for the purpose of SAREF, but this list can be extended. Tasks can be accomplished by devices (saref:isAccomplishedBy).</rdfs:comment>
        <rdfs:label xml:lang="en">Task</rdfs:label>
    </owl:Class>
    


    <!-- https://saref.etsi.org/core/Temperature -->


    <owl:Class rdf:about="https://saref.etsi.org/core/Temperature">
        <rdfs:subClassOf rdf:resource="https://saref.etsi.org/core/Property"/>
        <rdfs:comment xml:lang="en">A saref:Property related to some measurements that are characterized by a certain value that is measured in a temperature unit (degree_Celsius, degree_Fahrenheit, or degree_kelvin)</rdfs:comment>
        <rdfs:label xml:lang="en">Temperature</rdfs:label>
    </owl:Class>
    


    <!-- https://saref.etsi.org/core/TemperatureSensor -->


    <owl:Class rdf:about="https://saref.etsi.org/core/TemperatureSensor">
        <rdfs:subClassOf rdf:resource="https://saref.etsi.org/core/Sensor"/>
        <rdfs:subClassOf>
            <owl:Restriction>
                <owl:onProperty rdf:resource="https://saref.etsi.org/core/hasFunction"/>
                <owl:someValuesFrom rdf:resource="https://saref.etsi.org/core/SensingFunction"/>
            </owl:Restriction>
        </rdfs:subClassOf>
        <rdfs:subClassOf>
            <owl:Restriction>
                <owl:onProperty rdf:resource="https://saref.etsi.org/core/measuresProperty"/>
                <owl:someValuesFrom rdf:resource="https://saref.etsi.org/core/Temperature"/>
            </owl:Restriction>
        </rdfs:subClassOf>
        <rdfs:comment xml:lang="en">A sensor that is used for the purpose of sensing a property of type saref:Temperature. A saref:TemperatureSensor is typically used to saref:accomplish saref:Comfort.</rdfs:comment>
        <rdfs:label xml:lang="en">Temperature sensor</rdfs:label>
    </owl:Class>
    


    <!-- https://saref.etsi.org/core/TemperatureUnit -->


    <owl:Class rdf:about="https://saref.etsi.org/core/TemperatureUnit">
        <rdfs:subClassOf rdf:resource="https://saref.etsi.org/core/UnitOfMeasure"/>
        <rdfs:comment xml:lang="en">The unit of measure for temperature</rdfs:comment>
        <rdfs:label xml:lang="en">Temperature unit</rdfs:label>
    </owl:Class>
    


    <!-- https://saref.etsi.org/core/Time -->


    <owl:Class rdf:about="https://saref.etsi.org/core/Time">
        <rdfs:subClassOf rdf:resource="https://saref.etsi.org/core/Property"/>
        <rdfs:comment xml:lang="en">A class that allows to specify the time concept.</rdfs:comment>
        <rdfs:comment xml:lang="en">A saref:Property that allows to specify the time concept in terms of instants or intervals according to the imported W3C Time ontology.</rdfs:comment>
        <rdfs:label xml:lang="en">Time</rdfs:label>
    </owl:Class>
    


    <!-- https://saref.etsi.org/core/ToggleCommand -->


    <owl:Class rdf:about="https://saref.etsi.org/core/ToggleCommand">
        <rdfs:subClassOf rdf:resource="https://saref.etsi.org/core/Command"/>
        <rdfs:subClassOf>
            <owl:Restriction>
                <owl:onProperty rdf:resource="https://saref.etsi.org/core/isCommandOf"/>
                <owl:allValuesFrom rdf:resource="https://saref.etsi.org/core/OnOffFunction"/>
            </owl:Restriction>
        </rdfs:subClassOf>
        <rdfs:comment xml:lang="en">A type of command</rdfs:comment>
        <rdfs:label xml:lang="en">Toggle command</rdfs:label>
    </owl:Class>
    


    <!-- https://saref.etsi.org/core/UnitOfMeasure -->


    <owl:Class rdf:about="https://saref.etsi.org/core/UnitOfMeasure">
        <rdfs:comment xml:lang="en">The unit of measure is a standard for measurement of a quantity, such as a Property. For example,  Power is a property and Watt is a unit of power that represents a definite predetermined power: when we say 10 Watt, we actually mean 10 times the definite predetermined power called &quot;watt&quot;. Our definition is based on the definition of unit of measure in the Ontology of units of Measure (OM). We propose here a list of some units of measure that are relevant for the purpose of SAREF, but this list can be extended, also using some other ontologies rather than the Ontology of units of Measure (OM).</rdfs:comment>
        <rdfs:comment xml:lang="en">The unit of measure is a standard for measurement of a quantity, such as a Property. For example,  Power is a property and Watt is a unit of power that represents a definite predetermined power: when we say 10 Watt, we actually mean 10 times the definite predetermined power called &quot;watt&quot;. Our definition is based on the definition of unit of measure in the Ontology of units of Measure (OM). We propose here a list of some units of measure that are relevant for the purpose of the Smart Appliances ontology, but this list can be extended.</rdfs:comment>
        <rdfs:comment xml:lang="en">The unit of measure is a standard for measurement of a quantity, such as a Property. For example, Power is a property and Watt is a unit of power that represents a definite predetermined power: when we say 10 Watt, we actually mean 10 times the definite predetermined power called &quot;watt&quot;. Our definition is based on the definition of unit of measure in the Ontology of units of Measure (OM). We propose here a list of some units of measure that are relevant for the purpose of the Smart Appliances ontology, but this list can be extended.</rdfs:comment>
        <rdfs:isDefinedBy rdf:resource="http://www.wurvoc.org/vocabularies/om-1.6/Unit_of_measure"/>
        <rdfs:isDefinedBy rdf:resource="https://saref.etsi.org/core/"/>
        <rdfs:label xml:lang="en">Unit of measure</rdfs:label>
    </owl:Class>
    


    <!-- https://saref.etsi.org/core/Water -->


    <owl:Class rdf:about="https://saref.etsi.org/core/Water">
        <rdfs:subClassOf rdf:resource="https://saref.etsi.org/core/Commodity"/>
        <rdfs:comment xml:lang="en">A type of commodity</rdfs:comment>
        <rdfs:label xml:lang="en">Water</rdfs:label>
    </owl:Class>
    


    <!-- https://saref.etsi.org/saref4agri/Animal -->


    <owl:Class rdf:about="https://saref.etsi.org/saref4agri/Animal">
        <rdfs:subClassOf rdf:resource="https://saref.etsi.org/core/FeatureOfInterest"/>
        <rdfs:subClassOf>
            <owl:Restriction>
                <owl:onProperty rdf:resource="http://purl.obolibrary.org/obo/TAXRANK_1000000"/>
                <owl:someValuesFrom rdf:resource="http://purl.obolibrary.org/obo/TAXRANK_0000000"/>
            </owl:Restriction>
        </rdfs:subClassOf>
        <rdfs:subClassOf>
            <owl:Restriction>
                <owl:onProperty rdf:resource="https://saref.etsi.org/saref4agri/isLocatedIn"/>
                <owl:someValuesFrom rdf:resource="http://www.opengis.net/ont/geosparql#Feature"/>
            </owl:Restriction>
        </rdfs:subClassOf>
        <rdfs:subClassOf>
            <owl:Restriction>
                <owl:onProperty rdf:resource="https://saref.etsi.org/saref4agri/isMemberOf"/>
                <owl:someValuesFrom rdf:resource="https://saref.etsi.org/saref4agri/AnimalGroup"/>
            </owl:Restriction>
        </rdfs:subClassOf>
        <rdfs:subClassOf>
            <owl:Restriction>
                <owl:onProperty rdf:resource="https://saref.etsi.org/saref4agri/hasID"/>
                <owl:maxQualifiedCardinality rdf:datatype="http://www.w3.org/2001/XMLSchema#nonNegativeInteger">1</owl:maxQualifiedCardinality>
                <owl:onClass rdf:resource="https://saref.etsi.org/saref4agri/ID"/>
            </owl:Restriction>
        </rdfs:subClassOf>
        <rdfs:subClassOf>
            <owl:Restriction>
                <owl:onProperty rdf:resource="https://saref.etsi.org/saref4agri/hasBirthDate"/>
                <owl:maxQualifiedCardinality rdf:datatype="http://www.w3.org/2001/XMLSchema#nonNegativeInteger">1</owl:maxQualifiedCardinality>
                <owl:onDataRange rdf:resource="http://www.w3.org/2001/XMLSchema#dateTime"/>
            </owl:Restriction>
        </rdfs:subClassOf>
        <rdfs:subClassOf>
            <owl:Restriction>
                <owl:onProperty rdf:resource="https://saref.etsi.org/saref4agri/hasDeathDate"/>
                <owl:maxQualifiedCardinality rdf:datatype="http://www.w3.org/2001/XMLSchema#nonNegativeInteger">1</owl:maxQualifiedCardinality>
                <owl:onDataRange rdf:resource="http://www.w3.org/2001/XMLSchema#dateTime"/>
            </owl:Restriction>
        </rdfs:subClassOf>
        <rdfs:subClassOf>
            <owl:Restriction>
                <owl:onProperty rdf:resource="https://saref.etsi.org/saref4agri/hasName"/>
                <owl:maxQualifiedCardinality rdf:datatype="http://www.w3.org/2001/XMLSchema#nonNegativeInteger">1</owl:maxQualifiedCardinality>
                <owl:onDataRange rdf:resource="http://www.w3.org/2001/XMLSchema#string"/>
            </owl:Restriction>
        </rdfs:subClassOf>
        <rdfs:comment xml:lang="en">An individual and identifiable living organism that feeds on organic matter, typically having specialized sense organs and nervous system and able to respond rapidly to stimuli.</rdfs:comment>
        <rdfs:label xml:lang="en">Animal</rdfs:label>
    </owl:Class>
    


    <!-- https://saref.etsi.org/saref4agri/AnimalGroup -->


    <owl:Class rdf:about="https://saref.etsi.org/saref4agri/AnimalGroup">
        <rdfs:subClassOf rdf:resource="https://saref.etsi.org/core/FeatureOfInterest"/>
        <rdfs:subClassOf>
            <owl:Restriction>
                <owl:onProperty rdf:resource="https://saref.etsi.org/saref4agri/hasMember"/>
                <owl:someValuesFrom rdf:resource="https://saref.etsi.org/saref4agri/Animal"/>
            </owl:Restriction>
        </rdfs:subClassOf>
        <rdfs:subClassOf>
            <owl:Restriction>
                <owl:onProperty rdf:resource="https://saref.etsi.org/saref4agri/isLocatedIn"/>
                <owl:someValuesFrom rdf:resource="http://www.opengis.net/ont/geosparql#Feature"/>
            </owl:Restriction>
        </rdfs:subClassOf>
        <rdfs:subClassOf>
            <owl:Restriction>
                <owl:onProperty rdf:resource="https://saref.etsi.org/saref4agri/hasName"/>
                <owl:maxQualifiedCardinality rdf:datatype="http://www.w3.org/2001/XMLSchema#nonNegativeInteger">1</owl:maxQualifiedCardinality>
                <owl:onDataRange rdf:resource="http://www.w3.org/2001/XMLSchema#string"/>
            </owl:Restriction>
        </rdfs:subClassOf>
        <rdfs:comment xml:lang="en">A collection of one or multiple animals.</rdfs:comment>
        <rdfs:label xml:lang="en">Animal Group</rdfs:label>
    </owl:Class>
    


    <!-- https://saref.etsi.org/saref4agri/Building -->


    <owl:Class rdf:about="https://saref.etsi.org/saref4agri/Building">
        <rdfs:subClassOf rdf:resource="http://www.opengis.net/ont/geosparql#Feature"/>
        <rdfs:subClassOf>
            <owl:Restriction>
                <owl:onProperty rdf:resource="https://saref.etsi.org/saref4agri/contains"/>
                <owl:someValuesFrom rdf:resource="https://saref.etsi.org/saref4agri/BuildingSpace"/>
            </owl:Restriction>
        </rdfs:subClassOf>
        <rdfs:subClassOf>
            <owl:Restriction>
                <owl:onProperty rdf:resource="https://saref.etsi.org/saref4agri/hasName"/>
                <owl:maxCardinality rdf:datatype="http://www.w3.org/2001/XMLSchema#nonNegativeInteger">1</owl:maxCardinality>
            </owl:Restriction>
        </rdfs:subClassOf>
        <rdfs:comment xml:lang="en">A building represents a structure that provides shelter for its occupants or contents and stands in one place. The building is also used to provide a basic element within the spatial structure hierarchy for the components of a building project (together with site, storey, and space).</rdfs:comment>
        <rdfs:label xml:lang="en">Building</rdfs:label>
    </owl:Class>
    


    <!-- https://saref.etsi.org/saref4agri/BuildingSpace -->


    <owl:Class rdf:about="https://saref.etsi.org/saref4agri/BuildingSpace">
        <rdfs:subClassOf rdf:resource="http://www.opengis.net/ont/geosparql#Feature"/>
        <rdfs:comment xml:lang="en">An entity used to define the physical spaces of the building. A building space contains devices or building objects.</rdfs:comment>
        <rdfs:label xml:lang="en">Building space</rdfs:label>
    </owl:Class>
    


    <!-- https://saref.etsi.org/saref4agri/Crop -->


    <owl:Class rdf:about="https://saref.etsi.org/saref4agri/Crop">
        <rdfs:subClassOf rdf:resource="https://saref.etsi.org/core/FeatureOfInterest"/>
        <rdfs:subClassOf>
            <owl:Restriction>
                <owl:onProperty rdf:resource="http://purl.obolibrary.org/obo/TAXRANK_1000000"/>
                <owl:someValuesFrom rdf:resource="http://purl.obolibrary.org/obo/TAXRANK_0000000"/>
            </owl:Restriction>
        </rdfs:subClassOf>
        <rdfs:subClassOf>
            <owl:Restriction>
                <owl:onProperty rdf:resource="https://saref.etsi.org/saref4agri/hasHarvestDate"/>
                <owl:someValuesFrom rdf:resource="http://www.w3.org/2001/XMLSchema#dateTime"/>
            </owl:Restriction>
        </rdfs:subClassOf>
        <rdfs:subClassOf>
            <owl:Restriction>
                <owl:onProperty rdf:resource="https://saref.etsi.org/saref4agri/hasPlantDate"/>
                <owl:someValuesFrom rdf:resource="http://www.w3.org/2001/XMLSchema#dateTime"/>
            </owl:Restriction>
        </rdfs:subClassOf>
        <rdfs:comment xml:lang="en">A collection of cultivated plants that is grown on a large scale commercially, especially a cereal, fruit, or vegetable.</rdfs:comment>
        <rdfs:label xml:lang="en">Crop</rdfs:label>
    </owl:Class>
    


    <!-- https://saref.etsi.org/saref4agri/Deployment -->


    <owl:Class rdf:about="https://saref.etsi.org/saref4agri/Deployment">
        <rdfs:subClassOf rdf:resource="http://www.w3.org/ns/ssn/Deployment"/>
        <rdfs:subClassOf>
            <owl:Restriction>
                <owl:onProperty rdf:resource="http://www.w3.org/ns/ssn/deployedOnPlatform"/>
                <owl:someValuesFrom rdf:resource="http://www.w3.org/ns/sosa/Platform"/>
            </owl:Restriction>
        </rdfs:subClassOf>
        <rdfs:subClassOf>
            <owl:Restriction>
                <owl:onProperty rdf:resource="http://www.w3.org/ns/ssn/deployedSystem"/>
                <owl:someValuesFrom rdf:resource="http://www.w3.org/ns/ssn/System"/>
            </owl:Restriction>
        </rdfs:subClassOf>
        <rdfs:subClassOf>
            <owl:Restriction>
                <owl:onProperty rdf:resource="https://saref.etsi.org/saref4agri/hasDeploymentPeriod"/>
                <owl:someValuesFrom rdf:resource="http://www.w3.org/2006/time#TemporalEntity"/>
            </owl:Restriction>
        </rdfs:subClassOf>
        <rdfs:subClassOf>
            <owl:Restriction>
                <owl:onProperty rdf:resource="https://saref.etsi.org/saref4agri/isDeployedAtSpace"/>
                <owl:someValuesFrom rdf:resource="http://www.opengis.net/ont/geosparql#SpatialObject"/>
            </owl:Restriction>
        </rdfs:subClassOf>
        <rdfs:comment xml:lang="en">Deployment</rdfs:comment>
        <rdfs:comment xml:lang="en">The scenario, including temporal and spatial information, in which the systems and devices are installed.</rdfs:comment>
        <rdfs:label xml:lang="en">Deployment</rdfs:label>
    </owl:Class>
    


    <!-- https://saref.etsi.org/saref4agri/EatingActivitySensor -->


    <owl:Class rdf:about="https://saref.etsi.org/saref4agri/EatingActivitySensor">
        <rdfs:subClassOf rdf:resource="https://saref.etsi.org/core/Sensor"/>
        <rdfs:comment xml:lang="en">Eating activity sensor</rdfs:comment>
        <rdfs:label xml:lang="en">Eating activity sensor</rdfs:label>
    </owl:Class>
    


    <!-- https://saref.etsi.org/saref4agri/Farm -->


    <owl:Class rdf:about="https://saref.etsi.org/saref4agri/Farm">
        <rdfs:subClassOf rdf:resource="http://www.opengis.net/ont/geosparql#Feature"/>
        <rdfs:subClassOf>
            <owl:Restriction>
                <owl:onProperty rdf:resource="https://saref.etsi.org/saref4agri/contains"/>
                <owl:someValuesFrom rdf:resource="https://saref.etsi.org/saref4agri/Building"/>
            </owl:Restriction>
        </rdfs:subClassOf>
        <rdfs:subClassOf>
            <owl:Restriction>
                <owl:onProperty rdf:resource="https://saref.etsi.org/saref4agri/contains"/>
                <owl:someValuesFrom rdf:resource="https://saref.etsi.org/saref4agri/Parcel"/>
            </owl:Restriction>
        </rdfs:subClassOf>
        <rdfs:subClassOf>
            <owl:Restriction>
                <owl:onProperty rdf:resource="https://saref.etsi.org/saref4agri/hasName"/>
                <owl:maxCardinality rdf:datatype="http://www.w3.org/2001/XMLSchema#nonNegativeInteger">1</owl:maxCardinality>
            </owl:Restriction>
        </rdfs:subClassOf>
        <rdfs:comment xml:lang="en">A plot of land used for the scope of farming which can contain buildings and parcels.</rdfs:comment>
        <rdfs:label xml:lang="en">Farm</rdfs:label>
    </owl:Class>
    


    <!-- https://saref.etsi.org/saref4agri/FarmHolding -->


    <owl:Class rdf:about="https://saref.etsi.org/saref4agri/FarmHolding">
        <rdfs:subClassOf rdf:resource="https://schema.org/Organization"/>
        <rdfs:subClassOf>
            <owl:Restriction>
                <owl:onProperty rdf:resource="https://saref.etsi.org/saref4agri/managesFarm"/>
                <owl:someValuesFrom rdf:resource="https://saref.etsi.org/saref4agri/Farm"/>
            </owl:Restriction>
        </rdfs:subClassOf>
        <rdfs:subClassOf>
            <owl:Restriction>
                <owl:onProperty rdf:resource="https://saref.etsi.org/saref4agri/hasName"/>
                <owl:allValuesFrom rdf:resource="http://www.w3.org/2001/XMLSchema#string"/>
            </owl:Restriction>
        </rdfs:subClassOf>
        <rdfs:comment xml:lang="en">A class to decsribe a saref4agri farm holding as subcass of an org:Organization</rdfs:comment>
        <rdfs:label xml:lang="en">Farm holding</rdfs:label>
    </owl:Class>
    


    <!-- https://saref.etsi.org/saref4agri/Farmer -->


    <owl:Class rdf:about="https://saref.etsi.org/saref4agri/Farmer">
        <rdfs:subClassOf rdf:resource="http://xmlns.com/foaf/0.1/Person"/>
        <rdfs:subClassOf>
            <owl:Restriction>
                <owl:onProperty rdf:resource="https://saref.etsi.org/saref4agri/managesFarm"/>
                <owl:someValuesFrom rdf:resource="https://saref.etsi.org/saref4agri/Farm"/>
            </owl:Restriction>
        </rdfs:subClassOf>
        <rdfs:subClassOf>
            <owl:Restriction>
                <owl:onProperty rdf:resource="https://saref.etsi.org/saref4agri/hasName"/>
                <owl:allValuesFrom rdf:resource="http://www.w3.org/2001/XMLSchema#string"/>
            </owl:Restriction>
        </rdfs:subClassOf>
        <rdfs:comment xml:lang="en">A class to decsribe a saref4agri farmer as subcass of a foaf:Person</rdfs:comment>
        <rdfs:label xml:lang="en">Farmer</rdfs:label>
    </owl:Class>
    


    <!-- https://saref.etsi.org/saref4agri/ID -->


    <owl:Class rdf:about="https://saref.etsi.org/saref4agri/ID">
        <rdfs:comment xml:lang="en">ID</rdfs:comment>
        <rdfs:label xml:lang="en">ID</rdfs:label>
    </owl:Class>
    


    <!-- https://saref.etsi.org/saref4agri/Intake -->


    <owl:Class rdf:about="https://saref.etsi.org/saref4agri/Intake">
        <rdfs:comment xml:lang="en">The amount of food or other substance taken into the body of an animal or into the soil.</rdfs:comment>
        <rdfs:label xml:lang="en">Intake</rdfs:label>
    </owl:Class>
    


    <!-- https://saref.etsi.org/saref4agri/MilkingSensor -->


    <owl:Class rdf:about="https://saref.etsi.org/saref4agri/MilkingSensor">
        <rdfs:subClassOf rdf:resource="https://saref.etsi.org/core/Sensor"/>
        <rdfs:comment xml:lang="en">Milking sensor</rdfs:comment>
        <rdfs:label xml:lang="en">Milking sensor</rdfs:label>
    </owl:Class>
    


    <!-- https://saref.etsi.org/saref4agri/MovementActivitySensor -->


    <owl:Class rdf:about="https://saref.etsi.org/saref4agri/MovementActivitySensor">
        <rdfs:subClassOf rdf:resource="https://saref.etsi.org/core/Sensor"/>
        <rdfs:comment xml:lang="en">Movement activity sensor</rdfs:comment>
        <rdfs:label xml:lang="en">Movement activity sensor</rdfs:label>
    </owl:Class>
    


    <!-- https://saref.etsi.org/saref4agri/Parcel -->


    <owl:Class rdf:about="https://saref.etsi.org/saref4agri/Parcel">
        <rdfs:subClassOf rdf:resource="http://www.opengis.net/ont/geosparql#Feature"/>
        <rdfs:subClassOf>
            <owl:Restriction>
                <owl:onProperty rdf:resource="https://saref.etsi.org/saref4agri/contains"/>
                <owl:someValuesFrom rdf:resource="https://saref.etsi.org/saref4agri/Crop"/>
            </owl:Restriction>
        </rdfs:subClassOf>
        <rdfs:subClassOf>
            <owl:Restriction>
                <owl:onProperty rdf:resource="https://saref.etsi.org/saref4agri/hasName"/>
                <owl:maxQualifiedCardinality rdf:datatype="http://www.w3.org/2001/XMLSchema#nonNegativeInteger">1</owl:maxQualifiedCardinality>
                <owl:onDataRange rdf:resource="http://www.w3.org/2001/XMLSchema#string"/>
            </owl:Restriction>
        </rdfs:subClassOf>
        <rdfs:comment xml:lang="en">An area of land, which might be used for grazing animals or planting crops. The parcel is defined as an undividable logical area of land which contains homogeneous items.</rdfs:comment>
        <rdfs:label xml:lang="en">Parcel</rdfs:label>
    </owl:Class>
    


    <!-- https://saref.etsi.org/saref4agri/Platform -->


    <owl:Class rdf:about="https://saref.etsi.org/saref4agri/Platform">
        <rdfs:subClassOf rdf:resource="http://www.w3.org/ns/sosa/Platform"/>
        <rdfs:comment xml:lang="en">Platform</rdfs:comment>
        <rdfs:label xml:lang="en">Platform</rdfs:label>
    </owl:Class>
    


    <!-- https://saref.etsi.org/saref4agri/Pluviometer -->


    <owl:Class rdf:about="https://saref.etsi.org/saref4agri/Pluviometer">
        <rdfs:subClassOf rdf:resource="https://saref.etsi.org/core/Sensor"/>
        <rdfs:comment xml:lang="en">A sensor that measures the rain fall.</rdfs:comment>
        <rdfs:label xml:lang="en">Pluviometer</rdfs:label>
    </owl:Class>
    


    <!-- https://saref.etsi.org/saref4agri/Soil -->


    <owl:Class rdf:about="https://saref.etsi.org/saref4agri/Soil">
        <rdfs:subClassOf rdf:resource="https://saref.etsi.org/core/FeatureOfInterest"/>
        <rdfs:comment xml:lang="en">Upper layer of the earth in which plants grow.</rdfs:comment>
        <rdfs:label xml:lang="en">Soil</rdfs:label>
    </owl:Class>
    


    <!-- https://saref.etsi.org/saref4agri/SoilTensiometer -->


    <owl:Class rdf:about="https://saref.etsi.org/saref4agri/SoilTensiometer">
        <rdfs:subClassOf rdf:resource="https://saref.etsi.org/core/Sensor"/>
        <rdfs:comment xml:lang="en">A sensor that measures the soil moisture.</rdfs:comment>
        <rdfs:label xml:lang="en">Soil tensiometer</rdfs:label>
    </owl:Class>
    


    <!-- https://saref.etsi.org/saref4agri/Thermometer -->


    <owl:Class rdf:about="https://saref.etsi.org/saref4agri/Thermometer">
        <rdfs:subClassOf rdf:resource="https://saref.etsi.org/core/Sensor"/>
        <rdfs:comment xml:lang="en">Thermometer</rdfs:comment>
        <rdfs:label xml:lang="en">Thermometer</rdfs:label>
    </owl:Class>
    


    <!-- https://saref.etsi.org/saref4agri/WateringGun -->


    <owl:Class rdf:about="https://saref.etsi.org/saref4agri/WateringGun">
        <rdfs:subClassOf rdf:resource="https://saref.etsi.org/core/Actuator"/>
        <rdfs:comment xml:lang="en">An actuator to irrigate an space.</rdfs:comment>
        <rdfs:label xml:lang="en">Watering gun</rdfs:label>
    </owl:Class>
    


    <!-- https://saref.etsi.org/saref4agri/WateringSystem -->


    <owl:Class rdf:about="https://saref.etsi.org/saref4agri/WateringSystem">
        <rdfs:subClassOf rdf:resource="http://www.w3.org/ns/ssn/System"/>
        <rdfs:comment xml:lang="en">Watering system</rdfs:comment>
        <rdfs:label xml:lang="en">Watering system</rdfs:label>
    </owl:Class>
    


    <!-- https://saref.etsi.org/saref4agri/WateringValve -->


    <owl:Class rdf:about="https://saref.etsi.org/saref4agri/WateringValve">
        <rdfs:subClassOf rdf:resource="https://saref.etsi.org/core/Actuator"/>
        <rdfs:comment xml:lang="en">Watering valve</rdfs:comment>
        <rdfs:label xml:lang="en">Watering valve</rdfs:label>
    </owl:Class>
    


    <!-- https://saref.etsi.org/saref4agri/WeatherStation -->


    <owl:Class rdf:about="https://saref.etsi.org/saref4agri/WeatherStation">
        <rdfs:subClassOf rdf:resource="http://www.w3.org/ns/ssn/System"/>
        <rdfs:subClassOf rdf:resource="https://saref.etsi.org/core/Sensor"/>
        <rdfs:comment xml:lang="en">A sensor o system that measure weather conditions.</rdfs:comment>
        <rdfs:label xml:lang="en">Weather station</rdfs:label>
    </owl:Class>
    


    <!-- https://saref.etsi.org/saref4agri/WeightSensor -->


    <owl:Class rdf:about="https://saref.etsi.org/saref4agri/WeightSensor">
        <rdfs:subClassOf rdf:resource="https://saref.etsi.org/core/Sensor"/>
        <rdfs:comment xml:lang="en">Weight sensor</rdfs:comment>
        <rdfs:label xml:lang="en">Weight sensor</rdfs:label>
    </owl:Class>
    


    <!-- https://saref.etsi.org/saref4agri/Yield -->


    <owl:Class rdf:about="https://saref.etsi.org/saref4agri/Yield">
        <rdfs:comment xml:lang="en">The produced amount of food for animals or of agricultural products.</rdfs:comment>
        <rdfs:label xml:lang="en">Yield</rdfs:label>
    </owl:Class>
    


    <!-- https://saref.etsi.org/saref4bldg/Actuator -->


    <owl:Class rdf:about="https://saref.etsi.org/saref4bldg/Actuator">
        <rdfs:subClassOf rdf:resource="https://saref.etsi.org/core/Actuator"/>
        <rdfs:subClassOf rdf:resource="https://saref.etsi.org/saref4bldg/DistributionControlDevice"/>
        <rdfs:subClassOf>
            <owl:Restriction>
                <owl:onProperty rdf:resource="https://saref.etsi.org/saref4bldg/failPosition"/>
                <owl:allValuesFrom rdf:resource="http://www.w3.org/2001/XMLSchema#string"/>
            </owl:Restriction>
        </rdfs:subClassOf>
        <rdfs:subClassOf>
            <owl:Restriction>
                <owl:onProperty rdf:resource="https://saref.etsi.org/saref4bldg/manualOverride"/>
                <owl:allValuesFrom rdf:resource="http://www.w3.org/2001/XMLSchema#boolean"/>
            </owl:Restriction>
        </rdfs:subClassOf>
        <rdfs:comment xml:lang="en">An actuator is a mechanical device for moving or controlling a mechanism or system. An actuator takes energy, usually created by air, electricity, or liquid, and converts that into some kind of motion.</rdfs:comment>
        <rdfs:label xml:lang="en">Actuator</rdfs:label>
        <rdfs:seeAlso>https://w3id.org/ifc/IFC4_ADD1#IfcActuator</rdfs:seeAlso>
        <prov:hadPrimarySource rdf:resource="http://www.buildingsmart-tech.org/ifc/IFC4/Add1/html/schema/ifcbuildingcontrolsdomain/lexical/ifcactuator.htm"/>
        <prov:hadPrimarySource rdf:resource="http://www.buildingsmart-tech.org/ifc/IFC4/Add1/html/schema/ifcbuildingcontrolsdomain/pset/pset_actuatortypecommon.htm"/>
    </owl:Class>
    


    <!-- https://saref.etsi.org/saref4bldg/AirToAirHeatRecovery -->


    <owl:Class rdf:about="https://saref.etsi.org/saref4bldg/AirToAirHeatRecovery">
        <rdfs:subClassOf rdf:resource="https://saref.etsi.org/saref4bldg/EnergyConversionDevice"/>
        <rdfs:subClassOf>
            <owl:Restriction>
                <owl:onProperty rdf:resource="https://saref.etsi.org/saref4bldg/operationTemperatureMax"/>
                <owl:allValuesFrom rdf:resource="https://saref.etsi.org/core/Measurement"/>
            </owl:Restriction>
        </rdfs:subClassOf>
        <rdfs:subClassOf>
            <owl:Restriction>
                <owl:onProperty rdf:resource="https://saref.etsi.org/saref4bldg/operationTemperatureMin"/>
                <owl:allValuesFrom rdf:resource="https://saref.etsi.org/core/Measurement"/>
            </owl:Restriction>
        </rdfs:subClassOf>
        <rdfs:subClassOf>
            <owl:Restriction>
                <owl:onProperty rdf:resource="https://saref.etsi.org/saref4bldg/primaryAirFlowRateMax"/>
                <owl:allValuesFrom rdf:resource="https://saref.etsi.org/core/Measurement"/>
            </owl:Restriction>
        </rdfs:subClassOf>
        <rdfs:subClassOf>
            <owl:Restriction>
                <owl:onProperty rdf:resource="https://saref.etsi.org/saref4bldg/primaryAirFlowRateMin"/>
                <owl:allValuesFrom rdf:resource="https://saref.etsi.org/core/Measurement"/>
            </owl:Restriction>
        </rdfs:subClassOf>
        <rdfs:subClassOf>
            <owl:Restriction>
                <owl:onProperty rdf:resource="https://saref.etsi.org/saref4bldg/secondaryAirFlowRateMax"/>
                <owl:allValuesFrom rdf:resource="https://saref.etsi.org/core/Measurement"/>
            </owl:Restriction>
        </rdfs:subClassOf>
        <rdfs:subClassOf>
            <owl:Restriction>
                <owl:onProperty rdf:resource="https://saref.etsi.org/saref4bldg/secondaryAirFlowRateMin"/>
                <owl:allValuesFrom rdf:resource="https://saref.etsi.org/core/Measurement"/>
            </owl:Restriction>
        </rdfs:subClassOf>
        <rdfs:subClassOf>
            <owl:Restriction>
                <owl:onProperty rdf:resource="https://saref.etsi.org/saref4bldg/hasDefrost"/>
                <owl:allValuesFrom rdf:resource="http://www.w3.org/2001/XMLSchema#boolean"/>
            </owl:Restriction>
        </rdfs:subClassOf>
        <rdfs:subClassOf>
            <owl:Restriction>
                <owl:onProperty rdf:resource="https://saref.etsi.org/saref4bldg/heatTransferTypeEnum"/>
                <owl:allValuesFrom rdf:resource="http://www.w3.org/2001/XMLSchema#string"/>
            </owl:Restriction>
        </rdfs:subClassOf>
        <rdfs:comment xml:lang="en">An air-to-air heat recovery device employs a counter-flow heat exchanger between inbound and outbound air flow. It is typically used to transfer heat from warmer air in one chamber to cooler air in the second chamber (i.e., typically used to recover heat from the conditioned air being exhausted and the outside air being supplied to a building), resulting in energy savings from reduced heating (or cooling) requirements.</rdfs:comment>
        <rdfs:label xml:lang="en">Air to air heat recovery</rdfs:label>
        <rdfs:seeAlso>https://w3id.org/ifc/IFC4_ADD1#IfcAirToAirHeatRecovery</rdfs:seeAlso>
        <prov:hadPrimarySource rdf:resource="http://www.buildingsmart-tech.org/ifc/IFC4/Add1/html/schema/ifchvacdomain/lexical/ifcairtoairheatrecovery.htm"/>
        <prov:hadPrimarySource rdf:resource="http://www.buildingsmart-tech.org/ifc/IFC4/Add1/html/schema/ifchvacdomain/pset/pset_airtoairheatrecoverytypecommon.htm"/>
    </owl:Class>
    


    <!-- https://saref.etsi.org/saref4bldg/Alarm -->


    <owl:Class rdf:about="https://saref.etsi.org/saref4bldg/Alarm">
        <rdfs:subClassOf rdf:resource="https://saref.etsi.org/saref4bldg/DistributionControlDevice"/>
        <rdfs:comment xml:lang="en">An alarm is a device that signals the existence of a condition or situation that is outside the boundaries of normal expectation or that activates such a device.

Alarms include the provision of break glass buttons and manual pull boxes that are used to activate alarms.</rdfs:comment>
        <rdfs:label xml:lang="en">Alarm</rdfs:label>
        <rdfs:seeAlso>https://w3id.org/ifc/IFC4_ADD1#IfcAlarm</rdfs:seeAlso>
        <prov:hadPrimarySource rdf:resource="http://www.buildingsmart-tech.org/ifc/IFC4/Add1/html/schema/ifcbuildingcontrolsdomain/lexical/ifcalarm.htm"/>
        <prov:hadPrimarySource rdf:resource="http://www.buildingsmart-tech.org/ifc/IFC4/Add1/html/schema/ifcbuildingcontrolsdomain/pset/pset_alarmtypecommon.htm"/>
    </owl:Class>
    


    <!-- https://saref.etsi.org/saref4bldg/AudioVisualAppliance -->


    <owl:Class rdf:about="https://saref.etsi.org/saref4bldg/AudioVisualAppliance">
        <rdfs:subClassOf rdf:resource="https://saref.etsi.org/saref4bldg/FlowTerminal"/>
        <rdfs:subClassOf>
            <owl:Restriction>
                <owl:onProperty rdf:resource="https://saref.etsi.org/saref4bldg/audioVolume"/>
                <owl:allValuesFrom rdf:resource="https://saref.etsi.org/core/Measurement"/>
            </owl:Restriction>
        </rdfs:subClassOf>
        <rdfs:subClassOf>
            <owl:Restriction>
                <owl:onProperty rdf:resource="https://saref.etsi.org/saref4bldg/mediaSource"/>
                <owl:allValuesFrom rdf:resource="http://www.w3.org/2001/XMLSchema#string"/>
            </owl:Restriction>
        </rdfs:subClassOf>
        <rdfs:comment xml:lang="en">An audio-visual appliance is a device that displays, captures, transmits, or receives audio or video.

Audio-visual appliances may be fixed in place or may be able to be moved from one space to another. They may require an electrical supply that may be supplied either by an electrical circuit or provided from a local battery source. Audio-visual appliances may be connected to data circuits including specialist circuits for audio visual purposes only.</rdfs:comment>
        <rdfs:label xml:lang="en">Audio visual appliance</rdfs:label>
        <rdfs:seeAlso>https://w3id.org/ifc/IFC4_ADD1#IfcAudioVisualApplicance</rdfs:seeAlso>
        <prov:hadPrimarySource rdf:resource="http://www.buildingsmart-tech.org/ifc/IFC4/Add1/html/schema/ifcelectricaldomain/lexical/ifcaudiovisualappliance.htm"/>
        <prov:hadPrimarySource rdf:resource="http://www.buildingsmart-tech.org/ifc/IFC4/Add1/html/schema/ifcelectricaldomain/pset/pset_audiovisualappliancetypecommon.htm"/>
    </owl:Class>
    


    <!-- https://saref.etsi.org/saref4bldg/Boiler -->


    <owl:Class rdf:about="https://saref.etsi.org/saref4bldg/Boiler">
        <rdfs:subClassOf rdf:resource="https://saref.etsi.org/saref4bldg/EnergyConversionDevice"/>
        <rdfs:subClassOf>
            <owl:Restriction>
                <owl:onProperty rdf:resource="https://saref.etsi.org/saref4bldg/heatTransferSurfaceArea"/>
                <owl:allValuesFrom rdf:resource="https://saref.etsi.org/core/Measurement"/>
            </owl:Restriction>
        </rdfs:subClassOf>
        <rdfs:subClassOf>
            <owl:Restriction>
                <owl:onProperty rdf:resource="https://saref.etsi.org/saref4bldg/nominalEnergyConsumption"/>
                <owl:allValuesFrom rdf:resource="https://saref.etsi.org/core/Measurement"/>
            </owl:Restriction>
        </rdfs:subClassOf>
        <rdfs:subClassOf>
            <owl:Restriction>
                <owl:onProperty rdf:resource="https://saref.etsi.org/saref4bldg/nominalPartLoadRatio"/>
                <owl:allValuesFrom rdf:resource="https://saref.etsi.org/core/Measurement"/>
            </owl:Restriction>
        </rdfs:subClassOf>
        <rdfs:subClassOf>
            <owl:Restriction>
                <owl:onProperty rdf:resource="https://saref.etsi.org/saref4bldg/outletTemperatureMax"/>
                <owl:allValuesFrom rdf:resource="https://saref.etsi.org/core/Measurement"/>
            </owl:Restriction>
        </rdfs:subClassOf>
        <rdfs:subClassOf>
            <owl:Restriction>
                <owl:onProperty rdf:resource="https://saref.etsi.org/saref4bldg/outletTemperatureMin"/>
                <owl:allValuesFrom rdf:resource="https://saref.etsi.org/core/Measurement"/>
            </owl:Restriction>
        </rdfs:subClassOf>
        <rdfs:subClassOf>
            <owl:Restriction>
                <owl:onProperty rdf:resource="https://saref.etsi.org/saref4bldg/pressureRating"/>
                <owl:allValuesFrom rdf:resource="https://saref.etsi.org/core/Measurement"/>
            </owl:Restriction>
        </rdfs:subClassOf>
        <rdfs:subClassOf>
            <owl:Restriction>
                <owl:onProperty rdf:resource="https://saref.etsi.org/saref4bldg/waterInletTemperatureMax"/>
                <owl:allValuesFrom rdf:resource="https://saref.etsi.org/core/Measurement"/>
            </owl:Restriction>
        </rdfs:subClassOf>
        <rdfs:subClassOf>
            <owl:Restriction>
                <owl:onProperty rdf:resource="https://saref.etsi.org/saref4bldg/waterInletTemperatureMin"/>
                <owl:allValuesFrom rdf:resource="https://saref.etsi.org/core/Measurement"/>
            </owl:Restriction>
        </rdfs:subClassOf>
        <rdfs:subClassOf>
            <owl:Restriction>
                <owl:onProperty rdf:resource="https://saref.etsi.org/saref4bldg/waterStorageCapacity"/>
                <owl:allValuesFrom rdf:resource="https://saref.etsi.org/core/Measurement"/>
            </owl:Restriction>
        </rdfs:subClassOf>
        <rdfs:subClassOf>
            <owl:Restriction>
                <owl:onProperty rdf:resource="https://saref.etsi.org/saref4bldg/energySource"/>
                <owl:allValuesFrom rdf:resource="http://www.w3.org/2001/XMLSchema#string"/>
            </owl:Restriction>
        </rdfs:subClassOf>
        <rdfs:subClassOf>
            <owl:Restriction>
                <owl:onProperty rdf:resource="https://saref.etsi.org/saref4bldg/isWaterStorageHeater"/>
                <owl:allValuesFrom rdf:resource="http://www.w3.org/2001/XMLSchema#boolean"/>
            </owl:Restriction>
        </rdfs:subClassOf>
        <rdfs:subClassOf>
            <owl:Restriction>
                <owl:onProperty rdf:resource="https://saref.etsi.org/saref4bldg/operatingMode"/>
                <owl:allValuesFrom rdf:resource="http://www.w3.org/2001/XMLSchema#string"/>
            </owl:Restriction>
        </rdfs:subClassOf>
        <rdfs:comment xml:lang="en">A boiler is a closed, pressure-rated vessel in which water or other fluid is heated using an energy source such as natural gas, heating oil, or electricity. The fluid in the vessel is then circulated out of the boiler for use in various processes or heating applications.</rdfs:comment>
        <rdfs:label xml:lang="en">Boiler</rdfs:label>
        <rdfs:seeAlso>https://w3id.org/ifc/IFC4_ADD1#IfcBoiler</rdfs:seeAlso>
        <prov:hadPrimarySource rdf:resource="http://www.buildingsmart-tech.org/ifc/IFC4/Add1/html/schema/ifchvacdomain/lexical/ifcboiler.htm"/>
        <prov:hadPrimarySource rdf:resource="http://www.buildingsmart-tech.org/ifc/IFC4/Add1/html/schema/ifchvacdomain/pset/pset_boilertypecommon.htm"/>
    </owl:Class>
    


    <!-- https://saref.etsi.org/saref4bldg/Building -->


    <owl:Class rdf:about="https://saref.etsi.org/saref4bldg/Building">
        <rdfs:subClassOf>
            <owl:Restriction>
                <owl:onProperty rdf:resource="https://saref.etsi.org/saref4bldg/hasSpace"/>
                <owl:allValuesFrom rdf:resource="https://saref.etsi.org/saref4bldg/BuildingSpace"/>
            </owl:Restriction>
        </rdfs:subClassOf>
        <rdfs:comment xml:lang="en">A building represents a structure that provides shelter for its occupants or contents and stands in one place. The building is also used to provide a basic element within the spatial structure hierarchy for the components of a building project (together with site, storey, and space).</rdfs:comment>
        <rdfs:label xml:lang="en">Building</rdfs:label>
        <rdfs:seeAlso rdf:resource="https://w3id.org/ifc/IFC4_ADD1#IfcBuilding"/>
        <prov:hadPrimarySource rdf:resource="http://www.buildingsmart-tech.org/ifc/IFC4/Add1/html/schema/ifcproductextension/lexical/ifcbuilding.htm"/>
    </owl:Class>
    


    <!-- https://saref.etsi.org/saref4bldg/BuildingDevice -->


    <owl:Class rdf:about="https://saref.etsi.org/saref4bldg/BuildingDevice">
        <rdfs:subClassOf rdf:resource="https://saref.etsi.org/core/Device"/>
        <rdfs:subClassOf rdf:resource="https://saref.etsi.org/saref4bldg/BuildingObject"/>
        <rdfs:comment xml:lang="en">A tangible object designed to accomplish a particular task in a building.</rdfs:comment>
        <rdfs:label xml:lang="en">Building device</rdfs:label>
    </owl:Class>
    


    <!-- https://saref.etsi.org/saref4bldg/BuildingObject -->


    <owl:Class rdf:about="https://saref.etsi.org/saref4bldg/BuildingObject">
        <rdfs:subClassOf rdf:resource="https://saref.etsi.org/saref4bldg/PhysicalObject"/>
        <rdfs:comment xml:lang="en">An object in the building that can be controlled by devices, such as a door or a window that can be automatically opened or closed by an actuator.  (Definition taken from SAREF 1.0)</rdfs:comment>
        <rdfs:label xml:lang="en">Building object</rdfs:label>
    </owl:Class>
    


    <!-- https://saref.etsi.org/saref4bldg/BuildingSpace -->


    <owl:Class rdf:about="https://saref.etsi.org/saref4bldg/BuildingSpace">
        <rdfs:subClassOf>
            <owl:Restriction>
                <owl:onProperty rdf:resource="https://saref.etsi.org/saref4bldg/contains"/>
                <owl:allValuesFrom rdf:resource="https://saref.etsi.org/saref4bldg/PhysicalObject"/>
            </owl:Restriction>
        </rdfs:subClassOf>
        <rdfs:subClassOf>
            <owl:Restriction>
                <owl:onProperty rdf:resource="https://saref.etsi.org/saref4bldg/hasSpace"/>
                <owl:allValuesFrom rdf:resource="https://saref.etsi.org/saref4bldg/BuildingSpace"/>
            </owl:Restriction>
        </rdfs:subClassOf>
        <rdfs:subClassOf>
            <owl:Restriction>
                <owl:onProperty rdf:resource="https://saref.etsi.org/saref4bldg/isSpaceOf"/>
                <owl:allValuesFrom>
                    <owl:Class>
                        <owl:unionOf rdf:parseType="Collection">
                            <rdf:Description rdf:about="https://saref.etsi.org/saref4bldg/Building"/>
                            <rdf:Description rdf:about="https://saref.etsi.org/saref4bldg/BuildingSpace"/>
                        </owl:unionOf>
                    </owl:Class>
                </owl:allValuesFrom>
            </owl:Restriction>
        </rdfs:subClassOf>
        <rdfs:comment xml:lang="en">An entity used to define the physical spaces of the building. A building space contains devices or building objects.</rdfs:comment>
        <rdfs:label xml:lang="en">Building space</rdfs:label>
    </owl:Class>
    


    <!-- https://saref.etsi.org/saref4bldg/Burner -->


    <owl:Class rdf:about="https://saref.etsi.org/saref4bldg/Burner">
        <rdfs:subClassOf rdf:resource="https://saref.etsi.org/saref4bldg/EnergyConversionDevice"/>
        <rdfs:subClassOf>
            <owl:Restriction>
                <owl:onProperty rdf:resource="https://saref.etsi.org/saref4bldg/energySource"/>
                <owl:allValuesFrom rdf:resource="http://www.w3.org/2001/XMLSchema#string"/>
            </owl:Restriction>
        </rdfs:subClassOf>
        <rdfs:comment xml:lang="en">A burner is a device that converts fuel into heat through combustion. It includes gas, oil, and wood burners.</rdfs:comment>
        <rdfs:label xml:lang="en">Burner</rdfs:label>
        <rdfs:seeAlso>https://w3id.org/ifc/IFC4_ADD1#IfcBurner</rdfs:seeAlso>
        <prov:hadPrimarySource rdf:resource="http://www.buildingsmart-tech.org/ifc/IFC4/Add1/html/schema/ifchvacdomain/lexical/ifcburner.htm"/>
        <prov:hadPrimarySource rdf:resource="http://www.buildingsmart-tech.org/ifc/IFC4/Add1/html/schema/ifchvacdomain/pset/pset_burnertypecommon.htm"/>
    </owl:Class>
    


    <!-- https://saref.etsi.org/saref4bldg/Chiller -->


    <owl:Class rdf:about="https://saref.etsi.org/saref4bldg/Chiller">
        <rdfs:subClassOf rdf:resource="https://saref.etsi.org/saref4bldg/EnergyConversionDevice"/>
        <rdfs:subClassOf>
            <owl:Restriction>
                <owl:onProperty rdf:resource="https://saref.etsi.org/saref4bldg/nominalCapacity"/>
                <owl:allValuesFrom rdf:resource="https://saref.etsi.org/core/Measurement"/>
            </owl:Restriction>
        </rdfs:subClassOf>
        <rdfs:subClassOf>
            <owl:Restriction>
                <owl:onProperty rdf:resource="https://saref.etsi.org/saref4bldg/nominalCondensingTemperature"/>
                <owl:allValuesFrom rdf:resource="https://saref.etsi.org/core/Measurement"/>
            </owl:Restriction>
        </rdfs:subClassOf>
        <rdfs:subClassOf>
            <owl:Restriction>
                <owl:onProperty rdf:resource="https://saref.etsi.org/saref4bldg/nominalEfficiency"/>
                <owl:allValuesFrom rdf:resource="https://saref.etsi.org/core/Measurement"/>
            </owl:Restriction>
        </rdfs:subClassOf>
        <rdfs:subClassOf>
            <owl:Restriction>
                <owl:onProperty rdf:resource="https://saref.etsi.org/saref4bldg/nominalEvaporatingTemmperature"/>
                <owl:allValuesFrom rdf:resource="https://saref.etsi.org/core/Measurement"/>
            </owl:Restriction>
        </rdfs:subClassOf>
        <rdfs:subClassOf>
            <owl:Restriction>
                <owl:onProperty rdf:resource="https://saref.etsi.org/saref4bldg/nominalHeatRejectionRate"/>
                <owl:allValuesFrom rdf:resource="https://saref.etsi.org/core/Measurement"/>
            </owl:Restriction>
        </rdfs:subClassOf>
        <rdfs:subClassOf>
            <owl:Restriction>
                <owl:onProperty rdf:resource="https://saref.etsi.org/saref4bldg/nominalPowerConsumption"/>
                <owl:allValuesFrom rdf:resource="https://saref.etsi.org/core/Measurement"/>
            </owl:Restriction>
        </rdfs:subClassOf>
        <rdfs:comment xml:lang="en">A chiller is a device used to remove heat from a liquid via a vapor-compression or absorption refrigeration cycle to cool a fluid, typically water or a mixture of water and glycol. The chilled fluid is then used to cool and dehumidify air in a building.</rdfs:comment>
        <rdfs:label xml:lang="en">Chiller</rdfs:label>
        <rdfs:seeAlso>https://w3id.org/ifc/IFC4_ADD1#IfcChiller</rdfs:seeAlso>
        <prov:hadPrimarySource rdf:resource="http://www.buildingsmart-tech.org/ifc/IFC4/Add1/html/schema/ifchvacdomain/lexical/ifcchiller.htm"/>
        <prov:hadPrimarySource rdf:resource="http://www.buildingsmart-tech.org/ifc/IFC4/Add1/html/schema/ifchvacdomain/pset/pset_chillertypecommon.htm"/>
    </owl:Class>
    


    <!-- https://saref.etsi.org/saref4bldg/Coil -->


    <owl:Class rdf:about="https://saref.etsi.org/saref4bldg/Coil">
        <rdfs:subClassOf rdf:resource="https://saref.etsi.org/saref4bldg/EnergyConversionDevice"/>
        <rdfs:subClassOf>
            <owl:Restriction>
                <owl:onProperty rdf:resource="https://saref.etsi.org/saref4bldg/airFlowRateMax"/>
                <owl:allValuesFrom rdf:resource="https://saref.etsi.org/core/Measurement"/>
            </owl:Restriction>
        </rdfs:subClassOf>
        <rdfs:subClassOf>
            <owl:Restriction>
                <owl:onProperty rdf:resource="https://saref.etsi.org/saref4bldg/airFlowRateMin"/>
                <owl:allValuesFrom rdf:resource="https://saref.etsi.org/core/Measurement"/>
            </owl:Restriction>
        </rdfs:subClassOf>
        <rdfs:subClassOf>
            <owl:Restriction>
                <owl:onProperty rdf:resource="https://saref.etsi.org/saref4bldg/nominalLatentCapacity"/>
                <owl:allValuesFrom rdf:resource="https://saref.etsi.org/core/Measurement"/>
            </owl:Restriction>
        </rdfs:subClassOf>
        <rdfs:subClassOf>
            <owl:Restriction>
                <owl:onProperty rdf:resource="https://saref.etsi.org/saref4bldg/nominalSensibleCapacity"/>
                <owl:allValuesFrom rdf:resource="https://saref.etsi.org/core/Measurement"/>
            </owl:Restriction>
        </rdfs:subClassOf>
        <rdfs:subClassOf>
            <owl:Restriction>
                <owl:onProperty rdf:resource="https://saref.etsi.org/saref4bldg/nominalUa"/>
                <owl:allValuesFrom rdf:resource="https://saref.etsi.org/core/Measurement"/>
            </owl:Restriction>
        </rdfs:subClassOf>
        <rdfs:subClassOf>
            <owl:Restriction>
                <owl:onProperty rdf:resource="https://saref.etsi.org/saref4bldg/operationTemperatureMax"/>
                <owl:allValuesFrom rdf:resource="https://saref.etsi.org/core/Measurement"/>
            </owl:Restriction>
        </rdfs:subClassOf>
        <rdfs:subClassOf>
            <owl:Restriction>
                <owl:onProperty rdf:resource="https://saref.etsi.org/saref4bldg/operationTemperatureMin"/>
                <owl:allValuesFrom rdf:resource="https://saref.etsi.org/core/Measurement"/>
            </owl:Restriction>
        </rdfs:subClassOf>
        <rdfs:subClassOf>
            <owl:Restriction>
                <owl:onProperty rdf:resource="https://saref.etsi.org/saref4bldg/placementType"/>
                <owl:allValuesFrom rdf:resource="http://www.w3.org/2001/XMLSchema#string"/>
            </owl:Restriction>
        </rdfs:subClassOf>
        <rdfs:comment xml:lang="en">A coil is a device used to provide heat transfer between non-mixing media. A common example is a cooling coil, which utilizes a finned coil in which circulates chilled water, antifreeze, or refrigerant that is used to remove heat from air moving across the surface of the coil. A coil may be used either for heating or cooling purposes by placing a series of tubes (the coil) carrying a heating or cooling fluid into an airstream. The coil may be constructed from tubes bundled in a serpentine form or from finned tubes that give a extended heat transfer surface.

Coils may also be used for non-airflow cases such as embedded in a floor slab.</rdfs:comment>
        <rdfs:label xml:lang="en">Coil</rdfs:label>
        <rdfs:seeAlso>https://w3id.org/ifc/IFC4_ADD1#IfcCoil</rdfs:seeAlso>
        <prov:hadPrimarySource rdf:resource="http://www.buildingsmart-tech.org/ifc/IFC4/Add1/html/schema/ifchvacdomain/lexical/ifccoil.htm"/>
        <prov:hadPrimarySource rdf:resource="http://www.buildingsmart-tech.org/ifc/IFC4/Add1/html/schema/ifchvacdomain/pset/pset_coiltypecommon.htm"/>
    </owl:Class>
    


    <!-- https://saref.etsi.org/saref4bldg/CommunicationAppliance -->


    <owl:Class rdf:about="https://saref.etsi.org/saref4bldg/CommunicationAppliance">
        <rdfs:subClassOf rdf:resource="https://saref.etsi.org/saref4bldg/FlowTerminal"/>
        <rdfs:comment xml:lang="en">A communications appliance transmits and receives electronic or digital information as data or sound.

Communication appliances may be fixed in place or may be able to be moved from one space to another. Communication appliances require an electrical supply that may be supplied either by an electrical circuit or provided from a local battery source.</rdfs:comment>
        <rdfs:label xml:lang="en">Communication appliance</rdfs:label>
        <rdfs:seeAlso>https://w3id.org/ifc/IFC4_ADD1#IfcCommunicationAppliance</rdfs:seeAlso>
        <prov:hadPrimarySource rdf:resource="http://www.buildingsmart-tech.org/ifc/IFC4/Add1/html/schema/ifcelectricaldomain/lexical/ifccommunicationsappliance.htm"/>
        <prov:hadPrimarySource rdf:resource="http://www.buildingsmart-tech.org/ifc/IFC4/Add1/html/schema/ifcelectricaldomain/pset/pset_communicationsappliancetypecommon.htm"/>
    </owl:Class>
    


    <!-- https://saref.etsi.org/saref4bldg/Compressor -->


    <owl:Class rdf:about="https://saref.etsi.org/saref4bldg/Compressor">
        <rdfs:subClassOf rdf:resource="https://saref.etsi.org/saref4bldg/FlowMovingDevice"/>
        <rdfs:subClassOf>
            <owl:Restriction>
                <owl:onProperty rdf:resource="https://saref.etsi.org/saref4bldg/compressorSpeed"/>
                <owl:allValuesFrom rdf:resource="https://saref.etsi.org/core/Measurement"/>
            </owl:Restriction>
        </rdfs:subClassOf>
        <rdfs:subClassOf>
            <owl:Restriction>
                <owl:onProperty rdf:resource="https://saref.etsi.org/saref4bldg/idealCapacity"/>
                <owl:allValuesFrom rdf:resource="https://saref.etsi.org/core/Measurement"/>
            </owl:Restriction>
        </rdfs:subClassOf>
        <rdfs:subClassOf>
            <owl:Restriction>
                <owl:onProperty rdf:resource="https://saref.etsi.org/saref4bldg/idealShaftPower"/>
                <owl:allValuesFrom rdf:resource="https://saref.etsi.org/core/Measurement"/>
            </owl:Restriction>
        </rdfs:subClassOf>
        <rdfs:subClassOf>
            <owl:Restriction>
                <owl:onProperty rdf:resource="https://saref.etsi.org/saref4bldg/impellerDiameter"/>
                <owl:allValuesFrom rdf:resource="https://saref.etsi.org/core/Measurement"/>
            </owl:Restriction>
        </rdfs:subClassOf>
        <rdfs:subClassOf>
            <owl:Restriction>
                <owl:onProperty rdf:resource="https://saref.etsi.org/saref4bldg/nominalCapacity"/>
                <owl:allValuesFrom rdf:resource="https://saref.etsi.org/core/Measurement"/>
            </owl:Restriction>
        </rdfs:subClassOf>
        <rdfs:subClassOf>
            <owl:Restriction>
                <owl:onProperty rdf:resource="https://saref.etsi.org/saref4bldg/partLoadRatioMax"/>
                <owl:allValuesFrom rdf:resource="https://saref.etsi.org/core/Measurement"/>
            </owl:Restriction>
        </rdfs:subClassOf>
        <rdfs:subClassOf>
            <owl:Restriction>
                <owl:onProperty rdf:resource="https://saref.etsi.org/saref4bldg/partLoadRatioMin"/>
                <owl:allValuesFrom rdf:resource="https://saref.etsi.org/core/Measurement"/>
            </owl:Restriction>
        </rdfs:subClassOf>
        <rdfs:subClassOf>
            <owl:Restriction>
                <owl:onProperty rdf:resource="https://saref.etsi.org/saref4bldg/hasHotGasBypass"/>
                <owl:allValuesFrom rdf:resource="http://www.w3.org/2001/XMLSchema#boolean"/>
            </owl:Restriction>
        </rdfs:subClassOf>
        <rdfs:subClassOf>
            <owl:Restriction>
                <owl:onProperty rdf:resource="https://saref.etsi.org/saref4bldg/powerSource"/>
                <owl:allValuesFrom rdf:resource="http://www.w3.org/2001/XMLSchema#string"/>
            </owl:Restriction>
        </rdfs:subClassOf>
        <rdfs:subClassOf>
            <owl:Restriction>
                <owl:onProperty rdf:resource="https://saref.etsi.org/saref4bldg/refrigerantClass"/>
                <owl:allValuesFrom rdf:resource="http://www.w3.org/2001/XMLSchema#string"/>
            </owl:Restriction>
        </rdfs:subClassOf>
        <rdfs:comment xml:lang="en">A compressor is a device that compresses a fluid typically used in a refrigeration circuit.</rdfs:comment>
        <rdfs:label xml:lang="en">Compressor</rdfs:label>
        <rdfs:seeAlso>https://w3id.org/ifc/IFC4_ADD1#IfcCompressor</rdfs:seeAlso>
        <prov:hadPrimarySource rdf:resource="http://www.buildingsmart-tech.org/ifc/IFC4/Add1/html/schema/ifchvacdomain/lexical/ifccompressor.htm"/>
        <prov:hadPrimarySource rdf:resource="http://www.buildingsmart-tech.org/ifc/IFC4/Add1/html/schema/ifchvacdomain/pset/pset_compressortypecommon.htm"/>
    </owl:Class>
    


    <!-- https://saref.etsi.org/saref4bldg/Condenser -->


    <owl:Class rdf:about="https://saref.etsi.org/saref4bldg/Condenser">
        <rdfs:subClassOf rdf:resource="https://saref.etsi.org/saref4bldg/EnergyConversionDevice"/>
        <rdfs:subClassOf>
            <owl:Restriction>
                <owl:onProperty rdf:resource="https://saref.etsi.org/saref4bldg/externalSurfaceArea"/>
                <owl:allValuesFrom rdf:resource="https://saref.etsi.org/core/Measurement"/>
            </owl:Restriction>
        </rdfs:subClassOf>
        <rdfs:subClassOf>
            <owl:Restriction>
                <owl:onProperty rdf:resource="https://saref.etsi.org/saref4bldg/internalRefrigerantVolume"/>
                <owl:allValuesFrom rdf:resource="https://saref.etsi.org/core/Measurement"/>
            </owl:Restriction>
        </rdfs:subClassOf>
        <rdfs:subClassOf>
            <owl:Restriction>
                <owl:onProperty rdf:resource="https://saref.etsi.org/saref4bldg/internalSurfaceArea"/>
                <owl:allValuesFrom rdf:resource="https://saref.etsi.org/core/Measurement"/>
            </owl:Restriction>
        </rdfs:subClassOf>
        <rdfs:subClassOf>
            <owl:Restriction>
                <owl:onProperty rdf:resource="https://saref.etsi.org/saref4bldg/internalWaterVolume"/>
                <owl:allValuesFrom rdf:resource="https://saref.etsi.org/core/Measurement"/>
            </owl:Restriction>
        </rdfs:subClassOf>
        <rdfs:subClassOf>
            <owl:Restriction>
                <owl:onProperty rdf:resource="https://saref.etsi.org/saref4bldg/nominalHeatTransferArea"/>
                <owl:allValuesFrom rdf:resource="https://saref.etsi.org/core/Measurement"/>
            </owl:Restriction>
        </rdfs:subClassOf>
        <rdfs:subClassOf>
            <owl:Restriction>
                <owl:onProperty rdf:resource="https://saref.etsi.org/saref4bldg/nominalHeatTransferCoefficient"/>
                <owl:allValuesFrom rdf:resource="https://saref.etsi.org/core/Measurement"/>
            </owl:Restriction>
        </rdfs:subClassOf>
        <rdfs:subClassOf>
            <owl:Restriction>
                <owl:onProperty rdf:resource="https://saref.etsi.org/saref4bldg/refrigerantClass"/>
                <owl:allValuesFrom rdf:resource="http://www.w3.org/2001/XMLSchema#string"/>
            </owl:Restriction>
        </rdfs:subClassOf>
        <rdfs:comment xml:lang="en">A condenser is a device that is used to dissipate heat, typically by condensing a substance such as a refrigerant from its gaseous to its liquid state.</rdfs:comment>
        <rdfs:label xml:lang="en">Condenser</rdfs:label>
        <rdfs:seeAlso>https://w3id.org/ifc/IFC4_ADD1#IfcCondenser</rdfs:seeAlso>
        <prov:hadPrimarySource rdf:resource="http://www.buildingsmart-tech.org/ifc/IFC4/Add1/html/schema/ifchvacdomain/lexical/ifccondenser.htm"/>
        <prov:hadPrimarySource rdf:resource="http://www.buildingsmart-tech.org/ifc/IFC4/Add1/html/schema/ifchvacdomain/pset/pset_condensertypecommon.htm"/>
    </owl:Class>
    


    <!-- https://saref.etsi.org/saref4bldg/Controller -->


    <owl:Class rdf:about="https://saref.etsi.org/saref4bldg/Controller">
        <rdfs:subClassOf rdf:resource="https://saref.etsi.org/saref4bldg/DistributionControlDevice"/>
        <rdfs:comment xml:lang="en">A controller is a device that monitors inputs and controls outputs within a building automation system.

A controller may be physical (having placement within a spatial structure) or logical (a software interface or aggregated within a programmable physical controller).</rdfs:comment>
        <rdfs:label xml:lang="en">Controller</rdfs:label>
        <rdfs:seeAlso>https://w3id.org/ifc/IFC4_ADD1#IfcController</rdfs:seeAlso>
        <prov:hadPrimarySource rdf:resource="http://www.buildingsmart-tech.org/ifc/IFC4/Add1/html/schema/ifcbuildingcontrolsdomain/lexical/ifccontroller.htm"/>
        <prov:hadPrimarySource rdf:resource="http://www.buildingsmart-tech.org/ifc/IFC4/Add1/html/schema/ifcbuildingcontrolsdomain/pset/pset_controllertypecommon.htm"/>
    </owl:Class>
    


    <!-- https://saref.etsi.org/saref4bldg/CooledBeam -->


    <owl:Class rdf:about="https://saref.etsi.org/saref4bldg/CooledBeam">
        <rdfs:subClassOf rdf:resource="https://saref.etsi.org/saref4bldg/EnergyConversionDevice"/>
        <rdfs:subClassOf>
            <owl:Restriction>
                <owl:onProperty rdf:resource="https://saref.etsi.org/saref4bldg/coilLength"/>
                <owl:allValuesFrom rdf:resource="https://saref.etsi.org/core/Measurement"/>
            </owl:Restriction>
        </rdfs:subClassOf>
        <rdfs:subClassOf>
            <owl:Restriction>
                <owl:onProperty rdf:resource="https://saref.etsi.org/saref4bldg/coilWidth"/>
                <owl:allValuesFrom rdf:resource="https://saref.etsi.org/core/Measurement"/>
            </owl:Restriction>
        </rdfs:subClassOf>
        <rdfs:subClassOf>
            <owl:Restriction>
                <owl:onProperty rdf:resource="https://saref.etsi.org/saref4bldg/nominalCoolingCapacity"/>
                <owl:allValuesFrom rdf:resource="https://saref.etsi.org/core/Measurement"/>
            </owl:Restriction>
        </rdfs:subClassOf>
        <rdfs:subClassOf>
            <owl:Restriction>
                <owl:onProperty rdf:resource="https://saref.etsi.org/saref4bldg/nominalHeatingCapacity"/>
                <owl:allValuesFrom rdf:resource="https://saref.etsi.org/core/Measurement"/>
            </owl:Restriction>
        </rdfs:subClassOf>
        <rdfs:subClassOf>
            <owl:Restriction>
                <owl:onProperty rdf:resource="https://saref.etsi.org/saref4bldg/nominalReturnWaterTemperatureCooling"/>
                <owl:allValuesFrom rdf:resource="https://saref.etsi.org/core/Measurement"/>
            </owl:Restriction>
        </rdfs:subClassOf>
        <rdfs:subClassOf>
            <owl:Restriction>
                <owl:onProperty rdf:resource="https://saref.etsi.org/saref4bldg/nominalReturnWaterTemperatureHeating"/>
                <owl:allValuesFrom rdf:resource="https://saref.etsi.org/core/Measurement"/>
            </owl:Restriction>
        </rdfs:subClassOf>
        <rdfs:subClassOf>
            <owl:Restriction>
                <owl:onProperty rdf:resource="https://saref.etsi.org/saref4bldg/nominalSorroundingHumidityCooling"/>
                <owl:allValuesFrom rdf:resource="https://saref.etsi.org/core/Measurement"/>
            </owl:Restriction>
        </rdfs:subClassOf>
        <rdfs:subClassOf>
            <owl:Restriction>
                <owl:onProperty rdf:resource="https://saref.etsi.org/saref4bldg/nominalSorroundingTemperatureCooling"/>
                <owl:allValuesFrom rdf:resource="https://saref.etsi.org/core/Measurement"/>
            </owl:Restriction>
        </rdfs:subClassOf>
        <rdfs:subClassOf>
            <owl:Restriction>
                <owl:onProperty rdf:resource="https://saref.etsi.org/saref4bldg/nominalSorroundingTemperatureHeating"/>
                <owl:allValuesFrom rdf:resource="https://saref.etsi.org/core/Measurement"/>
            </owl:Restriction>
        </rdfs:subClassOf>
        <rdfs:subClassOf>
            <owl:Restriction>
                <owl:onProperty rdf:resource="https://saref.etsi.org/saref4bldg/nominalSupplyWaterTemperatureCooling"/>
                <owl:allValuesFrom rdf:resource="https://saref.etsi.org/core/Measurement"/>
            </owl:Restriction>
        </rdfs:subClassOf>
        <rdfs:subClassOf>
            <owl:Restriction>
                <owl:onProperty rdf:resource="https://saref.etsi.org/saref4bldg/nominalSupplyWaterTemperatureHeating"/>
                <owl:allValuesFrom rdf:resource="https://saref.etsi.org/core/Measurement"/>
            </owl:Restriction>
        </rdfs:subClassOf>
        <rdfs:subClassOf>
            <owl:Restriction>
                <owl:onProperty rdf:resource="https://saref.etsi.org/saref4bldg/nominalWaterFlowCooling"/>
                <owl:allValuesFrom rdf:resource="https://saref.etsi.org/core/Measurement"/>
            </owl:Restriction>
        </rdfs:subClassOf>
        <rdfs:subClassOf>
            <owl:Restriction>
                <owl:onProperty rdf:resource="https://saref.etsi.org/saref4bldg/nominalWaterFlowHeating"/>
                <owl:allValuesFrom rdf:resource="https://saref.etsi.org/core/Measurement"/>
            </owl:Restriction>
        </rdfs:subClassOf>
        <rdfs:subClassOf>
            <owl:Restriction>
                <owl:onProperty rdf:resource="https://saref.etsi.org/saref4bldg/waterPressureMax"/>
                <owl:allValuesFrom rdf:resource="https://saref.etsi.org/core/Measurement"/>
            </owl:Restriction>
        </rdfs:subClassOf>
        <rdfs:subClassOf>
            <owl:Restriction>
                <owl:onProperty rdf:resource="https://saref.etsi.org/saref4bldg/waterPressureMin"/>
                <owl:allValuesFrom rdf:resource="https://saref.etsi.org/core/Measurement"/>
            </owl:Restriction>
        </rdfs:subClassOf>
        <rdfs:subClassOf>
            <owl:Restriction>
                <owl:onProperty rdf:resource="https://saref.etsi.org/saref4bldg/finishColor"/>
                <owl:allValuesFrom rdf:resource="http://www.w3.org/2001/XMLSchema#string"/>
            </owl:Restriction>
        </rdfs:subClassOf>
        <rdfs:subClassOf>
            <owl:Restriction>
                <owl:onProperty rdf:resource="https://saref.etsi.org/saref4bldg/integratedLightingType"/>
                <owl:allValuesFrom rdf:resource="http://www.w3.org/2001/XMLSchema#string"/>
            </owl:Restriction>
        </rdfs:subClassOf>
        <rdfs:subClassOf>
            <owl:Restriction>
                <owl:onProperty rdf:resource="https://saref.etsi.org/saref4bldg/isFreeHanging"/>
                <owl:allValuesFrom rdf:resource="http://www.w3.org/2001/XMLSchema#boolean"/>
            </owl:Restriction>
        </rdfs:subClassOf>
        <rdfs:subClassOf>
            <owl:Restriction>
                <owl:onProperty rdf:resource="https://saref.etsi.org/saref4bldg/pipeConnectionEnum"/>
                <owl:allValuesFrom rdf:resource="http://www.w3.org/2001/XMLSchema#string"/>
            </owl:Restriction>
        </rdfs:subClassOf>
        <rdfs:subClassOf>
            <owl:Restriction>
                <owl:onProperty rdf:resource="https://saref.etsi.org/saref4bldg/waterFlowControlSystemType"/>
                <owl:allValuesFrom rdf:resource="http://www.w3.org/2001/XMLSchema#string"/>
            </owl:Restriction>
        </rdfs:subClassOf>
        <rdfs:comment xml:lang="en">A cooled beam (or chilled beam) is a device typically used to cool air by circulating a fluid such as chilled water through exposed finned tubes above a space. Typically mounted overhead near or within a ceiling, the cooled beam uses convection to cool the space below it by acting as a heat sink for the naturally rising warm air of the space. Once cooled, the air naturally drops back to the floor where the cycle begins again.</rdfs:comment>
        <rdfs:label xml:lang="en">Cooled beam</rdfs:label>
        <rdfs:seeAlso>https://w3id.org/ifc/IFC4_ADD1#IfcCooledBeam</rdfs:seeAlso>
        <prov:hadPrimarySource rdf:resource="http://www.buildingsmart-tech.org/ifc/IFC4/Add1/html/schema/ifchvacdomain/lexical/ifccooledbeam.htm"/>
        <prov:hadPrimarySource rdf:resource="http://www.buildingsmart-tech.org/ifc/IFC4/Add1/html/schema/ifchvacdomain/pset/pset_cooledbeamtypecommon.htm"/>
    </owl:Class>
    


    <!-- https://saref.etsi.org/saref4bldg/CoolingTower -->


    <owl:Class rdf:about="https://saref.etsi.org/saref4bldg/CoolingTower">
        <rdfs:subClassOf rdf:resource="https://saref.etsi.org/saref4bldg/EnergyConversionDevice"/>
        <rdfs:subClassOf>
            <owl:Restriction>
                <owl:onProperty rdf:resource="https://saref.etsi.org/saref4bldg/ambientDesignDryBulbTemperature"/>
                <owl:allValuesFrom rdf:resource="https://saref.etsi.org/core/Measurement"/>
            </owl:Restriction>
        </rdfs:subClassOf>
        <rdfs:subClassOf>
            <owl:Restriction>
                <owl:onProperty rdf:resource="https://saref.etsi.org/saref4bldg/ambientDesignWetBulbTemperature"/>
                <owl:allValuesFrom rdf:resource="https://saref.etsi.org/core/Measurement"/>
            </owl:Restriction>
        </rdfs:subClassOf>
        <rdfs:subClassOf>
            <owl:Restriction>
                <owl:onProperty rdf:resource="https://saref.etsi.org/saref4bldg/basinReserveVolume"/>
                <owl:allValuesFrom rdf:resource="https://saref.etsi.org/core/Measurement"/>
            </owl:Restriction>
        </rdfs:subClassOf>
        <rdfs:subClassOf>
            <owl:Restriction>
                <owl:onProperty rdf:resource="https://saref.etsi.org/saref4bldg/liftElevationDifference"/>
                <owl:allValuesFrom rdf:resource="https://saref.etsi.org/core/Measurement"/>
            </owl:Restriction>
        </rdfs:subClassOf>
        <rdfs:subClassOf>
            <owl:Restriction>
                <owl:onProperty rdf:resource="https://saref.etsi.org/saref4bldg/nominalCapacity"/>
                <owl:allValuesFrom rdf:resource="https://saref.etsi.org/core/Measurement"/>
            </owl:Restriction>
        </rdfs:subClassOf>
        <rdfs:subClassOf>
            <owl:Restriction>
                <owl:onProperty rdf:resource="https://saref.etsi.org/saref4bldg/operationTemperatureMax"/>
                <owl:allValuesFrom rdf:resource="https://saref.etsi.org/core/Measurement"/>
            </owl:Restriction>
        </rdfs:subClassOf>
        <rdfs:subClassOf>
            <owl:Restriction>
                <owl:onProperty rdf:resource="https://saref.etsi.org/saref4bldg/operationTemperatureMin"/>
                <owl:allValuesFrom rdf:resource="https://saref.etsi.org/core/Measurement"/>
            </owl:Restriction>
        </rdfs:subClassOf>
        <rdfs:subClassOf>
            <owl:Restriction>
                <owl:onProperty rdf:resource="https://saref.etsi.org/saref4bldg/waterRequirement"/>
                <owl:allValuesFrom rdf:resource="https://saref.etsi.org/core/Measurement"/>
            </owl:Restriction>
        </rdfs:subClassOf>
        <rdfs:subClassOf>
            <owl:Restriction>
                <owl:onProperty rdf:resource="https://saref.etsi.org/saref4bldg/capacityControl"/>
                <owl:allValuesFrom rdf:resource="http://www.w3.org/2001/XMLSchema#string"/>
            </owl:Restriction>
        </rdfs:subClassOf>
        <rdfs:subClassOf>
            <owl:Restriction>
                <owl:onProperty rdf:resource="https://saref.etsi.org/saref4bldg/circuitType"/>
                <owl:allValuesFrom rdf:resource="http://www.w3.org/2001/XMLSchema#string"/>
            </owl:Restriction>
        </rdfs:subClassOf>
        <rdfs:subClassOf>
            <owl:Restriction>
                <owl:onProperty rdf:resource="https://saref.etsi.org/saref4bldg/controlStrategy"/>
                <owl:allValuesFrom rdf:resource="http://www.w3.org/2001/XMLSchema#string"/>
            </owl:Restriction>
        </rdfs:subClassOf>
        <rdfs:subClassOf>
            <owl:Restriction>
                <owl:onProperty rdf:resource="https://saref.etsi.org/saref4bldg/flowArrangement"/>
                <owl:allValuesFrom rdf:resource="http://www.w3.org/2001/XMLSchema#string"/>
            </owl:Restriction>
        </rdfs:subClassOf>
        <rdfs:subClassOf>
            <owl:Restriction>
                <owl:onProperty rdf:resource="https://saref.etsi.org/saref4bldg/numberOfCells"/>
                <owl:allValuesFrom rdf:resource="http://www.w3.org/2001/XMLSchema#integer"/>
            </owl:Restriction>
        </rdfs:subClassOf>
        <rdfs:subClassOf>
            <owl:Restriction>
                <owl:onProperty rdf:resource="https://saref.etsi.org/saref4bldg/sprayType"/>
                <owl:allValuesFrom rdf:resource="http://www.w3.org/2001/XMLSchema#string"/>
            </owl:Restriction>
        </rdfs:subClassOf>
        <rdfs:comment xml:lang="en">A cooling tower is a device which rejects heat to ambient air by circulating a fluid such as water through it to reduce its temperature by partial evaporation.</rdfs:comment>
        <rdfs:label xml:lang="en">Cooling tower</rdfs:label>
        <rdfs:seeAlso>https://w3id.org/ifc/IFC4_ADD1#IfcCoolingTower</rdfs:seeAlso>
        <prov:hadPrimarySource rdf:resource="http://www.buildingsmart-tech.org/ifc/IFC4/Add1/html/schema/ifchvacdomain/lexical/ifccoolingtower.htm"/>
        <prov:hadPrimarySource rdf:resource="http://www.buildingsmart-tech.org/ifc/IFC4/Add1/html/schema/ifchvacdomain/pset/pset_coolingtowertypecommon.htm"/>
    </owl:Class>
    


    <!-- https://saref.etsi.org/saref4bldg/Damper -->


    <owl:Class rdf:about="https://saref.etsi.org/saref4bldg/Damper">
        <rdfs:subClassOf rdf:resource="https://saref.etsi.org/saref4bldg/FlowController"/>
        <rdfs:subClassOf>
            <owl:Restriction>
                <owl:onProperty rdf:resource="https://saref.etsi.org/saref4bldg/airFlowRateMax"/>
                <owl:allValuesFrom rdf:resource="https://saref.etsi.org/core/Measurement"/>
            </owl:Restriction>
        </rdfs:subClassOf>
        <rdfs:subClassOf>
            <owl:Restriction>
                <owl:onProperty rdf:resource="https://saref.etsi.org/saref4bldg/bladeThickness"/>
                <owl:allValuesFrom rdf:resource="https://saref.etsi.org/core/Measurement"/>
            </owl:Restriction>
        </rdfs:subClassOf>
        <rdfs:subClassOf>
            <owl:Restriction>
                <owl:onProperty rdf:resource="https://saref.etsi.org/saref4bldg/closeOffRating"/>
                <owl:allValuesFrom rdf:resource="https://saref.etsi.org/core/Measurement"/>
            </owl:Restriction>
        </rdfs:subClassOf>
        <rdfs:subClassOf>
            <owl:Restriction>
                <owl:onProperty rdf:resource="https://saref.etsi.org/saref4bldg/faceArea"/>
                <owl:allValuesFrom rdf:resource="https://saref.etsi.org/core/Measurement"/>
            </owl:Restriction>
        </rdfs:subClassOf>
        <rdfs:subClassOf>
            <owl:Restriction>
                <owl:onProperty rdf:resource="https://saref.etsi.org/saref4bldg/frameDepth"/>
                <owl:allValuesFrom rdf:resource="https://saref.etsi.org/core/Measurement"/>
            </owl:Restriction>
        </rdfs:subClassOf>
        <rdfs:subClassOf>
            <owl:Restriction>
                <owl:onProperty rdf:resource="https://saref.etsi.org/saref4bldg/frameThickness"/>
                <owl:allValuesFrom rdf:resource="https://saref.etsi.org/core/Measurement"/>
            </owl:Restriction>
        </rdfs:subClassOf>
        <rdfs:subClassOf>
            <owl:Restriction>
                <owl:onProperty rdf:resource="https://saref.etsi.org/saref4bldg/leakageFullyClosed"/>
                <owl:allValuesFrom rdf:resource="https://saref.etsi.org/core/Measurement"/>
            </owl:Restriction>
        </rdfs:subClassOf>
        <rdfs:subClassOf>
            <owl:Restriction>
                <owl:onProperty rdf:resource="https://saref.etsi.org/saref4bldg/nominalAirFlowRate"/>
                <owl:allValuesFrom rdf:resource="https://saref.etsi.org/core/Measurement"/>
            </owl:Restriction>
        </rdfs:subClassOf>
        <rdfs:subClassOf>
            <owl:Restriction>
                <owl:onProperty rdf:resource="https://saref.etsi.org/saref4bldg/openPressureDrop"/>
                <owl:allValuesFrom rdf:resource="https://saref.etsi.org/core/Measurement"/>
            </owl:Restriction>
        </rdfs:subClassOf>
        <rdfs:subClassOf>
            <owl:Restriction>
                <owl:onProperty rdf:resource="https://saref.etsi.org/saref4bldg/operationTemperatureMax"/>
                <owl:allValuesFrom rdf:resource="https://saref.etsi.org/core/Measurement"/>
            </owl:Restriction>
        </rdfs:subClassOf>
        <rdfs:subClassOf>
            <owl:Restriction>
                <owl:onProperty rdf:resource="https://saref.etsi.org/saref4bldg/operationTemperatureMin"/>
                <owl:allValuesFrom rdf:resource="https://saref.etsi.org/core/Measurement"/>
            </owl:Restriction>
        </rdfs:subClassOf>
        <rdfs:subClassOf>
            <owl:Restriction>
                <owl:onProperty rdf:resource="https://saref.etsi.org/saref4bldg/temperatureRating"/>
                <owl:allValuesFrom rdf:resource="https://saref.etsi.org/core/Measurement"/>
            </owl:Restriction>
        </rdfs:subClassOf>
        <rdfs:subClassOf>
            <owl:Restriction>
                <owl:onProperty rdf:resource="https://saref.etsi.org/saref4bldg/workingPressureMax"/>
                <owl:allValuesFrom rdf:resource="https://saref.etsi.org/core/Measurement"/>
            </owl:Restriction>
        </rdfs:subClassOf>
        <rdfs:subClassOf>
            <owl:Restriction>
                <owl:onProperty rdf:resource="https://saref.etsi.org/saref4bldg/bladeAction"/>
                <owl:allValuesFrom rdf:resource="http://www.w3.org/2001/XMLSchema#string"/>
            </owl:Restriction>
        </rdfs:subClassOf>
        <rdfs:subClassOf>
            <owl:Restriction>
                <owl:onProperty rdf:resource="https://saref.etsi.org/saref4bldg/bladeEdge"/>
                <owl:allValuesFrom rdf:resource="http://www.w3.org/2001/XMLSchema#string"/>
            </owl:Restriction>
        </rdfs:subClassOf>
        <rdfs:subClassOf>
            <owl:Restriction>
                <owl:onProperty rdf:resource="https://saref.etsi.org/saref4bldg/bladeShape"/>
                <owl:allValuesFrom rdf:resource="http://www.w3.org/2001/XMLSchema#string"/>
            </owl:Restriction>
        </rdfs:subClassOf>
        <rdfs:subClassOf>
            <owl:Restriction>
                <owl:onProperty rdf:resource="https://saref.etsi.org/saref4bldg/frameType"/>
                <owl:allValuesFrom rdf:resource="http://www.w3.org/2001/XMLSchema#string"/>
            </owl:Restriction>
        </rdfs:subClassOf>
        <rdfs:subClassOf>
            <owl:Restriction>
                <owl:onProperty rdf:resource="https://saref.etsi.org/saref4bldg/numberOfBlades"/>
                <owl:allValuesFrom rdf:resource="http://www.w3.org/2001/XMLSchema#integer"/>
            </owl:Restriction>
        </rdfs:subClassOf>
        <rdfs:subClassOf>
            <owl:Restriction>
                <owl:onProperty rdf:resource="https://saref.etsi.org/saref4bldg/operation"/>
                <owl:allValuesFrom rdf:resource="http://www.w3.org/2001/XMLSchema#string"/>
            </owl:Restriction>
        </rdfs:subClassOf>
        <rdfs:subClassOf>
            <owl:Restriction>
                <owl:onProperty rdf:resource="https://saref.etsi.org/saref4bldg/orientation"/>
                <owl:allValuesFrom rdf:resource="http://www.w3.org/2001/XMLSchema#string"/>
            </owl:Restriction>
        </rdfs:subClassOf>
        <rdfs:comment xml:lang="en">A damper typically participates in an HVAC duct distribution system and is used to control or modulate the flow of air.</rdfs:comment>
        <rdfs:label xml:lang="en">Damper</rdfs:label>
        <rdfs:seeAlso>https://w3id.org/ifc/IFC4_ADD1#IfcDamper</rdfs:seeAlso>
        <prov:hadPrimarySource rdf:resource="http://www.buildingsmart-tech.org/ifc/IFC4/Add1/html/schema/ifchvacdomain/lexical/ifcdamper.htm"/>
        <prov:hadPrimarySource rdf:resource="http://www.buildingsmart-tech.org/ifc/IFC4/Add1/html/schema/ifchvacdomain/pset/pset_dampertypecommon.htm"/>
    </owl:Class>
    


    <!-- https://saref.etsi.org/saref4bldg/DistributionControlDevice -->


    <owl:Class rdf:about="https://saref.etsi.org/saref4bldg/DistributionControlDevice">
        <rdfs:subClassOf rdf:resource="https://saref.etsi.org/saref4bldg/DistributionDevice"/>
        <rdfs:comment xml:lang="en">Represents devices of a building automation control system that are used to impart control over elements of a distribution system. (Definition adapated from http://www.buildingsmart-tech.org/ifc/IFC4/Add1/html/schema/ifcsharedbldgserviceelements/lexical/ifcdistributioncontrolelement.htm)</rdfs:comment>
        <rdfs:label xml:lang="en">Distribution control device</rdfs:label>
    </owl:Class>
    


    <!-- https://saref.etsi.org/saref4bldg/DistributionDevice -->


    <owl:Class rdf:about="https://saref.etsi.org/saref4bldg/DistributionDevice">
        <rdfs:subClassOf rdf:resource="https://saref.etsi.org/saref4bldg/BuildingDevice"/>
        <rdfs:comment xml:lang="en">Generalization of all devices that participate in a distribution system. (Definition adapated from http://www.buildingsmart-tech.org/ifc/IFC4/Add1/html/schema/ifcproductextension/lexical/ifcdistributionelement.htm)</rdfs:comment>
        <rdfs:label xml:lang="en">Distribution device</rdfs:label>
    </owl:Class>
    


    <!-- https://saref.etsi.org/saref4bldg/DistributionFlowDevice -->


    <owl:Class rdf:about="https://saref.etsi.org/saref4bldg/DistributionFlowDevice">
        <rdfs:subClassOf rdf:resource="https://saref.etsi.org/saref4bldg/DistributionDevice"/>
        <rdfs:comment xml:lang="en">Represents devices of a distribution system that facilitate the distribution of energy or matter, such as air, water or power. (Definition adapated from http://www.buildingsmart-tech.org/ifc/IFC4/Add1/html/schema/ifcsharedbldgserviceelements/lexical/ifcdistributionflowelement.htm)</rdfs:comment>
        <rdfs:label xml:lang="en">DistributionFlowDevice</rdfs:label>
    </owl:Class>
    


    <!-- https://saref.etsi.org/saref4bldg/DuctSilencer -->


    <owl:Class rdf:about="https://saref.etsi.org/saref4bldg/DuctSilencer">
        <rdfs:subClassOf rdf:resource="https://saref.etsi.org/saref4bldg/FlowTreatmentDevice"/>
        <rdfs:subClassOf>
            <owl:Restriction>
                <owl:onProperty rdf:resource="https://saref.etsi.org/saref4bldg/airFlowRateMax"/>
                <owl:allValuesFrom rdf:resource="https://saref.etsi.org/core/Measurement"/>
            </owl:Restriction>
        </rdfs:subClassOf>
        <rdfs:subClassOf>
            <owl:Restriction>
                <owl:onProperty rdf:resource="https://saref.etsi.org/saref4bldg/airFlowRateMin"/>
                <owl:allValuesFrom rdf:resource="https://saref.etsi.org/core/Measurement"/>
            </owl:Restriction>
        </rdfs:subClassOf>
        <rdfs:subClassOf>
            <owl:Restriction>
                <owl:onProperty rdf:resource="https://saref.etsi.org/saref4bldg/hydraulicDiameter"/>
                <owl:allValuesFrom rdf:resource="https://saref.etsi.org/core/Measurement"/>
            </owl:Restriction>
        </rdfs:subClassOf>
        <rdfs:subClassOf>
            <owl:Restriction>
                <owl:onProperty rdf:resource="https://saref.etsi.org/saref4bldg/length"/>
                <owl:allValuesFrom rdf:resource="https://saref.etsi.org/core/Measurement"/>
            </owl:Restriction>
        </rdfs:subClassOf>
        <rdfs:subClassOf>
            <owl:Restriction>
                <owl:onProperty rdf:resource="https://saref.etsi.org/saref4bldg/operationTemperatureMax"/>
                <owl:allValuesFrom rdf:resource="https://saref.etsi.org/core/Measurement"/>
            </owl:Restriction>
        </rdfs:subClassOf>
        <rdfs:subClassOf>
            <owl:Restriction>
                <owl:onProperty rdf:resource="https://saref.etsi.org/saref4bldg/operationTemperatureMin"/>
                <owl:allValuesFrom rdf:resource="https://saref.etsi.org/core/Measurement"/>
            </owl:Restriction>
        </rdfs:subClassOf>
        <rdfs:subClassOf>
            <owl:Restriction>
                <owl:onProperty rdf:resource="https://saref.etsi.org/saref4bldg/weight"/>
                <owl:allValuesFrom rdf:resource="https://saref.etsi.org/core/Measurement"/>
            </owl:Restriction>
        </rdfs:subClassOf>
        <rdfs:subClassOf>
            <owl:Restriction>
                <owl:onProperty rdf:resource="https://saref.etsi.org/saref4bldg/workingPressureMax"/>
                <owl:allValuesFrom rdf:resource="https://saref.etsi.org/core/Measurement"/>
            </owl:Restriction>
        </rdfs:subClassOf>
        <rdfs:subClassOf>
            <owl:Restriction>
                <owl:onProperty rdf:resource="https://saref.etsi.org/saref4bldg/workingPressureMin"/>
                <owl:allValuesFrom rdf:resource="https://saref.etsi.org/core/Measurement"/>
            </owl:Restriction>
        </rdfs:subClassOf>
        <rdfs:subClassOf>
            <owl:Restriction>
                <owl:onProperty rdf:resource="https://saref.etsi.org/saref4bldg/hasExteriorInsulation"/>
                <owl:allValuesFrom rdf:resource="http://www.w3.org/2001/XMLSchema#boolean"/>
            </owl:Restriction>
        </rdfs:subClassOf>
        <rdfs:comment xml:lang="en">A duct silencer is a device that is typically installed inside a duct distribution system for the purpose of reducing the noise levels from air movement, fan noise, etc. in the adjacent space or downstream of the duct silencer device.</rdfs:comment>
        <rdfs:label xml:lang="en">Duct silencer</rdfs:label>
        <rdfs:seeAlso>https://w3id.org/ifc/IFC4_ADD1#IfcDuctSilencer</rdfs:seeAlso>
        <prov:hadPrimarySource rdf:resource="http://www.buildingsmart-tech.org/ifc/IFC4/Add1/html/schema/ifchvacdomain/lexical/ifcductsilencer.htm"/>
        <prov:hadPrimarySource rdf:resource="http://www.buildingsmart-tech.org/ifc/IFC4/Add1/html/schema/ifchvacdomain/pset/pset_ductsilencertypecommon.htm"/>
    </owl:Class>
    


    <!-- https://saref.etsi.org/saref4bldg/ElectricAppliance -->


    <owl:Class rdf:about="https://saref.etsi.org/saref4bldg/ElectricAppliance">
        <rdfs:subClassOf rdf:resource="https://saref.etsi.org/saref4bldg/FlowTerminal"/>
        <rdfs:comment xml:lang="en">An electric appliance is a device intended for consumer usage that is powered by electricity.

Electric appliances may be fixed in place or may be able to be moved from one space to another. Electric appliances require an electrical supply that may be supplied either by an electrical circuit or provided from a local battery source.</rdfs:comment>
        <rdfs:label xml:lang="en">Electric appliance</rdfs:label>
        <rdfs:seeAlso>https://w3id.org/ifc/IFC4_ADD1#IfcElectricAppliance</rdfs:seeAlso>
        <prov:hadPrimarySource rdf:resource="http://www.buildingsmart-tech.org/ifc/IFC4/Add1/html/schema/ifcelectricaldomain/lexical/ifcelectricappliance.htm"/>
        <prov:hadPrimarySource rdf:resource="http://www.buildingsmart-tech.org/ifc/IFC4/Add1/html/schema/ifcelectricaldomain/pset/pset_electricappliancetypecommon.htm"/>
    </owl:Class>
    


    <!-- https://saref.etsi.org/saref4bldg/ElectricFlowStorageDevice -->


    <owl:Class rdf:about="https://saref.etsi.org/saref4bldg/ElectricFlowStorageDevice">
        <rdfs:subClassOf rdf:resource="https://saref.etsi.org/saref4bldg/FlowStorageDevice"/>
        <rdfs:subClassOf>
            <owl:Restriction>
                <owl:onProperty rdf:resource="https://saref.etsi.org/saref4bldg/nominalFrequency"/>
                <owl:allValuesFrom rdf:resource="https://saref.etsi.org/core/Measurement"/>
            </owl:Restriction>
        </rdfs:subClassOf>
        <rdfs:subClassOf>
            <owl:Restriction>
                <owl:onProperty rdf:resource="https://saref.etsi.org/saref4bldg/nominalSupplyVoltage"/>
                <owl:allValuesFrom rdf:resource="https://saref.etsi.org/core/Measurement"/>
            </owl:Restriction>
        </rdfs:subClassOf>
        <rdfs:subClassOf>
            <owl:Restriction>
                <owl:onProperty rdf:resource="https://saref.etsi.org/saref4bldg/nominalSupplyVoltageMin"/>
                <owl:allValuesFrom rdf:resource="https://saref.etsi.org/core/Measurement"/>
            </owl:Restriction>
        </rdfs:subClassOf>
        <rdfs:comment xml:lang="en">An electric flow storage device is a device in which electrical energy is stored and from which energy may be progressively released.</rdfs:comment>
        <rdfs:label xml:lang="en">Electric flow storage device</rdfs:label>
        <rdfs:seeAlso>https://w3id.org/ifc/IFC4_ADD1#IfcElectricFlowStorageDevice</rdfs:seeAlso>
        <prov:hadPrimarySource rdf:resource="http://www.buildingsmart-tech.org/ifc/IFC4/Add1/html/schema/ifcelectricaldomain/lexical/ifcelectricflowstoragedevice.htm"/>
        <prov:hadPrimarySource rdf:resource="http://www.buildingsmart-tech.org/ifc/IFC4/Add1/html/schema/ifcelectricaldomain/pset/pset_electricflowstoragedevicetypecommon.htm"/>
    </owl:Class>
    


    <!-- https://saref.etsi.org/saref4bldg/ElectricGenerator -->


    <owl:Class rdf:about="https://saref.etsi.org/saref4bldg/ElectricGenerator">
        <rdfs:subClassOf rdf:resource="https://saref.etsi.org/saref4bldg/EnergyConversionDevice"/>
        <rdfs:subClassOf>
            <owl:Restriction>
                <owl:onProperty rdf:resource="https://saref.etsi.org/saref4bldg/electricGeneratorEfficiency"/>
                <owl:allValuesFrom rdf:resource="https://saref.etsi.org/core/Measurement"/>
            </owl:Restriction>
        </rdfs:subClassOf>
        <rdfs:subClassOf>
            <owl:Restriction>
                <owl:onProperty rdf:resource="https://saref.etsi.org/saref4bldg/powerOutputMax"/>
                <owl:allValuesFrom rdf:resource="https://saref.etsi.org/core/Measurement"/>
            </owl:Restriction>
        </rdfs:subClassOf>
        <rdfs:subClassOf>
            <owl:Restriction>
                <owl:onProperty rdf:resource="https://saref.etsi.org/saref4bldg/startCurrentFactor"/>
                <owl:allValuesFrom rdf:resource="https://saref.etsi.org/core/Measurement"/>
            </owl:Restriction>
        </rdfs:subClassOf>
        <rdfs:comment xml:lang="en">An electric generator is an engine that is a machine for converting mechanical energy into electrical energy.</rdfs:comment>
        <rdfs:label xml:lang="en">Electric generator</rdfs:label>
        <rdfs:seeAlso>https://w3id.org/ifc/IFC4_ADD1#IfcElectricGenerator</rdfs:seeAlso>
        <prov:hadPrimarySource rdf:resource="http://www.buildingsmart-tech.org/ifc/IFC4/Add1/html/schema/ifcelectricaldomain/lexical/ifcelectricgenerator.htm"/>
        <prov:hadPrimarySource rdf:resource="http://www.buildingsmart-tech.org/ifc/IFC4/Add1/html/schema/ifcelectricaldomain/pset/pset_electricgeneratortypecommon.htm"/>
    </owl:Class>
    


    <!-- https://saref.etsi.org/saref4bldg/ElectricMotor -->


    <owl:Class rdf:about="https://saref.etsi.org/saref4bldg/ElectricMotor">
        <rdfs:subClassOf rdf:resource="https://saref.etsi.org/saref4bldg/EnergyConversionDevice"/>
        <rdfs:subClassOf>
            <owl:Restriction>
                <owl:onProperty rdf:resource="https://saref.etsi.org/saref4bldg/electricMotorEfficiency"/>
                <owl:allValuesFrom rdf:resource="https://saref.etsi.org/core/Measurement"/>
            </owl:Restriction>
        </rdfs:subClassOf>
        <rdfs:subClassOf>
            <owl:Restriction>
                <owl:onProperty rdf:resource="https://saref.etsi.org/saref4bldg/lockedRotorCurrent"/>
                <owl:allValuesFrom rdf:resource="https://saref.etsi.org/core/Measurement"/>
            </owl:Restriction>
        </rdfs:subClassOf>
        <rdfs:subClassOf>
            <owl:Restriction>
                <owl:onProperty rdf:resource="https://saref.etsi.org/saref4bldg/powerOutputMax"/>
                <owl:allValuesFrom rdf:resource="https://saref.etsi.org/core/Measurement"/>
            </owl:Restriction>
        </rdfs:subClassOf>
        <rdfs:subClassOf>
            <owl:Restriction>
                <owl:onProperty rdf:resource="https://saref.etsi.org/saref4bldg/startCurrentFactor"/>
                <owl:allValuesFrom rdf:resource="https://saref.etsi.org/core/Measurement"/>
            </owl:Restriction>
        </rdfs:subClassOf>
        <rdfs:subClassOf>
            <owl:Restriction>
                <owl:onProperty rdf:resource="https://saref.etsi.org/saref4bldg/startingTime"/>
                <owl:allValuesFrom rdf:resource="https://saref.etsi.org/core/Measurement"/>
            </owl:Restriction>
        </rdfs:subClassOf>
        <rdfs:subClassOf>
            <owl:Restriction>
                <owl:onProperty rdf:resource="https://saref.etsi.org/saref4bldg/teTime"/>
                <owl:allValuesFrom rdf:resource="https://saref.etsi.org/core/Measurement"/>
            </owl:Restriction>
        </rdfs:subClassOf>
        <rdfs:subClassOf>
            <owl:Restriction>
                <owl:onProperty rdf:resource="https://saref.etsi.org/saref4bldg/frameSize"/>
                <owl:allValuesFrom rdf:resource="http://www.w3.org/2001/XMLSchema#string"/>
            </owl:Restriction>
        </rdfs:subClassOf>
        <rdfs:subClassOf>
            <owl:Restriction>
                <owl:onProperty rdf:resource="https://saref.etsi.org/saref4bldg/hasPartWinding"/>
                <owl:allValuesFrom rdf:resource="http://www.w3.org/2001/XMLSchema#boolean"/>
            </owl:Restriction>
        </rdfs:subClassOf>
        <rdfs:subClassOf>
            <owl:Restriction>
                <owl:onProperty rdf:resource="https://saref.etsi.org/saref4bldg/isGuarded"/>
                <owl:allValuesFrom rdf:resource="http://www.w3.org/2001/XMLSchema#boolean"/>
            </owl:Restriction>
        </rdfs:subClassOf>
        <rdfs:subClassOf>
            <owl:Restriction>
                <owl:onProperty rdf:resource="https://saref.etsi.org/saref4bldg/motorEnclosureType"/>
                <owl:allValuesFrom rdf:resource="http://www.w3.org/2001/XMLSchema#string"/>
            </owl:Restriction>
        </rdfs:subClassOf>
        <rdfs:comment xml:lang="en">An electric motor is an engine that is a machine for converting electrical energy into mechanical energy.</rdfs:comment>
        <rdfs:label xml:lang="en">Electric motor</rdfs:label>
        <rdfs:seeAlso>https://w3id.org/ifc/IFC4_ADD1#IfcElectricMotor</rdfs:seeAlso>
        <prov:hadPrimarySource rdf:resource="http://www.buildingsmart-tech.org/ifc/IFC4/Add1/html/schema/ifcelectricaldomain/lexical/ifcelectricmotor.htm"/>
        <prov:hadPrimarySource rdf:resource="http://www.buildingsmart-tech.org/ifc/IFC4/Add1/html/schema/ifcelectricaldomain/pset/pset_electricmotortypecommon.htm"/>
    </owl:Class>
    


    <!-- https://saref.etsi.org/saref4bldg/ElectricTimeControl -->


    <owl:Class rdf:about="https://saref.etsi.org/saref4bldg/ElectricTimeControl">
        <rdfs:subClassOf rdf:resource="https://saref.etsi.org/saref4bldg/FlowController"/>
        <rdfs:comment xml:lang="en">An electric time control is a device that applies control to the provision or flow of electrical energy over time.</rdfs:comment>
        <rdfs:label xml:lang="en">Electric time control</rdfs:label>
        <rdfs:seeAlso>https://w3id.org/ifc/IFC4_ADD1#IfcElectricTimeControl</rdfs:seeAlso>
        <prov:hadPrimarySource rdf:resource="http://www.buildingsmart-tech.org/ifc/IFC4/Add1/html/schema/ifcelectricaldomain/lexical/ifcelectrictimecontrol.htm"/>
        <prov:hadPrimarySource rdf:resource="http://www.buildingsmart-tech.org/ifc/IFC4/Add1/html/schema/ifcelectricaldomain/pset/pset_electrictimecontroltypecommon.htm"/>
    </owl:Class>
    


    <!-- https://saref.etsi.org/saref4bldg/EnergyConversionDevice -->


    <owl:Class rdf:about="https://saref.etsi.org/saref4bldg/EnergyConversionDevice">
        <rdfs:subClassOf rdf:resource="https://saref.etsi.org/saref4bldg/DistributionFlowDevice"/>
        <rdfs:comment xml:lang="en">The distribution flow element EnergyConversionDevice defines the occurrence of a device used to perform energy conversion or heat transfer and typically participates in a flow distribution system.</rdfs:comment>
        <rdfs:label xml:lang="en">Energy conversion device</rdfs:label>
        <rdfs:seeAlso>https://w3id.org/ifc/IFC4_ADD1#IfcEnergyConversionDevice</rdfs:seeAlso>
        <prov:hadPrimarySource rdf:resource="http://www.buildingsmart-tech.org/ifc/IFC4/Add1/html/schema/ifcsharedbldgserviceelements/lexical/ifcenergyconversiondevice.htm"/>
    </owl:Class>
    


    <!-- https://saref.etsi.org/saref4bldg/Engine -->


    <owl:Class rdf:about="https://saref.etsi.org/saref4bldg/Engine">
        <rdfs:subClassOf rdf:resource="https://saref.etsi.org/saref4bldg/EnergyConversionDevice"/>
        <rdfs:subClassOf>
            <owl:Restriction>
                <owl:onProperty rdf:resource="https://saref.etsi.org/saref4bldg/energySource"/>
                <owl:allValuesFrom rdf:resource="http://www.w3.org/2001/XMLSchema#string"/>
            </owl:Restriction>
        </rdfs:subClassOf>
        <rdfs:comment xml:lang="en">An engine is a device that converts fuel into mechanical energy through combustion.</rdfs:comment>
        <rdfs:label xml:lang="en">Engine</rdfs:label>
        <rdfs:seeAlso>https://w3id.org/ifc/IFC4_ADD1#IfcEngine</rdfs:seeAlso>
        <prov:hadPrimarySource rdf:resource="http://www.buildingsmart-tech.org/ifc/IFC4/Add1/html/schema/ifchvacdomain/lexical/ifcengine.htm"/>
        <prov:hadPrimarySource rdf:resource="http://www.buildingsmart-tech.org/ifc/IFC4/Add1/html/schema/ifchvacdomain/pset/pset_enginetypecommon.htm"/>
    </owl:Class>
    


    <!-- https://saref.etsi.org/saref4bldg/EvaporativeCooler -->


    <owl:Class rdf:about="https://saref.etsi.org/saref4bldg/EvaporativeCooler">
        <rdfs:subClassOf rdf:resource="https://saref.etsi.org/saref4bldg/EnergyConversionDevice"/>
        <rdfs:subClassOf>
            <owl:Restriction>
                <owl:onProperty rdf:resource="https://saref.etsi.org/saref4bldg/heatExchangeArea"/>
                <owl:allValuesFrom rdf:resource="https://saref.etsi.org/core/Measurement"/>
            </owl:Restriction>
        </rdfs:subClassOf>
        <rdfs:subClassOf>
            <owl:Restriction>
                <owl:onProperty rdf:resource="https://saref.etsi.org/saref4bldg/operationTemperatureMax"/>
                <owl:allValuesFrom rdf:resource="https://saref.etsi.org/core/Measurement"/>
            </owl:Restriction>
        </rdfs:subClassOf>
        <rdfs:subClassOf>
            <owl:Restriction>
                <owl:onProperty rdf:resource="https://saref.etsi.org/saref4bldg/operationTemperatureMin"/>
                <owl:allValuesFrom rdf:resource="https://saref.etsi.org/core/Measurement"/>
            </owl:Restriction>
        </rdfs:subClassOf>
        <rdfs:subClassOf>
            <owl:Restriction>
                <owl:onProperty rdf:resource="https://saref.etsi.org/saref4bldg/waterRequirement"/>
                <owl:allValuesFrom rdf:resource="https://saref.etsi.org/core/Measurement"/>
            </owl:Restriction>
        </rdfs:subClassOf>
        <rdfs:subClassOf>
            <owl:Restriction>
                <owl:onProperty rdf:resource="https://saref.etsi.org/saref4bldg/flowArrangement"/>
                <owl:allValuesFrom rdf:resource="http://www.w3.org/2001/XMLSchema#string"/>
            </owl:Restriction>
        </rdfs:subClassOf>
        <rdfs:comment xml:lang="en">An evaporative cooler is a device that cools air by saturating it with water vapor.</rdfs:comment>
        <rdfs:label xml:lang="en">Evaporative cooler</rdfs:label>
        <rdfs:seeAlso>https://w3id.org/ifc/IFC4_ADD1#IfcEvaporativeCooler</rdfs:seeAlso>
        <prov:hadPrimarySource rdf:resource="http://www.buildingsmart-tech.org/ifc/IFC4/Add1/html/schema/ifchvacdomain/lexical/ifcevaporativecooler.htm"/>
        <prov:hadPrimarySource rdf:resource="http://www.buildingsmart-tech.org/ifc/IFC4/Add1/html/schema/ifchvacdomain/pset/pset_evaporativecoolertypecommon.htm"/>
    </owl:Class>
    


    <!-- https://saref.etsi.org/saref4bldg/Evaporator -->


    <owl:Class rdf:about="https://saref.etsi.org/saref4bldg/Evaporator">
        <rdfs:subClassOf rdf:resource="https://saref.etsi.org/saref4bldg/EnergyConversionDevice"/>
        <rdfs:subClassOf>
            <owl:Restriction>
                <owl:onProperty rdf:resource="https://saref.etsi.org/saref4bldg/externalSurfaceArea"/>
                <owl:allValuesFrom rdf:resource="https://saref.etsi.org/core/Measurement"/>
            </owl:Restriction>
        </rdfs:subClassOf>
        <rdfs:subClassOf>
            <owl:Restriction>
                <owl:onProperty rdf:resource="https://saref.etsi.org/saref4bldg/internalRefrigerantVolume"/>
                <owl:allValuesFrom rdf:resource="https://saref.etsi.org/core/Measurement"/>
            </owl:Restriction>
        </rdfs:subClassOf>
        <rdfs:subClassOf>
            <owl:Restriction>
                <owl:onProperty rdf:resource="https://saref.etsi.org/saref4bldg/internalSurfaceArea"/>
                <owl:allValuesFrom rdf:resource="https://saref.etsi.org/core/Measurement"/>
            </owl:Restriction>
        </rdfs:subClassOf>
        <rdfs:subClassOf>
            <owl:Restriction>
                <owl:onProperty rdf:resource="https://saref.etsi.org/saref4bldg/internalWaterVolume"/>
                <owl:allValuesFrom rdf:resource="https://saref.etsi.org/core/Measurement"/>
            </owl:Restriction>
        </rdfs:subClassOf>
        <rdfs:subClassOf>
            <owl:Restriction>
                <owl:onProperty rdf:resource="https://saref.etsi.org/saref4bldg/nominalHeatTransferArea"/>
                <owl:allValuesFrom rdf:resource="https://saref.etsi.org/core/Measurement"/>
            </owl:Restriction>
        </rdfs:subClassOf>
        <rdfs:subClassOf>
            <owl:Restriction>
                <owl:onProperty rdf:resource="https://saref.etsi.org/saref4bldg/nominalHeatTransferCoefficient"/>
                <owl:allValuesFrom rdf:resource="https://saref.etsi.org/core/Measurement"/>
            </owl:Restriction>
        </rdfs:subClassOf>
        <rdfs:subClassOf>
            <owl:Restriction>
                <owl:onProperty rdf:resource="https://saref.etsi.org/saref4bldg/evaporationCoolant"/>
                <owl:allValuesFrom rdf:resource="http://www.w3.org/2001/XMLSchema#string"/>
            </owl:Restriction>
        </rdfs:subClassOf>
        <rdfs:subClassOf>
            <owl:Restriction>
                <owl:onProperty rdf:resource="https://saref.etsi.org/saref4bldg/evaporationMediumType"/>
                <owl:allValuesFrom rdf:resource="http://www.w3.org/2001/XMLSchema#string"/>
            </owl:Restriction>
        </rdfs:subClassOf>
        <rdfs:subClassOf>
            <owl:Restriction>
                <owl:onProperty rdf:resource="https://saref.etsi.org/saref4bldg/refrigerantClass"/>
                <owl:allValuesFrom rdf:resource="http://www.w3.org/2001/XMLSchema#string"/>
            </owl:Restriction>
        </rdfs:subClassOf>
        <rdfs:comment xml:lang="en">An evaporator is a device in which a liquid refrigerent is vaporized and absorbs heat from the surrounding fluid.</rdfs:comment>
        <rdfs:label xml:lang="en">Evaporator</rdfs:label>
        <rdfs:seeAlso>https://w3id.org/ifc/IFC4_ADD1#IfcEvaporator</rdfs:seeAlso>
        <prov:hadPrimarySource rdf:resource="http://www.buildingsmart-tech.org/ifc/IFC4/Add1/html/schema/ifchvacdomain/lexical/ifcevaporator.htm"/>
        <prov:hadPrimarySource rdf:resource="http://www.buildingsmart-tech.org/ifc/IFC4/Add1/html/schema/ifchvacdomain/pset/pset_evaporatortypecommon.htm"/>
    </owl:Class>
    


    <!-- https://saref.etsi.org/saref4bldg/Fan -->


    <owl:Class rdf:about="https://saref.etsi.org/saref4bldg/Fan">
        <rdfs:subClassOf rdf:resource="https://saref.etsi.org/saref4bldg/FlowMovingDevice"/>
        <rdfs:subClassOf>
            <owl:Restriction>
                <owl:onProperty rdf:resource="https://saref.etsi.org/saref4bldg/nominalAirFlowRate"/>
                <owl:allValuesFrom rdf:resource="https://saref.etsi.org/core/Measurement"/>
            </owl:Restriction>
        </rdfs:subClassOf>
        <rdfs:subClassOf>
            <owl:Restriction>
                <owl:onProperty rdf:resource="https://saref.etsi.org/saref4bldg/nominalPowerRate"/>
                <owl:allValuesFrom rdf:resource="https://saref.etsi.org/core/Measurement"/>
            </owl:Restriction>
        </rdfs:subClassOf>
        <rdfs:subClassOf>
            <owl:Restriction>
                <owl:onProperty rdf:resource="https://saref.etsi.org/saref4bldg/nominalRotationSpeed"/>
                <owl:allValuesFrom rdf:resource="https://saref.etsi.org/core/Measurement"/>
            </owl:Restriction>
        </rdfs:subClassOf>
        <rdfs:subClassOf>
            <owl:Restriction>
                <owl:onProperty rdf:resource="https://saref.etsi.org/saref4bldg/nominalStaticPressure"/>
                <owl:allValuesFrom rdf:resource="https://saref.etsi.org/core/Measurement"/>
            </owl:Restriction>
        </rdfs:subClassOf>
        <rdfs:subClassOf>
            <owl:Restriction>
                <owl:onProperty rdf:resource="https://saref.etsi.org/saref4bldg/nominalTotalPressure"/>
                <owl:allValuesFrom rdf:resource="https://saref.etsi.org/core/Measurement"/>
            </owl:Restriction>
        </rdfs:subClassOf>
        <rdfs:subClassOf>
            <owl:Restriction>
                <owl:onProperty rdf:resource="https://saref.etsi.org/saref4bldg/operationTemperatureMax"/>
                <owl:allValuesFrom rdf:resource="https://saref.etsi.org/core/Measurement"/>
            </owl:Restriction>
        </rdfs:subClassOf>
        <rdfs:subClassOf>
            <owl:Restriction>
                <owl:onProperty rdf:resource="https://saref.etsi.org/saref4bldg/operationTemperatureMin"/>
                <owl:allValuesFrom rdf:resource="https://saref.etsi.org/core/Measurement"/>
            </owl:Restriction>
        </rdfs:subClassOf>
        <rdfs:subClassOf>
            <owl:Restriction>
                <owl:onProperty rdf:resource="https://saref.etsi.org/saref4bldg/operationalRiterial"/>
                <owl:allValuesFrom rdf:resource="https://saref.etsi.org/core/Measurement"/>
            </owl:Restriction>
        </rdfs:subClassOf>
        <rdfs:subClassOf>
            <owl:Restriction>
                <owl:onProperty rdf:resource="https://saref.etsi.org/saref4bldg/capacityControlType"/>
                <owl:allValuesFrom rdf:resource="http://www.w3.org/2001/XMLSchema#string"/>
            </owl:Restriction>
        </rdfs:subClassOf>
        <rdfs:subClassOf>
            <owl:Restriction>
                <owl:onProperty rdf:resource="https://saref.etsi.org/saref4bldg/motorDriveType"/>
                <owl:allValuesFrom rdf:resource="http://www.w3.org/2001/XMLSchema#string"/>
            </owl:Restriction>
        </rdfs:subClassOf>
        <rdfs:comment xml:lang="en">A fan is a device which imparts mechanical work on a gas. A typical usage of a fan is to induce airflow in a building services air distribution system.</rdfs:comment>
        <rdfs:label xml:lang="en">Fan</rdfs:label>
        <rdfs:seeAlso>https://w3id.org/ifc/IFC4_ADD1#IfcFan</rdfs:seeAlso>
        <prov:hadPrimarySource rdf:resource="http://www.buildingsmart-tech.org/ifc/IFC4/Add1/html/schema/ifchvacdomain/lexical/ifcfan.htm"/>
        <prov:hadPrimarySource rdf:resource="http://www.buildingsmart-tech.org/ifc/IFC4/Add1/html/schema/ifchvacdomain/pset/pset_fantypecommon.htm"/>
    </owl:Class>
    


    <!-- https://saref.etsi.org/saref4bldg/Filter -->


    <owl:Class rdf:about="https://saref.etsi.org/saref4bldg/Filter">
        <rdfs:subClassOf rdf:resource="https://saref.etsi.org/saref4bldg/FlowTreatmentDevice"/>
        <rdfs:subClassOf>
            <owl:Restriction>
                <owl:onProperty rdf:resource="https://saref.etsi.org/saref4bldg/finalResistance"/>
                <owl:allValuesFrom rdf:resource="https://saref.etsi.org/core/Measurement"/>
            </owl:Restriction>
        </rdfs:subClassOf>
        <rdfs:subClassOf>
            <owl:Restriction>
                <owl:onProperty rdf:resource="https://saref.etsi.org/saref4bldg/fluidFlowRateMax"/>
                <owl:allValuesFrom rdf:resource="https://saref.etsi.org/core/Measurement"/>
            </owl:Restriction>
        </rdfs:subClassOf>
        <rdfs:subClassOf>
            <owl:Restriction>
                <owl:onProperty rdf:resource="https://saref.etsi.org/saref4bldg/fluidFlowRateMin"/>
                <owl:allValuesFrom rdf:resource="https://saref.etsi.org/core/Measurement"/>
            </owl:Restriction>
        </rdfs:subClassOf>
        <rdfs:subClassOf>
            <owl:Restriction>
                <owl:onProperty rdf:resource="https://saref.etsi.org/saref4bldg/initialResistance"/>
                <owl:allValuesFrom rdf:resource="https://saref.etsi.org/core/Measurement"/>
            </owl:Restriction>
        </rdfs:subClassOf>
        <rdfs:subClassOf>
            <owl:Restriction>
                <owl:onProperty rdf:resource="https://saref.etsi.org/saref4bldg/nominalFilterFaceVelocity"/>
                <owl:allValuesFrom rdf:resource="https://saref.etsi.org/core/Measurement"/>
            </owl:Restriction>
        </rdfs:subClassOf>
        <rdfs:subClassOf>
            <owl:Restriction>
                <owl:onProperty rdf:resource="https://saref.etsi.org/saref4bldg/nominalFlowRate"/>
                <owl:allValuesFrom rdf:resource="https://saref.etsi.org/core/Measurement"/>
            </owl:Restriction>
        </rdfs:subClassOf>
        <rdfs:subClassOf>
            <owl:Restriction>
                <owl:onProperty rdf:resource="https://saref.etsi.org/saref4bldg/nominalMediaSurfaceVelocity"/>
                <owl:allValuesFrom rdf:resource="https://saref.etsi.org/core/Measurement"/>
            </owl:Restriction>
        </rdfs:subClassOf>
        <rdfs:subClassOf>
            <owl:Restriction>
                <owl:onProperty rdf:resource="https://saref.etsi.org/saref4bldg/nominalParticleGeometricMeanDiameter"/>
                <owl:allValuesFrom rdf:resource="https://saref.etsi.org/core/Measurement"/>
            </owl:Restriction>
        </rdfs:subClassOf>
        <rdfs:subClassOf>
            <owl:Restriction>
                <owl:onProperty rdf:resource="https://saref.etsi.org/saref4bldg/nominalParticleGeometricStandardDeviation"/>
                <owl:allValuesFrom rdf:resource="https://saref.etsi.org/core/Measurement"/>
            </owl:Restriction>
        </rdfs:subClassOf>
        <rdfs:subClassOf>
            <owl:Restriction>
                <owl:onProperty rdf:resource="https://saref.etsi.org/saref4bldg/nominalPressureDrop"/>
                <owl:allValuesFrom rdf:resource="https://saref.etsi.org/core/Measurement"/>
            </owl:Restriction>
        </rdfs:subClassOf>
        <rdfs:subClassOf>
            <owl:Restriction>
                <owl:onProperty rdf:resource="https://saref.etsi.org/saref4bldg/operationTemperatureMax"/>
                <owl:allValuesFrom rdf:resource="https://saref.etsi.org/core/Measurement"/>
            </owl:Restriction>
        </rdfs:subClassOf>
        <rdfs:subClassOf>
            <owl:Restriction>
                <owl:onProperty rdf:resource="https://saref.etsi.org/saref4bldg/operationTemperatureMin"/>
                <owl:allValuesFrom rdf:resource="https://saref.etsi.org/core/Measurement"/>
            </owl:Restriction>
        </rdfs:subClassOf>
        <rdfs:subClassOf>
            <owl:Restriction>
                <owl:onProperty rdf:resource="https://saref.etsi.org/saref4bldg/weight"/>
                <owl:allValuesFrom rdf:resource="https://saref.etsi.org/core/Measurement"/>
            </owl:Restriction>
        </rdfs:subClassOf>
        <rdfs:comment xml:lang="en">A filter is an apparatus used to remove particulate or gaseous matter from fluids and gases.</rdfs:comment>
        <rdfs:label xml:lang="en">Filter</rdfs:label>
        <rdfs:seeAlso>https://w3id.org/ifc/IFC4_ADD1#IfcFilter</rdfs:seeAlso>
        <prov:hadPrimarySource rdf:resource="http://www.buildingsmart-tech.org/ifc/IFC4/Add1/html/schema/ifchvacdomain/lexical/ifcfilter.htm"/>
        <prov:hadPrimarySource rdf:resource="http://www.buildingsmart-tech.org/ifc/IFC4/Add1/html/schema/ifchvacdomain/pset/pset_filtertypecommon.htm"/>
    </owl:Class>
    


    <!-- https://saref.etsi.org/saref4bldg/FireSuppressionTerminal -->


    <owl:Class rdf:about="https://saref.etsi.org/saref4bldg/FireSuppressionTerminal">
        <rdfs:subClassOf rdf:resource="https://saref.etsi.org/saref4bldg/FlowTerminal"/>
        <rdfs:comment xml:lang="en">A fire suppression terminal has the purpose of delivering a fluid (gas or liquid) that will suppress a fire.

A fire suppression terminal provides for all forms of sprinkler, spreader and other form of terminal that is connected to a pipework system and intended to act in the role of suppressing a fire.</rdfs:comment>
        <rdfs:label xml:lang="en">Fire suppression terminal</rdfs:label>
        <rdfs:seeAlso>https://w3id.org/ifc/IFC4_ADD1#IfcFireSuppressionTerminal</rdfs:seeAlso>
        <prov:hadPrimarySource rdf:resource="http://www.buildingsmart-tech.org/ifc/IFC4/Add1/html/schema/ifcplumbingfireprotectiondomain/lexical/ifcfiresuppressionterminal.htm"/>
        <prov:hadPrimarySource rdf:resource="http://www.buildingsmart-tech.org/ifc/IFC4/Add1/html/schema/ifcplumbingfireprotectiondomain/pset/pset_firesuppressionterminaltypecommon.htm"/>
    </owl:Class>
    


    <!-- https://saref.etsi.org/saref4bldg/FlowController -->


    <owl:Class rdf:about="https://saref.etsi.org/saref4bldg/FlowController">
        <rdfs:subClassOf rdf:resource="https://saref.etsi.org/saref4bldg/DistributionFlowDevice"/>
        <rdfs:comment xml:lang="en">The distribution flow element FlowController defines the occurrence of elements of a distribution system that are used to regulate flow through a distribution system. Examples include dampers, valves, switches, and relays.</rdfs:comment>
        <rdfs:label xml:lang="en">Flow controller</rdfs:label>
        <rdfs:seeAlso>https://w3id.org/ifc/IFC4_ADD1#IfcFlowController</rdfs:seeAlso>
        <prov:hadPrimarySource rdf:resource="http://www.buildingsmart-tech.org/ifc/IFC4/Add1/html/schema/ifcsharedbldgserviceelements/lexical/ifcflowcontroller.htm"/>
    </owl:Class>
    


    <!-- https://saref.etsi.org/saref4bldg/FlowInstrument -->


    <owl:Class rdf:about="https://saref.etsi.org/saref4bldg/FlowInstrument">
        <rdfs:subClassOf rdf:resource="https://saref.etsi.org/saref4bldg/DistributionControlDevice"/>
        <rdfs:comment xml:lang="en">A flow instrument reads and displays the value of a particular property of a system at a point, or displays the difference in the value of a property between two points.

Instrumentation is typically for the purpose of determining the value of the property at a point in time. It is not the purpose of an instrument to record or integrate the values over time (although they may be connected to recording devices that do perform such a function). This entity provides for all forms of mechanical flow instrument (thermometers, pressure gauges etc.) and electrical flow instruments (ammeters, voltmeters etc.)</rdfs:comment>
        <rdfs:label xml:lang="en">Flow instrument</rdfs:label>
        <rdfs:seeAlso>https://w3id.org/ifc/IFC4_ADD1#IfcFlowInstrument</rdfs:seeAlso>
        <prov:hadPrimarySource rdf:resource="http://www.buildingsmart-tech.org/ifc/IFC4/Add1/html/schema/ifcbuildingcontrolsdomain/lexical/ifcflowinstrument.htm"/>
        <prov:hadPrimarySource rdf:resource="http://www.buildingsmart-tech.org/ifc/IFC4/Add1/html/schema/ifcbuildingcontrolsdomain/pset/pset_flowinstrumenttypecommon.htm"/>
    </owl:Class>
    


    <!-- https://saref.etsi.org/saref4bldg/FlowMeter -->


    <owl:Class rdf:about="https://saref.etsi.org/saref4bldg/FlowMeter">
        <rdfs:subClassOf rdf:resource="https://saref.etsi.org/saref4bldg/FlowController"/>
        <rdfs:subClassOf>
            <owl:Restriction>
                <owl:onProperty rdf:resource="https://saref.etsi.org/saref4bldg/readOutType"/>
                <owl:allValuesFrom rdf:resource="http://www.w3.org/2001/XMLSchema#string"/>
            </owl:Restriction>
        </rdfs:subClassOf>
        <rdfs:subClassOf>
            <owl:Restriction>
                <owl:onProperty rdf:resource="https://saref.etsi.org/saref4bldg/remoteReading"/>
                <owl:allValuesFrom rdf:resource="http://www.w3.org/2001/XMLSchema#boolean"/>
            </owl:Restriction>
        </rdfs:subClassOf>
        <rdfs:comment xml:lang="en">A flow meter is a device that is used to measure the flow rate in a system.</rdfs:comment>
        <rdfs:label xml:lang="en">Flow meter</rdfs:label>
        <rdfs:seeAlso>https://w3id.org/ifc/IFC4_ADD1#IfcFlowMeter</rdfs:seeAlso>
        <prov:hadPrimarySource rdf:resource="http://www.buildingsmart-tech.org/ifc/IFC4/Add1/html/schema/ifchvacdomain/lexical/ifcflowmeter.htm"/>
        <prov:hadPrimarySource rdf:resource="http://www.buildingsmart-tech.org/ifc/IFC4/Add1/html/schema/ifchvacdomain/pset/pset_flowmetertypecommon.htm"/>
    </owl:Class>
    


    <!-- https://saref.etsi.org/saref4bldg/FlowMovingDevice -->


    <owl:Class rdf:about="https://saref.etsi.org/saref4bldg/FlowMovingDevice">
        <rdfs:subClassOf rdf:resource="https://saref.etsi.org/saref4bldg/DistributionFlowDevice"/>
        <rdfs:comment xml:lang="en">The distribution flow element FlowMovingDevice defines the occurrence of an apparatus used to distribute, circulate or perform conveyance of fluids, including liquids and gases (such as a pump or fan), and typically participates in a flow distribution system.</rdfs:comment>
        <rdfs:label xml:lang="en">Flow moving device</rdfs:label>
        <rdfs:seeAlso>https://w3id.org/ifc/IFC4_ADD1#IfcFlowMovingDevice</rdfs:seeAlso>
        <prov:hadPrimarySource rdf:resource="http://www.buildingsmart-tech.org/ifc/IFC4/Add1/html/schema/ifcsharedbldgserviceelements/lexical/ifcflowmovingdevice.htm"/>
    </owl:Class>
    


    <!-- https://saref.etsi.org/saref4bldg/FlowStorageDevice -->


    <owl:Class rdf:about="https://saref.etsi.org/saref4bldg/FlowStorageDevice">
        <rdfs:subClassOf rdf:resource="https://saref.etsi.org/saref4bldg/DistributionFlowDevice"/>
        <rdfs:comment xml:lang="en">The distribution flow element FlowStorageDevice defines the occurrence of a device that participates in a distribution system and is used for temporary storage (such as a tank).</rdfs:comment>
        <rdfs:label xml:lang="en">Flow storage device</rdfs:label>
        <rdfs:seeAlso>https://w3id.org/ifc/IFC4_ADD1#IfcFlowStorageDevice</rdfs:seeAlso>
        <prov:hadPrimarySource rdf:resource="http://www.buildingsmart-tech.org/ifc/IFC4/Add1/html/schema/ifcsharedbldgserviceelements/lexical/ifcflowstoragedevice.htm"/>
    </owl:Class>
    


    <!-- https://saref.etsi.org/saref4bldg/FlowTerminal -->


    <owl:Class rdf:about="https://saref.etsi.org/saref4bldg/FlowTerminal">
        <rdfs:subClassOf rdf:resource="https://saref.etsi.org/saref4bldg/DistributionFlowDevice"/>
        <rdfs:comment xml:lang="en">The distribution flow element FlowTerminal defines the occurrence of a permanently attached element that acts as a terminus or beginning of a distribution system (such as an air outlet, drain, water closet, or sink). A terminal is typically a point at which a system interfaces with an external environment.</rdfs:comment>
        <rdfs:label xml:lang="en">Flow terminal</rdfs:label>
        <rdfs:seeAlso>https://w3id.org/ifc/IFC4_ADD1#IfcFlowTerminal</rdfs:seeAlso>
        <prov:hadPrimarySource rdf:resource="http://www.buildingsmart-tech.org/ifc/IFC4/Add1/html/schema/ifcsharedbldgserviceelements/lexical/ifcflowterminal.htm"/>
    </owl:Class>
    


    <!-- https://saref.etsi.org/saref4bldg/FlowTreatmentDevice -->


    <owl:Class rdf:about="https://saref.etsi.org/saref4bldg/FlowTreatmentDevice">
        <rdfs:subClassOf rdf:resource="https://saref.etsi.org/saref4bldg/DistributionFlowDevice"/>
        <rdfs:comment xml:lang="en">The distribution flow element FlowTreatmentDevice defines the occurrence of a device typically used to remove unwanted matter from a fluid, either liquid or gas, and typically participates in a flow distribution system.</rdfs:comment>
        <rdfs:label xml:lang="en">Flow treatment device</rdfs:label>
        <rdfs:seeAlso>https://w3id.org/ifc/IFC4_ADD1#IfcFlowTreatmentDevice</rdfs:seeAlso>
        <prov:hadPrimarySource rdf:resource="http://www.buildingsmart-tech.org/ifc/IFC4/Add1/html/schema/ifcsharedbldgserviceelements/lexical/ifcflowtreatmentdevice.htm"/>
    </owl:Class>
    


    <!-- https://saref.etsi.org/saref4bldg/HeatExchanger -->


    <owl:Class rdf:about="https://saref.etsi.org/saref4bldg/HeatExchanger">
        <rdfs:subClassOf rdf:resource="https://saref.etsi.org/saref4bldg/EnergyConversionDevice"/>
        <rdfs:subClassOf>
            <owl:Restriction>
                <owl:onProperty rdf:resource="https://saref.etsi.org/saref4bldg/arrangement"/>
                <owl:allValuesFrom rdf:resource="http://www.w3.org/2001/XMLSchema#string"/>
            </owl:Restriction>
        </rdfs:subClassOf>
        <rdfs:comment xml:lang="en">A heat exchanger is a device used to provide heat transfer between non-mixing media such as plate and shell and tube heat exchangers. HeatExchanger is commonly used on water-side distribution systems to recover energy from a liquid to another liquid (typically water-based), whereas AirToAirHeatRecovery is commonly used on air-side distribution systems to recover energy from a gas to a gas (usually air).</rdfs:comment>
        <rdfs:label xml:lang="en">Heat exchanger</rdfs:label>
        <rdfs:seeAlso>https://w3id.org/ifc/IFC4_ADD1#IfcHeatExchanger</rdfs:seeAlso>
        <prov:hadPrimarySource rdf:resource="http://www.buildingsmart-tech.org/ifc/IFC4/Add1/html/schema/ifchvacdomain/lexical/ifcheatexchanger.htm"/>
        <prov:hadPrimarySource rdf:resource="http://www.buildingsmart-tech.org/ifc/IFC4/Add1/html/schema/ifchvacdomain/pset/pset_heatexchangertypecommon.htm"/>
    </owl:Class>
    


    <!-- https://saref.etsi.org/saref4bldg/Humidifier -->


    <owl:Class rdf:about="https://saref.etsi.org/saref4bldg/Humidifier">
        <rdfs:subClassOf rdf:resource="https://saref.etsi.org/saref4bldg/EnergyConversionDevice"/>
        <rdfs:subClassOf>
            <owl:Restriction>
                <owl:onProperty rdf:resource="https://saref.etsi.org/saref4bldg/nominalAirFlowRate"/>
                <owl:allValuesFrom rdf:resource="https://saref.etsi.org/core/Measurement"/>
            </owl:Restriction>
        </rdfs:subClassOf>
        <rdfs:subClassOf>
            <owl:Restriction>
                <owl:onProperty rdf:resource="https://saref.etsi.org/saref4bldg/nominalMoistureGain"/>
                <owl:allValuesFrom rdf:resource="https://saref.etsi.org/core/Measurement"/>
            </owl:Restriction>
        </rdfs:subClassOf>
        <rdfs:subClassOf>
            <owl:Restriction>
                <owl:onProperty rdf:resource="https://saref.etsi.org/saref4bldg/waterRequirement"/>
                <owl:allValuesFrom rdf:resource="https://saref.etsi.org/core/Measurement"/>
            </owl:Restriction>
        </rdfs:subClassOf>
        <rdfs:subClassOf>
            <owl:Restriction>
                <owl:onProperty rdf:resource="https://saref.etsi.org/saref4bldg/weight"/>
                <owl:allValuesFrom rdf:resource="https://saref.etsi.org/core/Measurement"/>
            </owl:Restriction>
        </rdfs:subClassOf>
        <rdfs:subClassOf>
            <owl:Restriction>
                <owl:onProperty rdf:resource="https://saref.etsi.org/saref4bldg/application"/>
                <owl:allValuesFrom rdf:resource="http://www.w3.org/2001/XMLSchema#string"/>
            </owl:Restriction>
        </rdfs:subClassOf>
        <rdfs:subClassOf>
            <owl:Restriction>
                <owl:onProperty rdf:resource="https://saref.etsi.org/saref4bldg/internalControl"/>
                <owl:allValuesFrom rdf:resource="http://www.w3.org/2001/XMLSchema#string"/>
            </owl:Restriction>
        </rdfs:subClassOf>
        <rdfs:comment xml:lang="en">A humidifier is a device that adds moisture into the air.</rdfs:comment>
        <rdfs:label xml:lang="en">Humidifier</rdfs:label>
        <rdfs:seeAlso>https://w3id.org/ifc/IFC4_ADD1#IfcHumidifier</rdfs:seeAlso>
        <prov:hadPrimarySource rdf:resource="http://www.buildingsmart-tech.org/ifc/IFC4/Add1/html/schema/ifchvacdomain/lexical/ifchumidifier.htm"/>
        <prov:hadPrimarySource rdf:resource="http://www.buildingsmart-tech.org/ifc/IFC4/Add1/html/schema/ifchvacdomain/pset/pset_humidifiertypecommon.htm"/>
    </owl:Class>
    


    <!-- https://saref.etsi.org/saref4bldg/Interceptor -->


    <owl:Class rdf:about="https://saref.etsi.org/saref4bldg/Interceptor">
        <rdfs:subClassOf rdf:resource="https://saref.etsi.org/saref4bldg/FlowTreatmentDevice"/>
        <rdfs:subClassOf>
            <owl:Restriction>
                <owl:onProperty rdf:resource="https://saref.etsi.org/saref4bldg/coverLength"/>
                <owl:allValuesFrom rdf:resource="https://saref.etsi.org/core/Measurement"/>
            </owl:Restriction>
        </rdfs:subClassOf>
        <rdfs:subClassOf>
            <owl:Restriction>
                <owl:onProperty rdf:resource="https://saref.etsi.org/saref4bldg/coverWidth"/>
                <owl:allValuesFrom rdf:resource="https://saref.etsi.org/core/Measurement"/>
            </owl:Restriction>
        </rdfs:subClassOf>
        <rdfs:subClassOf>
            <owl:Restriction>
                <owl:onProperty rdf:resource="https://saref.etsi.org/saref4bldg/inletConnectionSize"/>
                <owl:allValuesFrom rdf:resource="https://saref.etsi.org/core/Measurement"/>
            </owl:Restriction>
        </rdfs:subClassOf>
        <rdfs:subClassOf>
            <owl:Restriction>
                <owl:onProperty rdf:resource="https://saref.etsi.org/saref4bldg/nominalBodyDepth"/>
                <owl:allValuesFrom rdf:resource="https://saref.etsi.org/core/Measurement"/>
            </owl:Restriction>
        </rdfs:subClassOf>
        <rdfs:subClassOf>
            <owl:Restriction>
                <owl:onProperty rdf:resource="https://saref.etsi.org/saref4bldg/nominalBodyLength"/>
                <owl:allValuesFrom rdf:resource="https://saref.etsi.org/core/Measurement"/>
            </owl:Restriction>
        </rdfs:subClassOf>
        <rdfs:subClassOf>
            <owl:Restriction>
                <owl:onProperty rdf:resource="https://saref.etsi.org/saref4bldg/nominalBodyWidth"/>
                <owl:allValuesFrom rdf:resource="https://saref.etsi.org/core/Measurement"/>
            </owl:Restriction>
        </rdfs:subClassOf>
        <rdfs:subClassOf>
            <owl:Restriction>
                <owl:onProperty rdf:resource="https://saref.etsi.org/saref4bldg/outletConnectionSize"/>
                <owl:allValuesFrom rdf:resource="https://saref.etsi.org/core/Measurement"/>
            </owl:Restriction>
        </rdfs:subClassOf>
        <rdfs:subClassOf>
            <owl:Restriction>
                <owl:onProperty rdf:resource="https://saref.etsi.org/saref4bldg/ventilatingPipeSize"/>
                <owl:allValuesFrom rdf:resource="https://saref.etsi.org/core/Measurement"/>
            </owl:Restriction>
        </rdfs:subClassOf>
        <rdfs:comment xml:lang="en">An interceptor is a device designed and installed in order to separate and retain deleterious, hazardous or undesirable matter while permitting normal sewage or liquids to discharge into a collection system by gravity.</rdfs:comment>
        <rdfs:label xml:lang="en">Interceptor</rdfs:label>
        <rdfs:seeAlso>https://w3id.org/ifc/IFC4_ADD1#IfcInterceptor</rdfs:seeAlso>
        <prov:hadPrimarySource rdf:resource="http://www.buildingsmart-tech.org/ifc/IFC4/Add1/html/schema/ifcplumbingfireprotectiondomain/lexical/ifcinterceptor.htm"/>
        <prov:hadPrimarySource rdf:resource="http://www.buildingsmart-tech.org/ifc/IFC4/Add1/html/schema/ifcplumbingfireprotectiondomain/pset/pset_interceptortypecommon.htm"/>
    </owl:Class>
    


    <!-- https://saref.etsi.org/saref4bldg/Lamp -->


    <owl:Class rdf:about="https://saref.etsi.org/saref4bldg/Lamp">
        <rdfs:subClassOf rdf:resource="https://saref.etsi.org/saref4bldg/FlowTerminal"/>
        <rdfs:subClassOf>
            <owl:Restriction>
                <owl:onProperty rdf:resource="https://saref.etsi.org/saref4bldg/colorTemperature"/>
                <owl:allValuesFrom rdf:resource="https://saref.etsi.org/core/Measurement"/>
            </owl:Restriction>
        </rdfs:subClassOf>
        <rdfs:subClassOf>
            <owl:Restriction>
                <owl:onProperty rdf:resource="https://saref.etsi.org/saref4bldg/contributedLuminousFlux"/>
                <owl:allValuesFrom rdf:resource="https://saref.etsi.org/core/Measurement"/>
            </owl:Restriction>
        </rdfs:subClassOf>
        <rdfs:subClassOf>
            <owl:Restriction>
                <owl:onProperty rdf:resource="https://saref.etsi.org/saref4bldg/lampMaintenanceFactor"/>
                <owl:allValuesFrom rdf:resource="https://saref.etsi.org/core/Measurement"/>
            </owl:Restriction>
        </rdfs:subClassOf>
        <rdfs:subClassOf>
            <owl:Restriction>
                <owl:onProperty rdf:resource="https://saref.etsi.org/saref4bldg/lightEmitterNominalPower"/>
                <owl:allValuesFrom rdf:resource="https://saref.etsi.org/core/Measurement"/>
            </owl:Restriction>
        </rdfs:subClassOf>
        <rdfs:subClassOf>
            <owl:Restriction>
                <owl:onProperty rdf:resource="https://saref.etsi.org/saref4bldg/spectrumMax"/>
                <owl:allValuesFrom rdf:resource="https://saref.etsi.org/core/Measurement"/>
            </owl:Restriction>
        </rdfs:subClassOf>
        <rdfs:subClassOf>
            <owl:Restriction>
                <owl:onProperty rdf:resource="https://saref.etsi.org/saref4bldg/spectrumMin"/>
                <owl:allValuesFrom rdf:resource="https://saref.etsi.org/core/Measurement"/>
            </owl:Restriction>
        </rdfs:subClassOf>
        <rdfs:subClassOf>
            <owl:Restriction>
                <owl:onProperty rdf:resource="https://saref.etsi.org/saref4bldg/colorAppearance"/>
                <owl:allValuesFrom rdf:resource="http://www.w3.org/2001/XMLSchema#string"/>
            </owl:Restriction>
        </rdfs:subClassOf>
        <rdfs:subClassOf>
            <owl:Restriction>
                <owl:onProperty rdf:resource="https://saref.etsi.org/saref4bldg/colorRenderingIndex"/>
                <owl:allValuesFrom rdf:resource="http://www.w3.org/2001/XMLSchema#integer"/>
            </owl:Restriction>
        </rdfs:subClassOf>
        <rdfs:subClassOf>
            <owl:Restriction>
                <owl:onProperty rdf:resource="https://saref.etsi.org/saref4bldg/lampBallastType"/>
                <owl:allValuesFrom rdf:resource="http://www.w3.org/2001/XMLSchema#string"/>
            </owl:Restriction>
        </rdfs:subClassOf>
        <rdfs:subClassOf>
            <owl:Restriction>
                <owl:onProperty rdf:resource="https://saref.etsi.org/saref4bldg/lampCompensationType"/>
                <owl:allValuesFrom rdf:resource="http://www.w3.org/2001/XMLSchema#string"/>
            </owl:Restriction>
        </rdfs:subClassOf>
        <rdfs:comment xml:lang="en">A lamp is an artificial light source such as a light bulb or tube.</rdfs:comment>
        <rdfs:label xml:lang="en">Lamp</rdfs:label>
        <rdfs:seeAlso>https://w3id.org/ifc/IFC4_ADD1#IfcLamp</rdfs:seeAlso>
        <prov:hadPrimarySource rdf:resource="http://www.buildingsmart-tech.org/ifc/IFC4/Add1/html/schema/ifcelectricaldomain/lexical/ifclamp.htm"/>
        <prov:hadPrimarySource rdf:resource="http://www.buildingsmart-tech.org/ifc/IFC4/Add1/html/schema/ifcelectricaldomain/pset/pset_lamptypecommon.htm"/>
    </owl:Class>
    


    <!-- https://saref.etsi.org/saref4bldg/MedicalDevice -->


    <owl:Class rdf:about="https://saref.etsi.org/saref4bldg/MedicalDevice">
        <rdfs:subClassOf rdf:resource="https://saref.etsi.org/saref4bldg/FlowTerminal"/>
        <rdfs:comment xml:lang="en">A medical device is attached to a medical piping system and operates upon medical gases to perform a specific function. Medical gases include medical air, medical vacuum, oxygen, carbon dioxide, nitrogen, and nitrous oxide.</rdfs:comment>
        <rdfs:label xml:lang="en">Medical device</rdfs:label>
        <rdfs:seeAlso>https://w3id.org/ifc/IFC4_ADD1#IfcMedicalDevice</rdfs:seeAlso>
        <prov:hadPrimarySource rdf:resource="http://www.buildingsmart-tech.org/ifc/IFC4/Add1/html/schema/ifchvacdomain/lexical/ifcmedicaldevice.htm"/>
        <prov:hadPrimarySource rdf:resource="http://www.buildingsmart-tech.org/ifc/IFC4/Add1/html/schema/ifchvacdomain/pset/pset_medicaldevicetypecommon.htm"/>
    </owl:Class>
    


    <!-- https://saref.etsi.org/saref4bldg/Outlet -->


    <owl:Class rdf:about="https://saref.etsi.org/saref4bldg/Outlet">
        <rdfs:subClassOf rdf:resource="https://saref.etsi.org/saref4bldg/FlowTerminal"/>
        <rdfs:subClassOf>
            <owl:Restriction>
                <owl:onProperty rdf:resource="https://saref.etsi.org/saref4bldg/isPluggableOutlet"/>
                <owl:allValuesFrom rdf:resource="http://www.w3.org/2001/XMLSchema#boolean"/>
            </owl:Restriction>
        </rdfs:subClassOf>
        <rdfs:subClassOf>
            <owl:Restriction>
                <owl:onProperty rdf:resource="https://saref.etsi.org/saref4bldg/numberOsSockets"/>
                <owl:allValuesFrom rdf:resource="http://www.w3.org/2001/XMLSchema#integer"/>
            </owl:Restriction>
        </rdfs:subClassOf>
        <rdfs:comment xml:lang="en">An outlet is a device installed at a point to receive one or more inserted plugs for electrical power or communications.

Power outlets are commonly connected within a junction box; data outlets may be directly connected to a wall. For power outlets sharing the same circuit within a junction box, the ports should indicate the logical wiring relationship to the enclosing junction box, even though they may be physically connected to a cable going to another outlet, switch, or fixture.</rdfs:comment>
        <rdfs:label xml:lang="en">Outlet</rdfs:label>
        <rdfs:seeAlso>https://w3id.org/ifc/IFC4_ADD1#IfcOutlet</rdfs:seeAlso>
        <prov:hadPrimarySource rdf:resource="http://www.buildingsmart-tech.org/ifc/IFC4/Add1/html/schema/ifcelectricaldomain/lexical/ifcoutlet.htm"/>
        <prov:hadPrimarySource rdf:resource="http://www.buildingsmart-tech.org/ifc/IFC4/Add1/html/schema/ifcelectricaldomain/pset/pset_outlettypecommon.htm"/>
    </owl:Class>
    


    <!-- https://saref.etsi.org/saref4bldg/PhysicalObject -->


    <owl:Class rdf:about="https://saref.etsi.org/saref4bldg/PhysicalObject">
        <rdfs:subClassOf>
            <owl:Restriction>
                <owl:onProperty rdf:resource="https://saref.etsi.org/saref4bldg/contains"/>
                <owl:allValuesFrom rdf:resource="https://saref.etsi.org/saref4bldg/PhysicalObject"/>
            </owl:Restriction>
        </rdfs:subClassOf>
        <rdfs:subClassOf>
            <owl:Restriction>
                <owl:onProperty rdf:resource="https://saref.etsi.org/saref4bldg/isContainedIn"/>
                <owl:allValuesFrom>
                    <owl:Class>
                        <owl:unionOf rdf:parseType="Collection">
                            <rdf:Description rdf:about="https://saref.etsi.org/saref4bldg/BuildingSpace"/>
                            <rdf:Description rdf:about="https://saref.etsi.org/saref4bldg/PhysicalObject"/>
                        </owl:unionOf>
                    </owl:Class>
                </owl:allValuesFrom>
            </owl:Restriction>
        </rdfs:subClassOf>
        <rdfs:comment xml:lang="en">Any Object that has a proper space region.  (Definition extracted from DUL ontology)</rdfs:comment>
        <rdfs:label xml:lang="en">Physical object</rdfs:label>
    </owl:Class>
    


    <!-- https://saref.etsi.org/saref4bldg/ProtectiveDevice -->


    <owl:Class rdf:about="https://saref.etsi.org/saref4bldg/ProtectiveDevice">
        <rdfs:subClassOf rdf:resource="https://saref.etsi.org/saref4bldg/FlowController"/>
        <rdfs:comment xml:lang="en">A protective device breaks an electrical circuit when a stated electric current that passes through it is exceeded.

A protective device provides protection against electrical current only (not as a general protective device). It may be used to represent the complete set of elements including both the tripping unit and the breaking unit that provide the protection. This may be particularly useful at earlier stages of design where the approach to breaking the electrical supply may be determined but the method of tripping may not. Alternatively, this entity may be used to specifically represent the breaking unit alone (in which case the tripping unit will also be specifically identified). This entity is specific to dedicated protective devices and excludes electrical outlets that may have circuit protection.</rdfs:comment>
        <rdfs:label xml:lang="en">Protective device</rdfs:label>
        <rdfs:seeAlso>https://w3id.org/ifc/IFC4_ADD1#IfcProtectiveDevice</rdfs:seeAlso>
        <prov:hadPrimarySource rdf:resource="http://www.buildingsmart-tech.org/ifc/IFC4/Add1/html/schema/ifcelectricaldomain/lexical/ifcprotectivedevice.htm"/>
        <prov:hadPrimarySource rdf:resource="http://www.buildingsmart-tech.org/ifc/IFC4/Add1/html/schema/ifcelectricaldomain/pset/pset_protectivedevicetypecommon.htm"/>
    </owl:Class>
    


    <!-- https://saref.etsi.org/saref4bldg/ProtectiveDeviceTrippingUnit -->


    <owl:Class rdf:about="https://saref.etsi.org/saref4bldg/ProtectiveDeviceTrippingUnit">
        <rdfs:subClassOf rdf:resource="https://saref.etsi.org/saref4bldg/DistributionControlDevice"/>
        <rdfs:subClassOf>
            <owl:Restriction>
                <owl:onProperty rdf:resource="https://saref.etsi.org/saref4bldg/limitingTerminalSize"/>
                <owl:allValuesFrom rdf:resource="https://saref.etsi.org/core/Measurement"/>
            </owl:Restriction>
        </rdfs:subClassOf>
        <rdfs:subClassOf>
            <owl:Restriction>
                <owl:onProperty rdf:resource="https://saref.etsi.org/saref4bldg/standard"/>
                <owl:allValuesFrom rdf:resource="http://www.w3.org/2001/XMLSchema#string"/>
            </owl:Restriction>
        </rdfs:subClassOf>
        <rdfs:comment xml:lang="en">A protective device tripping unit breaks an electrical circuit at a separate breaking unit when a stated electric current that passes through the unit is exceeded.</rdfs:comment>
        <rdfs:label xml:lang="en">Protective device tripping unit</rdfs:label>
        <rdfs:seeAlso>https://w3id.org/ifc/IFC4_ADD1#IfcProtectiveDeviceTrippingUnit</rdfs:seeAlso>
        <prov:hadPrimarySource rdf:resource="http://www.buildingsmart-tech.org/ifc/IFC4/Add1/html/schema/ifcelectricaldomain/lexical/ifcprotectivedevicetrippingunit.htm"/>
        <prov:hadPrimarySource rdf:resource="http://www.buildingsmart-tech.org/ifc/IFC4/Add1/html/schema/ifcelectricaldomain/pset/pset_protectivedevicetrippingunittypecommon.htm"/>
    </owl:Class>
    


    <!-- https://saref.etsi.org/saref4bldg/Pump -->


    <owl:Class rdf:about="https://saref.etsi.org/saref4bldg/Pump">
        <rdfs:subClassOf rdf:resource="https://saref.etsi.org/saref4bldg/FlowMovingDevice"/>
        <rdfs:subClassOf>
            <owl:Restriction>
                <owl:onProperty rdf:resource="https://saref.etsi.org/saref4bldg/connectionSize"/>
                <owl:allValuesFrom rdf:resource="https://saref.etsi.org/core/Measurement"/>
            </owl:Restriction>
        </rdfs:subClassOf>
        <rdfs:subClassOf>
            <owl:Restriction>
                <owl:onProperty rdf:resource="https://saref.etsi.org/saref4bldg/flowResistanceMax"/>
                <owl:allValuesFrom rdf:resource="https://saref.etsi.org/core/Measurement"/>
            </owl:Restriction>
        </rdfs:subClassOf>
        <rdfs:subClassOf>
            <owl:Restriction>
                <owl:onProperty rdf:resource="https://saref.etsi.org/saref4bldg/flowResistanceMin"/>
                <owl:allValuesFrom rdf:resource="https://saref.etsi.org/core/Measurement"/>
            </owl:Restriction>
        </rdfs:subClassOf>
        <rdfs:subClassOf>
            <owl:Restriction>
                <owl:onProperty rdf:resource="https://saref.etsi.org/saref4bldg/netPositiveSuctionHead"/>
                <owl:allValuesFrom rdf:resource="https://saref.etsi.org/core/Measurement"/>
            </owl:Restriction>
        </rdfs:subClassOf>
        <rdfs:subClassOf>
            <owl:Restriction>
                <owl:onProperty rdf:resource="https://saref.etsi.org/saref4bldg/nomminalRotationSpeed"/>
                <owl:allValuesFrom rdf:resource="https://saref.etsi.org/core/Measurement"/>
            </owl:Restriction>
        </rdfs:subClassOf>
        <rdfs:subClassOf>
            <owl:Restriction>
                <owl:onProperty rdf:resource="https://saref.etsi.org/saref4bldg/operationTemperatureMax"/>
                <owl:allValuesFrom rdf:resource="https://saref.etsi.org/core/Measurement"/>
            </owl:Restriction>
        </rdfs:subClassOf>
        <rdfs:subClassOf>
            <owl:Restriction>
                <owl:onProperty rdf:resource="https://saref.etsi.org/saref4bldg/operationTemperatureMin"/>
                <owl:allValuesFrom rdf:resource="https://saref.etsi.org/core/Measurement"/>
            </owl:Restriction>
        </rdfs:subClassOf>
        <rdfs:subClassOf>
            <owl:Restriction>
                <owl:onProperty rdf:resource="https://saref.etsi.org/saref4bldg/pumpFlowRateMax"/>
                <owl:allValuesFrom rdf:resource="https://saref.etsi.org/core/Measurement"/>
            </owl:Restriction>
        </rdfs:subClassOf>
        <rdfs:subClassOf>
            <owl:Restriction>
                <owl:onProperty rdf:resource="https://saref.etsi.org/saref4bldg/pumpFlowRateMin"/>
                <owl:allValuesFrom rdf:resource="https://saref.etsi.org/core/Measurement"/>
            </owl:Restriction>
        </rdfs:subClassOf>
        <rdfs:comment xml:lang="en">A pump is a device which imparts mechanical work on fluids or slurries to move them through a channel or pipeline. A typical use of a pump is to circulate chilled water or heating hot water in a building services distribution system.</rdfs:comment>
        <rdfs:label xml:lang="en">Pump</rdfs:label>
        <rdfs:seeAlso>https://w3id.org/ifc/IFC4_ADD1#IfcPump</rdfs:seeAlso>
        <prov:hadPrimarySource rdf:resource="http://www.buildingsmart-tech.org/ifc/IFC4/Add1/html/schema/ifchvacdomain/lexical/ifcpump.htm"/>
        <prov:hadPrimarySource rdf:resource="http://www.buildingsmart-tech.org/ifc/IFC4/Add1/html/schema/ifchvacdomain/pset/pset_pumptypecommon.htm"/>
    </owl:Class>
    


    <!-- https://saref.etsi.org/saref4bldg/SanitaryTerminal -->


    <owl:Class rdf:about="https://saref.etsi.org/saref4bldg/SanitaryTerminal">
        <rdfs:subClassOf rdf:resource="https://saref.etsi.org/saref4bldg/FlowTerminal"/>
        <rdfs:comment xml:lang="en">A sanitary terminal is a fixed appliance or terminal usually supplied with water and used for drinking, cleaning or foul water disposal or that is an item of equipment directly used with such an appliance or terminal.</rdfs:comment>
        <rdfs:label xml:lang="en">Sanitary terminal</rdfs:label>
        <rdfs:seeAlso>https://w3id.org/ifc/IFC4_ADD1#IfcSanitaryTerminal</rdfs:seeAlso>
        <prov:hadPrimarySource rdf:resource="http://www.buildingsmart-tech.org/ifc/IFC4/Add1/html/schema/ifcplumbingfireprotectiondomain/lexical/ifcsanitaryterminal.htm"/>
        <prov:hadPrimarySource rdf:resource="http://www.buildingsmart-tech.org/ifc/IFC4/Add1/html/schema/ifcplumbingfireprotectiondomain/pset/pset_sanitaryterminaltypecommon.htm"/>
    </owl:Class>
    


    <!-- https://saref.etsi.org/saref4bldg/Sensor -->


    <owl:Class rdf:about="https://saref.etsi.org/saref4bldg/Sensor">
        <rdfs:subClassOf rdf:resource="https://saref.etsi.org/core/Sensor"/>
        <rdfs:subClassOf rdf:resource="https://saref.etsi.org/saref4bldg/DistributionControlDevice"/>
        <rdfs:comment xml:lang="en">A sensor is a device that measures a physical quantity and converts it into a signal which can be read by an observer or by an instrument.</rdfs:comment>
        <rdfs:label xml:lang="en">Sensor</rdfs:label>
        <rdfs:seeAlso>https://w3id.org/ifc/IFC4_ADD1#IfcSensor</rdfs:seeAlso>
        <prov:hadPrimarySource rdf:resource="http://www.buildingsmart-tech.org/ifc/IFC4/Add1/html/schema/ifcbuildingcontrolsdomain/lexical/ifcsensor.htm"/>
        <prov:hadPrimarySource rdf:resource="http://www.buildingsmart-tech.org/ifc/IFC4/Add1/html/schema/ifcbuildingcontrolsdomain/pset/pset_sensortypecommon.htm"/>
    </owl:Class>
    


    <!-- https://saref.etsi.org/saref4bldg/ShadingDevice -->


    <owl:Class rdf:about="https://saref.etsi.org/saref4bldg/ShadingDevice">
        <rdfs:subClassOf rdf:resource="https://saref.etsi.org/saref4bldg/BuildingDevice"/>
        <rdfs:subClassOf>
            <owl:Restriction>
                <owl:onProperty rdf:resource="https://saref.etsi.org/saref4bldg/solarReflectance"/>
                <owl:allValuesFrom rdf:resource="https://saref.etsi.org/core/Measurement"/>
            </owl:Restriction>
        </rdfs:subClassOf>
        <rdfs:subClassOf>
            <owl:Restriction>
                <owl:onProperty rdf:resource="https://saref.etsi.org/saref4bldg/solarTransmittance"/>
                <owl:allValuesFrom rdf:resource="https://saref.etsi.org/core/Measurement"/>
            </owl:Restriction>
        </rdfs:subClassOf>
        <rdfs:subClassOf>
            <owl:Restriction>
                <owl:onProperty rdf:resource="https://saref.etsi.org/saref4bldg/thermalTransmittance"/>
                <owl:allValuesFrom rdf:resource="https://saref.etsi.org/core/Measurement"/>
            </owl:Restriction>
        </rdfs:subClassOf>
        <rdfs:subClassOf>
            <owl:Restriction>
                <owl:onProperty rdf:resource="https://saref.etsi.org/saref4bldg/visibleLightReflectance"/>
                <owl:allValuesFrom rdf:resource="https://saref.etsi.org/core/Measurement"/>
            </owl:Restriction>
        </rdfs:subClassOf>
        <rdfs:subClassOf>
            <owl:Restriction>
                <owl:onProperty rdf:resource="https://saref.etsi.org/saref4bldg/visibleLightTransmittance"/>
                <owl:allValuesFrom rdf:resource="https://saref.etsi.org/core/Measurement"/>
            </owl:Restriction>
        </rdfs:subClassOf>
        <rdfs:subClassOf>
            <owl:Restriction>
                <owl:onProperty rdf:resource="https://saref.etsi.org/saref4bldg/isExternal"/>
                <owl:allValuesFrom rdf:resource="http://www.w3.org/2001/XMLSchema#boolean"/>
            </owl:Restriction>
        </rdfs:subClassOf>
        <rdfs:subClassOf>
            <owl:Restriction>
                <owl:onProperty rdf:resource="https://saref.etsi.org/saref4bldg/mechanicalOperated"/>
                <owl:allValuesFrom rdf:resource="http://www.w3.org/2001/XMLSchema#boolean"/>
            </owl:Restriction>
        </rdfs:subClassOf>
        <rdfs:subClassOf>
            <owl:Restriction>
                <owl:onProperty rdf:resource="https://saref.etsi.org/saref4bldg/roughness"/>
                <owl:allValuesFrom rdf:resource="http://www.w3.org/2001/XMLSchema#string"/>
            </owl:Restriction>
        </rdfs:subClassOf>
        <rdfs:subClassOf>
            <owl:Restriction>
                <owl:onProperty rdf:resource="https://saref.etsi.org/saref4bldg/shadingDeviceType"/>
                <owl:allValuesFrom rdf:resource="http://www.w3.org/2001/XMLSchema#string"/>
            </owl:Restriction>
        </rdfs:subClassOf>
        <rdfs:comment xml:lang="en">Shading devices are purpose built devices to protect from the sunlight, from natural light, or screening them from view. Shading devices can form part of the facade or can be mounted inside the building, they can be fixed or operable.</rdfs:comment>
        <rdfs:label xml:lang="en">Shading device</rdfs:label>
        <rdfs:seeAlso>https://w3id.org/ifc/IFC4_ADD1#IfcShadingDevice</rdfs:seeAlso>
        <prov:hadPrimarySource rdf:resource="http://www.buildingsmart-tech.org/ifc/IFC4/Add1/html/schema/ifcsharedbldgelements/lexical/ifcshadingdevice.htm"/>
        <prov:hadPrimarySource rdf:resource="http://www.buildingsmart-tech.org/ifc/IFC4/Add1/html/schema/ifcsharedbldgelements/pset/pset_shadingdevicecommon.htm"/>
    </owl:Class>
    


    <!-- https://saref.etsi.org/saref4bldg/SolarDevice -->


    <owl:Class rdf:about="https://saref.etsi.org/saref4bldg/SolarDevice">
        <rdfs:subClassOf rdf:resource="https://saref.etsi.org/saref4bldg/EnergyConversionDevice"/>
        <rdfs:comment xml:lang="en">A solar device converts solar radiation into other energy such as electric current or thermal energy.</rdfs:comment>
        <rdfs:label xml:lang="en">Solar device</rdfs:label>
        <rdfs:seeAlso>https://w3id.org/ifc/IFC4_ADD1#IfcSolarDevice</rdfs:seeAlso>
        <prov:hadPrimarySource rdf:resource="http://www.buildingsmart-tech.org/ifc/IFC4/Add1/html/schema/ifcelectricaldomain/lexical/ifcsolardevicetypeenum.htm"/>
        <prov:hadPrimarySource rdf:resource="http://www.buildingsmart-tech.org/ifc/IFC4/Add1/html/schema/ifcelectricaldomain/pset/pset_solardevicetypecommon.htm"/>
    </owl:Class>
    


    <!-- https://saref.etsi.org/saref4bldg/SpaceHeater -->


    <owl:Class rdf:about="https://saref.etsi.org/saref4bldg/SpaceHeater">
        <rdfs:subClassOf rdf:resource="https://saref.etsi.org/saref4bldg/FlowTerminal"/>
        <rdfs:subClassOf>
            <owl:Restriction>
                <owl:onProperty rdf:resource="https://saref.etsi.org/saref4bldg/bodyMass"/>
                <owl:allValuesFrom rdf:resource="https://saref.etsi.org/core/Measurement"/>
            </owl:Restriction>
        </rdfs:subClassOf>
        <rdfs:subClassOf>
            <owl:Restriction>
                <owl:onProperty rdf:resource="https://saref.etsi.org/saref4bldg/outputCapacity"/>
                <owl:allValuesFrom rdf:resource="https://saref.etsi.org/core/Measurement"/>
            </owl:Restriction>
        </rdfs:subClassOf>
        <rdfs:subClassOf>
            <owl:Restriction>
                <owl:onProperty rdf:resource="https://saref.etsi.org/saref4bldg/thermalEfficiency"/>
                <owl:allValuesFrom rdf:resource="https://saref.etsi.org/core/Measurement"/>
            </owl:Restriction>
        </rdfs:subClassOf>
        <rdfs:subClassOf>
            <owl:Restriction>
                <owl:onProperty rdf:resource="https://saref.etsi.org/saref4bldg/thermalMassHeatCapacity"/>
                <owl:allValuesFrom rdf:resource="https://saref.etsi.org/core/Measurement"/>
            </owl:Restriction>
        </rdfs:subClassOf>
        <rdfs:subClassOf>
            <owl:Restriction>
                <owl:onProperty rdf:resource="https://saref.etsi.org/saref4bldg/energySource"/>
                <owl:allValuesFrom rdf:resource="http://www.w3.org/2001/XMLSchema#string"/>
            </owl:Restriction>
        </rdfs:subClassOf>
        <rdfs:subClassOf>
            <owl:Restriction>
                <owl:onProperty rdf:resource="https://saref.etsi.org/saref4bldg/heatTransferDimension"/>
                <owl:allValuesFrom rdf:resource="http://www.w3.org/2001/XMLSchema#string"/>
            </owl:Restriction>
        </rdfs:subClassOf>
        <rdfs:subClassOf>
            <owl:Restriction>
                <owl:onProperty rdf:resource="https://saref.etsi.org/saref4bldg/heatTransferMedium"/>
                <owl:allValuesFrom rdf:resource="http://www.w3.org/2001/XMLSchema#string"/>
            </owl:Restriction>
        </rdfs:subClassOf>
        <rdfs:subClassOf>
            <owl:Restriction>
                <owl:onProperty rdf:resource="https://saref.etsi.org/saref4bldg/numberOfPanels"/>
                <owl:allValuesFrom rdf:resource="http://www.w3.org/2001/XMLSchema#integer"/>
            </owl:Restriction>
        </rdfs:subClassOf>
        <rdfs:subClassOf>
            <owl:Restriction>
                <owl:onProperty rdf:resource="https://saref.etsi.org/saref4bldg/numberOfSections"/>
                <owl:allValuesFrom rdf:resource="http://www.w3.org/2001/XMLSchema#integer"/>
            </owl:Restriction>
        </rdfs:subClassOf>
        <rdfs:subClassOf>
            <owl:Restriction>
                <owl:onProperty rdf:resource="https://saref.etsi.org/saref4bldg/placementType"/>
                <owl:allValuesFrom rdf:resource="http://www.w3.org/2001/XMLSchema#string"/>
            </owl:Restriction>
        </rdfs:subClassOf>
        <rdfs:subClassOf>
            <owl:Restriction>
                <owl:onProperty rdf:resource="https://saref.etsi.org/saref4bldg/temperatureClassification"/>
                <owl:allValuesFrom rdf:resource="http://www.w3.org/2001/XMLSchema#string"/>
            </owl:Restriction>
        </rdfs:subClassOf>
        <rdfs:comment xml:lang="en">Space heaters utilize a combination of radiation and/or natural convection using a heating source such as electricity, steam or hot water to heat a limited space or area. Examples of space heaters include radiators, convectors, baseboard and finned-tube heaters.

UnitaryEquipment should be used for packaged units supporting a combination of heating, cooling, and/or dehumidification; Coil should be used for coil-based floor heating.</rdfs:comment>
        <rdfs:label xml:lang="en">Space heater</rdfs:label>
        <rdfs:seeAlso>https://w3id.org/ifc/IFC4_ADD1#IfcSpaceHeater</rdfs:seeAlso>
        <prov:hadPrimarySource rdf:resource="http://www.buildingsmart-tech.org/ifc/IFC4/Add1/html/schema/ifchvacdomain/lexical/ifcspaceheater.htm"/>
        <prov:hadPrimarySource rdf:resource="http://www.buildingsmart-tech.org/ifc/IFC4/Add1/html/schema/ifchvacdomain/pset/pset_spaceheatertypecommon.htm"/>
    </owl:Class>
    


    <!-- https://saref.etsi.org/saref4bldg/SwitchingDevice -->


    <owl:Class rdf:about="https://saref.etsi.org/saref4bldg/SwitchingDevice">
        <rdfs:subClassOf rdf:resource="https://saref.etsi.org/saref4bldg/FlowController"/>
        <rdfs:subClassOf>
            <owl:Restriction>
                <owl:onProperty rdf:resource="https://saref.etsi.org/saref4bldg/hasLock"/>
                <owl:allValuesFrom rdf:resource="http://www.w3.org/2001/XMLSchema#boolean"/>
            </owl:Restriction>
        </rdfs:subClassOf>
        <rdfs:subClassOf>
            <owl:Restriction>
                <owl:onProperty rdf:resource="https://saref.etsi.org/saref4bldg/isIlluminated"/>
                <owl:allValuesFrom rdf:resource="http://www.w3.org/2001/XMLSchema#boolean"/>
            </owl:Restriction>
        </rdfs:subClassOf>
        <rdfs:subClassOf>
            <owl:Restriction>
                <owl:onProperty rdf:resource="https://saref.etsi.org/saref4bldg/legend"/>
                <owl:allValuesFrom rdf:resource="http://www.w3.org/2001/XMLSchema#string"/>
            </owl:Restriction>
        </rdfs:subClassOf>
        <rdfs:subClassOf>
            <owl:Restriction>
                <owl:onProperty rdf:resource="https://saref.etsi.org/saref4bldg/numberOfGangs"/>
                <owl:allValuesFrom rdf:resource="http://www.w3.org/2001/XMLSchema#integer"/>
            </owl:Restriction>
        </rdfs:subClassOf>
        <rdfs:subClassOf>
            <owl:Restriction>
                <owl:onProperty rdf:resource="https://saref.etsi.org/saref4bldg/switchFunction"/>
                <owl:allValuesFrom rdf:resource="http://www.w3.org/2001/XMLSchema#string"/>
            </owl:Restriction>
        </rdfs:subClassOf>
        <rdfs:comment xml:lang="en">A switch is used in a cable distribution system (electrical circuit) to control or modulate the flow of electricity.

Switches include those used for electrical power, communications, audio-visual, or other distribution system types as determined by the available ports.</rdfs:comment>
        <rdfs:label xml:lang="en">Switching device</rdfs:label>
        <rdfs:seeAlso>https://w3id.org/ifc/IFC4_ADD1#IfcSwitchingDevice</rdfs:seeAlso>
        <prov:hadPrimarySource rdf:resource="http://www.buildingsmart-tech.org/ifc/IFC4/Add1/html/schema/ifcelectricaldomain/lexical/ifcswitchingdevice.htm"/>
        <prov:hadPrimarySource rdf:resource="http://www.buildingsmart-tech.org/ifc/IFC4/Add1/html/schema/ifcelectricaldomain/pset/pset_switchingdevicetypecommon.htm"/>
    </owl:Class>
    


    <!-- https://saref.etsi.org/saref4bldg/Tank -->


    <owl:Class rdf:about="https://saref.etsi.org/saref4bldg/Tank">
        <rdfs:subClassOf rdf:resource="https://saref.etsi.org/saref4bldg/FlowStorageDevice"/>
        <rdfs:subClassOf>
            <owl:Restriction>
                <owl:onProperty rdf:resource="https://saref.etsi.org/saref4bldg/effectiveCapacity"/>
                <owl:allValuesFrom rdf:resource="https://saref.etsi.org/core/Measurement"/>
            </owl:Restriction>
        </rdfs:subClassOf>
        <rdfs:subClassOf>
            <owl:Restriction>
                <owl:onProperty rdf:resource="https://saref.etsi.org/saref4bldg/firstCurvatureRadius"/>
                <owl:allValuesFrom rdf:resource="https://saref.etsi.org/core/Measurement"/>
            </owl:Restriction>
        </rdfs:subClassOf>
        <rdfs:subClassOf>
            <owl:Restriction>
                <owl:onProperty rdf:resource="https://saref.etsi.org/saref4bldg/nominalDepth"/>
                <owl:allValuesFrom rdf:resource="https://saref.etsi.org/core/Measurement"/>
            </owl:Restriction>
        </rdfs:subClassOf>
        <rdfs:subClassOf>
            <owl:Restriction>
                <owl:onProperty rdf:resource="https://saref.etsi.org/saref4bldg/nominalLengthOrDiameter"/>
                <owl:allValuesFrom rdf:resource="https://saref.etsi.org/core/Measurement"/>
            </owl:Restriction>
        </rdfs:subClassOf>
        <rdfs:subClassOf>
            <owl:Restriction>
                <owl:onProperty rdf:resource="https://saref.etsi.org/saref4bldg/nominalVolumetricCapacity"/>
                <owl:allValuesFrom rdf:resource="https://saref.etsi.org/core/Measurement"/>
            </owl:Restriction>
        </rdfs:subClassOf>
        <rdfs:subClassOf>
            <owl:Restriction>
                <owl:onProperty rdf:resource="https://saref.etsi.org/saref4bldg/nominalWidthOrDiameter"/>
                <owl:allValuesFrom rdf:resource="https://saref.etsi.org/core/Measurement"/>
            </owl:Restriction>
        </rdfs:subClassOf>
        <rdfs:subClassOf>
            <owl:Restriction>
                <owl:onProperty rdf:resource="https://saref.etsi.org/saref4bldg/operatingWeight"/>
                <owl:allValuesFrom rdf:resource="https://saref.etsi.org/core/Measurement"/>
            </owl:Restriction>
        </rdfs:subClassOf>
        <rdfs:subClassOf>
            <owl:Restriction>
                <owl:onProperty rdf:resource="https://saref.etsi.org/saref4bldg/secondCurvatureRadius"/>
                <owl:allValuesFrom rdf:resource="https://saref.etsi.org/core/Measurement"/>
            </owl:Restriction>
        </rdfs:subClassOf>
        <rdfs:subClassOf>
            <owl:Restriction>
                <owl:onProperty rdf:resource="https://saref.etsi.org/saref4bldg/accessType"/>
                <owl:allValuesFrom rdf:resource="http://www.w3.org/2001/XMLSchema#string"/>
            </owl:Restriction>
        </rdfs:subClassOf>
        <rdfs:subClassOf>
            <owl:Restriction>
                <owl:onProperty rdf:resource="https://saref.etsi.org/saref4bldg/endShapeType"/>
                <owl:allValuesFrom rdf:resource="http://www.w3.org/2001/XMLSchema#string"/>
            </owl:Restriction>
        </rdfs:subClassOf>
        <rdfs:subClassOf>
            <owl:Restriction>
                <owl:onProperty rdf:resource="https://saref.etsi.org/saref4bldg/numberOfSections"/>
                <owl:allValuesFrom rdf:resource="http://www.w3.org/2001/XMLSchema#integer"/>
            </owl:Restriction>
        </rdfs:subClassOf>
        <rdfs:subClassOf>
            <owl:Restriction>
                <owl:onProperty rdf:resource="https://saref.etsi.org/saref4bldg/patternType"/>
                <owl:allValuesFrom rdf:resource="http://www.w3.org/2001/XMLSchema#string"/>
            </owl:Restriction>
        </rdfs:subClassOf>
        <rdfs:subClassOf>
            <owl:Restriction>
                <owl:onProperty rdf:resource="https://saref.etsi.org/saref4bldg/storageType"/>
                <owl:allValuesFrom rdf:resource="http://www.w3.org/2001/XMLSchema#string"/>
            </owl:Restriction>
        </rdfs:subClassOf>
        <rdfs:comment xml:lang="en">A tank is a vessel or container in which a fluid or gas is stored for later use.</rdfs:comment>
        <rdfs:label xml:lang="en">Tank</rdfs:label>
        <rdfs:seeAlso>https://w3id.org/ifc/IFC4_ADD1#IfcTank</rdfs:seeAlso>
        <prov:hadPrimarySource rdf:resource="http://www.buildingsmart-tech.org/ifc/IFC4/Add1/html/schema/ifchvacdomain/lexical/ifctank.htm"/>
        <prov:hadPrimarySource rdf:resource="http://www.buildingsmart-tech.org/ifc/IFC4/Add1/html/schema/ifchvacdomain/pset/pset_tanktypecommon.htm"/>
    </owl:Class>
    


    <!-- https://saref.etsi.org/saref4bldg/Transformer -->


    <owl:Class rdf:about="https://saref.etsi.org/saref4bldg/Transformer">
        <rdfs:subClassOf rdf:resource="https://saref.etsi.org/saref4bldg/EnergyConversionDevice"/>
        <rdfs:subClassOf>
            <owl:Restriction>
                <owl:onProperty rdf:resource="https://saref.etsi.org/saref4bldg/apparentPowerMax"/>
                <owl:allValuesFrom rdf:resource="https://saref.etsi.org/core/Measurement"/>
            </owl:Restriction>
        </rdfs:subClassOf>
        <rdfs:subClassOf>
            <owl:Restriction>
                <owl:onProperty rdf:resource="https://saref.etsi.org/saref4bldg/imaginaryImpedanceRatio"/>
                <owl:allValuesFrom rdf:resource="https://saref.etsi.org/core/Measurement"/>
            </owl:Restriction>
        </rdfs:subClassOf>
        <rdfs:subClassOf>
            <owl:Restriction>
                <owl:onProperty rdf:resource="https://saref.etsi.org/saref4bldg/primaryApparentPower"/>
                <owl:allValuesFrom rdf:resource="https://saref.etsi.org/core/Measurement"/>
            </owl:Restriction>
        </rdfs:subClassOf>
        <rdfs:subClassOf>
            <owl:Restriction>
                <owl:onProperty rdf:resource="https://saref.etsi.org/saref4bldg/primaryCurrent"/>
                <owl:allValuesFrom rdf:resource="https://saref.etsi.org/core/Measurement"/>
            </owl:Restriction>
        </rdfs:subClassOf>
        <rdfs:subClassOf>
            <owl:Restriction>
                <owl:onProperty rdf:resource="https://saref.etsi.org/saref4bldg/primaryFrequency"/>
                <owl:allValuesFrom rdf:resource="https://saref.etsi.org/core/Measurement"/>
            </owl:Restriction>
        </rdfs:subClassOf>
        <rdfs:subClassOf>
            <owl:Restriction>
                <owl:onProperty rdf:resource="https://saref.etsi.org/saref4bldg/primaryVoltage"/>
                <owl:allValuesFrom rdf:resource="https://saref.etsi.org/core/Measurement"/>
            </owl:Restriction>
        </rdfs:subClassOf>
        <rdfs:subClassOf>
            <owl:Restriction>
                <owl:onProperty rdf:resource="https://saref.etsi.org/saref4bldg/realImpedanceRatio"/>
                <owl:allValuesFrom rdf:resource="https://saref.etsi.org/core/Measurement"/>
            </owl:Restriction>
        </rdfs:subClassOf>
        <rdfs:subClassOf>
            <owl:Restriction>
                <owl:onProperty rdf:resource="https://saref.etsi.org/saref4bldg/secondaryApparentPower"/>
                <owl:allValuesFrom rdf:resource="https://saref.etsi.org/core/Measurement"/>
            </owl:Restriction>
        </rdfs:subClassOf>
        <rdfs:subClassOf>
            <owl:Restriction>
                <owl:onProperty rdf:resource="https://saref.etsi.org/saref4bldg/secondaryCurrent"/>
                <owl:allValuesFrom rdf:resource="https://saref.etsi.org/core/Measurement"/>
            </owl:Restriction>
        </rdfs:subClassOf>
        <rdfs:subClassOf>
            <owl:Restriction>
                <owl:onProperty rdf:resource="https://saref.etsi.org/saref4bldg/secondaryFrequency"/>
                <owl:allValuesFrom rdf:resource="https://saref.etsi.org/core/Measurement"/>
            </owl:Restriction>
        </rdfs:subClassOf>
        <rdfs:subClassOf>
            <owl:Restriction>
                <owl:onProperty rdf:resource="https://saref.etsi.org/saref4bldg/secondaryVoltage"/>
                <owl:allValuesFrom rdf:resource="https://saref.etsi.org/core/Measurement"/>
            </owl:Restriction>
        </rdfs:subClassOf>
        <rdfs:subClassOf>
            <owl:Restriction>
                <owl:onProperty rdf:resource="https://saref.etsi.org/saref4bldg/isNeutralPrimaryTerminalAvailable"/>
                <owl:allValuesFrom rdf:resource="http://www.w3.org/2001/XMLSchema#boolean"/>
            </owl:Restriction>
        </rdfs:subClassOf>
        <rdfs:subClassOf>
            <owl:Restriction>
                <owl:onProperty rdf:resource="https://saref.etsi.org/saref4bldg/isNeutralSecondaryTerminalAvailable"/>
                <owl:allValuesFrom rdf:resource="http://www.w3.org/2001/XMLSchema#boolean"/>
            </owl:Restriction>
        </rdfs:subClassOf>
        <rdfs:subClassOf>
            <owl:Restriction>
                <owl:onProperty rdf:resource="https://saref.etsi.org/saref4bldg/secondaryCurrentType"/>
                <owl:allValuesFrom rdf:resource="http://www.w3.org/2001/XMLSchema#string"/>
            </owl:Restriction>
        </rdfs:subClassOf>
        <rdfs:subClassOf>
            <owl:Restriction>
                <owl:onProperty rdf:resource="https://saref.etsi.org/saref4bldg/transformerVectorGroup"/>
                <owl:allValuesFrom rdf:resource="http://www.w3.org/2001/XMLSchema#string"/>
            </owl:Restriction>
        </rdfs:subClassOf>
        <rdfs:comment xml:lang="en">A transformer is an inductive stationary device that transfers electrical energy from one circuit to another.

Transformer is used to transform electric power; conversion of electric signals for other purposes is handled at other entities: Controller converts arbitrary signals, AudioVisualAppliance converts signals for audio or video streams, and CommunicationsAppliance converts signals for data or other communications usage.</rdfs:comment>
        <rdfs:label xml:lang="en">Transformer</rdfs:label>
        <rdfs:seeAlso>https://w3id.org/ifc/IFC4_ADD1#IfcTransformer</rdfs:seeAlso>
        <prov:hadPrimarySource rdf:resource="http://www.buildingsmart-tech.org/ifc/IFC4/Add1/html/schema/ifcelectricaldomain/lexical/ifctransformer.htm"/>
        <prov:hadPrimarySource rdf:resource="http://www.buildingsmart-tech.org/ifc/IFC4/Add1/html/schema/ifcelectricaldomain/pset/pset_transformertypecommon.htm"/>
    </owl:Class>
    


    <!-- https://saref.etsi.org/saref4bldg/TransportElement -->


    <owl:Class rdf:about="https://saref.etsi.org/saref4bldg/TransportElement">
        <rdfs:subClassOf rdf:resource="https://saref.etsi.org/core/Device"/>
        <rdfs:subClassOf>
            <owl:Restriction>
                <owl:onProperty rdf:resource="https://saref.etsi.org/saref4bldg/capacityWeight"/>
                <owl:allValuesFrom rdf:resource="https://saref.etsi.org/core/Measurement"/>
            </owl:Restriction>
        </rdfs:subClassOf>
        <rdfs:subClassOf>
            <owl:Restriction>
                <owl:onProperty rdf:resource="https://saref.etsi.org/saref4bldg/capacityPeople"/>
                <owl:allValuesFrom rdf:resource="http://www.w3.org/2001/XMLSchema#positiveInteger"/>
            </owl:Restriction>
        </rdfs:subClassOf>
        <rdfs:subClassOf>
            <owl:Restriction>
                <owl:onProperty rdf:resource="https://saref.etsi.org/saref4bldg/fireExit"/>
                <owl:allValuesFrom rdf:resource="http://www.w3.org/2001/XMLSchema#boolean"/>
            </owl:Restriction>
        </rdfs:subClassOf>
        <rdfs:comment xml:lang="en">A transport element is a generalization of all transport related objects that move people, animals or goods within a building or building complex. The TransportElement defines the occurrence of a transport element. </rdfs:comment>
        <rdfs:label xml:lang="en">Transport element</rdfs:label>
        <rdfs:seeAlso>https://w3id.org/ifc/IFC4_ADD1#IfcTransportElement</rdfs:seeAlso>
        <prov:hadPrimarySource rdf:resource="http://www.buildingsmart-tech.org/ifc/IFC4/Add1/html/schema/ifcproductextension/lexical/ifctransportelement.htm"/>
        <prov:hadPrimarySource rdf:resource="http://www.buildingsmart-tech.org/ifc/IFC4/Add1/html/schema/ifcproductextension/pset/pset_transportelementcommon.htm"/>
    </owl:Class>
    


    <!-- https://saref.etsi.org/saref4bldg/TubeBundle -->


    <owl:Class rdf:about="https://saref.etsi.org/saref4bldg/TubeBundle">
        <rdfs:subClassOf rdf:resource="https://saref.etsi.org/saref4bldg/EnergyConversionDevice"/>
        <rdfs:subClassOf>
            <owl:Restriction>
                <owl:onProperty rdf:resource="https://saref.etsi.org/saref4bldg/foulingFactor"/>
                <owl:allValuesFrom rdf:resource="https://saref.etsi.org/core/Measurement"/>
            </owl:Restriction>
        </rdfs:subClassOf>
        <rdfs:subClassOf>
            <owl:Restriction>
                <owl:onProperty rdf:resource="https://saref.etsi.org/saref4bldg/horizontalSpacing"/>
                <owl:allValuesFrom rdf:resource="https://saref.etsi.org/core/Measurement"/>
            </owl:Restriction>
        </rdfs:subClassOf>
        <rdfs:subClassOf>
            <owl:Restriction>
                <owl:onProperty rdf:resource="https://saref.etsi.org/saref4bldg/inLineRowSpacing"/>
                <owl:allValuesFrom rdf:resource="https://saref.etsi.org/core/Measurement"/>
            </owl:Restriction>
        </rdfs:subClassOf>
        <rdfs:subClassOf>
            <owl:Restriction>
                <owl:onProperty rdf:resource="https://saref.etsi.org/saref4bldg/insideDiameter"/>
                <owl:allValuesFrom rdf:resource="https://saref.etsi.org/core/Measurement"/>
            </owl:Restriction>
        </rdfs:subClassOf>
        <rdfs:subClassOf>
            <owl:Restriction>
                <owl:onProperty rdf:resource="https://saref.etsi.org/saref4bldg/length"/>
                <owl:allValuesFrom rdf:resource="https://saref.etsi.org/core/Measurement"/>
            </owl:Restriction>
        </rdfs:subClassOf>
        <rdfs:subClassOf>
            <owl:Restriction>
                <owl:onProperty rdf:resource="https://saref.etsi.org/saref4bldg/nominalDiameter"/>
                <owl:allValuesFrom rdf:resource="https://saref.etsi.org/core/Measurement"/>
            </owl:Restriction>
        </rdfs:subClassOf>
        <rdfs:subClassOf>
            <owl:Restriction>
                <owl:onProperty rdf:resource="https://saref.etsi.org/saref4bldg/outsideDiameter"/>
                <owl:allValuesFrom rdf:resource="https://saref.etsi.org/core/Measurement"/>
            </owl:Restriction>
        </rdfs:subClassOf>
        <rdfs:subClassOf>
            <owl:Restriction>
                <owl:onProperty rdf:resource="https://saref.etsi.org/saref4bldg/staggeredRowSpacing"/>
                <owl:allValuesFrom rdf:resource="https://saref.etsi.org/core/Measurement"/>
            </owl:Restriction>
        </rdfs:subClassOf>
        <rdfs:subClassOf>
            <owl:Restriction>
                <owl:onProperty rdf:resource="https://saref.etsi.org/saref4bldg/thermalConductivity"/>
                <owl:allValuesFrom rdf:resource="https://saref.etsi.org/core/Measurement"/>
            </owl:Restriction>
        </rdfs:subClassOf>
        <rdfs:subClassOf>
            <owl:Restriction>
                <owl:onProperty rdf:resource="https://saref.etsi.org/saref4bldg/verticalSpacing"/>
                <owl:allValuesFrom rdf:resource="https://saref.etsi.org/core/Measurement"/>
            </owl:Restriction>
        </rdfs:subClassOf>
        <rdfs:subClassOf>
            <owl:Restriction>
                <owl:onProperty rdf:resource="https://saref.etsi.org/saref4bldg/volumen"/>
                <owl:allValuesFrom rdf:resource="https://saref.etsi.org/core/Measurement"/>
            </owl:Restriction>
        </rdfs:subClassOf>
        <rdfs:subClassOf>
            <owl:Restriction>
                <owl:onProperty rdf:resource="https://saref.etsi.org/saref4bldg/hasTurbulator"/>
                <owl:allValuesFrom rdf:resource="http://www.w3.org/2001/XMLSchema#boolean"/>
            </owl:Restriction>
        </rdfs:subClassOf>
        <rdfs:subClassOf>
            <owl:Restriction>
                <owl:onProperty rdf:resource="https://saref.etsi.org/saref4bldg/numberOfCircuits"/>
                <owl:allValuesFrom rdf:resource="http://www.w3.org/2001/XMLSchema#integer"/>
            </owl:Restriction>
        </rdfs:subClassOf>
        <rdfs:subClassOf>
            <owl:Restriction>
                <owl:onProperty rdf:resource="https://saref.etsi.org/saref4bldg/numberOfRows"/>
                <owl:allValuesFrom rdf:resource="http://www.w3.org/2001/XMLSchema#integer"/>
            </owl:Restriction>
        </rdfs:subClassOf>
        <rdfs:comment xml:lang="en">A tube bundle is a device consisting of tubes and bundles of tubes used for heat transfer and contained typically within other energy conversion devices, such as a chiller or coil.</rdfs:comment>
        <rdfs:label xml:lang="en">Tube bundle</rdfs:label>
        <rdfs:seeAlso>https://w3id.org/ifc/IFC4_ADD1#IfcTubeBundle</rdfs:seeAlso>
        <prov:hadPrimarySource rdf:resource="http://www.buildingsmart-tech.org/ifc/IFC4/Add1/html/schema/ifchvacdomain/lexical/ifctubebundle.htm"/>
        <prov:hadPrimarySource rdf:resource="http://www.buildingsmart-tech.org/ifc/IFC4/Add1/html/schema/ifchvacdomain/pset/pset_tubebundletypecommon.htm"/>
    </owl:Class>
    


    <!-- https://saref.etsi.org/saref4bldg/UnitaryControlElement -->


    <owl:Class rdf:about="https://saref.etsi.org/saref4bldg/UnitaryControlElement">
        <rdfs:subClassOf rdf:resource="https://saref.etsi.org/saref4bldg/DistributionControlDevice"/>
        <rdfs:comment xml:lang="en">A unitary control element combines a number of control components into a single product, such as a thermostat or humidistat.

A unitary control element provides a housing for an aggregation of control or electrical distribution elements that, in combination, perform a singular (unitary) purpose. Each item in the aggregation may have its own geometric representation and location.</rdfs:comment>
        <rdfs:label xml:lang="en">Unitary control element</rdfs:label>
        <rdfs:seeAlso>https://w3id.org/ifc/IFC4_ADD1#IfcUnitaryControlElement</rdfs:seeAlso>
        <prov:hadPrimarySource rdf:resource="http://www.buildingsmart-tech.org/ifc/IFC4/Add1/html/schema/ifcbuildingcontrolsdomain/lexical/ifcunitarycontrolelement.htm"/>
        <prov:hadPrimarySource rdf:resource="http://www.buildingsmart-tech.org/ifc/IFC4/Add1/html/schema/ifcbuildingcontrolsdomain/pset/pset_unitarycontrolelementtypecommon.htm"/>
    </owl:Class>
    


    <!-- https://saref.etsi.org/saref4bldg/Valve -->


    <owl:Class rdf:about="https://saref.etsi.org/saref4bldg/Valve">
        <rdfs:subClassOf rdf:resource="https://saref.etsi.org/saref4bldg/FlowController"/>
        <rdfs:subClassOf>
            <owl:Restriction>
                <owl:onProperty rdf:resource="https://saref.etsi.org/saref4bldg/closeOffRating"/>
                <owl:allValuesFrom rdf:resource="https://saref.etsi.org/core/Measurement"/>
            </owl:Restriction>
        </rdfs:subClassOf>
        <rdfs:subClassOf>
            <owl:Restriction>
                <owl:onProperty rdf:resource="https://saref.etsi.org/saref4bldg/flowCoefficient"/>
                <owl:allValuesFrom rdf:resource="https://saref.etsi.org/core/Measurement"/>
            </owl:Restriction>
        </rdfs:subClassOf>
        <rdfs:subClassOf>
            <owl:Restriction>
                <owl:onProperty rdf:resource="https://saref.etsi.org/saref4bldg/size"/>
                <owl:allValuesFrom rdf:resource="https://saref.etsi.org/core/Measurement"/>
            </owl:Restriction>
        </rdfs:subClassOf>
        <rdfs:subClassOf>
            <owl:Restriction>
                <owl:onProperty rdf:resource="https://saref.etsi.org/saref4bldg/testPressure"/>
                <owl:allValuesFrom rdf:resource="https://saref.etsi.org/core/Measurement"/>
            </owl:Restriction>
        </rdfs:subClassOf>
        <rdfs:subClassOf>
            <owl:Restriction>
                <owl:onProperty rdf:resource="https://saref.etsi.org/saref4bldg/workingPressure"/>
                <owl:allValuesFrom rdf:resource="https://saref.etsi.org/core/Measurement"/>
            </owl:Restriction>
        </rdfs:subClassOf>
        <rdfs:subClassOf>
            <owl:Restriction>
                <owl:onProperty rdf:resource="https://saref.etsi.org/saref4bldg/valveMechanism"/>
                <owl:allValuesFrom rdf:resource="http://www.w3.org/2001/XMLSchema#string"/>
            </owl:Restriction>
        </rdfs:subClassOf>
        <rdfs:subClassOf>
            <owl:Restriction>
                <owl:onProperty rdf:resource="https://saref.etsi.org/saref4bldg/valveOperation"/>
                <owl:allValuesFrom rdf:resource="http://www.w3.org/2001/XMLSchema#string"/>
            </owl:Restriction>
        </rdfs:subClassOf>
        <rdfs:subClassOf>
            <owl:Restriction>
                <owl:onProperty rdf:resource="https://saref.etsi.org/saref4bldg/valvePattern"/>
                <owl:allValuesFrom rdf:resource="http://www.w3.org/2001/XMLSchema#string"/>
            </owl:Restriction>
        </rdfs:subClassOf>
        <rdfs:comment xml:lang="en">A valve is used in a building services piping distribution system to control or modulate the flow of the fluid.</rdfs:comment>
        <rdfs:label xml:lang="en">Valve</rdfs:label>
        <rdfs:seeAlso>https://w3id.org/ifc/IFC4_ADD1#IfcValve</rdfs:seeAlso>
        <prov:hadPrimarySource rdf:resource="http://www.buildingsmart-tech.org/ifc/IFC4/Add1/html/schema/ifchvacdomain/lexical/ifcvalve.htm"/>
        <prov:hadPrimarySource rdf:resource="http://www.buildingsmart-tech.org/ifc/IFC4/Add1/html/schema/ifchvacdomain/pset/pset_valvetypecommon.htm"/>
    </owl:Class>
    


    <!-- https://saref.etsi.org/saref4bldg/VibrationIsolator -->


    <owl:Class rdf:about="https://saref.etsi.org/saref4bldg/VibrationIsolator">
        <rdfs:subClassOf rdf:resource="https://saref.etsi.org/core/Device"/>
        <rdfs:subClassOf>
            <owl:Restriction>
                <owl:onProperty rdf:resource="https://saref.etsi.org/saref4bldg/height"/>
                <owl:allValuesFrom rdf:resource="https://saref.etsi.org/core/Measurement"/>
            </owl:Restriction>
        </rdfs:subClassOf>
        <rdfs:subClassOf>
            <owl:Restriction>
                <owl:onProperty rdf:resource="https://saref.etsi.org/saref4bldg/isolatorCompressibility"/>
                <owl:allValuesFrom rdf:resource="https://saref.etsi.org/core/Measurement"/>
            </owl:Restriction>
        </rdfs:subClassOf>
        <rdfs:subClassOf>
            <owl:Restriction>
                <owl:onProperty rdf:resource="https://saref.etsi.org/saref4bldg/isolatorStaticDeflection"/>
                <owl:allValuesFrom rdf:resource="https://saref.etsi.org/core/Measurement"/>
            </owl:Restriction>
        </rdfs:subClassOf>
        <rdfs:subClassOf>
            <owl:Restriction>
                <owl:onProperty rdf:resource="https://saref.etsi.org/saref4bldg/supportedWeightMax"/>
                <owl:allValuesFrom rdf:resource="https://saref.etsi.org/core/Measurement"/>
            </owl:Restriction>
        </rdfs:subClassOf>
        <rdfs:subClassOf>
            <owl:Restriction>
                <owl:onProperty rdf:resource="https://saref.etsi.org/saref4bldg/vibrationTransmissibility"/>
                <owl:allValuesFrom rdf:resource="https://saref.etsi.org/core/Measurement"/>
            </owl:Restriction>
        </rdfs:subClassOf>
        <rdfs:comment xml:lang="en">A vibration isolator is a device used to minimize the effects of vibration transmissibility in a building.</rdfs:comment>
        <rdfs:label xml:lang="en">Vibration isolator</rdfs:label>
        <rdfs:seeAlso>https://w3id.org/ifc/IFC4_ADD1#IfcVibrationIsolator</rdfs:seeAlso>
        <prov:hadPrimarySource rdf:resource="http://www.buildingsmart-tech.org/ifc/IFC4/Add1/html/schema/ifchvacdomain/lexical/ifcvibrationisolator.htm"/>
        <prov:hadPrimarySource rdf:resource="http://www.buildingsmart-tech.org/ifc/IFC4/Add1/html/schema/ifchvacdomain/pset/pset_vibrationisolatortypecommon.htm"/>
    </owl:Class>
    


    <!-- https://saref.etsi.org/saref4city/Agent -->


    <owl:Class rdf:about="https://saref.etsi.org/saref4city/Agent">
        <rdfs:comment xml:lang="en">An agent making an action in the context of a city. An agent could be a person, software, etc.</rdfs:comment>
        <rdfs:isDefinedBy rdf:resource="https://saref.etsi.org/saref4city/"/>
        <rdfs:label xml:lang="en">Agent</rdfs:label>
    </owl:Class>
    


    <!-- https://saref.etsi.org/saref4city/KeyPerformanceIndicator -->


    <owl:Class rdf:about="https://saref.etsi.org/saref4city/KeyPerformanceIndicator">
        <rdfs:subClassOf>
            <owl:Restriction>
                <owl:onProperty rdf:resource="https://saref.etsi.org/saref4city/hasCalculationPeriod"/>
                <owl:allValuesFrom rdf:resource="http://www.w3.org/2006/time#TemporalDuration"/>
            </owl:Restriction>
        </rdfs:subClassOf>
        <rdfs:subClassOf>
            <owl:Restriction>
                <owl:onProperty rdf:resource="https://saref.etsi.org/saref4city/isKPIOf"/>
                <owl:allValuesFrom rdf:resource="https://saref.etsi.org/core/FeatureOfInterest"/>
            </owl:Restriction>
        </rdfs:subClassOf>
        <rdfs:comment xml:lang="en">A Key Performance Indicator (KPI) is a type of performance measurement. KPIs evaluate the success of an organization or of a particular activity in which it engages. (Definition taken from FIWARE)</rdfs:comment>
        <rdfs:isDefinedBy rdf:resource="https://saref.etsi.org/saref4city/"/>
        <rdfs:label xml:lang="en">Key Performance Indicator</rdfs:label>
        <rdfs:seeAlso rdf:resource="http://fiware-datamodels.readthedocs.io/en/latest/KeyPerformanceIndicator/doc/spec/index.html"/>
    </owl:Class>
    


    <!-- https://saref.etsi.org/saref4city/KeyPerformanceIndicatorAssessment -->


    <owl:Class rdf:about="https://saref.etsi.org/saref4city/KeyPerformanceIndicatorAssessment">
        <rdfs:subClassOf>
            <owl:Restriction>
                <owl:onProperty rdf:resource="https://saref.etsi.org/core/isMeasuredIn"/>
                <owl:allValuesFrom rdf:resource="https://saref.etsi.org/core/UnitOfMeasure"/>
            </owl:Restriction>
        </rdfs:subClassOf>
        <rdfs:subClassOf>
            <owl:Restriction>
                <owl:onProperty rdf:resource="https://saref.etsi.org/saref4city/assesses"/>
                <owl:allValuesFrom rdf:resource="https://saref.etsi.org/core/FeatureOfInterest"/>
            </owl:Restriction>
        </rdfs:subClassOf>
        <rdfs:subClassOf>
            <owl:Restriction>
                <owl:onProperty rdf:resource="https://saref.etsi.org/saref4city/isAssessedBy"/>
                <owl:allValuesFrom rdf:resource="https://saref.etsi.org/saref4city/Agent"/>
            </owl:Restriction>
        </rdfs:subClassOf>
        <rdfs:subClassOf>
            <owl:Restriction>
                <owl:onProperty rdf:resource="https://saref.etsi.org/saref4city/isDerivedFrom"/>
                <owl:allValuesFrom rdf:resource="https://saref.etsi.org/core/Measurement"/>
            </owl:Restriction>
        </rdfs:subClassOf>
        <rdfs:subClassOf>
            <owl:Restriction>
                <owl:onProperty rdf:resource="https://saref.etsi.org/saref4city/quantifiesKPI"/>
                <owl:allValuesFrom rdf:resource="https://saref.etsi.org/saref4city/KeyPerformanceIndicator"/>
            </owl:Restriction>
        </rdfs:subClassOf>
        <rdfs:subClassOf>
            <owl:Restriction>
                <owl:onProperty rdf:resource="https://saref.etsi.org/saref4city/refersToTime"/>
                <owl:allValuesFrom rdf:resource="http://www.w3.org/2006/time#TemporalEntity"/>
            </owl:Restriction>
        </rdfs:subClassOf>
        <rdfs:subClassOf>
            <owl:Restriction>
                <owl:onProperty rdf:resource="https://saref.etsi.org/saref4city/hasCreationDate"/>
                <owl:allValuesFrom rdf:resource="http://www.w3.org/2001/XMLSchema#dateTime"/>
            </owl:Restriction>
        </rdfs:subClassOf>
        <rdfs:subClassOf>
            <owl:Restriction>
                <owl:onProperty rdf:resource="https://saref.etsi.org/saref4city/hasExpirationDate"/>
                <owl:allValuesFrom rdf:resource="http://www.w3.org/2001/XMLSchema#dateTime"/>
            </owl:Restriction>
        </rdfs:subClassOf>
        <rdfs:subClassOf>
            <owl:Restriction>
                <owl:onProperty rdf:resource="https://saref.etsi.org/saref4city/hasLastUpdateDate"/>
                <owl:allValuesFrom rdf:resource="http://www.w3.org/2001/XMLSchema#dateTime"/>
            </owl:Restriction>
        </rdfs:subClassOf>
        <rdfs:subClassOf>
            <owl:Restriction>
                <owl:onProperty rdf:resource="https://saref.etsi.org/core/hasValue"/>
                <owl:cardinality rdf:datatype="http://www.w3.org/2001/XMLSchema#nonNegativeInteger">1</owl:cardinality>
            </owl:Restriction>
        </rdfs:subClassOf>
        <rdfs:comment xml:lang="en">A Key Performance Indicator assessment represents the assessment of a KPI calculated by a given agent in a given time.</rdfs:comment>
        <rdfs:isDefinedBy rdf:resource="https://saref.etsi.org/saref4city/"/>
        <rdfs:label xml:lang="en">Key performance indicator assessment</rdfs:label>
    </owl:Class>
    


    <!-- https://saref.etsi.org/saref4syst/Connection -->


    <owl:Class rdf:about="https://saref.etsi.org/saref4syst/Connection">
        <rdfs:subClassOf>
            <owl:Restriction>
                <owl:onProperty rdf:resource="https://saref.etsi.org/saref4syst/connectsSystem"/>
                <owl:someValuesFrom rdf:resource="https://saref.etsi.org/saref4syst/System"/>
            </owl:Restriction>
        </rdfs:subClassOf>
        <rdfs:subClassOf>
            <owl:Restriction>
                <owl:onProperty rdf:resource="https://saref.etsi.org/saref4syst/connectsSystemAt"/>
                <owl:someValuesFrom rdf:resource="https://saref.etsi.org/saref4syst/ConnectionPoint"/>
            </owl:Restriction>
        </rdfs:subClassOf>
        <owl:disjointWith rdf:resource="https://saref.etsi.org/saref4syst/ConnectionPoint"/>
        <owl:disjointWith rdf:resource="https://saref.etsi.org/saref4syst/System"/>
        <rdfs:comment xml:lang="en">The class of connections between systems. This class qualifies property s4syst:connectedTo. A connection describes potential interactions between systems. Any two connected systems are connected through a connection. A connection can connect more than two systems at the same time.</rdfs:comment>
        <rdfs:label xml:lang="en">Connection</rdfs:label>
    </owl:Class>
    


    <!-- https://saref.etsi.org/saref4syst/ConnectionPoint -->


    <owl:Class rdf:about="https://saref.etsi.org/saref4syst/ConnectionPoint">
        <rdfs:subClassOf>
            <owl:Restriction>
                <owl:onProperty rdf:resource="https://saref.etsi.org/saref4syst/connectionPointOf"/>
                <owl:cardinality rdf:datatype="http://www.w3.org/2001/XMLSchema#nonNegativeInteger">1</owl:cardinality>
            </owl:Restriction>
        </rdfs:subClassOf>
        <owl:disjointWith rdf:resource="https://saref.etsi.org/saref4syst/System"/>
        <rdfs:comment xml:lang="en">The class of connection points of systems, at which they may be connected to other systems. This class qualifies properties s4syst:connectsSystem and s4syst:connectedThrough. A connection point belongs to exactly one system. Any system connected through a connection is connected at one of its connection points to the connection. The system of a connection point that is connected through a connection is itself connected through the connection.</rdfs:comment>
        <rdfs:label xml:lang="en">Connection Point</rdfs:label>
    </owl:Class>
    


    <!-- https://saref.etsi.org/saref4syst/System -->


    <owl:Class rdf:about="https://saref.etsi.org/saref4syst/System">
        <rdfs:comment xml:lang="en">The class of systems, i.e., systems virtually isolated from the environment, whose behaviour and interactions with the environment are modeled. Systems can be connected to other systems. Connected systems interact in some ways. Systems can also have subsystems. Properties of subsystems somehow contribute to the properties of the supersystem.</rdfs:comment>
        <rdfs:isDefinedBy rdf:resource="https://saref.etsi.org/saref4syst/"/>
        <rdfs:label xml:lang="en">System</rdfs:label>
    </owl:Class>
    


    <!-- https://saref.etsi.org/saref4watr/AcceptabilityProperty -->


    <owl:Class rdf:about="https://saref.etsi.org/saref4watr/AcceptabilityProperty">
        <rdfs:subClassOf rdf:resource="https://saref.etsi.org/saref4watr/WaterProperty"/>
        <rdfs:comment xml:lang="en">An acceptability property is a property of water that is related to its acceptability.</rdfs:comment>
        <rdfs:label xml:lang="en">Acceptability property</rdfs:label>
    </owl:Class>
    


    <!-- https://saref.etsi.org/saref4watr/Aquifer -->


    <owl:Class rdf:about="https://saref.etsi.org/saref4watr/Aquifer">
        <rdfs:subClassOf rdf:resource="https://saref.etsi.org/saref4watr/StorageAsset"/>
        <rdfs:comment xml:lang="en">An aquifer is an underground layer of water-bearing permeable rock, rock fractures or unconsolidated materials.</rdfs:comment>
        <rdfs:label xml:lang="en">Aquifer</rdfs:label>
    </owl:Class>
    


    <!-- https://saref.etsi.org/saref4watr/BacterialProperty -->


    <owl:Class rdf:about="https://saref.etsi.org/saref4watr/BacterialProperty">
        <rdfs:subClassOf rdf:resource="https://saref.etsi.org/saref4watr/MicrobialProperty"/>
        <rdfs:comment xml:lang="en">A bacterial property is a property of water that is related to bacteria.</rdfs:comment>
        <rdfs:label xml:lang="en">Bacterial property</rdfs:label>
    </owl:Class>
    


    <!-- https://saref.etsi.org/saref4watr/Channel -->


    <owl:Class rdf:about="https://saref.etsi.org/saref4watr/Channel">
        <rdfs:subClassOf rdf:resource="https://saref.etsi.org/saref4watr/Main"/>
        <rdfs:comment xml:lang="en">A channel is a passage of water flowing in an open conduit (i.e., subject to atmospheric pressure).</rdfs:comment>
        <rdfs:label xml:lang="en">Channel</rdfs:label>
    </owl:Class>
    


    <!-- https://saref.etsi.org/saref4watr/ChemicalProperty -->


    <owl:Class rdf:about="https://saref.etsi.org/saref4watr/ChemicalProperty">
        <rdfs:subClassOf rdf:resource="https://saref.etsi.org/saref4watr/WaterProperty"/>
        <rdfs:comment xml:lang="en">A chemical property is a property of water that is related to chemical components.</rdfs:comment>
        <rdfs:label xml:lang="en">ChemicalProperty</rdfs:label>
    </owl:Class>
    


    <!-- https://saref.etsi.org/saref4watr/ConsumptionBasedTariff -->


    <owl:Class rdf:about="https://saref.etsi.org/saref4watr/ConsumptionBasedTariff">
        <rdfs:subClassOf rdf:resource="https://saref.etsi.org/saref4watr/Tariff"/>
        <rdfs:comment xml:lang="en">A consumption-based tariff is a tariff that is based on consumption.</rdfs:comment>
        <rdfs:label xml:lang="en">Consumption-based tariff</rdfs:label>
    </owl:Class>
    


    <!-- https://saref.etsi.org/saref4watr/DistributionSystem -->


    <owl:Class rdf:about="https://saref.etsi.org/saref4watr/DistributionSystem">
        <rdfs:subClassOf rdf:resource="https://saref.etsi.org/saref4watr/WaterInfrastructure"/>
        <rdfs:comment xml:lang="en">A water distribution system is an infrastructure to carry potable water from a centralized treatment plant or wells to water consumers in order to adequately deliver water to satisfy residential, commercial, industrial and fire fighting requirements.</rdfs:comment>
        <rdfs:label xml:lang="en">Distribution system</rdfs:label>
    </owl:Class>
    


    <!-- https://saref.etsi.org/saref4watr/EnvironmentalProperty -->


    <owl:Class rdf:about="https://saref.etsi.org/saref4watr/EnvironmentalProperty">
        <rdfs:subClassOf rdf:resource="https://saref.etsi.org/core/Property"/>
        <rdfs:comment xml:lang="en">Class to group those properties related to the environment.</rdfs:comment>
        <rdfs:label xml:lang="en">Environmental property</rdfs:label>
    </owl:Class>
    


    <!-- https://saref.etsi.org/saref4watr/Estuary -->


    <owl:Class rdf:about="https://saref.etsi.org/saref4watr/Estuary">
        <rdfs:subClassOf rdf:resource="https://saref.etsi.org/saref4watr/SinkAsset"/>
        <rdfs:comment xml:lang="en">An estuary is a partially enclosed coastal body of brackish water with one or more rivers or streams flowing into it, and with a free connection to the open sea.</rdfs:comment>
        <rdfs:label xml:lang="en">Estuary</rdfs:label>
    </owl:Class>
    


    <!-- https://saref.etsi.org/saref4watr/FireHydrant -->


    <owl:Class rdf:about="https://saref.etsi.org/saref4watr/FireHydrant">
        <rdfs:subClassOf rdf:resource="https://saref.etsi.org/saref4watr/WaterDevice"/>
        <rdfs:comment xml:lang="en">A fire hydrant is a fitting in a street or other public place with a nozzle by which a fire hose may be attached to a water main.</rdfs:comment>
        <rdfs:label xml:lang="en">Fire hydrant</rdfs:label>
    </owl:Class>
    


    <!-- https://saref.etsi.org/saref4watr/GaugingStation -->


    <owl:Class rdf:about="https://saref.etsi.org/saref4watr/GaugingStation">
        <rdfs:subClassOf rdf:resource="https://saref.etsi.org/saref4watr/MonitoringInfrastructure"/>
        <rdfs:comment xml:lang="en">A gauging station is an infrastructure to monitor and test terrestrial bodies of water.</rdfs:comment>
        <rdfs:label xml:lang="en">Gauging station</rdfs:label>
    </owl:Class>
    


    <!-- https://saref.etsi.org/saref4watr/Glacier -->


    <owl:Class rdf:about="https://saref.etsi.org/saref4watr/Glacier">
        <rdfs:subClassOf rdf:resource="https://saref.etsi.org/saref4watr/SourceAsset"/>
        <rdfs:comment xml:lang="en">A glacier is a persistent body of dense ice that is constantly moving under its own weight.</rdfs:comment>
        <rdfs:label xml:lang="en">Glacier</rdfs:label>
    </owl:Class>
    


    <!-- https://saref.etsi.org/saref4watr/HydroelectricPowerPlant -->


    <owl:Class rdf:about="https://saref.etsi.org/saref4watr/HydroelectricPowerPlant">
        <rdfs:subClassOf rdf:resource="https://saref.etsi.org/saref4watr/WaterInfrastructure"/>
        <rdfs:comment xml:lang="en">A hydroelectric power plant is an infrastructure to generate electricity by conversion of the energy of running water.</rdfs:comment>
        <rdfs:label xml:lang="en">Hydroelectric power plant</rdfs:label>
    </owl:Class>
    


    <!-- https://saref.etsi.org/saref4watr/Intake -->


    <owl:Class rdf:about="https://saref.etsi.org/saref4watr/Intake">
        <rdfs:subClassOf rdf:resource="https://saref.etsi.org/saref4watr/TransportAsset"/>
        <rdfs:comment xml:lang="en">An intake is an installation for obtaining water from a source of supply (river, lake, reservoir, and so on).</rdfs:comment>
        <rdfs:label xml:lang="en">Intake</rdfs:label>
    </owl:Class>
    


    <!-- https://saref.etsi.org/saref4watr/Lagoon -->


    <owl:Class rdf:about="https://saref.etsi.org/saref4watr/Lagoon">
        <rdfs:subClassOf rdf:resource="https://saref.etsi.org/saref4watr/SourceAsset"/>
        <rdfs:comment xml:lang="en">A lagoon is a shallow body of water separated from a larger body of water by barrier islands or reefs.</rdfs:comment>
        <rdfs:label xml:lang="en">Lagoon</rdfs:label>
    </owl:Class>
    


    <!-- https://saref.etsi.org/saref4watr/Lake -->


    <owl:Class rdf:about="https://saref.etsi.org/saref4watr/Lake">
        <rdfs:subClassOf rdf:resource="https://saref.etsi.org/saref4watr/SourceAsset"/>
        <rdfs:comment xml:lang="en">A lake is an area filled with water, localized in a basin, surrounded by land, apart from any river or other outlet that serves to feed or drain the lake.</rdfs:comment>
        <rdfs:label xml:lang="en">Lake</rdfs:label>
    </owl:Class>
    


    <!-- https://saref.etsi.org/saref4watr/Main -->


    <owl:Class rdf:about="https://saref.etsi.org/saref4watr/Main">
        <rdfs:subClassOf rdf:resource="https://saref.etsi.org/saref4watr/TransportAsset"/>
        <rdfs:comment xml:lang="en">A main is a passage of water to flow through.</rdfs:comment>
        <rdfs:label xml:lang="en">Main</rdfs:label>
    </owl:Class>
    


    <!-- https://saref.etsi.org/saref4watr/Manhole -->


    <owl:Class rdf:about="https://saref.etsi.org/saref4watr/Manhole">
        <rdfs:subClassOf rdf:resource="https://saref.etsi.org/saref4watr/TransportAsset"/>
        <rdfs:comment xml:lang="en">A maintenance hole is an enclosure that facilitates human access to and working space for equipment.</rdfs:comment>
        <rdfs:label xml:lang="en">Maintenance hole</rdfs:label>
        <rdfs:label xml:lang="en">Manhole</rdfs:label>
    </owl:Class>
    


    <!-- https://saref.etsi.org/saref4watr/MicrobialProperty -->


    <owl:Class rdf:about="https://saref.etsi.org/saref4watr/MicrobialProperty">
        <rdfs:subClassOf rdf:resource="https://saref.etsi.org/saref4watr/WaterProperty"/>
        <rdfs:comment xml:lang="en">A microbial property is a property of water that is related to microbes.</rdfs:comment>
        <rdfs:label xml:lang="en">Microbial property</rdfs:label>
    </owl:Class>
    


    <!-- https://saref.etsi.org/saref4watr/MonitoringInfrastructure -->


    <owl:Class rdf:about="https://saref.etsi.org/saref4watr/MonitoringInfrastructure">
        <rdfs:subClassOf rdf:resource="https://saref.etsi.org/saref4watr/WaterInfrastructure"/>
        <rdfs:comment xml:lang="en">A monitoring infrastructure is an infrastructure to monitor water.</rdfs:comment>
        <rdfs:label xml:lang="en">Monitoring infrastructure</rdfs:label>
    </owl:Class>
    


    <!-- https://saref.etsi.org/saref4watr/Ocean -->


    <owl:Class rdf:about="https://saref.etsi.org/saref4watr/Ocean">
        <rdfs:subClassOf rdf:resource="https://saref.etsi.org/saref4watr/SinkAsset"/>
        <rdfs:comment xml:lang="en">An ocean is a large body of salt water.</rdfs:comment>
        <rdfs:label xml:lang="en">Ocean</rdfs:label>
    </owl:Class>
    


    <!-- https://saref.etsi.org/saref4watr/Pipe -->


    <owl:Class rdf:about="https://saref.etsi.org/saref4watr/Pipe">
        <rdfs:subClassOf rdf:resource="https://saref.etsi.org/saref4watr/Main"/>
        <rdfs:comment xml:lang="en">A pipe is a passage of water flowing in a closed conduit (i.e., not subject to atmospheric pressure).</rdfs:comment>
        <rdfs:label xml:lang="en">Pipe</rdfs:label>
    </owl:Class>
    


    <!-- https://saref.etsi.org/saref4watr/Pit -->


    <owl:Class rdf:about="https://saref.etsi.org/saref4watr/Pit">
        <rdfs:subClassOf rdf:resource="https://saref.etsi.org/saref4watr/TransportAsset"/>
        <rdfs:comment xml:lang="en">A pit is a well or hole sunk in the ground to procure, store or drain water.</rdfs:comment>
        <rdfs:label xml:lang="en">Pit</rdfs:label>
    </owl:Class>
    


    <!-- https://saref.etsi.org/saref4watr/Pump -->


    <owl:Class rdf:about="https://saref.etsi.org/saref4watr/Pump">
        <rdfs:subClassOf rdf:resource="https://saref.etsi.org/core/Actuator"/>
        <rdfs:subClassOf rdf:resource="https://saref.etsi.org/saref4watr/WaterDevice"/>
        <rdfs:comment xml:lang="en">A pump is a device for moving water by mechanical action.</rdfs:comment>
        <rdfs:label xml:lang="en">Pump</rdfs:label>
    </owl:Class>
    


    <!-- https://saref.etsi.org/saref4watr/Reservoir -->


    <owl:Class rdf:about="https://saref.etsi.org/saref4watr/Reservoir">
        <rdfs:subClassOf rdf:resource="https://saref.etsi.org/saref4watr/StorageAsset"/>
        <rdfs:comment xml:lang="en">A reservoir is an enlarged natural or artificial lake, pond or impoundment created using a dam or lock to store water.</rdfs:comment>
        <rdfs:label xml:lang="en">Reservoir</rdfs:label>
    </owl:Class>
    


    <!-- https://saref.etsi.org/saref4watr/River -->


    <owl:Class rdf:about="https://saref.etsi.org/saref4watr/River">
        <rdfs:subClassOf rdf:resource="https://saref.etsi.org/saref4watr/SinkAsset"/>
        <rdfs:comment xml:lang="en">A river is a natural flowing watercourse, usually freshwater, flowing towards an ocean, sea, lake or another river.</rdfs:comment>
        <rdfs:label xml:lang="en">River</rdfs:label>
    </owl:Class>
    


    <!-- https://saref.etsi.org/saref4watr/Sea -->


    <owl:Class rdf:about="https://saref.etsi.org/saref4watr/Sea">
        <rdfs:subClassOf rdf:resource="https://saref.etsi.org/saref4watr/SinkAsset"/>
        <rdfs:comment xml:lang="en">A sea is a body of salt water partly or fully enclosed by land.</rdfs:comment>
        <rdfs:label xml:lang="en">Sea</rdfs:label>
    </owl:Class>
    


    <!-- https://saref.etsi.org/saref4watr/SinkAsset -->


    <owl:Class rdf:about="https://saref.etsi.org/saref4watr/SinkAsset">
        <rdfs:subClassOf rdf:resource="https://saref.etsi.org/saref4watr/WaterAsset"/>
        <rdfs:comment xml:lang="en">A sink asset is a water asset where water sinks.</rdfs:comment>
        <rdfs:label xml:lang="en">Sink asset</rdfs:label>
    </owl:Class>
    


    <!-- https://saref.etsi.org/saref4watr/SourceAsset -->


    <owl:Class rdf:about="https://saref.etsi.org/saref4watr/SourceAsset">
        <rdfs:subClassOf rdf:resource="https://saref.etsi.org/saref4watr/WaterAsset"/>
        <rdfs:comment xml:lang="en">A source asset is a water asset that is a natural source of water.</rdfs:comment>
        <rdfs:label xml:lang="en">Source asset</rdfs:label>
    </owl:Class>
    


    <!-- https://saref.etsi.org/saref4watr/StorageAsset -->


    <owl:Class rdf:about="https://saref.etsi.org/saref4watr/StorageAsset">
        <rdfs:subClassOf rdf:resource="https://saref.etsi.org/saref4watr/WaterAsset"/>
        <rdfs:comment xml:lang="en">A storage asset is a water asset used to store water.</rdfs:comment>
        <rdfs:label xml:lang="en">Storage asset</rdfs:label>
    </owl:Class>
    


    <!-- https://saref.etsi.org/saref4watr/StorageInfrastructure -->


    <owl:Class rdf:about="https://saref.etsi.org/saref4watr/StorageInfrastructure">
        <rdfs:subClassOf rdf:resource="https://saref.etsi.org/saref4watr/WaterInfrastructure"/>
        <rdfs:comment xml:lang="en">An storage infrastructure is an infrastructure to storage both potable water for consumption, and non potable water for use in agriculture.</rdfs:comment>
        <rdfs:label xml:lang="en">Storage infrastructure</rdfs:label>
    </owl:Class>
    


    <!-- https://saref.etsi.org/saref4watr/Tank -->


    <owl:Class rdf:about="https://saref.etsi.org/saref4watr/Tank">
        <rdfs:subClassOf rdf:resource="https://saref.etsi.org/saref4watr/StorageAsset"/>
        <rdfs:comment xml:lang="en">A tank is a container for storing water.</rdfs:comment>
        <rdfs:label xml:lang="en">Tank</rdfs:label>
    </owl:Class>
    


    <!-- https://saref.etsi.org/saref4watr/Tariff -->


    <owl:Class rdf:about="https://saref.etsi.org/saref4watr/Tariff">
        <rdfs:comment xml:lang="en">A tariff is a schedule of rates or charges of a business or a public utility. Tariffs can be based on time, thresholds or consumption; however, combined tariffs may also exist that mix more than one of these types.</rdfs:comment>
        <rdfs:label xml:lang="en">Tariff</rdfs:label>
    </owl:Class>
    


    <!-- https://saref.etsi.org/saref4watr/ThresholdBasedTariff -->


    <owl:Class rdf:about="https://saref.etsi.org/saref4watr/ThresholdBasedTariff">
        <rdfs:subClassOf rdf:resource="https://saref.etsi.org/saref4watr/Tariff"/>
        <rdfs:comment xml:lang="en">A threshold-based tariff is a tariff that is based on a threshold.</rdfs:comment>
        <rdfs:label xml:lang="en">Threshold-based tariff</rdfs:label>
    </owl:Class>
    


    <!-- https://saref.etsi.org/saref4watr/TimeBasedTariff -->


    <owl:Class rdf:about="https://saref.etsi.org/saref4watr/TimeBasedTariff">
        <rdfs:subClassOf rdf:resource="https://saref.etsi.org/saref4watr/Tariff"/>
        <rdfs:comment xml:lang="en">A time-based tariff is a tariff that is based on time.</rdfs:comment>
        <rdfs:label xml:lang="en">Time-based tariff</rdfs:label>
    </owl:Class>
    


    <!-- https://saref.etsi.org/saref4watr/TransportAsset -->


    <owl:Class rdf:about="https://saref.etsi.org/saref4watr/TransportAsset">
        <rdfs:subClassOf rdf:resource="https://saref.etsi.org/saref4watr/WaterAsset"/>
        <rdfs:comment xml:lang="en">A transport asset is a water asset used to enable and support the transport and distribution of water.</rdfs:comment>
        <rdfs:label xml:lang="en">Transport asset</rdfs:label>
    </owl:Class>
    


    <!-- https://saref.etsi.org/saref4watr/TreatmentPlant -->


    <owl:Class rdf:about="https://saref.etsi.org/saref4watr/TreatmentPlant">
        <rdfs:subClassOf rdf:resource="https://saref.etsi.org/saref4watr/WaterInfrastructure"/>
        <rdfs:comment xml:lang="en">A treatment plant is an infrastructure to improve the quality of water to make it more acceptable for a specific end-use.</rdfs:comment>
        <rdfs:label xml:lang="en">Treatment plant</rdfs:label>
    </owl:Class>
    


    <!-- https://saref.etsi.org/saref4watr/Valve -->


    <owl:Class rdf:about="https://saref.etsi.org/saref4watr/Valve">
        <rdfs:subClassOf rdf:resource="https://saref.etsi.org/core/Actuator"/>
        <rdfs:subClassOf rdf:resource="https://saref.etsi.org/saref4watr/WaterDevice"/>
        <rdfs:comment xml:lang="en">A valve is a device designed to control water flow, pressure or volume.</rdfs:comment>
        <rdfs:label xml:lang="en">Valve</rdfs:label>
    </owl:Class>
    


    <!-- https://saref.etsi.org/saref4watr/Vent -->


    <owl:Class rdf:about="https://saref.etsi.org/saref4watr/Vent">
        <rdfs:subClassOf rdf:resource="https://saref.etsi.org/saref4watr/TransportAsset"/>
        <rdfs:comment xml:lang="en">A vent is the part of a system that allows air to enter a plumbing system to maintain proper air pressure and sewer gases to escape to the outside.</rdfs:comment>
        <rdfs:label xml:lang="en">Vent</rdfs:label>
    </owl:Class>
    


    <!-- https://saref.etsi.org/saref4watr/Water -->


    <owl:Class rdf:about="https://saref.etsi.org/saref4watr/Water">
        <rdfs:subClassOf rdf:resource="https://saref.etsi.org/core/FeatureOfInterest"/>
        <rdfs:subClassOf>
            <owl:Restriction>
                <owl:onProperty rdf:resource="https://saref.etsi.org/core/hasProperty"/>
                <owl:allValuesFrom rdf:resource="https://saref.etsi.org/saref4watr/WaterProperty"/>
            </owl:Restriction>
        </rdfs:subClassOf>
        <rdfs:comment xml:lang="en">This class is used to define a particular quantity or body of water.</rdfs:comment>
        <rdfs:label xml:lang="en">Water</rdfs:label>
    </owl:Class>
    


    <!-- https://saref.etsi.org/saref4watr/WaterAsset -->


    <owl:Class rdf:about="https://saref.etsi.org/saref4watr/WaterAsset">
        <rdfs:subClassOf rdf:resource="http://www.opengis.net/ont/geosparql#Feature"/>
        <rdfs:subClassOf rdf:resource="https://saref.etsi.org/core/FeatureOfInterest"/>
        <rdfs:subClassOf rdf:resource="https://saref.etsi.org/saref4syst/System"/>
        <rdfs:comment xml:lang="en">A water asset is a physical entity used in the process of transporting, treating, storing and distributing water.</rdfs:comment>
        <rdfs:label xml:lang="en">Water asset</rdfs:label>
    </owl:Class>
    


    <!-- https://saref.etsi.org/saref4watr/WaterDevice -->


    <owl:Class rdf:about="https://saref.etsi.org/saref4watr/WaterDevice">
        <rdfs:subClassOf rdf:resource="https://saref.etsi.org/core/Device"/>
        <rdfs:subClassOf rdf:resource="https://saref.etsi.org/saref4watr/WaterAsset"/>
        <rdfs:comment xml:lang="en">A water device is a device that is also a water asset.</rdfs:comment>
        <rdfs:label xml:lang="en">Water device</rdfs:label>
    </owl:Class>
    


    <!-- https://saref.etsi.org/saref4watr/WaterFlowProperty -->


    <owl:Class rdf:about="https://saref.etsi.org/saref4watr/WaterFlowProperty">
        <rdfs:subClassOf rdf:resource="https://saref.etsi.org/core/Property"/>
        <rdfs:comment xml:lang="en">Class to group those properties related to water flow.</rdfs:comment>
        <rdfs:label xml:lang="en">Water flow property</rdfs:label>
    </owl:Class>
    


    <!-- https://saref.etsi.org/saref4watr/WaterInfrastructure -->


    <owl:Class rdf:about="https://saref.etsi.org/saref4watr/WaterInfrastructure">
        <rdfs:subClassOf rdf:resource="http://www.opengis.net/ont/geosparql#Feature"/>
        <rdfs:subClassOf rdf:resource="https://saref.etsi.org/core/FeatureOfInterest"/>
        <rdfs:subClassOf rdf:resource="https://saref.etsi.org/saref4syst/System"/>
        <rdfs:subClassOf>
            <owl:Restriction>
                <owl:onProperty rdf:resource="https://saref.etsi.org/saref4watr/isDesignedFor"/>
                <owl:someValuesFrom rdf:resource="https://saref.etsi.org/saref4watr/Water"/>
            </owl:Restriction>
        </rdfs:subClassOf>
        <rdfs:subClassOf>
            <owl:Restriction>
                <owl:onProperty rdf:resource="https://saref.etsi.org/saref4watr/isIntendedFor"/>
                <owl:someValuesFrom rdf:resource="https://saref.etsi.org/saref4watr/WaterUse"/>
            </owl:Restriction>
        </rdfs:subClassOf>
        <rdfs:comment xml:lang="en">A water infrastructure is the set of facilities, services, and installations needed for water management.</rdfs:comment>
        <rdfs:label xml:lang="en">Water infrastructure</rdfs:label>
    </owl:Class>
    


    <!-- https://saref.etsi.org/saref4watr/WaterMeter -->


    <owl:Class rdf:about="https://saref.etsi.org/saref4watr/WaterMeter">
        <rdfs:subClassOf rdf:resource="https://saref.etsi.org/core/Meter"/>
        <rdfs:subClassOf rdf:resource="https://saref.etsi.org/saref4watr/WaterDevice"/>
        <rdfs:subClassOf>
            <owl:Restriction>
                <owl:onProperty rdf:resource="https://saref.etsi.org/core/measuresProperty"/>
                <owl:someValuesFrom rdf:resource="https://saref.etsi.org/saref4watr/WaterFlowProperty"/>
            </owl:Restriction>
        </rdfs:subClassOf>
        <rdfs:subClassOf>
            <owl:Restriction>
                <owl:onProperty rdf:resource="https://saref.etsi.org/core/hasProperty"/>
                <owl:allValuesFrom rdf:resource="https://saref.etsi.org/saref4watr/WaterMeterProperty"/>
            </owl:Restriction>
        </rdfs:subClassOf>
        <rdfs:subClassOf>
            <owl:Restriction>
                <owl:onProperty rdf:resource="https://saref.etsi.org/saref4watr/hasFabricationNumber"/>
                <owl:maxCardinality rdf:datatype="http://www.w3.org/2001/XMLSchema#nonNegativeInteger">1</owl:maxCardinality>
            </owl:Restriction>
        </rdfs:subClassOf>
        <rdfs:subClassOf>
            <owl:Restriction>
                <owl:onProperty rdf:resource="https://saref.etsi.org/saref4watr/hasFirmwareVersion"/>
                <owl:maxCardinality rdf:datatype="http://www.w3.org/2001/XMLSchema#nonNegativeInteger">1</owl:maxCardinality>
            </owl:Restriction>
        </rdfs:subClassOf>
        <rdfs:subClassOf>
            <owl:Restriction>
                <owl:onProperty rdf:resource="https://saref.etsi.org/saref4watr/hasHardwareVersion"/>
                <owl:maxCardinality rdf:datatype="http://www.w3.org/2001/XMLSchema#nonNegativeInteger">1</owl:maxCardinality>
            </owl:Restriction>
        </rdfs:subClassOf>
        <rdfs:subClassOf>
            <owl:Restriction>
                <owl:onProperty rdf:resource="https://saref.etsi.org/saref4watr/hasVersion"/>
                <owl:maxCardinality rdf:datatype="http://www.w3.org/2001/XMLSchema#nonNegativeInteger">1</owl:maxCardinality>
            </owl:Restriction>
        </rdfs:subClassOf>
        <rdfs:comment xml:lang="en">A water meter is an instrument intended to measure continuously, memorize, and display the volume of water passing through the meter.</rdfs:comment>
        <rdfs:label xml:lang="en">Water meter</rdfs:label>
    </owl:Class>
    


    <!-- https://saref.etsi.org/saref4watr/WaterMeterProperty -->


    <owl:Class rdf:about="https://saref.etsi.org/saref4watr/WaterMeterProperty">
        <rdfs:subClassOf rdf:resource="https://saref.etsi.org/core/Property"/>
        <rdfs:comment xml:lang="en">Class to group those properties related to water meters.</rdfs:comment>
        <rdfs:label xml:lang="en">Water meter property</rdfs:label>
    </owl:Class>
    


    <!-- https://saref.etsi.org/saref4watr/WaterProperty -->


    <owl:Class rdf:about="https://saref.etsi.org/saref4watr/WaterProperty">
        <rdfs:subClassOf rdf:resource="https://saref.etsi.org/core/Property"/>
        <rdfs:comment xml:lang="en">Class to group those properties related to the water.</rdfs:comment>
        <rdfs:label xml:lang="en">Water property</rdfs:label>
    </owl:Class>
    


    <!-- https://saref.etsi.org/saref4watr/WaterUse -->


    <owl:Class rdf:about="https://saref.etsi.org/saref4watr/WaterUse">
        <rdfs:comment xml:lang="en">This class is used to define the different uses of water.</rdfs:comment>
        <rdfs:label xml:lang="en">Water use</rdfs:label>
    </owl:Class>
    


    <!-- https://schema.org/Organization -->


    <owl:Class rdf:about="https://schema.org/Organization">
        <rdfs:subClassOf rdf:resource="http://xmlns.com/foaf/0.1/Agent"/>
        <rdfs:label xml:lang="en">Organization</rdfs:label>
    </owl:Class>
    


    <!-- https://schema.org/Person -->


    <owl:Class rdf:about="https://schema.org/Person"/>
    


    <!-- 
    ///////////////////////////////////////////////////////////////////////////////////////
    //
    // Individuals
    //
    ///////////////////////////////////////////////////////////////////////////////////////
     -->


    


    <!-- http://dbpedia.org/resource/DBM -->


    <owl:NamedIndividual rdf:about="http://dbpedia.org/resource/DBM">
        <rdf:type rdf:resource="https://saref.etsi.org/core/UnitOfMeasure"/>
        <rdfs:label xml:lang="en">decibel-milliwatts</rdfs:label>
    </owl:NamedIndividual>
    


    <!-- http://qudt.org/vocab/unit/KiloW-HR -->


    <owl:NamedIndividual rdf:about="http://qudt.org/vocab/unit/KiloW-HR">
        <rdf:type rdf:resource="https://saref.etsi.org/core/EnergyUnit"/>
    </owl:NamedIndividual>
    


    <!-- http://qudt.org/vocab/unit/M2 -->


    <owl:NamedIndividual rdf:about="http://qudt.org/vocab/unit/M2"/>
    


    <!-- http://www.ontology-of-units-of-measure.org/resource/om-2/degreeCelsius -->


    <owl:NamedIndividual rdf:about="http://www.ontology-of-units-of-measure.org/resource/om-2/degreeCelsius">
        <rdf:type rdf:resource="https://saref.etsi.org/core/UnitOfMeasure"/>
        <rdfs:label xml:lang="en">degree Celsius</rdfs:label>
    </owl:NamedIndividual>
    


    <!-- http://www.ontology-of-units-of-measure.org/resource/om-2/millibar -->


    <owl:NamedIndividual rdf:about="http://www.ontology-of-units-of-measure.org/resource/om-2/millibar">
        <rdf:type rdf:resource="https://saref.etsi.org/core/UnitOfMeasure"/>
        <rdfs:label xml:lang="en">millibar</rdfs:label>
    </owl:NamedIndividual>
    


    <!-- http://www.ontology-of-units-of-measure.org/resource/om-2/millimetre -->


    <owl:NamedIndividual rdf:about="http://www.ontology-of-units-of-measure.org/resource/om-2/millimetre">
        <rdf:type rdf:resource="https://saref.etsi.org/core/UnitOfMeasure"/>
        <rdfs:label xml:lang="en">millimetre</rdfs:label>
    </owl:NamedIndividual>
    


    <!-- http://www.ontology-of-units-of-measure.org/resource/om-2/millivolt -->


    <owl:NamedIndividual rdf:about="http://www.ontology-of-units-of-measure.org/resource/om-2/millivolt">
        <rdf:type rdf:resource="https://saref.etsi.org/core/UnitOfMeasure"/>
        <rdfs:label xml:lang="en">millivolt</rdfs:label>
    </owl:NamedIndividual>
    


    <!-- http://www.opengis.net/def/uom/ISO-8601/0/Gregorian -->


    <owl:NamedIndividual rdf:about="http://www.opengis.net/def/uom/ISO-8601/0/Gregorian"/>
    


    <!-- http://www.w3.org/2006/time#Friday -->


    <owl:NamedIndividual rdf:about="http://www.w3.org/2006/time#Friday">
        <rdf:type rdf:resource="http://www.w3.org/2006/time#DayOfWeek"/>
        <rdfs:label xml:lang="en">Friday</rdfs:label>
        <skos:prefLabel xml:lang="de">Freitag</skos:prefLabel>
        <skos:prefLabel xml:lang="en">Friday</skos:prefLabel>
        <skos:prefLabel xml:lang="pl">Piątek</skos:prefLabel>
        <skos:prefLabel xml:lang="pt">Sexta-feira</skos:prefLabel>
        <skos:prefLabel xml:lang="fr">Vendredi</skos:prefLabel>
        <skos:prefLabel xml:lang="it">Venerdì</skos:prefLabel>
        <skos:prefLabel xml:lang="es">Viernes</skos:prefLabel>
        <skos:prefLabel xml:lang="nl">Vrijdag</skos:prefLabel>
        <skos:prefLabel xml:lang="ru">Пятница</skos:prefLabel>
        <skos:prefLabel xml:lang="ar">الجمعة</skos:prefLabel>
        <skos:prefLabel xml:lang="zh">星期五</skos:prefLabel>
        <skos:prefLabel xml:lang="ja">金曜日</skos:prefLabel>
    </owl:NamedIndividual>
    


    <!-- http://www.w3.org/2006/time#Monday -->


    <owl:NamedIndividual rdf:about="http://www.w3.org/2006/time#Monday">
        <rdf:type rdf:resource="http://www.w3.org/2006/time#DayOfWeek"/>
        <rdfs:label xml:lang="en">Monday</rdfs:label>
        <skos:prefLabel xml:lang="fr">Lundi</skos:prefLabel>
        <skos:prefLabel xml:lang="it">Lunedì</skos:prefLabel>
        <skos:prefLabel xml:lang="es">Lunes</skos:prefLabel>
        <skos:prefLabel xml:lang="nl">Maandag</skos:prefLabel>
        <skos:prefLabel xml:lang="en">Monday</skos:prefLabel>
        <skos:prefLabel xml:lang="de">Montag</skos:prefLabel>
        <skos:prefLabel xml:lang="pl">Poniedziałek</skos:prefLabel>
        <skos:prefLabel xml:lang="pt">Segunda-feira</skos:prefLabel>
        <skos:prefLabel xml:lang="ru">Понедельник</skos:prefLabel>
        <skos:prefLabel xml:lang="ar">الاثنين</skos:prefLabel>
        <skos:prefLabel xml:lang="zh">星期一</skos:prefLabel>
        <skos:prefLabel xml:lang="ja">月曜日</skos:prefLabel>
    </owl:NamedIndividual>
    


    <!-- http://www.w3.org/2006/time#Saturday -->


    <owl:NamedIndividual rdf:about="http://www.w3.org/2006/time#Saturday">
        <rdf:type rdf:resource="http://www.w3.org/2006/time#DayOfWeek"/>
        <rdfs:label xml:lang="en">Saturday</rdfs:label>
        <skos:prefLabel xml:lang="it">Sabato</skos:prefLabel>
        <skos:prefLabel xml:lang="fr">Samedi</skos:prefLabel>
        <skos:prefLabel xml:lang="de">Samstag</skos:prefLabel>
        <skos:prefLabel xml:lang="en">Saturday</skos:prefLabel>
        <skos:prefLabel xml:lang="pl">Sobota</skos:prefLabel>
        <skos:prefLabel xml:lang="es">Sábado</skos:prefLabel>
        <skos:prefLabel xml:lang="pt">Sábado</skos:prefLabel>
        <skos:prefLabel xml:lang="nl">Zaterdag</skos:prefLabel>
        <skos:prefLabel xml:lang="ru">Суббота</skos:prefLabel>
        <skos:prefLabel xml:lang="ar">السبت</skos:prefLabel>
        <skos:prefLabel xml:lang="ja">土曜日</skos:prefLabel>
        <skos:prefLabel xml:lang="zh">星期六</skos:prefLabel>
    </owl:NamedIndividual>
    


    <!-- http://www.w3.org/2006/time#Sunday -->


    <owl:NamedIndividual rdf:about="http://www.w3.org/2006/time#Sunday">
        <rdf:type rdf:resource="http://www.w3.org/2006/time#DayOfWeek"/>
        <rdfs:label xml:lang="en">Sunday</rdfs:label>
        <skos:prefLabel xml:lang="fr">Dimanche</skos:prefLabel>
        <skos:prefLabel xml:lang="it">Domenica</skos:prefLabel>
        <skos:prefLabel xml:lang="es">Domingo</skos:prefLabel>
        <skos:prefLabel xml:lang="pt">Domingo</skos:prefLabel>
        <skos:prefLabel xml:lang="pl">Niedziela</skos:prefLabel>
        <skos:prefLabel xml:lang="de">Sonntag</skos:prefLabel>
        <skos:prefLabel xml:lang="en">Sunday</skos:prefLabel>
        <skos:prefLabel xml:lang="nl">Zondag</skos:prefLabel>
        <skos:prefLabel xml:lang="ru">Воскресенье</skos:prefLabel>
        <skos:prefLabel xml:lang="ar">الأحد (يوم)</skos:prefLabel>
        <skos:prefLabel xml:lang="ja">日曜日</skos:prefLabel>
        <skos:prefLabel xml:lang="zh">星期日</skos:prefLabel>
    </owl:NamedIndividual>
    


    <!-- http://www.w3.org/2006/time#Thursday -->


    <owl:NamedIndividual rdf:about="http://www.w3.org/2006/time#Thursday">
        <rdf:type rdf:resource="http://www.w3.org/2006/time#DayOfWeek"/>
        <rdfs:label xml:lang="en">Thursday</rdfs:label>
        <skos:prefLabel xml:lang="pl">Czwartek</skos:prefLabel>
        <skos:prefLabel xml:lang="nl">Donderdag</skos:prefLabel>
        <skos:prefLabel xml:lang="de">Donnerstag</skos:prefLabel>
        <skos:prefLabel xml:lang="it">Giovedì</skos:prefLabel>
        <skos:prefLabel xml:lang="fr">Jeudi</skos:prefLabel>
        <skos:prefLabel xml:lang="es">Jueves</skos:prefLabel>
        <skos:prefLabel xml:lang="pt">Quinta-feira</skos:prefLabel>
        <skos:prefLabel xml:lang="en">Thursday</skos:prefLabel>
        <skos:prefLabel xml:lang="ru">Четверг</skos:prefLabel>
        <skos:prefLabel xml:lang="ar">الخميس</skos:prefLabel>
        <skos:prefLabel xml:lang="zh">星期四</skos:prefLabel>
        <skos:prefLabel xml:lang="ja">木曜日</skos:prefLabel>
    </owl:NamedIndividual>
    


    <!-- http://www.w3.org/2006/time#Tuesday -->


    <owl:NamedIndividual rdf:about="http://www.w3.org/2006/time#Tuesday">
        <rdf:type rdf:resource="http://www.w3.org/2006/time#DayOfWeek"/>
        <rdfs:label xml:lang="en">Tuesday</rdfs:label>
        <skos:prefLabel xml:lang="de">Dienstag</skos:prefLabel>
        <skos:prefLabel xml:lang="nl">Dinsdag</skos:prefLabel>
        <skos:prefLabel xml:lang="fr">Mardi</skos:prefLabel>
        <skos:prefLabel xml:lang="it">Martedì</skos:prefLabel>
        <skos:prefLabel xml:lang="es">Martes</skos:prefLabel>
        <skos:prefLabel xml:lang="pt">Terça-feira</skos:prefLabel>
        <skos:prefLabel xml:lang="en">Tuesday</skos:prefLabel>
        <skos:prefLabel xml:lang="pl">Wtorek</skos:prefLabel>
        <skos:prefLabel xml:lang="ru">Вторник</skos:prefLabel>
        <skos:prefLabel xml:lang="ar">الثلاثاء</skos:prefLabel>
        <skos:prefLabel xml:lang="zh">星期二</skos:prefLabel>
        <skos:prefLabel xml:lang="ja">火曜日</skos:prefLabel>
    </owl:NamedIndividual>
    


    <!-- http://www.w3.org/2006/time#Wednesday -->


    <owl:NamedIndividual rdf:about="http://www.w3.org/2006/time#Wednesday">
        <rdf:type rdf:resource="http://www.w3.org/2006/time#DayOfWeek"/>
        <rdfs:label xml:lang="en">Wednesday</rdfs:label>
        <skos:prefLabel xml:lang="it">Mercoledì</skos:prefLabel>
        <skos:prefLabel xml:lang="fr">Mercredi</skos:prefLabel>
        <skos:prefLabel xml:lang="de">Mittwoch</skos:prefLabel>
        <skos:prefLabel xml:lang="es">Miércoles</skos:prefLabel>
        <skos:prefLabel xml:lang="pt">Quarta-feira</skos:prefLabel>
        <skos:prefLabel xml:lang="en">Wednesday</skos:prefLabel>
        <skos:prefLabel xml:lang="nl">Woensdag</skos:prefLabel>
        <skos:prefLabel xml:lang="pl">Środa</skos:prefLabel>
        <skos:prefLabel xml:lang="ru">Среда</skos:prefLabel>
        <skos:prefLabel xml:lang="ar">الأربعاء</skos:prefLabel>
        <skos:prefLabel xml:lang="zh">星期三</skos:prefLabel>
        <skos:prefLabel xml:lang="ja">水曜日</skos:prefLabel>
    </owl:NamedIndividual>
    


    <!-- http://www.w3.org/2006/time#unitDay -->


    <owl:NamedIndividual rdf:about="http://www.w3.org/2006/time#unitDay">
        <rdf:type rdf:resource="http://www.w3.org/2006/time#TemporalUnit"/>
        <time:days rdf:datatype="http://www.w3.org/2001/XMLSchema#integer">1</time:days>
        <time:hours rdf:datatype="http://www.w3.org/2001/XMLSchema#integer">0</time:hours>
        <time:minutes rdf:datatype="http://www.w3.org/2001/XMLSchema#integer">0</time:minutes>
        <time:months rdf:datatype="http://www.w3.org/2001/XMLSchema#integer">0</time:months>
        <time:seconds rdf:datatype="http://www.w3.org/2001/XMLSchema#integer">0</time:seconds>
        <time:weeks rdf:datatype="http://www.w3.org/2001/XMLSchema#integer">0</time:weeks>
        <time:years rdf:datatype="http://www.w3.org/2001/XMLSchema#integer">0</time:years>
        <rdfs:label xml:lang="en">Day (unit of temporal duration)</rdfs:label>
        <skos:prefLabel xml:lang="de">Tag</skos:prefLabel>
        <skos:prefLabel xml:lang="nl">dag</skos:prefLabel>
        <skos:prefLabel xml:lang="en">day</skos:prefLabel>
        <skos:prefLabel xml:lang="pt">dia</skos:prefLabel>
        <skos:prefLabel xml:lang="pl">doba</skos:prefLabel>
        <skos:prefLabel xml:lang="es">día</skos:prefLabel>
        <skos:prefLabel xml:lang="it">giorno</skos:prefLabel>
        <skos:prefLabel xml:lang="fr">jour</skos:prefLabel>
        <skos:prefLabel xml:lang="ar">يوماً ما</skos:prefLabel>
        <skos:prefLabel xml:lang="jp">ある日</skos:prefLabel>
        <skos:prefLabel xml:lang="zh">一天</skos:prefLabel>
        <skos:prefLabel xml:lang="kr">언젠가</skos:prefLabel>
    </owl:NamedIndividual>
    


    <!-- http://www.w3.org/2006/time#unitHour -->


    <owl:NamedIndividual rdf:about="http://www.w3.org/2006/time#unitHour">
        <rdf:type rdf:resource="http://www.w3.org/2006/time#TemporalUnit"/>
        <time:days rdf:datatype="http://www.w3.org/2001/XMLSchema#integer">0</time:days>
        <time:hours rdf:datatype="http://www.w3.org/2001/XMLSchema#integer">1</time:hours>
        <time:minutes rdf:datatype="http://www.w3.org/2001/XMLSchema#integer">0</time:minutes>
        <time:months rdf:datatype="http://www.w3.org/2001/XMLSchema#integer">0</time:months>
        <time:seconds rdf:datatype="http://www.w3.org/2001/XMLSchema#integer">0</time:seconds>
        <time:weeks rdf:datatype="http://www.w3.org/2001/XMLSchema#integer">0</time:weeks>
        <time:years rdf:datatype="http://www.w3.org/2001/XMLSchema#integer">0</time:years>
        <rdfs:label xml:lang="en">Hour (unit of temporal duration)</rdfs:label>
        <skos:prefLabel xml:lang="de">Stunde</skos:prefLabel>
        <skos:prefLabel xml:lang="pl">godzina</skos:prefLabel>
        <skos:prefLabel xml:lang="fr">heure</skos:prefLabel>
        <skos:prefLabel xml:lang="es">hora</skos:prefLabel>
        <skos:prefLabel xml:lang="pt">hora</skos:prefLabel>
        <skos:prefLabel xml:lang="en">hour</skos:prefLabel>
        <skos:prefLabel xml:lang="it">ora</skos:prefLabel>
        <skos:prefLabel xml:lang="nl">uur</skos:prefLabel>
        <skos:prefLabel xml:lang="ar">ساعة واحدة</skos:prefLabel>
        <skos:prefLabel xml:lang="zh">一小時</skos:prefLabel>
        <skos:prefLabel xml:lang="jp">一時間</skos:prefLabel>
        <skos:prefLabel xml:lang="kr">한 시간</skos:prefLabel>
        <skos:prefLabel>один час&quot;@ru</skos:prefLabel>
    </owl:NamedIndividual>
    


    <!-- http://www.w3.org/2006/time#unitMinute -->


    <owl:NamedIndividual rdf:about="http://www.w3.org/2006/time#unitMinute">
        <rdf:type rdf:resource="http://www.w3.org/2006/time#TemporalUnit"/>
        <time:days rdf:datatype="http://www.w3.org/2001/XMLSchema#integer">0</time:days>
        <time:hours rdf:datatype="http://www.w3.org/2001/XMLSchema#integer">0</time:hours>
        <time:minutes rdf:datatype="http://www.w3.org/2001/XMLSchema#integer">1</time:minutes>
        <time:months rdf:datatype="http://www.w3.org/2001/XMLSchema#integer">0</time:months>
        <time:seconds rdf:datatype="http://www.w3.org/2001/XMLSchema#integer">0</time:seconds>
        <time:weeks rdf:datatype="http://www.w3.org/2001/XMLSchema#integer">0</time:weeks>
        <time:years rdf:datatype="http://www.w3.org/2001/XMLSchema#integer">0</time:years>
        <rdfs:label xml:lang="en">Minute (unit of temporal duration)</rdfs:label>
        <skos:prefLabel xml:lang="de">Minute</skos:prefLabel>
        <skos:prefLabel xml:lang="pl">minuta</skos:prefLabel>
        <skos:prefLabel xml:lang="en">minute</skos:prefLabel>
        <skos:prefLabel xml:lang="fr">minute</skos:prefLabel>
        <skos:prefLabel xml:lang="es">minuto</skos:prefLabel>
        <skos:prefLabel xml:lang="it">minuto</skos:prefLabel>
        <skos:prefLabel xml:lang="pt">minuto</skos:prefLabel>
        <skos:prefLabel xml:lang="nl">minuut</skos:prefLabel>
        <skos:prefLabel xml:lang="ru">одна минута</skos:prefLabel>
        <skos:prefLabel xml:lang="ar">دقيقة واحدة</skos:prefLabel>
        <skos:prefLabel xml:lang="jp">一分</skos:prefLabel>
        <skos:prefLabel xml:lang="zh">等一下</skos:prefLabel>
        <skos:prefLabel xml:lang="kr">분</skos:prefLabel>
    </owl:NamedIndividual>
    


    <!-- http://www.w3.org/2006/time#unitMonth -->


    <owl:NamedIndividual rdf:about="http://www.w3.org/2006/time#unitMonth">
        <rdf:type rdf:resource="http://www.w3.org/2006/time#TemporalUnit"/>
        <time:days rdf:datatype="http://www.w3.org/2001/XMLSchema#integer">0</time:days>
        <time:hours rdf:datatype="http://www.w3.org/2001/XMLSchema#integer">0</time:hours>
        <time:minutes rdf:datatype="http://www.w3.org/2001/XMLSchema#integer">0</time:minutes>
        <time:months rdf:datatype="http://www.w3.org/2001/XMLSchema#integer">1</time:months>
        <time:seconds rdf:datatype="http://www.w3.org/2001/XMLSchema#integer">0</time:seconds>
        <time:weeks rdf:datatype="http://www.w3.org/2001/XMLSchema#integer">0</time:weeks>
        <time:years rdf:datatype="http://www.w3.org/2001/XMLSchema#integer">0</time:years>
        <rdfs:label xml:lang="en">Month (unit of temporal duration)</rdfs:label>
        <skos:prefLabel xml:lang="de">Monat</skos:prefLabel>
        <skos:prefLabel xml:lang="nl">maand</skos:prefLabel>
        <skos:prefLabel xml:lang="es">mes</skos:prefLabel>
        <skos:prefLabel xml:lang="it">mese</skos:prefLabel>
        <skos:prefLabel xml:lang="pl">miesiąc</skos:prefLabel>
        <skos:prefLabel xml:lang="fr">mois</skos:prefLabel>
        <skos:prefLabel xml:lang="en">month</skos:prefLabel>
        <skos:prefLabel xml:lang="ru">один месяц</skos:prefLabel>
        <skos:prefLabel xml:lang="ar">شهر واحد</skos:prefLabel>
        <skos:prefLabel xml:lang="jp">一か月</skos:prefLabel>
        <skos:prefLabel xml:lang="zh">一個月</skos:prefLabel>
        <skos:prefLabel xml:lang="kr">한달</skos:prefLabel>
    </owl:NamedIndividual>
    


    <!-- http://www.w3.org/2006/time#unitSecond -->


    <owl:NamedIndividual rdf:about="http://www.w3.org/2006/time#unitSecond">
        <rdf:type rdf:resource="http://www.w3.org/2006/time#TemporalUnit"/>
        <time:days rdf:datatype="http://www.w3.org/2001/XMLSchema#integer">0</time:days>
        <time:hours rdf:datatype="http://www.w3.org/2001/XMLSchema#integer">0</time:hours>
        <time:minutes rdf:datatype="http://www.w3.org/2001/XMLSchema#integer">0</time:minutes>
        <time:months rdf:datatype="http://www.w3.org/2001/XMLSchema#integer">0</time:months>
        <time:seconds rdf:datatype="http://www.w3.org/2001/XMLSchema#integer">1</time:seconds>
        <time:weeks rdf:datatype="http://www.w3.org/2001/XMLSchema#integer">0</time:weeks>
        <time:years rdf:datatype="http://www.w3.org/2001/XMLSchema#integer">0</time:years>
        <rdfs:label xml:lang="en">Second (unit of temporal duration)</rdfs:label>
        <skos:prefLabel xml:lang="de">Sekunde</skos:prefLabel>
        <skos:prefLabel xml:lang="pl">Sekundę</skos:prefLabel>
        <skos:prefLabel xml:lang="en">second</skos:prefLabel>
        <skos:prefLabel xml:lang="fr">seconde</skos:prefLabel>
        <skos:prefLabel xml:lang="nl">seconde</skos:prefLabel>
        <skos:prefLabel xml:lang="it">secondo</skos:prefLabel>
        <skos:prefLabel xml:lang="es">segundo</skos:prefLabel>
        <skos:prefLabel xml:lang="pt">segundo</skos:prefLabel>
        <skos:prefLabel xml:lang="ar">ثانية واحدة</skos:prefLabel>
        <skos:prefLabel xml:lang="jp">一秒</skos:prefLabel>
        <skos:prefLabel xml:lang="zh">一秒</skos:prefLabel>
        <skos:prefLabel xml:lang="kr">일초</skos:prefLabel>
    </owl:NamedIndividual>
    


    <!-- http://www.w3.org/2006/time#unitWeek -->


    <owl:NamedIndividual rdf:about="http://www.w3.org/2006/time#unitWeek">
        <rdf:type rdf:resource="http://www.w3.org/2006/time#TemporalUnit"/>
        <time:days rdf:datatype="http://www.w3.org/2001/XMLSchema#integer">0</time:days>
        <time:hours rdf:datatype="http://www.w3.org/2001/XMLSchema#integer">0</time:hours>
        <time:minutes rdf:datatype="http://www.w3.org/2001/XMLSchema#integer">0</time:minutes>
        <time:months rdf:datatype="http://www.w3.org/2001/XMLSchema#integer">0</time:months>
        <time:seconds rdf:datatype="http://www.w3.org/2001/XMLSchema#integer">0</time:seconds>
        <time:weeks rdf:datatype="http://www.w3.org/2001/XMLSchema#integer">1</time:weeks>
        <time:years rdf:datatype="http://www.w3.org/2001/XMLSchema#integer">0</time:years>
        <rdfs:label xml:lang="en">Week (unit of temporal duration)</rdfs:label>
        <skos:prefLabel xml:lang="de">Woche</skos:prefLabel>
        <skos:prefLabel xml:lang="fr">semaine</skos:prefLabel>
        <skos:prefLabel xml:lang="es">semana</skos:prefLabel>
        <skos:prefLabel xml:lang="pt">semana</skos:prefLabel>
        <skos:prefLabel xml:lang="it">settimana</skos:prefLabel>
        <skos:prefLabel xml:lang="pl">tydzień</skos:prefLabel>
        <skos:prefLabel xml:lang="en">week</skos:prefLabel>
        <skos:prefLabel xml:lang="nl">week</skos:prefLabel>
        <skos:prefLabel xml:lang="ru">одна неделя</skos:prefLabel>
        <skos:prefLabel xml:lang="ar">سبوع واحد</skos:prefLabel>
        <skos:prefLabel xml:lang="zh">一周</skos:prefLabel>
        <skos:prefLabel xml:lang="jp">一週間</skos:prefLabel>
        <skos:prefLabel xml:lang="kr">일주일</skos:prefLabel>
    </owl:NamedIndividual>
    


    <!-- http://www.w3.org/2006/time#unitYear -->


    <owl:NamedIndividual rdf:about="http://www.w3.org/2006/time#unitYear">
        <rdf:type rdf:resource="http://www.w3.org/2006/time#TemporalUnit"/>
        <time:days rdf:datatype="http://www.w3.org/2001/XMLSchema#integer">0</time:days>
        <time:hours rdf:datatype="http://www.w3.org/2001/XMLSchema#integer">0</time:hours>
        <time:minutes rdf:datatype="http://www.w3.org/2001/XMLSchema#integer">0</time:minutes>
        <time:months rdf:datatype="http://www.w3.org/2001/XMLSchema#integer">0</time:months>
        <time:seconds rdf:datatype="http://www.w3.org/2001/XMLSchema#integer">0</time:seconds>
        <time:weeks rdf:datatype="http://www.w3.org/2001/XMLSchema#integer">0</time:weeks>
        <time:years rdf:datatype="http://www.w3.org/2001/XMLSchema#integer">1</time:years>
        <rdfs:label xml:lang="en">Year (unit of temporal duration)</rdfs:label>
        <skos:prefLabel xml:lang="kr">1 년</skos:prefLabel>
        <skos:prefLabel xml:lang="jp">1年</skos:prefLabel>
        <skos:prefLabel xml:lang="de">Jahr</skos:prefLabel>
        <skos:prefLabel xml:lang="fr">an</skos:prefLabel>
        <skos:prefLabel xml:lang="it">anno</skos:prefLabel>
        <skos:prefLabel xml:lang="pt">ano</skos:prefLabel>
        <skos:prefLabel xml:lang="nl">jaar</skos:prefLabel>
        <skos:prefLabel xml:lang="pl">rok</skos:prefLabel>
        <skos:prefLabel xml:lang="es">un año</skos:prefLabel>
        <skos:prefLabel xml:lang="en">year</skos:prefLabel>
        <skos:prefLabel xml:lang="ru">один год</skos:prefLabel>
        <skos:prefLabel xml:lang="ar">سنة واحدة</skos:prefLabel>
        <skos:prefLabel xml:lang="zh">一年</skos:prefLabel>
    </owl:NamedIndividual>
    


    <!-- https://saref.etsi.org/core/Cleaning -->


    <owl:NamedIndividual rdf:about="https://saref.etsi.org/core/Cleaning">
        <rdf:type rdf:resource="https://saref.etsi.org/core/Task"/>
        <rdfs:comment xml:lang="en">A type of task for which a device is designed</rdfs:comment>
        <rdfs:label xml:lang="en">Cleaning</rdfs:label>
    </owl:NamedIndividual>
    


    <!-- https://saref.etsi.org/core/Comfort -->


    <owl:NamedIndividual rdf:about="https://saref.etsi.org/core/Comfort">
        <rdf:type rdf:resource="https://saref.etsi.org/core/Task"/>
        <rdfs:comment xml:lang="en">A type of task for which a device is designed</rdfs:comment>
        <rdfs:label xml:lang="en">Comfort</rdfs:label>
    </owl:NamedIndividual>
    


    <!-- https://saref.etsi.org/core/Drying -->


    <owl:NamedIndividual rdf:about="https://saref.etsi.org/core/Drying">
        <rdf:type rdf:resource="https://saref.etsi.org/core/Task"/>
        <rdfs:comment xml:lang="en">A type of task for which a device is designed</rdfs:comment>
        <rdfs:label xml:lang="en">Drying</rdfs:label>
    </owl:NamedIndividual>
    


    <!-- https://saref.etsi.org/core/EnergyEfficiency -->


    <owl:NamedIndividual rdf:about="https://saref.etsi.org/core/EnergyEfficiency">
        <rdf:type rdf:resource="https://saref.etsi.org/core/Task"/>
        <rdfs:comment xml:lang="en">A type of task for which a device is designed</rdfs:comment>
        <rdfs:label xml:lang="en">EnergyEfficiency</rdfs:label>
    </owl:NamedIndividual>
    


    <!-- https://saref.etsi.org/core/Entertainment -->


    <owl:NamedIndividual rdf:about="https://saref.etsi.org/core/Entertainment">
        <rdf:type rdf:resource="https://saref.etsi.org/core/Task"/>
        <rdfs:comment xml:lang="en">A type of task for which a device is designed</rdfs:comment>
        <rdfs:label xml:lang="en">Entertainment</rdfs:label>
    </owl:NamedIndividual>
    


    <!-- https://saref.etsi.org/core/Lighting -->


    <owl:NamedIndividual rdf:about="https://saref.etsi.org/core/Lighting">
        <rdf:type rdf:resource="https://saref.etsi.org/core/Task"/>
        <rdfs:comment xml:lang="en">A type of task for which a device is designed</rdfs:comment>
        <rdfs:label xml:lang="en">Lighting</rdfs:label>
    </owl:NamedIndividual>
    


    <!-- https://saref.etsi.org/core/MeterReading -->


    <owl:NamedIndividual rdf:about="https://saref.etsi.org/core/MeterReading">
        <rdf:type rdf:resource="https://saref.etsi.org/core/Task"/>
        <rdfs:comment xml:lang="en">A type of task for which a device is designed</rdfs:comment>
        <rdfs:label xml:lang="en">Meter reading</rdfs:label>
    </owl:NamedIndividual>
    


    <!-- https://saref.etsi.org/core/Safety -->


    <owl:NamedIndividual rdf:about="https://saref.etsi.org/core/Safety">
        <rdf:type rdf:resource="https://saref.etsi.org/core/Task"/>
        <rdfs:comment xml:lang="en">A type of task for which a device is designed</rdfs:comment>
        <rdfs:label xml:lang="en">Safety</rdfs:label>
    </owl:NamedIndividual>
    


    <!-- https://saref.etsi.org/core/Washing -->


    <owl:NamedIndividual rdf:about="https://saref.etsi.org/core/Washing">
        <rdf:type rdf:resource="https://saref.etsi.org/core/Task"/>
        <rdfs:comment xml:lang="en">A type of task for which a device is designed</rdfs:comment>
        <rdfs:label xml:lang="en">Washing</rdfs:label>
    </owl:NamedIndividual>
    


    <!-- https://saref.etsi.org/core/WellBeing -->


    <owl:NamedIndividual rdf:about="https://saref.etsi.org/core/WellBeing">
        <rdf:type rdf:resource="https://saref.etsi.org/core/Task"/>
        <rdfs:comment xml:lang="en">A type of task for which a device is designed</rdfs:comment>
        <rdfs:label xml:lang="en">WellBeing</rdfs:label>
    </owl:NamedIndividual>
    


    <!-- https://saref.etsi.org/saref4agri/AirTemperature -->


    <owl:NamedIndividual rdf:about="https://saref.etsi.org/saref4agri/AirTemperature">
        <rdf:type rdf:resource="https://saref.etsi.org/core/Temperature"/>
        <rdfs:comment xml:lang="en">The degree or intensity of heat present in the air.</rdfs:comment>
        <rdfs:label xml:lang="en">Air temperature</rdfs:label>
    </owl:NamedIndividual>
    


    <!-- https://saref.etsi.org/saref4agri/AmbientHumidity -->


    <owl:NamedIndividual rdf:about="https://saref.etsi.org/saref4agri/AmbientHumidity">
        <rdf:type rdf:resource="https://saref.etsi.org/core/Humidity"/>
        <rdfs:comment xml:lang="en">The amount of water vapour in the air.</rdfs:comment>
        <rdfs:label xml:lang="en">Ambient humidity</rdfs:label>
    </owl:NamedIndividual>
    


    <!-- https://saref.etsi.org/saref4agri/IrrigationWater -->


    <owl:NamedIndividual rdf:about="https://saref.etsi.org/saref4agri/IrrigationWater">
        <rdf:type rdf:resource="https://saref.etsi.org/core/Property"/>
        <rdfs:comment xml:lang="en">The amount of water falling in the soil by irrigation methods.</rdfs:comment>
        <rdfs:label xml:lang="en">Irrigation water</rdfs:label>
    </owl:NamedIndividual>
    


    <!-- https://saref.etsi.org/saref4agri/PlantGrowthStage -->


    <owl:NamedIndividual rdf:about="https://saref.etsi.org/saref4agri/PlantGrowthStage">
        <rdf:type rdf:resource="https://saref.etsi.org/core/Property"/>
        <rdfs:comment xml:lang="en">The level or stage of growth of the plant.</rdfs:comment>
        <rdfs:label xml:lang="en">Plant growth stage</rdfs:label>
    </owl:NamedIndividual>
    


    <!-- https://saref.etsi.org/saref4agri/Precipitation -->


    <owl:NamedIndividual rdf:about="https://saref.etsi.org/saref4agri/Precipitation">
        <rdf:type rdf:resource="https://saref.etsi.org/core/Property"/>
        <rdfs:comment xml:lang="en">The amount of water falling in the soil by natural process (e.g. rain).</rdfs:comment>
        <rdfs:label xml:lang="en">Precipitation</rdfs:label>
    </owl:NamedIndividual>
    


    <!-- https://saref.etsi.org/saref4agri/SoilMoisture -->


    <owl:NamedIndividual rdf:about="https://saref.etsi.org/saref4agri/SoilMoisture">
        <rdf:type rdf:resource="https://saref.etsi.org/core/Property"/>
        <rdfs:comment xml:lang="en">The amount of water or humidity contained in the soil.</rdfs:comment>
        <rdfs:label xml:lang="en">Soil moisture</rdfs:label>
    </owl:NamedIndividual>
    


    <!-- https://saref.etsi.org/saref4agri/SoilTemperature -->


    <owl:NamedIndividual rdf:about="https://saref.etsi.org/saref4agri/SoilTemperature">
        <rdf:type rdf:resource="https://saref.etsi.org/core/Temperature"/>
        <rdfs:comment xml:lang="en">The degree or intensity of heat present in the soil.</rdfs:comment>
        <rdfs:label xml:lang="en">Soil temperature</rdfs:label>
    </owl:NamedIndividual>
    


    <!-- https://saref.etsi.org/saref4watr/Acrylamide -->


    <owl:NamedIndividual rdf:about="https://saref.etsi.org/saref4watr/Acrylamide">
        <rdf:type rdf:resource="https://saref.etsi.org/saref4watr/ChemicalProperty"/>
        <rdfs:comment xml:lang="en">Property of the water indicating its concentration of acrylamide.</rdfs:comment>
        <rdfs:label xml:lang="en">Acrylamide</rdfs:label>
    </owl:NamedIndividual>
    


    <!-- https://saref.etsi.org/saref4watr/Agriculture -->


    <owl:NamedIndividual rdf:about="https://saref.etsi.org/saref4watr/Agriculture">
        <rdf:type rdf:resource="https://saref.etsi.org/saref4watr/WaterUse"/>
        <rdfs:comment xml:lang="en">Use of water for the farming of plants and livestock.</rdfs:comment>
        <rdfs:label xml:lang="en">Agriculture</rdfs:label>
    </owl:NamedIndividual>
    


    <!-- https://saref.etsi.org/saref4watr/Aluminium -->


    <owl:NamedIndividual rdf:about="https://saref.etsi.org/saref4watr/Aluminium">
        <rdf:type rdf:resource="https://saref.etsi.org/saref4watr/ChemicalProperty"/>
        <rdfs:comment xml:lang="en">Property of the water indicating its concentration of aluminium.</rdfs:comment>
        <rdfs:label xml:lang="en">Aluminium</rdfs:label>
    </owl:NamedIndividual>
    


    <!-- https://saref.etsi.org/saref4watr/Ammonium -->


    <owl:NamedIndividual rdf:about="https://saref.etsi.org/saref4watr/Ammonium">
        <rdf:type rdf:resource="https://saref.etsi.org/saref4watr/ChemicalProperty"/>
        <rdfs:comment xml:lang="en">Property of the water indicating its concentration of ammonium.</rdfs:comment>
        <rdfs:label xml:lang="en">Ammonium</rdfs:label>
    </owl:NamedIndividual>
    


    <!-- https://saref.etsi.org/saref4watr/Antimony -->


    <owl:NamedIndividual rdf:about="https://saref.etsi.org/saref4watr/Antimony">
        <rdf:type rdf:resource="https://saref.etsi.org/saref4watr/ChemicalProperty"/>
        <rdfs:comment xml:lang="en">Property of the water indicating its concentration of antimony.</rdfs:comment>
        <rdfs:label xml:lang="en">Antimony</rdfs:label>
    </owl:NamedIndividual>
    


    <!-- https://saref.etsi.org/saref4watr/Aquaculture -->


    <owl:NamedIndividual rdf:about="https://saref.etsi.org/saref4watr/Aquaculture">
        <rdf:type rdf:resource="https://saref.etsi.org/saref4watr/WaterUse"/>
        <rdfs:comment xml:lang="en">Use of water for the farming of fish, crustaceans, molluscs, aquatic plants, algae, and other organisms.</rdfs:comment>
        <rdfs:label xml:lang="en">Aquaculture</rdfs:label>
    </owl:NamedIndividual>
    


    <!-- https://saref.etsi.org/saref4watr/Arsenic -->


    <owl:NamedIndividual rdf:about="https://saref.etsi.org/saref4watr/Arsenic">
        <rdf:type rdf:resource="https://saref.etsi.org/saref4watr/ChemicalProperty"/>
        <rdfs:comment xml:lang="en">Property of the water indicating its concentration of arsenic.</rdfs:comment>
        <rdfs:label xml:lang="en">Arsenic</rdfs:label>
    </owl:NamedIndividual>
    


    <!-- https://saref.etsi.org/saref4watr/AtmosphericPressure -->


    <owl:NamedIndividual rdf:about="https://saref.etsi.org/saref4watr/AtmosphericPressure">
        <rdf:type rdf:resource="https://saref.etsi.org/saref4watr/EnvironmentalProperty"/>
        <rdfs:comment xml:lang="en">Property of the environment indicating the atmospheric pressure.</rdfs:comment>
        <rdfs:label xml:lang="en">Atmospheric pressure</rdfs:label>
    </owl:NamedIndividual>
    


    <!-- https://saref.etsi.org/saref4watr/BatteryLastChange -->


    <owl:NamedIndividual rdf:about="https://saref.etsi.org/saref4watr/BatteryLastChange">
        <rdf:type rdf:resource="https://saref.etsi.org/saref4watr/WaterMeterProperty"/>
        <rdfs:comment xml:lang="en">The time in which the battery was last changed.</rdfs:comment>
        <rdfs:label xml:lang="en">Battery last change</rdfs:label>
    </owl:NamedIndividual>
    


    <!-- https://saref.etsi.org/saref4watr/BatteryOperatingTime -->


    <owl:NamedIndividual rdf:about="https://saref.etsi.org/saref4watr/BatteryOperatingTime">
        <rdf:type rdf:resource="https://saref.etsi.org/saref4watr/WaterMeterProperty"/>
        <rdfs:comment xml:lang="en">The time for which the battery has been operating since the last charge.</rdfs:comment>
        <rdfs:label xml:lang="en">Battery operating time</rdfs:label>
    </owl:NamedIndividual>
    


    <!-- https://saref.etsi.org/saref4watr/BatteryRemainingTime -->


    <owl:NamedIndividual rdf:about="https://saref.etsi.org/saref4watr/BatteryRemainingTime">
        <rdf:type rdf:resource="https://saref.etsi.org/saref4watr/WaterMeterProperty"/>
        <rdfs:comment xml:lang="en">The time until the battery is discharged.</rdfs:comment>
        <rdfs:label xml:lang="en">Battery remaining time</rdfs:label>
    </owl:NamedIndividual>
    


    <!-- https://saref.etsi.org/saref4watr/Benzene -->


    <owl:NamedIndividual rdf:about="https://saref.etsi.org/saref4watr/Benzene">
        <rdf:type rdf:resource="https://saref.etsi.org/saref4watr/ChemicalProperty"/>
        <rdfs:comment xml:lang="en">Property of the water indicating its concentration of benzene.</rdfs:comment>
        <rdfs:label xml:lang="en">Benzene</rdfs:label>
    </owl:NamedIndividual>
    


    <!-- https://saref.etsi.org/saref4watr/Benzoapyrene -->


    <owl:NamedIndividual rdf:about="https://saref.etsi.org/saref4watr/Benzoapyrene">
        <rdf:type rdf:resource="https://saref.etsi.org/saref4watr/ChemicalProperty"/>
        <rdfs:comment xml:lang="en">Property of the water indicating its concentration of benzo(a)pyrene.</rdfs:comment>
        <rdfs:label xml:lang="en">Benzo(a)pyrene</rdfs:label>
    </owl:NamedIndividual>
    


    <!-- https://saref.etsi.org/saref4watr/Boron -->


    <owl:NamedIndividual rdf:about="https://saref.etsi.org/saref4watr/Boron">
        <rdf:type rdf:resource="https://saref.etsi.org/saref4watr/ChemicalProperty"/>
        <rdfs:comment xml:lang="en">Property of the water indicating its concentration of boron.</rdfs:comment>
        <rdfs:label xml:lang="en">Boron</rdfs:label>
    </owl:NamedIndividual>
    


    <!-- https://saref.etsi.org/saref4watr/Bromate -->


    <owl:NamedIndividual rdf:about="https://saref.etsi.org/saref4watr/Bromate">
        <rdf:type rdf:resource="https://saref.etsi.org/saref4watr/ChemicalProperty"/>
        <rdfs:comment xml:lang="en">Property of the water indicating its concentration of bromate.</rdfs:comment>
        <rdfs:label xml:lang="en">Bromate</rdfs:label>
    </owl:NamedIndividual>
    


    <!-- https://saref.etsi.org/saref4watr/Cadmium -->


    <owl:NamedIndividual rdf:about="https://saref.etsi.org/saref4watr/Cadmium">
        <rdf:type rdf:resource="https://saref.etsi.org/saref4watr/ChemicalProperty"/>
        <rdfs:comment xml:lang="en">Property of the water indicating its concentration of cadmium.</rdfs:comment>
        <rdfs:label xml:lang="en">Cadmium</rdfs:label>
    </owl:NamedIndividual>
    


    <!-- https://saref.etsi.org/saref4watr/Chloride -->


    <owl:NamedIndividual rdf:about="https://saref.etsi.org/saref4watr/Chloride">
        <rdf:type rdf:resource="https://saref.etsi.org/saref4watr/ChemicalProperty"/>
        <rdfs:comment xml:lang="en">Property of the water indicating its concentration of chloride.</rdfs:comment>
        <rdfs:label xml:lang="en">Chloride</rdfs:label>
    </owl:NamedIndividual>
    


    <!-- https://saref.etsi.org/saref4watr/Chromium -->


    <owl:NamedIndividual rdf:about="https://saref.etsi.org/saref4watr/Chromium">
        <rdf:type rdf:resource="https://saref.etsi.org/saref4watr/ChemicalProperty"/>
        <rdfs:comment xml:lang="en">Property of the water indicating its concentration of chromium.</rdfs:comment>
        <rdfs:label xml:lang="en">Chromium</rdfs:label>
    </owl:NamedIndividual>
    


    <!-- https://saref.etsi.org/saref4watr/ClostridiumPerfringens -->


    <owl:NamedIndividual rdf:about="https://saref.etsi.org/saref4watr/ClostridiumPerfringens">
        <rdf:type rdf:resource="https://saref.etsi.org/saref4watr/BacterialProperty"/>
        <rdfs:comment xml:lang="en">Property of the water indicating its concentration of clostridium perfringens.</rdfs:comment>
        <rdfs:label xml:lang="en">Clostridium perfringens</rdfs:label>
    </owl:NamedIndividual>
    


    <!-- https://saref.etsi.org/saref4watr/ColiformBacteria -->


    <owl:NamedIndividual rdf:about="https://saref.etsi.org/saref4watr/ColiformBacteria">
        <rdf:type rdf:resource="https://saref.etsi.org/saref4watr/BacterialProperty"/>
        <rdfs:comment xml:lang="en">Property of the water indicating its concentration of coliform bacteria.</rdfs:comment>
        <rdfs:label xml:lang="en">Coliform bacteria</rdfs:label>
    </owl:NamedIndividual>
    


    <!-- https://saref.etsi.org/saref4watr/ColonyCount22C -->


    <owl:NamedIndividual rdf:about="https://saref.etsi.org/saref4watr/ColonyCount22C">
        <rdf:type rdf:resource="https://saref.etsi.org/saref4watr/BacterialProperty"/>
        <rdfs:comment xml:lang="en">Property of the water indicating its colony count at 22 ºC.</rdfs:comment>
        <rdfs:label xml:lang="en">Colony count at 22 °C</rdfs:label>
    </owl:NamedIndividual>
    


    <!-- https://saref.etsi.org/saref4watr/ColonyCount37C -->


    <owl:NamedIndividual rdf:about="https://saref.etsi.org/saref4watr/ColonyCount37C">
        <rdf:type rdf:resource="https://saref.etsi.org/saref4watr/BacterialProperty"/>
        <rdfs:comment xml:lang="en">Property of the water indicating its colony count at 37 ºC.</rdfs:comment>
        <rdfs:label xml:lang="en">Colony count at 37 °C</rdfs:label>
    </owl:NamedIndividual>
    


    <!-- https://saref.etsi.org/saref4watr/Colour -->


    <owl:NamedIndividual rdf:about="https://saref.etsi.org/saref4watr/Colour">
        <rdf:type rdf:resource="https://saref.etsi.org/saref4watr/AcceptabilityProperty"/>
        <rdfs:comment xml:lang="en">Property of the water indicating its colour.</rdfs:comment>
        <rdfs:label xml:lang="en">Colour</rdfs:label>
    </owl:NamedIndividual>
    


    <!-- https://saref.etsi.org/saref4watr/Conductivity -->


    <owl:NamedIndividual rdf:about="https://saref.etsi.org/saref4watr/Conductivity">
        <rdf:type rdf:resource="https://saref.etsi.org/saref4watr/AcceptabilityProperty"/>
        <rdfs:comment xml:lang="en">Property of the water indicating its conductivity.</rdfs:comment>
        <rdfs:label xml:lang="en">Conductivity</rdfs:label>
    </owl:NamedIndividual>
    


    <!-- https://saref.etsi.org/saref4watr/Copper -->


    <owl:NamedIndividual rdf:about="https://saref.etsi.org/saref4watr/Copper">
        <rdf:type rdf:resource="https://saref.etsi.org/saref4watr/ChemicalProperty"/>
        <rdfs:comment xml:lang="en">Property of the water indicating its concentration of copper.</rdfs:comment>
        <rdfs:label xml:lang="en">Copper</rdfs:label>
    </owl:NamedIndividual>
    


    <!-- https://saref.etsi.org/saref4watr/Cyanide -->


    <owl:NamedIndividual rdf:about="https://saref.etsi.org/saref4watr/Cyanide">
        <rdf:type rdf:resource="https://saref.etsi.org/saref4watr/ChemicalProperty"/>
        <rdfs:comment xml:lang="en">Property of the water indicating its concentration of cyanide.</rdfs:comment>
        <rdfs:label xml:lang="en">Cyanide</rdfs:label>
    </owl:NamedIndividual>
    


    <!-- https://saref.etsi.org/saref4watr/Domestic -->


    <owl:NamedIndividual rdf:about="https://saref.etsi.org/saref4watr/Domestic">
        <rdf:type rdf:resource="https://saref.etsi.org/saref4watr/WaterUse"/>
        <rdfs:comment xml:lang="en">Use of water for domestic purposes.</rdfs:comment>
        <rdfs:label xml:lang="en">Domestic</rdfs:label>
    </owl:NamedIndividual>
    


    <!-- https://saref.etsi.org/saref4watr/DrinkingWater -->


    <owl:NamedIndividual rdf:about="https://saref.etsi.org/saref4watr/DrinkingWater">
        <rdf:type rdf:resource="https://saref.etsi.org/saref4watr/Water"/>
        <rdfs:comment xml:lang="en">Drinking water is water that is treated to comply with drinking water standards.</rdfs:comment>
        <rdfs:label xml:lang="en">Drinking water</rdfs:label>
        <rdfs:label xml:lang="en">Potable water</rdfs:label>
    </owl:NamedIndividual>
    


    <!-- https://saref.etsi.org/saref4watr/Enterococci -->


    <owl:NamedIndividual rdf:about="https://saref.etsi.org/saref4watr/Enterococci">
        <rdf:type rdf:resource="https://saref.etsi.org/saref4watr/BacterialProperty"/>
        <rdfs:comment xml:lang="en">Property of the water indicating its concentration of enterococci.</rdfs:comment>
        <rdfs:label xml:lang="en">Enterococci</rdfs:label>
    </owl:NamedIndividual>
    


    <!-- https://saref.etsi.org/saref4watr/Epichlorohydrin -->


    <owl:NamedIndividual rdf:about="https://saref.etsi.org/saref4watr/Epichlorohydrin">
        <rdf:type rdf:resource="https://saref.etsi.org/saref4watr/ChemicalProperty"/>
        <rdfs:comment xml:lang="en">Property of the water indicating its concentration of epichlorohydrin.</rdfs:comment>
        <rdfs:label xml:lang="en">Epichlorohydrin</rdfs:label>
    </owl:NamedIndividual>
    


    <!-- https://saref.etsi.org/saref4watr/EscherichiaColi -->


    <owl:NamedIndividual rdf:about="https://saref.etsi.org/saref4watr/EscherichiaColi">
        <rdf:type rdf:resource="https://saref.etsi.org/saref4watr/BacterialProperty"/>
        <rdfs:comment xml:lang="en">Property of the water indicating its concentration of escherichia coli.</rdfs:comment>
        <rdfs:label xml:lang="en">E. coli</rdfs:label>
        <rdfs:label xml:lang="en">Escherichia coli</rdfs:label>
    </owl:NamedIndividual>
    


    <!-- https://saref.etsi.org/saref4watr/ExternalTemperature -->


    <owl:NamedIndividual rdf:about="https://saref.etsi.org/saref4watr/ExternalTemperature">
        <rdf:type rdf:resource="https://saref.etsi.org/saref4watr/EnvironmentalProperty"/>
        <rdfs:comment xml:lang="en">Property of the environment indicating the temperature.</rdfs:comment>
        <rdfs:label xml:lang="en">External temperature</rdfs:label>
    </owl:NamedIndividual>
    


    <!-- https://saref.etsi.org/saref4watr/FlowPressure -->


    <owl:NamedIndividual rdf:about="https://saref.etsi.org/saref4watr/FlowPressure">
        <rdf:type rdf:resource="https://saref.etsi.org/saref4watr/WaterFlowProperty"/>
        <rdfs:comment xml:lang="en">Property indicating the pressure of a water flow.</rdfs:comment>
        <rdfs:label xml:lang="en">Flow pressure</rdfs:label>
    </owl:NamedIndividual>
    


    <!-- https://saref.etsi.org/saref4watr/FlowRate -->


    <owl:NamedIndividual rdf:about="https://saref.etsi.org/saref4watr/FlowRate">
        <rdf:type rdf:resource="https://saref.etsi.org/saref4watr/WaterFlowProperty"/>
        <rdfs:comment xml:lang="en">Property indicating the rate of a water flow.</rdfs:comment>
        <rdfs:label xml:lang="en">Flow rate</rdfs:label>
    </owl:NamedIndividual>
    


    <!-- https://saref.etsi.org/saref4watr/FlowTemperature -->


    <owl:NamedIndividual rdf:about="https://saref.etsi.org/saref4watr/FlowTemperature">
        <rdf:type rdf:resource="https://saref.etsi.org/saref4watr/WaterFlowProperty"/>
        <rdfs:comment xml:lang="en">Property indicating the temperature of a water flow.</rdfs:comment>
        <rdfs:label xml:lang="en">Flow temperature</rdfs:label>
    </owl:NamedIndividual>
    


    <!-- https://saref.etsi.org/saref4watr/FlowVolume -->


    <owl:NamedIndividual rdf:about="https://saref.etsi.org/saref4watr/FlowVolume">
        <rdf:type rdf:resource="https://saref.etsi.org/saref4watr/WaterFlowProperty"/>
        <rdfs:comment xml:lang="en">Property indicating the volume of a water flow.</rdfs:comment>
        <rdfs:label xml:lang="en">Flow volume</rdfs:label>
    </owl:NamedIndividual>
    


    <!-- https://saref.etsi.org/saref4watr/Fluoride -->


    <owl:NamedIndividual rdf:about="https://saref.etsi.org/saref4watr/Fluoride">
        <rdf:type rdf:resource="https://saref.etsi.org/saref4watr/ChemicalProperty"/>
        <rdfs:comment xml:lang="en">Property of the water indicating its concentration of fluoride.</rdfs:comment>
        <rdfs:label xml:lang="en">Fluoride</rdfs:label>
    </owl:NamedIndividual>
    


    <!-- https://saref.etsi.org/saref4watr/Hardness -->


    <owl:NamedIndividual rdf:about="https://saref.etsi.org/saref4watr/Hardness">
        <rdf:type rdf:resource="https://saref.etsi.org/saref4watr/AcceptabilityProperty"/>
        <rdfs:comment xml:lang="en">Property of the water indicating its hardness.</rdfs:comment>
        <rdfs:label xml:lang="en">Hardness</rdfs:label>
    </owl:NamedIndividual>
    


    <!-- https://saref.etsi.org/saref4watr/Humidity -->


    <owl:NamedIndividual rdf:about="https://saref.etsi.org/saref4watr/Humidity">
        <rdf:type rdf:resource="https://saref.etsi.org/saref4watr/EnvironmentalProperty"/>
        <rdfs:comment xml:lang="en">Property of the environment indicating the humidity.</rdfs:comment>
        <rdfs:label xml:lang="en">Humidity</rdfs:label>
    </owl:NamedIndividual>
    


    <!-- https://saref.etsi.org/saref4watr/HydrogenIonConcentration -->


    <owl:NamedIndividual rdf:about="https://saref.etsi.org/saref4watr/HydrogenIonConcentration">
        <rdf:type rdf:resource="https://saref.etsi.org/saref4watr/AcceptabilityProperty"/>
        <rdfs:comment xml:lang="en">Property of the water indicating its hydrogen ion concentration.</rdfs:comment>
        <rdfs:label xml:lang="en">Hydrogen ion concentration</rdfs:label>
        <rdfs:label xml:lang="en">pH</rdfs:label>
    </owl:NamedIndividual>
    


    <!-- https://saref.etsi.org/saref4watr/Industry -->


    <owl:NamedIndividual rdf:about="https://saref.etsi.org/saref4watr/Industry">
        <rdf:type rdf:resource="https://saref.etsi.org/saref4watr/WaterUse"/>
        <rdfs:comment xml:lang="en">Use of water for industrial purposes.</rdfs:comment>
        <rdfs:label xml:lang="en">Industry</rdfs:label>
    </owl:NamedIndividual>
    


    <!-- https://saref.etsi.org/saref4watr/Iron -->


    <owl:NamedIndividual rdf:about="https://saref.etsi.org/saref4watr/Iron">
        <rdf:type rdf:resource="https://saref.etsi.org/saref4watr/ChemicalProperty"/>
        <rdfs:comment xml:lang="en">Property of the water indicating its concentration of iron.</rdfs:comment>
        <rdfs:label xml:lang="en">Iron</rdfs:label>
    </owl:NamedIndividual>
    


    <!-- https://saref.etsi.org/saref4watr/Lead -->


    <owl:NamedIndividual rdf:about="https://saref.etsi.org/saref4watr/Lead">
        <rdf:type rdf:resource="https://saref.etsi.org/saref4watr/ChemicalProperty"/>
        <rdfs:comment xml:lang="en">Property of the water indicating its concentration of lead.</rdfs:comment>
        <rdfs:label xml:lang="en">Lead</rdfs:label>
    </owl:NamedIndividual>
    


    <!-- https://saref.etsi.org/saref4watr/Manganese -->


    <owl:NamedIndividual rdf:about="https://saref.etsi.org/saref4watr/Manganese">
        <rdf:type rdf:resource="https://saref.etsi.org/saref4watr/ChemicalProperty"/>
        <rdfs:comment xml:lang="en">Property of the water indicating its concentration of manganese.</rdfs:comment>
        <rdfs:label xml:lang="en">Manganese</rdfs:label>
    </owl:NamedIndividual>
    


    <!-- https://saref.etsi.org/saref4watr/Mercury -->


    <owl:NamedIndividual rdf:about="https://saref.etsi.org/saref4watr/Mercury">
        <rdf:type rdf:resource="https://saref.etsi.org/saref4watr/ChemicalProperty"/>
        <rdfs:comment xml:lang="en">Property of the water indicating its concentration of mercury.</rdfs:comment>
        <rdfs:label xml:lang="en">Mercury</rdfs:label>
    </owl:NamedIndividual>
    


    <!-- https://saref.etsi.org/saref4watr/MeterOnTime -->


    <owl:NamedIndividual rdf:about="https://saref.etsi.org/saref4watr/MeterOnTime">
        <rdf:type rdf:resource="https://saref.etsi.org/saref4watr/WaterMeterProperty"/>
        <rdfs:comment xml:lang="en">The duration of the meter power up.</rdfs:comment>
        <rdfs:label xml:lang="en">Meter on time</rdfs:label>
    </owl:NamedIndividual>
    


    <!-- https://saref.etsi.org/saref4watr/MeterOperatingTime -->


    <owl:NamedIndividual rdf:about="https://saref.etsi.org/saref4watr/MeterOperatingTime">
        <rdf:type rdf:resource="https://saref.etsi.org/saref4watr/WaterMeterProperty"/>
        <rdfs:comment xml:lang="en">The time for which the meter has been operating.</rdfs:comment>
        <rdfs:label xml:lang="en">Meter operating time</rdfs:label>
    </owl:NamedIndividual>
    


    <!-- https://saref.etsi.org/saref4watr/Nickel -->


    <owl:NamedIndividual rdf:about="https://saref.etsi.org/saref4watr/Nickel">
        <rdf:type rdf:resource="https://saref.etsi.org/saref4watr/ChemicalProperty"/>
        <rdfs:comment xml:lang="en">Property of the water indicating its concentration of nickel.</rdfs:comment>
        <rdfs:label xml:lang="en">Nickel</rdfs:label>
    </owl:NamedIndividual>
    


    <!-- https://saref.etsi.org/saref4watr/Nitrate -->


    <owl:NamedIndividual rdf:about="https://saref.etsi.org/saref4watr/Nitrate">
        <rdf:type rdf:resource="https://saref.etsi.org/saref4watr/ChemicalProperty"/>
        <rdfs:comment xml:lang="en">Property of the water indicating its concentration of nitrate.</rdfs:comment>
        <rdfs:label xml:lang="en">Nitrate</rdfs:label>
    </owl:NamedIndividual>
    


    <!-- https://saref.etsi.org/saref4watr/Nitrite -->


    <owl:NamedIndividual rdf:about="https://saref.etsi.org/saref4watr/Nitrite">
        <rdf:type rdf:resource="https://saref.etsi.org/saref4watr/ChemicalProperty"/>
        <rdfs:comment xml:lang="en">Property of the water indicating its concentration of nitrite.</rdfs:comment>
        <rdfs:label xml:lang="en">Nitrite</rdfs:label>
    </owl:NamedIndividual>
    


    <!-- https://saref.etsi.org/saref4watr/Odour -->


    <owl:NamedIndividual rdf:about="https://saref.etsi.org/saref4watr/Odour">
        <rdf:type rdf:resource="https://saref.etsi.org/saref4watr/AcceptabilityProperty"/>
        <rdfs:comment xml:lang="en">Property of the water indicating its odour.</rdfs:comment>
        <rdfs:label xml:lang="en">Odour</rdfs:label>
    </owl:NamedIndividual>
    


    <!-- https://saref.etsi.org/saref4watr/Oxidisability -->


    <owl:NamedIndividual rdf:about="https://saref.etsi.org/saref4watr/Oxidisability">
        <rdf:type rdf:resource="https://saref.etsi.org/saref4watr/AcceptabilityProperty"/>
        <rdfs:comment xml:lang="en">Property of the water indicating its oxidisability.</rdfs:comment>
        <rdfs:label xml:lang="en">Oxidisability</rdfs:label>
    </owl:NamedIndividual>
    


    <!-- https://saref.etsi.org/saref4watr/Oxygen -->


    <owl:NamedIndividual rdf:about="https://saref.etsi.org/saref4watr/Oxygen">
        <rdf:type rdf:resource="https://saref.etsi.org/saref4watr/ChemicalProperty"/>
        <rdfs:comment xml:lang="en">Property of the water indicating its oxygen saturation.</rdfs:comment>
        <rdfs:label xml:lang="en">Dissolved oxygen</rdfs:label>
        <rdfs:label xml:lang="en">Oxygen</rdfs:label>
        <rdfs:label xml:lang="en">Oxygen saturation</rdfs:label>
    </owl:NamedIndividual>
    


    <!-- https://saref.etsi.org/saref4watr/PolycyclicAromaticHydrocarbons -->


    <owl:NamedIndividual rdf:about="https://saref.etsi.org/saref4watr/PolycyclicAromaticHydrocarbons">
        <rdf:type rdf:resource="https://saref.etsi.org/saref4watr/ChemicalProperty"/>
        <rdfs:comment xml:lang="en">Property of the water indicating its concentration of polycyclic aromatic hydrocarbons.</rdfs:comment>
        <rdfs:label xml:lang="en">Polycyclic aromatic hydrocarbons</rdfs:label>
    </owl:NamedIndividual>
    


    <!-- https://saref.etsi.org/saref4watr/Precipitation -->


    <owl:NamedIndividual rdf:about="https://saref.etsi.org/saref4watr/Precipitation">
        <rdf:type rdf:resource="https://saref.etsi.org/saref4watr/EnvironmentalProperty"/>
        <rdfs:comment xml:lang="en">Property of the environment indicating the precipitation.</rdfs:comment>
        <rdfs:label xml:lang="en">Precipitation</rdfs:label>
    </owl:NamedIndividual>
    


    <!-- https://saref.etsi.org/saref4watr/PseudomonasAeruginosa -->


    <owl:NamedIndividual rdf:about="https://saref.etsi.org/saref4watr/PseudomonasAeruginosa">
        <rdf:type rdf:resource="https://saref.etsi.org/saref4watr/BacterialProperty"/>
        <rdfs:comment xml:lang="en">Property of the water indicating its concentration of pseudomonas aeruginosa.</rdfs:comment>
        <rdfs:label xml:lang="en">Pseudomonas aeruginosa</rdfs:label>
    </owl:NamedIndividual>
    


    <!-- https://saref.etsi.org/saref4watr/RawWater -->


    <owl:NamedIndividual rdf:about="https://saref.etsi.org/saref4watr/RawWater">
        <rdf:type rdf:resource="https://saref.etsi.org/saref4watr/Water"/>
        <rdfs:comment xml:lang="en">Raw water is water found in the environment that has not been treated and does not have any of its minerals, ions, particles, bacteria, or parasites removed.</rdfs:comment>
        <rdfs:label xml:lang="en">Raw water</rdfs:label>
    </owl:NamedIndividual>
    


    <!-- https://saref.etsi.org/saref4watr/Recreation -->


    <owl:NamedIndividual rdf:about="https://saref.etsi.org/saref4watr/Recreation">
        <rdf:type rdf:resource="https://saref.etsi.org/saref4watr/WaterUse"/>
        <rdfs:comment xml:lang="en">Use of water for recreational purposes.</rdfs:comment>
        <rdfs:label xml:lang="en">Recreation</rdfs:label>
    </owl:NamedIndividual>
    


    <!-- https://saref.etsi.org/saref4watr/Selenium -->


    <owl:NamedIndividual rdf:about="https://saref.etsi.org/saref4watr/Selenium">
        <rdf:type rdf:resource="https://saref.etsi.org/saref4watr/ChemicalProperty"/>
        <rdfs:comment xml:lang="en">Property of the water indicating its concentration of selenium.</rdfs:comment>
        <rdfs:label xml:lang="en">Selenium</rdfs:label>
    </owl:NamedIndividual>
    


    <!-- https://saref.etsi.org/saref4watr/Sodium -->


    <owl:NamedIndividual rdf:about="https://saref.etsi.org/saref4watr/Sodium">
        <rdf:type rdf:resource="https://saref.etsi.org/saref4watr/ChemicalProperty"/>
        <rdfs:comment xml:lang="en">Property of the water indicating its concentration of sodium.</rdfs:comment>
        <rdfs:label xml:lang="en">Sodium</rdfs:label>
    </owl:NamedIndividual>
    


    <!-- https://saref.etsi.org/saref4watr/Stormwater -->


    <owl:NamedIndividual rdf:about="https://saref.etsi.org/saref4watr/Stormwater">
        <rdf:type rdf:resource="https://saref.etsi.org/saref4watr/Water"/>
        <rdfs:comment xml:lang="en">Stormwater is water that originates during precipitation events and snow/ice melt.</rdfs:comment>
        <rdfs:label xml:lang="en">Storm water</rdfs:label>
    </owl:NamedIndividual>
    


    <!-- https://saref.etsi.org/saref4watr/Sulphate -->


    <owl:NamedIndividual rdf:about="https://saref.etsi.org/saref4watr/Sulphate">
        <rdf:type rdf:resource="https://saref.etsi.org/saref4watr/ChemicalProperty"/>
        <rdfs:comment xml:lang="en">Property of the water indicating its concentration of sulphate.</rdfs:comment>
        <rdfs:label xml:lang="en">Sulphate</rdfs:label>
    </owl:NamedIndividual>
    


    <!-- https://saref.etsi.org/saref4watr/Taste -->


    <owl:NamedIndividual rdf:about="https://saref.etsi.org/saref4watr/Taste">
        <rdf:type rdf:resource="https://saref.etsi.org/saref4watr/AcceptabilityProperty"/>
        <rdfs:comment xml:lang="en">Property of the water indicating its taste.</rdfs:comment>
        <rdfs:label xml:lang="en">Taste</rdfs:label>
    </owl:NamedIndividual>
    


    <!-- https://saref.etsi.org/saref4watr/Temperature -->


    <owl:NamedIndividual rdf:about="https://saref.etsi.org/saref4watr/Temperature">
        <rdf:type rdf:resource="https://saref.etsi.org/saref4watr/AcceptabilityProperty"/>
        <rdfs:comment xml:lang="en">Property of the water indicating its temperature.</rdfs:comment>
        <rdfs:label xml:lang="en">Temperature</rdfs:label>
    </owl:NamedIndividual>
    


    <!-- https://saref.etsi.org/saref4watr/Tetrachloroethene -->


    <owl:NamedIndividual rdf:about="https://saref.etsi.org/saref4watr/Tetrachloroethene">
        <rdf:type rdf:resource="https://saref.etsi.org/saref4watr/ChemicalProperty"/>
        <rdfs:comment xml:lang="en">Property of the water indicating its concentration of tetrachloroethene.</rdfs:comment>
        <rdfs:label xml:lang="en">Tetrachloroethene</rdfs:label>
    </owl:NamedIndividual>
    


    <!-- https://saref.etsi.org/saref4watr/TotalDissolvedSolids -->


    <owl:NamedIndividual rdf:about="https://saref.etsi.org/saref4watr/TotalDissolvedSolids">
        <rdf:type rdf:resource="https://saref.etsi.org/saref4watr/AcceptabilityProperty"/>
        <rdfs:comment xml:lang="en">Property of the water indicating the dissolved combined content of all inorganic and organic substances present in a sample of water.</rdfs:comment>
        <rdfs:label xml:lang="en">Total dissolved solids</rdfs:label>
    </owl:NamedIndividual>
    


    <!-- https://saref.etsi.org/saref4watr/TotalIndicativeDose -->


    <owl:NamedIndividual rdf:about="https://saref.etsi.org/saref4watr/TotalIndicativeDose">
        <rdf:type rdf:resource="https://saref.etsi.org/saref4watr/AcceptabilityProperty"/>
        <rdfs:comment xml:lang="en">Property of the water indicating its total indicative dose.</rdfs:comment>
        <rdfs:label xml:lang="en">Total indicative dose</rdfs:label>
    </owl:NamedIndividual>
    


    <!-- https://saref.etsi.org/saref4watr/TotalOrganicCarbon -->


    <owl:NamedIndividual rdf:about="https://saref.etsi.org/saref4watr/TotalOrganicCarbon">
        <rdf:type rdf:resource="https://saref.etsi.org/saref4watr/ChemicalProperty"/>
        <rdfs:comment xml:lang="en">Property of the water indicating its concentration of total organic carbon.</rdfs:comment>
        <rdfs:label xml:lang="en">TOC</rdfs:label>
        <rdfs:label xml:lang="en">Total organic carbon</rdfs:label>
    </owl:NamedIndividual>
    


    <!-- https://saref.etsi.org/saref4watr/TotalSuspendedSolids -->


    <owl:NamedIndividual rdf:about="https://saref.etsi.org/saref4watr/TotalSuspendedSolids">
        <rdf:type rdf:resource="https://saref.etsi.org/saref4watr/AcceptabilityProperty"/>
        <rdfs:comment xml:lang="en">Property of the water indicating the dry-weight of suspended particles, that are not dissolved, in a sample of water.</rdfs:comment>
        <rdfs:label xml:lang="en">Total suspended solids</rdfs:label>
    </owl:NamedIndividual>
    


    <!-- https://saref.etsi.org/saref4watr/Trichloroethene -->


    <owl:NamedIndividual rdf:about="https://saref.etsi.org/saref4watr/Trichloroethene">
        <rdf:type rdf:resource="https://saref.etsi.org/saref4watr/ChemicalProperty"/>
        <rdfs:comment xml:lang="en">Property of the water indicating its concentration of trichloroethene.</rdfs:comment>
        <rdfs:label xml:lang="en">Trichloroethene</rdfs:label>
    </owl:NamedIndividual>
    


    <!-- https://saref.etsi.org/saref4watr/Trihalomethanes -->


    <owl:NamedIndividual rdf:about="https://saref.etsi.org/saref4watr/Trihalomethanes">
        <rdf:type rdf:resource="https://saref.etsi.org/saref4watr/ChemicalProperty"/>
        <rdfs:comment xml:lang="en">Property of the water indicating its concentration of trihalomethanes.</rdfs:comment>
        <rdfs:label xml:lang="en">Trihalomethanes</rdfs:label>
    </owl:NamedIndividual>
    


    <!-- https://saref.etsi.org/saref4watr/Tritium -->


    <owl:NamedIndividual rdf:about="https://saref.etsi.org/saref4watr/Tritium">
        <rdf:type rdf:resource="https://saref.etsi.org/saref4watr/ChemicalProperty"/>
        <rdfs:comment xml:lang="en">Property of the water indicating its concentration of tritium.</rdfs:comment>
        <rdfs:label xml:lang="en">Tritium</rdfs:label>
    </owl:NamedIndividual>
    


    <!-- https://saref.etsi.org/saref4watr/Turbidity -->


    <owl:NamedIndividual rdf:about="https://saref.etsi.org/saref4watr/Turbidity">
        <rdf:type rdf:resource="https://saref.etsi.org/saref4watr/AcceptabilityProperty"/>
        <rdfs:comment xml:lang="en">Property of the water indicating its turbidity.</rdfs:comment>
        <rdfs:label xml:lang="en">Turbidity</rdfs:label>
    </owl:NamedIndividual>
    


    <!-- https://saref.etsi.org/saref4watr/VinylChloride -->


    <owl:NamedIndividual rdf:about="https://saref.etsi.org/saref4watr/VinylChloride">
        <rdf:type rdf:resource="https://saref.etsi.org/saref4watr/ChemicalProperty"/>
        <rdfs:comment xml:lang="en">Property of the water indicating its concentration of vinyl chloride.</rdfs:comment>
        <rdfs:label xml:lang="en">Vinyl chloride</rdfs:label>
    </owl:NamedIndividual>
    


    <!-- https://saref.etsi.org/saref4watr/Wastewater -->


    <owl:NamedIndividual rdf:about="https://saref.etsi.org/saref4watr/Wastewater">
        <rdf:type rdf:resource="https://saref.etsi.org/saref4watr/Water"/>
        <rdfs:comment xml:lang="en">Wastewater is water that has been used in the home, in a business, or as part of an industrial process.</rdfs:comment>
        <rdfs:label xml:lang="en">Waste water</rdfs:label>
    </owl:NamedIndividual>
    


    <!-- https://saref.etsi.org/saref4watr/12Dichloroethane -->


    <owl:NamedIndividual rdf:about="https://saref.etsi.org/saref4watr/12Dichloroethane">
        <rdf:type rdf:resource="https://saref.etsi.org/saref4watr/ChemicalProperty"/>
        <rdfs:comment xml:lang="en">Property of the water indicating its concentration of 1,2-dichloroethane.</rdfs:comment>
        <rdfs:label xml:lang="en">1,2-dichloroethane</rdfs:label>
    </owl:NamedIndividual>
    <rdf:Description>
        <foaf:PersonalProfileDocument rdf:resource="https://www.linkedin.com/in/tatianatarasova"/>
    </rdf:Description>
    <rdf:Description rdf:nodeID="genid540">
        <foaf:homepage rdf:resource="http://www.smartopendata.eu"/>
        <foaf:name>SmartOpenData project</foaf:name>
    </rdf:Description>
    <rdf:Description rdf:nodeID="genid541">
        <schema:affiliation>KU Leuven</schema:affiliation>
        <schema:affiliation>Neanex Technologies</schema:affiliation>
        <schema:email rdf:datatype="http://www.w3.org/2001/XMLSchema#anyURI">mathias.bonduel@neanex.com</schema:email>
        <schema:name>Mathias Bonduel</schema:name>
        <schema:url rdf:datatype="http://www.w3.org/2001/XMLSchema#anyURI">https://orcid.org/0000-0002-3313-924X</schema:url>
    </rdf:Description>
    <rdf:Description rdf:nodeID="genid542">
        <schema:affiliation>Oracle Corporation</schema:affiliation>
        <schema:email rdf:datatype="http://www.w3.org/2001/XMLSchema#anyURI">john.herring@oracle.com</schema:email>
        <schema:name>John Herring</schema:name>
    </rdf:Description>
    <rdf:Description rdf:nodeID="genid543">
        <schema:affiliation>Mainz University Of Applied Sciences</schema:affiliation>
        <schema:email rdf:datatype="http://www.w3.org/2001/XMLSchema#anyURI">timo.homburg@hs-mainz.de</schema:email>
        <schema:name>Timo Homburg</schema:name>
        <schema:url rdf:datatype="http://www.w3.org/2001/XMLSchema#anyURI">https://orcid.org/0000-0002-9499-5840</schema:url>
    </rdf:Description>
    <rdf:Description rdf:nodeID="genid544">
        <schema:affiliation>Oracle Corporation</schema:affiliation>
        <schema:email rdf:datatype="http://www.w3.org/2001/XMLSchema#anyURI">matthew.perry@oracle.com</schema:email>
        <schema:name>Matthew Perry</schema:name>
        <schema:url rdf:datatype="http://www.w3.org/2001/XMLSchema#anyURI">https://orcid.org/0000-0003-1988-462X</schema:url>
    </rdf:Description>
    <rdf:Description rdf:nodeID="genid545">
        <schema:email rdf:datatype="http://www.w3.org/2001/XMLSchema#anyURI">fjknibbe@gmail.com</schema:email>
        <schema:name>Frans Knibbe</schema:name>
        <schema:url rdf:datatype="http://www.w3.org/2001/XMLSchema#anyURI">https://orcid.org/0000-0003-3789-2260</schema:url>
    </rdf:Description>
    <rdf:Description rdf:nodeID="genid546">
        <schema:affiliation>CSIRO Australia</schema:affiliation>
        <schema:email rdf:datatype="http://www.w3.org/2001/XMLSchema#anyURI">simon.cox@csiro.au</schema:email>
        <schema:name>Simon J D Cox</schema:name>
        <schema:url rdf:datatype="http://www.w3.org/2001/XMLSchema#anyURI">https://orcid.org/0000-0002-3884-3420</schema:url>
    </rdf:Description>
    <rdf:Description rdf:nodeID="genid547">
        <schema:affiliation>Geoscape Australia</schema:affiliation>
        <schema:email rdf:datatype="http://www.w3.org/2001/XMLSchema#anyURI">joseph.abhayaratna@geoscape.com.au</schema:email>
        <schema:name>Joseph Abhayaratna</schema:name>
        <schema:url rdf:datatype="http://www.w3.org/2001/XMLSchema#anyURI">https://orcid.org/0000-0001-5075-6234</schema:url>
    </rdf:Description>
    <rdf:Description rdf:nodeID="genid548">
        <schema:name>Open Geospatial Consortium</schema:name>
        <schema:url rdf:datatype="http://www.w3.org/2001/XMLSchema#anyURI">https://www.ogc.org</schema:url>
    </rdf:Description>
    <rdf:Description rdf:nodeID="genid549">
        <schema:affiliation>Australian National University</schema:affiliation>
        <schema:affiliation>SURROUND Australia Pty Ltd</schema:affiliation>
        <schema:email rdf:datatype="http://www.w3.org/2001/XMLSchema#anyURI">nicholas.car@surroundaustralia.com</schema:email>
        <schema:name>Nicholas J. Car</schema:name>
        <schema:url rdf:datatype="http://www.w3.org/2001/XMLSchema#anyURI">https://orcid.org/0000-0002-8742-7730</schema:url>
    </rdf:Description>
    <rdf:Description>
        <xsd:pattern>--(0[1-9]|1[0-9]|20)(Z|(\+|-)((0[0-9]|1[0-3]):[0-5][0-9]|14:00))?</xsd:pattern>
    </rdf:Description>
    <rdf:Description>
        <xsd:pattern>-?([1-9][0-9]{3,}|0[0-9]{3})(Z|(\+|-)((0[0-9]|1[0-3]):[0-5][0-9]|14:00))?</xsd:pattern>
    </rdf:Description>
    <rdf:Description>
        <xsd:pattern>---(0[1-9]|[1-9][0-9])(Z|(\+|-)((0[0-9]|1[0-3]):[0-5][0-9]|14:00))?</xsd:pattern>
    </rdf:Description>
    


    <!-- 
    ///////////////////////////////////////////////////////////////////////////////////////
    //
    // Annotations
    //
    ///////////////////////////////////////////////////////////////////////////////////////
     -->


    <rdf:Description rdf:about="http://www.w3.org/2003/01/geo/wgs84_pos#">
        <dc:date>$Date: 2009/04/20 15:00:30 $</dc:date>
        <dc:description>A vocabulary for representing latitude, longitude and 
 altitude information in the WGS84 geodetic reference datum. 
 Version $Id: wgs84_pos.rdf,v 1.22 2009/04/20 15:00:30 timbl Exp $. See http://www.w3.org/2003/01/geo/ for more details.</dc:description>
        <dc:title>WGS84 Geo Positioning: an RDF vocabulary</dc:title>
        <rdfs:comment>
Recent changes to this namespace:
$Log: wgs84_pos.rdf,v $
Revision 1.22  2009/04/20 15:00:30  timbl
Remove the time bits which have been deal with elsewhere eg in iCal.

Revision 1.21  2009/04/20 12:52:47  timbl
try again

Revision 1.20  2009/04/20 12:42:11  timbl
Add Event (edited ages ago and never checked in), and location (following discussion http://chatlogs.planetrdf.com/swig/2009-04-20#T12-36-09)

Revision 1.19  2009/04/20 12:36:31  timbl
Add Event (edited ages ago and never checked in), and location (following discussion http://chatlogs.planetrdf.com/swig/2009-04-20#T12-36-09)

Revision 1.18  2006/02/01 22:01:04  danbri
Clarified that lat and long are decimal degrees, and that alt is decimal metres about local reference ellipsoid

Revision 1.17  2004/02/06 17:38:12  danbri
Fixed a bad commit screwup

Revision 1.15  2003/04/19 11:24:08  danbri
Fixed the typo even more.

Revision 1.14  2003/04/19 11:16:56  danbri
fixed a typo

Revision 1.13  2003/02/19 22:27:27  connolly
relaxed domain constraints on lat/long/alt from Point to SpatialThing

Revision 1.12  2003/01/12 01:41:41  danbri
Trying local copy of XSLT doc.

Revision 1.11  2003/01/12 01:20:18  danbri
added a link to morten&apos;s xslt rdfs viewer.

Revision 1.10  2003/01/11 18:56:49  danbri
Removed datatype range from lat and long properties, since they would
have required each occurance of the property to mention the datatype.

Revision 1.9  2003/01/11 11:41:31  danbri
Another typo; repaired rdfs:Property to rdf:Property x4

Revision 1.8  2003/01/11 11:05:02  danbri
Added an rdfs:range for each lat/long/alt property,
http://www.w3.org/2001/XMLSchema#float

Revision 1.7  2003/01/10 20:25:16  danbri
Longer rdfs:comment for Point, trying to be Earth-centric and neutral about
coordinate system(s) at the same time. Feedback welcomed.

Revision 1.6  2003/01/10 20:18:30  danbri
Added CVS log comments into the RDF/XML as an rdfs:comment property of the
vocabulary. Note that this is not common practice (but seems both harmless
and potentially useful).


revision 1.5
date: 2003/01/10 20:14:31;  author: danbri;  state: Exp;  lines: +16 -5
Updated schema:
Added a dc:date, added url for more info. Changed the rdfs:label of the
namespace from gp to geo. Added a class Point, set as the rdfs:domain of
each property. Added XML comment on the lat_long property suggesting that
we might not need it (based on #rdfig commentary from implementors).

revision 1.4
date: 2003/01/10 20:01:07;  author: danbri;  state: Exp;  lines: +6 -5
Fixed typo; several rdfs:about attributes are now rdf:about. Thanks to MortenF in
#rdfig for catching this error.

revision 1.3
date: 2003/01/10 11:59:03;  author: danbri;  state: Exp;  lines: +4 -3
fixed buglet in vocab, added more wgs links

revision 1.2
date: 2003/01/10 11:01:11;  author: danbri;  state: Exp;  lines: +4 -4
Removed alt from the as-a-flat-string property, and switched from
space separated to comma separated.

revision 1.1
date: 2003/01/10 10:53:23;  author: danbri;  state: Exp;
basic geo vocab

</rdfs:comment>
        <rdfs:label>geo</rdfs:label>
    </rdf:Description>
    <rdf:Description rdf:about="http://www.w3.org/2003/01/geo/wgs84_pos#alt">
        <rdfs:comment xml:lang="en">The WGS84 altitude of a SpatialThing (decimal meters above the local reference ellipsoid).</rdfs:comment>
        <rdfs:comment>The WGS84 altitude of a SpatialThing (decimal meters 
above the local reference ellipsoid).</rdfs:comment>
        <rdfs:label xml:lang="en">altitude</rdfs:label>
        <rdfs:label>altitude</rdfs:label>
    </rdf:Description>
    <rdf:Description rdf:about="http://www.w3.org/2003/01/geo/wgs84_pos#lat">
        <rdfs:comment xml:lang="en">The WGS84 latitude of a SpatialThing (decimal degrees).</rdfs:comment>
        <rdfs:comment>The WGS84 latitude of a SpatialThing (decimal degrees).</rdfs:comment>
        <rdfs:label xml:lang="en">latitude</rdfs:label>
        <rdfs:label>latitude</rdfs:label>
    </rdf:Description>
    <rdf:Description rdf:about="http://www.w3.org/2003/01/geo/wgs84_pos#lat_long">
        <rdfs:comment>A comma-separated representation of a latitude, longitude coordinate.</rdfs:comment>
        <rdfs:label>lat/long</rdfs:label>
    </rdf:Description>
    <rdf:Description rdf:about="http://www.w3.org/2003/01/geo/wgs84_pos#location">
        <rdfs:comment xml:lang="en">The relation between something and the point, 
 or other geometrical thing in space, where it is.  For example, the realtionship between
 a radio tower and a Point with a given lat and long.
 Or a relationship between a park and its outline as a closed arc of points, or a road and
 its location as a arc (a sequence of points).
 Clearly in practice there will be limit to the accuracy of any such statement, but one would expect
 an accuracy appropriate for the size of the object and uses such as mapping .
 </rdfs:comment>
        <rdfs:comment xml:lang="en">The relation between something and the point,  or other geometrical thing in space, where it is.  For example, the realtionship between a radio tower and a Point with a given lat and long. Or a relationship between a park and its outline as a closed arc of points, or a road and its location as a arc (a sequence of points). Clearly in practice there will be limit to the accuracy of any such statement, but one would expect an accuracy appropriate for the size of the object and uses such as mapping .</rdfs:comment>
        <rdfs:comment>The relation between something and the point, 
 or other geometrical thing in space, where it is.  For example, the realtionship between
 a radio tower and a Point with a given lat and long.
 Or a relationship between a park and its outline as a closed arc of points, or a road and
 its location as a arc (a sequence of points).
 Clearly in practice there will be limit to the accuracy of any such statement, but one would expect
 an accuracy appropriate for the size of the object and uses such as mapping .
 </rdfs:comment>
        <rdfs:isDefinedBy rdf:resource="http://www.w3.org/2003/01/geo/wgs84_pos#"/>
        <rdfs:label xml:lang="en">location</rdfs:label>
        <rdfs:label>location</rdfs:label>
    </rdf:Description>
    <rdf:Description rdf:about="http://www.w3.org/2003/01/geo/wgs84_pos#long">
        <rdfs:comment xml:lang="en">The WGS84 longitude of a SpatialThing (decimal degrees).</rdfs:comment>
        <rdfs:comment>The WGS84 longitude of a SpatialThing (decimal degrees).</rdfs:comment>
        <rdfs:label xml:lang="en">longitude</rdfs:label>
        <rdfs:label>longitude</rdfs:label>
    </rdf:Description>
</rdf:RDF>



<!-- Generated by the OWL API (version 5.1.18) https://github.com/owlcs/owlapi/ -->


